<?xml version="1.0"?>
<rdf:RDF xmlns="http://cpe.mitre.org/cpe#"
     xml:base="http://cpe.mitre.org/cpe"
     xmlns:rdf="http://www.w3.org/1999/02/22-rdf-syntax-ns#"
     xmlns:owl="http://www.w3.org/2002/07/owl#"
     xmlns:xml="http://www.w3.org/XML/1998/namespace"
     xmlns:xsd="http://www.w3.org/2001/XMLSchema#"
     xmlns:cpe="http://cpe.mitre.org/cpe#"
     xmlns:wgs84_pos="http://www.w3.org/2003/01/geo/wgs84_pos#"
     xmlns:rdfs="http://www.w3.org/2000/01/rdf-schema#"
     xmlns:foaf="http://xmlns.com/foaf/0.1/"
     xmlns:dc="http://purl.org/dc/elements/1.1/">
    <owl:Ontology rdf:about="http://cpe.mitre.org/cpe">
        <owl:imports rdf:resource="http://cybox.mitre.org/objects/System"/>
        <owl:imports rdf:resource="http://cybox.mitre.org/objects/Product"/>
        <owl:imports rdf:resource="http://scap.nist.gov/scap_core"/>
        <owl:imports rdf:resource="http://cybox.mitre.org/cyboxCommon"/>
        <owl:imports rdf:resource="http://cybox.mitre.org/objects/Device"/>
        <owl:versionInfo rdf:datatype="http://www.w3.org/2001/XMLSchema#string">2.3-000</owl:versionInfo>
        <rdfs:label>Common Platform Enumeration (CPE) Ontology</rdfs:label>
        <rdfs:comment>Ontology that provides a vocabulary and representation for the Common Platform Enumeration (CPE) which provides a standardized method of describing and identifying classes of applications, operating systems, and hardware devices present among an enterprise&apos;s computing assets.

The ontology is based on the Common Platform Enumeration schema maintained by NIST copyright 2011-2014.  The version number of the ontology is kept in sync with the schema in order to more easily relate between the ontology and the corresponding schema version.

Copyright (c) 2014, DaedaFusion, LLC.  All rights reserved.</rdfs:comment>
    </owl:Ontology>
    


    <!-- 
    ///////////////////////////////////////////////////////////////////////////////////////
    //
    // Object Properties
    //
    ///////////////////////////////////////////////////////////////////////////////////////
     -->

    


    <!-- http://cpe.mitre.org/cpe#alternateCPE -->

    <owl:ObjectProperty rdf:about="http://cpe.mitre.org/cpe#alternateCPE">
        <rdfs:range rdf:resource="http://cpe.mitre.org/cpe#CPE"/>
        <rdfs:comment>Specifies an alternate CPE that refers to the same platform but in a different format</rdfs:comment>
        <rdfs:label>Alternate CPE</rdfs:label>
    </owl:ObjectProperty>
    


    <!-- http://cpe.mitre.org/cpe#authorities -->

    <owl:ObjectProperty rdf:about="http://cpe.mitre.org/cpe#authorities">
        <rdfs:range rdf:resource="http://www.oasis-open.org/ciq_xpil#Organization"/>
        <rdfs:comment>Specifies one or more authorities responsible  for endorsing the identifier name.   Multiple authorities may endorse the  same identifier name.</rdfs:comment>
        <rdfs:label>Authorities</rdfs:label>
    </owl:ObjectProperty>
    


    <!-- http://cpe.mitre.org/cpe#changes -->

    <owl:ObjectProperty rdf:about="http://cpe.mitre.org/cpe#changes">
        <rdfs:range rdf:resource="http://cpe.mitre.org/cpe#ChangeDescription"/>
        <rdfs:comment>Specifies one or more descriptions of any changes made to  the identifier name or associated metadata.</rdfs:comment>
        <rdfs:label>Changes</rdfs:label>
    </owl:ObjectProperty>
    


    <!-- http://cpe.mitre.org/cpe#checkFactRef -->

    <owl:ObjectProperty rdf:about="http://cpe.mitre.org/cpe#checkFactRef">
        <rdfs:comment>Specifies zero or more references to a check that evaluates to TRUE, FALSE, or ERROR. Examples of types of checks are OVAL and OCIL checks.</rdfs:comment>
        <rdfs:label>Check Fact Reference</rdfs:label>
    </owl:ObjectProperty>
    


    <!-- http://cpe.mitre.org/cpe#checks -->

    <owl:ObjectProperty rdf:about="http://cpe.mitre.org/cpe#checks">
        <rdfs:range rdf:resource="http://cpe.mitre.org/cpe#CheckInfo"/>
        <rdfs:comment>Specifies zero or more checks, such as an OVAL definition, that can confirm or reject an IT system as an instance of the named platform</rdfs:comment>
        <rdfs:label>Checks</rdfs:label>
    </owl:ObjectProperty>
    


    <!-- http://cpe.mitre.org/cpe#contents -->

    <owl:ObjectProperty rdf:about="http://cpe.mitre.org/cpe#contents">
        <rdfs:range rdf:resource="http://cpe.mitre.org/cpe#CPE"/>
        <rdfs:comment>Specifies the CPE Name entries contained within the Platform Catalog.</rdfs:comment>
        <rdfs:label>Contents</rdfs:label>
    </owl:ObjectProperty>
    


    <!-- http://cpe.mitre.org/cpe#deprecatedBy -->

    <owl:ObjectProperty rdf:about="http://cpe.mitre.org/cpe#deprecatedBy">
        <rdfs:range rdf:resource="http://cpe.mitre.org/cpe#CPE"/>
        <rdfs:comment>Specifies one or more CPE names that deprecated the identifier name.</rdfs:comment>
        <rdfs:label>Deprecated By</rdfs:label>
    </owl:ObjectProperty>
    


    <!-- http://cpe.mitre.org/cpe#deprecationInfo -->

    <owl:ObjectProperty rdf:about="http://cpe.mitre.org/cpe#deprecationInfo">
        <rdfs:range rdf:resource="http://cpe.mitre.org/cpe#DeprecationInfo"/>
        <rdfs:comment>Specifies one or more deprecation entries for the given identifier name. It is possible for a single identifier name to have multiple deprecations that occur at different time periods.</rdfs:comment>
        <rdfs:label>Deprecation Information:</rdfs:label>
    </owl:ObjectProperty>
    


    <!-- http://cpe.mitre.org/cpe#factRef -->

    <owl:ObjectProperty rdf:about="http://cpe.mitre.org/cpe#factRef">
        <rdfs:range rdf:resource="http://cpe.mitre.org/cpe#CPE"/>
        <rdfs:comment>Specifies possible sets of product via CPE Names</rdfs:comment>
        <rdfs:label>Fact Reference</rdfs:label>
    </owl:ObjectProperty>
    


    <!-- http://cpe.mitre.org/cpe#generator -->

    <owl:ObjectProperty rdf:about="http://cpe.mitre.org/cpe#generator">
        <rdfs:range rdf:resource="http://cybox.mitre.org/cyboxCommon#ToolInformation"/>
        <rdfs:comment>Specifies information about the tool used to generate a specific CPE Dictionary</rdfs:comment>
        <rdfs:label>Generator</rdfs:label>
    </owl:ObjectProperty>
    


    <!-- http://cpe.mitre.org/cpe#logicalTest -->

    <owl:ObjectProperty rdf:about="http://cpe.mitre.org/cpe#logicalTest">
        <rdfs:range rdf:resource="http://cpe.mitre.org/cpe#LogicalTest"/>
        <rdfs:comment>Specifies logical tests to form a complex logical test using AND, OR, and/or negate operators.  This result of evaluating the nested logical test will result in TRUE, FALSE, or ERROR.</rdfs:comment>
        <rdfs:label>Logical Test</rdfs:label>
    </owl:ObjectProperty>
    


    <!-- http://cpe.mitre.org/cpe#references -->

    <owl:ObjectProperty rdf:about="http://cpe.mitre.org/cpe#references">
        <rdfs:range rdf:resource="http://cpe.mitre.org/cpe#ReferenceInfo"/>
        <rdfs:comment>Specifies zero of more external references to additional descriptive material</rdfs:comment>
        <rdfs:label>References</rdfs:label>
    </owl:ObjectProperty>
    


    <!-- http://cpe.mitre.org/cpe#relatedDevice -->

    <owl:ObjectProperty rdf:about="http://cpe.mitre.org/cpe#relatedDevice">
        <rdfs:range rdf:resource="http://cybox.mitre.org/objects/Device#Device"/>
        <rdfs:comment>Specifies a reference to the associated device to which the CPE names refers</rdfs:comment>
        <rdfs:label>Related Device</rdfs:label>
    </owl:ObjectProperty>
    


    <!-- http://cpe.mitre.org/cpe#relatedOperatingSystem -->

    <owl:ObjectProperty rdf:about="http://cpe.mitre.org/cpe#relatedOperatingSystem">
        <rdfs:range rdf:resource="http://cybox.mitre.org/objects/System#OperatingSystemInfo"/>
        <rdfs:comment>Specifies a reference to the associated operating system to which the CPE names refers</rdfs:comment>
        <rdfs:label>Related Operating System</rdfs:label>
    </owl:ObjectProperty>
    


    <!-- http://cpe.mitre.org/cpe#relatedProduct -->

    <owl:ObjectProperty rdf:about="http://cpe.mitre.org/cpe#relatedProduct">
        <rdfs:range rdf:resource="http://cybox.mitre.org/objects/Product#Product"/>
        <rdfs:comment>Specifies a reference to the associated product to which the CPE names refers</rdfs:comment>
        <rdfs:label>Related Product</rdfs:label>
    </owl:ObjectProperty>
    


    <!-- http://cpe.mitre.org/cpe#submitter -->

    <owl:ObjectProperty rdf:about="http://cpe.mitre.org/cpe#submitter">
        <rdfs:range rdf:resource="http://www.oasis-open.org/ciq_xpil#Organization"/>
        <rdfs:comment>Specifies the  organization responsible for submitting the identifier name.</rdfs:comment>
        <rdfs:label>Submitting Organization</rdfs:label>
    </owl:ObjectProperty>
    


    <!-- http://cpe.mitre.org/cpe#vendor -->

    <owl:ObjectProperty rdf:about="http://cpe.mitre.org/cpe#vendor">
        <rdfs:range rdf:resource="http://www.oasis-open.org/ciq_xpil#Organization"/>
        <rdfs:comment>Specifies the identity of the person or organization that manufactured or created the product</rdfs:comment>
        <rdfs:label>Vendor</rdfs:label>
    </owl:ObjectProperty>
    


    <!-- http://scap.nist.gov/scap_core#generator -->

    <owl:ObjectProperty rdf:about="http://scap.nist.gov/scap_core#generator">
        <rdfs:range rdf:resource="http://cybox.mitre.org/cyboxCommon#ToolInformation"/>
    </owl:ObjectProperty>
    


    <!-- 
    ///////////////////////////////////////////////////////////////////////////////////////
    //
    // Data properties
    //
    ///////////////////////////////////////////////////////////////////////////////////////
     -->

    


    <!-- http://cpe.mitre.org/cpe#changeDate -->

    <owl:DatatypeProperty rdf:about="http://cpe.mitre.org/cpe#changeDate">
        <rdfs:range rdf:resource="http://www.w3.org/2001/XMLSchema#dateTime"/>
        <rdfs:comment>Specifies the date and time when the change occurred.</rdfs:comment>
        <rdfs:label>Date of Change</rdfs:label>
    </owl:DatatypeProperty>
    


    <!-- http://cpe.mitre.org/cpe#changeType -->

    <owl:DatatypeProperty rdf:about="http://cpe.mitre.org/cpe#changeType">
        <rdfs:range>
            <rdfs:Datatype>
                <owl:oneOf>
                    <rdf:Description>
                        <rdf:type rdf:resource="http://www.w3.org/1999/02/22-rdf-syntax-ns#List"/>
                        <rdf:first rdf:datatype="http://www.w3.org/2001/XMLSchema#string">AUTHORITY_CHANGE</rdf:first>
                        <rdf:rest>
                            <rdf:Description>
                                <rdf:type rdf:resource="http://www.w3.org/1999/02/22-rdf-syntax-ns#List"/>
                                <rdf:first rdf:datatype="http://www.w3.org/2001/XMLSchema#string">DEPRECATION</rdf:first>
                                <rdf:rest>
                                    <rdf:Description>
                                        <rdf:type rdf:resource="http://www.w3.org/1999/02/22-rdf-syntax-ns#List"/>
                                        <rdf:first rdf:datatype="http://www.w3.org/2001/XMLSchema#string">DEPRECATION_MODIFICATION</rdf:first>
                                        <rdf:rest>
                                            <rdf:Description>
                                                <rdf:type rdf:resource="http://www.w3.org/1999/02/22-rdf-syntax-ns#List"/>
                                                <rdf:first rdf:datatype="http://www.w3.org/2001/XMLSchema#string">ORIGINAL_RECORD</rdf:first>
                                                <rdf:rest rdf:resource="http://www.w3.org/1999/02/22-rdf-syntax-ns#nil"/>
                                            </rdf:Description>
                                        </rdf:rest>
                                    </rdf:Description>
                                </rdf:rest>
                            </rdf:Description>
                        </rdf:rest>
                    </rdf:Description>
                </owl:oneOf>
            </rdfs:Datatype>
        </rdfs:range>
        <rdfs:comment>Specifies the type of change that occurred.</rdfs:comment>
        <rdfs:label>Change Type</rdfs:label>
    </owl:DatatypeProperty>
    


    <!-- http://cpe.mitre.org/cpe#checkSystem -->

    <owl:DatatypeProperty rdf:about="http://cpe.mitre.org/cpe#checkSystem">
        <rdfs:range rdf:resource="http://www.w3.org/2001/XMLSchema#anyURI"/>
        <rdfs:comment>Specifies the URI for a particular version of OVAL or a related system testing language</rdfs:comment>
        <rdfs:label>Check System URI</rdfs:label>
    </owl:DatatypeProperty>
    


    <!-- http://cpe.mitre.org/cpe#comments -->

    <owl:DatatypeProperty rdf:about="http://cpe.mitre.org/cpe#comments">
        <rdfs:range rdf:resource="http://www.w3.org/2001/XMLSchema#string"/>
        <rdfs:comment>Specifies comments explaining the rationale for the  change.</rdfs:comment>
        <rdfs:label>Comments</rdfs:label>
    </owl:DatatypeProperty>
    


    <!-- http://cpe.mitre.org/cpe#cpeName -->

    <owl:DatatypeProperty rdf:about="http://cpe.mitre.org/cpe#cpeName">
        <rdfs:range rdf:resource="http://www.w3.org/2001/XMLSchema#string"/>
        <rdfs:comment>Specifies the name of the Common Platform Enumeration item.</rdfs:comment>
        <rdfs:label>CPE Name</rdfs:label>
    </owl:DatatypeProperty>
    


    <!-- http://cpe.mitre.org/cpe#deprecated -->

    <owl:DatatypeProperty rdf:about="http://cpe.mitre.org/cpe#deprecated">
        <rdfs:range rdf:resource="http://www.w3.org/2001/XMLSchema#boolean"/>
        <rdfs:comment>Specifies whether the CPE has been deprecated</rdfs:comment>
        <rdfs:label>Deprecated</rdfs:label>
    </owl:DatatypeProperty>
    


    <!-- http://cpe.mitre.org/cpe#deprecationDate -->

    <owl:DatatypeProperty rdf:about="http://cpe.mitre.org/cpe#deprecationDate">
        <rdfs:range rdf:resource="http://www.w3.org/2001/XMLSchema#dateTime"/>
        <rdfs:comment>Specified the date and time when the deprecation occurred.</rdfs:comment>
        <rdfs:label>Date of Deprecation</rdfs:label>
    </owl:DatatypeProperty>
    


    <!-- http://cpe.mitre.org/cpe#deprecationType -->

    <owl:DatatypeProperty rdf:about="http://cpe.mitre.org/cpe#deprecationType">
        <rdfs:range>
            <rdfs:Datatype>
                <owl:oneOf>
                    <rdf:Description>
                        <rdf:type rdf:resource="http://www.w3.org/1999/02/22-rdf-syntax-ns#List"/>
                        <rdf:first rdf:datatype="http://www.w3.org/2001/XMLSchema#string">ADDITIONAL_INFORMATION</rdf:first>
                        <rdf:rest>
                            <rdf:Description>
                                <rdf:type rdf:resource="http://www.w3.org/1999/02/22-rdf-syntax-ns#List"/>
                                <rdf:first rdf:datatype="http://www.w3.org/2001/XMLSchema#string">NAME_CORRECTION</rdf:first>
                                <rdf:rest>
                                    <rdf:Description>
                                        <rdf:type rdf:resource="http://www.w3.org/1999/02/22-rdf-syntax-ns#List"/>
                                        <rdf:first rdf:datatype="http://www.w3.org/2001/XMLSchema#string">NAME_REMOVAL</rdf:first>
                                        <rdf:rest>
                                            <rdf:Description>
                                                <rdf:type rdf:resource="http://www.w3.org/1999/02/22-rdf-syntax-ns#List"/>
                                                <rdf:first rdf:datatype="http://www.w3.org/2001/XMLSchema#string">UNSPECIFIED</rdf:first>
                                                <rdf:rest rdf:resource="http://www.w3.org/1999/02/22-rdf-syntax-ns#nil"/>
                                            </rdf:Description>
                                        </rdf:rest>
                                    </rdf:Description>
                                </rdf:rest>
                            </rdf:Description>
                        </rdf:rest>
                    </rdf:Description>
                </owl:oneOf>
            </rdfs:Datatype>
        </rdfs:range>
        <rdfs:comment>Specifies the type of the deprecation.</rdfs:comment>
        <rdfs:label>Type of Deprecation</rdfs:label>
    </owl:DatatypeProperty>
    


    <!-- http://cpe.mitre.org/cpe#description -->

    <owl:DatatypeProperty rdf:about="http://cpe.mitre.org/cpe#description">
        <rdfs:range rdf:resource="http://www.w3.org/2001/XMLSchema#string"/>
        <rdfs:comment>Specifies a description of an entity</rdfs:comment>
        <rdfs:isDefinedBy rdf:resource="http://cpe.mitre.org/cpe"/>
        <rdfs:label>Description</rdfs:label>
    </owl:DatatypeProperty>
    


    <!-- http://cpe.mitre.org/cpe#edition -->

    <owl:DatatypeProperty rdf:about="http://cpe.mitre.org/cpe#edition">
        <rdfs:range rdf:resource="http://www.w3.org/2001/XMLSchema#string"/>
        <rdfs:comment>Specifies edition-related terms applied by the vendor to the product</rdfs:comment>
        <rdfs:label>Edition</rdfs:label>
    </owl:DatatypeProperty>
    


    <!-- http://cpe.mitre.org/cpe#evidenceExternalLink -->

    <owl:DatatypeProperty rdf:about="http://cpe.mitre.org/cpe#evidenceExternalLink">
        <rdfs:range rdf:resource="http://www.w3.org/2001/XMLSchema#anyURI"/>
        <rdfs:comment>Specifies an external link to a specific piece of evidence</rdfs:comment>
        <rdfs:label>External Link to Evidence</rdfs:label>
    </owl:DatatypeProperty>
    


    <!-- http://cpe.mitre.org/cpe#evidenceType -->

    <owl:DatatypeProperty rdf:about="http://cpe.mitre.org/cpe#evidenceType">
        <rdfs:range>
            <rdfs:Datatype>
                <owl:oneOf>
                    <rdf:Description>
                        <rdf:type rdf:resource="http://www.w3.org/1999/02/22-rdf-syntax-ns#List"/>
                        <rdf:first rdf:datatype="http://www.w3.org/2001/XMLSchema#string">CURATOR_UPDATE</rdf:first>
                        <rdf:rest>
                            <rdf:Description>
                                <rdf:type rdf:resource="http://www.w3.org/1999/02/22-rdf-syntax-ns#List"/>
                                <rdf:first rdf:datatype="http://www.w3.org/2001/XMLSchema#string">THIRD_PARTY_FIX</rdf:first>
                                <rdf:rest>
                                    <rdf:Description>
                                        <rdf:type rdf:resource="http://www.w3.org/1999/02/22-rdf-syntax-ns#List"/>
                                        <rdf:first rdf:datatype="http://www.w3.org/2001/XMLSchema#string">VENDOR_FIX</rdf:first>
                                        <rdf:rest rdf:resource="http://www.w3.org/1999/02/22-rdf-syntax-ns#nil"/>
                                    </rdf:Description>
                                </rdf:rest>
                            </rdf:Description>
                        </rdf:rest>
                    </rdf:Description>
                </owl:oneOf>
            </rdfs:Datatype>
        </rdfs:range>
        <rdfs:comment>Specifies the type of evidence</rdfs:comment>
        <rdfs:label>Evidence Type</rdfs:label>
    </owl:DatatypeProperty>
    


    <!-- http://cpe.mitre.org/cpe#externalLink -->

    <owl:DatatypeProperty rdf:about="http://cpe.mitre.org/cpe#externalLink">
        <rdfs:range rdf:resource="http://www.w3.org/2001/XMLSchema#anyURI"/>
        <rdfs:comment>Specifies a hyperlink to an external source of additional information</rdfs:comment>
        <rdfs:label>External Link</rdfs:label>
    </owl:DatatypeProperty>
    


    <!-- http://cpe.mitre.org/cpe#generationDate -->

    <owl:DatatypeProperty rdf:about="http://cpe.mitre.org/cpe#generationDate">
        <rdfs:range rdf:resource="http://www.w3.org/2001/XMLSchema#dateTime"/>
        <rdfs:comment>Specifies the date and time when the CPE Dictionary was generated.</rdfs:comment>
        <rdfs:label>Generation Date</rdfs:label>
    </owl:DatatypeProperty>
    


    <!-- http://cpe.mitre.org/cpe#id -->

    <owl:DatatypeProperty rdf:about="http://cpe.mitre.org/cpe#id">
        <rdfs:range rdf:resource="http://www.w3.org/2001/XMLSchema#string"/>
        <rdfs:comment>Specifies the unique identifier associated with the instance</rdfs:comment>
        <rdfs:isDefinedBy rdf:resource="http://cpe.mitre.org/cpe"/>
        <rdfs:label>ID</rdfs:label>
    </owl:DatatypeProperty>
    


    <!-- http://cpe.mitre.org/cpe#identifier -->

    <owl:DatatypeProperty rdf:about="http://cpe.mitre.org/cpe#identifier">
        <rdfs:range rdf:resource="http://www.w3.org/2001/XMLSchema#string"/>
        <rdfs:comment>Specifies an identifier of a test written in that language</rdfs:comment>
        <rdfs:label>Identifier</rdfs:label>
    </owl:DatatypeProperty>
    


    <!-- http://cpe.mitre.org/cpe#language -->

    <owl:DatatypeProperty rdf:about="http://cpe.mitre.org/cpe#language">
        <rdfs:range rdf:resource="http://www.w3.org/2001/XMLSchema#string"/>
        <rdfs:comment>Specifies the language tags, per RFC5646, supported in the user interface of the product being described</rdfs:comment>
        <rdfs:label>Language</rdfs:label>
    </owl:DatatypeProperty>
    


    <!-- http://cpe.mitre.org/cpe#logicalOperator -->

    <owl:DatatypeProperty rdf:about="http://cpe.mitre.org/cpe#logicalOperator">
        <rdfs:range>
            <rdfs:Datatype>
                <owl:oneOf>
                    <rdf:Description>
                        <rdf:type rdf:resource="http://www.w3.org/1999/02/22-rdf-syntax-ns#List"/>
                        <rdf:first rdf:datatype="http://www.w3.org/2001/XMLSchema#string">AND</rdf:first>
                        <rdf:rest>
                            <rdf:Description>
                                <rdf:type rdf:resource="http://www.w3.org/1999/02/22-rdf-syntax-ns#List"/>
                                <rdf:first rdf:datatype="http://www.w3.org/2001/XMLSchema#string">OR</rdf:first>
                                <rdf:rest rdf:resource="http://www.w3.org/1999/02/22-rdf-syntax-ns#nil"/>
                            </rdf:Description>
                        </rdf:rest>
                    </rdf:Description>
                </owl:oneOf>
            </rdfs:Datatype>
        </rdfs:range>
        <rdfs:comment>Specifies the logical operator applied to the results of evaluating the factRef, checkFactRef, and 
logicalTest elements. The permitted operators are “AND” and “OR”.</rdfs:comment>
        <rdfs:label>Logical Operator</rdfs:label>
    </owl:DatatypeProperty>
    


    <!-- http://cpe.mitre.org/cpe#negate -->

    <owl:DatatypeProperty rdf:about="http://cpe.mitre.org/cpe#negate">
        <rdfs:range rdf:resource="http://www.w3.org/2001/XMLSchema#boolean"/>
        <rdfs:comment>Specifies whether the result of applying the operator should be negated. Possible values are “TRUE” and “FALSE”. Ignored if the result of applying the operator is “ERROR”</rdfs:comment>
        <rdfs:label>Negate</rdfs:label>
    </owl:DatatypeProperty>
    


    <!-- http://cpe.mitre.org/cpe#notes -->

    <owl:DatatypeProperty rdf:about="http://cpe.mitre.org/cpe#notes">
        <rdfs:range rdf:resource="http://www.w3.org/2001/XMLSchema#string"/>
        <rdfs:comment>Specifies additional description material for the CPE</rdfs:comment>
        <rdfs:label>Notes</rdfs:label>
    </owl:DatatypeProperty>
    


    <!-- http://cpe.mitre.org/cpe#other -->

    <owl:DatatypeProperty rdf:about="http://cpe.mitre.org/cpe#other">
        <rdfs:range rdf:resource="http://www.w3.org/2001/XMLSchema#string"/>
        <rdfs:comment>Specifies any other general descriptive or identifying information which is vendor or product-specific and which does not logically fit in any other attribute value</rdfs:comment>
        <rdfs:label>Other</rdfs:label>
    </owl:DatatypeProperty>
    


    <!-- http://cpe.mitre.org/cpe#part -->

    <owl:DatatypeProperty rdf:about="http://cpe.mitre.org/cpe#part">
        <rdfs:range rdf:resource="http://www.w3.org/2001/XMLSchema#string"/>
        <rdfs:comment>Specifies the type of part to which the CPE refers.  Valid part values are &apos;a&apos; for application, &apos;o&apos; for operating system, and &apos;h&apos; for hardware devices.</rdfs:comment>
        <rdfs:label>Type of Part</rdfs:label>
    </owl:DatatypeProperty>
    


    <!-- http://cpe.mitre.org/cpe#platformIdentifier -->

    <owl:DatatypeProperty rdf:about="http://cpe.mitre.org/cpe#platformIdentifier">
        <rdfs:range rdf:resource="http://www.w3.org/2001/XMLSchema#string"/>
        <rdfs:comment>Specifies the unique identifier associated with the platform.</rdfs:comment>
        <rdfs:label>Platform Identifier</rdfs:label>
    </owl:DatatypeProperty>
    


    <!-- http://cpe.mitre.org/cpe#productName -->

    <owl:DatatypeProperty rdf:about="http://cpe.mitre.org/cpe#productName">
        <rdfs:range rdf:resource="http://www.w3.org/2001/XMLSchema#string"/>
        <rdfs:comment>Specifies the name of the product</rdfs:comment>
        <rdfs:label>Product Name</rdfs:label>
    </owl:DatatypeProperty>
    


    <!-- http://cpe.mitre.org/cpe#remark -->

    <owl:DatatypeProperty rdf:about="http://cpe.mitre.org/cpe#remark">
        <rdfs:range rdf:resource="http://www.w3.org/2001/XMLSchema#string"/>
        <rdfs:comment>Specifies additional description information.</rdfs:comment>
        <rdfs:label>Remark</rdfs:label>
    </owl:DatatypeProperty>
    


    <!-- http://cpe.mitre.org/cpe#softwareEdition -->

    <owl:DatatypeProperty rdf:about="http://cpe.mitre.org/cpe#softwareEdition">
        <rdfs:range rdf:resource="http://www.w3.org/2001/XMLSchema#string"/>
        <rdfs:comment>Specifies how the product is tailored to a particular market or class for end users</rdfs:comment>
        <rdfs:label>Software Edition</rdfs:label>
    </owl:DatatypeProperty>
    


    <!-- http://cpe.mitre.org/cpe#targetHardware -->

    <owl:DatatypeProperty rdf:about="http://cpe.mitre.org/cpe#targetHardware">
        <rdfs:range rdf:resource="http://www.w3.org/2001/XMLSchema#string"/>
        <rdfs:comment>Specifies the instruction set architecture (e.g., x86) on which the product being described or identified operates.  Bytecode-intermediate languages, such as Java bytecode or Microsoft CLR) should be considered instruction set architectures.</rdfs:comment>
        <rdfs:label>Target Hardware</rdfs:label>
    </owl:DatatypeProperty>
    


    <!-- http://cpe.mitre.org/cpe#targetSoftware -->

    <owl:DatatypeProperty rdf:about="http://cpe.mitre.org/cpe#targetSoftware">
        <rdfs:range rdf:resource="http://www.w3.org/2001/XMLSchema#string"/>
        <rdfs:comment>Specifies how the product is tailored to a particular market or class of end users.</rdfs:comment>
        <rdfs:label>Target Software</rdfs:label>
    </owl:DatatypeProperty>
    


    <!-- http://cpe.mitre.org/cpe#testIdentifer -->

    <owl:DatatypeProperty rdf:about="http://cpe.mitre.org/cpe#testIdentifer">
        <rdfs:range rdf:resource="http://www.w3.org/2001/XMLSchema#string"/>
        <rdfs:comment>Specifies a unique identifier for a logical test</rdfs:comment>
        <rdfs:isDefinedBy rdf:resource="http://cpe.mitre.org/cpe"/>
        <rdfs:label>Test Identifer</rdfs:label>
    </owl:DatatypeProperty>
    


    <!-- http://cpe.mitre.org/cpe#title -->

    <owl:DatatypeProperty rdf:about="http://cpe.mitre.org/cpe#title">
        <rdfs:range rdf:resource="http://www.w3.org/2001/XMLSchema#string"/>
        <rdfs:comment>Specifies a human-readable title associated with the reference</rdfs:comment>
        <rdfs:label>Title</rdfs:label>
    </owl:DatatypeProperty>
    


    <!-- http://cpe.mitre.org/cpe#updateIdentifier -->

    <owl:DatatypeProperty rdf:about="http://cpe.mitre.org/cpe#updateIdentifier">
        <rdfs:range rdf:resource="http://www.w3.org/2001/XMLSchema#string"/>
        <rdfs:comment>Specifies the vendor-specific alphanumeric strings characterizing the particular update, service pack, or point release of the product.</rdfs:comment>
        <rdfs:label>Update</rdfs:label>
    </owl:DatatypeProperty>
    


    <!-- http://cpe.mitre.org/cpe#vendorName -->

    <owl:DatatypeProperty rdf:about="http://cpe.mitre.org/cpe#vendorName">
        <rdfs:range rdf:resource="http://www.w3.org/2001/XMLSchema#string"/>
        <rdfs:comment>Specifies the name of the vendor.</rdfs:comment>
        <rdfs:label>Vendor Name</rdfs:label>
    </owl:DatatypeProperty>
    


    <!-- http://cpe.mitre.org/cpe#version -->

    <owl:DatatypeProperty rdf:about="http://cpe.mitre.org/cpe#version">
        <rdfs:range rdf:resource="http://www.w3.org/2001/XMLSchema#string"/>
        <rdfs:comment>Specifies the vendor-specific alphanumeric string characterizing the particular release version of the product.</rdfs:comment>
        <rdfs:label>Version</rdfs:label>
    </owl:DatatypeProperty>
    


    <!-- 
    ///////////////////////////////////////////////////////////////////////////////////////
    //
    // Classes
    //
    ///////////////////////////////////////////////////////////////////////////////////////
     -->

    


    <!-- http://cpe.mitre.org/cpe#CPE -->

    <owl:Class rdf:about="http://cpe.mitre.org/cpe#CPE">
        <rdfs:subClassOf>
            <owl:Restriction>
                <owl:onProperty rdf:resource="http://cpe.mitre.org/cpe#vendor"/>
                <owl:cardinality rdf:datatype="http://www.w3.org/2001/XMLSchema#nonNegativeInteger">1</owl:cardinality>
            </owl:Restriction>
        </rdfs:subClassOf>
        <rdfs:subClassOf>
            <owl:Restriction>
                <owl:onProperty rdf:resource="http://cpe.mitre.org/cpe#alternateCPE"/>
                <owl:maxCardinality rdf:datatype="http://www.w3.org/2001/XMLSchema#nonNegativeInteger">1</owl:maxCardinality>
            </owl:Restriction>
        </rdfs:subClassOf>
        <rdfs:subClassOf>
            <owl:Restriction>
                <owl:onProperty rdf:resource="http://cpe.mitre.org/cpe#relatedDevice"/>
                <owl:maxCardinality rdf:datatype="http://www.w3.org/2001/XMLSchema#nonNegativeInteger">1</owl:maxCardinality>
            </owl:Restriction>
        </rdfs:subClassOf>
        <rdfs:subClassOf>
            <owl:Restriction>
                <owl:onProperty rdf:resource="http://cpe.mitre.org/cpe#relatedOperatingSystem"/>
                <owl:maxCardinality rdf:datatype="http://www.w3.org/2001/XMLSchema#nonNegativeInteger">1</owl:maxCardinality>
            </owl:Restriction>
        </rdfs:subClassOf>
        <rdfs:subClassOf>
            <owl:Restriction>
                <owl:onProperty rdf:resource="http://cpe.mitre.org/cpe#relatedProduct"/>
                <owl:maxCardinality rdf:datatype="http://www.w3.org/2001/XMLSchema#nonNegativeInteger">1</owl:maxCardinality>
            </owl:Restriction>
        </rdfs:subClassOf>
        <rdfs:subClassOf>
            <owl:Restriction>
                <owl:onProperty rdf:resource="http://cpe.mitre.org/cpe#submitter"/>
                <owl:maxCardinality rdf:datatype="http://www.w3.org/2001/XMLSchema#nonNegativeInteger">1</owl:maxCardinality>
            </owl:Restriction>
        </rdfs:subClassOf>
        <rdfs:subClassOf>
            <owl:Restriction>
                <owl:onProperty rdf:resource="http://cpe.mitre.org/cpe#cpeName"/>
                <owl:cardinality rdf:datatype="http://www.w3.org/2001/XMLSchema#nonNegativeInteger">1</owl:cardinality>
            </owl:Restriction>
        </rdfs:subClassOf>
        <rdfs:subClassOf>
            <owl:Restriction>
                <owl:onProperty rdf:resource="http://cpe.mitre.org/cpe#deprecated"/>
                <owl:cardinality rdf:datatype="http://www.w3.org/2001/XMLSchema#nonNegativeInteger">1</owl:cardinality>
            </owl:Restriction>
        </rdfs:subClassOf>
        <rdfs:subClassOf>
            <owl:Restriction>
                <owl:onProperty rdf:resource="http://cpe.mitre.org/cpe#part"/>
                <owl:cardinality rdf:datatype="http://www.w3.org/2001/XMLSchema#nonNegativeInteger">1</owl:cardinality>
            </owl:Restriction>
        </rdfs:subClassOf>
        <rdfs:subClassOf>
            <owl:Restriction>
                <owl:onProperty rdf:resource="http://cpe.mitre.org/cpe#productName"/>
                <owl:cardinality rdf:datatype="http://www.w3.org/2001/XMLSchema#nonNegativeInteger">1</owl:cardinality>
            </owl:Restriction>
        </rdfs:subClassOf>
        <rdfs:subClassOf>
            <owl:Restriction>
                <owl:onProperty rdf:resource="http://cpe.mitre.org/cpe#edition"/>
                <owl:maxCardinality rdf:datatype="http://www.w3.org/2001/XMLSchema#nonNegativeInteger">1</owl:maxCardinality>
            </owl:Restriction>
        </rdfs:subClassOf>
        <rdfs:subClassOf>
            <owl:Restriction>
                <owl:onProperty rdf:resource="http://cpe.mitre.org/cpe#language"/>
                <owl:maxCardinality rdf:datatype="http://www.w3.org/2001/XMLSchema#nonNegativeInteger">1</owl:maxCardinality>
            </owl:Restriction>
        </rdfs:subClassOf>
        <rdfs:subClassOf>
            <owl:Restriction>
                <owl:onProperty rdf:resource="http://cpe.mitre.org/cpe#other"/>
                <owl:maxCardinality rdf:datatype="http://www.w3.org/2001/XMLSchema#nonNegativeInteger">1</owl:maxCardinality>
            </owl:Restriction>
        </rdfs:subClassOf>
        <rdfs:subClassOf>
            <owl:Restriction>
                <owl:onProperty rdf:resource="http://cpe.mitre.org/cpe#softwareEdition"/>
                <owl:maxCardinality rdf:datatype="http://www.w3.org/2001/XMLSchema#nonNegativeInteger">1</owl:maxCardinality>
            </owl:Restriction>
        </rdfs:subClassOf>
        <rdfs:subClassOf>
            <owl:Restriction>
                <owl:onProperty rdf:resource="http://cpe.mitre.org/cpe#targetSoftware"/>
                <owl:maxCardinality rdf:datatype="http://www.w3.org/2001/XMLSchema#nonNegativeInteger">1</owl:maxCardinality>
            </owl:Restriction>
        </rdfs:subClassOf>
        <rdfs:subClassOf>
            <owl:Restriction>
                <owl:onProperty rdf:resource="http://cpe.mitre.org/cpe#updateIdentifier"/>
                <owl:maxCardinality rdf:datatype="http://www.w3.org/2001/XMLSchema#nonNegativeInteger">1</owl:maxCardinality>
            </owl:Restriction>
        </rdfs:subClassOf>
        <rdfs:subClassOf>
            <owl:Restriction>
                <owl:onProperty rdf:resource="http://cpe.mitre.org/cpe#version"/>
                <owl:maxCardinality rdf:datatype="http://www.w3.org/2001/XMLSchema#nonNegativeInteger">1</owl:maxCardinality>
            </owl:Restriction>
        </rdfs:subClassOf>
        <rdfs:comment>Specifies the label to be used in a human display</rdfs:comment>
        <rdfs:isDefinedBy rdf:resource="http://cpe.mitre.org/cpe"/>
        <rdfs:label>CPE</rdfs:label>
    </owl:Class>
    


    <!-- http://cpe.mitre.org/cpe#ChangeDescription -->

    <owl:Class rdf:about="http://cpe.mitre.org/cpe#ChangeDescription">
        <rdfs:subClassOf>
            <owl:Restriction>
                <owl:onProperty rdf:resource="http://cpe.mitre.org/cpe#changeType"/>
                <owl:cardinality rdf:datatype="http://www.w3.org/2001/XMLSchema#nonNegativeInteger">1</owl:cardinality>
            </owl:Restriction>
        </rdfs:subClassOf>
        <rdfs:subClassOf>
            <owl:Restriction>
                <owl:onProperty rdf:resource="http://cpe.mitre.org/cpe#changeDate"/>
                <owl:maxCardinality rdf:datatype="http://www.w3.org/2001/XMLSchema#nonNegativeInteger">1</owl:maxCardinality>
            </owl:Restriction>
        </rdfs:subClassOf>
        <rdfs:subClassOf>
            <owl:Restriction>
                <owl:onProperty rdf:resource="http://cpe.mitre.org/cpe#evidenceExternalLink"/>
                <owl:maxCardinality rdf:datatype="http://www.w3.org/2001/XMLSchema#nonNegativeInteger">1</owl:maxCardinality>
            </owl:Restriction>
        </rdfs:subClassOf>
        <rdfs:subClassOf>
            <owl:Restriction>
                <owl:onProperty rdf:resource="http://cpe.mitre.org/cpe#evidenceType"/>
                <owl:maxCardinality rdf:datatype="http://www.w3.org/2001/XMLSchema#nonNegativeInteger">1</owl:maxCardinality>
            </owl:Restriction>
        </rdfs:subClassOf>
        <rdfs:comment>Specifies a description of any changes made to the identifier name or associated metadata.</rdfs:comment>
        <rdfs:isDefinedBy rdf:resource="http://cpe.mitre.org/cpe"/>
        <rdfs:label>Change Description</rdfs:label>
    </owl:Class>
    


    <!-- http://cpe.mitre.org/cpe#CheckInfo -->

    <owl:Class rdf:about="http://cpe.mitre.org/cpe#CheckInfo">
        <rdfs:subClassOf rdf:resource="http://cpe.mitre.org/cpe#FactRef"/>
        <rdfs:subClassOf>
            <owl:Restriction>
                <owl:onProperty rdf:resource="http://cpe.mitre.org/cpe#checkSystem"/>
                <owl:cardinality rdf:datatype="http://www.w3.org/2001/XMLSchema#nonNegativeInteger">1</owl:cardinality>
            </owl:Restriction>
        </rdfs:subClassOf>
        <rdfs:subClassOf>
            <owl:Restriction>
                <owl:onProperty rdf:resource="http://cpe.mitre.org/cpe#externalLink"/>
                <owl:cardinality rdf:datatype="http://www.w3.org/2001/XMLSchema#nonNegativeInteger">1</owl:cardinality>
            </owl:Restriction>
        </rdfs:subClassOf>
        <rdfs:subClassOf>
            <owl:Restriction>
                <owl:onProperty rdf:resource="http://cpe.mitre.org/cpe#identifier"/>
                <owl:cardinality rdf:datatype="http://www.w3.org/2001/XMLSchema#nonNegativeInteger">1</owl:cardinality>
            </owl:Restriction>
        </rdfs:subClassOf>
        <rdfs:subClassOf>
            <owl:Restriction>
                <owl:onProperty rdf:resource="http://cpe.mitre.org/cpe#description"/>
                <owl:maxCardinality rdf:datatype="http://www.w3.org/2001/XMLSchema#nonNegativeInteger">1</owl:maxCardinality>
            </owl:Restriction>
        </rdfs:subClassOf>
        <rdfs:comment>Characterizes a a check that always evaluates to a TRUE, FALSE, or ERROR</rdfs:comment>
        <rdfs:isDefinedBy rdf:resource="http://cpe.mitre.org/cpe"/>
        <rdfs:label>Check fact ref</rdfs:label>
    </owl:Class>
    


    <!-- http://cpe.mitre.org/cpe#DeprecationInfo -->

    <owl:Class rdf:about="http://cpe.mitre.org/cpe#DeprecationInfo">
        <rdfs:subClassOf>
            <owl:Restriction>
                <owl:onProperty rdf:resource="http://cpe.mitre.org/cpe#deprecatedBy"/>
                <owl:minCardinality rdf:datatype="http://www.w3.org/2001/XMLSchema#nonNegativeInteger">1</owl:minCardinality>
            </owl:Restriction>
        </rdfs:subClassOf>
        <rdfs:subClassOf>
            <owl:Restriction>
                <owl:onProperty rdf:resource="http://cpe.mitre.org/cpe#deprecationType"/>
                <owl:cardinality rdf:datatype="http://www.w3.org/2001/XMLSchema#nonNegativeInteger">1</owl:cardinality>
            </owl:Restriction>
        </rdfs:subClassOf>
        <rdfs:subClassOf>
            <owl:Restriction>
                <owl:onProperty rdf:resource="http://cpe.mitre.org/cpe#deprecationDate"/>
                <owl:maxCardinality rdf:datatype="http://www.w3.org/2001/XMLSchema#nonNegativeInteger">1</owl:maxCardinality>
            </owl:Restriction>
        </rdfs:subClassOf>
        <rdfs:comment>Specifies the deprecation information for a specific deprecation of a given identifier name.  If a name is deprecated multiple times, there would be a separate instance of the deprecation element for each deprecation.</rdfs:comment>
        <rdfs:isDefinedBy rdf:resource="http://cpe.mitre.org/cpe"/>
        <rdfs:label>Deprecation Info</rdfs:label>
    </owl:Class>
    


    <!-- http://cpe.mitre.org/cpe#FactRef -->

    <owl:Class rdf:about="http://cpe.mitre.org/cpe#FactRef">
        <rdfs:comment></rdfs:comment>
        <rdfs:isDefinedBy rdf:resource="http://cpe.mitre.org/cpe"/>
        <rdfs:label>Fact ref</rdfs:label>
    </owl:Class>
    


    <!-- http://cpe.mitre.org/cpe#LogicalTest -->

    <owl:Class rdf:about="http://cpe.mitre.org/cpe#LogicalTest">
        <rdfs:subClassOf>
            <owl:Restriction>
                <owl:onProperty rdf:resource="http://cpe.mitre.org/cpe#logicalOperator"/>
                <owl:cardinality rdf:datatype="http://www.w3.org/2001/XMLSchema#nonNegativeInteger">1</owl:cardinality>
            </owl:Restriction>
        </rdfs:subClassOf>
        <rdfs:subClassOf>
            <owl:Restriction>
                <owl:onProperty rdf:resource="http://cpe.mitre.org/cpe#negate"/>
                <owl:cardinality rdf:datatype="http://www.w3.org/2001/XMLSchema#nonNegativeInteger">1</owl:cardinality>
            </owl:Restriction>
        </rdfs:subClassOf>
        <rdfs:subClassOf>
            <owl:Restriction>
                <owl:onProperty rdf:resource="http://cpe.mitre.org/cpe#testIdentifer"/>
                <owl:cardinality rdf:datatype="http://www.w3.org/2001/XMLSchema#nonNegativeInteger">1</owl:cardinality>
            </owl:Restriction>
        </rdfs:subClassOf>
        <rdfs:comment>Defines a logical test of a platform.</rdfs:comment>
        <rdfs:isDefinedBy rdf:resource="http://cpe.mitre.org/cpe"/>
        <rdfs:label>Logical Test</rdfs:label>
    </owl:Class>
    


    <!-- http://cpe.mitre.org/cpe#Platform -->

    <owl:Class rdf:about="http://cpe.mitre.org/cpe#Platform">
        <rdfs:subClassOf>
            <owl:Restriction>
                <owl:onProperty rdf:resource="http://cpe.mitre.org/cpe#logicalTest"/>
                <owl:cardinality rdf:datatype="http://www.w3.org/2001/XMLSchema#nonNegativeInteger">1</owl:cardinality>
            </owl:Restriction>
        </rdfs:subClassOf>
        <rdfs:subClassOf>
            <owl:Restriction>
                <owl:onProperty rdf:resource="http://cpe.mitre.org/cpe#platformIdentifier"/>
                <owl:cardinality rdf:datatype="http://www.w3.org/2001/XMLSchema#nonNegativeInteger">1</owl:cardinality>
            </owl:Restriction>
        </rdfs:subClassOf>
        <rdfs:comment>Defines a description or qualifications of a particular IT platform type.</rdfs:comment>
        <rdfs:isDefinedBy rdf:resource="http://cpe.mitre.org/cpe"/>
        <rdfs:label>Platform</rdfs:label>
    </owl:Class>
    


    <!-- http://cpe.mitre.org/cpe#PlatformCatalog -->

    <owl:Class rdf:about="http://cpe.mitre.org/cpe#PlatformCatalog">
        <rdfs:subClassOf rdf:resource="http://scap.nist.gov/scap_core#Catalog"/>
        <rdfs:subClassOf>
            <owl:Restriction>
                <owl:onProperty rdf:resource="http://cpe.mitre.org/cpe#generator"/>
                <owl:maxCardinality rdf:datatype="http://www.w3.org/2001/XMLSchema#nonNegativeInteger">1</owl:maxCardinality>
            </owl:Restriction>
        </rdfs:subClassOf>
        <rdfs:subClassOf>
            <owl:Restriction>
                <owl:onProperty rdf:resource="http://scap.nist.gov/scap_core#generator"/>
                <owl:maxCardinality rdf:datatype="http://www.w3.org/2001/XMLSchema#nonNegativeInteger">1</owl:maxCardinality>
            </owl:Restriction>
        </rdfs:subClassOf>
        <rdfs:subClassOf>
            <owl:Restriction>
                <owl:onProperty rdf:resource="http://cpe.mitre.org/cpe#generationDate"/>
                <owl:cardinality rdf:datatype="http://www.w3.org/2001/XMLSchema#nonNegativeInteger">1</owl:cardinality>
            </owl:Restriction>
        </rdfs:subClassOf>
        <rdfs:comment>Characterizes a catalog of Platform names represented as CPE names.</rdfs:comment>
        <rdfs:isDefinedBy rdf:resource="http://cpe.mitre.org/cpe"/>
        <rdfs:label>Platform Catalog</rdfs:label>
    </owl:Class>
    


    <!-- http://cpe.mitre.org/cpe#ReferenceInfo -->

    <owl:Class rdf:about="http://cpe.mitre.org/cpe#ReferenceInfo">
        <rdfs:subClassOf>
            <owl:Restriction>
                <owl:onProperty rdf:resource="http://cpe.mitre.org/cpe#externalLink"/>
                <owl:cardinality rdf:datatype="http://www.w3.org/2001/XMLSchema#nonNegativeInteger">1</owl:cardinality>
            </owl:Restriction>
        </rdfs:subClassOf>
        <rdfs:subClassOf>
            <owl:Restriction>
                <owl:onProperty rdf:resource="http://cpe.mitre.org/cpe#title"/>
                <owl:cardinality rdf:datatype="http://www.w3.org/2001/XMLSchema#nonNegativeInteger">1</owl:cardinality>
            </owl:Restriction>
        </rdfs:subClassOf>
        <rdfs:comment>Specifies reference information associated with a CPE</rdfs:comment>
        <rdfs:isDefinedBy rdf:resource="http://cpe.mitre.org/cpe"/>
        <rdfs:label>Reference</rdfs:label>
    </owl:Class>
</rdf:RDF>



<!-- Generated by the OWL API (version 4.2.6.20160910-2108) https://github.com/owlcs/owlapi -->

