<?xml version="1.0"?>
<rdf:RDF
    xmlns:rdf="http://www.w3.org/1999/02/22-rdf-syntax-ns#"
    xmlns:emailMsgObj="http://cybox.mitre.org/objects/EmailMessage#"
    xmlns:owl="http://www.w3.org/2002/07/owl#"
    xmlns:xsd="http://www.w3.org/2001/XMLSchema#"
    
    xmlns:rdfs="http://www.w3.org/2000/01/rdf-schema#"
  xml:base="http://cybox.mitre.org/objects/EmailMessage">
  <owl:Ontology rdf:about="http://cybox.mitre.org/objects/EmailMessage">
    <owl:imports rdf:resource="http://cybox.mitre.org/objects/File"/>
    <owl:imports rdf:resource="http://cybox.mitre.org/objects/URI"/>
    <owl:imports rdf:resource="http://cybox.mitre.org/cybox_core"/>
    
    <rdfs:label >Cyber Observable eXpression (CybOX) Email Message Ontology</rdfs:label>
    <rdfs:comment >This ontology provides a vocabulary and representation of an Email Message for the  Cyber Observable eXpression (CybOX).  &#xD;
&#xD;
CybOX  provides a common mechansim (structure and content) to convey the full range of potential cyber observable information and strives to be fully expressive, flexible, extensible, automatable, and as human-readable as possible.&#xD;
&#xD;
The ontology is based on the Cybox Email Message object schema maintained by The MITRE Corporation copyright 2012-2014.  The version number of the ontology is kept in sync with the schema in order to more easily relate between the ontology and the corresponding schema version.&#xD;
&#xD;
Copyright (c) 2014, DaedaFusion, LLC.  All rights reserved.</rdfs:comment>
    <owl:versionInfo rdf:datatype="http://www.w3.org/2001/XMLSchema#string"
    >Created with TopBraid Composer</owl:versionInfo>
  </owl:Ontology>
  <owl:Class rdf:ID="EmailReceivedLine">
    <rdfs:subClassOf>
      <owl:Restriction>
        <owl:maxCardinality rdf:datatype="http://www.w3.org/2001/XMLSchema#nonNegativeInteger"
        >1</owl:maxCardinality>
        <owl:onProperty>
          <owl:DatatypeProperty rdf:ID="timestamp"/>
        </owl:onProperty>
      </owl:Restriction>
    </rdfs:subClassOf>
    <rdfs:comment >Characterizes  a single 'Received' line in an email message header.</rdfs:comment>
    <rdfs:subClassOf>
      <owl:Restriction>
        <owl:maxCardinality rdf:datatype="http://www.w3.org/2001/XMLSchema#nonNegativeInteger"
        >1</owl:maxCardinality>
        <owl:onProperty>
          <owl:DatatypeProperty rdf:ID="via"/>
        </owl:onProperty>
      </owl:Restriction>
    </rdfs:subClassOf>
    <rdfs:subClassOf>
      <owl:Restriction>
        <owl:maxCardinality rdf:datatype="http://www.w3.org/2001/XMLSchema#nonNegativeInteger"
        >1</owl:maxCardinality>
        <owl:onProperty>
          <owl:DatatypeProperty rdf:ID="for"/>
        </owl:onProperty>
      </owl:Restriction>
    </rdfs:subClassOf>
    
    <rdfs:label >Email Received Line</rdfs:label>
    <rdfs:subClassOf>
      <owl:Restriction>
        <owl:maxCardinality rdf:datatype="http://www.w3.org/2001/XMLSchema#nonNegativeInteger"
        >1</owl:maxCardinality>
        <owl:onProperty>
          <owl:DatatypeProperty rdf:ID="with"/>
        </owl:onProperty>
      </owl:Restriction>
    </rdfs:subClassOf>
    <rdfs:subClassOf>
      <owl:Restriction>
        <owl:cardinality rdf:datatype="http://www.w3.org/2001/XMLSchema#nonNegativeInteger"
        >1</owl:cardinality>
        <owl:onProperty>
          <rdf:Description rdf:about="http://cybox.mitre.org/cyboxCommon#id">
            <rdfs:domain rdf:resource="#EmailReceivedLine"/>
          </rdf:Description>
        </owl:onProperty>
      </owl:Restriction>
    </rdfs:subClassOf>
    <rdfs:subClassOf>
      <owl:Restriction>
        <owl:maxCardinality rdf:datatype="http://www.w3.org/2001/XMLSchema#nonNegativeInteger"
        >1</owl:maxCardinality>
        <owl:onProperty>
          <owl:DatatypeProperty rdf:ID="from"/>
        </owl:onProperty>
      </owl:Restriction>
    </rdfs:subClassOf>
    <rdfs:subClassOf>
      <owl:Restriction>
        <owl:maxCardinality rdf:datatype="http://www.w3.org/2001/XMLSchema#nonNegativeInteger"
        >1</owl:maxCardinality>
        <owl:onProperty>
          <owl:DatatypeProperty rdf:ID="by"/>
        </owl:onProperty>
      </owl:Restriction>
    </rdfs:subClassOf>
    <rdfs:subClassOf>
      <owl:Restriction>
        <owl:cardinality rdf:datatype="http://www.w3.org/2001/XMLSchema#nonNegativeInteger"
        >1</owl:cardinality>
        <owl:onProperty>
          <rdf:Description rdf:about="http://cybox.mitre.org/cyboxCommon#parentId">
            <rdfs:domain rdf:resource="#EmailReceivedLine"/>
          </rdf:Description>
        </owl:onProperty>
      </owl:Restriction>
    </rdfs:subClassOf>
    <rdfs:isDefinedBy rdf:resource=""/>
    <rdfs:subClassOf rdf:resource="http://www.w3.org/2002/07/owl#Thing"/>
    <rdfs:subClassOf>
      <owl:Restriction>
        <owl:maxCardinality rdf:datatype="http://www.w3.org/2001/XMLSchema#nonNegativeInteger"
        >1</owl:maxCardinality>
        <owl:onProperty>
          <owl:DatatypeProperty rdf:ID="ID"/>
        </owl:onProperty>
      </owl:Restriction>
    </rdfs:subClassOf>
  </owl:Class>
  <owl:Class rdf:ID="EmailMessage">
    <rdfs:subClassOf>
      <owl:Restriction>
        <owl:maxCardinality rdf:datatype="http://www.w3.org/2001/XMLSchema#nonNegativeInteger"
        >1</owl:maxCardinality>
        <owl:onProperty>
          <owl:DatatypeProperty rdf:ID="header.xPriority"/>
        </owl:onProperty>
      </owl:Restriction>
    </rdfs:subClassOf>
    
    <rdfs:subClassOf>
      <owl:Restriction>
        <owl:maxCardinality rdf:datatype="http://www.w3.org/2001/XMLSchema#nonNegativeInteger"
        >1</owl:maxCardinality>
        <owl:onProperty>
          <owl:DatatypeProperty rdf:ID="header.precedence"/>
        </owl:onProperty>
      </owl:Restriction>
    </rdfs:subClassOf>
    <rdfs:subClassOf>
      <owl:Restriction>
        <owl:maxCardinality rdf:datatype="http://www.w3.org/2001/XMLSchema#nonNegativeInteger"
        >1</owl:maxCardinality>
        <owl:onProperty>
          <owl:DatatypeProperty rdf:ID="rawBody"/>
        </owl:onProperty>
      </owl:Restriction>
    </rdfs:subClassOf>
    <rdfs:subClassOf>
      <owl:Restriction>
        <owl:maxCardinality rdf:datatype="http://www.w3.org/2001/XMLSchema#nonNegativeInteger"
        >1</owl:maxCardinality>
        <owl:onProperty>
          <owl:ObjectProperty rdf:ID="header.replyTo"/>
        </owl:onProperty>
      </owl:Restriction>
    </rdfs:subClassOf>
<!--     <rdfs:subClassOf>
      <owl:Restriction>
        <owl:maxCardinality rdf:datatype="http://www.w3.org/2001/XMLSchema#nonNegativeInteger"
        >1</owl:maxCardinality>
        <owl:onProperty rdf:resource="http://cybox.mitre.org/cybox_core#definedEffect"/>
      </owl:Restriction>
    </rdfs:subClassOf> -->
<!--     <rdfs:subClassOf>
      <owl:Restriction>
        <owl:maxCardinality rdf:datatype="http://www.w3.org/2001/XMLSchema#nonNegativeInteger"
        >1</owl:maxCardinality>
        <owl:onProperty rdf:resource="http://cybox.mitre.org/cybox_core#discoveryMethod"/>
      </owl:Restriction>
    </rdfs:subClassOf> -->
    <rdfs:subClassOf>
      <owl:Restriction>
        <owl:maxCardinality rdf:datatype="http://www.w3.org/2001/XMLSchema#nonNegativeInteger"
        >1</owl:maxCardinality>
        <owl:onProperty>
          <owl:DatatypeProperty rdf:ID="emailServer"/>
        </owl:onProperty>
      </owl:Restriction>
    </rdfs:subClassOf>
    <rdfs:subClassOf>
      <owl:Restriction>
        <owl:maxCardinality rdf:datatype="http://www.w3.org/2001/XMLSchema#nonNegativeInteger"
        >1</owl:maxCardinality>
        <owl:onProperty>
          <owl:ObjectProperty rdf:ID="header.xOriginatingIP"/>
        </owl:onProperty>
      </owl:Restriction>
    </rdfs:subClassOf>
    <rdfs:subClassOf>
      <owl:Restriction>
        <owl:maxCardinality rdf:datatype="http://www.w3.org/2001/XMLSchema#nonNegativeInteger"
        >1</owl:maxCardinality>
        <owl:onProperty>
          <owl:DatatypeProperty rdf:ID="header.messageID"/>
        </owl:onProperty>
      </owl:Restriction>
    </rdfs:subClassOf>
    <rdfs:subClassOf>
      <owl:Restriction>
        <owl:maxCardinality rdf:datatype="http://www.w3.org/2001/XMLSchema#nonNegativeInteger"
        >1</owl:maxCardinality>
        <owl:onProperty>
          <owl:DatatypeProperty rdf:ID="header.subject"/>
        </owl:onProperty>
      </owl:Restriction>
    </rdfs:subClassOf>
    <rdfs:subClassOf>
      <owl:Restriction>
        <owl:maxCardinality rdf:datatype="http://www.w3.org/2001/XMLSchema#nonNegativeInteger"
        >1</owl:maxCardinality>
        <owl:onProperty>
          <owl:DatatypeProperty rdf:ID="header.boundary"/>
        </owl:onProperty>
      </owl:Restriction>
    </rdfs:subClassOf>
<!--     <rdfs:subClassOf>
      <owl:Restriction>
        <owl:maxCardinality rdf:datatype="http://www.w3.org/2001/XMLSchema#nonNegativeInteger"
        >1</owl:maxCardinality>
        <owl:onProperty rdf:resource="http://cybox.mitre.org/cybox_core#physicalLocation"/>
      </owl:Restriction>
    </rdfs:subClassOf> -->
    
<!--     <rdfs:subClassOf>
      <owl:Restriction>
        <owl:maxCardinality rdf:datatype="http://www.w3.org/2001/XMLSchema#nonNegativeInteger"
        >1</owl:maxCardinality>
        <owl:onProperty rdf:resource="http://cybox.mitre.org/cybox_core#description"/>
      </owl:Restriction>
    </rdfs:subClassOf> -->
    <rdfs:subClassOf>
      <owl:Restriction>
        <owl:maxCardinality rdf:datatype="http://www.w3.org/2001/XMLSchema#nonNegativeInteger"
        >1</owl:maxCardinality>
        <owl:onProperty>
          <owl:DatatypeProperty rdf:ID="header.errorsTo"/>
        </owl:onProperty>
      </owl:Restriction>
    </rdfs:subClassOf>
    <rdfs:subClassOf>
      <owl:Restriction>
        <owl:maxCardinality rdf:datatype="http://www.w3.org/2001/XMLSchema#nonNegativeInteger"
        >1</owl:maxCardinality>
        <owl:onProperty>
          <owl:ObjectProperty rdf:ID="header.from"/>
        </owl:onProperty>
      </owl:Restriction>
    </rdfs:subClassOf>
    <rdfs:label >Email Message</rdfs:label>
    <rdfs:subClassOf rdf:resource="http://cybox.mitre.org/cybox_core#Object"/>
    <rdfs:subClassOf>
      <owl:Restriction>
        <owl:onProperty>
          <owl:DatatypeProperty rdf:ID="header.contentType"/>
        </owl:onProperty>
        <owl:maxCardinality rdf:datatype="http://www.w3.org/2001/XMLSchema#nonNegativeInteger"
        >1</owl:maxCardinality>
      </owl:Restriction>
    </rdfs:subClassOf>
    <rdfs:subClassOf>
      <owl:Restriction>
        <owl:onProperty>
          <owl:DatatypeProperty rdf:ID="header.inReplyTo"/>
        </owl:onProperty>
        <owl:maxCardinality rdf:datatype="http://www.w3.org/2001/XMLSchema#nonNegativeInteger"
        >1</owl:maxCardinality>
      </owl:Restriction>
    </rdfs:subClassOf>
    <rdfs:isDefinedBy rdf:resource=""/>
<!--     <rdfs:subClassOf>
      <owl:Restriction>
        <owl:maxCardinality rdf:datatype="http://www.w3.org/2001/XMLSchema#nonNegativeInteger"
        >1</owl:maxCardinality>
        <owl:onProperty rdf:resource="http://cybox.mitre.org/cybox_core#state"/>
      </owl:Restriction>
    </rdfs:subClassOf> -->
    <rdfs:comment >Characterize an individual email message.</rdfs:comment>
<!--     <rdfs:subClassOf>
      <owl:Restriction>
        <owl:cardinality rdf:datatype="http://www.w3.org/2001/XMLSchema#nonNegativeInteger"
        >1</owl:cardinality>
        <owl:onProperty rdf:resource="http://cybox.mitre.org/cyboxCommon#id"/>
      </owl:Restriction>
    </rdfs:subClassOf> -->
<!--     <rdfs:subClassOf>
      <owl:Restriction>
        <owl:maxCardinality rdf:datatype="http://www.w3.org/2001/XMLSchema#nonNegativeInteger"
        >1</owl:maxCardinality>
        <owl:onProperty rdf:resource="http://cybox.mitre.org/cybox_core#hasChanged"/>
      </owl:Restriction>
    </rdfs:subClassOf> -->
    <rdfs:subClassOf>
      <owl:Restriction>
        <owl:maxCardinality rdf:datatype="http://www.w3.org/2001/XMLSchema#nonNegativeInteger"
        >1</owl:maxCardinality>
        <owl:onProperty>
          <owl:DatatypeProperty rdf:ID="header.userAgent"/>
        </owl:onProperty>
      </owl:Restriction>
    </rdfs:subClassOf>
    <rdfs:subClassOf>
      <owl:Restriction>
        <owl:maxCardinality rdf:datatype="http://www.w3.org/2001/XMLSchema#nonNegativeInteger"
        >1</owl:maxCardinality>
        <owl:onProperty>
          <owl:DatatypeProperty rdf:ID="header.xMailer"/>
        </owl:onProperty>
      </owl:Restriction>
    </rdfs:subClassOf>
  </owl:Class>
  <owl:ObjectProperty rdf:ID="header.to">
    <rdfs:range rdf:resource="http://cybox.mitre.org/objects/Address#EmailAddress"/>
    <rdfs:comment >Specifies the email addresses of the recipients of the email message.</rdfs:comment>
    <rdfs:domain rdf:resource="#EmailMessage"/>
    <rdfs:isDefinedBy rdf:resource=""/>
    
    <rdfs:label >To</rdfs:label>
  </owl:ObjectProperty>
  <owl:ObjectProperty rdf:ID="header.receivedLines">
    <rdfs:range rdf:resource="#EmailReceivedLine"/>
    <rdfs:comment >Specifies one or more 'Received' lines that may be included in the email header.</rdfs:comment>
    <rdfs:isDefinedBy rdf:resource=""/>
    <rdfs:label >Received Lines</rdfs:label>
    
    <rdfs:domain rdf:resource="#EmailMessage"/>
  </owl:ObjectProperty>
  <owl:ObjectProperty rdf:ID="header.sender">
    <rdfs:range rdf:resource="http://cybox.mitre.org/objects/Address#EmailAddress"/>
    <rdfs:label >Sender</rdfs:label>
    <rdfs:comment >Specifies the email address of the sender who is acting on behalf of the author listed in the From: field.</rdfs:comment>
    
    <rdfs:isDefinedBy rdf:resource=""/>
    <rdfs:domain rdf:resource="#EmailMessage"/>
  </owl:ObjectProperty>
  <owl:ObjectProperty rdf:ID="header.cc">
    <rdfs:label >Carbon Copied (cc)</rdfs:label>
    <rdfs:domain rdf:resource="#EmailMessage"/>
    <rdfs:range rdf:resource="http://cybox.mitre.org/objects/Address#EmailAddress"/>
    <rdfs:isDefinedBy rdf:resource=""/>
    
    <rdfs:comment >Specifies the email addresses of any recipients that were included in the carbon copy header of the email message.</rdfs:comment>
  </owl:ObjectProperty>
  <owl:ObjectProperty rdf:ID="links">
    <rdfs:comment >Specifies any URL links contained within the email message.</rdfs:comment>
    <rdfs:domain rdf:resource="#EmailMessage"/>
    <rdfs:range rdf:resource="http://cybox.mitre.org/objects/URI#Link"/>
    <rdfs:isDefinedBy rdf:resource=""/>
    
    <rdfs:label >Links</rdfs:label>
  </owl:ObjectProperty>
  <owl:ObjectProperty rdf:ID="header.bcc">
    <rdfs:range rdf:resource="http://cybox.mitre.org/objects/Address#EmailAddress"/>
    <rdfs:comment >Specifies the email addresses of any recipients that were included in the blind carbon copy header of the email message.</rdfs:comment>
    <rdfs:domain rdf:resource="#EmailMessage"/>
    <rdfs:isDefinedBy rdf:resource=""/>
    
    <rdfs:label >Blind Carbon Copied (bcc)</rdfs:label>
  </owl:ObjectProperty>
  <owl:ObjectProperty rdf:about="#header.xOriginatingIP">
    <rdfs:comment >Specifies the originating IP Address of the email sender, in terms of their connection to the mail server used to send the email message.&#xD;
&#xD;
This field is non-standard.</rdfs:comment>
    <rdfs:domain rdf:resource="#EmailMessage"/>
    <rdfs:range>
      <owl:Class>
        <owl:unionOf rdf:parseType="Collection">
          <rdf:Description rdf:about="http://cybox.mitre.org/objects/Address#IPv4Address"/>
          <rdf:Description rdf:about="http://cybox.mitre.org/objects/Address#IPv6Address"/>
        </owl:unionOf>
      </owl:Class>
    </rdfs:range>
    <rdfs:isDefinedBy rdf:resource=""/>
    
    <rdfs:label >X-Originating-IP</rdfs:label>
  </owl:ObjectProperty>
  <owl:ObjectProperty rdf:about="#header.replyTo">
    <rdfs:range rdf:resource="http://cybox.mitre.org/objects/Address#EmailAddress"/>
    <rdfs:comment >Specifies the email address that should be used when replying to the email message.</rdfs:comment>
    <rdfs:domain rdf:resource="#EmailMessage"/>
    <rdfs:isDefinedBy rdf:resource=""/>
    
    <rdfs:label >Reply To</rdfs:label>
  </owl:ObjectProperty>
  <owl:ObjectProperty rdf:ID="attachments">
    <rdfs:comment >Specifies any files that were attached to the email message.</rdfs:comment>
    <rdfs:isDefinedBy rdf:resource=""/>
    <rdfs:domain rdf:resource="#EmailMessage"/>
    <rdfs:range rdf:resource="http://cybox.mitre.org/objects/File#File"/>
    
    <rdfs:label >Attachments</rdfs:label>
  </owl:ObjectProperty>
  <owl:ObjectProperty rdf:about="#header.from">
    <rdfs:comment >Specifies the email address of the sender of the email message.</rdfs:comment>
    <rdfs:domain rdf:resource="#EmailMessage"/>
    <rdfs:range rdf:resource="http://cybox.mitre.org/objects/Address#EmailAddress"/>
    <rdfs:isDefinedBy rdf:resource=""/>
    
    <rdfs:label >Header From</rdfs:label>
  </owl:ObjectProperty>
  <owl:DatatypeProperty rdf:about="#header.xMailer">
    <rdfs:comment >Specifies the software used to send the email message. This field is non-standard.</rdfs:comment>
    <rdfs:range rdf:resource="http://www.w3.org/2001/XMLSchema#string"/>
    <rdfs:domain rdf:resource="#EmailMessage"/>
    <rdfs:isDefinedBy rdf:resource=""/>
    
    <rdfs:label >X-Mailer</rdfs:label>
  </owl:DatatypeProperty>
  <owl:DatatypeProperty rdf:about="#header.xPriority">
    <rdfs:range rdf:resource="http://www.w3.org/2001/XMLSchema#positiveInteger"/>
    <rdfs:comment >Specifies the numerical priority of the email message. &#xD;
&#xD;
This is a non-standard field, but typically a value of '1' is considered the highest priority, '3' is normal, and '5' is the lowest priority.</rdfs:comment>
    <rdfs:domain rdf:resource="#EmailMessage"/>
    <rdfs:isDefinedBy rdf:resource=""/>
    
    <rdfs:label >X-Priority</rdfs:label>
  </owl:DatatypeProperty>
  <owl:DatatypeProperty rdf:about="#via">
    <rdfs:label >Via</rdfs:label>
    <rdfs:range rdf:resource="http://www.w3.org/2001/XMLSchema#string"/>
    <rdfs:isDefinedBy rdf:resource=""/>
    <rdfs:domain rdf:resource="#EmailReceivedLine"/>
    
    <rdfs:comment >Specifies  the 'via' portion of the Received line, if applicable.</rdfs:comment>
  </owl:DatatypeProperty>
  <owl:DatatypeProperty rdf:ID="header.dateSentDateTime">
    <rdfs:domain rdf:resource="#EmailMessage"/>
    <rdfs:range rdf:resource="http://www.w3.org/2001/XMLSchema#dateTime"/>
    <rdfs:isDefinedBy rdf:resource=""/>
    
    <rdfs:label >Date Sent</rdfs:label>
    <rdfs:comment >Specifies the date/time that the email message was sent.</rdfs:comment>
  </owl:DatatypeProperty>
  <owl:DatatypeProperty rdf:about="#header.inReplyTo">
    <rdfs:isDefinedBy rdf:resource=""/>
    <rdfs:label >In Reply To</rdfs:label>
    
    <rdfs:comment >Specifies the message ID of the message that this email is a reply to.</rdfs:comment>
    <rdfs:range rdf:resource="http://www.w3.org/2001/XMLSchema#string"/>
    <rdfs:domain rdf:resource="#EmailMessage"/>
  </owl:DatatypeProperty>
  <owl:DatatypeProperty rdf:about="#header.subject">
    <rdfs:label >Subject</rdfs:label>
    <rdfs:range rdf:resource="http://www.w3.org/2001/XMLSchema#string"/>
    <rdfs:isDefinedBy rdf:resource=""/>
    <rdfs:domain rdf:resource="#EmailMessage"/>
    
    <rdfs:comment >Specifies the subject (a brief summary of the message topic) of the email message.</rdfs:comment>
  </owl:DatatypeProperty>
  <owl:DatatypeProperty rdf:about="#header.messageID">
    <rdfs:comment >Specifies the automatically generated ID of the email message.</rdfs:comment>
    <rdfs:range rdf:resource="http://www.w3.org/2001/XMLSchema#string"/>
    <rdfs:domain rdf:resource="#EmailMessage"/>
    <rdfs:isDefinedBy rdf:resource=""/>
    
    <rdfs:label >Message ID</rdfs:label>
  </owl:DatatypeProperty>
  <owl:DatatypeProperty rdf:about="#for">
    <rdfs:label >For</rdfs:label>
    <rdfs:range rdf:resource="http://www.w3.org/2001/XMLSchema#string"/>
    <rdfs:isDefinedBy rdf:resource=""/>
    <rdfs:domain rdf:resource="#EmailReceivedLine"/>
    
    <rdfs:comment >Specifies the 'for' portion of the Received line, if applicable.</rdfs:comment>
  </owl:DatatypeProperty>
  <owl:DatatypeProperty rdf:about="#header.precedence">
    <rdfs:comment >Specifies the (non-standard) priority value of the message, which can influence transmission speed and delivery.&#xD;
&#xD;
Use of this field is typically discouraged, as per IETF RFC2076 (http://www.faqs.org/rfcs/rfc2076.html).</rdfs:comment>
    <rdfs:range rdf:resource="http://www.w3.org/2001/XMLSchema#string"/>
    <rdfs:domain rdf:resource="#EmailMessage"/>
    <rdfs:isDefinedBy rdf:resource=""/>
    
    <rdfs:label >Precedence</rdfs:label>
  </owl:DatatypeProperty>
  <owl:DatatypeProperty rdf:about="#emailServer">
    <rdfs:range rdf:resource="http://www.w3.org/2001/XMLSchema#string"/>
    <rdfs:comment >Specifies the relevant email server.</rdfs:comment>
    <rdfs:domain rdf:resource="#EmailMessage"/>
    <rdfs:isDefinedBy rdf:resource=""/>
    
    <rdfs:label >Email Server</rdfs:label>
  </owl:DatatypeProperty>
  <owl:DatatypeProperty rdf:ID="header.mimeVersion">
    <rdfs:comment >Specifies the version of the MIME formatting used in the email message.</rdfs:comment>
    <rdfs:label >MIME Version</rdfs:label>
    
    <rdfs:isDefinedBy rdf:resource=""/>
    <rdfs:range rdf:resource="http://www.w3.org/2001/XMLSchema#string"/>
    <rdfs:domain rdf:resource="#EmailMessage"/>
  </owl:DatatypeProperty>
  <owl:DatatypeProperty rdf:about="#header.userAgent">
    <rdfs:comment >Specifies the identity of the email user agent software that may have been used to send the email message.</rdfs:comment>
    <rdfs:range rdf:resource="http://www.w3.org/2001/XMLSchema#string"/>
    <rdfs:domain rdf:resource="#EmailMessage"/>
    <rdfs:isDefinedBy rdf:resource=""/>
    
    <rdfs:label >User Agent</rdfs:label>
  </owl:DatatypeProperty>
  <owl:DatatypeProperty rdf:about="#header.boundary">
    <rdfs:label >Boundary</rdfs:label>
    <rdfs:domain rdf:resource="#EmailMessage"/>
    <rdfs:isDefinedBy rdf:resource=""/>
    <rdfs:range rdf:resource="http://www.w3.org/2001/XMLSchema#string"/>
    
    <rdfs:comment >Specifies a boundary tag that may be included in a MIME multipart message. This boundary tag is used to indicate the parts of a multipart message.</rdfs:comment>
  </owl:DatatypeProperty>
  <owl:DatatypeProperty rdf:about="#with">
    <rdfs:label >With</rdfs:label>
    <rdfs:range rdf:resource="http://www.w3.org/2001/XMLSchema#string"/>
    <rdfs:isDefinedBy rdf:resource=""/>
    <rdfs:domain rdf:resource="#EmailReceivedLine"/>
    
    <rdfs:comment >Specifies the 'with' portion of the Received line, if applicable.</rdfs:comment>
  </owl:DatatypeProperty>
  <owl:DatatypeProperty rdf:ID="rawHeader">
    <rdfs:comment >Specifies the complete (raw) headers of the email message.</rdfs:comment>
    <rdfs:range rdf:resource="http://www.w3.org/2001/XMLSchema#string"/>
    <rdfs:domain rdf:resource="#EmailMessage"/>
    <rdfs:isDefinedBy rdf:resource=""/>
    
    <rdfs:label >Raw Header</rdfs:label>
  </owl:DatatypeProperty>
  <owl:DatatypeProperty rdf:about="#from">
    <rdfs:comment >Specifies the 'from' portion of the Received line, if applicable.</rdfs:comment>
    <rdfs:range rdf:resource="http://www.w3.org/2001/XMLSchema#string"/>
    <rdfs:domain rdf:resource="#EmailReceivedLine"/>
    <rdfs:isDefinedBy rdf:resource=""/>
    
    <rdfs:label >From</rdfs:label>
  </owl:DatatypeProperty>
  <owl:DatatypeProperty rdf:about="#timestamp">
    <rdfs:label >Timestamp</rdfs:label>
    <rdfs:range rdf:resource="http://www.w3.org/2001/XMLSchema#dateTime"/>
    <rdfs:isDefinedBy rdf:resource=""/>
    <rdfs:domain rdf:resource="#EmailReceivedLine"/>
    
    <rdfs:comment >Specifies the timestamp portion of the Received line, if applicable.</rdfs:comment>
  </owl:DatatypeProperty>
  <owl:DatatypeProperty rdf:about="#header.errorsTo">
    <rdfs:comment >Specifies the entry in the (deprecated) errors_to header of the email message.</rdfs:comment>
    <rdfs:range rdf:resource="http://www.w3.org/2001/XMLSchema#string"/>
    <rdfs:domain rdf:resource="#EmailMessage"/>
    <rdfs:isDefinedBy rdf:resource=""/>
    
    <rdfs:label >Errors To</rdfs:label>
  </owl:DatatypeProperty>
  <owl:DatatypeProperty rdf:about="#rawBody">
    <rdfs:comment >Specifies the complete (raw) body of the email message.</rdfs:comment>
    <rdfs:range rdf:resource="http://www.w3.org/2001/XMLSchema#string"/>
    <rdfs:domain rdf:resource="#EmailMessage"/>
    <rdfs:isDefinedBy rdf:resource=""/>
    
    <rdfs:label >Raw Body</rdfs:label>
  </owl:DatatypeProperty>
  <owl:DatatypeProperty rdf:about="#ID">
    <rdfs:isDefinedBy rdf:resource=""/>
    <rdfs:range rdf:resource="http://www.w3.org/2001/XMLSchema#string"/>
    <rdfs:label >ID</rdfs:label>
    <rdfs:domain rdf:resource="#EmailReceivedLine"/>
    
    <rdfs:comment >Specifies the 'id' portion of the Received line, if applicable.</rdfs:comment>
  </owl:DatatypeProperty>
  <owl:DatatypeProperty rdf:about="#by">
    <rdfs:label >By</rdfs:label>
    <rdfs:range rdf:resource="http://www.w3.org/2001/XMLSchema#string"/>
    <rdfs:isDefinedBy rdf:resource=""/>
    <rdfs:domain rdf:resource="#EmailReceivedLine"/>
    
    <rdfs:comment >Specifies  the 'by' portion of the Received line, if applicable.</rdfs:comment>
  </owl:DatatypeProperty>
  <owl:DatatypeProperty rdf:about="#header.contentType">
    <rdfs:label >Content Type</rdfs:label>
    
    <rdfs:isDefinedBy rdf:resource=""/>
    <rdfs:domain rdf:resource="#EmailMessage"/>
    <rdfs:range rdf:resource="http://www.w3.org/2001/XMLSchema#string"/>
    <rdfs:comment >Specifies the internet media, or MIME, type of the email message content.</rdfs:comment>
  </owl:DatatypeProperty>
</rdf:RDF>

<!-- Created with TopBraid -->
