<?xml version="1.0" encoding="UTF-8"?>
<rdf:RDF
	xmlns="http://cybox.mitre.org/objects/File#"
	xmlns:owl="http://www.w3.org/2002/07/owl#"
	xmlns:rdf="http://www.w3.org/1999/02/22-rdf-syntax-ns#"
	xmlns:xml="http://www.w3.org/XML/1998/namespace"
	xmlns:xsd="http://www.w3.org/2001/XMLSchema#"
	xmlns:rdfs="http://www.w3.org/2000/01/rdf-schema#"
	xmlns:fileObj="http://cybox.mitre.org/objects/File#">

<rdf:Description rdf:about="http://cybox.mitre.org/objects/File">
	<rdf:type rdf:resource="http://www.w3.org/2002/07/owl#Ontology"/>
	<owl:imports rdf:resource="http://cybox.mitre.org/objects/Code"/>
	<owl:imports rdf:resource="http://cybox.mitre.org/objects/Library"/>
	<owl:imports rdf:resource="http://cybox.mitre.org/cybox_core"/>
	<rdfs:label>Cyber Observable eXpression (CybOX) File Ontology</rdfs:label>
	<rdfs:comment>This ontology provides a vocabulary and representation of a File for the  Cyber Observable eXpression (CybOX).  &#xD;
&#xD;
CybOX  provides a common mechansim (structure and content) to convey the full range of potential cyber observable information and strives to be fully expressive, flexible, extensible, automatable, and as human-readable as possible.&#xD;
&#xD;
Copyright (c) 2014, DaedaFusion, LLC.  All rights reserved.</rdfs:comment>
	<owl:versionInfo rdf:datatype="http://www.w3.org/2001/XMLSchema#string">1.0.0-000</owl:versionInfo>
</rdf:Description>
<!--  -->
<!--  -->
<!-- ################################################################# -->
<!-- # -->
<!-- #    Annotation properties -->
<!-- # -->
<!-- ################################################################# -->
<!--  -->
<!--  -->
<!-- http://www.w3.org/2002/07/owl#cardinality -->

<rdf:Description rdf:about="http://www.w3.org/2002/07/owl#cardinality">
	<rdf:type rdf:resource="http://www.w3.org/2002/07/owl#AnnotationProperty"/>
</rdf:Description>
<!--  -->
<!-- http://www.w3.org/2002/07/owl#maxCardinality -->

<rdf:Description rdf:about="http://www.w3.org/2002/07/owl#maxCardinality">
	<rdf:type rdf:resource="http://www.w3.org/2002/07/owl#AnnotationProperty"/>
</rdf:Description>
<!--  -->
<!-- http://www.w3.org/2002/07/owl#minCardinality -->

<rdf:Description rdf:about="http://www.w3.org/2002/07/owl#minCardinality">
	<rdf:type rdf:resource="http://www.w3.org/2002/07/owl#AnnotationProperty"/>
</rdf:Description>
<!--  -->
<!--  -->
<!--  -->
<!-- ################################################################# -->
<!-- # -->
<!-- #    Object Properties -->
<!-- # -->
<!-- ################################################################# -->
<!--  -->
<!--  -->
<!-- http://cybox.mitre.org/cyboxCommon#codeSnippets -->

<rdf:Description rdf:about="http://cybox.mitre.org/cyboxCommon#codeSnippets">
	<rdf:type rdf:resource="http://www.w3.org/2002/07/owl#ObjectProperty"/>
	<rdfs:range rdf:resource="http://cybox.mitre.org/objects/Code#Code"/>
</rdf:Description>

<rdf:Description rdf:about="http://cybox.mitre.org/objects/Code#Code">
	<rdf:type rdf:resource="http://www.w3.org/2002/07/owl#Class"/>
</rdf:Description>
<!--  -->
<!-- http://cybox.mitre.org/objects/File#archivedFile -->

<rdf:Description rdf:about="http://cybox.mitre.org/objects/File#archivedFile">
	<rdf:type rdf:resource="http://www.w3.org/2002/07/owl#ObjectProperty"/>
	<rdfs:range rdf:resource="http://cybox.mitre.org/objects/File#File"/>
	<rdfs:comment>Specifies the individual files contained within the archive.</rdfs:comment>
	<rdfs:isDefinedBy rdf:resource="http://cybox.mitre.org/objects/File"/>
	<rdfs:label>Archived File</rdfs:label>
</rdf:Description>
<!--  -->
<!-- http://cybox.mitre.org/objects/File#crossReferenceEntries -->

<rdf:Description rdf:about="http://cybox.mitre.org/objects/File#crossReferenceEntries">
	<rdf:type rdf:resource="http://www.w3.org/2002/07/owl#ObjectProperty"/>
	<rdfs:range rdf:resource="http://cybox.mitre.org/objects/File#PDFXrefEntry"/>
	<rdfs:comment>Specifies the cross-reference entries contained in this cross-reference subsection.</rdfs:comment>
	<rdfs:isDefinedBy rdf:resource="http://cybox.mitre.org/objects/File"/>
	<rdfs:label>Cross-Reference Entries</rdfs:label>
</rdf:Description>
<!--  -->
<!-- http://cybox.mitre.org/objects/File#dataHash.details -->

<rdf:Description rdf:about="http://cybox.mitre.org/objects/File#dataHash.details">
	<rdf:type rdf:resource="http://www.w3.org/2002/07/owl#ObjectProperty"/>
	<rdfs:range rdf:resource="http://cybox.mitre.org/cyboxCommon#Hash"/>
</rdf:Description>

<rdf:Description rdf:about="http://cybox.mitre.org/cyboxCommon#Hash">
	<rdf:type rdf:resource="http://www.w3.org/2002/07/owl#Class"/>
</rdf:Description>

<rdf:Description rdf:about="http://cybox.mitre.org/objects/File#dataHash.details">
	<rdfs:comment>Specifies details about any hash values computed using the data contained in the specified PE binary section as input.</rdfs:comment>
	<rdfs:isDefinedBy rdf:resource="http://cybox.mitre.org/objects/File"/>
	<rdfs:label>Data Hashes</rdfs:label>
</rdf:Description>
<!--  -->
<!-- http://cybox.mitre.org/objects/File#decodedStreamHashDetails -->

<rdf:Description rdf:about="http://cybox.mitre.org/objects/File#decodedStreamHashDetails">
	<rdf:type rdf:resource="http://www.w3.org/2002/07/owl#ObjectProperty"/>
	<rdfs:range rdf:resource="http://cybox.mitre.org/cyboxCommon#Hash"/>
	<rdfs:comment>Specifies details about any hash generated of the decoded stream.</rdfs:comment>
	<rdfs:isDefinedBy rdf:resource="http://cybox.mitre.org/objects/File"/>
	<rdfs:label>Decoded Stream Hashes</rdfs:label>
</rdf:Description>
<!--  -->
<!-- http://cybox.mitre.org/objects/File#detectedEntrypointSignatures -->

<rdf:Description rdf:about="http://cybox.mitre.org/objects/File#detectedEntrypointSignatures">
	<rdf:type rdf:resource="http://www.w3.org/2002/07/owl#ObjectProperty"/>
	<rdfs:range rdf:resource="http://cybox.mitre.org/objects/File#EntryPointSignature"/>
	<rdfs:comment>Specifies the entrypoint signatures that were detected for the packer.</rdfs:comment>
	<rdfs:isDefinedBy rdf:datatype="http://www.w3.org/2001/XMLSchema#string">&lt;http://cybox.mitre.org/objects/File&gt;</rdfs:isDefinedBy>
	<rdfs:label>Detected Entrypoint Signatures</rdfs:label>
</rdf:Description>
<!--  -->
<!-- http://cybox.mitre.org/objects/File#deviceObjects -->

<rdf:Description rdf:about="http://cybox.mitre.org/objects/File#deviceObjects">
	<rdf:type rdf:resource="http://www.w3.org/2002/07/owl#ObjectProperty"/>
	<rdfs:range rdf:resource="http://cybox.mitre.org/objects/File#DeviceObjectStruct"/>
	<rdfs:comment>Specifies the device objects that were created by the driver.</rdfs:comment>
	<rdfs:isDefinedBy rdf:resource="http://cybox.mitre.org/objects/File"/>
	<rdfs:label>Device Objects</rdfs:label>
</rdf:Description>
<!--  -->
<!-- http://cybox.mitre.org/objects/File#digitalSignature -->

<rdf:Description rdf:about="http://cybox.mitre.org/objects/File#digitalSignature">
	<rdf:type rdf:resource="http://www.w3.org/2002/07/owl#ObjectProperty"/>
	<rdfs:range rdf:resource="http://cybox.mitre.org/cyboxCommon#DigitalSignature"/>
</rdf:Description>

<rdf:Description rdf:about="http://cybox.mitre.org/cyboxCommon#DigitalSignature">
	<rdf:type rdf:resource="http://www.w3.org/2002/07/owl#Class"/>
</rdf:Description>

<rdf:Description rdf:about="http://cybox.mitre.org/objects/File#digitalSignature">
	<rdfs:comment>Specifies the information about the digital signature used to sign the PE binary.</rdfs:comment>
	<rdfs:isDefinedBy rdf:resource="http://cybox.mitre.org/objects/File"/>
	<rdfs:label>Digital Signature</rdfs:label>
</rdf:Description>
<!--  -->
<!-- http://cybox.mitre.org/objects/File#dosHeader.hashDetails -->

<rdf:Description rdf:about="http://cybox.mitre.org/objects/File#dosHeader.hashDetails">
	<rdf:type rdf:resource="http://www.w3.org/2002/07/owl#ObjectProperty"/>
	<rdfs:range rdf:resource="http://cybox.mitre.org/cyboxCommon#Hash"/>
	<rdfs:comment>Specifies details about any hash values computed using the specified PE binary MS-DOS header as input.</rdfs:comment>
	<rdfs:isDefinedBy rdf:resource="http://cybox.mitre.org/objects/File"/>
	<rdfs:label>DOS Headers Hashes</rdfs:label>
</rdf:Description>
<!--  -->
<!-- http://cybox.mitre.org/objects/File#encrypt.objectRef -->

<rdf:Description rdf:about="http://cybox.mitre.org/objects/File#encrypt.objectRef">
	<rdf:type rdf:resource="http://www.w3.org/2002/07/owl#ObjectProperty"/>
	<rdfs:range rdf:resource="http://cybox.mitre.org/objects/File#PDFIndirectObject"/>
	<rdfs:comment>Specifies the PDF document's encryption dictionary as an indirect reference.</rdfs:comment>
	<rdfs:isDefinedBy rdf:resource="http://cybox.mitre.org/objects/File"/>
	<rdfs:label>Encryption Dictionary Reference</rdfs:label>
</rdf:Description>
<!--  -->
<!-- http://cybox.mitre.org/objects/File#exportedFunctions -->

<rdf:Description rdf:about="http://cybox.mitre.org/objects/File#exportedFunctions">
	<rdf:type rdf:resource="http://www.w3.org/2002/07/owl#ObjectProperty"/>
	<rdfs:range rdf:resource="http://cybox.mitre.org/objects/File#PEExportedFunction"/>
	<rdfs:comment>Specifies a list of the exported functions in this section.</rdfs:comment>
	<rdfs:isDefinedBy rdf:resource="http://cybox.mitre.org/objects/File"/>
	<rdfs:label>Exported Functions</rdfs:label>
</rdf:Description>
<!--  -->
<!-- http://cybox.mitre.org/objects/File#exports -->

<rdf:Description rdf:about="http://cybox.mitre.org/objects/File#exports">
	<rdf:type rdf:resource="http://www.w3.org/2002/07/owl#ObjectProperty"/>
	<rdfs:range rdf:resource="http://cybox.mitre.org/objects/File#PEExports"/>
	<rdfs:comment>Specifies a reference to the PE Export Table of the PE Binary</rdfs:comment>
	<rdfs:isDefinedBy rdf:resource="http://cybox.mitre.org/objects/File"/>
	<rdfs:label>Exports</rdfs:label>
</rdf:Description>
<!--  -->
<!-- http://cybox.mitre.org/objects/File#fileAttributes -->

<rdf:Description rdf:about="http://cybox.mitre.org/objects/File#fileAttributes">
	<rdf:type rdf:resource="http://www.w3.org/2002/07/owl#ObjectProperty"/>
	<rdfs:range rdf:resource="http://cybox.mitre.org/objects/File#FileAttribute"/>
	<rdfs:comment>Specifies the particular special attributes set for the file.</rdfs:comment>
	<rdfs:isDefinedBy rdf:resource="http://cybox.mitre.org/objects/File"/>
	<rdfs:label>File Attributes</rdfs:label>
</rdf:Description>
<!--  -->
<!-- http://cybox.mitre.org/objects/File#fileHeader.hashDetails -->

<rdf:Description rdf:about="http://cybox.mitre.org/objects/File#fileHeader.hashDetails">
	<rdf:type rdf:resource="http://www.w3.org/2002/07/owl#ObjectProperty"/>
	<rdfs:range rdf:resource="http://cybox.mitre.org/cyboxCommon#Hash"/>
	<rdfs:comment>Specifies details about any hash computed for the Optional Header.</rdfs:comment>
	<rdfs:isDefinedBy rdf:resource="http://cybox.mitre.org/objects/File"/>
	<rdfs:label>File Header Hash Details</rdfs:label>
</rdf:Description>
<!--  -->
<!-- http://cybox.mitre.org/objects/File#hashDetails -->

<rdf:Description rdf:about="http://cybox.mitre.org/objects/File#hashDetails">
	<rdf:type rdf:resource="http://www.w3.org/2002/07/owl#ObjectProperty"/>
	<rdfs:range rdf:resource="http://cybox.mitre.org/cyboxCommon#Hash"/>
	<rdfs:comment>Specifies details about any hashes that were computed for the PDF indirect object.</rdfs:comment>
	<rdfs:isDefinedBy rdf:resource="http://cybox.mitre.org/objects/File"/>
	<rdfs:label>Hash Details</rdfs:label>
</rdf:Description>
<!--  -->
<!-- http://cybox.mitre.org/objects/File#headerHash.details -->

<rdf:Description rdf:about="http://cybox.mitre.org/objects/File#headerHash.details">
	<rdf:type rdf:resource="http://www.w3.org/2002/07/owl#ObjectProperty"/>
	<rdfs:range rdf:resource="http://cybox.mitre.org/cyboxCommon#Hash"/>
	<rdfs:comment>Specifies details about any hash values computed using the header of the specified PE binary section as input.</rdfs:comment>
	<rdfs:isDefinedBy rdf:resource="http://cybox.mitre.org/objects/File"/>
	<rdfs:label>Header Hash Details</rdfs:label>
</rdf:Description>
<!--  -->
<!-- http://cybox.mitre.org/objects/File#headers -->

<rdf:Description rdf:about="http://cybox.mitre.org/objects/File#headers">
	<rdf:type rdf:resource="http://www.w3.org/2002/07/owl#ObjectProperty"/>
	<rdfs:range rdf:resource="http://cybox.mitre.org/objects/File#PEHeaders"/>
	<rdfs:comment>Specifies fields for characterizing aspects the various types of PE headers.</rdfs:comment>
	<rdfs:isDefinedBy rdf:resource="http://cybox.mitre.org/objects/File"/>
	<rdfs:label>Headers</rdfs:label>
</rdf:Description>
<!--  -->
<!-- http://cybox.mitre.org/objects/File#importFile -->

<rdf:Description rdf:about="http://cybox.mitre.org/objects/File#importFile">
	<rdf:type rdf:resource="http://www.w3.org/2002/07/owl#ObjectProperty"/>
	<rdfs:range rdf:nodeID="genid1"/>
</rdf:Description>

<rdf:Description rdf:nodeID="genid1">
	<rdf:type rdf:resource="http://www.w3.org/2002/07/owl#Class"/>
	<owl:unionOf rdf:nodeID="genid3"/>
</rdf:Description>

<rdf:Description rdf:nodeID="genid3">
	<rdf:type rdf:resource="http://www.w3.org/1999/02/22-rdf-syntax-ns#List"/>
	<rdf:first rdf:resource="http://cybox.mitre.org/objects/File#WindowsExecutableFile"/>
	<rdf:rest rdf:nodeID="genid2"/>
</rdf:Description>

<rdf:Description rdf:nodeID="genid2">
	<rdf:type rdf:resource="http://www.w3.org/1999/02/22-rdf-syntax-ns#List"/>
	<rdf:first rdf:resource="http://cybox.mitre.org/objects/Library#Library"/>
</rdf:Description>

<rdf:Description rdf:about="http://cybox.mitre.org/objects/Library#Library">
	<rdf:type rdf:resource="http://www.w3.org/2002/07/owl#Class"/>
</rdf:Description>

<rdf:Description rdf:nodeID="genid2">
	<rdf:rest rdf:resource="http://www.w3.org/1999/02/22-rdf-syntax-ns#nil"/>
</rdf:Description>

<rdf:Description rdf:about="http://cybox.mitre.org/objects/File#importFile">
	<rdfs:comment>Specifies a reference to the import file</rdfs:comment>
	<rdfs:isDefinedBy rdf:resource="http://cybox.mitre.org/objects/File"/>
	<rdfs:label>import file</rdfs:label>
</rdf:Description>
<!--  -->
<!-- http://cybox.mitre.org/objects/File#importedFunctions -->

<rdf:Description rdf:about="http://cybox.mitre.org/objects/File#importedFunctions">
	<rdf:type rdf:resource="http://www.w3.org/2002/07/owl#ObjectProperty"/>
	<rdfs:range rdf:resource="http://cybox.mitre.org/objects/File#PEImportedFunction"/>
	<rdfs:comment>Specifies any functions imported from a particular library.</rdfs:comment>
	<rdfs:isDefinedBy rdf:resource="http://cybox.mitre.org/objects/File"/>
	<rdfs:label>Imported Functions</rdfs:label>
</rdf:Description>
<!--  -->
<!-- http://cybox.mitre.org/objects/File#imports -->

<rdf:Description rdf:about="http://cybox.mitre.org/objects/File#imports">
	<rdf:type rdf:resource="http://www.w3.org/2002/07/owl#ObjectProperty"/>
	<rdfs:range rdf:resource="http://cybox.mitre.org/objects/File#PEImport"/>
	<rdfs:comment>Specifies the PE Import Table of the binary.</rdfs:comment>
	<rdfs:isDefinedBy rdf:resource="http://cybox.mitre.org/objects/File"/>
	<rdfs:label>Imports</rdfs:label>
</rdf:Description>
<!--  -->
<!-- http://cybox.mitre.org/objects/File#info -->

<rdf:Description rdf:about="http://cybox.mitre.org/objects/File#info">
	<rdf:type rdf:resource="http://www.w3.org/2002/07/owl#ObjectProperty"/>
	<rdfs:range rdf:resource="http://cybox.mitre.org/objects/File#PDFIndirectObject"/>
	<rdfs:comment>Specifies an indirect object reference that points to the document information dictionary.</rdfs:comment>
	<rdfs:isDefinedBy rdf:resource="http://cybox.mitre.org/objects/File"/>
	<rdfs:label>Information Dictionary Reference</rdfs:label>
</rdf:Description>
<!--  -->
<!-- http://cybox.mitre.org/objects/File#optionalHeader.dataDirectory -->

<rdf:Description rdf:about="http://cybox.mitre.org/objects/File#optionalHeader.dataDirectory">
	<rdf:type rdf:resource="http://www.w3.org/2002/07/owl#ObjectProperty"/>
	<rdfs:range rdf:resource="http://cybox.mitre.org/objects/File#PEDataDirectory"/>
	<rdfs:comment>Specifies the data directories in the remainder in the optional header. This field will be repeated for each data directory.</rdfs:comment>
	<rdfs:isDefinedBy rdf:resource="http://cybox.mitre.org/objects/File"/>
	<rdfs:label>Data Directory</rdfs:label>
</rdf:Description>
<!--  -->
<!-- http://cybox.mitre.org/objects/File#optionalHeader.hashDetails -->

<rdf:Description rdf:about="http://cybox.mitre.org/objects/File#optionalHeader.hashDetails">
	<rdf:type rdf:resource="http://www.w3.org/2002/07/owl#ObjectProperty"/>
	<rdfs:range rdf:resource="http://cybox.mitre.org/cyboxCommon#Hash"/>
	<rdfs:comment>Specifies details about any hash values computed using the specified PE binary optional header as input.</rdfs:comment>
	<rdfs:isDefinedBy rdf:resource="http://cybox.mitre.org/objects/File"/>
	<rdfs:label>Optional Header - Hash Details</rdfs:label>
</rdf:Description>
<!--  -->
<!-- http://cybox.mitre.org/objects/File#packers -->

<rdf:Description rdf:about="http://cybox.mitre.org/objects/File#packers">
	<rdf:type rdf:resource="http://www.w3.org/2002/07/owl#ObjectProperty"/>
	<rdfs:range rdf:resource="http://cybox.mitre.org/objects/File#Packer"/>
	<rdfs:comment>Specifies any packers that the file may be packed with. The term 'packer' here refers to packers, as well as things like archivers and installers.</rdfs:comment>
	<rdfs:isDefinedBy rdf:resource="http://cybox.mitre.org/objects/File"/>
	<rdfs:label>Packer List</rdfs:label>
</rdf:Description>
<!--  -->
<!-- http://cybox.mitre.org/objects/File#pdfCrossReferenceTables -->

<rdf:Description rdf:about="http://cybox.mitre.org/objects/File#pdfCrossReferenceTables">
	<rdf:type rdf:resource="http://www.w3.org/2002/07/owl#ObjectProperty"/>
	<rdfs:range rdf:resource="http://cybox.mitre.org/objects/File#PDFXrefTable"/>
	<rdfs:comment>Specifies the cross-reference tables included in the PDF file, used for facilitating random access of indirect PDF objects.</rdfs:comment>
	<rdfs:isDefinedBy rdf:resource="http://cybox.mitre.org/objects/File"/>
	<rdfs:label>Cross Reference Tables</rdfs:label>
</rdf:Description>
<!--  -->
<!-- http://cybox.mitre.org/objects/File#pdfIndirectObjects -->

<rdf:Description rdf:about="http://cybox.mitre.org/objects/File#pdfIndirectObjects">
	<rdf:type rdf:resource="http://www.w3.org/2002/07/owl#ObjectProperty"/>
	<rdfs:range rdf:resource="http://cybox.mitre.org/objects/File#PDFIndirectObject"/>
	<rdfs:comment>Specifies references to the indirect objects included in the PDF file, representing the contents of a document.</rdfs:comment>
	<rdfs:isDefinedBy rdf:resource="http://cybox.mitre.org/objects/File"/>
	<rdfs:label>Indirect Objects</rdfs:label>
</rdf:Description>
<!--  -->
<!-- http://cybox.mitre.org/objects/File#pdfMetadata -->

<rdf:Description rdf:about="http://cybox.mitre.org/objects/File#pdfMetadata">
	<rdf:type rdf:resource="http://www.w3.org/2002/07/owl#ObjectProperty"/>
	<rdfs:range rdf:resource="http://cybox.mitre.org/objects/File#PDFMetadata"/>
	<rdfs:comment>Specifies some useful metadata associated with the PDF file.</rdfs:comment>
	<rdfs:isDefinedBy rdf:resource="http://cybox.mitre.org/objects/File"/>
	<rdfs:label>PDF Metadata</rdfs:label>
</rdf:Description>
<!--  -->
<!-- http://cybox.mitre.org/objects/File#pdfTrailers -->

<rdf:Description rdf:about="http://cybox.mitre.org/objects/File#pdfTrailers">
	<rdf:type rdf:resource="http://www.w3.org/2002/07/owl#ObjectProperty"/>
	<rdfs:range rdf:resource="http://cybox.mitre.org/objects/File#PDFTrailer"/>
	<rdfs:comment>Specifies references to the trailers included in the PDF file, used for capturing offsets to the cross-reference table and important objects.</rdfs:comment>
	<rdfs:isDefinedBy rdf:resource="http://cybox.mitre.org/objects/File"/>
	<rdfs:label>Trailers</rdfs:label>
</rdf:Description>
<!--  -->
<!-- http://cybox.mitre.org/objects/File#peHeadersHash.details -->

<rdf:Description rdf:about="http://cybox.mitre.org/objects/File#peHeadersHash.details">
	<rdf:type rdf:resource="http://www.w3.org/2002/07/owl#ObjectProperty"/>
	<rdfs:range rdf:resource="http://cybox.mitre.org/cyboxCommon#Hash"/>
	<rdfs:comment>Specifies details about any hash values conputed using the specified PE bindary file header an input.</rdfs:comment>
	<rdfs:isDefinedBy rdf:resource="http://cybox.mitre.org/objects/File"/>
	<rdfs:label>PEHeaders Hash Details</rdfs:label>
</rdf:Description>
<!--  -->
<!-- http://cybox.mitre.org/objects/File#permissions -->

<rdf:Description rdf:about="http://cybox.mitre.org/objects/File#permissions">
	<rdf:type rdf:resource="http://www.w3.org/2002/07/owl#ObjectProperty"/>
	<rdfs:range rdf:resource="http://cybox.mitre.org/objects/File#FilePermission"/>
	<rdfs:comment>Specifies that particular permissions that a file may have.</rdfs:comment>
	<rdfs:isDefinedBy rdf:resource="http://cybox.mitre.org/objects/File"/>
	<rdfs:label>Permissions</rdfs:label>
</rdf:Description>
<!--  -->
<!-- http://cybox.mitre.org/objects/File#rawStreamHashDetails -->

<rdf:Description rdf:about="http://cybox.mitre.org/objects/File#rawStreamHashDetails">
	<rdf:type rdf:resource="http://www.w3.org/2002/07/owl#ObjectProperty"/>
	<rdfs:range rdf:resource="http://cybox.mitre.org/cyboxCommon#Hash"/>
	<rdfs:comment>Specifies any hashes of the raw, undecoded stream.</rdfs:comment>
	<rdfs:isDefinedBy rdf:resource="http://cybox.mitre.org/objects/File"/>
	<rdfs:label>Raw Stream Hashes</rdfs:label>
</rdf:Description>
<!--  -->
<!-- http://cybox.mitre.org/objects/File#resourceHash.details -->

<rdf:Description rdf:about="http://cybox.mitre.org/objects/File#resourceHash.details">
	<rdf:type rdf:resource="http://www.w3.org/2002/07/owl#ObjectProperty"/>
	<rdfs:range rdf:resource="http://cybox.mitre.org/cyboxCommon#Hash"/>
	<rdfs:comment>Specifies any hash values computed using the specified PE binary resource as input.</rdfs:comment>
	<rdfs:isDefinedBy rdf:resource="http://cybox.mitre.org/objects/File"/>
	<rdfs:label>Resource Hash Details</rdfs:label>
</rdf:Description>
<!--  -->
<!-- http://cybox.mitre.org/objects/File#resources -->

<rdf:Description rdf:about="http://cybox.mitre.org/objects/File#resources">
	<rdf:type rdf:resource="http://www.w3.org/2002/07/owl#ObjectProperty"/>
	<rdfs:range rdf:resource="http://cybox.mitre.org/objects/File#PEResource"/>
	<rdfs:comment>Specifies references to the PE Resources of the binary.</rdfs:comment>
	<rdfs:isDefinedBy rdf:resource="http://cybox.mitre.org/objects/File"/>
	<rdfs:label>Resources</rdfs:label>
</rdf:Description>
<!--  -->
<!-- http://cybox.mitre.org/objects/File#root -->

<rdf:Description rdf:about="http://cybox.mitre.org/objects/File#root">
	<rdf:type rdf:resource="http://www.w3.org/2002/07/owl#ObjectProperty"/>
	<rdfs:range rdf:resource="http://cybox.mitre.org/objects/File#PDFIndirectObject"/>
	<rdfs:comment>Specifies an indirect object reference that points to the catalog dictionary for the PDF document contained in the file.</rdfs:comment>
	<rdfs:isDefinedBy rdf:resource="http://cybox.mitre.org/objects/File"/>
	<rdfs:label>Root</rdfs:label>
</rdf:Description>
<!--  -->
<!-- http://cybox.mitre.org/objects/File#sections -->

<rdf:Description rdf:about="http://cybox.mitre.org/objects/File#sections">
	<rdf:type rdf:resource="http://www.w3.org/2002/07/owl#ObjectProperty"/>
	<rdfs:range rdf:resource="http://cybox.mitre.org/objects/File#PESection"/>
	<rdfs:comment>Specifies references to the PE Sections of the binary.</rdfs:comment>
	<rdfs:isDefinedBy rdf:resource="http://cybox.mitre.org/objects/File"/>
	<rdfs:label>Sections</rdfs:label>
</rdf:Description>
<!--  -->
<!-- http://cybox.mitre.org/objects/File#steams -->

<rdf:Description rdf:about="http://cybox.mitre.org/objects/File#steams">
	<rdf:type rdf:resource="http://www.w3.org/2002/07/owl#ObjectProperty"/>
	<rdfs:range rdf:resource="http://cybox.mitre.org/objects/File#WindowsStream"/>
	<rdfs:comment>Characterize NTFS alternate data streams.</rdfs:comment>
	<rdfs:isDefinedBy rdf:resource="http://cybox.mitre.org/objects/File"/>
	<rdfs:label>Steams</rdfs:label>
</rdf:Description>
<!--  -->
<!-- http://cybox.mitre.org/objects/File#streamContents -->

<rdf:Description rdf:about="http://cybox.mitre.org/objects/File#streamContents">
	<rdf:type rdf:resource="http://www.w3.org/2002/07/owl#ObjectProperty"/>
	<rdfs:range rdf:resource="http://cybox.mitre.org/objects/File#PDFStream"/>
	<rdfs:comment>Specifies the stream contained within in the PDF indirect object, if applicable.</rdfs:comment>
	<rdfs:isDefinedBy rdf:resource="http://cybox.mitre.org/objects/File"/>
	<rdfs:label>Stream Contents</rdfs:label>
</rdf:Description>
<!--  -->
<!-- http://cybox.mitre.org/objects/File#subsections -->

<rdf:Description rdf:about="http://cybox.mitre.org/objects/File#subsections">
	<rdf:type rdf:resource="http://www.w3.org/2002/07/owl#ObjectProperty"/>
	<rdfs:range rdf:resource="http://cybox.mitre.org/objects/File#PDFXrefTableSubsection"/>
	<rdfs:comment>Specifies the subsections contained in the cross-reference table.</rdfs:comment>
	<rdfs:isDefinedBy rdf:resource="http://cybox.mitre.org/objects/File"/>
	<rdfs:label>Subsections</rdfs:label>
</rdf:Description>
<!--  -->
<!--  -->
<!--  -->
<!-- ################################################################# -->
<!-- # -->
<!-- #    Data properties -->
<!-- # -->
<!-- ################################################################# -->
<!--  -->
<!--  -->
<!-- http://cybox.mitre.org/objects/File#ID -->

<rdf:Description rdf:about="http://cybox.mitre.org/objects/File#ID">
	<rdf:type rdf:resource="http://www.w3.org/2002/07/owl#DatatypeProperty"/>
	<rdfs:range rdf:resource="http://www.w3.org/2001/XMLSchema#string"/>
	<rdfs:comment>Specifies an array of two strings that constitutes a file identifier.</rdfs:comment>
	<rdfs:isDefinedBy rdf:resource="http://cybox.mitre.org/objects/File"/>
	<rdfs:label>File Identifier</rdfs:label>
</rdf:Description>
<!--  -->
<!-- http://cybox.mitre.org/objects/File#IRP_MJ_CLEANUP -->

<rdf:Description rdf:about="http://cybox.mitre.org/objects/File#IRP_MJ_CLEANUP">
	<rdf:type rdf:resource="http://www.w3.org/2002/07/owl#DatatypeProperty"/>
	<rdfs:range rdf:resource="http://www.w3.org/2001/XMLSchema#unsignedLong"/>
	<rdfs:comment>Specifies  a count of the number of times the CLEANUP function code was processed by the driver.</rdfs:comment>
	<rdfs:isDefinedBy rdf:resource="http://cybox.mitre.org/objects/File"/>
	<rdfs:label>IRP MJ CLEANUP</rdfs:label>
</rdf:Description>
<!--  -->
<!-- http://cybox.mitre.org/objects/File#IRP_MJ_CLOSE -->

<rdf:Description rdf:about="http://cybox.mitre.org/objects/File#IRP_MJ_CLOSE">
	<rdf:type rdf:resource="http://www.w3.org/2002/07/owl#DatatypeProperty"/>
	<rdfs:range rdf:resource="http://www.w3.org/2001/XMLSchema#unsignedLong"/>
	<rdfs:comment>Specifies a count of the number of times the CLOSE function code was processed by the driver.</rdfs:comment>
	<rdfs:isDefinedBy rdf:resource="http://cybox.mitre.org/objects/File"/>
	<rdfs:label>IRP MJ CLOSE</rdfs:label>
</rdf:Description>
<!--  -->
<!-- http://cybox.mitre.org/objects/File#IRP_MJ_CREATE -->

<rdf:Description rdf:about="http://cybox.mitre.org/objects/File#IRP_MJ_CREATE">
	<rdf:type rdf:resource="http://www.w3.org/2002/07/owl#DatatypeProperty"/>
	<rdfs:range rdf:resource="http://www.w3.org/2001/XMLSchema#unsignedLong"/>
	<rdfs:comment>Specifies a count of the number of times the CREATE function code was processed by the driver.</rdfs:comment>
	<rdfs:isDefinedBy rdf:resource="http://cybox.mitre.org/objects/File"/>
	<rdfs:label>IRP MJ CREATE</rdfs:label>
</rdf:Description>
<!--  -->
<!-- http://cybox.mitre.org/objects/File#IRP_MJ_CREATE_MAILSLOT -->

<rdf:Description rdf:about="http://cybox.mitre.org/objects/File#IRP_MJ_CREATE_MAILSLOT">
	<rdf:type rdf:resource="http://www.w3.org/2002/07/owl#DatatypeProperty"/>
	<rdfs:range rdf:resource="http://www.w3.org/2001/XMLSchema#unsignedLong"/>
	<rdfs:comment>Specifies a count of the number of times the CREATE_MAILSLOT function code was processed by the driver.</rdfs:comment>
	<rdfs:isDefinedBy rdf:resource="http://cybox.mitre.org/objects/File"/>
	<rdfs:label>IRP MJ CREATE MAILSLOT</rdfs:label>
</rdf:Description>
<!--  -->
<!-- http://cybox.mitre.org/objects/File#IRP_MJ_CREATE_NAMED_PIPE -->

<rdf:Description rdf:about="http://cybox.mitre.org/objects/File#IRP_MJ_CREATE_NAMED_PIPE">
	<rdf:type rdf:resource="http://www.w3.org/2002/07/owl#DatatypeProperty"/>
	<rdfs:range rdf:resource="http://www.w3.org/2001/XMLSchema#unsignedLong"/>
	<rdfs:comment>Specifies count of the number of times the CREATE_NAMED_PIPE function code was processed by the driver.</rdfs:comment>
	<rdfs:isDefinedBy rdf:resource="http://cybox.mitre.org/objects/File"/>
	<rdfs:label>IRP MJ CREATE NAMED PIPE</rdfs:label>
</rdf:Description>
<!--  -->
<!-- http://cybox.mitre.org/objects/File#IRP_MJ_DEVICE_CHANGE -->

<rdf:Description rdf:about="http://cybox.mitre.org/objects/File#IRP_MJ_DEVICE_CHANGE">
	<rdf:type rdf:resource="http://www.w3.org/2002/07/owl#DatatypeProperty"/>
	<rdfs:range rdf:resource="http://www.w3.org/2001/XMLSchema#unsignedLong"/>
	<rdfs:comment>Specifies a count of the number of times the DEVICE_CHANGE function code was processed by the driver.</rdfs:comment>
	<rdfs:isDefinedBy rdf:resource="http://cybox.mitre.org/objects/File"/>
	<rdfs:label>IRP MJ DEVICE CHANGE</rdfs:label>
</rdf:Description>
<!--  -->
<!-- http://cybox.mitre.org/objects/File#IRP_MJ_DEVICE_CONTROL -->

<rdf:Description rdf:about="http://cybox.mitre.org/objects/File#IRP_MJ_DEVICE_CONTROL">
	<rdf:type rdf:resource="http://www.w3.org/2002/07/owl#DatatypeProperty"/>
	<rdfs:range rdf:resource="http://www.w3.org/2001/XMLSchema#unsignedLong"/>
	<rdfs:comment>Specifies a count of the number of times the DEVICE_CONTROL function code was processed by the driver.</rdfs:comment>
	<rdfs:isDefinedBy rdf:resource="http://cybox.mitre.org/objects/File"/>
	<rdfs:label>IRP MJ DEVICE CONTROL</rdfs:label>
</rdf:Description>
<!--  -->
<!-- http://cybox.mitre.org/objects/File#IRP_MJ_DIRECTORY_CONTROL -->

<rdf:Description rdf:about="http://cybox.mitre.org/objects/File#IRP_MJ_DIRECTORY_CONTROL">
	<rdf:type rdf:resource="http://www.w3.org/2002/07/owl#DatatypeProperty"/>
	<rdfs:range rdf:resource="http://www.w3.org/2001/XMLSchema#unsignedLong"/>
	<rdfs:comment>Specifies a count of the number of times the DIRECTORY_CONTROL function code was processed by the driver.</rdfs:comment>
	<rdfs:isDefinedBy rdf:resource="http://cybox.mitre.org/objects/File"/>
	<rdfs:label>IRP MJ DIRECTORY CONTROL</rdfs:label>
</rdf:Description>
<!--  -->
<!-- http://cybox.mitre.org/objects/File#IRP_MJ_FILE_SYSTEM_CONTROL -->

<rdf:Description rdf:about="http://cybox.mitre.org/objects/File#IRP_MJ_FILE_SYSTEM_CONTROL">
	<rdf:type rdf:resource="http://www.w3.org/2002/07/owl#DatatypeProperty"/>
	<rdfs:range rdf:resource="http://www.w3.org/2001/XMLSchema#unsignedLong"/>
	<rdfs:comment>Specifies a count of the number of times the FILE_SYSTEM_CONTROL function code was processed by the driver.</rdfs:comment>
	<rdfs:isDefinedBy rdf:resource="http://cybox.mitre.org/objects/File"/>
	<rdfs:label>IRP MJ FILE SYSTEM CONTROL</rdfs:label>
</rdf:Description>
<!--  -->
<!-- http://cybox.mitre.org/objects/File#IRP_MJ_FLUSH_BUFFERS -->

<rdf:Description rdf:about="http://cybox.mitre.org/objects/File#IRP_MJ_FLUSH_BUFFERS">
	<rdf:type rdf:resource="http://www.w3.org/2002/07/owl#DatatypeProperty"/>
	<rdfs:range rdf:resource="http://www.w3.org/2001/XMLSchema#unsignedLong"/>
	<rdfs:comment>Specifies a count of the number of times the FLUSH_BUFFERS function code was processed by the driver.</rdfs:comment>
	<rdfs:isDefinedBy rdf:resource="http://cybox.mitre.org/objects/File"/>
	<rdfs:label>IRP MJ FLUSH BUFFERS</rdfs:label>
</rdf:Description>
<!--  -->
<!-- http://cybox.mitre.org/objects/File#IRP_MJ_INTERNAL_DEVICE_CONTROL -->

<rdf:Description rdf:about="http://cybox.mitre.org/objects/File#IRP_MJ_INTERNAL_DEVICE_CONTROL">
	<rdf:type rdf:resource="http://www.w3.org/2002/07/owl#DatatypeProperty"/>
	<rdfs:range rdf:resource="http://www.w3.org/2001/XMLSchema#unsignedLong"/>
	<rdfs:comment>Specifies a  count of the number of times the INTERNAL_DEVICE_CONTROL function code was processed by the driver.</rdfs:comment>
	<rdfs:isDefinedBy rdf:resource="http://cybox.mitre.org/objects/File"/>
	<rdfs:label>IRP MJ INTERNAL DEVICE CONTROL</rdfs:label>
</rdf:Description>
<!--  -->
<!-- http://cybox.mitre.org/objects/File#IRP_MJ_LOCK_CONTROL -->

<rdf:Description rdf:about="http://cybox.mitre.org/objects/File#IRP_MJ_LOCK_CONTROL">
	<rdf:type rdf:resource="http://www.w3.org/2002/07/owl#DatatypeProperty"/>
	<rdfs:range rdf:resource="http://www.w3.org/2001/XMLSchema#unsignedLong"/>
	<rdfs:comment>Specifies a count of the number of times the LOCK_CONROL function code was processed by the driver.</rdfs:comment>
	<rdfs:isDefinedBy rdf:resource="http://cybox.mitre.org/objects/File"/>
	<rdfs:label>IRP MJ LOCK CONTROL</rdfs:label>
</rdf:Description>
<!--  -->
<!-- http://cybox.mitre.org/objects/File#IRP_MJ_PNP -->

<rdf:Description rdf:about="http://cybox.mitre.org/objects/File#IRP_MJ_PNP">
	<rdf:type rdf:resource="http://www.w3.org/2002/07/owl#DatatypeProperty"/>
	<rdfs:range rdf:resource="http://www.w3.org/2001/XMLSchema#unsignedLong"/>
	<rdfs:comment>Specifies a count of the number of times the PNP function code was processed by the driver.</rdfs:comment>
	<rdfs:isDefinedBy rdf:resource="http://cybox.mitre.org/objects/File"/>
	<rdfs:label>IRP MJ PNP</rdfs:label>
</rdf:Description>
<!--  -->
<!-- http://cybox.mitre.org/objects/File#IRP_MJ_POWER -->

<rdf:Description rdf:about="http://cybox.mitre.org/objects/File#IRP_MJ_POWER">
	<rdf:type rdf:resource="http://www.w3.org/2002/07/owl#DatatypeProperty"/>
	<rdfs:range rdf:resource="http://www.w3.org/2001/XMLSchema#unsignedLong"/>
	<rdfs:comment>Specifies a count of the number of times the POWER function code was processed by the driver.</rdfs:comment>
	<rdfs:isDefinedBy rdf:resource="http://cybox.mitre.org/objects/File"/>
	<rdfs:label>IRP MJ POWER</rdfs:label>
</rdf:Description>
<!--  -->
<!-- http://cybox.mitre.org/objects/File#IRP_MJ_QUERY_EA -->

<rdf:Description rdf:about="http://cybox.mitre.org/objects/File#IRP_MJ_QUERY_EA">
	<rdf:type rdf:resource="http://www.w3.org/2002/07/owl#DatatypeProperty"/>
	<rdfs:range rdf:resource="http://www.w3.org/2001/XMLSchema#unsignedLong"/>
	<rdfs:comment>Specifies a count of the number of times the QUERY_EA function code was processed by the driver.</rdfs:comment>
	<rdfs:isDefinedBy rdf:resource="http://cybox.mitre.org/objects/File"/>
	<rdfs:label>IRP MJ QUERY EA</rdfs:label>
</rdf:Description>
<!--  -->
<!-- http://cybox.mitre.org/objects/File#IRP_MJ_QUERY_INFORMATION -->

<rdf:Description rdf:about="http://cybox.mitre.org/objects/File#IRP_MJ_QUERY_INFORMATION">
	<rdf:type rdf:resource="http://www.w3.org/2002/07/owl#DatatypeProperty"/>
	<rdfs:range rdf:resource="http://www.w3.org/2001/XMLSchema#unsignedLong"/>
	<rdfs:comment>Specifies a count of the number of times the QUERY_INFORMATION function code was processed by the driver.</rdfs:comment>
	<rdfs:isDefinedBy rdf:resource="http://cybox.mitre.org/objects/File"/>
	<rdfs:label>IRP MJ QUERY INFORMATION</rdfs:label>
</rdf:Description>
<!--  -->
<!-- http://cybox.mitre.org/objects/File#IRP_MJ_QUERY_QUOTA -->

<rdf:Description rdf:about="http://cybox.mitre.org/objects/File#IRP_MJ_QUERY_QUOTA">
	<rdf:type rdf:resource="http://www.w3.org/2002/07/owl#DatatypeProperty"/>
	<rdfs:range rdf:resource="http://www.w3.org/2001/XMLSchema#unsignedLong"/>
	<rdfs:comment>Specifies a count of the number of times the QUERY_QUOTA function code was processed by the driver.</rdfs:comment>
	<rdfs:isDefinedBy rdf:resource="http://cybox.mitre.org/objects/File"/>
	<rdfs:label>IRP MJ QUERY QUOTA</rdfs:label>
</rdf:Description>
<!--  -->
<!-- http://cybox.mitre.org/objects/File#IRP_MJ_QUERY_SECURITY -->

<rdf:Description rdf:about="http://cybox.mitre.org/objects/File#IRP_MJ_QUERY_SECURITY">
	<rdf:type rdf:resource="http://www.w3.org/2002/07/owl#DatatypeProperty"/>
	<rdfs:range rdf:resource="http://www.w3.org/2001/XMLSchema#unsignedLong"/>
	<rdfs:comment>Specifies a count of the number of times the QUERY_SECURITY function code was processed by the driver.</rdfs:comment>
	<rdfs:isDefinedBy rdf:resource="http://cybox.mitre.org/objects/File"/>
	<rdfs:label>IRP MJ QUERY SECURITY</rdfs:label>
</rdf:Description>
<!--  -->
<!-- http://cybox.mitre.org/objects/File#IRP_MJ_QUERY_VOLUME_INFORMATION -->

<rdf:Description rdf:about="http://cybox.mitre.org/objects/File#IRP_MJ_QUERY_VOLUME_INFORMATION">
	<rdf:type rdf:resource="http://www.w3.org/2002/07/owl#DatatypeProperty"/>
	<rdfs:range rdf:resource="http://www.w3.org/2001/XMLSchema#unsignedLong"/>
	<rdfs:comment>Specifies a count of the number of times the QUERY_VOLUME_INFORMATION function code was processed by the driver.</rdfs:comment>
	<rdfs:isDefinedBy rdf:resource="http://cybox.mitre.org/objects/File"/>
	<rdfs:label>IRP MJ QUERY VOLUME INFORMATION</rdfs:label>
</rdf:Description>
<!--  -->
<!-- http://cybox.mitre.org/objects/File#IRP_MJ_READ -->

<rdf:Description rdf:about="http://cybox.mitre.org/objects/File#IRP_MJ_READ">
	<rdf:type rdf:resource="http://www.w3.org/2002/07/owl#DatatypeProperty"/>
	<rdfs:range rdf:resource="http://www.w3.org/2001/XMLSchema#unsignedLong"/>
	<rdfs:comment>Specifies a count of the number of times the READ function code was processed by the driver.</rdfs:comment>
	<rdfs:isDefinedBy rdf:resource="http://cybox.mitre.org/objects/File"/>
	<rdfs:label>IRP MJ READ</rdfs:label>
</rdf:Description>
<!--  -->
<!-- http://cybox.mitre.org/objects/File#IRP_MJ_SET_EA -->

<rdf:Description rdf:about="http://cybox.mitre.org/objects/File#IRP_MJ_SET_EA">
	<rdf:type rdf:resource="http://www.w3.org/2002/07/owl#DatatypeProperty"/>
	<rdfs:range rdf:resource="http://www.w3.org/2001/XMLSchema#unsignedLong"/>
	<rdfs:comment>Specifies a count of the number of times the SET_EA function code was processed by the driver.</rdfs:comment>
	<rdfs:isDefinedBy rdf:resource="http://cybox.mitre.org/objects/File"/>
	<rdfs:label>IRP MJ SET EA</rdfs:label>
</rdf:Description>
<!--  -->
<!-- http://cybox.mitre.org/objects/File#IRP_MJ_SET_INFORMATION -->

<rdf:Description rdf:about="http://cybox.mitre.org/objects/File#IRP_MJ_SET_INFORMATION">
	<rdf:type rdf:resource="http://www.w3.org/2002/07/owl#DatatypeProperty"/>
	<rdfs:range rdf:resource="http://www.w3.org/2001/XMLSchema#unsignedLong"/>
	<rdfs:comment>Specifies a count of the number of times the SET_INFORMATION function code was processed by the driver.</rdfs:comment>
	<rdfs:isDefinedBy rdf:datatype="http://www.w3.org/2001/XMLSchema#string">&lt;http://cybox.mitre.org/objects/File&gt;</rdfs:isDefinedBy>
	<rdfs:label>IRP MJ SET INFORMATION</rdfs:label>
</rdf:Description>
<!--  -->
<!-- http://cybox.mitre.org/objects/File#IRP_MJ_SET_QUOTA -->

<rdf:Description rdf:about="http://cybox.mitre.org/objects/File#IRP_MJ_SET_QUOTA">
	<rdf:type rdf:resource="http://www.w3.org/2002/07/owl#DatatypeProperty"/>
	<rdfs:range rdf:resource="http://www.w3.org/2001/XMLSchema#unsignedLong"/>
	<rdfs:comment>Specifies a count of the number of times the SET_QUOTA function code was processed by the driver.</rdfs:comment>
	<rdfs:isDefinedBy rdf:resource="http://cybox.mitre.org/objects/File"/>
	<rdfs:label>IRP MJ SET QUOTA</rdfs:label>
</rdf:Description>
<!--  -->
<!-- http://cybox.mitre.org/objects/File#IRP_MJ_SET_SECURITY -->

<rdf:Description rdf:about="http://cybox.mitre.org/objects/File#IRP_MJ_SET_SECURITY">
	<rdf:type rdf:resource="http://www.w3.org/2002/07/owl#DatatypeProperty"/>
	<rdfs:range rdf:resource="http://www.w3.org/2001/XMLSchema#unsignedLong"/>
	<rdfs:comment>Specifies a count of the number of times the SET_SECURITY function code was processed by the driver.</rdfs:comment>
	<rdfs:isDefinedBy rdf:resource="http://cybox.mitre.org/objects/File"/>
	<rdfs:label>IRP MJ SET SECURITY</rdfs:label>
</rdf:Description>
<!--  -->
<!-- http://cybox.mitre.org/objects/File#IRP_MJ_SET_VOLUME_INFORMATION -->

<rdf:Description rdf:about="http://cybox.mitre.org/objects/File#IRP_MJ_SET_VOLUME_INFORMATION">
	<rdf:type rdf:resource="http://www.w3.org/2002/07/owl#DatatypeProperty"/>
	<rdfs:range rdf:resource="http://www.w3.org/2001/XMLSchema#unsignedLong"/>
	<rdfs:comment>Specifies a count of the number of times the SET_VOLUME_INFORMATION function code was processed by the driver.</rdfs:comment>
	<rdfs:isDefinedBy rdf:resource="http://cybox.mitre.org/objects/File"/>
	<rdfs:label>IRP MJ SET VOLUME INFORMATION</rdfs:label>
</rdf:Description>
<!--  -->
<!-- http://cybox.mitre.org/objects/File#IRP_MJ_SHUTDOWN -->

<rdf:Description rdf:about="http://cybox.mitre.org/objects/File#IRP_MJ_SHUTDOWN">
	<rdf:type rdf:resource="http://www.w3.org/2002/07/owl#DatatypeProperty"/>
	<rdfs:range rdf:resource="http://www.w3.org/2001/XMLSchema#unsignedLong"/>
	<rdfs:comment>Specifies a count of the number of times the SHUTDOWN function code was processed by the driver.</rdfs:comment>
	<rdfs:isDefinedBy rdf:resource="http://cybox.mitre.org/objects/File"/>
	<rdfs:label>IRP MJ SHUTDOWN</rdfs:label>
</rdf:Description>
<!--  -->
<!-- http://cybox.mitre.org/objects/File#IRP_MJ_SYSTEM_CONTROL -->

<rdf:Description rdf:about="http://cybox.mitre.org/objects/File#IRP_MJ_SYSTEM_CONTROL">
	<rdf:type rdf:resource="http://www.w3.org/2002/07/owl#DatatypeProperty"/>
	<rdfs:range rdf:resource="http://www.w3.org/2001/XMLSchema#unsignedLong"/>
	<rdfs:comment>Specifies a count of the number of times the SYSTEM_CONTROL function code was processed by the driver.</rdfs:comment>
	<rdfs:isDefinedBy rdf:resource="http://cybox.mitre.org/objects/File"/>
	<rdfs:label>IRP MJ SYSTEM CONTROL</rdfs:label>
</rdf:Description>
<!--  -->
<!-- http://cybox.mitre.org/objects/File#IRP_MJ_WRITE -->

<rdf:Description rdf:about="http://cybox.mitre.org/objects/File#IRP_MJ_WRITE">
	<rdf:type rdf:resource="http://www.w3.org/2002/07/owl#DatatypeProperty"/>
	<rdfs:range rdf:resource="http://www.w3.org/2001/XMLSchema#unsignedLong"/>
	<rdfs:comment>Specifies a count of the number of times the WRITE function code was processed by the driver.</rdfs:comment>
	<rdfs:isDefinedBy rdf:resource="http://cybox.mitre.org/objects/File"/>
	<rdfs:label>IRP MJ WRITE</rdfs:label>
</rdf:Description>
<!--  -->
<!-- http://cybox.mitre.org/objects/File#aaCount.nonObfuscated -->

<rdf:Description rdf:about="http://cybox.mitre.org/objects/File#aaCount.nonObfuscated">
	<rdf:type rdf:resource="http://www.w3.org/2002/07/owl#DatatypeProperty"/>
	<rdfs:range rdf:resource="http://www.w3.org/2001/XMLSchema#nonNegativeInteger"/>
	<rdfs:comment>Specifies the number of non-obfuscated occurrences of the '/AA' keyword in the PDF file.</rdfs:comment>
	<rdfs:isDefinedBy rdf:datatype="http://www.w3.org/2001/XMLSchema#string">&lt;http://cybox.mitre.org/objects/File&gt;</rdfs:isDefinedBy>
	<rdfs:label>'/AA' Non-obfuscated Count</rdfs:label>
</rdf:Description>
<!--  -->
<!-- http://cybox.mitre.org/objects/File#aaCount.obfuscated -->

<rdf:Description rdf:about="http://cybox.mitre.org/objects/File#aaCount.obfuscated">
	<rdf:type rdf:resource="http://www.w3.org/2002/07/owl#DatatypeProperty"/>
	<rdfs:range rdf:resource="http://www.w3.org/2001/XMLSchema#nonNegativeInteger"/>
	<rdfs:comment>Specifies the number of obfuscated occurrences of the '/AA' keyword in the PDF file with some form of obfuscation, such as with hexcodes.</rdfs:comment>
	<rdfs:isDefinedBy rdf:resource="http://cybox.mitre.org/objects/File"/>
	<rdfs:label>'/AA' Obfuscated Count</rdfs:label>
</rdf:Description>
<!--  -->
<!-- http://cybox.mitre.org/objects/File#architecture.size -->

<rdf:Description rdf:about="http://cybox.mitre.org/objects/File#architecture.size">
	<rdf:type rdf:resource="http://www.w3.org/2002/07/owl#DatatypeProperty"/>
	<rdfs:range rdf:resource="http://www.w3.org/2001/XMLSchema#nonNegativeInteger"/>
	<rdfs:comment>Reserved; Must be 0</rdfs:comment>
	<rdfs:isDefinedBy rdf:resource="http://cybox.mitre.org/objects/File"/>
	<rdfs:label>Architecture Size</rdfs:label>
</rdf:Description>
<!--  -->
<!-- http://cybox.mitre.org/objects/File#architecture.virtualAddress -->

<rdf:Description rdf:about="http://cybox.mitre.org/objects/File#architecture.virtualAddress">
	<rdf:type rdf:resource="http://www.w3.org/2002/07/owl#DatatypeProperty"/>
	<rdfs:range rdf:resource="http://www.w3.org/2001/XMLSchema#hexBinary"/>
	<rdfs:comment>Reserved; must be 0</rdfs:comment>
	<rdfs:isDefinedBy rdf:resource="http://cybox.mitre.org/objects/File"/>
	<rdfs:label>Architecture Virtual Address</rdfs:label>
</rdf:Description>
<!--  -->
<!-- http://cybox.mitre.org/objects/File#archive -->

<rdf:Description rdf:about="http://cybox.mitre.org/objects/File#archive">
	<rdf:type rdf:resource="http://www.w3.org/2002/07/owl#DatatypeProperty"/>
	<rdfs:range rdf:resource="http://www.w3.org/2001/XMLSchema#boolean"/>
	<rdfs:comment>Specifies a file or directory that is an archive file or directory, as denoted by the constant value, 0x20. Applications typically use this attribute to mark files for backup or removal.</rdfs:comment>
	<rdfs:isDefinedBy rdf:resource="http://cybox.mitre.org/objects/File"/>
	<rdfs:label>Archive</rdfs:label>
</rdf:Description>
<!--  -->
<!-- http://cybox.mitre.org/objects/File#archiveComment -->

<rdf:Description rdf:about="http://cybox.mitre.org/objects/File#archiveComment">
	<rdf:type rdf:resource="http://www.w3.org/2002/07/owl#DatatypeProperty"/>
	<rdfs:range rdf:resource="http://www.w3.org/2001/XMLSchema#string"/>
	<rdfs:comment>Specifies the comment information associated with archive file.</rdfs:comment>
	<rdfs:isDefinedBy rdf:resource="http://cybox.mitre.org/objects/File"/>
	<rdfs:label>Comment</rdfs:label>
</rdf:Description>
<!--  -->
<!-- http://cybox.mitre.org/objects/File#archiveFormat -->

<rdf:Description rdf:about="http://cybox.mitre.org/objects/File#archiveFormat">
	<rdf:type rdf:resource="http://www.w3.org/2002/07/owl#DatatypeProperty"/>
	<rdfs:range rdf:resource="http://www.w3.org/2001/XMLSchema#string"/>
	<rdfs:comment>Specifies the format of the archive file.</rdfs:comment>
	<rdfs:isDefinedBy rdf:resource="http://cybox.mitre.org/objects/File"/>
	<rdfs:label>Archive Format</rdfs:label>
</rdf:Description>
<!--  -->
<!-- http://cybox.mitre.org/objects/File#archiveVersion -->

<rdf:Description rdf:about="http://cybox.mitre.org/objects/File#archiveVersion">
	<rdf:type rdf:resource="http://www.w3.org/2002/07/owl#DatatypeProperty"/>
	<rdfs:range rdf:resource="http://www.w3.org/2001/XMLSchema#string"/>
	<rdfs:comment>Specifies the archive type used to create archive file.</rdfs:comment>
	<rdfs:isDefinedBy rdf:resource="http://cybox.mitre.org/objects/File"/>
	<rdfs:label>Archive Version</rdfs:label>
</rdf:Description>
<!--  -->
<!-- http://cybox.mitre.org/objects/File#ascii85DecodeCount.nonObfuscated -->

<rdf:Description rdf:about="http://cybox.mitre.org/objects/File#ascii85DecodeCount.nonObfuscated">
	<rdf:type rdf:resource="http://www.w3.org/2002/07/owl#DatatypeProperty"/>
	<rdfs:range rdf:resource="http://www.w3.org/2001/XMLSchema#nonNegativeInteger"/>
	<rdfs:comment>Specifies the number of non-obfuscated occurrences of the '/ASCII85Decode' keyword in the PDF.</rdfs:comment>
	<rdfs:isDefinedBy rdf:resource="http://cybox.mitre.org/objects/File"/>
	<rdfs:label>'/ASCII85Decode' Non-obfuscated Count</rdfs:label>
</rdf:Description>
<!--  -->
<!-- http://cybox.mitre.org/objects/File#ascii85DecodeCount.obfuscated -->

<rdf:Description rdf:about="http://cybox.mitre.org/objects/File#ascii85DecodeCount.obfuscated">
	<rdf:type rdf:resource="http://www.w3.org/2002/07/owl#DatatypeProperty"/>
	<rdfs:range rdf:resource="http://www.w3.org/2001/XMLSchema#nonNegativeInteger"/>
	<rdfs:comment>Specifies the number of obfuscated occurrences of the '/ASCII85Decode' keyword in the PDF file with some form of obfuscation, such as with hexcodes.</rdfs:comment>
	<rdfs:isDefinedBy rdf:resource="http://cybox.mitre.org/objects/File"/>
	<rdfs:label>'/ASCII8585Decode' Obfuscated Count</rdfs:label>
</rdf:Description>
<!--  -->
<!-- http://cybox.mitre.org/objects/File#asciiHexDecodeCount.nonObfuscated -->

<rdf:Description rdf:about="http://cybox.mitre.org/objects/File#asciiHexDecodeCount.nonObfuscated">
	<rdf:type rdf:resource="http://www.w3.org/2002/07/owl#DatatypeProperty"/>
	<rdfs:range rdf:resource="http://www.w3.org/2001/XMLSchema#nonNegativeInteger"/>
	<rdfs:comment>Specifies the number of non-obfuscated occurrences of the '/ASCIIHexDecode' keyword in the PDF file.</rdfs:comment>
	<rdfs:isDefinedBy rdf:resource="http://cybox.mitre.org/objects/File"/>
	<rdfs:label>'/ASCIIHexDecode' Non-obfuscated Count</rdfs:label>
</rdf:Description>
<!--  -->
<!-- http://cybox.mitre.org/objects/File#asciiHexDecodeCount.obfuscated -->

<rdf:Description rdf:about="http://cybox.mitre.org/objects/File#asciiHexDecodeCount.obfuscated">
	<rdf:type rdf:resource="http://www.w3.org/2002/07/owl#DatatypeProperty"/>
	<rdfs:range rdf:resource="http://www.w3.org/2001/XMLSchema#nonNegativeInteger"/>
	<rdfs:comment>Specifies the number of obfuscated occurrences of the '/ASCIIHexDecode' keyword in the PDF file with some form of obfuscation, such as with hexcodes.</rdfs:comment>
	<rdfs:isDefinedBy rdf:resource="http://cybox.mitre.org/objects/File"/>
	<rdfs:label>pdf metadata.ascii hex decode count obfuscated</rdfs:label>
</rdf:Description>
<!--  -->
<!-- http://cybox.mitre.org/objects/File#attachedDeviceName -->

<rdf:Description rdf:about="http://cybox.mitre.org/objects/File#attachedDeviceName">
	<rdf:type rdf:resource="http://www.w3.org/2002/07/owl#DatatypeProperty"/>
	<rdfs:range rdf:resource="http://www.w3.org/2001/XMLSchema#string"/>
	<rdfs:comment>Specifies the name of another device object that was attached to this one. 

See also: http://msdn.microsoft.com/en-us/library/windows/hardware/ff543147(v=vs.85).aspx.</rdfs:comment>
	<rdfs:isDefinedBy rdf:resource="http://cybox.mitre.org/objects/File"/>
	<rdfs:label>Attached Device Name</rdfs:label>
</rdf:Description>
<!--  -->
<!-- http://cybox.mitre.org/objects/File#attachedDeviceObject -->

<rdf:Description rdf:about="http://cybox.mitre.org/objects/File#attachedDeviceObject">
	<rdf:type rdf:resource="http://www.w3.org/2002/07/owl#DatatypeProperty"/>
	<rdfs:range rdf:resource="http://www.w3.org/2001/XMLSchema#hexBinary"/>
	<rdfs:comment>Specifies a pointer to another device object that was attached to this one. Typically this is a filter driver. 

See also: http://msdn.microsoft.com/en-us/library/windows/hardware/ff543147(v=vs.85).aspx.</rdfs:comment>
	<rdfs:isDefinedBy rdf:resource="http://cybox.mitre.org/objects/File"/>
	<rdfs:label>Attached Device Object</rdfs:label>
</rdf:Description>
<!--  -->
<!-- http://cybox.mitre.org/objects/File#attachedToDeviceName -->

<rdf:Description rdf:about="http://cybox.mitre.org/objects/File#attachedToDeviceName">
	<rdf:type rdf:resource="http://www.w3.org/2002/07/owl#DatatypeProperty"/>
	<rdfs:range rdf:resource="http://www.w3.org/2001/XMLSchema#string"/>
	<rdfs:comment>Specifies the name of another device object that this one was attached to.</rdfs:comment>
	<rdfs:isDefinedBy rdf:resource="http://cybox.mitre.org/objects/File"/>
	<rdfs:label>Attached-To Device Name</rdfs:label>
</rdf:Description>
<!--  -->
<!-- http://cybox.mitre.org/objects/File#attachedToDeviceObject -->

<rdf:Description rdf:about="http://cybox.mitre.org/objects/File#attachedToDeviceObject">
	<rdf:type rdf:resource="http://www.w3.org/2002/07/owl#DatatypeProperty"/>
	<rdfs:range rdf:resource="http://www.w3.org/2001/XMLSchema#hexBinary"/>
	<rdfs:comment>Specifies a pointer to another device object that this one was attached to.</rdfs:comment>
	<rdfs:isDefinedBy rdf:resource="http://cybox.mitre.org/objects/File"/>
	<rdfs:label>Attached-To Device Object</rdfs:label>
</rdf:Description>
<!--  -->
<!-- http://cybox.mitre.org/objects/File#attachedToDriverName -->

<rdf:Description rdf:about="http://cybox.mitre.org/objects/File#attachedToDriverName">
	<rdf:type rdf:resource="http://www.w3.org/2002/07/owl#DatatypeProperty"/>
	<rdfs:range rdf:resource="http://www.w3.org/2001/XMLSchema#string"/>
	<rdfs:comment>Specifies the name of the driver to which this device object was attached.</rdfs:comment>
	<rdfs:isDefinedBy rdf:resource="http://cybox.mitre.org/objects/File"/>
	<rdfs:label>Attached-To Driver Name</rdfs:label>
</rdf:Description>
<!--  -->
<!-- http://cybox.mitre.org/objects/File#attachedToDriverObject -->

<rdf:Description rdf:about="http://cybox.mitre.org/objects/File#attachedToDriverObject">
	<rdf:type rdf:resource="http://www.w3.org/2002/07/owl#DatatypeProperty"/>
	<rdfs:range rdf:resource="http://www.w3.org/2001/XMLSchema#hexBinary"/>
	<rdfs:comment>Specifies a pointer to the driver to which this device object was attached.</rdfs:comment>
	<rdfs:isDefinedBy rdf:resource="http://cybox.mitre.org/objects/File"/>
	<rdfs:label>Attached-To Driver Object</rdfs:label>
</rdf:Description>
<!--  -->
<!-- http://cybox.mitre.org/objects/File#baseRelocationTable.size -->

<rdf:Description rdf:about="http://cybox.mitre.org/objects/File#baseRelocationTable.size">
	<rdf:type rdf:resource="http://www.w3.org/2002/07/owl#DatatypeProperty"/>
	<rdfs:range rdf:resource="http://www.w3.org/2001/XMLSchema#nonNegativeInteger"/>
	<rdfs:comment>specifies the size of the data structure, in bytes, of the base relocation table data directory.</rdfs:comment>
	<rdfs:isDefinedBy rdf:resource="http://cybox.mitre.org/objects/File"/>
	<rdfs:label>Base Relocation Table Size</rdfs:label>
</rdf:Description>
<!--  -->
<!-- http://cybox.mitre.org/objects/File#baseRelocationTable.virtualAddress -->

<rdf:Description rdf:about="http://cybox.mitre.org/objects/File#baseRelocationTable.virtualAddress">
	<rdf:type rdf:resource="http://www.w3.org/2002/07/owl#DatatypeProperty"/>
	<rdfs:range rdf:resource="http://www.w3.org/2001/XMLSchema#hexBinary"/>
	<rdfs:comment>Specifies the relative virtual address (RVA) of the base relocation table data directory.</rdfs:comment>
	<rdfs:isDefinedBy rdf:resource="http://cybox.mitre.org/objects/File"/>
	<rdfs:label>Base Relocation Table Virtual Address</rdfs:label>
</rdf:Description>
<!--  -->
<!-- http://cybox.mitre.org/objects/File#bitsPerPixel -->

<rdf:Description rdf:about="http://cybox.mitre.org/objects/File#bitsPerPixel">
	<rdf:type rdf:resource="http://www.w3.org/2002/07/owl#DatatypeProperty"/>
	<rdfs:range rdf:resource="http://www.w3.org/2001/XMLSchema#positiveInteger"/>
	<rdfs:comment>Specifies the sum of bits used for each color channel in the image in the image file, and thus the total number of pixels used for expressing the color depth of the image.</rdfs:comment>
	<rdfs:isDefinedBy rdf:resource="http://cybox.mitre.org/objects/File"/>
	<rdfs:label>Bits per Pixel</rdfs:label>
</rdf:Description>
<!--  -->
<!-- http://cybox.mitre.org/objects/File#bound -->

<rdf:Description rdf:about="http://cybox.mitre.org/objects/File#bound">
	<rdf:type rdf:resource="http://www.w3.org/2002/07/owl#DatatypeProperty"/>
	<rdfs:range rdf:resource="http://www.w3.org/2001/XMLSchema#hexBinary"/>
	<rdfs:comment>Specifies the precomputed address if the imported function is bound.</rdfs:comment>
	<rdfs:isDefinedBy rdf:resource="http://cybox.mitre.org/objects/File"/>
	<rdfs:label>Bound</rdfs:label>
</rdf:Description>
<!--  -->
<!-- http://cybox.mitre.org/objects/File#boundImport.size -->

<rdf:Description rdf:about="http://cybox.mitre.org/objects/File#boundImport.size">
	<rdf:type rdf:resource="http://www.w3.org/2002/07/owl#DatatypeProperty"/>
	<rdfs:range rdf:resource="http://www.w3.org/2001/XMLSchema#nonNegativeInteger"/>
	<rdfs:comment>Specifies the size of the data structure, in bytes, of the Bound Import data directory.</rdfs:comment>
	<rdfs:isDefinedBy rdf:resource="http://cybox.mitre.org/objects/File"/>
	<rdfs:label>Bound Import Size</rdfs:label>
</rdf:Description>
<!--  -->
<!-- http://cybox.mitre.org/objects/File#boundImport.virtualAddress -->

<rdf:Description rdf:about="http://cybox.mitre.org/objects/File#boundImport.virtualAddress">
	<rdf:type rdf:resource="http://www.w3.org/2002/07/owl#DatatypeProperty"/>
	<rdfs:range rdf:resource="http://www.w3.org/2001/XMLSchema#hexBinary"/>
	<rdfs:comment>Specifies the relative virtual address (RVA) of the Bound Import data directory.</rdfs:comment>
	<rdfs:isDefinedBy rdf:resource="http://cybox.mitre.org/objects/File"/>
	<rdfs:label>Bound Import Virtual Address</rdfs:label>
</rdf:Description>
<!--  -->
<!-- http://cybox.mitre.org/objects/File#buildInfo.compilerName -->

<rdf:Description rdf:about="http://cybox.mitre.org/objects/File#buildInfo.compilerName">
	<rdf:type rdf:resource="http://www.w3.org/2002/07/owl#DatatypeProperty"/>
	<rdfs:range rdf:resource="http://www.w3.org/2001/XMLSchema#string"/>
	<rdfs:comment>Specifies the name of the compiler used to compile the binary.</rdfs:comment>
	<rdfs:isDefinedBy rdf:resource="http://cybox.mitre.org/objects/File"/>
	<rdfs:label>Compiler Name</rdfs:label>
</rdf:Description>
<!--  -->
<!-- http://cybox.mitre.org/objects/File#buildInfo.compilerVersion -->

<rdf:Description rdf:about="http://cybox.mitre.org/objects/File#buildInfo.compilerVersion">
	<rdf:type rdf:resource="http://www.w3.org/2002/07/owl#DatatypeProperty"/>
	<rdfs:range rdf:resource="http://www.w3.org/2001/XMLSchema#string"/>
	<rdfs:comment>Specifies the version of the compiler used to compile the binary.</rdfs:comment>
	<rdfs:isDefinedBy rdf:resource="http://cybox.mitre.org/objects/File"/>
	<rdfs:label>Compiler Version</rdfs:label>
</rdf:Description>
<!--  -->
<!-- http://cybox.mitre.org/objects/File#buildInfo.linkerName -->

<rdf:Description rdf:about="http://cybox.mitre.org/objects/File#buildInfo.linkerName">
	<rdf:type rdf:resource="http://www.w3.org/2002/07/owl#DatatypeProperty"/>
	<rdfs:range rdf:resource="http://www.w3.org/2001/XMLSchema#string"/>
	<rdfs:comment>Specifies the name of the linker used to link the PE binary.</rdfs:comment>
	<rdfs:isDefinedBy rdf:resource="http://cybox.mitre.org/objects/File"/>
	<rdfs:label>Linker Name</rdfs:label>
</rdf:Description>
<!--  -->
<!-- http://cybox.mitre.org/objects/File#buildInfo.linkerVersion -->

<rdf:Description rdf:about="http://cybox.mitre.org/objects/File#buildInfo.linkerVersion">
	<rdf:type rdf:resource="http://www.w3.org/2002/07/owl#DatatypeProperty"/>
	<rdfs:range rdf:resource="http://www.w3.org/2001/XMLSchema#string"/>
	<rdfs:comment>Specifies the version of the linker used to link the PE binary.</rdfs:comment>
	<rdfs:isDefinedBy rdf:resource="http://cybox.mitre.org/objects/File"/>
	<rdfs:label>Linker Version</rdfs:label>
</rdf:Description>
<!--  -->
<!-- http://cybox.mitre.org/objects/File#byteOffset -->

<rdf:Description rdf:about="http://cybox.mitre.org/objects/File#byteOffset">
	<rdf:type rdf:resource="http://www.w3.org/2002/07/owl#DatatypeProperty"/>
	<rdfs:range rdf:resource="http://www.w3.org/2001/XMLSchema#integer"/>
	<rdfs:comment>Specifies the 10-digit number, padded with leading zeros if necessary, that specifies the number of bytes from the beginning of the file to the beginning of the object.</rdfs:comment>
	<rdfs:isDefinedBy rdf:resource="http://cybox.mitre.org/objects/File"/>
	<rdfs:label>Byte Offset</rdfs:label>
</rdf:Description>
<!--  -->
<!-- http://cybox.mitre.org/objects/File#ccittFaxDecodeCount.nonObfuscated -->

<rdf:Description rdf:about="http://cybox.mitre.org/objects/File#ccittFaxDecodeCount.nonObfuscated">
	<rdf:type rdf:resource="http://www.w3.org/2002/07/owl#DatatypeProperty"/>
	<rdfs:range rdf:resource="http://www.w3.org/2001/XMLSchema#nonNegativeInteger"/>
	<rdfs:comment>Specifies the number of non-obfuscated occurrences of the '/CCITTFaxDecode' keyword in the PDF file.</rdfs:comment>
	<rdfs:isDefinedBy rdf:resource="http://cybox.mitre.org/objects/File"/>
	<rdfs:label>'/CCITTFaxDecode' Non-obfuscated Count</rdfs:label>
</rdf:Description>
<!--  -->
<!-- http://cybox.mitre.org/objects/File#ccittFaxDecodeCount.obfuscated -->

<rdf:Description rdf:about="http://cybox.mitre.org/objects/File#ccittFaxDecodeCount.obfuscated">
	<rdf:type rdf:resource="http://www.w3.org/2002/07/owl#DatatypeProperty"/>
	<rdfs:range rdf:resource="http://www.w3.org/2001/XMLSchema#nonNegativeInteger"/>
	<rdfs:comment>Specifies the number of obfuscated occurrences of the '/CCITTFaxDecode' keyword in the PDF file with some form of obfuscation, such as with hexcodes.</rdfs:comment>
	<rdfs:isDefinedBy rdf:resource="http://cybox.mitre.org/objects/File"/>
	<rdfs:label>'/CCITTFaxDecode' Obfuscated Count</rdfs:label>
</rdf:Description>
<!--  -->
<!-- http://cybox.mitre.org/objects/File#certificateTable.size -->

<rdf:Description rdf:about="http://cybox.mitre.org/objects/File#certificateTable.size">
	<rdf:type rdf:resource="http://www.w3.org/2002/07/owl#DatatypeProperty"/>
	<rdfs:range rdf:resource="http://www.w3.org/2001/XMLSchema#nonNegativeInteger"/>
	<rdfs:comment>Specifies the size of the data structure, in bytes, of the Certificate Table data directory.</rdfs:comment>
	<rdfs:isDefinedBy rdf:resource="http://cybox.mitre.org/objects/File"/>
	<rdfs:label>Certificate Table Size</rdfs:label>
</rdf:Description>
<!--  -->
<!-- http://cybox.mitre.org/objects/File#certificateTable.virtualAddress -->

<rdf:Description rdf:about="http://cybox.mitre.org/objects/File#certificateTable.virtualAddress">
	<rdf:type rdf:resource="http://www.w3.org/2002/07/owl#DatatypeProperty"/>
	<rdfs:range rdf:resource="http://www.w3.org/2001/XMLSchema#hexBinary"/>
	<rdfs:comment>Specifies the relative virtual address (RVA) of the ertificate table data directory.</rdfs:comment>
	<rdfs:isDefinedBy rdf:resource="http://cybox.mitre.org/objects/File"/>
	<rdfs:label>CertificateTable. Vrtual Address</rdfs:label>
</rdf:Description>
<!--  -->
<!-- http://cybox.mitre.org/objects/File#clrRuntimeHeader.size -->

<rdf:Description rdf:about="http://cybox.mitre.org/objects/File#clrRuntimeHeader.size">
	<rdf:type rdf:resource="http://www.w3.org/2002/07/owl#DatatypeProperty"/>
	<rdfs:range rdf:resource="http://www.w3.org/2001/XMLSchema#nonNegativeInteger"/>
	<rdfs:comment>Specifies the size of the data structure, in bytes, of the Common Language Runtine (CLR) Runtime Header data directory.</rdfs:comment>
	<rdfs:isDefinedBy rdf:resource="http://cybox.mitre.org/objects/File"/>
	<rdfs:label>Common Language Runtime (CLR) Runtime Header Size</rdfs:label>
</rdf:Description>
<!--  -->
<!-- http://cybox.mitre.org/objects/File#clrRuntimeHeader.virtualAddress -->

<rdf:Description rdf:about="http://cybox.mitre.org/objects/File#clrRuntimeHeader.virtualAddress">
	<rdf:type rdf:resource="http://www.w3.org/2002/07/owl#DatatypeProperty"/>
	<rdfs:range rdf:resource="http://www.w3.org/2001/XMLSchema#hexBinary"/>
	<rdfs:comment>Specifies the relative virtual address (RVA) of the Common Language Runtime (CLR) Runtime header.</rdfs:comment>
	<rdfs:isDefinedBy rdf:resource="http://cybox.mitre.org/objects/File"/>
	<rdfs:label>Common Language Runtime (CLR) Runtime Header Virtual Address</rdfs:label>
</rdf:Description>
<!--  -->
<!-- http://cybox.mitre.org/objects/File#comments -->

<rdf:Description rdf:about="http://cybox.mitre.org/objects/File#comments">
	<rdf:type rdf:resource="http://www.w3.org/2002/07/owl#DatatypeProperty"/>
	<rdfs:range rdf:resource="http://www.w3.org/2001/XMLSchema#string"/>
	<rdfs:comment>Specifies any additional information that should be displayed for diagnostic purposes.</rdfs:comment>
	<rdfs:isDefinedBy rdf:resource="http://cybox.mitre.org/objects/File"/>
	<rdfs:label>Comments</rdfs:label>
</rdf:Description>
<!--  -->
<!-- http://cybox.mitre.org/objects/File#companyName -->

<rdf:Description rdf:about="http://cybox.mitre.org/objects/File#companyName">
	<rdf:type rdf:resource="http://www.w3.org/2002/07/owl#DatatypeProperty"/>
	<rdfs:range rdf:resource="http://www.w3.org/2001/XMLSchema#string"/>
	<rdfs:comment>Specifies the company that produced the file - for example, "Microsoft Corporation" or "Standard Microsystems Corporation, Inc.".</rdfs:comment>
	<rdfs:isDefinedBy rdf:resource="http://cybox.mitre.org/objects/File"/>
	<rdfs:label>Company Name</rdfs:label>
</rdf:Description>
<!--  -->
<!-- http://cybox.mitre.org/objects/File#compressed -->

<rdf:Description rdf:about="http://cybox.mitre.org/objects/File#compressed">
	<rdf:type rdf:resource="http://www.w3.org/2002/07/owl#DatatypeProperty"/>
	<rdfs:range rdf:resource="http://www.w3.org/2001/XMLSchema#boolean"/>
	<rdfs:comment>Specifies a file or directory that is compressed, as denoted by the constant value, 0x800. For a file, all of the data in the file is compressed. For a directory, compression is the default for newly created files and subdirectories.</rdfs:comment>
	<rdfs:isDefinedBy rdf:resource="http://cybox.mitre.org/objects/File"/>
	<rdfs:label>Compressed</rdfs:label>
</rdf:Description>
<!--  -->
<!-- http://cybox.mitre.org/objects/File#compressionAlgorithm -->

<rdf:Description rdf:about="http://cybox.mitre.org/objects/File#compressionAlgorithm">
	<rdf:type rdf:resource="http://www.w3.org/2002/07/owl#DatatypeProperty"/>
	<rdfs:range rdf:resource="http://www.w3.org/2001/XMLSchema#string"/>
	<rdfs:comment>Specifies the name of the compression algorithm used to compress the image, if applicable. &#xD;
&#xD;
Note that for many popular image formats, such as JPEG, the compression algorithm is inherent to the file format and so does need to be captured here as long as the format itself is identified in the Image File Format field.</rdfs:comment>
	<rdfs:isDefinedBy rdf:resource="http://cybox.mitre.org/objects/File"/>
	<rdfs:label>Compression Algorithm</rdfs:label>
</rdf:Description>
<!--  -->
<!-- http://cybox.mitre.org/objects/File#compressionComment -->

<rdf:Description rdf:about="http://cybox.mitre.org/objects/File#compressionComment">
	<rdf:type rdf:resource="http://www.w3.org/2002/07/owl#DatatypeProperty"/>
	<rdfs:range rdf:resource="http://www.w3.org/2001/XMLSchema#string"/>
	<rdfs:comment>Specifies the comment string associated with the compressed file.</rdfs:comment>
	<rdfs:isDefinedBy rdf:datatype="http://www.w3.org/2001/XMLSchema#string">&lt;http://cybox.mitre.org/objects/File&gt;</rdfs:isDefinedBy>
	<rdfs:label>Compression Comment</rdfs:label>
</rdf:Description>
<!--  -->
<!-- http://cybox.mitre.org/objects/File#compressionMethod -->

<rdf:Description rdf:about="http://cybox.mitre.org/objects/File#compressionMethod">
	<rdf:type rdf:resource="http://www.w3.org/2002/07/owl#DatatypeProperty"/>
	<rdfs:range rdf:resource="http://www.w3.org/2001/XMLSchema#string"/>
	<rdfs:comment>Specifies the method used to compress the file.</rdfs:comment>
	<rdfs:isDefinedBy rdf:resource="http://cybox.mitre.org/objects/File"/>
	<rdfs:label>Compression Method</rdfs:label>
</rdf:Description>
<!--  -->
<!-- http://cybox.mitre.org/objects/File#compressionVersion -->

<rdf:Description rdf:about="http://cybox.mitre.org/objects/File#compressionVersion">
	<rdf:type rdf:resource="http://www.w3.org/2002/07/owl#DatatypeProperty"/>
	<rdfs:range rdf:resource="http://www.w3.org/2001/XMLSchema#string"/>
	<rdfs:comment>Specifies the version of the compression method used to compress the file.</rdfs:comment>
	<rdfs:isDefinedBy rdf:datatype="http://www.w3.org/2001/XMLSchema#string">&lt;http://cybox.mitre.org/objects/File&gt;</rdfs:isDefinedBy>
	<rdfs:label>Compression Version</rdfs:label>
</rdf:Description>
<!--  -->
<!-- http://cybox.mitre.org/objects/File#createdDateTime -->

<rdf:Description rdf:about="http://cybox.mitre.org/objects/File#createdDateTime">
	<rdf:type rdf:resource="http://www.w3.org/2002/07/owl#DatatypeProperty"/>
	<rdfs:range rdf:resource="http://www.w3.org/2001/XMLSchema#dateTime"/>
	<rdfs:comment>Specifies the date/time the file was created.</rdfs:comment>
	<rdfs:isDefinedBy rdf:datatype="http://www.w3.org/2001/XMLSchema#string">&lt;http://cybox.mitre.org/objects/File&gt;</rdfs:isDefinedBy>
	<rdfs:label>Created Time</rdfs:label>
</rdf:Description>
<!--  -->
<!-- http://cybox.mitre.org/objects/File#dataHash.value -->

<rdf:Description rdf:about="http://cybox.mitre.org/objects/File#dataHash.value">
	<rdf:type rdf:resource="http://www.w3.org/2002/07/owl#DatatypeProperty"/>
	<rdfs:range rdf:resource="http://www.w3.org/2001/XMLSchema#string"/>
	<rdfs:comment>Specifies the values, in the format of 'hash-type':'hash-value', for any hash computed using the data contained in the specified PE binary section as input.</rdfs:comment>
	<rdfs:isDefinedBy rdf:resource="http://cybox.mitre.org/objects/File"/>
	<rdfs:label>Data Hash Value</rdfs:label>
</rdf:Description>
<!--  -->
<!-- http://cybox.mitre.org/objects/File#dctDecodeCount.nonObfuscated -->

<rdf:Description rdf:about="http://cybox.mitre.org/objects/File#dctDecodeCount.nonObfuscated">
	<rdf:type rdf:resource="http://www.w3.org/2002/07/owl#DatatypeProperty"/>
	<rdfs:range rdf:resource="http://www.w3.org/2001/XMLSchema#nonNegativeInteger"/>
	<rdfs:comment>Specifies the number of non-obfuscated occurrences of the '/DCTDecode' keyword in the PDF file.</rdfs:comment>
	<rdfs:isDefinedBy rdf:resource="http://cybox.mitre.org/objects/File"/>
	<rdfs:label>'/DCTDecode' Non-Obfuscated Count</rdfs:label>
</rdf:Description>
<!--  -->
<!-- http://cybox.mitre.org/objects/File#dctDecodeCount.obfuscated -->

<rdf:Description rdf:about="http://cybox.mitre.org/objects/File#dctDecodeCount.obfuscated">
	<rdf:type rdf:resource="http://www.w3.org/2002/07/owl#DatatypeProperty"/>
	<rdfs:range rdf:resource="http://www.w3.org/2001/XMLSchema#nonNegativeInteger"/>
	<rdfs:comment>Specifies the number of obfuscated occurrences of the '/DCTDecode' keyword in the PDF file with some form of obfuscation, such as with hexcodes.</rdfs:comment>
	<rdfs:isDefinedBy rdf:resource="http://cybox.mitre.org/objects/File"/>
	<rdfs:label>'/DCTDecode' Obfuscated Count</rdfs:label>
</rdf:Description>
<!--  -->
<!-- http://cybox.mitre.org/objects/File#debug.size -->

<rdf:Description rdf:about="http://cybox.mitre.org/objects/File#debug.size">
	<rdf:type rdf:resource="http://www.w3.org/2002/07/owl#DatatypeProperty"/>
	<rdfs:range rdf:resource="http://www.w3.org/2001/XMLSchema#nonNegativeInteger"/>
	<rdfs:comment>Specifies the size of the data structure, in bytes, of  the debug data directory.</rdfs:comment>
	<rdfs:isDefinedBy rdf:resource="http://cybox.mitre.org/objects/File"/>
	<rdfs:label>Debug Size</rdfs:label>
</rdf:Description>
<!--  -->
<!-- http://cybox.mitre.org/objects/File#debug.virtualAddress -->

<rdf:Description rdf:about="http://cybox.mitre.org/objects/File#debug.virtualAddress">
	<rdf:type rdf:resource="http://www.w3.org/2002/07/owl#DatatypeProperty"/>
	<rdfs:range rdf:resource="http://www.w3.org/2001/XMLSchema#hexBinary"/>
	<rdfs:comment>Specifies the relative virtual address (RVA) of the debug data directory.</rdfs:comment>
	<rdfs:isDefinedBy rdf:resource="http://cybox.mitre.org/objects/File"/>
	<rdfs:label>Debug Virtual Address</rdfs:label>
</rdf:Description>
<!--  -->
<!-- http://cybox.mitre.org/objects/File#decodedStream -->

<rdf:Description rdf:about="http://cybox.mitre.org/objects/File#decodedStream">
	<rdf:type rdf:resource="http://www.w3.org/2002/07/owl#DatatypeProperty"/>
	<rdfs:range rdf:resource="http://www.w3.org/2001/XMLSchema#hexBinary"/>
	<rdfs:comment>Specifies the decoded stream (i.e., after undoing the specified filters in the correct order) as a hex string.</rdfs:comment>
	<rdfs:isDefinedBy rdf:resource="http://cybox.mitre.org/objects/File"/>
	<rdfs:label>Decoded Stream</rdfs:label>
</rdf:Description>
<!--  -->
<!-- http://cybox.mitre.org/objects/File#decodedStreamHashValues -->

<rdf:Description rdf:about="http://cybox.mitre.org/objects/File#decodedStreamHashValues">
	<rdf:type rdf:resource="http://www.w3.org/2002/07/owl#DatatypeProperty"/>
	<rdfs:range rdf:resource="http://www.w3.org/2001/XMLSchema#string"/>
	<rdfs:comment>Specifies the values, in the format of 'hash-type':'hash-value', for any hash computed of the decoded stream.</rdfs:comment>
	<rdfs:isDefinedBy rdf:resource="http://cybox.mitre.org/objects/File"/>
	<rdfs:label>Decode Stream Hash Values</rdfs:label>
</rdf:Description>
<!--  -->
<!-- http://cybox.mitre.org/objects/File#decryptionKey -->

<rdf:Description rdf:about="http://cybox.mitre.org/objects/File#decryptionKey">
	<rdf:type rdf:resource="http://www.w3.org/2002/07/owl#DatatypeProperty"/>
	<rdfs:range rdf:resource="http://www.w3.org/2001/XMLSchema#string"/>
	<rdfs:comment>Specifies the key used to decrypt the file.</rdfs:comment>
	<rdfs:isDefinedBy rdf:datatype="http://www.w3.org/2001/XMLSchema#string">&lt;http://cybox.mitre.org/objects/File&gt;</rdfs:isDefinedBy>
	<rdfs:label>Decryption Key</rdfs:label>
</rdf:Description>
<!--  -->
<!-- http://cybox.mitre.org/objects/File#delayImportDescriptor.size -->

<rdf:Description rdf:about="http://cybox.mitre.org/objects/File#delayImportDescriptor.size">
	<rdf:type rdf:resource="http://www.w3.org/2002/07/owl#DatatypeProperty"/>
	<rdfs:range rdf:resource="http://www.w3.org/2001/XMLSchema#nonNegativeInteger"/>
	<rdfs:comment>Specifies the size of the data structure, in bytes, of the Delay Import Descriptor data directory.</rdfs:comment>
	<rdfs:isDefinedBy rdf:resource="http://cybox.mitre.org/objects/File"/>
	<rdfs:label>Delay Import Descriptor Size</rdfs:label>
</rdf:Description>
<!--  -->
<!-- http://cybox.mitre.org/objects/File#delayImportDescriptor.virtualAddress -->

<rdf:Description rdf:about="http://cybox.mitre.org/objects/File#delayImportDescriptor.virtualAddress">
	<rdf:type rdf:resource="http://www.w3.org/2002/07/owl#DatatypeProperty"/>
	<rdfs:range rdf:resource="http://www.w3.org/2001/XMLSchema#hexBinary"/>
	<rdfs:comment>Specifies the size of the data structure, in byte, the Delay Import Descriptor data directory.</rdfs:comment>
	<rdfs:isDefinedBy rdf:resource="http://cybox.mitre.org/objects/File"/>
	<rdfs:label>Delay Import Descriptor Virtual Address</rdfs:label>
</rdf:Description>
<!--  -->
<!-- http://cybox.mitre.org/objects/File#delayLoad -->

<rdf:Description rdf:about="http://cybox.mitre.org/objects/File#delayLoad">
	<rdf:type rdf:resource="http://www.w3.org/2002/07/owl#DatatypeProperty"/>
	<rdfs:range rdf:resource="http://www.w3.org/2001/XMLSchema#boolean"/>
	<rdfs:comment></rdfs:comment>
	<rdfs:isDefinedBy rdf:datatype="http://www.w3.org/2001/XMLSchema#string">&lt;http://cybox.mitre.org/objects/File&gt;</rdfs:isDefinedBy>
	<rdfs:label>delay load</rdfs:label>
</rdf:Description>
<!--  -->
<!-- http://cybox.mitre.org/objects/File#deleted -->

<rdf:Description rdf:about="http://cybox.mitre.org/objects/File#deleted">
	<rdf:type rdf:resource="http://www.w3.org/2002/07/owl#DatatypeProperty"/>
	<rdfs:range rdf:resource="http://www.w3.org/2001/XMLSchema#boolean"/>
	<rdfs:comment>Specifies a file or directory that is marked as deleted.</rdfs:comment>
	<rdfs:isDefinedBy rdf:resource="http://cybox.mitre.org/objects/File"/>
	<rdfs:label>Deleted</rdfs:label>
</rdf:Description>
<!--  -->
<!-- http://cybox.mitre.org/objects/File#device -->

<rdf:Description rdf:about="http://cybox.mitre.org/objects/File#device">
	<rdf:type rdf:resource="http://www.w3.org/2002/07/owl#DatatypeProperty"/>
	<rdfs:range rdf:resource="http://www.w3.org/2001/XMLSchema#boolean"/>
	<rdfs:comment>Specifies a reserved system value, as denoted by the constant value, 0x40.</rdfs:comment>
	<rdfs:isDefinedBy rdf:resource="http://cybox.mitre.org/objects/File"/>
	<rdfs:label>Device</rdfs:label>
</rdf:Description>
<!--  -->
<!-- http://cybox.mitre.org/objects/File#deviceName -->

<rdf:Description rdf:about="http://cybox.mitre.org/objects/File#deviceName">
	<rdf:type rdf:resource="http://www.w3.org/2002/07/owl#DatatypeProperty"/>
	<rdfs:range rdf:resource="http://www.w3.org/2001/XMLSchema#string"/>
	<rdfs:comment>Specifies the name of the device object.</rdfs:comment>
	<rdfs:isDefinedBy rdf:resource="http://cybox.mitre.org/objects/File"/>
	<rdfs:label>Device Name</rdfs:label>
</rdf:Description>
<!--  -->
<!-- http://cybox.mitre.org/objects/File#deviceObject -->

<rdf:Description rdf:about="http://cybox.mitre.org/objects/File#deviceObject">
	<rdf:type rdf:resource="http://www.w3.org/2002/07/owl#DatatypeProperty"/>
	<rdfs:range rdf:resource="http://www.w3.org/2001/XMLSchema#hexBinary"/>
	<rdfs:comment>Specifies a pointer to the driver object for the caller.</rdfs:comment>
	<rdfs:isDefinedBy rdf:resource="http://cybox.mitre.org/objects/File"/>
	<rdfs:label>Device Object</rdfs:label>
</rdf:Description>
<!--  -->
<!-- http://cybox.mitre.org/objects/File#devicePath -->

<rdf:Description rdf:about="http://cybox.mitre.org/objects/File#devicePath">
	<rdf:type rdf:resource="http://www.w3.org/2002/07/owl#DatatypeProperty"/>
	<rdfs:range rdf:resource="http://www.w3.org/2001/XMLSchema#string"/>
	<rdfs:comment>Specifies the path to the physical device where the file system containing the file resides.</rdfs:comment>
	<rdfs:isDefinedBy rdf:datatype="http://www.w3.org/2001/XMLSchema#string">&lt;http://cybox.mitre.org/objects/File&gt;</rdfs:isDefinedBy>
	<rdfs:label>Device Path</rdfs:label>
</rdf:Description>
<!--  -->
<!-- http://cybox.mitre.org/objects/File#directory -->

<rdf:Description rdf:about="http://cybox.mitre.org/objects/File#directory">
	<rdf:type rdf:resource="http://www.w3.org/2002/07/owl#DatatypeProperty"/>
	<rdfs:range rdf:resource="http://www.w3.org/2001/XMLSchema#boolean"/>
	<rdfs:comment>Specifies a directory, as denoted by the constant value, 0x10.</rdfs:comment>
	<rdfs:isDefinedBy rdf:resource="http://cybox.mitre.org/objects/File"/>
	<rdfs:label>Directory</rdfs:label>
</rdf:Description>
<!--  -->
<!-- http://cybox.mitre.org/objects/File#docInfo.authorName -->

<rdf:Description rdf:about="http://cybox.mitre.org/objects/File#docInfo.authorName">
	<rdf:type rdf:resource="http://www.w3.org/2002/07/owl#DatatypeProperty"/>
	<rdfs:range rdf:resource="http://www.w3.org/2001/XMLSchema#string"/>
	<rdfs:comment>Specifies the name of the person who created the PDF document.</rdfs:comment>
	<rdfs:isDefinedBy rdf:resource="http://cybox.mitre.org/objects/File"/>
	<rdfs:label>Documentation Author Name</rdfs:label>
</rdf:Description>
<!--  -->
<!-- http://cybox.mitre.org/objects/File#docInfo.creationDate -->

<rdf:Description rdf:about="http://cybox.mitre.org/objects/File#docInfo.creationDate">
	<rdf:type rdf:resource="http://www.w3.org/2002/07/owl#DatatypeProperty"/>
	<rdfs:range rdf:resource="http://www.w3.org/2001/XMLSchema#dateTime"/>
	<rdfs:comment>Specifies the date and time that the document was created.</rdfs:comment>
	<rdfs:isDefinedBy rdf:resource="http://cybox.mitre.org/objects/File"/>
	<rdfs:label>Creation Date</rdfs:label>
</rdf:Description>
<!--  -->
<!-- http://cybox.mitre.org/objects/File#docInfo.creatorAppName -->

<rdf:Description rdf:about="http://cybox.mitre.org/objects/File#docInfo.creatorAppName">
	<rdf:type rdf:resource="http://www.w3.org/2002/07/owl#DatatypeProperty"/>
	<rdfs:range rdf:resource="http://www.w3.org/2001/XMLSchema#string"/>
	<rdfs:comment>Specifies the name of the application that created the original document, for cases where the original document was then converted to PDF.</rdfs:comment>
	<rdfs:isDefinedBy rdf:resource="http://cybox.mitre.org/objects/File"/>
	<rdfs:label>Creation Application Name</rdfs:label>
</rdf:Description>
<!--  -->
<!-- http://cybox.mitre.org/objects/File#docInfo.keywords -->

<rdf:Description rdf:about="http://cybox.mitre.org/objects/File#docInfo.keywords">
	<rdf:type rdf:resource="http://www.w3.org/2002/07/owl#DatatypeProperty"/>
	<rdfs:range rdf:resource="http://www.w3.org/2001/XMLSchema#string"/>
	<rdfs:comment>Specifies the keywords associated with the PDF document.</rdfs:comment>
	<rdfs:isDefinedBy rdf:resource="http://cybox.mitre.org/objects/File"/>
	<rdfs:label>document information.keywords</rdfs:label>
</rdf:Description>
<!--  -->
<!-- http://cybox.mitre.org/objects/File#docInfo.modificationDate -->

<rdf:Description rdf:about="http://cybox.mitre.org/objects/File#docInfo.modificationDate">
	<rdf:type rdf:resource="http://www.w3.org/2002/07/owl#DatatypeProperty"/>
	<rdfs:range rdf:resource="http://www.w3.org/2001/XMLSchema#dateTime"/>
	<rdfs:comment>Specifies the date and time that the document was most recently modified.</rdfs:comment>
	<rdfs:isDefinedBy rdf:resource="http://cybox.mitre.org/objects/File"/>
	<rdfs:label>PDF Modification Date</rdfs:label>
</rdf:Description>
<!--  -->
<!-- http://cybox.mitre.org/objects/File#docInfo.producerAppName -->

<rdf:Description rdf:about="http://cybox.mitre.org/objects/File#docInfo.producerAppName">
	<rdf:type rdf:resource="http://www.w3.org/2002/07/owl#DatatypeProperty"/>
	<rdfs:range rdf:resource="http://www.w3.org/2001/XMLSchema#string"/>
	<rdfs:comment>Specifies the name of the application that converted the document to PDF, for cases where the original document was then converted to PDF.</rdfs:comment>
	<rdfs:isDefinedBy rdf:resource="http://cybox.mitre.org/objects/File"/>
	<rdfs:label>Producer Application Name</rdfs:label>
</rdf:Description>
<!--  -->
<!-- http://cybox.mitre.org/objects/File#docInfo.subject -->

<rdf:Description rdf:about="http://cybox.mitre.org/objects/File#docInfo.subject">
	<rdf:type rdf:resource="http://www.w3.org/2002/07/owl#DatatypeProperty"/>
	<rdfs:range rdf:resource="http://www.w3.org/2001/XMLSchema#string"/>
	<rdfs:comment>Specifies the subject of the PDF document.</rdfs:comment>
	<rdfs:isDefinedBy rdf:resource="http://cybox.mitre.org/objects/File"/>
	<rdfs:label>Document Subject</rdfs:label>
</rdf:Description>
<!--  -->
<!-- http://cybox.mitre.org/objects/File#docInfo.title -->

<rdf:Description rdf:about="http://cybox.mitre.org/objects/File#docInfo.title">
	<rdf:type rdf:resource="http://www.w3.org/2002/07/owl#DatatypeProperty"/>
	<rdfs:range rdf:resource="http://www.w3.org/2001/XMLSchema#string"/>
	<rdfs:comment>Specifies the title of the PDF document.</rdfs:comment>
	<rdfs:isDefinedBy rdf:resource="http://cybox.mitre.org/objects/File"/>
	<rdfs:label>Document Title</rdfs:label>
</rdf:Description>
<!--  -->
<!-- http://cybox.mitre.org/objects/File#docInfo.trapped -->

<rdf:Description rdf:about="http://cybox.mitre.org/objects/File#docInfo.trapped">
	<rdf:type rdf:resource="http://www.w3.org/2002/07/owl#DatatypeProperty"/>
	<rdfs:range rdf:resource="http://www.w3.org/2001/XMLSchema#string"/>
	<rdfs:comment>Specifies  a name object indicating whether the document has been modified to included trapping information.</rdfs:comment>
	<rdfs:isDefinedBy rdf:resource="http://cybox.mitre.org/objects/File"/>
	<rdfs:label>Trapping Name</rdfs:label>
</rdf:Description>
<!--  -->
<!-- http://cybox.mitre.org/objects/File#dosHeader.e_cblp -->

<rdf:Description rdf:about="http://cybox.mitre.org/objects/File#dosHeader.e_cblp">
	<rdf:type rdf:resource="http://www.w3.org/2002/07/owl#DatatypeProperty"/>
	<rdfs:range rdf:resource="http://www.w3.org/2001/XMLSchema#hexBinary"/>
	<rdfs:comment>Specifies the number of bytes actually used in the last page, with the special case of a full page being represented by a value of zero (since the last page is never empty). For example, assuming a page size of 512 bytes, this value would be 0x0000 for a 1024 byte file, and 0x0001 for a 1025 byte file (since it only contains one valid byte).</rdfs:comment>
	<rdfs:isDefinedBy rdf:resource="http://cybox.mitre.org/objects/File"/>
	<rdfs:label>DOS Header e_cblp</rdfs:label>
</rdf:Description>
<!--  -->
<!-- http://cybox.mitre.org/objects/File#dosHeader.e_cp -->

<rdf:Description rdf:about="http://cybox.mitre.org/objects/File#dosHeader.e_cp">
	<rdf:type rdf:resource="http://www.w3.org/2002/07/owl#DatatypeProperty"/>
	<rdfs:range rdf:resource="http://www.w3.org/2001/XMLSchema#hexBinary"/>
	<rdfs:comment>Specifies the number of pages required to hold the file. &#xD;
&#xD;
For example, if the file contains 1024 bytes, and we assume the file has pages of a size of 512 bytes, this word would contain 0x0002; if the file contains 1025 bytes, this word would contain 0x0003.</rdfs:comment>
	<rdfs:isDefinedBy rdf:resource="http://cybox.mitre.org/objects/File"/>
	<rdfs:label>DOS Header e_cp</rdfs:label>
</rdf:Description>
<!--  -->
<!-- http://cybox.mitre.org/objects/File#dosHeader.e_cparhdr -->

<rdf:Description rdf:about="http://cybox.mitre.org/objects/File#dosHeader.e_cparhdr">
	<rdf:type rdf:resource="http://www.w3.org/2002/07/owl#DatatypeProperty"/>
	<rdfs:range rdf:resource="http://www.w3.org/2001/XMLSchema#hexBinary"/>
	<rdfs:comment>Specifies the size of the executable header in terms of paragraphs (16 byte chunks). It indicates the offset of the program's compiled/assembled and linked image (the load module) within the executable file. The size of the load module can be deduced by subtracting this value (converted to bytes) from the overall file size derived from combining the e_cp (number of file pages) and e_cblp (number of bytes in last page) values. The header always spans an even number of paragraphs.</rdfs:comment>
	<rdfs:isDefinedBy rdf:resource="http://cybox.mitre.org/objects/File"/>
	<rdfs:label>DOS Header e_cparhdr</rdfs:label>
</rdf:Description>
<!--  -->
<!-- http://cybox.mitre.org/objects/File#dosHeader.e_crlc -->

<rdf:Description rdf:about="http://cybox.mitre.org/objects/File#dosHeader.e_crlc">
	<rdf:type rdf:resource="http://www.w3.org/2002/07/owl#DatatypeProperty"/>
	<rdfs:range rdf:resource="http://www.w3.org/2001/XMLSchema#hexBinary"/>
	<rdfs:comment>Specifies the number of relocation items, i.e. the number of entries that exist in the relocation pointer table. If there are no relocation entries, this value is zero.</rdfs:comment>
	<rdfs:isDefinedBy rdf:resource="http://cybox.mitre.org/objects/File"/>
	<rdfs:label>DOS header e_crlc</rdfs:label>
</rdf:Description>
<!--  -->
<!-- http://cybox.mitre.org/objects/File#dosHeader.e_cs -->

<rdf:Description rdf:about="http://cybox.mitre.org/objects/File#dosHeader.e_cs">
	<rdf:type rdf:resource="http://www.w3.org/2002/07/owl#DatatypeProperty"/>
	<rdfs:range rdf:resource="http://www.w3.org/2001/XMLSchema#hexBinary"/>
	<rdfs:comment>Specifies the pre-relocated initial CS value, relative to the start of the load module, that should be placed in the CS register in order to transfer control to the program. At load time, this value is relocated by adding the address of the start segment of the program to it, and the resulting value is placed in the CS register when control is transferred.</rdfs:comment>
	<rdfs:isDefinedBy rdf:resource="http://cybox.mitre.org/objects/File"/>
	<rdfs:label>DOS Header e_cs</rdfs:label>
</rdf:Description>
<!--  -->
<!-- http://cybox.mitre.org/objects/File#dosHeader.e_csum -->

<rdf:Description rdf:about="http://cybox.mitre.org/objects/File#dosHeader.e_csum">
	<rdf:type rdf:resource="http://www.w3.org/2002/07/owl#DatatypeProperty"/>
	<rdfs:range rdf:resource="http://www.w3.org/2001/XMLSchema#hexBinary"/>
	<rdfs:comment>Specifies the checksum of the contents of the executable file. It is used to ensure the integrity of the data within the file. For full details on how this checksum is calculated, see http://www.tavi.co.uk/phobos/exeformat.html#checksum.</rdfs:comment>
	<rdfs:isDefinedBy rdf:resource="http://cybox.mitre.org/objects/File"/>
	<rdfs:label>DOS Header e_csum</rdfs:label>
</rdf:Description>
<!--  -->
<!-- http://cybox.mitre.org/objects/File#dosHeader.e_ip -->

<rdf:Description rdf:about="http://cybox.mitre.org/objects/File#dosHeader.e_ip">
	<rdf:type rdf:resource="http://www.w3.org/2002/07/owl#DatatypeProperty"/>
	<rdfs:range rdf:resource="http://www.w3.org/2001/XMLSchema#hexBinary"/>
	<rdfs:comment>Specifies the initial IP value, which is the absolute value that should be loaded into the IP register in order to transfer control to the program. Since the actual code segment is determined by the loader, and this is merely a value within that segment, it does not need to be relocated.</rdfs:comment>
	<rdfs:isDefinedBy rdf:resource="http://cybox.mitre.org/objects/File"/>
	<rdfs:label>DOS Header e_ip</rdfs:label>
</rdf:Description>
<!--  -->
<!-- http://cybox.mitre.org/objects/File#dosHeader.e_lfanew -->

<rdf:Description rdf:about="http://cybox.mitre.org/objects/File#dosHeader.e_lfanew">
	<rdf:type rdf:resource="http://www.w3.org/2002/07/owl#DatatypeProperty"/>
	<rdfs:range rdf:resource="http://www.w3.org/2001/XMLSchema#hexBinary"/>
	<rdfs:comment>Specifies the file address of the of the new exe header. In particular, it is a 4-byte offset into the file where the PE file header is located. It is necessary to use this offset to locate the PE header in the file.</rdfs:comment>
	<rdfs:isDefinedBy rdf:resource="http://cybox.mitre.org/objects/File"/>
	<rdfs:label>DOS Header e_lfanew</rdfs:label>
</rdf:Description>
<!--  -->
<!-- http://cybox.mitre.org/objects/File#dosHeader.e_lfarlc -->

<rdf:Description rdf:about="http://cybox.mitre.org/objects/File#dosHeader.e_lfarlc">
	<rdf:type rdf:resource="http://www.w3.org/2002/07/owl#DatatypeProperty"/>
	<rdfs:range rdf:resource="http://www.w3.org/2001/XMLSchema#hexBinary"/>
	<rdfs:comment>Specifies the file address of the relocation table, or more specifically, the offset from the start of the file to the relocation pointer table. This value must be used to locate the relocation pointer table (rather than assuming a fixed location) because variable-length information pertaining to program overlays can occur before this table, causing its position to vary. A value of 0x40 in this field generally indicates a different kind of executable file, not a DOS 'MZ' type.</rdfs:comment>
	<rdfs:isDefinedBy rdf:resource="http://cybox.mitre.org/objects/File"/>
	<rdfs:label>DOS Header e_lfarlc</rdfs:label>
</rdf:Description>
<!--  -->
<!-- http://cybox.mitre.org/objects/File#dosHeader.e_magic -->

<rdf:Description rdf:about="http://cybox.mitre.org/objects/File#dosHeader.e_magic">
	<rdf:type rdf:resource="http://www.w3.org/2002/07/owl#DatatypeProperty"/>
	<rdfs:range rdf:resource="http://www.w3.org/2001/XMLSchema#hexBinary"/>
	<rdfs:comment>Specifies the magic number, specifically the Windows OS signature value, which can either take on MZ for DOS (which is, for all intensive purposes, MOST Windows executables), NE for OS2, LE for OS2 LE, or PE00 for NT.</rdfs:comment>
	<rdfs:isDefinedBy rdf:resource="http://cybox.mitre.org/objects/File"/>
	<rdfs:label>DOS Header e_magic</rdfs:label>
</rdf:Description>
<!--  -->
<!-- http://cybox.mitre.org/objects/File#dosHeader.e_maxalloc -->

<rdf:Description rdf:about="http://cybox.mitre.org/objects/File#dosHeader.e_maxalloc">
	<rdf:type rdf:resource="http://www.w3.org/2002/07/owl#DatatypeProperty"/>
	<rdfs:range rdf:resource="http://www.w3.org/2001/XMLSchema#hexBinary"/>
	<rdfs:comment>Specifies the maximum number of extra paragraphs needed to be allocated by the program before it begins execution. This indicates ADDITIONAL memory over and above that required by the load module and the value specified by MINALLOC. If the request cannot be satisfied, the program is allocated as much memory as is available.</rdfs:comment>
	<rdfs:isDefinedBy rdf:resource="http://cybox.mitre.org/objects/File"/>
	<rdfs:label>DOS Header e_maxalloc</rdfs:label>
</rdf:Description>
<!--  -->
<!-- http://cybox.mitre.org/objects/File#dosHeader.e_minalloc -->

<rdf:Description rdf:about="http://cybox.mitre.org/objects/File#dosHeader.e_minalloc">
	<rdf:type rdf:resource="http://www.w3.org/2002/07/owl#DatatypeProperty"/>
	<rdfs:range rdf:resource="http://www.w3.org/2001/XMLSchema#hexBinary"/>
	<rdfs:comment>Specifies the minimum number of extra paragraphs needed to be allocated to begin execution. This is IN ADDITION to the memory required to hold the load module. This value normally represents the total size of any uninitialised data and/or stack segments that are linked at the end of a program. This space is not directly included in the load module, since there are no particular initializing values and it would simply waste disk space.</rdfs:comment>
	<rdfs:isDefinedBy rdf:resource="http://cybox.mitre.org/objects/File"/>
	<rdfs:label>DOS Header e_minalloc</rdfs:label>
</rdf:Description>
<!--  -->
<!-- http://cybox.mitre.org/objects/File#dosHeader.e_oemid -->

<rdf:Description rdf:about="http://cybox.mitre.org/objects/File#dosHeader.e_oemid">
	<rdf:type rdf:resource="http://www.w3.org/2002/07/owl#DatatypeProperty"/>
	<rdfs:range rdf:resource="http://www.w3.org/2001/XMLSchema#hexBinary"/>
	<rdfs:comment>Specifies the identifier for the OEM for e_oeminfo.</rdfs:comment>
	<rdfs:isDefinedBy rdf:resource="http://cybox.mitre.org/objects/File"/>
	<rdfs:label>DOS Header e_oemid</rdfs:label>
</rdf:Description>
<!--  -->
<!-- http://cybox.mitre.org/objects/File#dosHeader.e_oeminfo -->

<rdf:Description rdf:about="http://cybox.mitre.org/objects/File#dosHeader.e_oeminfo">
	<rdf:type rdf:resource="http://www.w3.org/2002/07/owl#DatatypeProperty"/>
	<rdfs:range rdf:resource="http://www.w3.org/2001/XMLSchema#hexBinary"/>
	<rdfs:comment>Specifies the OEM information for a specific value of e_oeminfo.</rdfs:comment>
	<rdfs:isDefinedBy rdf:resource="http://cybox.mitre.org/objects/File"/>
	<rdfs:label>DOS Header e_oeminfo</rdfs:label>
</rdf:Description>
<!--  -->
<!-- http://cybox.mitre.org/objects/File#dosHeader.e_ovro -->

<rdf:Description rdf:about="http://cybox.mitre.org/objects/File#dosHeader.e_ovro">
	<rdf:type rdf:resource="http://www.w3.org/2002/07/owl#DatatypeProperty"/>
	<rdfs:range rdf:resource="http://www.w3.org/2001/XMLSchema#hexBinary"/>
	<rdfs:comment>Specifies the overlay number, which is normally set to 0x0000, because few programs actually have overlays. It changes only in files containing programs that use overlays. See http://www.tavi.co.uk/phobos/exeformat.html#overlaynote for more information about overlays.</rdfs:comment>
	<rdfs:isDefinedBy rdf:resource="http://cybox.mitre.org/objects/File"/>
	<rdfs:label>DOS Header e_ovro</rdfs:label>
</rdf:Description>
<!--  -->
<!-- http://cybox.mitre.org/objects/File#dosHeader.e_sp -->

<rdf:Description rdf:about="http://cybox.mitre.org/objects/File#dosHeader.e_sp">
	<rdf:type rdf:resource="http://www.w3.org/2002/07/owl#DatatypeProperty"/>
	<rdfs:range rdf:resource="http://www.w3.org/2001/XMLSchema#hexBinary"/>
	<rdfs:comment>Specifies the initial SP value, which is the absolute value that must be loaded into the SP register before the program is given control. Since the actual stack segment is determined by the loader, and this is merely a value within that segment, it does not need to be relocated.</rdfs:comment>
	<rdfs:isDefinedBy rdf:resource="http://cybox.mitre.org/objects/File"/>
	<rdfs:label>DOS Header e_sp</rdfs:label>
</rdf:Description>
<!--  -->
<!-- http://cybox.mitre.org/objects/File#dosHeader.e_ss -->

<rdf:Description rdf:about="http://cybox.mitre.org/objects/File#dosHeader.e_ss">
	<rdf:type rdf:resource="http://www.w3.org/2002/07/owl#DatatypeProperty"/>
	<rdfs:range rdf:resource="http://www.w3.org/2001/XMLSchema#hexBinary"/>
	<rdfs:comment>Specifies the initial SS value, which is the paragraph address of the stack segment relative to the start of the load module. At load time, this value is relocated by adding the address of the start segment of the program to it, and the resulting value is placed in the SS register before the program is started. In DOS, the start segment of the program is the first segment boundary in memory after the PSP.</rdfs:comment>
	<rdfs:isDefinedBy rdf:resource="http://cybox.mitre.org/objects/File"/>
	<rdfs:label>DOS Header e_ss</rdfs:label>
</rdf:Description>
<!--  -->
<!-- http://cybox.mitre.org/objects/File#dosHeader.hashValue -->

<rdf:Description rdf:about="http://cybox.mitre.org/objects/File#dosHeader.hashValue">
	<rdf:type rdf:resource="http://www.w3.org/2002/07/owl#DatatypeProperty"/>
	<rdfs:range rdf:resource="http://www.w3.org/2001/XMLSchema#string"/>
	<rdfs:comment>Specifies the values, in the format of 'hash-type':'hash-value' for any hash computed using the specified PE binary MS-DOS header as input.</rdfs:comment>
	<rdfs:isDefinedBy rdf:resource="http://cybox.mitre.org/objects/File"/>
	<rdfs:label>DOS Header Hash Value</rdfs:label>
</rdf:Description>
<!--  -->
<!-- http://cybox.mitre.org/objects/File#dosHeader.reserved1 -->

<rdf:Description rdf:about="http://cybox.mitre.org/objects/File#dosHeader.reserved1">
	<rdf:type rdf:resource="http://www.w3.org/2002/07/owl#DatatypeProperty"/>
	<rdfs:range rdf:resource="http://www.w3.org/2001/XMLSchema#hexBinary"/>
	<rdfs:comment>Specifies reserved words for the program (known in winnt.h as e_res[4]), usually set to zero by the linker. In this case, just use a single reserved1 set to zero; if not zero create four reserved1 with the correct value.</rdfs:comment>
	<rdfs:isDefinedBy rdf:resource="http://cybox.mitre.org/objects/File"/>
	<rdfs:label>DOS Header Reserved1</rdfs:label>
</rdf:Description>
<!--  -->
<!-- http://cybox.mitre.org/objects/File#dosHeader.reserved2 -->

<rdf:Description rdf:about="http://cybox.mitre.org/objects/File#dosHeader.reserved2">
	<rdf:type rdf:resource="http://www.w3.org/2002/07/owl#DatatypeProperty"/>
	<rdfs:range rdf:resource="http://www.w3.org/2001/XMLSchema#hexBinary"/>
	<rdfs:comment>Specifies reserved words for the program (known in winnt.h as e_res[10]), usually set to zero by the linker. In this case, just use a single reserved1 set to zero; if not zero create ten reserved1 with the correct value.</rdfs:comment>
	<rdfs:isDefinedBy rdf:resource="http://cybox.mitre.org/objects/File"/>
	<rdfs:label>DOS Header Reserved2</rdfs:label>
</rdf:Description>
<!--  -->
<!-- http://cybox.mitre.org/objects/File#drive -->

<rdf:Description rdf:about="http://cybox.mitre.org/objects/File#drive">
	<rdf:type rdf:resource="http://www.w3.org/2002/07/owl#DatatypeProperty"/>
	<rdfs:range rdf:resource="http://www.w3.org/2001/XMLSchema#string"/>
	<rdfs:comment>Specifies the drive letter of the drive that the file resides on.</rdfs:comment>
	<rdfs:isDefinedBy rdf:resource="http://cybox.mitre.org/objects/File"/>
	<rdfs:label>Drive</rdfs:label>
</rdf:Description>
<!--  -->
<!-- http://cybox.mitre.org/objects/File#driverInit -->

<rdf:Description rdf:about="http://cybox.mitre.org/objects/File#driverInit">
	<rdf:type rdf:resource="http://www.w3.org/2002/07/owl#DatatypeProperty"/>
	<rdfs:range rdf:resource="http://www.w3.org/2001/XMLSchema#hexBinary"/>
	<rdfs:comment>Specifies the entry point for the driver's DriverEntry routine. 

See also: http://msdn.microsoft.com/en-us/library/windows/hardware/ff544174(v=vs.85).aspx.</rdfs:comment>
	<rdfs:isDefinedBy rdf:resource="http://cybox.mitre.org/objects/File"/>
	<rdfs:label>Driver Init</rdfs:label>
</rdf:Description>
<!--  -->
<!-- http://cybox.mitre.org/objects/File#driverName -->

<rdf:Description rdf:about="http://cybox.mitre.org/objects/File#driverName">
	<rdf:type rdf:resource="http://www.w3.org/2002/07/owl#DatatypeProperty"/>
	<rdfs:range rdf:resource="http://www.w3.org/2001/XMLSchema#string"/>
	<rdfs:comment>Specifies the name of the driver.</rdfs:comment>
	<rdfs:isDefinedBy rdf:resource="http://cybox.mitre.org/objects/File"/>
	<rdfs:label>Driver Name</rdfs:label>
</rdf:Description>
<!--  -->
<!-- http://cybox.mitre.org/objects/File#driverObjectAddress -->

<rdf:Description rdf:about="http://cybox.mitre.org/objects/File#driverObjectAddress">
	<rdf:type rdf:resource="http://www.w3.org/2002/07/owl#DatatypeProperty"/>
	<rdfs:range rdf:resource="http://www.w3.org/2001/XMLSchema#hexBinary"/>
	<rdfs:comment>Specifies the address to the driver's driver object, which contains the storage for the entry point to many of the driver's standard routines. 

See also: http://msdn.mic</rdfs:comment>
	<rdfs:isDefinedBy rdf:resource="http://cybox.mitre.org/objects/File"/>
	<rdfs:label>Driver Object Address</rdfs:label>
</rdf:Description>
<!--  -->
<!-- http://cybox.mitre.org/objects/File#driverStartIO -->

<rdf:Description rdf:about="http://cybox.mitre.org/objects/File#driverStartIO">
	<rdf:type rdf:resource="http://www.w3.org/2002/07/owl#DatatypeProperty"/>
	<rdfs:range rdf:resource="http://www.w3.org/2001/XMLSchema#hexBinary"/>
	<rdfs:comment>Specifies the entry point for the driver's StartIO routine. 

See also: http://msdn.microsoft.com/en-us/library/windows/hardware/ff544174(v=vs.85).aspx.</rdfs:comment>
	<rdfs:isDefinedBy rdf:resource="http://cybox.mitre.org/objects/File"/>
	<rdfs:label>Driver StartIO Routine Address</rdfs:label>
</rdf:Description>
<!--  -->
<!-- http://cybox.mitre.org/objects/File#driverUnload -->

<rdf:Description rdf:about="http://cybox.mitre.org/objects/File#driverUnload">
	<rdf:type rdf:resource="http://www.w3.org/2002/07/owl#DatatypeProperty"/>
	<rdfs:range rdf:resource="http://www.w3.org/2001/XMLSchema#hexBinary"/>
	<rdfs:comment>Specifies the entry point for the driver's unload routine. 

See also: http://msdn.microsoft.com/en-us/library/windows/hardware/ff544174(v=vs.85).aspx.</rdfs:comment>
	<rdfs:isDefinedBy rdf:resource="http://cybox.mitre.org/objects/File"/>
	<rdfs:label>Driver Unload Routine Address</rdfs:label>
</rdf:Description>
<!--  -->
<!-- http://cybox.mitre.org/objects/File#encrypt.rawContents -->

<rdf:Description rdf:about="http://cybox.mitre.org/objects/File#encrypt.rawContents">
	<rdf:type rdf:resource="http://www.w3.org/2002/07/owl#DatatypeProperty"/>
	<rdfs:range rdf:resource="http://www.w3.org/2001/XMLSchema#string"/>
	<rdfs:comment>Specifies the PDF document's encryption dictionary as embedded set of key/value pairs.</rdfs:comment>
	<rdfs:isDefinedBy rdf:resource="http://cybox.mitre.org/objects/File"/>
	<rdfs:label>Encryption Dictionary Key/Value Pairs</rdfs:label>
</rdf:Description>
<!--  -->
<!-- http://cybox.mitre.org/objects/File#encryptCount.nonObfuscated -->

<rdf:Description rdf:about="http://cybox.mitre.org/objects/File#encryptCount.nonObfuscated">
	<rdf:type rdf:resource="http://www.w3.org/2002/07/owl#DatatypeProperty"/>
	<rdfs:range rdf:resource="http://www.w3.org/2001/XMLSchema#nonNegativeInteger"/>
	<rdfs:comment>Specifies the number of non-obfuscated occurrences of the '/Encrypt' keyword in the PDF file, which indicates that the PDF uses encryption.</rdfs:comment>
	<rdfs:isDefinedBy rdf:resource="http://cybox.mitre.org/objects/File"/>
	<rdfs:label>'/Encrypt' Non-obfuscated Count</rdfs:label>
</rdf:Description>
<!--  -->
<!-- http://cybox.mitre.org/objects/File#encryptCount.obfuscated -->

<rdf:Description rdf:about="http://cybox.mitre.org/objects/File#encryptCount.obfuscated">
	<rdf:type rdf:resource="http://www.w3.org/2002/07/owl#DatatypeProperty"/>
	<rdfs:range rdf:resource="http://www.w3.org/2001/XMLSchema#nonNegativeInteger"/>
	<rdfs:comment>Specifies the number of obfuscated occurrences of the '/Encrypt' keyword in the PDF file with some form of obfuscation, such as with hexcodes.

The use of the '/Encrypt' keyword indicates that the PDF uses encryption.</rdfs:comment>
	<rdfs:isDefinedBy rdf:resource="http://cybox.mitre.org/objects/File"/>
	<rdfs:label>'/Encrypt' Obfuscated Count</rdfs:label>
</rdf:Description>
<!--  -->
<!-- http://cybox.mitre.org/objects/File#encrypted -->

<rdf:Description rdf:about="http://cybox.mitre.org/objects/File#encrypted">
	<rdf:type rdf:resource="http://www.w3.org/2002/07/owl#DatatypeProperty"/>
	<rdfs:range rdf:resource="http://www.w3.org/2001/XMLSchema#boolean"/>
	<rdfs:comment>Specifies a file or directory that is encrypted, as denoted by the constant value, 0x4000. For a file, all data streams in the file are encrypted. For a directory, encryption is the default for newly created files and subdirectories</rdfs:comment>
	<rdfs:isDefinedBy rdf:resource="http://cybox.mitre.org/objects/File"/>
	<rdfs:label>Encrypted</rdfs:label>
</rdf:Description>
<!--  -->
<!-- http://cybox.mitre.org/objects/File#encryptionAlgorithm -->

<rdf:Description rdf:about="http://cybox.mitre.org/objects/File#encryptionAlgorithm">
	<rdf:type rdf:resource="http://www.w3.org/2002/07/owl#DatatypeProperty"/>
	<rdfs:range rdf:resource="http://www.w3.org/2001/XMLSchema#string"/>
	<rdfs:comment>Specifies the algorithm used to encrypt the file.</rdfs:comment>
	<rdfs:isDefinedBy rdf:resource="http://cybox.mitre.org/objects/File"/>
	<rdfs:label>Encryption Algorithm</rdfs:label>
</rdf:Description>
<!--  -->
<!-- http://cybox.mitre.org/objects/File#entropy.max -->

<rdf:Description rdf:about="http://cybox.mitre.org/objects/File#entropy.max">
	<rdf:type rdf:resource="http://www.w3.org/2002/07/owl#DatatypeProperty"/>
	<rdfs:range rdf:resource="http://www.w3.org/2001/XMLSchema#float"/>
	<rdfs:comment>Specifies the largest possible value for the entropy computation (e.g., this would be 8 if the entropy computations is based on bits of information).</rdfs:comment>
	<rdfs:isDefinedBy rdf:resource="http://cybox.mitre.org/objects/File"/>
	<rdfs:label>Entropy Max</rdfs:label>
</rdf:Description>
<!--  -->
<!-- http://cybox.mitre.org/objects/File#entropy.min -->

<rdf:Description rdf:about="http://cybox.mitre.org/objects/File#entropy.min">
	<rdf:type rdf:resource="http://www.w3.org/2002/07/owl#DatatypeProperty"/>
	<rdfs:range rdf:resource="http://www.w3.org/2001/XMLSchema#float"/>
	<rdfs:comment>Specifies the smallest possible value for the entropy computation.</rdfs:comment>
	<rdfs:isDefinedBy rdf:resource="http://cybox.mitre.org/objects/File"/>
	<rdfs:label>Entropy Min</rdfs:label>
</rdf:Description>
<!--  -->
<!-- http://cybox.mitre.org/objects/File#entropy.value -->

<rdf:Description rdf:about="http://cybox.mitre.org/objects/File#entropy.value">
	<rdf:type rdf:resource="http://www.w3.org/2002/07/owl#DatatypeProperty"/>
	<rdfs:range rdf:resource="http://www.w3.org/2001/XMLSchema#float"/>
	<rdfs:comment>Specifies the computed entropy value.</rdfs:comment>
	<rdfs:isDefinedBy rdf:resource="http://cybox.mitre.org/objects/File"/>
	<rdfs:label>Entropy Value</rdfs:label>
</rdf:Description>
<!--  -->
<!-- http://cybox.mitre.org/objects/File#entryPoint -->

<rdf:Description rdf:about="http://cybox.mitre.org/objects/File#entryPoint">
	<rdf:type rdf:resource="http://www.w3.org/2002/07/owl#DatatypeProperty"/>
	<rdfs:range rdf:resource="http://www.w3.org/2001/XMLSchema#hexBinary"/>
	<rdfs:comment>Specifies the entry point address, if applicable.</rdfs:comment>
	<rdfs:isDefinedBy rdf:datatype="http://www.w3.org/2001/XMLSchema#string">&lt;http://cybox.mitre.org/objects/File&gt;</rdfs:isDefinedBy>
	<rdfs:label>Entry Point</rdfs:label>
</rdf:Description>
<!--  -->
<!-- http://cybox.mitre.org/objects/File#entrypointSignatureName -->

<rdf:Description rdf:about="http://cybox.mitre.org/objects/File#entrypointSignatureName">
	<rdf:type rdf:resource="http://www.w3.org/2002/07/owl#DatatypeProperty"/>
	<rdfs:range rdf:resource="http://www.w3.org/2001/XMLSchema#string"/>
	<rdfs:comment>Specifies the signature name.</rdfs:comment>
	<rdfs:isDefinedBy rdf:datatype="http://www.w3.org/2001/XMLSchema#string">&lt;http://cybox.mitre.org/objects/File&gt;</rdfs:isDefinedBy>
	<rdfs:label>Entrypoint Signature Name</rdfs:label>
</rdf:Description>
<!--  -->
<!-- http://cybox.mitre.org/objects/File#entrypointSignatureType -->

<rdf:Description rdf:about="http://cybox.mitre.org/objects/File#entrypointSignatureType">
	<rdf:type rdf:resource="http://www.w3.org/2002/07/owl#DatatypeProperty"/>
	<rdfs:range rdf:resource="http://www.w3.org/2001/XMLSchema#string"/>
	<rdfs:comment>Specifies the type of entry point detected (e.g., packer, compiled file).</rdfs:comment>
	<rdfs:isDefinedBy rdf:resource="http://cybox.mitre.org/objects/File"/>
	<rdfs:label>Entrypoint Signature Type</rdfs:label>
</rdf:Description>
<!--  -->
<!-- http://cybox.mitre.org/objects/File#epJumpCode.depth -->

<rdf:Description rdf:about="http://cybox.mitre.org/objects/File#epJumpCode.depth">
	<rdf:type rdf:resource="http://www.w3.org/2002/07/owl#DatatypeProperty"/>
	<rdfs:domain rdf:resource="http://cybox.mitre.org/objects/File#Packer"/>
	<rdfs:range rdf:resource="http://www.w3.org/2001/XMLSchema#integer"/>
	<rdfs:comment>Specifies the frequency that a jump instruction is found to be immediately followed by another jump instruction within the PE(Portable Executable) entry point.</rdfs:comment>
	<rdfs:isDefinedBy rdf:datatype="http://www.w3.org/2001/XMLSchema#string">&lt;http://cybox.mitre.org/objects/File&gt;</rdfs:isDefinedBy>
	<rdfs:label>ep jump code.depth</rdfs:label>
</rdf:Description>
<!--  -->
<!-- http://cybox.mitre.org/objects/File#epJumpCode.opCodes -->

<rdf:Description rdf:about="http://cybox.mitre.org/objects/File#epJumpCode.opCodes">
	<rdf:type rdf:resource="http://www.w3.org/2002/07/owl#DatatypeProperty"/>
	<rdfs:range rdf:resource="http://www.w3.org/2001/XMLSchema#string"/>
	<rdfs:comment>Specifies the hex value of the bytes located at the jump location for a relative jump identified in the PE(Portable Executable) entry point up to 10 bytes or the end of the RVA(Relative Virtual Address) section.</rdfs:comment>
	<rdfs:isDefinedBy rdf:datatype="http://www.w3.org/2001/XMLSchema#string">&lt;http://cybox.mitre.org/objects/File&gt;</rdfs:isDefinedBy>
	<rdfs:label>ep jump code.op codes</rdfs:label>
</rdf:Description>
<!--  -->
<!-- http://cybox.mitre.org/objects/File#exceptionTable.size -->

<rdf:Description rdf:about="http://cybox.mitre.org/objects/File#exceptionTable.size">
	<rdf:type rdf:resource="http://www.w3.org/2002/07/owl#DatatypeProperty"/>
	<rdfs:range rdf:resource="http://www.w3.org/2001/XMLSchema#nonNegativeInteger"/>
	<rdfs:comment>Specifies the size of the data structure, in bytes, of the exception table data directory.</rdfs:comment>
	<rdfs:isDefinedBy rdf:resource="http://cybox.mitre.org/objects/File"/>
	<rdfs:label>Exception Table Size</rdfs:label>
</rdf:Description>
<!--  -->
<!-- http://cybox.mitre.org/objects/File#exceptionTable.virtualAddress -->

<rdf:Description rdf:about="http://cybox.mitre.org/objects/File#exceptionTable.virtualAddress">
	<rdf:type rdf:resource="http://www.w3.org/2002/07/owl#DatatypeProperty"/>
	<rdfs:range rdf:resource="http://www.w3.org/2001/XMLSchema#hexBinary"/>
	<rdfs:comment>Specifies the relative virtual address (RVA) of the exception table data directory.</rdfs:comment>
	<rdfs:isDefinedBy rdf:resource="http://cybox.mitre.org/objects/File"/>
	<rdfs:label>Exception Table Virtual Address</rdfs:label>
</rdf:Description>
<!--  -->
<!-- http://cybox.mitre.org/objects/File#exportTable.size -->

<rdf:Description rdf:about="http://cybox.mitre.org/objects/File#exportTable.size">
	<rdf:type rdf:resource="http://www.w3.org/2002/07/owl#DatatypeProperty"/>
	<rdfs:range rdf:resource="http://www.w3.org/2001/XMLSchema#nonNegativeInteger"/>
	<rdfs:comment>Specifies the size of the data structure, in bytes, of  the export table data directory.</rdfs:comment>
	<rdfs:isDefinedBy rdf:resource="http://cybox.mitre.org/objects/File"/>
	<rdfs:label>Export Table Size</rdfs:label>
</rdf:Description>
<!--  -->
<!-- http://cybox.mitre.org/objects/File#exportTable.virtualAddress -->

<rdf:Description rdf:about="http://cybox.mitre.org/objects/File#exportTable.virtualAddress">
	<rdf:type rdf:resource="http://www.w3.org/2002/07/owl#DatatypeProperty"/>
	<rdfs:range rdf:resource="http://www.w3.org/2001/XMLSchema#hexBinary"/>
	<rdfs:comment>Specifies the relative virtual address (RVA) of the data structure of the export table data directory.</rdfs:comment>
	<rdfs:isDefinedBy rdf:resource="http://cybox.mitre.org/objects/File"/>
	<rdfs:label>Export Table Virtual Address</rdfs:label>
</rdf:Description>
<!--  -->
<!-- http://cybox.mitre.org/objects/File#exportsTimestamp -->

<rdf:Description rdf:about="http://cybox.mitre.org/objects/File#exportsTimestamp">
	<rdf:type rdf:resource="http://www.w3.org/2002/07/owl#DatatypeProperty"/>
	<rdfs:range rdf:resource="http://www.w3.org/2001/XMLSchema#dateTime"/>
	<rdfs:comment>Specifies the date and time the export data was created.</rdfs:comment>
	<rdfs:isDefinedBy rdf:resource="http://cybox.mitre.org/objects/File"/>
	<rdfs:label>Exports Timestamp</rdfs:label>
</rdf:Description>
<!--  -->
<!-- http://cybox.mitre.org/objects/File#extraneousBytes -->

<rdf:Description rdf:about="http://cybox.mitre.org/objects/File#extraneousBytes">
	<rdf:type rdf:resource="http://www.w3.org/2002/07/owl#DatatypeProperty"/>
	<rdfs:range rdf:resource="http://www.w3.org/2001/XMLSchema#integer"/>
	<rdfs:comment>Specifies the number of extraneous bytes contained in the PE binary.</rdfs:comment>
	<rdfs:isDefinedBy rdf:resource="http://cybox.mitre.org/objects/File"/>
	<rdfs:label>Extraneous Bytes</rdfs:label>
</rdf:Description>
<!--  -->
<!-- http://cybox.mitre.org/objects/File#fileCount -->

<rdf:Description rdf:about="http://cybox.mitre.org/objects/File#fileCount">
	<rdf:type rdf:resource="http://www.w3.org/2002/07/owl#DatatypeProperty"/>
	<rdfs:range rdf:resource="http://www.w3.org/2001/XMLSchema#positiveInteger"/>
	<rdfs:comment>Specifies the number of files contained within the archive.</rdfs:comment>
	<rdfs:isDefinedBy rdf:resource="http://cybox.mitre.org/objects/File"/>
	<rdfs:label>File Count</rdfs:label>
</rdf:Description>
<!--  -->
<!-- http://cybox.mitre.org/objects/File#fileDescription -->

<rdf:Description rdf:about="http://cybox.mitre.org/objects/File#fileDescription">
	<rdf:type rdf:resource="http://www.w3.org/2002/07/owl#DatatypeProperty"/>
	<rdfs:range rdf:resource="http://www.w3.org/2001/XMLSchema#string"/>
	<rdfs:comment>Specifies  the file description to be presented to users. This string may be displayed in a list box when the user is choosing files to install - for example, "Keyboard Driver for AT-Style Keyboards".</rdfs:comment>
	<rdfs:isDefinedBy rdf:resource="http://cybox.mitre.org/objects/File"/>
	<rdfs:label>File Description</rdfs:label>
</rdf:Description>
<!--  -->
<!-- http://cybox.mitre.org/objects/File#fileExtension -->

<rdf:Description rdf:about="http://cybox.mitre.org/objects/File#fileExtension">
	<rdf:type rdf:resource="http://www.w3.org/2002/07/owl#DatatypeProperty"/>
	<rdfs:range rdf:resource="http://www.w3.org/2001/XMLSchema#string"/>
	<rdfs:comment>Specifies the extension of the name of the file.  &#xD;
&#xD;
The fileExtension field must not conflict with the ending of the fileName field. The fileExtension field should not begin with a "." character, but may contain a "." character in the case of a compound file extension, such as "tar.gz".</rdfs:comment>
	<rdfs:isDefinedBy rdf:datatype="http://www.w3.org/2001/XMLSchema#string">&lt;http://cybox.mitre.org/objects/File&gt;</rdfs:isDefinedBy>
	<rdfs:label>File Extension</rdfs:label>
</rdf:Description>
<!--  -->
<!-- http://cybox.mitre.org/objects/File#fileFormat -->

<rdf:Description rdf:about="http://cybox.mitre.org/objects/File#fileFormat">
	<rdf:type rdf:resource="http://www.w3.org/2002/07/owl#DatatypeProperty"/>
	<rdfs:range rdf:resource="http://www.w3.org/2001/XMLSchema#string"/>
	<rdfs:comment>Specifies the particular file format of the file, most typically specified by a tool such as the UNIX file command.</rdfs:comment>
	<rdfs:isDefinedBy rdf:datatype="http://www.w3.org/2001/XMLSchema#string">&lt;http://cybox.mitre.org/objects/File&gt;</rdfs:isDefinedBy>
	<rdfs:label>File Format</rdfs:label>
</rdf:Description>
<!--  -->
<!-- http://cybox.mitre.org/objects/File#fileHeader.characteristics -->

<rdf:Description rdf:about="http://cybox.mitre.org/objects/File#fileHeader.characteristics">
	<rdf:type rdf:resource="http://www.w3.org/2002/07/owl#DatatypeProperty"/>
	<rdfs:range rdf:resource="http://www.w3.org/2001/XMLSchema#hexBinary"/>
	<rdfs:comment>Specifies the flags that indicate the file's characteristics.</rdfs:comment>
	<rdfs:isDefinedBy rdf:resource="http://cybox.mitre.org/objects/File"/>
	<rdfs:label>File Header Characteristics</rdfs:label>
</rdf:Description>
<!--  -->
<!-- http://cybox.mitre.org/objects/File#fileHeader.hashValues -->

<rdf:Description rdf:about="http://cybox.mitre.org/objects/File#fileHeader.hashValues">
	<rdf:type rdf:resource="http://www.w3.org/2002/07/owl#DatatypeProperty"/>
	<rdfs:range rdf:resource="http://www.w3.org/2001/XMLSchema#string"/>
	<rdfs:comment>Specifies the values, in the format of 'hash-type':'hash-value', for any hash computed for the Optional Header.</rdfs:comment>
	<rdfs:isDefinedBy rdf:resource="http://cybox.mitre.org/objects/File"/>
	<rdfs:label>File Header Hash Values</rdfs:label>
</rdf:Description>
<!--  -->
<!-- http://cybox.mitre.org/objects/File#fileHeader.machine -->

<rdf:Description rdf:about="http://cybox.mitre.org/objects/File#fileHeader.machine">
	<rdf:type rdf:resource="http://www.w3.org/2002/07/owl#DatatypeProperty"/>
	<rdfs:range rdf:resource="http://www.w3.org/2001/XMLSchema#hexBinary"/>
	<rdfs:comment>Specifies the type of target machine.</rdfs:comment>
	<rdfs:isDefinedBy rdf:resource="http://cybox.mitre.org/objects/File"/>
	<rdfs:label>File Header Machine</rdfs:label>
</rdf:Description>
<!--  -->
<!-- http://cybox.mitre.org/objects/File#fileHeader.numberOfSections -->

<rdf:Description rdf:about="http://cybox.mitre.org/objects/File#fileHeader.numberOfSections">
	<rdf:type rdf:resource="http://www.w3.org/2002/07/owl#DatatypeProperty"/>
	<rdfs:range rdf:resource="http://www.w3.org/2001/XMLSchema#nonNegativeInteger"/>
	<rdfs:comment>Specifies the number of sections in the file.</rdfs:comment>
	<rdfs:isDefinedBy rdf:resource="http://cybox.mitre.org/objects/File"/>
	<rdfs:label>File Header Number of Sections</rdfs:label>
</rdf:Description>
<!--  -->
<!-- http://cybox.mitre.org/objects/File#fileHeader.numberOfSymbols -->

<rdf:Description rdf:about="http://cybox.mitre.org/objects/File#fileHeader.numberOfSymbols">
	<rdf:type rdf:resource="http://www.w3.org/2002/07/owl#DatatypeProperty"/>
	<rdfs:range rdf:resource="http://www.w3.org/2001/XMLSchema#nonNegativeInteger"/>
	<rdfs:comment>Specifies the number of entries in the symbol table. Should be 0.</rdfs:comment>
	<rdfs:isDefinedBy rdf:resource="http://cybox.mitre.org/objects/File"/>
	<rdfs:label>File Header Number of Symbols</rdfs:label>
</rdf:Description>
<!--  -->
<!-- http://cybox.mitre.org/objects/File#fileHeader.pointerToSymbolTable -->

<rdf:Description rdf:about="http://cybox.mitre.org/objects/File#fileHeader.pointerToSymbolTable">
	<rdf:type rdf:resource="http://www.w3.org/2002/07/owl#DatatypeProperty"/>
	<rdfs:range rdf:resource="http://www.w3.org/2001/XMLSchema#hexBinary"/>
	<rdfs:comment>Specifies the file offset of the COFF symbol table (should be 0).</rdfs:comment>
	<rdfs:isDefinedBy rdf:resource="http://cybox.mitre.org/objects/File"/>
	<rdfs:label>File Header Pointer to Symbol Table</rdfs:label>
</rdf:Description>
<!--  -->
<!-- http://cybox.mitre.org/objects/File#fileHeader.sizeOfOptionalHeader -->

<rdf:Description rdf:about="http://cybox.mitre.org/objects/File#fileHeader.sizeOfOptionalHeader">
	<rdf:type rdf:resource="http://www.w3.org/2002/07/owl#DatatypeProperty"/>
	<rdfs:range rdf:resource="http://www.w3.org/2001/XMLSchema#hexBinary"/>
	<rdfs:comment>Specifies the size of the optional header. Should be 0 for object files and non-zero for executables.</rdfs:comment>
	<rdfs:isDefinedBy rdf:resource="http://cybox.mitre.org/objects/File"/>
	<rdfs:label>File Header Size of Optional Header</rdfs:label>
</rdf:Description>
<!--  -->
<!-- http://cybox.mitre.org/objects/File#fileHeader.timestamp -->

<rdf:Description rdf:about="http://cybox.mitre.org/objects/File#fileHeader.timestamp">
	<rdf:type rdf:resource="http://www.w3.org/2002/07/owl#DatatypeProperty"/>
	<rdfs:range rdf:resource="http://www.w3.org/2001/XMLSchema#hexBinary"/>
	<rdfs:comment>Specifies the time when the file was created (the low 32 bits of the number of seconds since epoch).</rdfs:comment>
	<rdfs:isDefinedBy rdf:resource="http://cybox.mitre.org/objects/File"/>
	<rdfs:label>File Header Timestamp</rdfs:label>
</rdf:Description>
<!--  -->
<!-- http://cybox.mitre.org/objects/File#fileName -->

<rdf:Description rdf:about="http://cybox.mitre.org/objects/File#fileName">
	<rdf:type rdf:resource="http://www.w3.org/2002/07/owl#DatatypeProperty"/>
	<rdfs:range rdf:resource="http://www.w3.org/2001/XMLSchema#string"/>
	<rdfs:comment>Specifies the base name of the file (including an extension, if present).</rdfs:comment>
	<rdfs:isDefinedBy rdf:datatype="http://www.w3.org/2001/XMLSchema#string">&lt;http://cybox.mitre.org/objects/File&gt;</rdfs:isDefinedBy>
	<rdfs:label>File Name</rdfs:label>
</rdf:Description>
<!--  -->
<!-- http://cybox.mitre.org/objects/File#filePath -->

<rdf:Description rdf:about="http://cybox.mitre.org/objects/File#filePath">
	<rdf:type rdf:resource="http://www.w3.org/2002/07/owl#DatatypeProperty"/>
	<rdfs:range rdf:resource="http://www.w3.org/2001/XMLSchema#string"/>
	<rdfs:comment>Specifies the relative or fully-qualified path to the file, not including the path to the device where the file system containing the file resides. &#xD;
&#xD;
Whether the path is relative or fully-qualified can be specified via the 'fully_qualified' attribute of this field.  The File_Path field should contain only the path of the directory containing the file, and should end with a terminating path separator("\" or "/").</rdfs:comment>
	<rdfs:isDefinedBy rdf:datatype="http://www.w3.org/2001/XMLSchema#string">&lt;http://cybox.mitre.org/objects/File&gt;</rdfs:isDefinedBy>
	<rdfs:label>File Path</rdfs:label>
</rdf:Description>
<!--  -->
<!-- http://cybox.mitre.org/objects/File#filePath.fullyQualified -->

<rdf:Description rdf:about="http://cybox.mitre.org/objects/File#filePath.fullyQualified">
	<rdf:type rdf:resource="http://www.w3.org/2002/07/owl#DatatypeProperty"/>
	<rdfs:range rdf:resource="http://www.w3.org/2001/XMLSchema#boolean"/>
	<rdfs:comment>Specifies whether the path is fully qualified.</rdfs:comment>
	<rdfs:isDefinedBy rdf:datatype="http://www.w3.org/2001/XMLSchema#string">&lt;http://cybox.mitre.org/objects/File&gt;</rdfs:isDefinedBy>
	<rdfs:label>Fully-Qualified File Path</rdfs:label>
</rdf:Description>
<!--  -->
<!-- http://cybox.mitre.org/objects/File#fileVersion -->

<rdf:Description rdf:about="http://cybox.mitre.org/objects/File#fileVersion">
	<rdf:type rdf:resource="http://www.w3.org/2002/07/owl#DatatypeProperty"/>
	<rdfs:range rdf:resource="http://www.w3.org/2001/XMLSchema#string"/>
	<rdfs:comment>Specifies the version number of the file - for example, "3.10" or "5.00.RC2".</rdfs:comment>
	<rdfs:isDefinedBy rdf:resource="http://cybox.mitre.org/objects/File"/>
	<rdfs:label>File Version</rdfs:label>
</rdf:Description>
<!--  -->
<!-- http://cybox.mitre.org/objects/File#filenameAccessTime -->

<rdf:Description rdf:about="http://cybox.mitre.org/objects/File#filenameAccessTime">
	<rdf:type rdf:resource="http://www.w3.org/2002/07/owl#DatatypeProperty"/>
	<rdfs:range rdf:resource="http://www.w3.org/2001/XMLSchema#dateTime"/>
	<rdfs:comment>Specifies the date/time the filename of the Windows file was last accessed.</rdfs:comment>
	<rdfs:isDefinedBy rdf:resource="http://cybox.mitre.org/objects/File"/>
	<rdfs:label>Filename Access Time</rdfs:label>
</rdf:Description>
<!--  -->
<!-- http://cybox.mitre.org/objects/File#filenameCreatedTime -->

<rdf:Description rdf:about="http://cybox.mitre.org/objects/File#filenameCreatedTime">
	<rdf:type rdf:resource="http://www.w3.org/2002/07/owl#DatatypeProperty"/>
	<rdfs:range rdf:resource="http://www.w3.org/2001/XMLSchema#dateTime"/>
	<rdfs:comment>Specifies the date/time the filename of the Windows file was created.</rdfs:comment>
	<rdfs:isDefinedBy rdf:resource="http://cybox.mitre.org/objects/File"/>
	<rdfs:label>Filename Created Time</rdfs:label>
</rdf:Description>
<!--  -->
<!-- http://cybox.mitre.org/objects/File#filenameModifiedTime -->

<rdf:Description rdf:about="http://cybox.mitre.org/objects/File#filenameModifiedTime">
	<rdf:type rdf:resource="http://www.w3.org/2002/07/owl#DatatypeProperty"/>
	<rdfs:range rdf:resource="http://www.w3.org/2001/XMLSchema#dateTime"/>
	<rdfs:comment>Specifies the date/time the filename of the Windows file was last modified.</rdfs:comment>
	<rdfs:isDefinedBy rdf:resource="http://cybox.mitre.org/objects/File"/>
	<rdfs:label>Filename Modified Time</rdfs:label>
</rdf:Description>
<!--  -->
<!-- http://cybox.mitre.org/objects/File#firstObjectNumber -->

<rdf:Description rdf:about="http://cybox.mitre.org/objects/File#firstObjectNumber">
	<rdf:type rdf:resource="http://www.w3.org/2002/07/owl#DatatypeProperty"/>
	<rdfs:range rdf:resource="http://www.w3.org/2001/XMLSchema#nonNegativeInteger"/>
	<rdfs:comment>Specifies the object number of the first object for which there is a corresponding entry in this cross-reference subsection.</rdfs:comment>
	<rdfs:isDefinedBy rdf:resource="http://cybox.mitre.org/objects/File"/>
	<rdfs:label>First Object Number</rdfs:label>
</rdf:Description>
<!--  -->
<!-- http://cybox.mitre.org/objects/File#flateDecodeCount.nonObfuscated -->

<rdf:Description rdf:about="http://cybox.mitre.org/objects/File#flateDecodeCount.nonObfuscated">
	<rdf:type rdf:resource="http://www.w3.org/2002/07/owl#DatatypeProperty"/>
	<rdfs:range rdf:resource="http://www.w3.org/2001/XMLSchema#nonNegativeInteger"/>
	<rdfs:comment>Specifies the number of non-obfuscated occurrences of the '/FlateDecode' keyword in the PDF file.</rdfs:comment>
	<rdfs:isDefinedBy rdf:resource="http://cybox.mitre.org/objects/File"/>
	<rdfs:label>'/FlateDecode' Non-obfuscated Count</rdfs:label>
</rdf:Description>
<!--  -->
<!-- http://cybox.mitre.org/objects/File#flateDecodeCount.obfuscated -->

<rdf:Description rdf:about="http://cybox.mitre.org/objects/File#flateDecodeCount.obfuscated">
	<rdf:type rdf:resource="http://www.w3.org/2002/07/owl#DatatypeProperty"/>
	<rdfs:range rdf:resource="http://www.w3.org/2001/XMLSchema#nonNegativeInteger"/>
	<rdfs:comment>Specified the number of obfuscated occurrences of the '/FlateDecode' keyword in the PDF file with some form of obfuscation, such as with hexcodes.</rdfs:comment>
	<rdfs:isDefinedBy rdf:resource="http://cybox.mitre.org/objects/File"/>
	<rdfs:label>'/FlateDecode' Obfuscated Count</rdfs:label>
</rdf:Description>
<!--  -->
<!-- http://cybox.mitre.org/objects/File#fullControl -->

<rdf:Description rdf:about="http://cybox.mitre.org/objects/File#fullControl">
	<rdf:type rdf:resource="http://www.w3.org/2002/07/owl#DatatypeProperty"/>
	<rdfs:range rdf:resource="http://www.w3.org/2001/XMLSchema#boolean"/>
	<rdfs:comment>Specifies whether reading, writing, changing and deleting of the file is permitted.</rdfs:comment>
	<rdfs:isDefinedBy rdf:resource="http://cybox.mitre.org/objects/File"/>
	<rdfs:label>Full Control</rdfs:label>
</rdf:Description>
<!--  -->
<!-- http://cybox.mitre.org/objects/File#fullPath -->

<rdf:Description rdf:about="http://cybox.mitre.org/objects/File#fullPath">
	<rdf:type rdf:resource="http://www.w3.org/2002/07/owl#DatatypeProperty"/>
	<rdfs:range rdf:resource="http://www.w3.org/2001/XMLSchema#string"/>
	<rdfs:comment>Specifies the complete path to the file, including the device path.&#xD;
&#xD;
It should contain the contents that would otherwise be in the devicePath, filePath, and fileName fields, and can be used in case the producer is unable or does not wish to separate the devicePath, filePath, and fileName fields.  The fullPath field MUST NOT conflict with the devicePath,  filePath and fileName fields.</rdfs:comment>
	<rdfs:isDefinedBy rdf:datatype="http://www.w3.org/2001/XMLSchema#string">&lt;http://cybox.mitre.org/objects/File&gt;</rdfs:isDefinedBy>
	<rdfs:label>Full Path</rdfs:label>
</rdf:Description>
<!--  -->
<!-- http://cybox.mitre.org/objects/File#functionName -->

<rdf:Description rdf:about="http://cybox.mitre.org/objects/File#functionName">
	<rdf:type rdf:resource="http://www.w3.org/2002/07/owl#DatatypeProperty"/>
	<rdfs:range rdf:resource="http://www.w3.org/2001/XMLSchema#string"/>
	<rdfs:comment>Specifies the name of the function from the specified library.</rdfs:comment>
	<rdfs:isDefinedBy rdf:resource="http://cybox.mitre.org/objects/File"/>
	<rdfs:label>Function Name</rdfs:label>
</rdf:Description>
<!--  -->
<!-- http://cybox.mitre.org/objects/File#generationNumber -->

<rdf:Description rdf:about="http://cybox.mitre.org/objects/File#generationNumber">
	<rdf:type rdf:resource="http://www.w3.org/2002/07/owl#DatatypeProperty"/>
	<rdfs:range rdf:resource="http://www.w3.org/2001/XMLSchema#nonNegativeInteger"/>
	<rdfs:comment>Specifies the 5-digit generation number to be used when an object with the same object number is created.</rdfs:comment>
	<rdfs:isDefinedBy rdf:resource="http://cybox.mitre.org/objects/File"/>
	<rdfs:label>Generation Number</rdfs:label>
</rdf:Description>
<!--  -->
<!-- http://cybox.mitre.org/objects/File#gexec -->

<rdf:Description rdf:about="http://cybox.mitre.org/objects/File#gexec">
	<rdf:type rdf:resource="http://www.w3.org/2002/07/owl#DatatypeProperty"/>
	<rdfs:range rdf:resource="http://www.w3.org/2001/XMLSchema#boolean"/>
	<rdfs:comment>Specifies whether or not the group owner of the file can execute it.</rdfs:comment>
	<rdfs:isDefinedBy rdf:resource="http://cybox.mitre.org/objects/File"/>
	<rdfs:label>gexec</rdfs:label>
</rdf:Description>
<!--  -->
<!-- http://cybox.mitre.org/objects/File#globalPtr.size -->

<rdf:Description rdf:about="http://cybox.mitre.org/objects/File#globalPtr.size">
	<rdf:type rdf:resource="http://www.w3.org/2002/07/owl#DatatypeProperty"/>
	<rdfs:range rdf:resource="http://www.w3.org/2001/XMLSchema#nonNegativeInteger"/>
	<rdfs:comment>Specifies the size of the data structure, in bytes, of the Global Pointer Register</rdfs:comment>
	<rdfs:isDefinedBy rdf:resource="http://cybox.mitre.org/objects/File"/>
	<rdfs:label>Global Pointer Register Size</rdfs:label>
</rdf:Description>
<!--  -->
<!-- http://cybox.mitre.org/objects/File#globalPtr.virtualAddress -->

<rdf:Description rdf:about="http://cybox.mitre.org/objects/File#globalPtr.virtualAddress">
	<rdf:type rdf:resource="http://www.w3.org/2002/07/owl#DatatypeProperty"/>
	<rdfs:range rdf:resource="http://www.w3.org/2001/XMLSchema#hexBinary"/>
	<rdfs:comment>Specifies the relative virtual address (RVA) of the Global Pointer Register.</rdfs:comment>
	<rdfs:isDefinedBy rdf:resource="http://cybox.mitre.org/objects/File"/>
	<rdfs:label>Global Pointer Register Virtual Address</rdfs:label>
</rdf:Description>
<!--  -->
<!-- http://cybox.mitre.org/objects/File#gread -->

<rdf:Description rdf:about="http://cybox.mitre.org/objects/File#gread">
	<rdf:type rdf:resource="http://www.w3.org/2002/07/owl#DatatypeProperty"/>
	<rdfs:range rdf:resource="http://www.w3.org/2001/XMLSchema#boolean"/>
	<rdfs:comment>Specifies whether or not the group owner of the file can read its contents.</rdfs:comment>
	<rdfs:isDefinedBy rdf:resource="http://cybox.mitre.org/objects/File"/>
	<rdfs:label>gread</rdfs:label>
</rdf:Description>
<!--  -->
<!-- http://cybox.mitre.org/objects/File#groupOwner -->

<rdf:Description rdf:about="http://cybox.mitre.org/objects/File#groupOwner">
	<rdf:type rdf:resource="http://www.w3.org/2002/07/owl#DatatypeProperty"/>
	<rdfs:range rdf:resource="http://www.w3.org/2001/XMLSchema#string"/>
	<rdfs:comment>Specifies the name of the group which owns the file.</rdfs:comment>
	<rdfs:isDefinedBy rdf:resource="http://cybox.mitre.org/objects/File"/>
	<rdfs:label>Group Owner</rdfs:label>
</rdf:Description>
<!--  -->
<!-- http://cybox.mitre.org/objects/File#gwrite -->

<rdf:Description rdf:about="http://cybox.mitre.org/objects/File#gwrite">
	<rdf:type rdf:resource="http://www.w3.org/2002/07/owl#DatatypeProperty"/>
	<rdfs:range rdf:resource="http://www.w3.org/2001/XMLSchema#boolean"/>
	<rdfs:comment>Specifies whether or not the group owner of the file can write to it.</rdfs:comment>
	<rdfs:isDefinedBy rdf:resource="http://cybox.mitre.org/objects/File"/>
	<rdfs:label>gwrite</rdfs:label>
</rdf:Description>
<!--  -->
<!-- http://cybox.mitre.org/objects/File#hashValue -->

<rdf:Description rdf:about="http://cybox.mitre.org/objects/File#hashValue">
	<rdf:type rdf:resource="http://www.w3.org/2002/07/owl#DatatypeProperty"/>
	<rdfs:range rdf:resource="http://www.w3.org/2001/XMLSchema#string"/>
	<rdfs:comment>Specifies the values, in the format of 'hash-type':'hash-value', for any hash computed for the PDF indirect object.</rdfs:comment>
	<rdfs:isDefinedBy rdf:resource="http://cybox.mitre.org/objects/File"/>
	<rdfs:label>Hash Value</rdfs:label>
</rdf:Description>
<!--  -->
<!-- http://cybox.mitre.org/objects/File#headerHash.value -->

<rdf:Description rdf:about="http://cybox.mitre.org/objects/File#headerHash.value">
	<rdf:type rdf:resource="http://www.w3.org/2002/07/owl#DatatypeProperty"/>
	<rdfs:range rdf:resource="http://www.w3.org/2001/XMLSchema#string"/>
	<rdfs:comment>Specifies the values, in the format of 'hash-type':'hash-value', for any hash computed using the header of the specified PE binary section as input.</rdfs:comment>
	<rdfs:isDefinedBy rdf:resource="http://cybox.mitre.org/objects/File"/>
	<rdfs:label>Header Hash Value</rdfs:label>
</rdf:Description>
<!--  -->
<!-- http://cybox.mitre.org/objects/File#hidden -->

<rdf:Description rdf:about="http://cybox.mitre.org/objects/File#hidden">
	<rdf:type rdf:resource="http://www.w3.org/2002/07/owl#DatatypeProperty"/>
	<rdfs:range rdf:resource="http://www.w3.org/2001/XMLSchema#boolean"/>
	<rdfs:comment>Specifies a file or directory is hidden, as denoted by the constant value, 0x2. It is not included in an ordinary directory listing.</rdfs:comment>
	<rdfs:isDefinedBy rdf:resource="http://cybox.mitre.org/objects/File"/>
	<rdfs:label>Hidden</rdfs:label>
</rdf:Description>
<!--  -->
<!-- http://cybox.mitre.org/objects/File#hint -->

<rdf:Description rdf:about="http://cybox.mitre.org/objects/File#hint">
	<rdf:type rdf:resource="http://www.w3.org/2002/07/owl#DatatypeProperty"/>
	<rdfs:range rdf:resource="http://www.w3.org/2001/XMLSchema#hexBinary"/>
	<rdfs:comment>Specifies the index into the export table of the library that the function is found in.</rdfs:comment>
	<rdfs:isDefinedBy rdf:resource="http://cybox.mitre.org/objects/File"/>
	<rdfs:label>Hint</rdfs:label>
</rdf:Description>
<!--  -->
<!-- http://cybox.mitre.org/objects/File#iNode -->

<rdf:Description rdf:about="http://cybox.mitre.org/objects/File#iNode">
	<rdf:type rdf:resource="http://www.w3.org/2002/07/owl#DatatypeProperty"/>
	<rdfs:range rdf:resource="http://www.w3.org/2001/XMLSchema#unsignedLong"/>
	<rdfs:comment>Specifies the inode, or index node, value of the file.</rdfs:comment>
	<rdfs:isDefinedBy rdf:resource="http://cybox.mitre.org/objects/File"/>
	<rdfs:label>iNode</rdfs:label>
</rdf:Description>
<!--  -->
<!-- http://cybox.mitre.org/objects/File#imageBase -->

<rdf:Description rdf:about="http://cybox.mitre.org/objects/File#imageBase">
	<rdf:type rdf:resource="http://www.w3.org/2002/07/owl#DatatypeProperty"/>
	<rdfs:range rdf:resource="http://www.w3.org/2001/XMLSchema#hexBinary"/>
	<rdfs:comment>Specifies the preferred address of the first byte of the driver's image when it is loaded into memory.</rdfs:comment>
	<rdfs:isDefinedBy rdf:resource="http://cybox.mitre.org/objects/File"/>
	<rdfs:label>Image Base</rdfs:label>
</rdf:Description>
<!--  -->
<!-- http://cybox.mitre.org/objects/File#imageFileFormat -->

<rdf:Description rdf:about="http://cybox.mitre.org/objects/File#imageFileFormat">
	<rdf:type rdf:resource="http://www.w3.org/2002/07/owl#DatatypeProperty"/>
	<rdfs:range rdf:resource="http://www.w3.org/2001/XMLSchema#string"/>
	<rdfs:comment>Specifies the name of the file format used in the image file.</rdfs:comment>
	<rdfs:isDefinedBy rdf:resource="http://cybox.mitre.org/objects/File"/>
	<rdfs:label>Image File Format</rdfs:label>
</rdf:Description>
<!--  -->
<!-- http://cybox.mitre.org/objects/File#imageHeight -->

<rdf:Description rdf:about="http://cybox.mitre.org/objects/File#imageHeight">
	<rdf:type rdf:resource="http://www.w3.org/2002/07/owl#DatatypeProperty"/>
	<rdfs:range rdf:resource="http://www.w3.org/2001/XMLSchema#integer"/>
	<rdfs:comment>Specifies the height of the image in the image file, in pixels.</rdfs:comment>
	<rdfs:isDefinedBy rdf:resource="http://cybox.mitre.org/objects/File"/>
	<rdfs:label>Image Height</rdfs:label>
</rdf:Description>
<!--  -->
<!-- http://cybox.mitre.org/objects/File#imageIsCompressed -->

<rdf:Description rdf:about="http://cybox.mitre.org/objects/File#imageIsCompressed">
	<rdf:type rdf:resource="http://www.w3.org/2002/07/owl#DatatypeProperty"/>
	<rdfs:range rdf:resource="http://www.w3.org/2001/XMLSchema#boolean"/>
	<rdfs:comment>Specifies whether the image in the image file is compressed.</rdfs:comment>
	<rdfs:isDefinedBy rdf:resource="http://cybox.mitre.org/objects/File"/>
	<rdfs:label>Compressed Image</rdfs:label>
</rdf:Description>
<!--  -->
<!-- http://cybox.mitre.org/objects/File#imageSize -->

<rdf:Description rdf:about="http://cybox.mitre.org/objects/File#imageSize">
	<rdf:type rdf:resource="http://www.w3.org/2002/07/owl#DatatypeProperty"/>
	<rdfs:range rdf:resource="http://www.w3.org/2001/XMLSchema#hexBinary"/>
	<rdfs:comment>Specifies the size of the driver's image, in bytes.</rdfs:comment>
	<rdfs:isDefinedBy rdf:resource="http://cybox.mitre.org/objects/File"/>
	<rdfs:label>Image Size</rdfs:label>
</rdf:Description>
<!--  -->
<!-- http://cybox.mitre.org/objects/File#imageWidth -->

<rdf:Description rdf:about="http://cybox.mitre.org/objects/File#imageWidth">
	<rdf:type rdf:resource="http://www.w3.org/2002/07/owl#DatatypeProperty"/>
	<rdfs:range rdf:resource="http://www.w3.org/2001/XMLSchema#integer"/>
	<rdfs:comment>Specifies the width of the image in the image file, in pixels.</rdfs:comment>
	<rdfs:isDefinedBy rdf:resource="http://cybox.mitre.org/objects/File"/>
	<rdfs:label>Image Width</rdfs:label>
</rdf:Description>
<!--  -->
<!-- http://cybox.mitre.org/objects/File#importAddressTable.size -->

<rdf:Description rdf:about="http://cybox.mitre.org/objects/File#importAddressTable.size">
	<rdf:type rdf:resource="http://www.w3.org/2002/07/owl#DatatypeProperty"/>
	<rdfs:range rdf:resource="http://www.w3.org/2001/XMLSchema#nonNegativeInteger"/>
	<rdfs:comment>Specifies the size of the data structure, in bytes, of the Import Address Table data directory.</rdfs:comment>
	<rdfs:isDefinedBy rdf:resource="http://cybox.mitre.org/objects/File"/>
	<rdfs:label>Import Address Table Size</rdfs:label>
</rdf:Description>
<!--  -->
<!-- http://cybox.mitre.org/objects/File#importAddressTable.virtualAddress -->

<rdf:Description rdf:about="http://cybox.mitre.org/objects/File#importAddressTable.virtualAddress">
	<rdf:type rdf:resource="http://www.w3.org/2002/07/owl#DatatypeProperty"/>
	<rdfs:range rdf:resource="http://www.w3.org/2001/XMLSchema#hexBinary"/>
	<rdfs:comment>Specifies the relative virtual address (RVA) of the Import Address Table data directory.</rdfs:comment>
	<rdfs:isDefinedBy rdf:resource="http://cybox.mitre.org/objects/File"/>
	<rdfs:label>Import Address Table Virtual Address</rdfs:label>
</rdf:Description>
<!--  -->
<!-- http://cybox.mitre.org/objects/File#importFileName -->

<rdf:Description rdf:about="http://cybox.mitre.org/objects/File#importFileName">
	<rdf:type rdf:resource="http://www.w3.org/2002/07/owl#DatatypeProperty"/>
	<rdfs:range rdf:resource="http://www.w3.org/2001/XMLSchema#string"/>
	<rdfs:comment></rdfs:comment>
	<rdfs:isDefinedBy rdf:datatype="http://www.w3.org/2001/XMLSchema#string">&lt;http://cybox.mitre.org/objects/File&gt;</rdfs:isDefinedBy>
	<rdfs:label>import file name</rdfs:label>
</rdf:Description>
<!--  -->
<!-- http://cybox.mitre.org/objects/File#importOrdinal -->

<rdf:Description rdf:about="http://cybox.mitre.org/objects/File#importOrdinal">
	<rdf:type rdf:resource="http://www.w3.org/2002/07/owl#DatatypeProperty"/>
	<rdfs:range rdf:resource="http://www.w3.org/2001/XMLSchema#nonNegativeInteger"/>
	<rdfs:comment>Specifies the ordinal value (index) of the function in the library that is found in.</rdfs:comment>
	<rdfs:isDefinedBy rdf:resource="http://cybox.mitre.org/objects/File"/>
	<rdfs:label>Import Ordinal</rdfs:label>
</rdf:Description>
<!--  -->
<!-- http://cybox.mitre.org/objects/File#importTable.size -->

<rdf:Description rdf:about="http://cybox.mitre.org/objects/File#importTable.size">
	<rdf:type rdf:resource="http://www.w3.org/2002/07/owl#DatatypeProperty"/>
	<rdfs:range rdf:resource="http://www.w3.org/2001/XMLSchema#nonNegativeInteger"/>
	<rdfs:comment>Specifies the size of the data structure, in bytes, of the Import Table data directory.</rdfs:comment>
	<rdfs:isDefinedBy rdf:resource="http://cybox.mitre.org/objects/File"/>
	<rdfs:label>Import Table Size</rdfs:label>
</rdf:Description>
<!--  -->
<!-- http://cybox.mitre.org/objects/File#importTable.virtualAddress -->

<rdf:Description rdf:about="http://cybox.mitre.org/objects/File#importTable.virtualAddress">
	<rdf:type rdf:resource="http://www.w3.org/2002/07/owl#DatatypeProperty"/>
	<rdfs:range rdf:resource="http://www.w3.org/2001/XMLSchema#hexBinary"/>
	<rdfs:comment>Specifies the relative virtual address (RVA) of the data structure of the Import Table data directory</rdfs:comment>
	<rdfs:isDefinedBy rdf:resource="http://cybox.mitre.org/objects/File"/>
	<rdfs:label>Import Table Virtual Address</rdfs:label>
</rdf:Description>
<!--  -->
<!-- http://cybox.mitre.org/objects/File#importVirtualAddress -->

<rdf:Description rdf:about="http://cybox.mitre.org/objects/File#importVirtualAddress">
	<rdf:type rdf:resource="http://www.w3.org/2002/07/owl#DatatypeProperty"/>
	<rdfs:range rdf:resource="http://www.w3.org/2001/XMLSchema#hexBinary"/>
	<rdfs:comment>Specifies the relative virtual address (RVA) of the PE binary library import.</rdfs:comment>
	<rdfs:isDefinedBy rdf:resource="http://cybox.mitre.org/objects/File"/>
	<rdfs:label>Import Virtual Address</rdfs:label>
</rdf:Description>
<!--  -->
<!-- http://cybox.mitre.org/objects/File#indirectObjectOffset -->

<rdf:Description rdf:about="http://cybox.mitre.org/objects/File#indirectObjectOffset">
	<rdf:type rdf:resource="http://www.w3.org/2002/07/owl#DatatypeProperty"/>
	<rdfs:range rdf:resource="http://www.w3.org/2001/XMLSchema#positiveInteger"/>
	<rdfs:comment>Specifies the offset of the PDF indirect object from the beginning of the file, in bytes.</rdfs:comment>
	<rdfs:isDefinedBy rdf:resource="http://cybox.mitre.org/objects/File"/>
	<rdfs:label>Indirect Object Offset</rdfs:label>
</rdf:Description>
<!--  -->
<!-- http://cybox.mitre.org/objects/File#initiallyVisible -->

<rdf:Description rdf:about="http://cybox.mitre.org/objects/File#initiallyVisible">
	<rdf:type rdf:resource="http://www.w3.org/2002/07/owl#DatatypeProperty"/>
	<rdfs:range rdf:resource="http://www.w3.org/2001/XMLSchema#boolean"/>
	<rdfs:comment></rdfs:comment>
	<rdfs:isDefinedBy rdf:datatype="http://www.w3.org/2001/XMLSchema#string">&lt;http://cybox.mitre.org/objects/File&gt;</rdfs:isDefinedBy>
	<rdfs:label>initially visible</rdfs:label>
</rdf:Description>
<!--  -->
<!-- http://cybox.mitre.org/objects/File#integrityStream -->

<rdf:Description rdf:about="http://cybox.mitre.org/objects/File#integrityStream">
	<rdf:type rdf:resource="http://www.w3.org/2002/07/owl#DatatypeProperty"/>
	<rdfs:range rdf:resource="http://www.w3.org/2001/XMLSchema#boolean"/>
	<rdfs:comment>Specifies the directory or user data stream is configured with integrity (only supported on ReFS volumes), as denoted by the constant value, 0x8000. It is not included in an ordinary directory listing. The integrity setting persists with the file if it's renamed. If a file is copied the destination file will have integrity set if either the source file or destination directory have integrity set. NOTE: This flag is supported ONLY for Windows Server 8 Beta and later</rdfs:comment>
	<rdfs:isDefinedBy rdf:resource="http://cybox.mitre.org/objects/File"/>
	<rdfs:label>Integrity Stream</rdfs:label>
</rdf:Description>
<!--  -->
<!-- http://cybox.mitre.org/objects/File#internalName -->

<rdf:Description rdf:about="http://cybox.mitre.org/objects/File#internalName">
	<rdf:type rdf:resource="http://www.w3.org/2002/07/owl#DatatypeProperty"/>
	<rdfs:range rdf:resource="http://www.w3.org/2001/XMLSchema#string"/>
	<rdfs:comment>Specifies  the internal name of the file, if one exists - for example, a module name if the file is a dynamic-link library.   If the file has no internal name, this string should be the original filename, without extension.</rdfs:comment>
	<rdfs:isDefinedBy rdf:resource="http://cybox.mitre.org/objects/File"/>
	<rdfs:label>Internal Name</rdfs:label>
</rdf:Description>
<!--  -->
<!-- http://cybox.mitre.org/objects/File#isMasqueraded -->

<rdf:Description rdf:about="http://cybox.mitre.org/objects/File#isMasqueraded">
	<rdf:type rdf:resource="http://www.w3.org/2002/07/owl#DatatypeProperty"/>
	<rdfs:range rdf:resource="http://www.w3.org/2001/XMLSchema#boolean"/>
	<rdfs:comment>Specifies whether the file is masqueraded as another type of file; e.g., a PDF file that has had its extension changed to TXT to masquerade itself as a text file.</rdfs:comment>
	<rdfs:isDefinedBy rdf:datatype="http://www.w3.org/2001/XMLSchema#string">&lt;http://cybox.mitre.org/objects/File&gt;</rdfs:isDefinedBy>
	<rdfs:label>Masqueraded</rdfs:label>
</rdf:Description>
<!--  -->
<!-- http://cybox.mitre.org/objects/File#isPacked -->

<rdf:Description rdf:about="http://cybox.mitre.org/objects/File#isPacked">
	<rdf:type rdf:resource="http://www.w3.org/2002/07/owl#DatatypeProperty"/>
	<rdfs:range rdf:resource="http://www.w3.org/2001/XMLSchema#boolean"/>
	<rdfs:comment>Specifies whether the file is packed or not.</rdfs:comment>
	<rdfs:isDefinedBy rdf:datatype="http://www.w3.org/2001/XMLSchema#string">&lt;http://cybox.mitre.org/objects/File&gt;</rdfs:isDefinedBy>
	<rdfs:label>Packed</rdfs:label>
</rdf:Description>
<!--  -->
<!-- http://cybox.mitre.org/objects/File#javascriptCount.nonObfuscated -->

<rdf:Description rdf:about="http://cybox.mitre.org/objects/File#javascriptCount.nonObfuscated">
	<rdf:type rdf:resource="http://www.w3.org/2002/07/owl#DatatypeProperty"/>
	<rdfs:range rdf:resource="http://www.w3.org/2001/XMLSchema#nonNegativeInteger"/>
	<rdfs:comment>Specifies the number of non-obfuscated occurrences of the '/JavaScript' keyword in the PDF file.</rdfs:comment>
	<rdfs:isDefinedBy rdf:resource="http://cybox.mitre.org/objects/File"/>
	<rdfs:label>'/JavaScript' Non-obfuscated Count</rdfs:label>
</rdf:Description>
<!--  -->
<!-- http://cybox.mitre.org/objects/File#javascriptCount.obfuscated -->

<rdf:Description rdf:about="http://cybox.mitre.org/objects/File#javascriptCount.obfuscated">
	<rdf:type rdf:resource="http://www.w3.org/2002/07/owl#DatatypeProperty"/>
	<rdfs:range rdf:resource="http://www.w3.org/2001/XMLSchema#nonNegativeInteger"/>
	<rdfs:comment>Specifies the number of obfuscated occurrences of the '/JavaScript' keyword in the PDF file with some form of obfuscation, such as with hexcodes.</rdfs:comment>
	<rdfs:isDefinedBy rdf:resource="http://cybox.mitre.org/objects/File"/>
	<rdfs:label>'/JavaScript' Obfuscated Count</rdfs:label>
</rdf:Description>
<!--  -->
<!-- http://cybox.mitre.org/objects/File#jbig2DecodeCount.nonObfuscated -->

<rdf:Description rdf:about="http://cybox.mitre.org/objects/File#jbig2DecodeCount.nonObfuscated">
	<rdf:type rdf:resource="http://www.w3.org/2002/07/owl#DatatypeProperty"/>
	<rdfs:range rdf:resource="http://www.w3.org/2001/XMLSchema#nonNegativeInteger"/>
	<rdfs:comment>Specifies the number of non-obfuscated occurrences of the '/JBIG2Decode' keyword in the PDF file.</rdfs:comment>
	<rdfs:isDefinedBy rdf:resource="http://cybox.mitre.org/objects/File"/>
	<rdfs:label>'/JBIG2Decode' Non-obfuscated Count</rdfs:label>
</rdf:Description>
<!--  -->
<!-- http://cybox.mitre.org/objects/File#jbig2DecodeCount.obfuscated -->

<rdf:Description rdf:about="http://cybox.mitre.org/objects/File#jbig2DecodeCount.obfuscated">
	<rdf:type rdf:resource="http://www.w3.org/2002/07/owl#DatatypeProperty"/>
	<rdfs:range rdf:resource="http://www.w3.org/2001/XMLSchema#nonNegativeInteger"/>
	<rdfs:comment>Specifies the number of obfuscated occurrences of the '/JBIG2Decode' keyword in the PDF file with some form of obfuscation, such as with hexcodes.</rdfs:comment>
	<rdfs:isDefinedBy rdf:resource="http://cybox.mitre.org/objects/File"/>
	<rdfs:label>'/JBIG2Decode' Obfuscated Count</rdfs:label>
</rdf:Description>
<!--  -->
<!-- http://cybox.mitre.org/objects/File#jsCount.nonObfuscated -->

<rdf:Description rdf:about="http://cybox.mitre.org/objects/File#jsCount.nonObfuscated">
	<rdf:type rdf:resource="http://www.w3.org/2002/07/owl#DatatypeProperty"/>
	<rdfs:range rdf:resource="http://www.w3.org/2001/XMLSchema#nonNegativeInteger"/>
	<rdfs:comment>Specifies the number of non-obfuscated occurrences of the '/JS' keyword in the PDF file.</rdfs:comment>
	<rdfs:isDefinedBy rdf:resource="http://cybox.mitre.org/objects/File"/>
	<rdfs:label>'/JS' Non-obfuscated Count</rdfs:label>
</rdf:Description>
<!--  -->
<!-- http://cybox.mitre.org/objects/File#jsCount.obfuscated -->

<rdf:Description rdf:about="http://cybox.mitre.org/objects/File#jsCount.obfuscated">
	<rdf:type rdf:resource="http://www.w3.org/2002/07/owl#DatatypeProperty"/>
	<rdfs:range rdf:resource="http://www.w3.org/2001/XMLSchema#nonNegativeInteger"/>
	<rdfs:comment>Specifies the number of obfuscated occurrences of the '/JS' keyword in the PDF file with some form of obfuscation, such as with hexcodes.</rdfs:comment>
	<rdfs:isDefinedBy rdf:resource="http://cybox.mitre.org/objects/File"/>
	<rdfs:label>'/JS' Obfuscated Count</rdfs:label>
</rdf:Description>
<!--  -->
<!-- http://cybox.mitre.org/objects/File#langID -->

<rdf:Description rdf:about="http://cybox.mitre.org/objects/File#langID">
	<rdf:type rdf:resource="http://www.w3.org/2002/07/owl#DatatypeProperty"/>
	<rdfs:range rdf:resource="http://www.w3.org/2001/XMLSchema#string"/>
	<rdfs:comment>Specifies the localization language identifier specified in the version-information resource.</rdfs:comment>
	<rdfs:isDefinedBy rdf:resource="http://cybox.mitre.org/objects/File"/>
	<rdfs:label>Lang ID</rdfs:label>
</rdf:Description>
<!--  -->
<!-- http://cybox.mitre.org/objects/File#language -->

<rdf:Description rdf:about="http://cybox.mitre.org/objects/File#language">
	<rdf:type rdf:resource="http://www.w3.org/2002/07/owl#DatatypeProperty"/>
	<rdfs:range rdf:resource="http://www.w3.org/2001/XMLSchema#string"/>
	<rdfs:comment>Specifies the name of the language (LANG) defined for the resource, if applicable.</rdfs:comment>
	<rdfs:isDefinedBy rdf:resource="http://cybox.mitre.org/objects/File"/>
	<rdfs:label>Language</rdfs:label>
</rdf:Description>
<!--  -->
<!-- http://cybox.mitre.org/objects/File#lastAccessedDateTime -->

<rdf:Description rdf:about="http://cybox.mitre.org/objects/File#lastAccessedDateTime">
	<rdf:type rdf:resource="http://www.w3.org/2002/07/owl#DatatypeProperty"/>
	<rdfs:range rdf:resource="http://www.w3.org/2001/XMLSchema#dateTime"/>
	<rdfs:comment>Specifies the date/time the file was last accessed.</rdfs:comment>
	<rdfs:isDefinedBy rdf:datatype="http://www.w3.org/2001/XMLSchema#string">&lt;http://cybox.mitre.org/objects/File&gt;</rdfs:isDefinedBy>
	<rdfs:label>Last Accessed Time</rdfs:label>
</rdf:Description>
<!--  -->
<!-- http://cybox.mitre.org/objects/File#lastCrossRefOffset -->

<rdf:Description rdf:about="http://cybox.mitre.org/objects/File#lastCrossRefOffset">
	<rdf:type rdf:resource="http://www.w3.org/2002/07/owl#DatatypeProperty"/>
	<rdfs:range rdf:resource="http://www.w3.org/2001/XMLSchema#positiveInteger"/>
	<rdfs:comment>Specifies the byte offset, relative to the beginning of the file, of the last cross-reference table contained in the file.</rdfs:comment>
	<rdfs:isDefinedBy rdf:resource="http://cybox.mitre.org/objects/File"/>
	<rdfs:label>Last Cross-Reference Offset</rdfs:label>
</rdf:Description>
<!--  -->
<!-- http://cybox.mitre.org/objects/File#lastModifiedDateTime -->

<rdf:Description rdf:about="http://cybox.mitre.org/objects/File#lastModifiedDateTime">
	<rdf:type rdf:resource="http://www.w3.org/2002/07/owl#DatatypeProperty"/>
	<rdfs:range rdf:resource="http://www.w3.org/2001/XMLSchema#dateTime"/>
	<rdfs:comment>Specifies the date/time the file was last modified.</rdfs:comment>
	<rdfs:isDefinedBy rdf:datatype="http://www.w3.org/2001/XMLSchema#string">&lt;http://cybox.mitre.org/objects/File&gt;</rdfs:isDefinedBy>
	<rdfs:label>Last Modified Time</rdfs:label>
</rdf:Description>
<!--  -->
<!-- http://cybox.mitre.org/objects/File#launchCount.nonObfuscated -->

<rdf:Description rdf:about="http://cybox.mitre.org/objects/File#launchCount.nonObfuscated">
	<rdf:type rdf:resource="http://www.w3.org/2002/07/owl#DatatypeProperty"/>
	<rdfs:range rdf:resource="http://www.w3.org/2001/XMLSchema#nonNegativeInteger"/>
	<rdfs:comment>Specifies the number of non-obfuscated occurrences of the '/Launch' keyword in the PDF file.</rdfs:comment>
	<rdfs:isDefinedBy rdf:resource="http://cybox.mitre.org/objects/File"/>
	<rdfs:label>'/Launch' Non-obfuscated Count</rdfs:label>
</rdf:Description>
<!--  -->
<!-- http://cybox.mitre.org/objects/File#launchCount.obfuscated -->

<rdf:Description rdf:about="http://cybox.mitre.org/objects/File#launchCount.obfuscated">
	<rdf:type rdf:resource="http://www.w3.org/2002/07/owl#DatatypeProperty"/>
	<rdfs:range rdf:resource="http://www.w3.org/2001/XMLSchema#nonNegativeInteger"/>
	<rdfs:comment>Specifies the number of obfuscated occurrences of the '/Launch' keyword in the PDF file with some form of obfuscation, such as with hexcodes.</rdfs:comment>
	<rdfs:isDefinedBy rdf:resource="http://cybox.mitre.org/objects/File"/>
	<rdfs:label>'/Launch' Obfuscated Count</rdfs:label>
</rdf:Description>
<!--  -->
<!-- http://cybox.mitre.org/objects/File#legalCopyright -->

<rdf:Description rdf:about="http://cybox.mitre.org/objects/File#legalCopyright">
	<rdf:type rdf:resource="http://www.w3.org/2002/07/owl#DatatypeProperty"/>
	<rdfs:range rdf:resource="http://www.w3.org/2001/XMLSchema#string"/>
	<rdfs:comment>Specifies the copyright notices that apply to the file. This should include the full text of all notices, legal symbols, copyright dates, and so on.</rdfs:comment>
	<rdfs:isDefinedBy rdf:resource="http://cybox.mitre.org/objects/File"/>
	<rdfs:label>Legal Copyright</rdfs:label>
</rdf:Description>
<!--  -->
<!-- http://cybox.mitre.org/objects/File#legalTrademarks -->

<rdf:Description rdf:about="http://cybox.mitre.org/objects/File#legalTrademarks">
	<rdf:type rdf:resource="http://www.w3.org/2002/07/owl#DatatypeProperty"/>
	<rdfs:range rdf:resource="http://www.w3.org/2001/XMLSchema#string"/>
	<rdfs:comment>Specifies the trademarks and registered trademarks that apply to the file. This should include the full text of all notices, legal symbols, trademark numbers, and so on.</rdfs:comment>
	<rdfs:isDefinedBy rdf:resource="http://cybox.mitre.org/objects/File"/>
	<rdfs:label>Legal Trademarks</rdfs:label>
</rdf:Description>
<!--  -->
<!-- http://cybox.mitre.org/objects/File#loadConfigTable.size -->

<rdf:Description rdf:about="http://cybox.mitre.org/objects/File#loadConfigTable.size">
	<rdf:type rdf:resource="http://www.w3.org/2002/07/owl#DatatypeProperty"/>
	<rdfs:range rdf:resource="http://www.w3.org/2001/XMLSchema#nonNegativeInteger"/>
	<rdfs:comment>Specifies the size of the data structure, in bytes, of the Load Configuration Table.</rdfs:comment>
	<rdfs:isDefinedBy rdf:resource="http://cybox.mitre.org/objects/File"/>
	<rdfs:label>Load Configuration Table Size</rdfs:label>
</rdf:Description>
<!--  -->
<!-- http://cybox.mitre.org/objects/File#loadConfigTable.virtualAddress -->

<rdf:Description rdf:about="http://cybox.mitre.org/objects/File#loadConfigTable.virtualAddress">
	<rdf:type rdf:resource="http://www.w3.org/2002/07/owl#DatatypeProperty"/>
	<rdfs:range rdf:resource="http://www.w3.org/2001/XMLSchema#hexBinary"/>
	<rdfs:comment>Specifies the relative virtual address (RVA) of the Load Configuration Table</rdfs:comment>
	<rdfs:isDefinedBy rdf:resource="http://cybox.mitre.org/objects/File"/>
	<rdfs:label>Load Configuration Table Virtual Address</rdfs:label>
</rdf:Description>
<!--  -->
<!-- http://cybox.mitre.org/objects/File#lzwDecodeCount.nonObfuscated -->

<rdf:Description rdf:about="http://cybox.mitre.org/objects/File#lzwDecodeCount.nonObfuscated">
	<rdf:type rdf:resource="http://www.w3.org/2002/07/owl#DatatypeProperty"/>
	<rdfs:range rdf:resource="http://www.w3.org/2001/XMLSchema#nonNegativeInteger"/>
	<rdfs:comment>Specifies the number of non-obfuscated occurrences of the '/LZWDecode' keyword in the PDF file.</rdfs:comment>
	<rdfs:isDefinedBy rdf:resource="http://cybox.mitre.org/objects/File"/>
	<rdfs:label>'/LZWDecode' Non-obfuscated Count</rdfs:label>
</rdf:Description>
<!--  -->
<!-- http://cybox.mitre.org/objects/File#lzwDecodeCount.obfuscated -->

<rdf:Description rdf:about="http://cybox.mitre.org/objects/File#lzwDecodeCount.obfuscated">
	<rdf:type rdf:resource="http://www.w3.org/2002/07/owl#DatatypeProperty"/>
	<rdfs:range rdf:resource="http://www.w3.org/2001/XMLSchema#nonNegativeInteger"/>
	<rdfs:comment>Specifies the number of obfuscated occurrences of the '/LZWDecode' keyword in the PDF file with some form of obfuscation, such as with hexcodes.</rdfs:comment>
	<rdfs:isDefinedBy rdf:resource="http://cybox.mitre.org/objects/File"/>
	<rdfs:label>'/LZWDecode' Obfuscated Count</rdfs:label>
</rdf:Description>
<!--  -->
<!-- http://cybox.mitre.org/objects/File#magicNumber -->

<rdf:Description rdf:about="http://cybox.mitre.org/objects/File#magicNumber">
	<rdf:type rdf:resource="http://www.w3.org/2002/07/owl#DatatypeProperty"/>
	<rdfs:range rdf:resource="http://www.w3.org/2001/XMLSchema#hexBinary"/>
	<rdfs:comment>Specifies the particular magic number (typically a hexadecimal constant used to identify a file format) corresponding to the file, if applicable.</rdfs:comment>
	<rdfs:isDefinedBy rdf:datatype="http://www.w3.org/2001/XMLSchema#string">&lt;http://cybox.mitre.org/objects/File&gt;</rdfs:isDefinedBy>
	<rdfs:label>Magic Number</rdfs:label>
</rdf:Description>
<!--  -->
<!-- http://cybox.mitre.org/objects/File#modify -->

<rdf:Description rdf:about="http://cybox.mitre.org/objects/File#modify">
	<rdf:type rdf:resource="http://www.w3.org/2002/07/owl#DatatypeProperty"/>
	<rdfs:range rdf:resource="http://www.w3.org/2001/XMLSchema#boolean"/>
	<rdfs:comment>Specifies whether reading and writing or deletion of the file is permitted.</rdfs:comment>
	<rdfs:isDefinedBy rdf:resource="http://cybox.mitre.org/objects/File"/>
	<rdfs:label>Modify</rdfs:label>
</rdf:Description>
<!--  -->
<!-- http://cybox.mitre.org/objects/File#noScrubData -->

<rdf:Description rdf:about="http://cybox.mitre.org/objects/File#noScrubData">
	<rdf:type rdf:resource="http://www.w3.org/2002/07/owl#DatatypeProperty"/>
	<rdfs:range rdf:resource="http://www.w3.org/2001/XMLSchema#boolean"/>
	<rdfs:comment>The user data stream not to be read by the background data integrity scanner (AKA scrubber), as denoted by the constant value, 0x20000. When set on a directory it only provides inheritance. This flag is only supported on Storage Spaces and ReFS volumes in Windows 8 and Windows Server 8 Beta and later. It is not included in an ordinary directory listing</rdfs:comment>
	<rdfs:isDefinedBy rdf:resource="http://cybox.mitre.org/objects/File"/>
	<rdfs:label>No Scrub Data</rdfs:label>
</rdf:Description>
<!--  -->
<!-- http://cybox.mitre.org/objects/File#nonStreamContents -->

<rdf:Description rdf:about="http://cybox.mitre.org/objects/File#nonStreamContents">
	<rdf:type rdf:resource="http://www.w3.org/2002/07/owl#DatatypeProperty"/>
	<rdfs:range rdf:resource="http://www.w3.org/2001/XMLSchema#string"/>
	<rdfs:comment>Specifies the raw contents of the PDF indirect object excluding any stream data (i.e. everything after the 'obj' keyword and before the 'endobj' keyword up to but not including anything between the 'stream' and 'endstream' keywords) as a string enclosed in an XML CDATA section.</rdfs:comment>
	<rdfs:isDefinedBy rdf:resource="http://cybox.mitre.org/objects/File"/>
	<rdfs:label>Non-stream Contents</rdfs:label>
</rdf:Description>
<!--  -->
<!-- http://cybox.mitre.org/objects/File#normal -->

<rdf:Description rdf:about="http://cybox.mitre.org/objects/File#normal">
	<rdf:type rdf:resource="http://www.w3.org/2002/07/owl#DatatypeProperty"/>
	<rdfs:range rdf:resource="http://www.w3.org/2001/XMLSchema#boolean"/>
	<rdfs:comment>Specifies a file that has no other attributes set, and is only valid when this attribute is used alone, as denoted by the constant value, 0x80.</rdfs:comment>
	<rdfs:isDefinedBy rdf:resource="http://cybox.mitre.org/objects/File"/>
	<rdfs:label>Normal</rdfs:label>
</rdf:Description>
<!--  -->
<!-- http://cybox.mitre.org/objects/File#notContentIndexed -->

<rdf:Description rdf:about="http://cybox.mitre.org/objects/File#notContentIndexed">
	<rdf:type rdf:resource="http://www.w3.org/2002/07/owl#DatatypeProperty"/>
	<rdfs:range rdf:resource="http://www.w3.org/2001/XMLSchema#boolean"/>
	<rdfs:comment>Specifies that a file is not to be indexed by the content indexing service, as denoted by the constant value, 0x2000.</rdfs:comment>
	<rdfs:isDefinedBy rdf:resource="http://cybox.mitre.org/objects/File"/>
	<rdfs:label>Not Content Indexed</rdfs:label>
</rdf:Description>
<!--  -->
<!-- http://cybox.mitre.org/objects/File#numberOfAddresses -->

<rdf:Description rdf:about="http://cybox.mitre.org/objects/File#numberOfAddresses">
	<rdf:type rdf:resource="http://www.w3.org/2002/07/owl#DatatypeProperty"/>
	<rdfs:range rdf:resource="http://www.w3.org/2001/XMLSchema#long"/>
	<rdfs:comment>Specifies the number of addresses in the export data section's address table.</rdfs:comment>
	<rdfs:isDefinedBy rdf:resource="http://cybox.mitre.org/objects/File"/>
	<rdfs:label>Number of Addresses</rdfs:label>
</rdf:Description>
<!--  -->
<!-- http://cybox.mitre.org/objects/File#numberOfCrossRefTables -->

<rdf:Description rdf:about="http://cybox.mitre.org/objects/File#numberOfCrossRefTables">
	<rdf:type rdf:resource="http://www.w3.org/2002/07/owl#DatatypeProperty"/>
	<rdfs:range rdf:resource="http://www.w3.org/2001/XMLSchema#positiveInteger"/>
	<rdfs:comment>Specifies the number of cross-reference tables contained in the file.</rdfs:comment>
	<rdfs:isDefinedBy rdf:resource="http://cybox.mitre.org/objects/File"/>
	<rdfs:label>Number of Cross-Reference Tables</rdfs:label>
</rdf:Description>
<!--  -->
<!-- http://cybox.mitre.org/objects/File#numberOfIndirectObjects -->

<rdf:Description rdf:about="http://cybox.mitre.org/objects/File#numberOfIndirectObjects">
	<rdf:type rdf:resource="http://www.w3.org/2002/07/owl#DatatypeProperty"/>
	<rdfs:range rdf:resource="http://www.w3.org/2001/XMLSchema#positiveInteger"/>
	<rdfs:comment>Specifies the number of indirect PDF objects contained in the file.</rdfs:comment>
	<rdfs:isDefinedBy rdf:resource="http://cybox.mitre.org/objects/File"/>
	<rdfs:label>Number of Indirect Objects</rdfs:label>
</rdf:Description>
<!--  -->
<!-- http://cybox.mitre.org/objects/File#numberOfNames -->

<rdf:Description rdf:about="http://cybox.mitre.org/objects/File#numberOfNames">
	<rdf:type rdf:resource="http://www.w3.org/2002/07/owl#DatatypeProperty"/>
	<rdfs:range rdf:resource="http://www.w3.org/2001/XMLSchema#long"/>
	<rdfs:comment>Specifies the number of names in the export data section's name table.</rdfs:comment>
	<rdfs:isDefinedBy rdf:resource="http://cybox.mitre.org/objects/File"/>
	<rdfs:label>Number of Names</rdfs:label>
</rdf:Description>
<!--  -->
<!-- http://cybox.mitre.org/objects/File#numberOfObjects -->

<rdf:Description rdf:about="http://cybox.mitre.org/objects/File#numberOfObjects">
	<rdf:type rdf:resource="http://www.w3.org/2002/07/owl#DatatypeProperty"/>
	<rdfs:range rdf:resource="http://www.w3.org/2001/XMLSchema#nonNegativeInteger"/>
	<rdfs:comment>Specifies the number of objects for which there are corresponding entries in this cross-reference subsection.</rdfs:comment>
	<rdfs:isDefinedBy rdf:resource="http://cybox.mitre.org/objects/File"/>
	<rdfs:label>Number of Objects</rdfs:label>
</rdf:Description>
<!--  -->
<!-- http://cybox.mitre.org/objects/File#numberOfTrailers -->

<rdf:Description rdf:about="http://cybox.mitre.org/objects/File#numberOfTrailers">
	<rdf:type rdf:resource="http://www.w3.org/2002/07/owl#DatatypeProperty"/>
	<rdfs:range rdf:resource="http://www.w3.org/2001/XMLSchema#positiveInteger"/>
	<rdfs:comment>Specifies the number of trailers contained in the file.</rdfs:comment>
	<rdfs:isDefinedBy rdf:resource="http://cybox.mitre.org/objects/File"/>
	<rdfs:label>Number of Trailers</rdfs:label>
</rdf:Description>
<!--  -->
<!-- http://cybox.mitre.org/objects/File#numberofFunctions -->

<rdf:Description rdf:about="http://cybox.mitre.org/objects/File#numberofFunctions">
	<rdf:type rdf:resource="http://www.w3.org/2002/07/owl#DatatypeProperty"/>
	<rdfs:range rdf:resource="http://www.w3.org/2001/XMLSchema#long"/>
	<rdfs:comment>Specifies the total number of functions that are exported by the PE file.</rdfs:comment>
	<rdfs:isDefinedBy rdf:resource="http://cybox.mitre.org/objects/File"/>
	<rdfs:label>Number of Functions</rdfs:label>
</rdf:Description>
<!--  -->
<!-- http://cybox.mitre.org/objects/File#objStmCount.nonObfuscated -->

<rdf:Description rdf:about="http://cybox.mitre.org/objects/File#objStmCount.nonObfuscated">
	<rdf:type rdf:resource="http://www.w3.org/2002/07/owl#DatatypeProperty"/>
	<rdfs:range rdf:resource="http://www.w3.org/2001/XMLSchema#nonNegativeInteger"/>
	<rdfs:comment>Specifies the number of non-obfuscated occurrences of the '/ObjStm' keyword in the PDF file.</rdfs:comment>
	<rdfs:isDefinedBy rdf:resource="http://cybox.mitre.org/objects/File"/>
	<rdfs:label>'/ObjStm' Non-obfuscated Count</rdfs:label>
</rdf:Description>
<!--  -->
<!-- http://cybox.mitre.org/objects/File#objStmCount.obfuscated -->

<rdf:Description rdf:about="http://cybox.mitre.org/objects/File#objStmCount.obfuscated">
	<rdf:type rdf:resource="http://www.w3.org/2002/07/owl#DatatypeProperty"/>
	<rdfs:range rdf:resource="http://www.w3.org/2001/XMLSchema#nonNegativeInteger"/>
	<rdfs:comment>Specifies the number of obfuscated occurrences of the '/ObjStm' keyword in the PDF filewith some form of obfuscation, such as with hexcodes.</rdfs:comment>
	<rdfs:isDefinedBy rdf:resource="http://cybox.mitre.org/objects/File"/>
	<rdfs:label>pdf metadata.obj stm count obfuscated</rdfs:label>
</rdf:Description>
<!--  -->
<!-- http://cybox.mitre.org/objects/File#objectNumber -->

<rdf:Description rdf:about="http://cybox.mitre.org/objects/File#objectNumber">
	<rdf:type rdf:resource="http://www.w3.org/2002/07/owl#DatatypeProperty"/>
	<rdfs:range rdf:resource="http://www.w3.org/2001/XMLSchema#nonNegativeInteger"/>
	<rdfs:comment>Specifies the 10-digit object number of the next free object.</rdfs:comment>
	<rdfs:isDefinedBy rdf:resource="http://cybox.mitre.org/objects/File"/>
	<rdfs:label>Object Number</rdfs:label>
</rdf:Description>
<!--  -->
<!-- http://cybox.mitre.org/objects/File#oexec -->

<rdf:Description rdf:about="http://cybox.mitre.org/objects/File#oexec">
	<rdf:type rdf:resource="http://www.w3.org/2002/07/owl#DatatypeProperty"/>
	<rdfs:range rdf:resource="http://www.w3.org/2001/XMLSchema#boolean"/>
	<rdfs:comment>Specifies whether or not all other users can execute the file.</rdfs:comment>
	<rdfs:isDefinedBy rdf:resource="http://cybox.mitre.org/objects/File"/>
	<rdfs:label>oexec</rdfs:label>
</rdf:Description>
<!--  -->
<!-- http://cybox.mitre.org/objects/File#offline -->

<rdf:Description rdf:about="http://cybox.mitre.org/objects/File#offline">
	<rdf:type rdf:resource="http://www.w3.org/2002/07/owl#DatatypeProperty"/>
	<rdfs:range rdf:resource="http://www.w3.org/2001/XMLSchema#boolean"/>
	<rdfs:comment>Specifies that the data of a file is not available immediately, as denoted by the constant value, 0x1000. This attribute indicates that the file data is physically moved to offline storage. This attribute is used by Remote Storage, which is the hierarchical storage management software. Applications should not arbitrarily change this attribute.</rdfs:comment>
	<rdfs:isDefinedBy rdf:resource="http://cybox.mitre.org/objects/File"/>
	<rdfs:label>Offline</rdfs:label>
</rdf:Description>
<!--  -->
<!-- http://cybox.mitre.org/objects/File#offset -->

<rdf:Description rdf:about="http://cybox.mitre.org/objects/File#offset">
	<rdf:type rdf:resource="http://www.w3.org/2002/07/owl#DatatypeProperty"/>
	<rdfs:range rdf:resource="http://www.w3.org/2001/XMLSchema#positiveInteger"/>
	<rdfs:comment>Specifies the offset of the trailer from the beginning of the file, in bytes.</rdfs:comment>
	<rdfs:isDefinedBy rdf:resource="http://cybox.mitre.org/objects/File"/>
	<rdfs:label>Offset</rdfs:label>
</rdf:Description>
<!--  -->
<!-- http://cybox.mitre.org/objects/File#openActionCount.nonObfuscated -->

<rdf:Description rdf:about="http://cybox.mitre.org/objects/File#openActionCount.nonObfuscated">
	<rdf:type rdf:resource="http://www.w3.org/2002/07/owl#DatatypeProperty"/>
	<rdfs:range rdf:resource="http://www.w3.org/2001/XMLSchema#nonNegativeInteger"/>
	<rdfs:comment>Specifies the number of non-obfuscated occurrences of the '/OpenAction' keyword in the PDF file.</rdfs:comment>
	<rdfs:isDefinedBy rdf:resource="http://cybox.mitre.org/objects/File"/>
	<rdfs:label>'/OpenAction' Non-obfuscated Count</rdfs:label>
</rdf:Description>
<!--  -->
<!-- http://cybox.mitre.org/objects/File#openActionCount.obfuscated -->

<rdf:Description rdf:about="http://cybox.mitre.org/objects/File#openActionCount.obfuscated">
	<rdf:type rdf:resource="http://www.w3.org/2002/07/owl#DatatypeProperty"/>
	<rdfs:range rdf:resource="http://www.w3.org/2001/XMLSchema#nonNegativeInteger"/>
	<rdfs:comment>Specifies the number of obfuscated occurrences of the '/OpenAction' keyword in the PDF file with some form of obfuscation, such as with hexcodes.</rdfs:comment>
	<rdfs:isDefinedBy rdf:resource="http://cybox.mitre.org/objects/File"/>
	<rdfs:label>'/OpenAction' Obfuscated Count</rdfs:label>
</rdf:Description>
<!--  -->
<!-- http://cybox.mitre.org/objects/File#optionalHeader.addressOfEntryPoint -->

<rdf:Description rdf:about="http://cybox.mitre.org/objects/File#optionalHeader.addressOfEntryPoint">
	<rdf:type rdf:resource="http://www.w3.org/2002/07/owl#DatatypeProperty"/>
	<rdfs:range rdf:resource="http://www.w3.org/2001/XMLSchema#hexBinary"/>
	<rdfs:comment>Specifies the address of the entry point relative to the image base when the executable is loaded into memory. When there is no entry point (e.g., optional for DLLs), the value should be 0.</rdfs:comment>
	<rdfs:isDefinedBy rdf:resource="http://cybox.mitre.org/objects/File"/>
	<rdfs:label>Optional Header Address of Entry Point</rdfs:label>
</rdf:Description>
<!--  -->
<!-- http://cybox.mitre.org/objects/File#optionalHeader.baseOfCode -->

<rdf:Description rdf:about="http://cybox.mitre.org/objects/File#optionalHeader.baseOfCode">
	<rdf:type rdf:resource="http://www.w3.org/2002/07/owl#DatatypeProperty"/>
	<rdfs:range rdf:resource="http://www.w3.org/2001/XMLSchema#hexBinary"/>
	<rdfs:comment>Specifies the address that is relative to the image base of the beginning-of-code section when it is loaded into memory.</rdfs:comment>
	<rdfs:isDefinedBy rdf:resource="http://cybox.mitre.org/objects/File"/>
	<rdfs:label>Optional Header Base of Code</rdfs:label>
</rdf:Description>
<!--  -->
<!-- http://cybox.mitre.org/objects/File#optionalHeader.baseOfData -->

<rdf:Description rdf:about="http://cybox.mitre.org/objects/File#optionalHeader.baseOfData">
	<rdf:type rdf:resource="http://www.w3.org/2002/07/owl#DatatypeProperty"/>
	<rdfs:range rdf:resource="http://www.w3.org/2001/XMLSchema#hexBinary"/>
	<rdfs:comment>Specifies the address that is relative to the image base of the beginning-of-data section when it is loaded into memory.</rdfs:comment>
	<rdfs:isDefinedBy rdf:resource="http://cybox.mitre.org/objects/File"/>
	<rdfs:label>Optional Header Base of Data</rdfs:label>
</rdf:Description>
<!--  -->
<!-- http://cybox.mitre.org/objects/File#optionalHeader.checksum -->

<rdf:Description rdf:about="http://cybox.mitre.org/objects/File#optionalHeader.checksum">
	<rdf:type rdf:resource="http://www.w3.org/2002/07/owl#DatatypeProperty"/>
	<rdfs:range rdf:resource="http://www.w3.org/2001/XMLSchema#hexBinary"/>
	<rdfs:comment>Specifies the checksum of the PE file.</rdfs:comment>
	<rdfs:isDefinedBy rdf:resource="http://cybox.mitre.org/objects/File"/>
	<rdfs:label>Optional Header Checksum</rdfs:label>
</rdf:Description>
<!--  -->
<!-- http://cybox.mitre.org/objects/File#optionalHeader.dllCharacteristics -->

<rdf:Description rdf:about="http://cybox.mitre.org/objects/File#optionalHeader.dllCharacteristics">
	<rdf:type rdf:resource="http://www.w3.org/2002/07/owl#DatatypeProperty"/>
	<rdfs:range rdf:resource="http://www.w3.org/2001/XMLSchema#hexBinary"/>
	<rdfs:comment>Specifies flags that characterize the PE file.</rdfs:comment>
	<rdfs:isDefinedBy rdf:resource="http://cybox.mitre.org/objects/File"/>
	<rdfs:label>Optional Header DLL Characteristics</rdfs:label>
</rdf:Description>
<!--  -->
<!-- http://cybox.mitre.org/objects/File#optionalHeader.fileAlignment -->

<rdf:Description rdf:about="http://cybox.mitre.org/objects/File#optionalHeader.fileAlignment">
	<rdf:type rdf:resource="http://www.w3.org/2002/07/owl#DatatypeProperty"/>
	<rdfs:range rdf:resource="http://www.w3.org/2001/XMLSchema#hexBinary"/>
	<rdfs:comment>Specifies the factor (in bytes) that is used to align the raw data of sections in the image file.</rdfs:comment>
	<rdfs:isDefinedBy rdf:resource="http://cybox.mitre.org/objects/File"/>
	<rdfs:label>Optional Header File Alignment</rdfs:label>
</rdf:Description>
<!--  -->
<!-- http://cybox.mitre.org/objects/File#optionalHeader.hashValue -->

<rdf:Description rdf:about="http://cybox.mitre.org/objects/File#optionalHeader.hashValue">
	<rdf:type rdf:resource="http://www.w3.org/2002/07/owl#DatatypeProperty"/>
	<rdfs:range rdf:resource="http://www.w3.org/2001/XMLSchema#string"/>
	<rdfs:comment>Specifies the values, in the format of 'hash-type':'hash-value', for any hash computed using the specified PE binary optional header as input.</rdfs:comment>
	<rdfs:isDefinedBy rdf:resource="http://cybox.mitre.org/objects/File"/>
	<rdfs:label>Optional Header - Hash Value</rdfs:label>
</rdf:Description>
<!--  -->
<!-- http://cybox.mitre.org/objects/File#optionalHeader.imageBase -->

<rdf:Description rdf:about="http://cybox.mitre.org/objects/File#optionalHeader.imageBase">
	<rdf:type rdf:resource="http://www.w3.org/2002/07/owl#DatatypeProperty"/>
	<rdfs:range rdf:resource="http://www.w3.org/2001/XMLSchema#hexBinary"/>
	<rdfs:comment>Specifies the preferred address of the first byte of image when loaded into memory; must be a multiple of 64 K.</rdfs:comment>
	<rdfs:isDefinedBy rdf:resource="http://cybox.mitre.org/objects/File"/>
	<rdfs:label>Optional Header  Image Base</rdfs:label>
</rdf:Description>
<!--  -->
<!-- http://cybox.mitre.org/objects/File#optionalHeader.loaderFlags -->

<rdf:Description rdf:about="http://cybox.mitre.org/objects/File#optionalHeader.loaderFlags">
	<rdf:type rdf:resource="http://www.w3.org/2002/07/owl#DatatypeProperty"/>
	<rdfs:range rdf:resource="http://www.w3.org/2001/XMLSchema#hexBinary"/>
	<rdfs:comment>Reserved; must be 0.</rdfs:comment>
	<rdfs:isDefinedBy rdf:resource="http://cybox.mitre.org/objects/File"/>
	<rdfs:label>Optional Header Loader Flags</rdfs:label>
</rdf:Description>
<!--  -->
<!-- http://cybox.mitre.org/objects/File#optionalHeader.magic -->

<rdf:Description rdf:about="http://cybox.mitre.org/objects/File#optionalHeader.magic">
	<rdf:type rdf:resource="http://www.w3.org/2002/07/owl#DatatypeProperty"/>
	<rdfs:range rdf:resource="http://www.w3.org/2001/XMLSchema#hexBinary"/>
	<rdfs:comment>Specifies the unsigned integer that indicates the type of executable file.</rdfs:comment>
	<rdfs:isDefinedBy rdf:resource="http://cybox.mitre.org/objects/File"/>
	<rdfs:label>Optional Header Magic</rdfs:label>
</rdf:Description>
<!--  -->
<!-- http://cybox.mitre.org/objects/File#optionalHeader.majorImageVersion -->

<rdf:Description rdf:about="http://cybox.mitre.org/objects/File#optionalHeader.majorImageVersion">
	<rdf:type rdf:resource="http://www.w3.org/2002/07/owl#DatatypeProperty"/>
	<rdfs:range rdf:resource="http://www.w3.org/2001/XMLSchema#hexBinary"/>
	<rdfs:comment>Specifies the major version number of the image.</rdfs:comment>
	<rdfs:isDefinedBy rdf:resource="http://cybox.mitre.org/objects/File"/>
	<rdfs:label>Optional Header Major Image Version</rdfs:label>
</rdf:Description>
<!--  -->
<!-- http://cybox.mitre.org/objects/File#optionalHeader.majorLinkerVersion -->

<rdf:Description rdf:about="http://cybox.mitre.org/objects/File#optionalHeader.majorLinkerVersion">
	<rdf:type rdf:resource="http://www.w3.org/2002/07/owl#DatatypeProperty"/>
	<rdfs:range rdf:resource="http://www.w3.org/2001/XMLSchema#hexBinary"/>
	<rdfs:comment>Specifies the linker major version number.</rdfs:comment>
	<rdfs:isDefinedBy rdf:resource="http://cybox.mitre.org/objects/File"/>
	<rdfs:label>Optional Header Major Linker Version</rdfs:label>
</rdf:Description>
<!--  -->
<!-- http://cybox.mitre.org/objects/File#optionalHeader.majorOSVersion -->

<rdf:Description rdf:about="http://cybox.mitre.org/objects/File#optionalHeader.majorOSVersion">
	<rdf:type rdf:resource="http://www.w3.org/2002/07/owl#DatatypeProperty"/>
	<rdfs:range rdf:resource="http://www.w3.org/2001/XMLSchema#hexBinary"/>
	<rdfs:comment>Specifies the major version number of the required operating system.</rdfs:comment>
	<rdfs:isDefinedBy rdf:resource="http://cybox.mitre.org/objects/File"/>
	<rdfs:label>Optional Header Major OSV ersion</rdfs:label>
</rdf:Description>
<!--  -->
<!-- http://cybox.mitre.org/objects/File#optionalHeader.majorSubsystemVersion -->

<rdf:Description rdf:about="http://cybox.mitre.org/objects/File#optionalHeader.majorSubsystemVersion">
	<rdf:type rdf:resource="http://www.w3.org/2002/07/owl#DatatypeProperty"/>
	<rdfs:range rdf:resource="http://www.w3.org/2001/XMLSchema#hexBinary"/>
	<rdfs:comment>Specifies the major version number of the subsystem.</rdfs:comment>
	<rdfs:isDefinedBy rdf:resource="http://cybox.mitre.org/objects/File"/>
	<rdfs:label>Optional Header Major Subsystem Version</rdfs:label>
</rdf:Description>
<!--  -->
<!-- http://cybox.mitre.org/objects/File#optionalHeader.minorImageVersion -->

<rdf:Description rdf:about="http://cybox.mitre.org/objects/File#optionalHeader.minorImageVersion">
	<rdf:type rdf:resource="http://www.w3.org/2002/07/owl#DatatypeProperty"/>
	<rdfs:range rdf:resource="http://www.w3.org/2001/XMLSchema#hexBinary"/>
	<rdfs:comment>Specifies the minor version number of the image.</rdfs:comment>
	<rdfs:isDefinedBy rdf:resource="http://cybox.mitre.org/objects/File"/>
	<rdfs:label>Optional Header Minor Image Version</rdfs:label>
</rdf:Description>
<!--  -->
<!-- http://cybox.mitre.org/objects/File#optionalHeader.minorLinkerVersion -->

<rdf:Description rdf:about="http://cybox.mitre.org/objects/File#optionalHeader.minorLinkerVersion">
	<rdf:type rdf:resource="http://www.w3.org/2002/07/owl#DatatypeProperty"/>
	<rdfs:range rdf:resource="http://www.w3.org/2001/XMLSchema#hexBinary"/>
	<rdfs:comment>Specifies the linker minor version number.</rdfs:comment>
	<rdfs:isDefinedBy rdf:datatype="http://www.w3.org/2001/XMLSchema#string">&lt;http://cybox.mitre.org/objects/File&gt;</rdfs:isDefinedBy>
	<rdfs:label>Optional Header Minor Linker Version</rdfs:label>
</rdf:Description>
<!--  -->
<!-- http://cybox.mitre.org/objects/File#optionalHeader.minorOSVersion -->

<rdf:Description rdf:about="http://cybox.mitre.org/objects/File#optionalHeader.minorOSVersion">
	<rdf:type rdf:resource="http://www.w3.org/2002/07/owl#DatatypeProperty"/>
	<rdfs:range rdf:resource="http://www.w3.org/2001/XMLSchema#hexBinary"/>
	<rdfs:comment>Specifies the minor version number of the required operating system.</rdfs:comment>
	<rdfs:isDefinedBy rdf:resource="http://cybox.mitre.org/objects/File"/>
	<rdfs:label>Optional Header Minor OS Version</rdfs:label>
</rdf:Description>
<!--  -->
<!-- http://cybox.mitre.org/objects/File#optionalHeader.minorSubsystemVersion -->

<rdf:Description rdf:about="http://cybox.mitre.org/objects/File#optionalHeader.minorSubsystemVersion">
	<rdf:type rdf:resource="http://www.w3.org/2002/07/owl#DatatypeProperty"/>
	<rdfs:range rdf:resource="http://www.w3.org/2001/XMLSchema#hexBinary"/>
	<rdfs:comment>Specifies the minor version number of the subsystem.</rdfs:comment>
	<rdfs:isDefinedBy rdf:resource="http://cybox.mitre.org/objects/File"/>
	<rdfs:label>Optional Header Minor Subsystem Version</rdfs:label>
</rdf:Description>
<!--  -->
<!-- http://cybox.mitre.org/objects/File#optionalHeader.numberOfRvaAndSizes -->

<rdf:Description rdf:about="http://cybox.mitre.org/objects/File#optionalHeader.numberOfRvaAndSizes">
	<rdf:type rdf:resource="http://www.w3.org/2002/07/owl#DatatypeProperty"/>
	<rdfs:range rdf:resource="http://www.w3.org/2001/XMLSchema#hexBinary"/>
	<rdfs:comment>Specifies the number of data-directory entries in the remainder of the optional header.</rdfs:comment>
	<rdfs:isDefinedBy rdf:resource="http://cybox.mitre.org/objects/File"/>
	<rdfs:label>Optional Header Number of Rva and Sizes</rdfs:label>
</rdf:Description>
<!--  -->
<!-- http://cybox.mitre.org/objects/File#optionalHeader.sectionAlignment -->

<rdf:Description rdf:about="http://cybox.mitre.org/objects/File#optionalHeader.sectionAlignment">
	<rdf:type rdf:resource="http://www.w3.org/2002/07/owl#DatatypeProperty"/>
	<rdfs:range rdf:resource="http://www.w3.org/2001/XMLSchema#hexBinary"/>
	<rdfs:comment>Specifies the alignment (in bytes) of sections when they are loaded into memory.</rdfs:comment>
	<rdfs:isDefinedBy rdf:resource="http://cybox.mitre.org/objects/File"/>
	<rdfs:label>Optional Header Section Alignment</rdfs:label>
</rdf:Description>
<!--  -->
<!-- http://cybox.mitre.org/objects/File#optionalHeader.sizeOfCode -->

<rdf:Description rdf:about="http://cybox.mitre.org/objects/File#optionalHeader.sizeOfCode">
	<rdf:type rdf:resource="http://www.w3.org/2002/07/owl#DatatypeProperty"/>
	<rdfs:range rdf:resource="http://www.w3.org/2001/XMLSchema#hexBinary"/>
	<rdfs:comment>Specifies the size of the code (text) section. If there are multiple sections, size is the sum of the sizes if each.</rdfs:comment>
	<rdfs:isDefinedBy rdf:resource="http://cybox.mitre.org/objects/File"/>
	<rdfs:label>Optional Header Size of Code</rdfs:label>
</rdf:Description>
<!--  -->
<!-- http://cybox.mitre.org/objects/File#optionalHeader.sizeOfHeaders -->

<rdf:Description rdf:about="http://cybox.mitre.org/objects/File#optionalHeader.sizeOfHeaders">
	<rdf:type rdf:resource="http://www.w3.org/2002/07/owl#DatatypeProperty"/>
	<rdfs:range rdf:resource="http://www.w3.org/2001/XMLSchema#hexBinary"/>
	<rdfs:comment>Specifies the combined size of the MS DOS header, PE header, and section headers rounded up to a multiple of FileAlignment.</rdfs:comment>
	<rdfs:isDefinedBy rdf:resource="http://cybox.mitre.org/objects/File"/>
	<rdfs:label>Optional Header Size of Headers</rdfs:label>
</rdf:Description>
<!--  -->
<!-- http://cybox.mitre.org/objects/File#optionalHeader.sizeOfHeapCommit -->

<rdf:Description rdf:about="http://cybox.mitre.org/objects/File#optionalHeader.sizeOfHeapCommit">
	<rdf:type rdf:resource="http://www.w3.org/2002/07/owl#DatatypeProperty"/>
	<rdfs:range rdf:resource="http://www.w3.org/2001/XMLSchema#hexBinary"/>
	<rdfs:comment>Specifies the size of the local heap space to commit.</rdfs:comment>
	<rdfs:isDefinedBy rdf:resource="http://cybox.mitre.org/objects/File"/>
	<rdfs:label>Optional Header Size of Heap Commit</rdfs:label>
</rdf:Description>
<!--  -->
<!-- http://cybox.mitre.org/objects/File#optionalHeader.sizeOfHeapReserve -->

<rdf:Description rdf:about="http://cybox.mitre.org/objects/File#optionalHeader.sizeOfHeapReserve">
	<rdf:type rdf:resource="http://www.w3.org/2002/07/owl#DatatypeProperty"/>
	<rdfs:range rdf:resource="http://www.w3.org/2001/XMLSchema#hexBinary"/>
	<rdfs:comment>Specifies the size of the local heap space to reserve.</rdfs:comment>
	<rdfs:isDefinedBy rdf:resource="http://cybox.mitre.org/objects/File"/>
	<rdfs:label>Optional Header Size of Heap Reserve</rdfs:label>
</rdf:Description>
<!--  -->
<!-- http://cybox.mitre.org/objects/File#optionalHeader.sizeOfImage -->

<rdf:Description rdf:about="http://cybox.mitre.org/objects/File#optionalHeader.sizeOfImage">
	<rdf:type rdf:resource="http://www.w3.org/2002/07/owl#DatatypeProperty"/>
	<rdfs:range rdf:resource="http://www.w3.org/2001/XMLSchema#hexBinary"/>
	<rdfs:comment>Specifies the size (in bytes) of the image, including all headers, as the image is loaded in memory.</rdfs:comment>
	<rdfs:isDefinedBy rdf:resource="http://cybox.mitre.org/objects/File"/>
	<rdfs:label>Optional Header Size of Image</rdfs:label>
</rdf:Description>
<!--  -->
<!-- http://cybox.mitre.org/objects/File#optionalHeader.sizeOfInitializedData -->

<rdf:Description rdf:about="http://cybox.mitre.org/objects/File#optionalHeader.sizeOfInitializedData">
	<rdf:type rdf:resource="http://www.w3.org/2002/07/owl#DatatypeProperty"/>
	<rdfs:range rdf:resource="http://www.w3.org/2001/XMLSchema#hexBinary"/>
	<rdfs:comment>Specifies the size of the initialized data section. If there are multiple sections, size is the sum of the sizes if each.</rdfs:comment>
	<rdfs:isDefinedBy rdf:resource="http://cybox.mitre.org/objects/File"/>
	<rdfs:label>Optional Header Size of Initialized Data</rdfs:label>
</rdf:Description>
<!--  -->
<!-- http://cybox.mitre.org/objects/File#optionalHeader.sizeOfStackCommit -->

<rdf:Description rdf:about="http://cybox.mitre.org/objects/File#optionalHeader.sizeOfStackCommit">
	<rdf:type rdf:resource="http://www.w3.org/2002/07/owl#DatatypeProperty"/>
	<rdfs:range rdf:resource="http://www.w3.org/2001/XMLSchema#hexBinary"/>
	<rdfs:comment>Specifies the size of the stack to commit.</rdfs:comment>
	<rdfs:isDefinedBy rdf:resource="http://cybox.mitre.org/objects/File"/>
	<rdfs:label>Optional Header Size of Stack Commit</rdfs:label>
</rdf:Description>
<!--  -->
<!-- http://cybox.mitre.org/objects/File#optionalHeader.sizeOfStackReserve -->

<rdf:Description rdf:about="http://cybox.mitre.org/objects/File#optionalHeader.sizeOfStackReserve">
	<rdf:type rdf:resource="http://www.w3.org/2002/07/owl#DatatypeProperty"/>
	<rdfs:range rdf:resource="http://www.w3.org/2001/XMLSchema#hexBinary"/>
	<rdfs:comment>Specifies the size of the stack to reserve.</rdfs:comment>
	<rdfs:isDefinedBy rdf:resource="http://cybox.mitre.org/objects/File"/>
	<rdfs:label>Optional Header Size of Stack Reserve</rdfs:label>
</rdf:Description>
<!--  -->
<!-- http://cybox.mitre.org/objects/File#optionalHeader.sizeOfUninitializedData -->

<rdf:Description rdf:about="http://cybox.mitre.org/objects/File#optionalHeader.sizeOfUninitializedData">
	<rdf:type rdf:resource="http://www.w3.org/2002/07/owl#DatatypeProperty"/>
	<rdfs:range rdf:resource="http://www.w3.org/2001/XMLSchema#hexBinary"/>
	<rdfs:comment>Specifies the size of the uninitialized (bss) data section. If there are multiple sections, size is the sum of the sizes if each.</rdfs:comment>
	<rdfs:isDefinedBy rdf:resource="http://cybox.mitre.org/objects/File"/>
	<rdfs:label>Optional Header Size of Uninitialized Data</rdfs:label>
</rdf:Description>
<!--  -->
<!-- http://cybox.mitre.org/objects/File#optionalHeader.subsystem -->

<rdf:Description rdf:about="http://cybox.mitre.org/objects/File#optionalHeader.subsystem">
	<rdf:type rdf:resource="http://www.w3.org/2002/07/owl#DatatypeProperty"/>
	<rdfs:range rdf:resource="http://www.w3.org/2001/XMLSchema#hexBinary"/>
	<rdfs:comment>Specifies the subsystem (e.g., GUI, device driver) that is required to run this image.</rdfs:comment>
	<rdfs:isDefinedBy rdf:resource="http://cybox.mitre.org/objects/File"/>
	<rdfs:label>Optional Header Subsystem</rdfs:label>
</rdf:Description>
<!--  -->
<!-- http://cybox.mitre.org/objects/File#optionalHeader.win32VersionValue -->

<rdf:Description rdf:about="http://cybox.mitre.org/objects/File#optionalHeader.win32VersionValue">
	<rdf:type rdf:resource="http://www.w3.org/2002/07/owl#DatatypeProperty"/>
	<rdfs:range rdf:resource="http://www.w3.org/2001/XMLSchema#hexBinary"/>
	<rdfs:comment>Reserved; must be 0.</rdfs:comment>
	<rdfs:isDefinedBy rdf:resource="http://cybox.mitre.org/objects/File"/>
	<rdfs:label>Optional Header Win32 Version Value</rdfs:label>
</rdf:Description>
<!--  -->
<!-- http://cybox.mitre.org/objects/File#ordinal -->

<rdf:Description rdf:about="http://cybox.mitre.org/objects/File#ordinal">
	<rdf:type rdf:resource="http://www.w3.org/2002/07/owl#DatatypeProperty"/>
	<rdfs:range rdf:resource="http://www.w3.org/2001/XMLSchema#nonNegativeInteger"/>
	<rdfs:comment>Specifies the ordinal value (index) of the function exported by the PE binary.</rdfs:comment>
	<rdfs:isDefinedBy rdf:resource="http://cybox.mitre.org/objects/File"/>
	<rdfs:label>Ordinal</rdfs:label>
</rdf:Description>
<!--  -->
<!-- http://cybox.mitre.org/objects/File#oread -->

<rdf:Description rdf:about="http://cybox.mitre.org/objects/File#oread">
	<rdf:type rdf:resource="http://www.w3.org/2002/07/owl#DatatypeProperty"/>
	<rdfs:range rdf:resource="http://www.w3.org/2001/XMLSchema#boolean"/>
	<rdfs:comment>Specifies whether or not all other users can read the contents of the file.</rdfs:comment>
	<rdfs:isDefinedBy rdf:resource="http://cybox.mitre.org/objects/File"/>
	<rdfs:label>oread</rdfs:label>
</rdf:Description>
<!--  -->
<!-- http://cybox.mitre.org/objects/File#originalFilename -->

<rdf:Description rdf:about="http://cybox.mitre.org/objects/File#originalFilename">
	<rdf:type rdf:resource="http://www.w3.org/2002/07/owl#DatatypeProperty"/>
	<rdfs:range rdf:resource="http://www.w3.org/2001/XMLSchema#string"/>
	<rdfs:comment>Specifies the original name of the file, not including a path. &#xD;
&#xD;
This information enables an application to determine whether a file has been renamed by a user. The format of the name depends on the file system for which the file was created.</rdfs:comment>
	<rdfs:isDefinedBy rdf:resource="http://cybox.mitre.org/objects/File"/>
	<rdfs:label>Original Filename</rdfs:label>
</rdf:Description>
<!--  -->
<!-- http://cybox.mitre.org/objects/File#ownerName -->

<rdf:Description rdf:about="http://cybox.mitre.org/objects/File#ownerName">
	<rdf:type rdf:resource="http://www.w3.org/2002/07/owl#DatatypeProperty"/>
	<rdfs:range rdf:resource="http://www.w3.org/2001/XMLSchema#string"/>
	<rdfs:comment>Specifies the name of the user that owns the file.</rdfs:comment>
	<rdfs:isDefinedBy rdf:datatype="http://www.w3.org/2001/XMLSchema#string">&lt;http://cybox.mitre.org/objects/File&gt;</rdfs:isDefinedBy>
	<rdfs:label>File Owner Name</rdfs:label>
</rdf:Description>
<!--  -->
<!-- http://cybox.mitre.org/objects/File#owrite -->

<rdf:Description rdf:about="http://cybox.mitre.org/objects/File#owrite">
	<rdf:type rdf:resource="http://www.w3.org/2002/07/owl#DatatypeProperty"/>
	<rdfs:range rdf:resource="http://www.w3.org/2001/XMLSchema#boolean"/>
	<rdfs:comment>Specifies whether or not all other users can write to the file.</rdfs:comment>
	<rdfs:isDefinedBy rdf:resource="http://cybox.mitre.org/objects/File"/>
	<rdfs:label>owrite</rdfs:label>
</rdf:Description>
<!--  -->
<!-- http://cybox.mitre.org/objects/File#packerName -->

<rdf:Description rdf:about="http://cybox.mitre.org/objects/File#packerName">
	<rdf:type rdf:resource="http://www.w3.org/2002/07/owl#DatatypeProperty"/>
	<rdfs:range rdf:resource="http://www.w3.org/2001/XMLSchema#string"/>
	<rdfs:comment>Specifies the name of the packer.</rdfs:comment>
	<rdfs:isDefinedBy rdf:datatype="http://www.w3.org/2001/XMLSchema#string">&lt;http://cybox.mitre.org/objects/File&gt;</rdfs:isDefinedBy>
	<rdfs:label>Name</rdfs:label>
</rdf:Description>
<!--  -->
<!-- http://cybox.mitre.org/objects/File#packerType -->

<rdf:Description rdf:about="http://cybox.mitre.org/objects/File#packerType">
	<rdf:type rdf:resource="http://www.w3.org/2002/07/owl#DatatypeProperty"/>
	<rdfs:range rdf:resource="http://www.w3.org/2001/XMLSchema#string"/>
	<rdfs:comment>Specifies the type of packer being characterized.</rdfs:comment>
	<rdfs:isDefinedBy rdf:resource="http://cybox.mitre.org/objects/File"/>
	<rdfs:label>Type</rdfs:label>
</rdf:Description>
<!--  -->
<!-- http://cybox.mitre.org/objects/File#packerVersion -->

<rdf:Description rdf:about="http://cybox.mitre.org/objects/File#packerVersion">
	<rdf:type rdf:resource="http://www.w3.org/2002/07/owl#DatatypeProperty"/>
	<rdfs:range rdf:resource="http://www.w3.org/2001/XMLSchema#string"/>
	<rdfs:comment>Specifies the version of the packer.</rdfs:comment>
	<rdfs:isDefinedBy rdf:datatype="http://www.w3.org/2001/XMLSchema#string">&lt;http://cybox.mitre.org/objects/File&gt;</rdfs:isDefinedBy>
	<rdfs:label>Version</rdfs:label>
</rdf:Description>
<!--  -->
<!-- http://cybox.mitre.org/objects/File#pageCount.nonObfuscated -->

<rdf:Description rdf:about="http://cybox.mitre.org/objects/File#pageCount.nonObfuscated">
	<rdf:type rdf:resource="http://www.w3.org/2002/07/owl#DatatypeProperty"/>
	<rdfs:range rdf:resource="http://www.w3.org/2001/XMLSchema#nonNegativeInteger"/>
	<rdfs:comment>Specifies the number of non-obfuscated occurrences of the '/Page' keyword in the PDF file, which provides an indication of the number of pages in the PDF document.</rdfs:comment>
	<rdfs:isDefinedBy rdf:resource="http://cybox.mitre.org/objects/File"/>
	<rdfs:label>pdf metadata.page count non obfuscated</rdfs:label>
</rdf:Description>
<!--  -->
<!-- http://cybox.mitre.org/objects/File#pageCount.obfuscated -->

<rdf:Description rdf:about="http://cybox.mitre.org/objects/File#pageCount.obfuscated">
	<rdf:type rdf:resource="http://www.w3.org/2002/07/owl#DatatypeProperty"/>
	<rdfs:range rdf:resource="http://www.w3.org/2001/XMLSchema#nonNegativeInteger"/>
	<rdfs:comment>Specifies the number of occurrences of the '/Page' keyword in the PDF file with some form of obfuscation, such as with hexcodes.

The '/Page' keyword provides an indication of the number of pages in the PDF document.</rdfs:comment>
	<rdfs:isDefinedBy rdf:resource="http://cybox.mitre.org/objects/File"/>
	<rdfs:label>'/Page' Obfuscated Count</rdfs:label>
</rdf:Description>
<!--  -->
<!-- http://cybox.mitre.org/objects/File#pdfEncypted -->

<rdf:Description rdf:about="http://cybox.mitre.org/objects/File#pdfEncypted">
	<rdf:type rdf:resource="http://www.w3.org/2002/07/owl#DatatypeProperty"/>
	<rdfs:range rdf:resource="http://www.w3.org/2001/XMLSchema#boolean"/>
	<rdfs:comment>Specifies whether the PDF file is encrypted.</rdfs:comment>
	<rdfs:isDefinedBy rdf:resource="http://cybox.mitre.org/objects/File"/>
	<rdfs:label>PDF Encypted</rdfs:label>
</rdf:Description>
<!--  -->
<!-- http://cybox.mitre.org/objects/File#pdfObjectId.generation -->

<rdf:Description rdf:about="http://cybox.mitre.org/objects/File#pdfObjectId.generation">
	<rdf:type rdf:resource="http://www.w3.org/2002/07/owl#DatatypeProperty"/>
	<rdfs:range rdf:resource="http://www.w3.org/2001/XMLSchema#nonNegativeInteger"/>
	<rdfs:comment>Specifies the generation number portion of the indirect object ID.</rdfs:comment>
	<rdfs:isDefinedBy rdf:resource="http://cybox.mitre.org/objects/File"/>
	<rdfs:label>Object ID Generation</rdfs:label>
</rdf:Description>
<!--  -->
<!-- http://cybox.mitre.org/objects/File#pdfObjectId.number -->

<rdf:Description rdf:about="http://cybox.mitre.org/objects/File#pdfObjectId.number">
	<rdf:type rdf:resource="http://www.w3.org/2002/07/owl#DatatypeProperty"/>
	<rdfs:range rdf:resource="http://www.w3.org/2001/XMLSchema#positiveInteger"/>
	<rdfs:comment>Specifies the number portion of the indirect object ID.</rdfs:comment>
	<rdfs:isDefinedBy rdf:resource="http://cybox.mitre.org/objects/File"/>
	<rdfs:label>Object ID Number</rdfs:label>
</rdf:Description>
<!--  -->
<!-- http://cybox.mitre.org/objects/File#pdfObjectType -->

<rdf:Description rdf:about="http://cybox.mitre.org/objects/File#pdfObjectType">
	<rdf:type rdf:resource="http://www.w3.org/2002/07/owl#DatatypeProperty"/>
	<rdfs:range rdf:nodeID="genid4"/>
</rdf:Description>

<rdf:Description rdf:nodeID="genid4">
	<rdf:type rdf:resource="http://www.w3.org/2000/01/rdf-schema#Datatype"/>
	<owl:oneOf rdf:nodeID="genid12"/>
</rdf:Description>

<rdf:Description rdf:nodeID="genid12">
	<rdf:type rdf:resource="http://www.w3.org/1999/02/22-rdf-syntax-ns#List"/>
	<rdf:first rdf:datatype="http://www.w3.org/2001/XMLSchema#string">Array</rdf:first>
	<rdf:rest rdf:nodeID="genid11"/>
</rdf:Description>

<rdf:Description rdf:nodeID="genid11">
	<rdf:type rdf:resource="http://www.w3.org/1999/02/22-rdf-syntax-ns#List"/>
	<rdf:first rdf:datatype="http://www.w3.org/2001/XMLSchema#string">Boolean</rdf:first>
	<rdf:rest rdf:nodeID="genid10"/>
</rdf:Description>

<rdf:Description rdf:nodeID="genid10">
	<rdf:type rdf:resource="http://www.w3.org/1999/02/22-rdf-syntax-ns#List"/>
	<rdf:first rdf:datatype="http://www.w3.org/2001/XMLSchema#string">Dictionary</rdf:first>
	<rdf:rest rdf:nodeID="genid9"/>
</rdf:Description>

<rdf:Description rdf:nodeID="genid9">
	<rdf:type rdf:resource="http://www.w3.org/1999/02/22-rdf-syntax-ns#List"/>
	<rdf:first rdf:datatype="http://www.w3.org/2001/XMLSchema#string">Integer</rdf:first>
	<rdf:rest rdf:nodeID="genid8"/>
</rdf:Description>

<rdf:Description rdf:nodeID="genid8">
	<rdf:type rdf:resource="http://www.w3.org/1999/02/22-rdf-syntax-ns#List"/>
	<rdf:first rdf:datatype="http://www.w3.org/2001/XMLSchema#string">Name</rdf:first>
	<rdf:rest rdf:nodeID="genid7"/>
</rdf:Description>

<rdf:Description rdf:nodeID="genid7">
	<rdf:type rdf:resource="http://www.w3.org/1999/02/22-rdf-syntax-ns#List"/>
	<rdf:first rdf:datatype="http://www.w3.org/2001/XMLSchema#string">Null</rdf:first>
	<rdf:rest rdf:nodeID="genid6"/>
</rdf:Description>

<rdf:Description rdf:nodeID="genid6">
	<rdf:type rdf:resource="http://www.w3.org/1999/02/22-rdf-syntax-ns#List"/>
	<rdf:first rdf:datatype="http://www.w3.org/2001/XMLSchema#string">Stream</rdf:first>
	<rdf:rest rdf:nodeID="genid5"/>
</rdf:Description>

<rdf:Description rdf:nodeID="genid5">
	<rdf:type rdf:resource="http://www.w3.org/1999/02/22-rdf-syntax-ns#List"/>
	<rdf:first rdf:datatype="http://www.w3.org/2001/XMLSchema#string">String</rdf:first>
	<rdf:rest rdf:resource="http://www.w3.org/1999/02/22-rdf-syntax-ns#nil"/>
</rdf:Description>

<rdf:Description rdf:about="http://cybox.mitre.org/objects/File#pdfObjectType">
	<rdfs:comment>Specifies the basic type of the PDF indirect object.</rdfs:comment>
	<rdfs:isDefinedBy rdf:resource="http://cybox.mitre.org/objects/File"/>
	<rdfs:label>PDF Indirect Object Type</rdfs:label>
</rdf:Description>
<!--  -->
<!-- http://cybox.mitre.org/objects/File#pdfOptimized -->

<rdf:Description rdf:about="http://cybox.mitre.org/objects/File#pdfOptimized">
	<rdf:type rdf:resource="http://www.w3.org/2002/07/owl#DatatypeProperty"/>
	<rdfs:range rdf:resource="http://www.w3.org/2001/XMLSchema#boolean"/>
	<rdfs:comment>Specifies whether the PDF file has been optimized.</rdfs:comment>
	<rdfs:isDefinedBy rdf:resource="http://cybox.mitre.org/objects/File"/>
	<rdfs:label>PDF Optimized</rdfs:label>
</rdf:Description>
<!--  -->
<!-- http://cybox.mitre.org/objects/File#pdfSpecVersion -->

<rdf:Description rdf:about="http://cybox.mitre.org/objects/File#pdfSpecVersion">
	<rdf:type rdf:resource="http://www.w3.org/2002/07/owl#DatatypeProperty"/>
	<rdfs:range rdf:resource="http://www.w3.org/2001/XMLSchema#double"/>
	<rdfs:comment>Specifies the decimal version number portion of the string from the PDF Header that specifies the version of the PDF specification to which the PDF file conforms, e.g. '1.4'.</rdfs:comment>
	<rdfs:isDefinedBy rdf:resource="http://cybox.mitre.org/objects/File"/>
	<rdfs:label>PDF Spec Version</rdfs:label>
</rdf:Description>
<!--  -->
<!-- http://cybox.mitre.org/objects/File#peChecksum.computedAPI -->

<rdf:Description rdf:about="http://cybox.mitre.org/objects/File#peChecksum.computedAPI">
	<rdf:type rdf:resource="http://www.w3.org/2002/07/owl#DatatypeProperty"/>
	<rdfs:range rdf:resource="http://www.w3.org/2001/XMLSchema#long"/>
	<rdfs:comment>Specifies a checksum computed by an external algorithm.</rdfs:comment>
	<rdfs:isDefinedBy rdf:resource="http://cybox.mitre.org/objects/File"/>
	<rdfs:label>PE Computed API Checksum</rdfs:label>
</rdf:Description>
<!--  -->
<!-- http://cybox.mitre.org/objects/File#peChecksum.fileAPI -->

<rdf:Description rdf:about="http://cybox.mitre.org/objects/File#peChecksum.fileAPI">
	<rdf:type rdf:resource="http://www.w3.org/2002/07/owl#DatatypeProperty"/>
	<rdfs:range rdf:resource="http://www.w3.org/2001/XMLSchema#long"/>
	<rdfs:comment>Specified the checksum computed by IMAGHELP.DLL.</rdfs:comment>
	<rdfs:isDefinedBy rdf:resource="http://cybox.mitre.org/objects/File"/>
	<rdfs:label>PE File API Checksum</rdfs:label>
</rdf:Description>
<!--  -->
<!-- http://cybox.mitre.org/objects/File#peChecksum.fileRaw -->

<rdf:Description rdf:about="http://cybox.mitre.org/objects/File#peChecksum.fileRaw">
	<rdf:type rdf:resource="http://www.w3.org/2002/07/owl#DatatypeProperty"/>
	<rdfs:range rdf:resource="http://www.w3.org/2001/XMLSchema#long"/>
	<rdfs:comment>Specifies the checksum found in the PE file (in the Optional Header).</rdfs:comment>
	<rdfs:isDefinedBy rdf:resource="http://cybox.mitre.org/objects/File"/>
	<rdfs:label>PE File Raw Checksum</rdfs:label>
</rdf:Description>
<!--  -->
<!-- http://cybox.mitre.org/objects/File#peHeadersHash.value -->

<rdf:Description rdf:about="http://cybox.mitre.org/objects/File#peHeadersHash.value">
	<rdf:type rdf:resource="http://www.w3.org/2002/07/owl#DatatypeProperty"/>
	<rdfs:range rdf:resource="http://www.w3.org/2001/XMLSchema#string"/>
	<rdfs:comment>Specifies the values, in the format of 'hash-type:hash-value', for any hash computed using the specified PE bindary file header an input.</rdfs:comment>
	<rdfs:isDefinedBy rdf:resource="http://cybox.mitre.org/objects/File"/>
	<rdfs:label>PEHeaders Hash Value</rdfs:label>
</rdf:Description>
<!--  -->
<!-- http://cybox.mitre.org/objects/File#peModuleName -->

<rdf:Description rdf:about="http://cybox.mitre.org/objects/File#peModuleName">
	<rdf:type rdf:resource="http://www.w3.org/2002/07/owl#DatatypeProperty"/>
	<rdfs:range rdf:resource="http://www.w3.org/2001/XMLSchema#string"/>
	<rdfs:comment>Specifies the actual name of the PE module, as used by the PE loader when it is imported by another executable.</rdfs:comment>
	<rdfs:isDefinedBy rdf:resource="http://cybox.mitre.org/objects/File"/>
	<rdfs:label>PE Module Name</rdfs:label>
</rdf:Description>
<!--  -->
<!-- http://cybox.mitre.org/objects/File#peSignature -->

<rdf:Description rdf:about="http://cybox.mitre.org/objects/File#peSignature">
	<rdf:type rdf:resource="http://www.w3.org/2002/07/owl#DatatypeProperty"/>
	<rdfs:range rdf:resource="http://www.w3.org/2001/XMLSchema#hexBinary"/>
	<rdfs:comment>Specifes the Signature field specifies the 4-bytes sugnature that identifies the file as a PE file.</rdfs:comment>
	<rdfs:isDefinedBy rdf:resource="http://cybox.mitre.org/objects/File"/>
	<rdfs:label>PE Header Signature</rdfs:label>
</rdf:Description>
<!--  -->
<!-- http://cybox.mitre.org/objects/File#peType -->

<rdf:Description rdf:about="http://cybox.mitre.org/objects/File#peType">
	<rdf:type rdf:resource="http://www.w3.org/2002/07/owl#DatatypeProperty"/>
	<rdfs:range rdf:resource="http://www.w3.org/2001/XMLSchema#string"/>
	<rdfs:comment>Specifies the particular type of the PE binary, e.g. Executable.</rdfs:comment>
	<rdfs:isDefinedBy rdf:resource="http://cybox.mitre.org/objects/File"/>
	<rdfs:label>PE Type</rdfs:label>
</rdf:Description>
<!--  -->
<!-- http://cybox.mitre.org/objects/File#peakEntropy -->

<rdf:Description rdf:about="http://cybox.mitre.org/objects/File#peakEntropy">
	<rdf:type rdf:resource="http://www.w3.org/2002/07/owl#DatatypeProperty"/>
	<rdfs:range rdf:resource="http://www.w3.org/2001/XMLSchema#double"/>
	<rdfs:comment>Specifies the calculated peak entropy of the file.</rdfs:comment>
	<rdfs:isDefinedBy rdf:datatype="http://www.w3.org/2001/XMLSchema#string">&lt;http://cybox.mitre.org/objects/File&gt;</rdfs:isDefinedBy>
	<rdfs:label>Peak Entropy</rdfs:label>
</rdf:Description>
<!--  -->
<!-- http://cybox.mitre.org/objects/File#prev -->

<rdf:Description rdf:about="http://cybox.mitre.org/objects/File#prev">
	<rdf:type rdf:resource="http://www.w3.org/2002/07/owl#DatatypeProperty"/>
	<rdfs:range rdf:resource="http://www.w3.org/2001/XMLSchema#positiveInteger"/>
	<rdfs:comment>Specifies  the byte offset from the beginning of the file to the beginning of the previous cross-reference table. This is only applicable for files that have more than one cross-reference table.</rdfs:comment>
	<rdfs:isDefinedBy rdf:resource="http://cybox.mitre.org/objects/File"/>
	<rdfs:label>Prev</rdfs:label>
</rdf:Description>
<!--  -->
<!-- http://cybox.mitre.org/objects/File#privateBuild -->

<rdf:Description rdf:about="http://cybox.mitre.org/objects/File#privateBuild">
	<rdf:type rdf:resource="http://www.w3.org/2002/07/owl#DatatypeProperty"/>
	<rdfs:range rdf:resource="http://www.w3.org/2001/XMLSchema#string"/>
	<rdfs:comment>Specifies the information about a private version of the file - for example, "Built by TESTER1 on \TESTBED". &#xD;
&#xD;
This string should be present only if VS_FF_PRIVATEBUILD is specified in the fileflags parameter of the root block.</rdfs:comment>
	<rdfs:isDefinedBy rdf:resource="http://cybox.mitre.org/objects/File"/>
	<rdfs:label>Private Build</rdfs:label>
</rdf:Description>
<!--  -->
<!-- http://cybox.mitre.org/objects/File#productName -->

<rdf:Description rdf:about="http://cybox.mitre.org/objects/File#productName">
	<rdf:type rdf:resource="http://www.w3.org/2002/07/owl#DatatypeProperty"/>
	<rdfs:range rdf:resource="http://www.w3.org/2001/XMLSchema#string"/>
	<rdfs:comment>Specifies the name of the product with which the file is distributed. This string is required.</rdfs:comment>
	<rdfs:isDefinedBy rdf:resource="http://cybox.mitre.org/objects/File"/>
	<rdfs:label>Product Name</rdfs:label>
</rdf:Description>
<!--  -->
<!-- http://cybox.mitre.org/objects/File#productVersion -->

<rdf:Description rdf:about="http://cybox.mitre.org/objects/File#productVersion">
	<rdf:type rdf:resource="http://www.w3.org/2002/07/owl#DatatypeProperty"/>
	<rdfs:range rdf:resource="http://www.w3.org/2001/XMLSchema#string"/>
	<rdfs:comment>Specifies the version of the product with which the file is distributed - for example, "3.10" or "5.00.RC2".</rdfs:comment>
	<rdfs:isDefinedBy rdf:resource="http://cybox.mitre.org/objects/File"/>
	<rdfs:label>Product Version</rdfs:label>
</rdf:Description>
<!--  -->
<!-- http://cybox.mitre.org/objects/File#rawStream -->

<rdf:Description rdf:about="http://cybox.mitre.org/objects/File#rawStream">
	<rdf:type rdf:resource="http://www.w3.org/2002/07/owl#DatatypeProperty"/>
	<rdfs:range rdf:resource="http://www.w3.org/2001/XMLSchema#string"/>
	<rdfs:comment>Specifie the raw, undecoded stream (i.e., everything between the 'stream' and 'endstream' keywords), as a hex string.</rdfs:comment>
	<rdfs:isDefinedBy rdf:resource="http://cybox.mitre.org/objects/File"/>
	<rdfs:label>Raw Stream</rdfs:label>
</rdf:Description>
<!--  -->
<!-- http://cybox.mitre.org/objects/File#read -->

<rdf:Description rdf:about="http://cybox.mitre.org/objects/File#read">
	<rdf:type rdf:resource="http://www.w3.org/2002/07/owl#DatatypeProperty"/>
	<rdfs:range rdf:resource="http://www.w3.org/2001/XMLSchema#boolean"/>
	<rdfs:comment>Specifies whether viewing or accessing of the file's contents is permitted.</rdfs:comment>
	<rdfs:isDefinedBy rdf:resource="http://cybox.mitre.org/objects/File"/>
	<rdfs:label>Read</rdfs:label>
</rdf:Description>
<!--  -->
<!-- http://cybox.mitre.org/objects/File#readAndExecute -->

<rdf:Description rdf:about="http://cybox.mitre.org/objects/File#readAndExecute">
	<rdf:type rdf:resource="http://www.w3.org/2002/07/owl#DatatypeProperty"/>
	<rdfs:range rdf:resource="http://www.w3.org/2001/XMLSchema#boolean"/>
	<rdfs:comment>Specifies whether viewing and accessing of the file's contents as well as executing of the file is permitted.</rdfs:comment>
	<rdfs:isDefinedBy rdf:resource="http://cybox.mitre.org/objects/File"/>
	<rdfs:label>Read and Execute</rdfs:label>
</rdf:Description>
<!--  -->
<!-- http://cybox.mitre.org/objects/File#readOnly -->

<rdf:Description rdf:about="http://cybox.mitre.org/objects/File#readOnly">
	<rdf:type rdf:resource="http://www.w3.org/2002/07/owl#DatatypeProperty"/>
	<rdfs:range rdf:resource="http://www.w3.org/2001/XMLSchema#boolean"/>
	<rdfs:comment>Specifies a file is read only, as denoted by the constant value, 0x1. Applications can read the file, but cannot write to it or delete it. This attribute is not honored on directories. For more information as to why, see http://go.microsoft.com/FWLink/?LinkId=125896.</rdfs:comment>
	<rdfs:isDefinedBy rdf:resource="http://cybox.mitre.org/objects/File"/>
	<rdfs:label>Read-Only</rdfs:label>
</rdf:Description>
<!--  -->
<!-- http://cybox.mitre.org/objects/File#reparsePoint -->

<rdf:Description rdf:about="http://cybox.mitre.org/objects/File#reparsePoint">
	<rdf:type rdf:resource="http://www.w3.org/2002/07/owl#DatatypeProperty"/>
	<rdfs:range rdf:resource="http://www.w3.org/2001/XMLSchema#boolean"/>
	<rdfs:comment>Specifies a file or directory that has an associated reparse point, or a file that is a symbolic link, as denoted by the constant value, 0x400.</rdfs:comment>
	<rdfs:isDefinedBy rdf:resource="http://cybox.mitre.org/objects/File"/>
	<rdfs:label>Reparse Point</rdfs:label>
</rdf:Description>
<!--  -->
<!-- http://cybox.mitre.org/objects/File#reserved.size -->

<rdf:Description rdf:about="http://cybox.mitre.org/objects/File#reserved.size">
	<rdf:type rdf:resource="http://www.w3.org/2002/07/owl#DatatypeProperty"/>
	<rdfs:range rdf:resource="http://www.w3.org/2001/XMLSchema#nonNegativeInteger"/>
	<rdfs:comment>Reserved; must be 0</rdfs:comment>
	<rdfs:isDefinedBy rdf:resource="http://cybox.mitre.org/objects/File"/>
	<rdfs:label>Reserved Size</rdfs:label>
</rdf:Description>
<!--  -->
<!-- http://cybox.mitre.org/objects/File#reserved.virtualAddress -->

<rdf:Description rdf:about="http://cybox.mitre.org/objects/File#reserved.virtualAddress">
	<rdf:type rdf:resource="http://www.w3.org/2002/07/owl#DatatypeProperty"/>
	<rdfs:range rdf:resource="http://www.w3.org/2001/XMLSchema#hexBinary"/>
	<rdfs:comment>Reserved; must be 0</rdfs:comment>
	<rdfs:isDefinedBy rdf:resource="http://cybox.mitre.org/objects/File"/>
	<rdfs:label>Reserved Virtual Address</rdfs:label>
</rdf:Description>
<!--  -->
<!-- http://cybox.mitre.org/objects/File#resourceData -->

<rdf:Description rdf:about="http://cybox.mitre.org/objects/File#resourceData">
	<rdf:type rdf:resource="http://www.w3.org/2002/07/owl#DatatypeProperty"/>
	<rdfs:range rdf:resource="http://www.w3.org/2001/XMLSchema#string"/>
	<rdfs:comment>Specifies  the actual data contained in the resource, most commonly as a base64-encoded string encapsulated in a CDATA () section.</rdfs:comment>
	<rdfs:isDefinedBy rdf:resource="http://cybox.mitre.org/objects/File"/>
	<rdfs:label>Resource Data</rdfs:label>
</rdf:Description>
<!--  -->
<!-- http://cybox.mitre.org/objects/File#resourceHash.value -->

<rdf:Description rdf:about="http://cybox.mitre.org/objects/File#resourceHash.value">
	<rdf:type rdf:resource="http://www.w3.org/2002/07/owl#DatatypeProperty"/>
	<rdfs:range rdf:resource="http://www.w3.org/2001/XMLSchema#string"/>
	<rdfs:comment>Specifies the values, in the format of 'hash-type':'hash-value', for any hash computed using the specified PE binary resource as input.</rdfs:comment>
	<rdfs:isDefinedBy rdf:resource="http://cybox.mitre.org/objects/File"/>
	<rdfs:label>Resource Hash Value</rdfs:label>
</rdf:Description>
<!--  -->
<!-- http://cybox.mitre.org/objects/File#resourceName -->

<rdf:Description rdf:about="http://cybox.mitre.org/objects/File#resourceName">
	<rdf:type rdf:resource="http://www.w3.org/2002/07/owl#DatatypeProperty"/>
	<rdfs:range rdf:resource="http://www.w3.org/2001/XMLSchema#string"/>
	<rdfs:comment>Specifies the name of the resource used by the PE binary.</rdfs:comment>
	<rdfs:isDefinedBy rdf:resource="http://cybox.mitre.org/objects/File"/>
	<rdfs:label>Resource Name</rdfs:label>
</rdf:Description>
<!--  -->
<!-- http://cybox.mitre.org/objects/File#resourceSize -->

<rdf:Description rdf:about="http://cybox.mitre.org/objects/File#resourceSize">
	<rdf:type rdf:resource="http://www.w3.org/2002/07/owl#DatatypeProperty"/>
	<rdfs:range rdf:resource="http://www.w3.org/2001/XMLSchema#positiveInteger"/>
	<rdfs:comment>Specifies the size of the resource, in bytes.</rdfs:comment>
	<rdfs:isDefinedBy rdf:resource="http://cybox.mitre.org/objects/File"/>
	<rdfs:label>Resource Size</rdfs:label>
</rdf:Description>
<!--  -->
<!-- http://cybox.mitre.org/objects/File#resourceTable.size -->

<rdf:Description rdf:about="http://cybox.mitre.org/objects/File#resourceTable.size">
	<rdf:type rdf:resource="http://www.w3.org/2002/07/owl#DatatypeProperty"/>
	<rdfs:range rdf:resource="http://www.w3.org/2001/XMLSchema#nonNegativeInteger"/>
	<rdfs:comment>Specifies the size of the data structure, in bytes, of the resource table data directory.</rdfs:comment>
	<rdfs:isDefinedBy rdf:resource="http://cybox.mitre.org/objects/File"/>
	<rdfs:label>Resource Table Size</rdfs:label>
</rdf:Description>
<!--  -->
<!-- http://cybox.mitre.org/objects/File#resourceTable.virtualAddress -->

<rdf:Description rdf:about="http://cybox.mitre.org/objects/File#resourceTable.virtualAddress">
	<rdf:type rdf:resource="http://www.w3.org/2002/07/owl#DatatypeProperty"/>
	<rdfs:range rdf:resource="http://www.w3.org/2001/XMLSchema#hexBinary"/>
	<rdfs:comment>Specifies the relative virtual address (RVA) of the data structure of the resource table data directory.</rdfs:comment>
	<rdfs:isDefinedBy rdf:resource="http://cybox.mitre.org/objects/File"/>
	<rdfs:label>Resource Table Virtual Address</rdfs:label>
</rdf:Description>
<!--  -->
<!-- http://cybox.mitre.org/objects/File#resourceType -->

<rdf:Description rdf:about="http://cybox.mitre.org/objects/File#resourceType">
	<rdf:type rdf:resource="http://www.w3.org/2002/07/owl#DatatypeProperty"/>
	<rdfs:range rdf:resource="http://www.w3.org/2001/XMLSchema#string"/>
	<rdfs:comment>Specifies the type of data referred to by this resource.</rdfs:comment>
	<rdfs:isDefinedBy rdf:resource="http://cybox.mitre.org/objects/File"/>
	<rdfs:label>Resource Type</rdfs:label>
</rdf:Description>
<!--  -->
<!-- http://cybox.mitre.org/objects/File#richMediaCount.nonObfuscated -->

<rdf:Description rdf:about="http://cybox.mitre.org/objects/File#richMediaCount.nonObfuscated">
	<rdf:type rdf:resource="http://www.w3.org/2002/07/owl#DatatypeProperty"/>
	<rdfs:range rdf:resource="http://www.w3.org/2001/XMLSchema#nonNegativeInteger"/>
	<rdfs:comment>Specifies the number of non-obfuscated occurrences of the '/RichMedia' keyword in the PDF file.</rdfs:comment>
	<rdfs:isDefinedBy rdf:resource="http://cybox.mitre.org/objects/File"/>
	<rdfs:label>'/RichMedia' Non-obfuscated Count</rdfs:label>
</rdf:Description>
<!--  -->
<!-- http://cybox.mitre.org/objects/File#richMediaCount.obfuscated -->

<rdf:Description rdf:about="http://cybox.mitre.org/objects/File#richMediaCount.obfuscated">
	<rdf:type rdf:resource="http://www.w3.org/2002/07/owl#DatatypeProperty"/>
	<rdfs:range rdf:resource="http://www.w3.org/2001/XMLSchema#nonNegativeInteger"/>
	<rdfs:comment>Specifes the number of obfuscated occurrences of the '/RichMedia' keyword in the PDF file.</rdfs:comment>
	<rdfs:isDefinedBy rdf:resource="http://cybox.mitre.org/objects/File"/>
	<rdfs:label>'/RichMedia' Obfuscated Count</rdfs:label>
</rdf:Description>
<!--  -->
<!-- http://cybox.mitre.org/objects/File#root.generationNumber -->

<rdf:Description rdf:about="http://cybox.mitre.org/objects/File#root.generationNumber">
	<rdf:type rdf:resource="http://www.w3.org/2002/07/owl#DatatypeProperty"/>
	<rdfs:comment></rdfs:comment>
	<rdfs:isDefinedBy rdf:datatype="http://www.w3.org/2001/XMLSchema#string">&lt;http://cybox.mitre.org/objects/File&gt;</rdfs:isDefinedBy>
	<rdfs:label>root.generation number</rdfs:label>
</rdf:Description>
<!--  -->
<!-- http://cybox.mitre.org/objects/File#root.objectNumber -->

<rdf:Description rdf:about="http://cybox.mitre.org/objects/File#root.objectNumber">
	<rdf:type rdf:resource="http://www.w3.org/2002/07/owl#DatatypeProperty"/>
	<rdfs:comment></rdfs:comment>
	<rdfs:isDefinedBy rdf:datatype="http://www.w3.org/2001/XMLSchema#string">&lt;http://cybox.mitre.org/objects/File&gt;</rdfs:isDefinedBy>
	<rdfs:label>root.object number</rdfs:label>
</rdf:Description>
<!--  -->
<!-- http://cybox.mitre.org/objects/File#runLengthDecodeCount.nonObfuscated -->

<rdf:Description rdf:about="http://cybox.mitre.org/objects/File#runLengthDecodeCount.nonObfuscated">
	<rdf:type rdf:resource="http://www.w3.org/2002/07/owl#DatatypeProperty"/>
	<rdfs:range rdf:resource="http://www.w3.org/2001/XMLSchema#nonNegativeInteger"/>
	<rdfs:comment>Specifies the number of non-obfuscated occurrences of the '/RunLengthDecode' keyword in the PDF file.</rdfs:comment>
	<rdfs:isDefinedBy rdf:resource="http://cybox.mitre.org/objects/File"/>
	<rdfs:label>'/RunLengthDecode' Non-obfuscated Count</rdfs:label>
</rdf:Description>
<!--  -->
<!-- http://cybox.mitre.org/objects/File#runLengthDecodeCount.obfuscated -->

<rdf:Description rdf:about="http://cybox.mitre.org/objects/File#runLengthDecodeCount.obfuscated">
	<rdf:type rdf:resource="http://www.w3.org/2002/07/owl#DatatypeProperty"/>
	<rdfs:range rdf:resource="http://www.w3.org/2001/XMLSchema#nonNegativeInteger"/>
	<rdfs:comment>Specifies the number of obfuscated occurrences of the '/RunLengthDecode' keyword in the PDF file with some form of obfuscation, such as with hexcodes.</rdfs:comment>
	<rdfs:isDefinedBy rdf:resource="http://cybox.mitre.org/objects/File"/>
	<rdfs:label>run length decode.obfuscated</rdfs:label>
</rdf:Description>
<!--  -->
<!-- http://cybox.mitre.org/objects/File#sectionHeader.characteristics -->

<rdf:Description rdf:about="http://cybox.mitre.org/objects/File#sectionHeader.characteristics">
	<rdf:type rdf:resource="http://www.w3.org/2002/07/owl#DatatypeProperty"/>
	<rdfs:range rdf:resource="http://www.w3.org/2001/XMLSchema#hexBinary"/>
	<rdfs:comment>Specifies any flags defined for the specified PE binary section.</rdfs:comment>
	<rdfs:isDefinedBy rdf:resource="http://cybox.mitre.org/objects/File"/>
	<rdfs:label>Section Characteristics</rdfs:label>
</rdf:Description>
<!--  -->
<!-- http://cybox.mitre.org/objects/File#sectionHeader.name -->

<rdf:Description rdf:about="http://cybox.mitre.org/objects/File#sectionHeader.name">
	<rdf:type rdf:resource="http://www.w3.org/2002/07/owl#DatatypeProperty"/>
	<rdfs:range rdf:resource="http://www.w3.org/2001/XMLSchema#string"/>
	<rdfs:comment>Specifies the name of the PE binary section.</rdfs:comment>
	<rdfs:isDefinedBy rdf:resource="http://cybox.mitre.org/objects/File"/>
	<rdfs:label>Section Name</rdfs:label>
</rdf:Description>
<!--  -->
<!-- http://cybox.mitre.org/objects/File#sectionHeader.numberOfLinenumbers -->

<rdf:Description rdf:about="http://cybox.mitre.org/objects/File#sectionHeader.numberOfLinenumbers">
	<rdf:type rdf:resource="http://www.w3.org/2002/07/owl#DatatypeProperty"/>
	<rdfs:range rdf:resource="http://www.w3.org/2001/XMLSchema#nonNegativeInteger"/>
	<rdfs:comment>Specifies the number of line number entries for the section. Should be 0.</rdfs:comment>
	<rdfs:isDefinedBy rdf:resource="http://cybox.mitre.org/objects/File"/>
	<rdfs:label>Section Number of Linenumbers</rdfs:label>
</rdf:Description>
<!--  -->
<!-- http://cybox.mitre.org/objects/File#sectionHeader.numberOfRelocations -->

<rdf:Description rdf:about="http://cybox.mitre.org/objects/File#sectionHeader.numberOfRelocations">
	<rdf:type rdf:resource="http://www.w3.org/2002/07/owl#DatatypeProperty"/>
	<rdfs:range rdf:resource="http://www.w3.org/2001/XMLSchema#nonNegativeInteger"/>
	<rdfs:comment>Specifies the number of relocations defined for the specified PE binary section.</rdfs:comment>
	<rdfs:isDefinedBy rdf:resource="http://cybox.mitre.org/objects/File"/>
	<rdfs:label>Section Number of Relocations</rdfs:label>
</rdf:Description>
<!--  -->
<!-- http://cybox.mitre.org/objects/File#sectionHeader.pointerToLinenumbers -->

<rdf:Description rdf:about="http://cybox.mitre.org/objects/File#sectionHeader.pointerToLinenumbers">
	<rdf:type rdf:resource="http://www.w3.org/2002/07/owl#DatatypeProperty"/>
	<rdfs:range rdf:resource="http://www.w3.org/2001/XMLSchema#hexBinary"/>
	<rdfs:comment>Specifies the beginning of line-number entries for the section. Should be 0.</rdfs:comment>
	<rdfs:isDefinedBy rdf:resource="http://cybox.mitre.org/objects/File"/>
	<rdfs:label>Section Pointer to Linenumbers</rdfs:label>
</rdf:Description>
<!--  -->
<!-- http://cybox.mitre.org/objects/File#sectionHeader.pointerToRawData -->

<rdf:Description rdf:about="http://cybox.mitre.org/objects/File#sectionHeader.pointerToRawData">
	<rdf:type rdf:resource="http://www.w3.org/2002/07/owl#DatatypeProperty"/>
	<rdfs:range rdf:resource="http://www.w3.org/2001/XMLSchema#hexBinary"/>
	<rdfs:comment>Specifies the file offset of the beginning of the PE binary section.</rdfs:comment>
	<rdfs:isDefinedBy rdf:resource="http://cybox.mitre.org/objects/File"/>
	<rdfs:label>Section Pointer to Raw Data</rdfs:label>
</rdf:Description>
<!--  -->
<!-- http://cybox.mitre.org/objects/File#sectionHeader.pointerToRelocations -->

<rdf:Description rdf:about="http://cybox.mitre.org/objects/File#sectionHeader.pointerToRelocations">
	<rdf:type rdf:resource="http://www.w3.org/2002/07/owl#DatatypeProperty"/>
	<rdfs:range rdf:resource="http://www.w3.org/2001/XMLSchema#hexBinary"/>
	<rdfs:comment>Specifies the offset of the PE binary section relocations, if applicable.</rdfs:comment>
	<rdfs:isDefinedBy rdf:resource="http://cybox.mitre.org/objects/File"/>
	<rdfs:label>Section Pointer to Relcoations</rdfs:label>
</rdf:Description>
<!--  -->
<!-- http://cybox.mitre.org/objects/File#sectionHeader.sizeOfRawData -->

<rdf:Description rdf:about="http://cybox.mitre.org/objects/File#sectionHeader.sizeOfRawData">
	<rdf:type rdf:resource="http://www.w3.org/2002/07/owl#DatatypeProperty"/>
	<rdfs:range rdf:resource="http://www.w3.org/2001/XMLSchema#hexBinary"/>
	<rdfs:comment>Specifies the size of the data contained in the PE binary section.</rdfs:comment>
	<rdfs:isDefinedBy rdf:resource="http://cybox.mitre.org/objects/File"/>
	<rdfs:label>Section Size of Raw Data</rdfs:label>
</rdf:Description>
<!--  -->
<!-- http://cybox.mitre.org/objects/File#sectionHeader.virtualAddress -->

<rdf:Description rdf:about="http://cybox.mitre.org/objects/File#sectionHeader.virtualAddress">
	<rdf:type rdf:resource="http://www.w3.org/2002/07/owl#DatatypeProperty"/>
	<rdfs:range rdf:resource="http://www.w3.org/2001/XMLSchema#hexBinary"/>
	<rdfs:comment>Specifies the relative virtual address (RVA) of the PE binary section.</rdfs:comment>
	<rdfs:isDefinedBy rdf:resource="http://cybox.mitre.org/objects/File"/>
	<rdfs:label>Section Virtual Address</rdfs:label>
</rdf:Description>
<!--  -->
<!-- http://cybox.mitre.org/objects/File#sectionHeader.virtualSize -->

<rdf:Description rdf:about="http://cybox.mitre.org/objects/File#sectionHeader.virtualSize">
	<rdf:type rdf:resource="http://www.w3.org/2002/07/owl#DatatypeProperty"/>
	<rdfs:range rdf:resource="http://www.w3.org/2001/XMLSchema#hexBinary"/>
	<rdfs:comment>Specifies the total size of the PE binary section when loaded into memory. It is valid only for executables and should be 0 for object files.</rdfs:comment>
	<rdfs:isDefinedBy rdf:resource="http://cybox.mitre.org/objects/File"/>
	<rdfs:label>Section Virtual Size</rdfs:label>
</rdf:Description>
<!--  -->
<!-- http://cybox.mitre.org/objects/File#sgid -->

<rdf:Description rdf:about="http://cybox.mitre.org/objects/File#sgid">
	<rdf:type rdf:resource="http://www.w3.org/2002/07/owl#DatatypeProperty"/>
	<rdfs:range rdf:resource="http://www.w3.org/2001/XMLSchema#boolean"/>
	<rdfs:comment>Specifies whether or not the file may be executed with the privileges of the file's group owner.</rdfs:comment>
	<rdfs:isDefinedBy rdf:resource="http://cybox.mitre.org/objects/File"/>
	<rdfs:label>sgid</rdfs:label>
</rdf:Description>
<!--  -->
<!-- http://cybox.mitre.org/objects/File#signature -->

<rdf:Description rdf:about="http://cybox.mitre.org/objects/File#signature">
	<rdf:type rdf:resource="http://www.w3.org/2002/07/owl#DatatypeProperty"/>
	<rdfs:range rdf:resource="http://www.w3.org/2001/XMLSchema#string"/>
	<rdfs:comment>Specifies the matching signature detected for the packer, if applicable.</rdfs:comment>
	<rdfs:isDefinedBy rdf:datatype="http://www.w3.org/2001/XMLSchema#string">&lt;http://cybox.mitre.org/objects/File&gt;</rdfs:isDefinedBy>
	<rdfs:label>Signature</rdfs:label>
</rdf:Description>
<!--  -->
<!-- http://cybox.mitre.org/objects/File#size -->

<rdf:Description rdf:about="http://cybox.mitre.org/objects/File#size">
	<rdf:type rdf:resource="http://www.w3.org/2002/07/owl#DatatypeProperty"/>
	<rdfs:range rdf:resource="http://www.w3.org/2001/XMLSchema#positiveInteger"/>
	<rdfs:comment>Specifies the total number of entries in the file's cross-reference table.</rdfs:comment>
	<rdfs:isDefinedBy rdf:resource="http://cybox.mitre.org/objects/File"/>
	<rdfs:label>Size</rdfs:label>
</rdf:Description>
<!--  -->
<!-- http://cybox.mitre.org/objects/File#sizeInBytes -->

<rdf:Description rdf:about="http://cybox.mitre.org/objects/File#sizeInBytes">
	<rdf:type rdf:resource="http://www.w3.org/2002/07/owl#DatatypeProperty"/>
	<rdfs:range rdf:resource="http://www.w3.org/2001/XMLSchema#unsignedLong"/>
	<rdfs:comment>Specifies the size of the file, in bytes.</rdfs:comment>
	<rdfs:isDefinedBy rdf:resource="http://cybox.mitre.org/objects/File"/>
	<rdfs:label>Size in Bytes</rdfs:label>
</rdf:Description>
<!--  -->
<!-- http://cybox.mitre.org/objects/File#sparseFile -->

<rdf:Description rdf:about="http://cybox.mitre.org/objects/File#sparseFile">
	<rdf:type rdf:resource="http://www.w3.org/2002/07/owl#DatatypeProperty"/>
	<rdfs:range rdf:resource="http://www.w3.org/2001/XMLSchema#boolean"/>
	<rdfs:comment>Specifies a sparse file, as denoted by the constant value, 0x200.</rdfs:comment>
	<rdfs:isDefinedBy rdf:resource="http://cybox.mitre.org/objects/File"/>
	<rdfs:label>Sparse File</rdfs:label>
</rdf:Description>
<!--  -->
<!-- http://cybox.mitre.org/objects/File#specialBuild -->

<rdf:Description rdf:about="http://cybox.mitre.org/objects/File#specialBuild">
	<rdf:type rdf:resource="http://www.w3.org/2002/07/owl#DatatypeProperty"/>
	<rdfs:range rdf:resource="http://www.w3.org/2001/XMLSchema#string"/>
	<rdfs:comment>Specifies the text that indicates how this version of the file differs from the standard version - for example, "Private build for TESTER1 solving mouse problems on M250 and M250E computers". &#xD;
&#xD;
This string should be present only if VS_FF_SPECIALBUILD is specified in the fileflags parameter of the root block.</rdfs:comment>
	<rdfs:isDefinedBy rdf:resource="http://cybox.mitre.org/objects/File"/>
	<rdfs:label>Special Build</rdfs:label>
</rdf:Description>
<!--  -->
<!-- http://cybox.mitre.org/objects/File#streamName -->

<rdf:Description rdf:about="http://cybox.mitre.org/objects/File#streamName">
	<rdf:type rdf:resource="http://www.w3.org/2002/07/owl#DatatypeProperty"/>
	<rdfs:range rdf:resource="http://www.w3.org/2001/XMLSchema#string"/>
	<rdfs:comment></rdfs:comment>
	<rdfs:isDefinedBy rdf:datatype="http://www.w3.org/2001/XMLSchema#string">&lt;http://cybox.mitre.org/objects/File&gt;</rdfs:isDefinedBy>
	<rdfs:label>stream name</rdfs:label>
</rdf:Description>
<!--  -->
<!-- http://cybox.mitre.org/objects/File#subLanguage -->

<rdf:Description rdf:about="http://cybox.mitre.org/objects/File#subLanguage">
	<rdf:type rdf:resource="http://www.w3.org/2002/07/owl#DatatypeProperty"/>
	<rdfs:range rdf:resource="http://www.w3.org/2001/XMLSchema#string"/>
	<rdfs:comment>Specifies the name of the sub language (SUBLANG) defined for the resource, if applicable.</rdfs:comment>
	<rdfs:isDefinedBy rdf:resource="http://cybox.mitre.org/objects/File"/>
	<rdfs:label>Sub-language</rdfs:label>
</rdf:Description>
<!--  -->
<!-- http://cybox.mitre.org/objects/File#suid -->

<rdf:Description rdf:about="http://cybox.mitre.org/objects/File#suid">
	<rdf:type rdf:resource="http://www.w3.org/2002/07/owl#DatatypeProperty"/>
	<rdfs:range rdf:resource="http://www.w3.org/2001/XMLSchema#boolean"/>
	<rdfs:comment>Specifies whether or not the file may be exectued with the privileges of the file's owner.</rdfs:comment>
	<rdfs:isDefinedBy rdf:resource="http://cybox.mitre.org/objects/File"/>
	<rdfs:label>suid</rdfs:label>
</rdf:Description>
<!--  -->
<!-- http://cybox.mitre.org/objects/File#symbolicLinks -->

<rdf:Description rdf:about="http://cybox.mitre.org/objects/File#symbolicLinks">
	<rdf:type rdf:resource="http://www.w3.org/2002/07/owl#DatatypeProperty"/>
	<rdfs:range rdf:resource="http://www.w3.org/2001/XMLSchema#string"/>
	<rdfs:comment>Specifies any symbolic links that may exist for the file.</rdfs:comment>
	<rdfs:isDefinedBy rdf:datatype="http://www.w3.org/2001/XMLSchema#string">&lt;http://cybox.mitre.org/objects/File&gt;</rdfs:isDefinedBy>
	<rdfs:label>Symbolic Links</rdfs:label>
</rdf:Description>
<!--  -->
<!-- http://cybox.mitre.org/objects/File#system -->

<rdf:Description rdf:about="http://cybox.mitre.org/objects/File#system">
	<rdf:type rdf:resource="http://www.w3.org/2002/07/owl#DatatypeProperty"/>
	<rdfs:range rdf:resource="http://www.w3.org/2001/XMLSchema#boolean"/>
	<rdfs:comment>Specifies a file or directory that the operating system uses a part of, or uses exclusively, as denoted by the constant value, 0x4.</rdfs:comment>
	<rdfs:isDefinedBy rdf:resource="http://cybox.mitre.org/objects/File"/>
	<rdfs:label>System</rdfs:label>
</rdf:Description>
<!--  -->
<!-- http://cybox.mitre.org/objects/File#temporary -->

<rdf:Description rdf:about="http://cybox.mitre.org/objects/File#temporary">
	<rdf:type rdf:resource="http://www.w3.org/2002/07/owl#DatatypeProperty"/>
	<rdfs:range rdf:resource="http://www.w3.org/2001/XMLSchema#boolean"/>
	<rdfs:comment>Specifies a file being used for temporary storage, as denoted by the constant value, 0x100.</rdfs:comment>
	<rdfs:isDefinedBy rdf:resource="http://cybox.mitre.org/objects/File"/>
	<rdfs:label>Temporary</rdfs:label>
</rdf:Description>
<!--  -->
<!-- http://cybox.mitre.org/objects/File#tlsTable.size -->

<rdf:Description rdf:about="http://cybox.mitre.org/objects/File#tlsTable.size">
	<rdf:type rdf:resource="http://www.w3.org/2002/07/owl#DatatypeProperty"/>
	<rdfs:range rdf:resource="http://www.w3.org/2001/XMLSchema#nonNegativeInteger"/>
	<rdfs:comment>Specifies the size of the data structure, in bytes, of the Thread Local Storage (TLS) Table</rdfs:comment>
	<rdfs:isDefinedBy rdf:resource="http://cybox.mitre.org/objects/File"/>
	<rdfs:label>Thread Local Storage (TLS) Table Size</rdfs:label>
</rdf:Description>
<!--  -->
<!-- http://cybox.mitre.org/objects/File#tlsTable.virtualAddress -->

<rdf:Description rdf:about="http://cybox.mitre.org/objects/File#tlsTable.virtualAddress">
	<rdf:type rdf:resource="http://www.w3.org/2002/07/owl#DatatypeProperty"/>
	<rdfs:range rdf:resource="http://www.w3.org/2001/XMLSchema#hexBinary"/>
	<rdfs:comment>Secifies the relative virtual address (RVA) of the Thread Local Storage (TLS) Table.</rdfs:comment>
	<rdfs:isDefinedBy rdf:resource="http://cybox.mitre.org/objects/File"/>
	<rdfs:label>Thread Local Storage (TLS) Table Virtual Address</rdfs:label>
</rdf:Description>
<!--  -->
<!-- http://cybox.mitre.org/objects/File#uexec -->

<rdf:Description rdf:about="http://cybox.mitre.org/objects/File#uexec">
	<rdf:type rdf:resource="http://www.w3.org/2002/07/owl#DatatypeProperty"/>
	<rdfs:range rdf:resource="http://www.w3.org/2001/XMLSchema#boolean"/>
	<rdfs:comment>Specifies whether or not the owner of the file can execute it.</rdfs:comment>
	<rdfs:isDefinedBy rdf:resource="http://cybox.mitre.org/objects/File"/>
	<rdfs:label>uexec</rdfs:label>
</rdf:Description>
<!--  -->
<!-- http://cybox.mitre.org/objects/File#unixFileType -->

<rdf:Description rdf:about="http://cybox.mitre.org/objects/File#unixFileType">
	<rdf:type rdf:resource="http://www.w3.org/2002/07/owl#DatatypeProperty"/>
	<rdfs:range rdf:resource="http://www.w3.org/2001/XMLSchema#string"/>
	<rdfs:comment>Specifies file type.</rdfs:comment>
	<rdfs:isDefinedBy rdf:resource="http://cybox.mitre.org/objects/File"/>
	<rdfs:label>Unix File Type</rdfs:label>
</rdf:Description>
<!--  -->
<!-- http://cybox.mitre.org/objects/File#uread -->

<rdf:Description rdf:about="http://cybox.mitre.org/objects/File#uread">
	<rdf:type rdf:resource="http://www.w3.org/2002/07/owl#DatatypeProperty"/>
	<rdfs:range rdf:resource="http://www.w3.org/2001/XMLSchema#boolean"/>
	<rdfs:comment>Specifies whether or not the owner of the file can read its contents.</rdfs:comment>
	<rdfs:isDefinedBy rdf:resource="http://cybox.mitre.org/objects/File"/>
	<rdfs:label>uread</rdfs:label>
</rdf:Description>
<!--  -->
<!-- http://cybox.mitre.org/objects/File#uwrite -->

<rdf:Description rdf:about="http://cybox.mitre.org/objects/File#uwrite">
	<rdf:type rdf:resource="http://www.w3.org/2002/07/owl#DatatypeProperty"/>
	<rdfs:range rdf:resource="http://www.w3.org/2001/XMLSchema#boolean"/>
	<rdfs:comment>Specifies whether or not the owner of the file can write to it.</rdfs:comment>
	<rdfs:isDefinedBy rdf:resource="http://cybox.mitre.org/objects/File"/>
	<rdfs:label>uwrite</rdfs:label>
</rdf:Description>
<!--  -->
<!-- http://cybox.mitre.org/objects/File#virtual -->

<rdf:Description rdf:about="http://cybox.mitre.org/objects/File#virtual">
	<rdf:type rdf:resource="http://www.w3.org/2002/07/owl#DatatypeProperty"/>
	<rdfs:range rdf:resource="http://www.w3.org/2001/XMLSchema#boolean"/>
	<rdfs:comment>Specifies a reserved system value, as denoted by the constant value, 0x10000.</rdfs:comment>
	<rdfs:isDefinedBy rdf:resource="http://cybox.mitre.org/objects/File"/>
	<rdfs:label>Virtual</rdfs:label>
</rdf:Description>
<!--  -->
<!-- http://cybox.mitre.org/objects/File#virtualAddress -->

<rdf:Description rdf:about="http://cybox.mitre.org/objects/File#virtualAddress">
	<rdf:type rdf:resource="http://www.w3.org/2002/07/owl#DatatypeProperty"/>
	<rdfs:range rdf:resource="http://www.w3.org/2001/XMLSchema#hexBinary"/>
	<rdfs:comment>Specifies the relative virtual address (RVA) of the entity within  PE binary library.</rdfs:comment>
	<rdfs:isDefinedBy rdf:resource="http://cybox.mitre.org/objects/File"/>
	<rdfs:label>Virtual Address</rdfs:label>
</rdf:Description>
<!--  -->
<!-- http://cybox.mitre.org/objects/File#write -->

<rdf:Description rdf:about="http://cybox.mitre.org/objects/File#write">
	<rdf:type rdf:resource="http://www.w3.org/2002/07/owl#DatatypeProperty"/>
	<rdfs:range rdf:resource="http://www.w3.org/2001/XMLSchema#boolean"/>
	<rdfs:comment>Specifies whether writing to the file is permitted.</rdfs:comment>
	<rdfs:isDefinedBy rdf:resource="http://cybox.mitre.org/objects/File"/>
	<rdfs:label>Write</rdfs:label>
</rdf:Description>
<!--  -->
<!-- http://cybox.mitre.org/objects/File#xfaCount.nonObfuscated -->

<rdf:Description rdf:about="http://cybox.mitre.org/objects/File#xfaCount.nonObfuscated">
	<rdf:type rdf:resource="http://www.w3.org/2002/07/owl#DatatypeProperty"/>
	<rdfs:range rdf:resource="http://www.w3.org/2001/XMLSchema#nonNegativeInteger"/>
	<rdfs:comment>Specifies the number of non-obfuscated occurrences of the '/XFA' keyword in the PDF file.</rdfs:comment>
	<rdfs:isDefinedBy rdf:resource="http://cybox.mitre.org/objects/File"/>
	<rdfs:label>'/XFA' Non-obfuscated Count</rdfs:label>
</rdf:Description>
<!--  -->
<!-- http://cybox.mitre.org/objects/File#xfaCount.obfuscated -->

<rdf:Description rdf:about="http://cybox.mitre.org/objects/File#xfaCount.obfuscated">
	<rdf:type rdf:resource="http://www.w3.org/2002/07/owl#DatatypeProperty"/>
	<rdfs:range rdf:resource="http://www.w3.org/2001/XMLSchema#nonNegativeInteger"/>
	<rdfs:comment>Specifies the number of obfuscated occurrences of the '/XFA' keyword in the PDF file with some form of obfuscation, such as with hexcodes.</rdfs:comment>
	<rdfs:isDefinedBy rdf:resource="http://cybox.mitre.org/objects/File"/>
	<rdfs:label>'/XFA' Obfuscated Count</rdfs:label>
</rdf:Description>
<!--  -->
<!-- http://cybox.mitre.org/objects/File#xrefEntryType -->

<rdf:Description rdf:about="http://cybox.mitre.org/objects/File#xrefEntryType">
	<rdf:type rdf:resource="http://www.w3.org/2002/07/owl#DatatypeProperty"/>
	<rdfs:range rdf:nodeID="genid13"/>
</rdf:Description>

<rdf:Description rdf:nodeID="genid13">
	<rdf:type rdf:resource="http://www.w3.org/2000/01/rdf-schema#Datatype"/>
	<owl:oneOf rdf:nodeID="genid15"/>
</rdf:Description>

<rdf:Description rdf:nodeID="genid15">
	<rdf:type rdf:resource="http://www.w3.org/1999/02/22-rdf-syntax-ns#List"/>
	<rdf:first rdf:datatype="http://www.w3.org/2001/XMLSchema#string">Free</rdf:first>
	<rdf:rest rdf:nodeID="genid14"/>
</rdf:Description>

<rdf:Description rdf:nodeID="genid14">
	<rdf:type rdf:resource="http://www.w3.org/1999/02/22-rdf-syntax-ns#List"/>
	<rdf:first rdf:datatype="http://www.w3.org/2001/XMLSchema#string">In-Use</rdf:first>
	<rdf:rest rdf:resource="http://www.w3.org/1999/02/22-rdf-syntax-ns#nil"/>
</rdf:Description>

<rdf:Description rdf:about="http://cybox.mitre.org/objects/File#xrefEntryType">
	<rdfs:comment>Specifies the type of the cross-reference entry.</rdfs:comment>
	<rdfs:isDefinedBy rdf:resource="http://cybox.mitre.org/objects/File"/>
	<rdfs:label>Cross-Reference Entry Type</rdfs:label>
</rdf:Description>
<!--  -->
<!-- http://cybox.mitre.org/objects/File#xrefOffset -->

<rdf:Description rdf:about="http://cybox.mitre.org/objects/File#xrefOffset">
	<rdf:type rdf:resource="http://www.w3.org/2002/07/owl#DatatypeProperty"/>
	<rdfs:range rdf:resource="http://www.w3.org/2001/XMLSchema#positiveInteger"/>
	<rdfs:comment>Sspecifies the offset of the cross-reference from the beginning of the file, in bytes.</rdfs:comment>
	<rdfs:isDefinedBy rdf:resource="http://cybox.mitre.org/objects/File"/>
	<rdfs:label>Cross-Reference Table Offset</rdfs:label>
</rdf:Description>
<!--  -->
<!--  -->
<!--  -->
<!-- ################################################################# -->
<!-- # -->
<!-- #    Classes -->
<!-- # -->
<!-- ################################################################# -->
<!--  -->
<!--  -->
<!-- http://cybox.mitre.org/cyboxCommon#DigitalSignature -->
<!--  -->
<!-- http://cybox.mitre.org/cyboxCommon#Hash -->
<!--  -->
<!-- http://cybox.mitre.org/cybox_core#Object -->

<rdf:Description rdf:about="http://cybox.mitre.org/cybox_core#Object">
	<rdf:type rdf:resource="http://www.w3.org/2002/07/owl#Class"/>
</rdf:Description>
<!--  -->
<!-- http://cybox.mitre.org/objects/Code#Code -->
<!--  -->
<!-- http://cybox.mitre.org/objects/File#ArchiveFile -->

<rdf:Description rdf:about="http://cybox.mitre.org/objects/File#ArchiveFile">
	<rdf:type rdf:resource="http://www.w3.org/2002/07/owl#Class"/>
	<rdfs:subClassOf rdf:resource="http://cybox.mitre.org/objects/File#File"/>
	<rdfs:subClassOf rdf:nodeID="genid16"/>
</rdf:Description>

<rdf:Description rdf:nodeID="genid16">
	<rdf:type rdf:resource="http://www.w3.org/2002/07/owl#Restriction"/>
	<owl:onProperty rdf:resource="http://cybox.mitre.org/objects/File#archiveComment"/>
	<owl:maxCardinality rdf:datatype="http://www.w3.org/2001/XMLSchema#nonNegativeInteger">1</owl:maxCardinality>
</rdf:Description>

<rdf:Description rdf:about="http://cybox.mitre.org/objects/File#ArchiveFile">
	<rdfs:subClassOf rdf:nodeID="genid17"/>
</rdf:Description>

<rdf:Description rdf:nodeID="genid17">
	<rdf:type rdf:resource="http://www.w3.org/2002/07/owl#Restriction"/>
	<owl:onProperty rdf:resource="http://cybox.mitre.org/objects/File#archiveFormat"/>
	<owl:maxCardinality rdf:datatype="http://www.w3.org/2001/XMLSchema#nonNegativeInteger">1</owl:maxCardinality>
</rdf:Description>

<rdf:Description rdf:about="http://cybox.mitre.org/objects/File#ArchiveFile">
	<rdfs:subClassOf rdf:nodeID="genid18"/>
</rdf:Description>

<rdf:Description rdf:nodeID="genid18">
	<rdf:type rdf:resource="http://www.w3.org/2002/07/owl#Restriction"/>
	<owl:onProperty rdf:resource="http://cybox.mitre.org/objects/File#archiveVersion"/>
	<owl:maxCardinality rdf:datatype="http://www.w3.org/2001/XMLSchema#nonNegativeInteger">1</owl:maxCardinality>
</rdf:Description>

<rdf:Description rdf:about="http://cybox.mitre.org/objects/File#ArchiveFile">
	<rdfs:subClassOf rdf:nodeID="genid19"/>
</rdf:Description>

<rdf:Description rdf:nodeID="genid19">
	<rdf:type rdf:resource="http://www.w3.org/2002/07/owl#Restriction"/>
	<owl:onProperty rdf:resource="http://cybox.mitre.org/objects/File#fileCount"/>
	<owl:maxCardinality rdf:datatype="http://www.w3.org/2001/XMLSchema#nonNegativeInteger">1</owl:maxCardinality>
</rdf:Description>

<rdf:Description rdf:about="http://cybox.mitre.org/objects/File#ArchiveFile">
	<rdfs:comment>Characterize archive files.</rdfs:comment>
	<rdfs:isDefinedBy rdf:resource="http://cybox.mitre.org/objects/File"/>
	<rdfs:label>Archive file</rdfs:label>
</rdf:Description>
<!--  -->
<!-- http://cybox.mitre.org/objects/File#DeviceObjectStruct -->

<rdf:Description rdf:about="http://cybox.mitre.org/objects/File#DeviceObjectStruct">
	<rdf:type rdf:resource="http://www.w3.org/2002/07/owl#Class"/>
	<rdfs:subClassOf rdf:nodeID="genid20"/>
</rdf:Description>

<rdf:Description rdf:nodeID="genid20">
	<rdf:type rdf:resource="http://www.w3.org/2002/07/owl#Restriction"/>
	<owl:onProperty rdf:resource="http://cybox.mitre.org/objects/File#deviceName"/>
	<owl:cardinality rdf:datatype="http://www.w3.org/2001/XMLSchema#nonNegativeInteger">1</owl:cardinality>
</rdf:Description>

<rdf:Description rdf:about="http://cybox.mitre.org/objects/File#DeviceObjectStruct">
	<rdfs:subClassOf rdf:nodeID="genid21"/>
</rdf:Description>

<rdf:Description rdf:nodeID="genid21">
	<rdf:type rdf:resource="http://www.w3.org/2002/07/owl#Restriction"/>
	<owl:onProperty rdf:resource="http://cybox.mitre.org/objects/File#deviceObject"/>
	<owl:cardinality rdf:datatype="http://www.w3.org/2001/XMLSchema#nonNegativeInteger">1</owl:cardinality>
</rdf:Description>

<rdf:Description rdf:about="http://cybox.mitre.org/objects/File#DeviceObjectStruct">
	<rdfs:subClassOf rdf:nodeID="genid22"/>
</rdf:Description>

<rdf:Description rdf:nodeID="genid22">
	<rdf:type rdf:resource="http://www.w3.org/2002/07/owl#Restriction"/>
	<owl:onProperty rdf:resource="http://cybox.mitre.org/objects/File#attachedDeviceName"/>
	<owl:maxCardinality rdf:datatype="http://www.w3.org/2001/XMLSchema#nonNegativeInteger">1</owl:maxCardinality>
</rdf:Description>

<rdf:Description rdf:about="http://cybox.mitre.org/objects/File#DeviceObjectStruct">
	<rdfs:subClassOf rdf:nodeID="genid23"/>
</rdf:Description>

<rdf:Description rdf:nodeID="genid23">
	<rdf:type rdf:resource="http://www.w3.org/2002/07/owl#Restriction"/>
	<owl:onProperty rdf:resource="http://cybox.mitre.org/objects/File#attachedDeviceObject"/>
	<owl:maxCardinality rdf:datatype="http://www.w3.org/2001/XMLSchema#nonNegativeInteger">1</owl:maxCardinality>
</rdf:Description>

<rdf:Description rdf:about="http://cybox.mitre.org/objects/File#DeviceObjectStruct">
	<rdfs:subClassOf rdf:nodeID="genid24"/>
</rdf:Description>

<rdf:Description rdf:nodeID="genid24">
	<rdf:type rdf:resource="http://www.w3.org/2002/07/owl#Restriction"/>
	<owl:onProperty rdf:resource="http://cybox.mitre.org/objects/File#attachedToDeviceName"/>
	<owl:maxCardinality rdf:datatype="http://www.w3.org/2001/XMLSchema#nonNegativeInteger">1</owl:maxCardinality>
</rdf:Description>

<rdf:Description rdf:about="http://cybox.mitre.org/objects/File#DeviceObjectStruct">
	<rdfs:subClassOf rdf:nodeID="genid25"/>
</rdf:Description>

<rdf:Description rdf:nodeID="genid25">
	<rdf:type rdf:resource="http://www.w3.org/2002/07/owl#Restriction"/>
	<owl:onProperty rdf:resource="http://cybox.mitre.org/objects/File#attachedToDeviceObject"/>
	<owl:maxCardinality rdf:datatype="http://www.w3.org/2001/XMLSchema#nonNegativeInteger">1</owl:maxCardinality>
</rdf:Description>

<rdf:Description rdf:about="http://cybox.mitre.org/objects/File#DeviceObjectStruct">
	<rdfs:subClassOf rdf:nodeID="genid26"/>
</rdf:Description>

<rdf:Description rdf:nodeID="genid26">
	<rdf:type rdf:resource="http://www.w3.org/2002/07/owl#Restriction"/>
	<owl:onProperty rdf:resource="http://cybox.mitre.org/objects/File#attachedToDriverName"/>
	<owl:maxCardinality rdf:datatype="http://www.w3.org/2001/XMLSchema#nonNegativeInteger">1</owl:maxCardinality>
</rdf:Description>

<rdf:Description rdf:about="http://cybox.mitre.org/objects/File#DeviceObjectStruct">
	<rdfs:subClassOf rdf:nodeID="genid27"/>
</rdf:Description>

<rdf:Description rdf:nodeID="genid27">
	<rdf:type rdf:resource="http://www.w3.org/2002/07/owl#Restriction"/>
	<owl:onProperty rdf:resource="http://cybox.mitre.org/objects/File#attachedToDriverObject"/>
	<owl:maxCardinality rdf:datatype="http://www.w3.org/2001/XMLSchema#nonNegativeInteger">1</owl:maxCardinality>
</rdf:Description>

<rdf:Description rdf:about="http://cybox.mitre.org/objects/File#DeviceObjectStruct">
	<rdfs:comment>Characterizes the properties of a device object. In this context, a device object represents a logical, virtual, or physical device for which a driver handles I/O requests. 

See also: http://msdn.microsoft.com/en-us/library/windows/hardware/ff543147(v=vs.85).aspx.</rdfs:comment>
	<rdfs:isDefinedBy rdf:resource="http://cybox.mitre.org/objects/File"/>
	<rdfs:label>Device Object Struct</rdfs:label>
</rdf:Description>
<!--  -->
<!-- http://cybox.mitre.org/objects/File#EntryPointSignature -->

<rdf:Description rdf:about="http://cybox.mitre.org/objects/File#EntryPointSignature">
	<rdf:type rdf:resource="http://www.w3.org/2002/07/owl#Class"/>
</rdf:Description>


<rdf:Description rdf:about="http://cybox.mitre.org/objects/File#EntryPointSignature">
	<rdfs:subClassOf rdf:nodeID="genid28"/>
</rdf:Description>

<rdf:Description rdf:nodeID="genid28">
	<rdf:type rdf:resource="http://www.w3.org/2002/07/owl#Restriction"/>
	<owl:onProperty rdf:resource="http://cybox.mitre.org/objects/File#entrypointSignatureName"/>
	<owl:cardinality rdf:datatype="http://www.w3.org/2001/XMLSchema#nonNegativeInteger">1</owl:cardinality>
</rdf:Description>

<rdf:Description rdf:about="http://cybox.mitre.org/objects/File#EntryPointSignature">
	<rdfs:subClassOf rdf:nodeID="genid29"/>
</rdf:Description>

<rdf:Description rdf:nodeID="genid29">
	<rdf:type rdf:resource="http://www.w3.org/2002/07/owl#Restriction"/>
	<owl:onProperty rdf:resource="http://cybox.mitre.org/objects/File#entrypointSignatureType"/>
	<owl:maxCardinality rdf:datatype="http://www.w3.org/2001/XMLSchema#nonNegativeInteger">1</owl:maxCardinality>
</rdf:Description>

<rdf:Description rdf:about="http://cybox.mitre.org/objects/File#EntryPointSignature">
	<rdfs:comment>Characterizes an  entry point signature for a packer.</rdfs:comment>
	<rdfs:isDefinedBy rdf:resource="http://cybox.mitre.org/objects/File"/>
	<rdfs:label>Entrypoint Signature</rdfs:label>
</rdf:Description>
<!--  -->
<!-- http://cybox.mitre.org/objects/File#File -->

<rdf:Description rdf:about="http://cybox.mitre.org/objects/File#File">
	<rdf:type rdf:resource="http://www.w3.org/2002/07/owl#Class"/>
	<rdfs:subClassOf rdf:resource="http://cybox.mitre.org/cybox_core#Object"/>
	<rdfs:subClassOf rdf:nodeID="genid30"/>
</rdf:Description>

<rdf:Description rdf:nodeID="genid30">
	<rdf:type rdf:resource="http://www.w3.org/2002/07/owl#Restriction"/>
	<owl:onProperty rdf:resource="http://cybox.mitre.org/objects/File#fileAttributes"/>
	<owl:maxCardinality rdf:datatype="http://www.w3.org/2001/XMLSchema#nonNegativeInteger">1</owl:maxCardinality>
</rdf:Description>

<rdf:Description rdf:about="http://cybox.mitre.org/objects/File#File">
	<rdfs:subClassOf rdf:nodeID="genid31"/>
</rdf:Description>

<rdf:Description rdf:nodeID="genid31">
	<rdf:type rdf:resource="http://www.w3.org/2002/07/owl#Restriction"/>
	<owl:onProperty rdf:resource="http://cybox.mitre.org/objects/File#permissions"/>
	<owl:maxCardinality rdf:datatype="http://www.w3.org/2001/XMLSchema#nonNegativeInteger">1</owl:maxCardinality>
</rdf:Description>

<rdf:Description rdf:about="http://cybox.mitre.org/objects/File#File">
	<rdfs:subClassOf rdf:nodeID="genid32"/>
</rdf:Description>

<rdf:Description rdf:nodeID="genid32">
	<rdf:type rdf:resource="http://www.w3.org/2002/07/owl#Restriction"/>
	<owl:onProperty rdf:resource="http://cybox.mitre.org/objects/File#fileExtension"/>
	<owl:cardinality rdf:datatype="http://www.w3.org/2001/XMLSchema#nonNegativeInteger">1</owl:cardinality>
</rdf:Description>

<rdf:Description rdf:about="http://cybox.mitre.org/objects/File#File">
	<rdfs:subClassOf rdf:nodeID="genid33"/>
</rdf:Description>

<rdf:Description rdf:nodeID="genid33">
	<rdf:type rdf:resource="http://www.w3.org/2002/07/owl#Restriction"/>
	<owl:onProperty rdf:resource="http://cybox.mitre.org/objects/File#fileName"/>
	<owl:cardinality rdf:datatype="http://www.w3.org/2001/XMLSchema#nonNegativeInteger">1</owl:cardinality>
</rdf:Description>

<rdf:Description rdf:about="http://cybox.mitre.org/objects/File#File">
	<rdfs:subClassOf rdf:nodeID="genid34"/>
</rdf:Description>

<rdf:Description rdf:nodeID="genid34">
	<rdf:type rdf:resource="http://www.w3.org/2002/07/owl#Restriction"/>
	<owl:onProperty rdf:resource="http://cybox.mitre.org/objects/File#filePath"/>
	<owl:cardinality rdf:datatype="http://www.w3.org/2001/XMLSchema#nonNegativeInteger">1</owl:cardinality>
</rdf:Description>

<rdf:Description rdf:about="http://cybox.mitre.org/objects/File#File">
	<rdfs:subClassOf rdf:nodeID="genid35"/>
</rdf:Description>

<rdf:Description rdf:nodeID="genid35">
	<rdf:type rdf:resource="http://www.w3.org/2002/07/owl#Restriction"/>
	<owl:onProperty rdf:resource="http://cybox.mitre.org/objects/File#filePath.fullyQualified"/>
	<owl:cardinality rdf:datatype="http://www.w3.org/2001/XMLSchema#nonNegativeInteger">1</owl:cardinality>
</rdf:Description>

<rdf:Description rdf:about="http://cybox.mitre.org/objects/File#File">
	<rdfs:subClassOf rdf:nodeID="genid36"/>
</rdf:Description>

<rdf:Description rdf:nodeID="genid36">
	<rdf:type rdf:resource="http://www.w3.org/2002/07/owl#Restriction"/>
	<owl:onProperty rdf:resource="http://cybox.mitre.org/objects/File#fullPath"/>
	<owl:cardinality rdf:datatype="http://www.w3.org/2001/XMLSchema#nonNegativeInteger">1</owl:cardinality>
</rdf:Description>

<rdf:Description rdf:about="http://cybox.mitre.org/objects/File#File">
	<rdfs:subClassOf rdf:nodeID="genid37"/>
</rdf:Description>

<rdf:Description rdf:nodeID="genid37">
	<rdf:type rdf:resource="http://www.w3.org/2002/07/owl#Restriction"/>
	<owl:onProperty rdf:resource="http://cybox.mitre.org/objects/File#compressionComment"/>
	<owl:maxCardinality rdf:datatype="http://www.w3.org/2001/XMLSchema#nonNegativeInteger">1</owl:maxCardinality>
</rdf:Description>

<rdf:Description rdf:about="http://cybox.mitre.org/objects/File#File">
	<rdfs:subClassOf rdf:nodeID="genid38"/>
</rdf:Description>

<rdf:Description rdf:nodeID="genid38">
	<rdf:type rdf:resource="http://www.w3.org/2002/07/owl#Restriction"/>
	<owl:onProperty rdf:resource="http://cybox.mitre.org/objects/File#compressionMethod"/>
	<owl:maxCardinality rdf:datatype="http://www.w3.org/2001/XMLSchema#nonNegativeInteger">1</owl:maxCardinality>
</rdf:Description>

<rdf:Description rdf:about="http://cybox.mitre.org/objects/File#File">
	<rdfs:subClassOf rdf:nodeID="genid39"/>
</rdf:Description>

<rdf:Description rdf:nodeID="genid39">
	<rdf:type rdf:resource="http://www.w3.org/2002/07/owl#Restriction"/>
	<owl:onProperty rdf:resource="http://cybox.mitre.org/objects/File#compressionVersion"/>
	<owl:maxCardinality rdf:datatype="http://www.w3.org/2001/XMLSchema#nonNegativeInteger">1</owl:maxCardinality>
</rdf:Description>

<rdf:Description rdf:about="http://cybox.mitre.org/objects/File#File">
	<rdfs:subClassOf rdf:nodeID="genid40"/>
</rdf:Description>

<rdf:Description rdf:nodeID="genid40">
	<rdf:type rdf:resource="http://www.w3.org/2002/07/owl#Restriction"/>
	<owl:onProperty rdf:resource="http://cybox.mitre.org/objects/File#createdDateTime"/>
	<owl:maxCardinality rdf:datatype="http://www.w3.org/2001/XMLSchema#nonNegativeInteger">1</owl:maxCardinality>
</rdf:Description>

<rdf:Description rdf:about="http://cybox.mitre.org/objects/File#File">
	<rdfs:subClassOf rdf:nodeID="genid41"/>
</rdf:Description>

<rdf:Description rdf:nodeID="genid41">
	<rdf:type rdf:resource="http://www.w3.org/2002/07/owl#Restriction"/>
	<owl:onProperty rdf:resource="http://cybox.mitre.org/objects/File#decryptionKey"/>
	<owl:maxCardinality rdf:datatype="http://www.w3.org/2001/XMLSchema#nonNegativeInteger">1</owl:maxCardinality>
</rdf:Description>

<rdf:Description rdf:about="http://cybox.mitre.org/objects/File#File">
	<rdfs:subClassOf rdf:nodeID="genid42"/>
</rdf:Description>

<rdf:Description rdf:nodeID="genid42">
	<rdf:type rdf:resource="http://www.w3.org/2002/07/owl#Restriction"/>
	<owl:onProperty rdf:resource="http://cybox.mitre.org/objects/File#devicePath"/>
	<owl:maxCardinality rdf:datatype="http://www.w3.org/2001/XMLSchema#nonNegativeInteger">1</owl:maxCardinality>
</rdf:Description>

<rdf:Description rdf:about="http://cybox.mitre.org/objects/File#File">
	<rdfs:subClassOf rdf:nodeID="genid43"/>
</rdf:Description>

<rdf:Description rdf:nodeID="genid43">
	<rdf:type rdf:resource="http://www.w3.org/2002/07/owl#Restriction"/>
	<owl:onProperty rdf:resource="http://cybox.mitre.org/objects/File#encryptionAlgorithm"/>
	<owl:maxCardinality rdf:datatype="http://www.w3.org/2001/XMLSchema#nonNegativeInteger">1</owl:maxCardinality>
</rdf:Description>

<rdf:Description rdf:about="http://cybox.mitre.org/objects/File#File">
	<rdfs:subClassOf rdf:nodeID="genid44"/>
</rdf:Description>

<rdf:Description rdf:nodeID="genid44">
	<rdf:type rdf:resource="http://www.w3.org/2002/07/owl#Restriction"/>
	<owl:onProperty rdf:resource="http://cybox.mitre.org/objects/File#fileFormat"/>
	<owl:maxCardinality rdf:datatype="http://www.w3.org/2001/XMLSchema#nonNegativeInteger">1</owl:maxCardinality>
</rdf:Description>

<rdf:Description rdf:about="http://cybox.mitre.org/objects/File#File">
	<rdfs:subClassOf rdf:nodeID="genid45"/>
</rdf:Description>

<rdf:Description rdf:nodeID="genid45">
	<rdf:type rdf:resource="http://www.w3.org/2002/07/owl#Restriction"/>
	<owl:onProperty rdf:resource="http://cybox.mitre.org/objects/File#isMasqueraded"/>
	<owl:maxCardinality rdf:datatype="http://www.w3.org/2001/XMLSchema#nonNegativeInteger">1</owl:maxCardinality>
</rdf:Description>

<rdf:Description rdf:about="http://cybox.mitre.org/objects/File#File">
	<rdfs:subClassOf rdf:nodeID="genid46"/>
</rdf:Description>

<rdf:Description rdf:nodeID="genid46">
	<rdf:type rdf:resource="http://www.w3.org/2002/07/owl#Restriction"/>
	<owl:onProperty rdf:resource="http://cybox.mitre.org/objects/File#isPacked"/>
	<owl:maxCardinality rdf:datatype="http://www.w3.org/2001/XMLSchema#nonNegativeInteger">1</owl:maxCardinality>
</rdf:Description>

<rdf:Description rdf:about="http://cybox.mitre.org/objects/File#File">
	<rdfs:subClassOf rdf:nodeID="genid47"/>
</rdf:Description>

<rdf:Description rdf:nodeID="genid47">
	<rdf:type rdf:resource="http://www.w3.org/2002/07/owl#Restriction"/>
	<owl:onProperty rdf:resource="http://cybox.mitre.org/objects/File#lastAccessedDateTime"/>
	<owl:maxCardinality rdf:datatype="http://www.w3.org/2001/XMLSchema#nonNegativeInteger">1</owl:maxCardinality>
</rdf:Description>

<rdf:Description rdf:about="http://cybox.mitre.org/objects/File#File">
	<rdfs:subClassOf rdf:nodeID="genid48"/>
</rdf:Description>

<rdf:Description rdf:nodeID="genid48">
	<rdf:type rdf:resource="http://www.w3.org/2002/07/owl#Restriction"/>
	<owl:onProperty rdf:resource="http://cybox.mitre.org/objects/File#lastModifiedDateTime"/>
	<owl:maxCardinality rdf:datatype="http://www.w3.org/2001/XMLSchema#nonNegativeInteger">1</owl:maxCardinality>
</rdf:Description>

<rdf:Description rdf:about="http://cybox.mitre.org/objects/File#File">
	<rdfs:subClassOf rdf:nodeID="genid49"/>
</rdf:Description>

<rdf:Description rdf:nodeID="genid49">
	<rdf:type rdf:resource="http://www.w3.org/2002/07/owl#Restriction"/>
	<owl:onProperty rdf:resource="http://cybox.mitre.org/objects/File#magicNumber"/>
	<owl:maxCardinality rdf:datatype="http://www.w3.org/2001/XMLSchema#nonNegativeInteger">1</owl:maxCardinality>
</rdf:Description>

<rdf:Description rdf:about="http://cybox.mitre.org/objects/File#File">
	<rdfs:subClassOf rdf:nodeID="genid50"/>
</rdf:Description>

<rdf:Description rdf:nodeID="genid50">
	<rdf:type rdf:resource="http://www.w3.org/2002/07/owl#Restriction"/>
	<owl:onProperty rdf:resource="http://cybox.mitre.org/objects/File#ownerName"/>
	<owl:maxCardinality rdf:datatype="http://www.w3.org/2001/XMLSchema#nonNegativeInteger">1</owl:maxCardinality>
</rdf:Description>

<rdf:Description rdf:about="http://cybox.mitre.org/objects/File#File">
	<rdfs:subClassOf rdf:nodeID="genid51"/>
</rdf:Description>

<rdf:Description rdf:nodeID="genid51">
	<rdf:type rdf:resource="http://www.w3.org/2002/07/owl#Restriction"/>
	<owl:onProperty rdf:resource="http://cybox.mitre.org/objects/File#peakEntropy"/>
	<owl:maxCardinality rdf:datatype="http://www.w3.org/2001/XMLSchema#nonNegativeInteger">1</owl:maxCardinality>
</rdf:Description>

<rdf:Description rdf:about="http://cybox.mitre.org/objects/File#File">
	<rdfs:subClassOf rdf:nodeID="genid52"/>
</rdf:Description>

<rdf:Description rdf:nodeID="genid52">
	<rdf:type rdf:resource="http://www.w3.org/2002/07/owl#Restriction"/>
	<owl:onProperty rdf:resource="http://cybox.mitre.org/objects/File#sizeInBytes"/>
	<owl:maxCardinality rdf:datatype="http://www.w3.org/2001/XMLSchema#nonNegativeInteger">1</owl:maxCardinality>
</rdf:Description>

<rdf:Description rdf:about="http://cybox.mitre.org/objects/File#File">
	<rdfs:comment>Characterizes information about a generic file.</rdfs:comment>
	<rdfs:isDefinedBy rdf:resource="http://cybox.mitre.org/objects/File"/>
	<rdfs:label>File</rdfs:label>
</rdf:Description>
<!--  -->
<!-- http://cybox.mitre.org/objects/File#FileAttribute -->

<rdf:Description rdf:about="http://cybox.mitre.org/objects/File#FileAttribute">
	<rdf:type rdf:resource="http://www.w3.org/2002/07/owl#Class"/>
	<rdfs:comment>Characterizes attributes of a file</rdfs:comment>
	<rdfs:isDefinedBy rdf:resource="http://cybox.mitre.org/objects/File"/>
	<rdfs:label>File Attribute</rdfs:label>
</rdf:Description>
<!--  -->
<!-- http://cybox.mitre.org/objects/File#FilePermission -->

<rdf:Description rdf:about="http://cybox.mitre.org/objects/File#FilePermission">
	<rdf:type rdf:resource="http://www.w3.org/2002/07/owl#Class"/>
	<rdfs:comment>Characterizes permissions on a file.</rdfs:comment>
	<rdfs:isDefinedBy rdf:resource="http://cybox.mitre.org/objects/File"/>
	<rdfs:label>File Permission</rdfs:label>
</rdf:Description>
<!--  -->
<!-- http://cybox.mitre.org/objects/File#ImageFile -->

<rdf:Description rdf:about="http://cybox.mitre.org/objects/File#ImageFile">
	<rdf:type rdf:resource="http://www.w3.org/2002/07/owl#Class"/>
	<rdfs:subClassOf rdf:resource="http://cybox.mitre.org/objects/File#File"/>
	<rdfs:subClassOf rdf:nodeID="genid53"/>
</rdf:Description>

<rdf:Description rdf:nodeID="genid53">
	<rdf:type rdf:resource="http://www.w3.org/2002/07/owl#Restriction"/>
	<owl:onProperty rdf:resource="http://cybox.mitre.org/objects/File#bitsPerPixel"/>
	<owl:maxCardinality rdf:datatype="http://www.w3.org/2001/XMLSchema#nonNegativeInteger">1</owl:maxCardinality>
</rdf:Description>

<rdf:Description rdf:about="http://cybox.mitre.org/objects/File#ImageFile">
	<rdfs:subClassOf rdf:nodeID="genid54"/>
</rdf:Description>

<rdf:Description rdf:nodeID="genid54">
	<rdf:type rdf:resource="http://www.w3.org/2002/07/owl#Restriction"/>
	<owl:onProperty rdf:resource="http://cybox.mitre.org/objects/File#compressionAlgorithm"/>
	<owl:maxCardinality rdf:datatype="http://www.w3.org/2001/XMLSchema#nonNegativeInteger">1</owl:maxCardinality>
</rdf:Description>

<rdf:Description rdf:about="http://cybox.mitre.org/objects/File#ImageFile">
	<rdfs:subClassOf rdf:nodeID="genid55"/>
</rdf:Description>

<rdf:Description rdf:nodeID="genid55">
	<rdf:type rdf:resource="http://www.w3.org/2002/07/owl#Restriction"/>
	<owl:onProperty rdf:resource="http://cybox.mitre.org/objects/File#imageFileFormat"/>
	<owl:maxCardinality rdf:datatype="http://www.w3.org/2001/XMLSchema#nonNegativeInteger">1</owl:maxCardinality>
</rdf:Description>

<rdf:Description rdf:about="http://cybox.mitre.org/objects/File#ImageFile">
	<rdfs:subClassOf rdf:nodeID="genid56"/>
</rdf:Description>

<rdf:Description rdf:nodeID="genid56">
	<rdf:type rdf:resource="http://www.w3.org/2002/07/owl#Restriction"/>
	<owl:onProperty rdf:resource="http://cybox.mitre.org/objects/File#imageHeight"/>
	<owl:maxCardinality rdf:datatype="http://www.w3.org/2001/XMLSchema#nonNegativeInteger">1</owl:maxCardinality>
</rdf:Description>

<rdf:Description rdf:about="http://cybox.mitre.org/objects/File#ImageFile">
	<rdfs:subClassOf rdf:nodeID="genid57"/>
</rdf:Description>

<rdf:Description rdf:nodeID="genid57">
	<rdf:type rdf:resource="http://www.w3.org/2002/07/owl#Restriction"/>
	<owl:onProperty rdf:resource="http://cybox.mitre.org/objects/File#imageIsCompressed"/>
	<owl:maxCardinality rdf:datatype="http://www.w3.org/2001/XMLSchema#nonNegativeInteger">1</owl:maxCardinality>
</rdf:Description>

<rdf:Description rdf:about="http://cybox.mitre.org/objects/File#ImageFile">
	<rdfs:subClassOf rdf:nodeID="genid58"/>
</rdf:Description>

<rdf:Description rdf:nodeID="genid58">
	<rdf:type rdf:resource="http://www.w3.org/2002/07/owl#Restriction"/>
	<owl:onProperty rdf:resource="http://cybox.mitre.org/objects/File#imageWidth"/>
	<owl:maxCardinality rdf:datatype="http://www.w3.org/2001/XMLSchema#nonNegativeInteger">1</owl:maxCardinality>
</rdf:Description>

<rdf:Description rdf:about="http://cybox.mitre.org/objects/File#ImageFile">
	<rdfs:comment>Characterize image files.</rdfs:comment>
	<rdfs:isDefinedBy rdf:resource="http://cybox.mitre.org/objects/File"/>
	<rdfs:label>Image file</rdfs:label>
</rdf:Description>
<!--  -->
<!-- http://cybox.mitre.org/objects/File#PDFFile -->

<rdf:Description rdf:about="http://cybox.mitre.org/objects/File#PDFFile">
	<rdf:type rdf:resource="http://www.w3.org/2002/07/owl#Class"/>
	<rdfs:subClassOf rdf:resource="http://cybox.mitre.org/objects/File#File"/>
	<rdfs:subClassOf rdf:nodeID="genid59"/>
</rdf:Description>

<rdf:Description rdf:nodeID="genid59">
	<rdf:type rdf:resource="http://www.w3.org/2002/07/owl#Restriction"/>
	<owl:onProperty rdf:resource="http://cybox.mitre.org/objects/File#aaCount.nonObfuscated"/>
	<owl:maxCardinality rdf:datatype="http://www.w3.org/2001/XMLSchema#nonNegativeInteger">1</owl:maxCardinality>
</rdf:Description>

<rdf:Description rdf:about="http://cybox.mitre.org/objects/File#PDFFile">
	<rdfs:subClassOf rdf:nodeID="genid60"/>
</rdf:Description>

<rdf:Description rdf:nodeID="genid60">
	<rdf:type rdf:resource="http://www.w3.org/2002/07/owl#Restriction"/>
	<owl:onProperty rdf:resource="http://cybox.mitre.org/objects/File#aaCount.obfuscated"/>
	<owl:maxCardinality rdf:datatype="http://www.w3.org/2001/XMLSchema#nonNegativeInteger">1</owl:maxCardinality>
</rdf:Description>

<rdf:Description rdf:about="http://cybox.mitre.org/objects/File#PDFFile">
	<rdfs:subClassOf rdf:nodeID="genid61"/>
</rdf:Description>

<rdf:Description rdf:nodeID="genid61">
	<rdf:type rdf:resource="http://www.w3.org/2002/07/owl#Restriction"/>
	<owl:onProperty rdf:resource="http://cybox.mitre.org/objects/File#asciiHexDecodeCount.nonObfuscated"/>
	<owl:maxCardinality rdf:datatype="http://www.w3.org/2001/XMLSchema#nonNegativeInteger">1</owl:maxCardinality>
</rdf:Description>

<rdf:Description rdf:about="http://cybox.mitre.org/objects/File#PDFFile">
	<rdfs:subClassOf rdf:nodeID="genid62"/>
</rdf:Description>

<rdf:Description rdf:nodeID="genid62">
	<rdf:type rdf:resource="http://www.w3.org/2002/07/owl#Restriction"/>
	<owl:onProperty rdf:resource="http://cybox.mitre.org/objects/File#asciiHexDecodeCount.obfuscated"/>
	<owl:maxCardinality rdf:datatype="http://www.w3.org/2001/XMLSchema#nonNegativeInteger">1</owl:maxCardinality>
</rdf:Description>

<rdf:Description rdf:about="http://cybox.mitre.org/objects/File#PDFFile">
	<rdfs:subClassOf rdf:nodeID="genid63"/>
</rdf:Description>

<rdf:Description rdf:nodeID="genid63">
	<rdf:type rdf:resource="http://www.w3.org/2002/07/owl#Restriction"/>
	<owl:onProperty rdf:resource="http://cybox.mitre.org/objects/File#docInfo.authorName"/>
	<owl:maxCardinality rdf:datatype="http://www.w3.org/2001/XMLSchema#nonNegativeInteger">1</owl:maxCardinality>
</rdf:Description>

<rdf:Description rdf:about="http://cybox.mitre.org/objects/File#PDFFile">
	<rdfs:subClassOf rdf:nodeID="genid64"/>
</rdf:Description>

<rdf:Description rdf:nodeID="genid64">
	<rdf:type rdf:resource="http://www.w3.org/2002/07/owl#Restriction"/>
	<owl:onProperty rdf:resource="http://cybox.mitre.org/objects/File#docInfo.creationDate"/>
	<owl:maxCardinality rdf:datatype="http://www.w3.org/2001/XMLSchema#nonNegativeInteger">1</owl:maxCardinality>
</rdf:Description>

<rdf:Description rdf:about="http://cybox.mitre.org/objects/File#PDFFile">
	<rdfs:subClassOf rdf:nodeID="genid65"/>
</rdf:Description>

<rdf:Description rdf:nodeID="genid65">
	<rdf:type rdf:resource="http://www.w3.org/2002/07/owl#Restriction"/>
	<owl:onProperty rdf:resource="http://cybox.mitre.org/objects/File#docInfo.modificationDate"/>
	<owl:maxCardinality rdf:datatype="http://www.w3.org/2001/XMLSchema#nonNegativeInteger">1</owl:maxCardinality>
</rdf:Description>

<rdf:Description rdf:about="http://cybox.mitre.org/objects/File#PDFFile">
	<rdfs:subClassOf rdf:nodeID="genid66"/>
</rdf:Description>

<rdf:Description rdf:nodeID="genid66">
	<rdf:type rdf:resource="http://www.w3.org/2002/07/owl#Restriction"/>
	<owl:onProperty rdf:resource="http://cybox.mitre.org/objects/File#docInfo.producerAppName"/>
	<owl:maxCardinality rdf:datatype="http://www.w3.org/2001/XMLSchema#nonNegativeInteger">1</owl:maxCardinality>
</rdf:Description>

<rdf:Description rdf:about="http://cybox.mitre.org/objects/File#PDFFile">
	<rdfs:subClassOf rdf:nodeID="genid67"/>
</rdf:Description>

<rdf:Description rdf:nodeID="genid67">
	<rdf:type rdf:resource="http://www.w3.org/2002/07/owl#Restriction"/>
	<owl:onProperty rdf:resource="http://cybox.mitre.org/objects/File#docInfo.subject"/>
	<owl:maxCardinality rdf:datatype="http://www.w3.org/2001/XMLSchema#nonNegativeInteger">1</owl:maxCardinality>
</rdf:Description>

<rdf:Description rdf:about="http://cybox.mitre.org/objects/File#PDFFile">
	<rdfs:subClassOf rdf:nodeID="genid68"/>
</rdf:Description>

<rdf:Description rdf:nodeID="genid68">
	<rdf:type rdf:resource="http://www.w3.org/2002/07/owl#Restriction"/>
	<owl:onProperty rdf:resource="http://cybox.mitre.org/objects/File#docInfo.title"/>
	<owl:maxCardinality rdf:datatype="http://www.w3.org/2001/XMLSchema#nonNegativeInteger">1</owl:maxCardinality>
</rdf:Description>

<rdf:Description rdf:about="http://cybox.mitre.org/objects/File#PDFFile">
	<rdfs:subClassOf rdf:nodeID="genid69"/>
</rdf:Description>

<rdf:Description rdf:nodeID="genid69">
	<rdf:type rdf:resource="http://www.w3.org/2002/07/owl#Restriction"/>
	<owl:onProperty rdf:resource="http://cybox.mitre.org/objects/File#docInfo.trapped"/>
	<owl:maxCardinality rdf:datatype="http://www.w3.org/2001/XMLSchema#nonNegativeInteger">1</owl:maxCardinality>
</rdf:Description>

<rdf:Description rdf:about="http://cybox.mitre.org/objects/File#PDFFile">
	<rdfs:subClassOf rdf:nodeID="genid70"/>
</rdf:Description>

<rdf:Description rdf:nodeID="genid70">
	<rdf:type rdf:resource="http://www.w3.org/2002/07/owl#Restriction"/>
	<owl:onProperty rdf:resource="http://cybox.mitre.org/objects/File#encryptCount.nonObfuscated"/>
	<owl:maxCardinality rdf:datatype="http://www.w3.org/2001/XMLSchema#nonNegativeInteger">1</owl:maxCardinality>
</rdf:Description>

<rdf:Description rdf:about="http://cybox.mitre.org/objects/File#PDFFile">
	<rdfs:subClassOf rdf:nodeID="genid71"/>
</rdf:Description>

<rdf:Description rdf:nodeID="genid71">
	<rdf:type rdf:resource="http://www.w3.org/2002/07/owl#Restriction"/>
	<owl:onProperty rdf:resource="http://cybox.mitre.org/objects/File#encryptCount.obfuscated"/>
	<owl:maxCardinality rdf:datatype="http://www.w3.org/2001/XMLSchema#nonNegativeInteger">1</owl:maxCardinality>
</rdf:Description>

<rdf:Description rdf:about="http://cybox.mitre.org/objects/File#PDFFile">
	<rdfs:subClassOf rdf:nodeID="genid72"/>
</rdf:Description>

<rdf:Description rdf:nodeID="genid72">
	<rdf:type rdf:resource="http://www.w3.org/2002/07/owl#Restriction"/>
	<owl:onProperty rdf:resource="http://cybox.mitre.org/objects/File#javascriptCount.nonObfuscated"/>
	<owl:maxCardinality rdf:datatype="http://www.w3.org/2001/XMLSchema#nonNegativeInteger">1</owl:maxCardinality>
</rdf:Description>

<rdf:Description rdf:about="http://cybox.mitre.org/objects/File#PDFFile">
	<rdfs:subClassOf rdf:nodeID="genid73"/>
</rdf:Description>

<rdf:Description rdf:nodeID="genid73">
	<rdf:type rdf:resource="http://www.w3.org/2002/07/owl#Restriction"/>
	<owl:onProperty rdf:resource="http://cybox.mitre.org/objects/File#javascriptCount.obfuscated"/>
	<owl:maxCardinality rdf:datatype="http://www.w3.org/2001/XMLSchema#nonNegativeInteger">1</owl:maxCardinality>
</rdf:Description>

<rdf:Description rdf:about="http://cybox.mitre.org/objects/File#PDFFile">
	<rdfs:subClassOf rdf:nodeID="genid74"/>
</rdf:Description>

<rdf:Description rdf:nodeID="genid74">
	<rdf:type rdf:resource="http://www.w3.org/2002/07/owl#Restriction"/>
	<owl:onProperty rdf:resource="http://cybox.mitre.org/objects/File#jsCount.nonObfuscated"/>
	<owl:maxCardinality rdf:datatype="http://www.w3.org/2001/XMLSchema#nonNegativeInteger">1</owl:maxCardinality>
</rdf:Description>

<rdf:Description rdf:about="http://cybox.mitre.org/objects/File#PDFFile">
	<rdfs:subClassOf rdf:nodeID="genid75"/>
</rdf:Description>

<rdf:Description rdf:nodeID="genid75">
	<rdf:type rdf:resource="http://www.w3.org/2002/07/owl#Restriction"/>
	<owl:onProperty rdf:resource="http://cybox.mitre.org/objects/File#jsCount.obfuscated"/>
	<owl:maxCardinality rdf:datatype="http://www.w3.org/2001/XMLSchema#nonNegativeInteger">1</owl:maxCardinality>
</rdf:Description>

<rdf:Description rdf:about="http://cybox.mitre.org/objects/File#PDFFile">
	<rdfs:subClassOf rdf:nodeID="genid76"/>
</rdf:Description>

<rdf:Description rdf:nodeID="genid76">
	<rdf:type rdf:resource="http://www.w3.org/2002/07/owl#Restriction"/>
	<owl:onProperty rdf:resource="http://cybox.mitre.org/objects/File#numberOfCrossRefTables"/>
	<owl:maxCardinality rdf:datatype="http://www.w3.org/2001/XMLSchema#nonNegativeInteger">1</owl:maxCardinality>
</rdf:Description>

<rdf:Description rdf:about="http://cybox.mitre.org/objects/File#PDFFile">
	<rdfs:subClassOf rdf:nodeID="genid77"/>
</rdf:Description>

<rdf:Description rdf:nodeID="genid77">
	<rdf:type rdf:resource="http://www.w3.org/2002/07/owl#Restriction"/>
	<owl:onProperty rdf:resource="http://cybox.mitre.org/objects/File#numberOfIndirectObjects"/>
	<owl:maxCardinality rdf:datatype="http://www.w3.org/2001/XMLSchema#nonNegativeInteger">1</owl:maxCardinality>
</rdf:Description>

<rdf:Description rdf:about="http://cybox.mitre.org/objects/File#PDFFile">
	<rdfs:subClassOf rdf:nodeID="genid78"/>
</rdf:Description>

<rdf:Description rdf:nodeID="genid78">
	<rdf:type rdf:resource="http://www.w3.org/2002/07/owl#Restriction"/>
	<owl:onProperty rdf:resource="http://cybox.mitre.org/objects/File#numberOfTrailers"/>
	<owl:maxCardinality rdf:datatype="http://www.w3.org/2001/XMLSchema#nonNegativeInteger">1</owl:maxCardinality>
</rdf:Description>

<rdf:Description rdf:about="http://cybox.mitre.org/objects/File#PDFFile">
	<rdfs:subClassOf rdf:nodeID="genid79"/>
</rdf:Description>

<rdf:Description rdf:nodeID="genid79">
	<rdf:type rdf:resource="http://www.w3.org/2002/07/owl#Restriction"/>
	<owl:onProperty rdf:resource="http://cybox.mitre.org/objects/File#objStmCount.nonObfuscated"/>
	<owl:maxCardinality rdf:datatype="http://www.w3.org/2001/XMLSchema#nonNegativeInteger">1</owl:maxCardinality>
</rdf:Description>

<rdf:Description rdf:about="http://cybox.mitre.org/objects/File#PDFFile">
	<rdfs:subClassOf rdf:nodeID="genid80"/>
</rdf:Description>

<rdf:Description rdf:nodeID="genid80">
	<rdf:type rdf:resource="http://www.w3.org/2002/07/owl#Restriction"/>
	<owl:onProperty rdf:resource="http://cybox.mitre.org/objects/File#objStmCount.obfuscated"/>
	<owl:maxCardinality rdf:datatype="http://www.w3.org/2001/XMLSchema#nonNegativeInteger">1</owl:maxCardinality>
</rdf:Description>

<rdf:Description rdf:about="http://cybox.mitre.org/objects/File#PDFFile">
	<rdfs:subClassOf rdf:nodeID="genid81"/>
</rdf:Description>

<rdf:Description rdf:nodeID="genid81">
	<rdf:type rdf:resource="http://www.w3.org/2002/07/owl#Restriction"/>
	<owl:onProperty rdf:resource="http://cybox.mitre.org/objects/File#openActionCount.nonObfuscated"/>
	<owl:maxCardinality rdf:datatype="http://www.w3.org/2001/XMLSchema#nonNegativeInteger">1</owl:maxCardinality>
</rdf:Description>

<rdf:Description rdf:about="http://cybox.mitre.org/objects/File#PDFFile">
	<rdfs:subClassOf rdf:nodeID="genid82"/>
</rdf:Description>

<rdf:Description rdf:nodeID="genid82">
	<rdf:type rdf:resource="http://www.w3.org/2002/07/owl#Restriction"/>
	<owl:onProperty rdf:resource="http://cybox.mitre.org/objects/File#openActionCount.obfuscated"/>
	<owl:maxCardinality rdf:datatype="http://www.w3.org/2001/XMLSchema#nonNegativeInteger">1</owl:maxCardinality>
</rdf:Description>

<rdf:Description rdf:about="http://cybox.mitre.org/objects/File#PDFFile">
	<rdfs:subClassOf rdf:nodeID="genid83"/>
</rdf:Description>

<rdf:Description rdf:nodeID="genid83">
	<rdf:type rdf:resource="http://www.w3.org/2002/07/owl#Restriction"/>
	<owl:onProperty rdf:resource="http://cybox.mitre.org/objects/File#pageCount.nonObfuscated"/>
	<owl:maxCardinality rdf:datatype="http://www.w3.org/2001/XMLSchema#nonNegativeInteger">1</owl:maxCardinality>
</rdf:Description>

<rdf:Description rdf:about="http://cybox.mitre.org/objects/File#PDFFile">
	<rdfs:subClassOf rdf:nodeID="genid84"/>
</rdf:Description>

<rdf:Description rdf:nodeID="genid84">
	<rdf:type rdf:resource="http://www.w3.org/2002/07/owl#Restriction"/>
	<owl:onProperty rdf:resource="http://cybox.mitre.org/objects/File#pageCount.obfuscated"/>
	<owl:maxCardinality rdf:datatype="http://www.w3.org/2001/XMLSchema#nonNegativeInteger">1</owl:maxCardinality>
</rdf:Description>

<rdf:Description rdf:about="http://cybox.mitre.org/objects/File#PDFFile">
	<rdfs:subClassOf rdf:nodeID="genid85"/>
</rdf:Description>

<rdf:Description rdf:nodeID="genid85">
	<rdf:type rdf:resource="http://www.w3.org/2002/07/owl#Restriction"/>
	<owl:onProperty rdf:resource="http://cybox.mitre.org/objects/File#pdfEncypted"/>
	<owl:maxCardinality rdf:datatype="http://www.w3.org/2001/XMLSchema#nonNegativeInteger">1</owl:maxCardinality>
</rdf:Description>

<rdf:Description rdf:about="http://cybox.mitre.org/objects/File#PDFFile">
	<rdfs:subClassOf rdf:nodeID="genid86"/>
</rdf:Description>

<rdf:Description rdf:nodeID="genid86">
	<rdf:type rdf:resource="http://www.w3.org/2002/07/owl#Restriction"/>
	<owl:onProperty rdf:resource="http://cybox.mitre.org/objects/File#pdfOptimized"/>
	<owl:maxCardinality rdf:datatype="http://www.w3.org/2001/XMLSchema#nonNegativeInteger">1</owl:maxCardinality>
</rdf:Description>

<rdf:Description rdf:about="http://cybox.mitre.org/objects/File#PDFFile">
	<rdfs:subClassOf rdf:nodeID="genid87"/>
</rdf:Description>

<rdf:Description rdf:nodeID="genid87">
	<rdf:type rdf:resource="http://www.w3.org/2002/07/owl#Restriction"/>
	<owl:onProperty rdf:resource="http://cybox.mitre.org/objects/File#pdfSpecVersion"/>
	<owl:maxCardinality rdf:datatype="http://www.w3.org/2001/XMLSchema#nonNegativeInteger">1</owl:maxCardinality>
</rdf:Description>

<rdf:Description rdf:about="http://cybox.mitre.org/objects/File#PDFFile">
	<rdfs:comment>Characterize the structural makeup of PDF files.</rdfs:comment>
	<rdfs:isDefinedBy rdf:resource="http://cybox.mitre.org/objects/File"/>
	<rdfs:label>PDF File</rdfs:label>
</rdf:Description>
<!--  -->
<!-- http://cybox.mitre.org/objects/File#PDFIndirectObject -->

<rdf:Description rdf:about="http://cybox.mitre.org/objects/File#PDFIndirectObject">
	<rdf:type rdf:resource="http://www.w3.org/2002/07/owl#Class"/>
	<rdfs:subClassOf rdf:nodeID="genid88"/>
</rdf:Description>

<rdf:Description rdf:nodeID="genid88">
	<rdf:type rdf:resource="http://www.w3.org/2002/07/owl#Restriction"/>
	<owl:onProperty rdf:resource="http://cybox.mitre.org/objects/File#streamContents"/>
	<owl:maxCardinality rdf:datatype="http://www.w3.org/2001/XMLSchema#nonNegativeInteger">1</owl:maxCardinality>
</rdf:Description>

<rdf:Description rdf:about="http://cybox.mitre.org/objects/File#PDFIndirectObject">
	<rdfs:subClassOf rdf:nodeID="genid89"/>
</rdf:Description>

<rdf:Description rdf:nodeID="genid89">
	<rdf:type rdf:resource="http://www.w3.org/2002/07/owl#Restriction"/>
	<owl:onProperty rdf:resource="http://cybox.mitre.org/objects/File#pdfObjectId.generation"/>
	<owl:cardinality rdf:datatype="http://www.w3.org/2001/XMLSchema#nonNegativeInteger">1</owl:cardinality>
</rdf:Description>

<rdf:Description rdf:about="http://cybox.mitre.org/objects/File#PDFIndirectObject">
	<rdfs:subClassOf rdf:nodeID="genid90"/>
</rdf:Description>

<rdf:Description rdf:nodeID="genid90">
	<rdf:type rdf:resource="http://www.w3.org/2002/07/owl#Restriction"/>
	<owl:onProperty rdf:resource="http://cybox.mitre.org/objects/File#pdfObjectId.number"/>
	<owl:cardinality rdf:datatype="http://www.w3.org/2001/XMLSchema#nonNegativeInteger">1</owl:cardinality>
</rdf:Description>

<rdf:Description rdf:about="http://cybox.mitre.org/objects/File#PDFIndirectObject">
	<rdfs:subClassOf rdf:nodeID="genid91"/>
</rdf:Description>

<rdf:Description rdf:nodeID="genid91">
	<rdf:type rdf:resource="http://www.w3.org/2002/07/owl#Restriction"/>
	<owl:onProperty rdf:resource="http://cybox.mitre.org/objects/File#pdfObjectType"/>
	<owl:cardinality rdf:datatype="http://www.w3.org/2001/XMLSchema#nonNegativeInteger">1</owl:cardinality>
</rdf:Description>

<rdf:Description rdf:about="http://cybox.mitre.org/objects/File#PDFIndirectObject">
	<rdfs:subClassOf rdf:nodeID="genid92"/>
</rdf:Description>

<rdf:Description rdf:nodeID="genid92">
	<rdf:type rdf:resource="http://www.w3.org/2002/07/owl#Restriction"/>
	<owl:onProperty rdf:resource="http://cybox.mitre.org/objects/File#indirectObjectOffset"/>
	<owl:maxCardinality rdf:datatype="http://www.w3.org/2001/XMLSchema#nonNegativeInteger">1</owl:maxCardinality>
</rdf:Description>

<rdf:Description rdf:about="http://cybox.mitre.org/objects/File#PDFIndirectObject">
	<rdfs:subClassOf rdf:nodeID="genid93"/>
</rdf:Description>

<rdf:Description rdf:nodeID="genid93">
	<rdf:type rdf:resource="http://www.w3.org/2002/07/owl#Restriction"/>
	<owl:onProperty rdf:resource="http://cybox.mitre.org/objects/File#nonStreamContents"/>
	<owl:maxCardinality rdf:datatype="http://www.w3.org/2001/XMLSchema#nonNegativeInteger">1</owl:maxCardinality>
</rdf:Description>

<rdf:Description rdf:about="http://cybox.mitre.org/objects/File#PDFIndirectObject">
	<rdfs:comment>Characterizes the details of a PDF document indirect object, used in constructing and storing data associated with the PDF document.</rdfs:comment>
	<rdfs:isDefinedBy rdf:resource="http://cybox.mitre.org/objects/File"/>
	<rdfs:label>PDFIndirect object</rdfs:label>
</rdf:Description>
<!--  -->
<!-- http://cybox.mitre.org/objects/File#PDFMetadata -->

<rdf:Description rdf:about="http://cybox.mitre.org/objects/File#PDFMetadata">
	<rdf:type rdf:resource="http://www.w3.org/2002/07/owl#Class"/>
	<rdfs:subClassOf rdf:nodeID="genid94"/>
</rdf:Description>

<rdf:Description rdf:nodeID="genid94">
	<rdf:type rdf:resource="http://www.w3.org/2002/07/owl#Restriction"/>
	<owl:onProperty rdf:resource="http://cybox.mitre.org/objects/File#aaCount.nonObfuscated"/>
	<owl:maxCardinality rdf:datatype="http://www.w3.org/2001/XMLSchema#nonNegativeInteger">1</owl:maxCardinality>
</rdf:Description>

<rdf:Description rdf:about="http://cybox.mitre.org/objects/File#PDFMetadata">
	<rdfs:subClassOf rdf:nodeID="genid95"/>
</rdf:Description>

<rdf:Description rdf:nodeID="genid95">
	<rdf:type rdf:resource="http://www.w3.org/2002/07/owl#Restriction"/>
	<owl:onProperty rdf:resource="http://cybox.mitre.org/objects/File#aaCount.obfuscated"/>
	<owl:maxCardinality rdf:datatype="http://www.w3.org/2001/XMLSchema#nonNegativeInteger">1</owl:maxCardinality>
</rdf:Description>

<rdf:Description rdf:about="http://cybox.mitre.org/objects/File#PDFMetadata">
	<rdfs:subClassOf rdf:nodeID="genid96"/>
</rdf:Description>

<rdf:Description rdf:nodeID="genid96">
	<rdf:type rdf:resource="http://www.w3.org/2002/07/owl#Restriction"/>
	<owl:onProperty rdf:resource="http://cybox.mitre.org/objects/File#ascii85DecodeCount.nonObfuscated"/>
	<owl:maxCardinality rdf:datatype="http://www.w3.org/2001/XMLSchema#nonNegativeInteger">1</owl:maxCardinality>
</rdf:Description>

<rdf:Description rdf:about="http://cybox.mitre.org/objects/File#PDFMetadata">
	<rdfs:subClassOf rdf:nodeID="genid97"/>
</rdf:Description>

<rdf:Description rdf:nodeID="genid97">
	<rdf:type rdf:resource="http://www.w3.org/2002/07/owl#Restriction"/>
	<owl:onProperty rdf:resource="http://cybox.mitre.org/objects/File#ascii85DecodeCount.obfuscated"/>
	<owl:maxCardinality rdf:datatype="http://www.w3.org/2001/XMLSchema#nonNegativeInteger">1</owl:maxCardinality>
</rdf:Description>

<rdf:Description rdf:about="http://cybox.mitre.org/objects/File#PDFMetadata">
	<rdfs:subClassOf rdf:nodeID="genid98"/>
</rdf:Description>

<rdf:Description rdf:nodeID="genid98">
	<rdf:type rdf:resource="http://www.w3.org/2002/07/owl#Restriction"/>
	<owl:onProperty rdf:resource="http://cybox.mitre.org/objects/File#asciiHexDecodeCount.nonObfuscated"/>
	<owl:maxCardinality rdf:datatype="http://www.w3.org/2001/XMLSchema#nonNegativeInteger">1</owl:maxCardinality>
</rdf:Description>

<rdf:Description rdf:about="http://cybox.mitre.org/objects/File#PDFMetadata">
	<rdfs:subClassOf rdf:nodeID="genid99"/>
</rdf:Description>

<rdf:Description rdf:nodeID="genid99">
	<rdf:type rdf:resource="http://www.w3.org/2002/07/owl#Restriction"/>
	<owl:onProperty rdf:resource="http://cybox.mitre.org/objects/File#asciiHexDecodeCount.obfuscated"/>
	<owl:maxCardinality rdf:datatype="http://www.w3.org/2001/XMLSchema#nonNegativeInteger">1</owl:maxCardinality>
</rdf:Description>

<rdf:Description rdf:about="http://cybox.mitre.org/objects/File#PDFMetadata">
	<rdfs:subClassOf rdf:nodeID="genid100"/>
</rdf:Description>

<rdf:Description rdf:nodeID="genid100">
	<rdf:type rdf:resource="http://www.w3.org/2002/07/owl#Restriction"/>
	<owl:onProperty rdf:resource="http://cybox.mitre.org/objects/File#ccittFaxDecodeCount.nonObfuscated"/>
	<owl:maxCardinality rdf:datatype="http://www.w3.org/2001/XMLSchema#nonNegativeInteger">1</owl:maxCardinality>
</rdf:Description>

<rdf:Description rdf:about="http://cybox.mitre.org/objects/File#PDFMetadata">
	<rdfs:subClassOf rdf:nodeID="genid101"/>
</rdf:Description>

<rdf:Description rdf:nodeID="genid101">
	<rdf:type rdf:resource="http://www.w3.org/2002/07/owl#Restriction"/>
	<owl:onProperty rdf:resource="http://cybox.mitre.org/objects/File#ccittFaxDecodeCount.obfuscated"/>
	<owl:maxCardinality rdf:datatype="http://www.w3.org/2001/XMLSchema#nonNegativeInteger">1</owl:maxCardinality>
</rdf:Description>

<rdf:Description rdf:about="http://cybox.mitre.org/objects/File#PDFMetadata">
	<rdfs:subClassOf rdf:nodeID="genid102"/>
</rdf:Description>

<rdf:Description rdf:nodeID="genid102">
	<rdf:type rdf:resource="http://www.w3.org/2002/07/owl#Restriction"/>
	<owl:onProperty rdf:resource="http://cybox.mitre.org/objects/File#dctDecodeCount.nonObfuscated"/>
	<owl:maxCardinality rdf:datatype="http://www.w3.org/2001/XMLSchema#nonNegativeInteger">1</owl:maxCardinality>
</rdf:Description>

<rdf:Description rdf:about="http://cybox.mitre.org/objects/File#PDFMetadata">
	<rdfs:subClassOf rdf:nodeID="genid103"/>
</rdf:Description>

<rdf:Description rdf:nodeID="genid103">
	<rdf:type rdf:resource="http://www.w3.org/2002/07/owl#Restriction"/>
	<owl:onProperty rdf:resource="http://cybox.mitre.org/objects/File#dctDecodeCount.obfuscated"/>
	<owl:maxCardinality rdf:datatype="http://www.w3.org/2001/XMLSchema#nonNegativeInteger">1</owl:maxCardinality>
</rdf:Description>

<rdf:Description rdf:about="http://cybox.mitre.org/objects/File#PDFMetadata">
	<rdfs:subClassOf rdf:nodeID="genid104"/>
</rdf:Description>

<rdf:Description rdf:nodeID="genid104">
	<rdf:type rdf:resource="http://www.w3.org/2002/07/owl#Restriction"/>
	<owl:onProperty rdf:resource="http://cybox.mitre.org/objects/File#docInfo.authorName"/>
	<owl:maxCardinality rdf:datatype="http://www.w3.org/2001/XMLSchema#nonNegativeInteger">1</owl:maxCardinality>
</rdf:Description>

<rdf:Description rdf:about="http://cybox.mitre.org/objects/File#PDFMetadata">
	<rdfs:subClassOf rdf:nodeID="genid105"/>
</rdf:Description>

<rdf:Description rdf:nodeID="genid105">
	<rdf:type rdf:resource="http://www.w3.org/2002/07/owl#Restriction"/>
	<owl:onProperty rdf:resource="http://cybox.mitre.org/objects/File#docInfo.creationDate"/>
	<owl:maxCardinality rdf:datatype="http://www.w3.org/2001/XMLSchema#nonNegativeInteger">1</owl:maxCardinality>
</rdf:Description>

<rdf:Description rdf:about="http://cybox.mitre.org/objects/File#PDFMetadata">
	<rdfs:subClassOf rdf:nodeID="genid106"/>
</rdf:Description>

<rdf:Description rdf:nodeID="genid106">
	<rdf:type rdf:resource="http://www.w3.org/2002/07/owl#Restriction"/>
	<owl:onProperty rdf:resource="http://cybox.mitre.org/objects/File#docInfo.creatorAppName"/>
	<owl:maxCardinality rdf:datatype="http://www.w3.org/2001/XMLSchema#nonNegativeInteger">1</owl:maxCardinality>
</rdf:Description>

<rdf:Description rdf:about="http://cybox.mitre.org/objects/File#PDFMetadata">
	<rdfs:subClassOf rdf:nodeID="genid107"/>
</rdf:Description>

<rdf:Description rdf:nodeID="genid107">
	<rdf:type rdf:resource="http://www.w3.org/2002/07/owl#Restriction"/>
	<owl:onProperty rdf:resource="http://cybox.mitre.org/objects/File#docInfo.modificationDate"/>
	<owl:maxCardinality rdf:datatype="http://www.w3.org/2001/XMLSchema#nonNegativeInteger">1</owl:maxCardinality>
</rdf:Description>

<rdf:Description rdf:about="http://cybox.mitre.org/objects/File#PDFMetadata">
	<rdfs:subClassOf rdf:nodeID="genid108"/>
</rdf:Description>

<rdf:Description rdf:nodeID="genid108">
	<rdf:type rdf:resource="http://www.w3.org/2002/07/owl#Restriction"/>
	<owl:onProperty rdf:resource="http://cybox.mitre.org/objects/File#docInfo.producerAppName"/>
	<owl:maxCardinality rdf:datatype="http://www.w3.org/2001/XMLSchema#nonNegativeInteger">1</owl:maxCardinality>
</rdf:Description>

<rdf:Description rdf:about="http://cybox.mitre.org/objects/File#PDFMetadata">
	<rdfs:subClassOf rdf:nodeID="genid109"/>
</rdf:Description>

<rdf:Description rdf:nodeID="genid109">
	<rdf:type rdf:resource="http://www.w3.org/2002/07/owl#Restriction"/>
	<owl:onProperty rdf:resource="http://cybox.mitre.org/objects/File#docInfo.subject"/>
	<owl:maxCardinality rdf:datatype="http://www.w3.org/2001/XMLSchema#nonNegativeInteger">1</owl:maxCardinality>
</rdf:Description>

<rdf:Description rdf:about="http://cybox.mitre.org/objects/File#PDFMetadata">
	<rdfs:subClassOf rdf:nodeID="genid110"/>
</rdf:Description>

<rdf:Description rdf:nodeID="genid110">
	<rdf:type rdf:resource="http://www.w3.org/2002/07/owl#Restriction"/>
	<owl:onProperty rdf:resource="http://cybox.mitre.org/objects/File#docInfo.title"/>
	<owl:maxCardinality rdf:datatype="http://www.w3.org/2001/XMLSchema#nonNegativeInteger">1</owl:maxCardinality>
</rdf:Description>

<rdf:Description rdf:about="http://cybox.mitre.org/objects/File#PDFMetadata">
	<rdfs:subClassOf rdf:nodeID="genid111"/>
</rdf:Description>

<rdf:Description rdf:nodeID="genid111">
	<rdf:type rdf:resource="http://www.w3.org/2002/07/owl#Restriction"/>
	<owl:onProperty rdf:resource="http://cybox.mitre.org/objects/File#docInfo.trapped"/>
	<owl:maxCardinality rdf:datatype="http://www.w3.org/2001/XMLSchema#nonNegativeInteger">1</owl:maxCardinality>
</rdf:Description>

<rdf:Description rdf:about="http://cybox.mitre.org/objects/File#PDFMetadata">
	<rdfs:subClassOf rdf:nodeID="genid112"/>
</rdf:Description>

<rdf:Description rdf:nodeID="genid112">
	<rdf:type rdf:resource="http://www.w3.org/2002/07/owl#Restriction"/>
	<owl:onProperty rdf:resource="http://cybox.mitre.org/objects/File#encryptCount.nonObfuscated"/>
	<owl:maxCardinality rdf:datatype="http://www.w3.org/2001/XMLSchema#nonNegativeInteger">1</owl:maxCardinality>
</rdf:Description>

<rdf:Description rdf:about="http://cybox.mitre.org/objects/File#PDFMetadata">
	<rdfs:subClassOf rdf:nodeID="genid113"/>
</rdf:Description>

<rdf:Description rdf:nodeID="genid113">
	<rdf:type rdf:resource="http://www.w3.org/2002/07/owl#Restriction"/>
	<owl:onProperty rdf:resource="http://cybox.mitre.org/objects/File#encryptCount.obfuscated"/>
	<owl:maxCardinality rdf:datatype="http://www.w3.org/2001/XMLSchema#nonNegativeInteger">1</owl:maxCardinality>
</rdf:Description>

<rdf:Description rdf:about="http://cybox.mitre.org/objects/File#PDFMetadata">
	<rdfs:subClassOf rdf:nodeID="genid114"/>
</rdf:Description>

<rdf:Description rdf:nodeID="genid114">
	<rdf:type rdf:resource="http://www.w3.org/2002/07/owl#Restriction"/>
	<owl:onProperty rdf:resource="http://cybox.mitre.org/objects/File#flateDecodeCount.nonObfuscated"/>
	<owl:maxCardinality rdf:datatype="http://www.w3.org/2001/XMLSchema#nonNegativeInteger">1</owl:maxCardinality>
</rdf:Description>

<rdf:Description rdf:about="http://cybox.mitre.org/objects/File#PDFMetadata">
	<rdfs:subClassOf rdf:nodeID="genid115"/>
</rdf:Description>

<rdf:Description rdf:nodeID="genid115">
	<rdf:type rdf:resource="http://www.w3.org/2002/07/owl#Restriction"/>
	<owl:onProperty rdf:resource="http://cybox.mitre.org/objects/File#flateDecodeCount.obfuscated"/>
	<owl:maxCardinality rdf:datatype="http://www.w3.org/2001/XMLSchema#nonNegativeInteger">1</owl:maxCardinality>
</rdf:Description>

<rdf:Description rdf:about="http://cybox.mitre.org/objects/File#PDFMetadata">
	<rdfs:subClassOf rdf:nodeID="genid116"/>
</rdf:Description>

<rdf:Description rdf:nodeID="genid116">
	<rdf:type rdf:resource="http://www.w3.org/2002/07/owl#Restriction"/>
	<owl:onProperty rdf:resource="http://cybox.mitre.org/objects/File#javascriptCount.nonObfuscated"/>
	<owl:maxCardinality rdf:datatype="http://www.w3.org/2001/XMLSchema#nonNegativeInteger">1</owl:maxCardinality>
</rdf:Description>

<rdf:Description rdf:about="http://cybox.mitre.org/objects/File#PDFMetadata">
	<rdfs:subClassOf rdf:nodeID="genid117"/>
</rdf:Description>

<rdf:Description rdf:nodeID="genid117">
	<rdf:type rdf:resource="http://www.w3.org/2002/07/owl#Restriction"/>
	<owl:onProperty rdf:resource="http://cybox.mitre.org/objects/File#javascriptCount.obfuscated"/>
	<owl:maxCardinality rdf:datatype="http://www.w3.org/2001/XMLSchema#nonNegativeInteger">1</owl:maxCardinality>
</rdf:Description>

<rdf:Description rdf:about="http://cybox.mitre.org/objects/File#PDFMetadata">
	<rdfs:subClassOf rdf:nodeID="genid118"/>
</rdf:Description>

<rdf:Description rdf:nodeID="genid118">
	<rdf:type rdf:resource="http://www.w3.org/2002/07/owl#Restriction"/>
	<owl:onProperty rdf:resource="http://cybox.mitre.org/objects/File#jbig2DecodeCount.nonObfuscated"/>
	<owl:maxCardinality rdf:datatype="http://www.w3.org/2001/XMLSchema#nonNegativeInteger">1</owl:maxCardinality>
</rdf:Description>

<rdf:Description rdf:about="http://cybox.mitre.org/objects/File#PDFMetadata">
	<rdfs:subClassOf rdf:nodeID="genid119"/>
</rdf:Description>

<rdf:Description rdf:nodeID="genid119">
	<rdf:type rdf:resource="http://www.w3.org/2002/07/owl#Restriction"/>
	<owl:onProperty rdf:resource="http://cybox.mitre.org/objects/File#jbig2DecodeCount.obfuscated"/>
	<owl:maxCardinality rdf:datatype="http://www.w3.org/2001/XMLSchema#nonNegativeInteger">1</owl:maxCardinality>
</rdf:Description>

<rdf:Description rdf:about="http://cybox.mitre.org/objects/File#PDFMetadata">
	<rdfs:subClassOf rdf:nodeID="genid120"/>
</rdf:Description>

<rdf:Description rdf:nodeID="genid120">
	<rdf:type rdf:resource="http://www.w3.org/2002/07/owl#Restriction"/>
	<owl:onProperty rdf:resource="http://cybox.mitre.org/objects/File#jsCount.nonObfuscated"/>
	<owl:maxCardinality rdf:datatype="http://www.w3.org/2001/XMLSchema#nonNegativeInteger">1</owl:maxCardinality>
</rdf:Description>

<rdf:Description rdf:about="http://cybox.mitre.org/objects/File#PDFMetadata">
	<rdfs:subClassOf rdf:nodeID="genid121"/>
</rdf:Description>

<rdf:Description rdf:nodeID="genid121">
	<rdf:type rdf:resource="http://www.w3.org/2002/07/owl#Restriction"/>
	<owl:onProperty rdf:resource="http://cybox.mitre.org/objects/File#jsCount.obfuscated"/>
	<owl:maxCardinality rdf:datatype="http://www.w3.org/2001/XMLSchema#nonNegativeInteger">1</owl:maxCardinality>
</rdf:Description>

<rdf:Description rdf:about="http://cybox.mitre.org/objects/File#PDFMetadata">
	<rdfs:subClassOf rdf:nodeID="genid122"/>
</rdf:Description>

<rdf:Description rdf:nodeID="genid122">
	<rdf:type rdf:resource="http://www.w3.org/2002/07/owl#Restriction"/>
	<owl:onProperty rdf:resource="http://cybox.mitre.org/objects/File#launchCount.nonObfuscated"/>
	<owl:maxCardinality rdf:datatype="http://www.w3.org/2001/XMLSchema#nonNegativeInteger">1</owl:maxCardinality>
</rdf:Description>

<rdf:Description rdf:about="http://cybox.mitre.org/objects/File#PDFMetadata">
	<rdfs:subClassOf rdf:nodeID="genid123"/>
</rdf:Description>

<rdf:Description rdf:nodeID="genid123">
	<rdf:type rdf:resource="http://www.w3.org/2002/07/owl#Restriction"/>
	<owl:onProperty rdf:resource="http://cybox.mitre.org/objects/File#launchCount.obfuscated"/>
	<owl:maxCardinality rdf:datatype="http://www.w3.org/2001/XMLSchema#nonNegativeInteger">1</owl:maxCardinality>
</rdf:Description>

<rdf:Description rdf:about="http://cybox.mitre.org/objects/File#PDFMetadata">
	<rdfs:subClassOf rdf:nodeID="genid124"/>
</rdf:Description>

<rdf:Description rdf:nodeID="genid124">
	<rdf:type rdf:resource="http://www.w3.org/2002/07/owl#Restriction"/>
	<owl:onProperty rdf:resource="http://cybox.mitre.org/objects/File#lzwDecodeCount.nonObfuscated"/>
	<owl:maxCardinality rdf:datatype="http://www.w3.org/2001/XMLSchema#nonNegativeInteger">1</owl:maxCardinality>
</rdf:Description>

<rdf:Description rdf:about="http://cybox.mitre.org/objects/File#PDFMetadata">
	<rdfs:subClassOf rdf:nodeID="genid125"/>
</rdf:Description>

<rdf:Description rdf:nodeID="genid125">
	<rdf:type rdf:resource="http://www.w3.org/2002/07/owl#Restriction"/>
	<owl:onProperty rdf:resource="http://cybox.mitre.org/objects/File#lzwDecodeCount.obfuscated"/>
	<owl:maxCardinality rdf:datatype="http://www.w3.org/2001/XMLSchema#nonNegativeInteger">1</owl:maxCardinality>
</rdf:Description>

<rdf:Description rdf:about="http://cybox.mitre.org/objects/File#PDFMetadata">
	<rdfs:subClassOf rdf:nodeID="genid126"/>
</rdf:Description>

<rdf:Description rdf:nodeID="genid126">
	<rdf:type rdf:resource="http://www.w3.org/2002/07/owl#Restriction"/>
	<owl:onProperty rdf:resource="http://cybox.mitre.org/objects/File#numberOfCrossRefTables"/>
	<owl:maxCardinality rdf:datatype="http://www.w3.org/2001/XMLSchema#nonNegativeInteger">1</owl:maxCardinality>
</rdf:Description>

<rdf:Description rdf:about="http://cybox.mitre.org/objects/File#PDFMetadata">
	<rdfs:subClassOf rdf:nodeID="genid127"/>
</rdf:Description>

<rdf:Description rdf:nodeID="genid127">
	<rdf:type rdf:resource="http://www.w3.org/2002/07/owl#Restriction"/>
	<owl:onProperty rdf:resource="http://cybox.mitre.org/objects/File#numberOfIndirectObjects"/>
	<owl:maxCardinality rdf:datatype="http://www.w3.org/2001/XMLSchema#nonNegativeInteger">1</owl:maxCardinality>
</rdf:Description>

<rdf:Description rdf:about="http://cybox.mitre.org/objects/File#PDFMetadata">
	<rdfs:subClassOf rdf:nodeID="genid128"/>
</rdf:Description>

<rdf:Description rdf:nodeID="genid128">
	<rdf:type rdf:resource="http://www.w3.org/2002/07/owl#Restriction"/>
	<owl:onProperty rdf:resource="http://cybox.mitre.org/objects/File#numberOfTrailers"/>
	<owl:maxCardinality rdf:datatype="http://www.w3.org/2001/XMLSchema#nonNegativeInteger">1</owl:maxCardinality>
</rdf:Description>

<rdf:Description rdf:about="http://cybox.mitre.org/objects/File#PDFMetadata">
	<rdfs:subClassOf rdf:nodeID="genid129"/>
</rdf:Description>

<rdf:Description rdf:nodeID="genid129">
	<rdf:type rdf:resource="http://www.w3.org/2002/07/owl#Restriction"/>
	<owl:onProperty rdf:resource="http://cybox.mitre.org/objects/File#objStmCount.nonObfuscated"/>
	<owl:maxCardinality rdf:datatype="http://www.w3.org/2001/XMLSchema#nonNegativeInteger">11</owl:maxCardinality>
</rdf:Description>

<rdf:Description rdf:about="http://cybox.mitre.org/objects/File#PDFMetadata">
	<rdfs:subClassOf rdf:nodeID="genid130"/>
</rdf:Description>

<rdf:Description rdf:nodeID="genid130">
	<rdf:type rdf:resource="http://www.w3.org/2002/07/owl#Restriction"/>
	<owl:onProperty rdf:resource="http://cybox.mitre.org/objects/File#objStmCount.obfuscated"/>
	<owl:maxCardinality rdf:datatype="http://www.w3.org/2001/XMLSchema#nonNegativeInteger">1</owl:maxCardinality>
</rdf:Description>

<rdf:Description rdf:about="http://cybox.mitre.org/objects/File#PDFMetadata">
	<rdfs:subClassOf rdf:nodeID="genid131"/>
</rdf:Description>

<rdf:Description rdf:nodeID="genid131">
	<rdf:type rdf:resource="http://www.w3.org/2002/07/owl#Restriction"/>
	<owl:onProperty rdf:resource="http://cybox.mitre.org/objects/File#openActionCount.nonObfuscated"/>
	<owl:maxCardinality rdf:datatype="http://www.w3.org/2001/XMLSchema#nonNegativeInteger">1</owl:maxCardinality>
</rdf:Description>

<rdf:Description rdf:about="http://cybox.mitre.org/objects/File#PDFMetadata">
	<rdfs:subClassOf rdf:nodeID="genid132"/>
</rdf:Description>

<rdf:Description rdf:nodeID="genid132">
	<rdf:type rdf:resource="http://www.w3.org/2002/07/owl#Restriction"/>
	<owl:onProperty rdf:resource="http://cybox.mitre.org/objects/File#openActionCount.obfuscated"/>
	<owl:maxCardinality rdf:datatype="http://www.w3.org/2001/XMLSchema#nonNegativeInteger">1</owl:maxCardinality>
</rdf:Description>

<rdf:Description rdf:about="http://cybox.mitre.org/objects/File#PDFMetadata">
	<rdfs:subClassOf rdf:nodeID="genid133"/>
</rdf:Description>

<rdf:Description rdf:nodeID="genid133">
	<rdf:type rdf:resource="http://www.w3.org/2002/07/owl#Restriction"/>
	<owl:onProperty rdf:resource="http://cybox.mitre.org/objects/File#pageCount.nonObfuscated"/>
	<owl:maxCardinality rdf:datatype="http://www.w3.org/2001/XMLSchema#nonNegativeInteger">1</owl:maxCardinality>
</rdf:Description>

<rdf:Description rdf:about="http://cybox.mitre.org/objects/File#PDFMetadata">
	<rdfs:subClassOf rdf:nodeID="genid134"/>
</rdf:Description>

<rdf:Description rdf:nodeID="genid134">
	<rdf:type rdf:resource="http://www.w3.org/2002/07/owl#Restriction"/>
	<owl:onProperty rdf:resource="http://cybox.mitre.org/objects/File#pageCount.obfuscated"/>
	<owl:maxCardinality rdf:datatype="http://www.w3.org/2001/XMLSchema#nonNegativeInteger">1</owl:maxCardinality>
</rdf:Description>

<rdf:Description rdf:about="http://cybox.mitre.org/objects/File#PDFMetadata">
	<rdfs:subClassOf rdf:nodeID="genid135"/>
</rdf:Description>

<rdf:Description rdf:nodeID="genid135">
	<rdf:type rdf:resource="http://www.w3.org/2002/07/owl#Restriction"/>
	<owl:onProperty rdf:resource="http://cybox.mitre.org/objects/File#pdfEncypted"/>
	<owl:maxCardinality rdf:datatype="http://www.w3.org/2001/XMLSchema#nonNegativeInteger">1</owl:maxCardinality>
</rdf:Description>

<rdf:Description rdf:about="http://cybox.mitre.org/objects/File#PDFMetadata">
	<rdfs:subClassOf rdf:nodeID="genid136"/>
</rdf:Description>

<rdf:Description rdf:nodeID="genid136">
	<rdf:type rdf:resource="http://www.w3.org/2002/07/owl#Restriction"/>
	<owl:onProperty rdf:resource="http://cybox.mitre.org/objects/File#pdfOptimized"/>
	<owl:maxCardinality rdf:datatype="http://www.w3.org/2001/XMLSchema#nonNegativeInteger">1</owl:maxCardinality>
</rdf:Description>

<rdf:Description rdf:about="http://cybox.mitre.org/objects/File#PDFMetadata">
	<rdfs:subClassOf rdf:nodeID="genid137"/>
</rdf:Description>

<rdf:Description rdf:nodeID="genid137">
	<rdf:type rdf:resource="http://www.w3.org/2002/07/owl#Restriction"/>
	<owl:onProperty rdf:resource="http://cybox.mitre.org/objects/File#richMediaCount.nonObfuscated"/>
	<owl:maxCardinality rdf:datatype="http://www.w3.org/2001/XMLSchema#nonNegativeInteger">1</owl:maxCardinality>
</rdf:Description>

<rdf:Description rdf:about="http://cybox.mitre.org/objects/File#PDFMetadata">
	<rdfs:subClassOf rdf:nodeID="genid138"/>
</rdf:Description>

<rdf:Description rdf:nodeID="genid138">
	<rdf:type rdf:resource="http://www.w3.org/2002/07/owl#Restriction"/>
	<owl:onProperty rdf:resource="http://cybox.mitre.org/objects/File#richMediaCount.obfuscated"/>
	<owl:maxCardinality rdf:datatype="http://www.w3.org/2001/XMLSchema#nonNegativeInteger">1</owl:maxCardinality>
</rdf:Description>

<rdf:Description rdf:about="http://cybox.mitre.org/objects/File#PDFMetadata">
	<rdfs:subClassOf rdf:nodeID="genid139"/>
</rdf:Description>

<rdf:Description rdf:nodeID="genid139">
	<rdf:type rdf:resource="http://www.w3.org/2002/07/owl#Restriction"/>
	<owl:onProperty rdf:resource="http://cybox.mitre.org/objects/File#runLengthDecodeCount.nonObfuscated"/>
	<owl:maxCardinality rdf:datatype="http://www.w3.org/2001/XMLSchema#nonNegativeInteger">1</owl:maxCardinality>
</rdf:Description>

<rdf:Description rdf:about="http://cybox.mitre.org/objects/File#PDFMetadata">
	<rdfs:subClassOf rdf:nodeID="genid140"/>
</rdf:Description>

<rdf:Description rdf:nodeID="genid140">
	<rdf:type rdf:resource="http://www.w3.org/2002/07/owl#Restriction"/>
	<owl:onProperty rdf:resource="http://cybox.mitre.org/objects/File#runLengthDecodeCount.obfuscated"/>
	<owl:maxCardinality rdf:datatype="http://www.w3.org/2001/XMLSchema#nonNegativeInteger">1</owl:maxCardinality>
</rdf:Description>

<rdf:Description rdf:about="http://cybox.mitre.org/objects/File#PDFMetadata">
	<rdfs:subClassOf rdf:nodeID="genid141"/>
</rdf:Description>

<rdf:Description rdf:nodeID="genid141">
	<rdf:type rdf:resource="http://www.w3.org/2002/07/owl#Restriction"/>
	<owl:onProperty rdf:resource="http://cybox.mitre.org/objects/File#xfaCount.nonObfuscated"/>
	<owl:maxCardinality rdf:datatype="http://www.w3.org/2001/XMLSchema#nonNegativeInteger">1</owl:maxCardinality>
</rdf:Description>

<rdf:Description rdf:about="http://cybox.mitre.org/objects/File#PDFMetadata">
	<rdfs:subClassOf rdf:nodeID="genid142"/>
</rdf:Description>

<rdf:Description rdf:nodeID="genid142">
	<rdf:type rdf:resource="http://www.w3.org/2002/07/owl#Restriction"/>
	<owl:onProperty rdf:resource="http://cybox.mitre.org/objects/File#xfaCount.obfuscated"/>
	<owl:maxCardinality rdf:datatype="http://www.w3.org/2001/XMLSchema#nonNegativeInteger">1</owl:maxCardinality>
</rdf:Description>

<rdf:Description rdf:about="http://cybox.mitre.org/objects/File#PDFMetadata">
	<rdfs:comment>Characterizes metadata regarding the PDF file object.</rdfs:comment>
	<rdfs:isDefinedBy rdf:resource="http://cybox.mitre.org/objects/File"/>
	<rdfs:label>PDF Metadata</rdfs:label>
</rdf:Description>
<!--  -->
<!-- http://cybox.mitre.org/objects/File#PDFStream -->

<rdf:Description rdf:about="http://cybox.mitre.org/objects/File#PDFStream">
	<rdf:type rdf:resource="http://www.w3.org/2002/07/owl#Class"/>
	<rdfs:subClassOf rdf:nodeID="genid143"/>
</rdf:Description>

<rdf:Description rdf:nodeID="genid143">
	<rdf:type rdf:resource="http://www.w3.org/2002/07/owl#Restriction"/>
	<owl:onProperty rdf:resource="http://cybox.mitre.org/objects/File#decodedStream"/>
	<owl:maxCardinality rdf:datatype="http://www.w3.org/2001/XMLSchema#nonNegativeInteger">1</owl:maxCardinality>
</rdf:Description>

<rdf:Description rdf:about="http://cybox.mitre.org/objects/File#PDFStream">
	<rdfs:subClassOf rdf:nodeID="genid144"/>
</rdf:Description>

<rdf:Description rdf:nodeID="genid144">
	<rdf:type rdf:resource="http://www.w3.org/2002/07/owl#Restriction"/>
	<owl:onProperty rdf:resource="http://cybox.mitre.org/objects/File#rawStream"/>
	<owl:maxCardinality rdf:datatype="http://www.w3.org/2001/XMLSchema#nonNegativeInteger">1</owl:maxCardinality>
</rdf:Description>

<rdf:Description rdf:about="http://cybox.mitre.org/objects/File#PDFStream">
	<rdfs:comment>Characterizes details of PDF document stream objects, which represent arbitrary sequences of bytes.</rdfs:comment>
	<rdfs:isDefinedBy rdf:resource="http://cybox.mitre.org/objects/File"/>
	<rdfs:label>PDFStream</rdfs:label>
</rdf:Description>
<!--  -->
<!-- http://cybox.mitre.org/objects/File#PDFTrailer -->

<rdf:Description rdf:about="http://cybox.mitre.org/objects/File#PDFTrailer">
	<rdf:type rdf:resource="http://www.w3.org/2002/07/owl#Class"/>
	<rdfs:subClassOf rdf:nodeID="genid145"/>
</rdf:Description>

<rdf:Description rdf:nodeID="genid145">
	<rdf:type rdf:resource="http://www.w3.org/2002/07/owl#Restriction"/>
	<owl:onProperty rdf:resource="http://cybox.mitre.org/objects/File#encrypt.objectRef"/>
	<owl:maxCardinality rdf:datatype="http://www.w3.org/2001/XMLSchema#nonNegativeInteger">1</owl:maxCardinality>
</rdf:Description>

<rdf:Description rdf:about="http://cybox.mitre.org/objects/File#PDFTrailer">
	<rdfs:subClassOf rdf:nodeID="genid146"/>
</rdf:Description>

<rdf:Description rdf:nodeID="genid146">
	<rdf:type rdf:resource="http://www.w3.org/2002/07/owl#Restriction"/>
	<owl:onProperty rdf:resource="http://cybox.mitre.org/objects/File#info"/>
	<owl:maxCardinality rdf:datatype="http://www.w3.org/2001/XMLSchema#nonNegativeInteger">1</owl:maxCardinality>
</rdf:Description>

<rdf:Description rdf:about="http://cybox.mitre.org/objects/File#PDFTrailer">
	<rdfs:subClassOf rdf:nodeID="genid147"/>
</rdf:Description>

<rdf:Description rdf:nodeID="genid147">
	<rdf:type rdf:resource="http://www.w3.org/2002/07/owl#Restriction"/>
	<owl:onProperty rdf:resource="http://cybox.mitre.org/objects/File#root"/>
	<owl:maxCardinality rdf:datatype="http://www.w3.org/2001/XMLSchema#nonNegativeInteger">1</owl:maxCardinality>
</rdf:Description>

<rdf:Description rdf:about="http://cybox.mitre.org/objects/File#PDFTrailer">
	<rdfs:subClassOf rdf:nodeID="genid148"/>
</rdf:Description>

<rdf:Description rdf:nodeID="genid148">
	<rdf:type rdf:resource="http://www.w3.org/2002/07/owl#Restriction"/>
	<owl:onProperty rdf:resource="http://cybox.mitre.org/objects/File#ID"/>
	<owl:minCardinality rdf:datatype="http://www.w3.org/2001/XMLSchema#nonNegativeInteger">0</owl:minCardinality>
</rdf:Description>

<rdf:Description rdf:about="http://cybox.mitre.org/objects/File#PDFTrailer">
	<rdfs:subClassOf rdf:nodeID="genid149"/>
</rdf:Description>

<rdf:Description rdf:nodeID="genid149">
	<rdf:type rdf:resource="http://www.w3.org/2002/07/owl#Restriction"/>
	<owl:onProperty rdf:resource="http://cybox.mitre.org/objects/File#ID"/>
	<owl:maxCardinality rdf:datatype="http://www.w3.org/2001/XMLSchema#nonNegativeInteger">2</owl:maxCardinality>
</rdf:Description>

<rdf:Description rdf:about="http://cybox.mitre.org/objects/File#PDFTrailer">
	<rdfs:subClassOf rdf:nodeID="genid150"/>
</rdf:Description>

<rdf:Description rdf:nodeID="genid150">
	<rdf:type rdf:resource="http://www.w3.org/2002/07/owl#Restriction"/>
	<owl:onProperty rdf:resource="http://cybox.mitre.org/objects/File#encrypt.rawContents"/>
	<owl:maxCardinality rdf:datatype="http://www.w3.org/2001/XMLSchema#nonNegativeInteger">1</owl:maxCardinality>
</rdf:Description>

<rdf:Description rdf:about="http://cybox.mitre.org/objects/File#PDFTrailer">
	<rdfs:subClassOf rdf:nodeID="genid151"/>
</rdf:Description>

<rdf:Description rdf:nodeID="genid151">
	<rdf:type rdf:resource="http://www.w3.org/2002/07/owl#Restriction"/>
	<owl:onProperty rdf:resource="http://cybox.mitre.org/objects/File#lastCrossRefOffset"/>
	<owl:maxCardinality rdf:datatype="http://www.w3.org/2001/XMLSchema#nonNegativeInteger">1</owl:maxCardinality>
</rdf:Description>

<rdf:Description rdf:about="http://cybox.mitre.org/objects/File#PDFTrailer">
	<rdfs:subClassOf rdf:nodeID="genid152"/>
</rdf:Description>

<rdf:Description rdf:nodeID="genid152">
	<rdf:type rdf:resource="http://www.w3.org/2002/07/owl#Restriction"/>
	<owl:onProperty rdf:resource="http://cybox.mitre.org/objects/File#offset"/>
	<owl:maxCardinality rdf:datatype="http://www.w3.org/2001/XMLSchema#nonNegativeInteger">1</owl:maxCardinality>
</rdf:Description>

<rdf:Description rdf:about="http://cybox.mitre.org/objects/File#PDFTrailer">
	<rdfs:subClassOf rdf:nodeID="genid153"/>
</rdf:Description>

<rdf:Description rdf:nodeID="genid153">
	<rdf:type rdf:resource="http://www.w3.org/2002/07/owl#Restriction"/>
	<owl:onProperty rdf:resource="http://cybox.mitre.org/objects/File#prev"/>
	<owl:maxCardinality rdf:datatype="http://www.w3.org/2001/XMLSchema#nonNegativeInteger">1</owl:maxCardinality>
</rdf:Description>

<rdf:Description rdf:about="http://cybox.mitre.org/objects/File#PDFTrailer">
	<rdfs:subClassOf rdf:nodeID="genid154"/>
</rdf:Description>

<rdf:Description rdf:nodeID="genid154">
	<rdf:type rdf:resource="http://www.w3.org/2002/07/owl#Restriction"/>
	<owl:onProperty rdf:resource="http://cybox.mitre.org/objects/File#size"/>
	<owl:maxCardinality rdf:datatype="http://www.w3.org/2001/XMLSchema#nonNegativeInteger">1</owl:maxCardinality>
</rdf:Description>

<rdf:Description rdf:about="http://cybox.mitre.org/objects/File#PDFTrailer">
	<rdfs:comment>Characterizes the details of a PDF trailer.</rdfs:comment>
	<rdfs:isDefinedBy rdf:resource="http://cybox.mitre.org/objects/File"/>
	<rdfs:label>PDFTrailer</rdfs:label>
</rdf:Description>
<!--  -->
<!-- http://cybox.mitre.org/objects/File#PDFXrefEntry -->

<rdf:Description rdf:about="http://cybox.mitre.org/objects/File#PDFXrefEntry">
	<rdf:type rdf:resource="http://www.w3.org/2002/07/owl#Class"/>
	<rdfs:subClassOf rdf:nodeID="genid155"/>
</rdf:Description>

<rdf:Description rdf:nodeID="genid155">
	<rdf:type rdf:resource="http://www.w3.org/2002/07/owl#Restriction"/>
	<owl:onProperty rdf:resource="http://cybox.mitre.org/objects/File#xrefEntryType"/>
	<owl:cardinality rdf:datatype="http://www.w3.org/2001/XMLSchema#nonNegativeInteger">1</owl:cardinality>
</rdf:Description>

<rdf:Description rdf:about="http://cybox.mitre.org/objects/File#PDFXrefEntry">
	<rdfs:subClassOf rdf:nodeID="genid156"/>
</rdf:Description>

<rdf:Description rdf:nodeID="genid156">
	<rdf:type rdf:resource="http://www.w3.org/2002/07/owl#Restriction"/>
	<owl:onProperty rdf:resource="http://cybox.mitre.org/objects/File#byteOffset"/>
	<owl:maxCardinality rdf:datatype="http://www.w3.org/2001/XMLSchema#nonNegativeInteger">1</owl:maxCardinality>
</rdf:Description>

<rdf:Description rdf:about="http://cybox.mitre.org/objects/File#PDFXrefEntry">
	<rdfs:subClassOf rdf:nodeID="genid157"/>
</rdf:Description>

<rdf:Description rdf:nodeID="genid157">
	<rdf:type rdf:resource="http://www.w3.org/2002/07/owl#Restriction"/>
	<owl:onProperty rdf:resource="http://cybox.mitre.org/objects/File#generationNumber"/>
	<owl:maxCardinality rdf:datatype="http://www.w3.org/2001/XMLSchema#nonNegativeInteger">1</owl:maxCardinality>
</rdf:Description>

<rdf:Description rdf:about="http://cybox.mitre.org/objects/File#PDFXrefEntry">
	<rdfs:subClassOf rdf:nodeID="genid158"/>
</rdf:Description>

<rdf:Description rdf:nodeID="genid158">
	<rdf:type rdf:resource="http://www.w3.org/2002/07/owl#Restriction"/>
	<owl:onProperty rdf:resource="http://cybox.mitre.org/objects/File#objectNumber"/>
	<owl:maxCardinality rdf:datatype="http://www.w3.org/2001/XMLSchema#nonNegativeInteger">1</owl:maxCardinality>
</rdf:Description>

<rdf:Description rdf:about="http://cybox.mitre.org/objects/File#PDFXrefEntry">
	<rdfs:comment>Characterizes details of a cross-reference table subsection entry.</rdfs:comment>
	<rdfs:isDefinedBy rdf:resource="http://cybox.mitre.org/objects/File"/>
	<rdfs:label>PDFXref entry</rdfs:label>
</rdf:Description>
<!--  -->
<!-- http://cybox.mitre.org/objects/File#PDFXrefTable -->

<rdf:Description rdf:about="http://cybox.mitre.org/objects/File#PDFXrefTable">
	<rdf:type rdf:resource="http://www.w3.org/2002/07/owl#Class"/>
	<rdfs:subClassOf rdf:nodeID="genid159"/>
</rdf:Description>

<rdf:Description rdf:nodeID="genid159">
	<rdf:type rdf:resource="http://www.w3.org/2002/07/owl#Restriction"/>
	<owl:onProperty rdf:resource="http://cybox.mitre.org/objects/File#xrefOffset"/>
	<owl:maxCardinality rdf:datatype="http://www.w3.org/2001/XMLSchema#nonNegativeInteger">1</owl:maxCardinality>
</rdf:Description>

<rdf:Description rdf:about="http://cybox.mitre.org/objects/File#PDFXrefTable">
	<rdfs:comment>Characterizes the details of a PDF cross-reference table, which provides a capability for the random access of indirect objects contained in the file.</rdfs:comment>
	<rdfs:isDefinedBy rdf:resource="http://cybox.mitre.org/objects/File"/>
	<rdfs:label>PDF Cross-Reference Table</rdfs:label>
</rdf:Description>
<!--  -->
<!-- http://cybox.mitre.org/objects/File#PDFXrefTableSubsection -->

<rdf:Description rdf:about="http://cybox.mitre.org/objects/File#PDFXrefTableSubsection">
	<rdf:type rdf:resource="http://www.w3.org/2002/07/owl#Class"/>
	<rdfs:subClassOf rdf:nodeID="genid160"/>
</rdf:Description>

<rdf:Description rdf:nodeID="genid160">
	<rdf:type rdf:resource="http://www.w3.org/2002/07/owl#Restriction"/>
	<owl:onProperty rdf:resource="http://cybox.mitre.org/objects/File#firstObjectNumber"/>
	<owl:maxCardinality rdf:datatype="http://www.w3.org/2001/XMLSchema#nonNegativeInteger">1</owl:maxCardinality>
</rdf:Description>

<rdf:Description rdf:about="http://cybox.mitre.org/objects/File#PDFXrefTableSubsection">
	<rdfs:subClassOf rdf:nodeID="genid161"/>
</rdf:Description>

<rdf:Description rdf:nodeID="genid161">
	<rdf:type rdf:resource="http://www.w3.org/2002/07/owl#Restriction"/>
	<owl:onProperty rdf:resource="http://cybox.mitre.org/objects/File#numberOfObjects"/>
	<owl:maxCardinality rdf:datatype="http://www.w3.org/2001/XMLSchema#nonNegativeInteger">1</owl:maxCardinality>
</rdf:Description>

<rdf:Description rdf:about="http://cybox.mitre.org/objects/File#PDFXrefTableSubsection">
	<rdfs:comment>Characterizes  details of subsections contained within a PDF cross-reference table.</rdfs:comment>
	<rdfs:isDefinedBy rdf:resource="http://cybox.mitre.org/objects/File"/>
	<rdfs:label>PDFXref table subsection</rdfs:label>
</rdf:Description>
<!--  -->
<!-- http://cybox.mitre.org/objects/File#PEDataDirectory -->

<rdf:Description rdf:about="http://cybox.mitre.org/objects/File#PEDataDirectory">
	<rdf:type rdf:resource="http://www.w3.org/2002/07/owl#Class"/>
	<rdfs:subClassOf rdf:nodeID="genid162"/>
</rdf:Description>

<rdf:Description rdf:nodeID="genid162">
	<rdf:type rdf:resource="http://www.w3.org/2002/07/owl#Restriction"/>
	<owl:onProperty rdf:resource="http://cybox.mitre.org/objects/File#architecture.size"/>
	<owl:maxCardinality rdf:datatype="http://www.w3.org/2001/XMLSchema#nonNegativeInteger">1</owl:maxCardinality>
</rdf:Description>

<rdf:Description rdf:about="http://cybox.mitre.org/objects/File#PEDataDirectory">
	<rdfs:subClassOf rdf:nodeID="genid163"/>
</rdf:Description>

<rdf:Description rdf:nodeID="genid163">
	<rdf:type rdf:resource="http://www.w3.org/2002/07/owl#Restriction"/>
	<owl:onProperty rdf:resource="http://cybox.mitre.org/objects/File#architecture.virtualAddress"/>
	<owl:maxCardinality rdf:datatype="http://www.w3.org/2001/XMLSchema#nonNegativeInteger">1</owl:maxCardinality>
</rdf:Description>

<rdf:Description rdf:about="http://cybox.mitre.org/objects/File#PEDataDirectory">
	<rdfs:subClassOf rdf:nodeID="genid164"/>
</rdf:Description>

<rdf:Description rdf:nodeID="genid164">
	<rdf:type rdf:resource="http://www.w3.org/2002/07/owl#Restriction"/>
	<owl:onProperty rdf:resource="http://cybox.mitre.org/objects/File#baseRelocationTable.size"/>
	<owl:maxCardinality rdf:datatype="http://www.w3.org/2001/XMLSchema#nonNegativeInteger">1</owl:maxCardinality>
</rdf:Description>

<rdf:Description rdf:about="http://cybox.mitre.org/objects/File#PEDataDirectory">
	<rdfs:subClassOf rdf:nodeID="genid165"/>
</rdf:Description>

<rdf:Description rdf:nodeID="genid165">
	<rdf:type rdf:resource="http://www.w3.org/2002/07/owl#Restriction"/>
	<owl:onProperty rdf:resource="http://cybox.mitre.org/objects/File#boundImport.size"/>
	<owl:maxCardinality rdf:datatype="http://www.w3.org/2001/XMLSchema#nonNegativeInteger">1</owl:maxCardinality>
</rdf:Description>

<rdf:Description rdf:about="http://cybox.mitre.org/objects/File#PEDataDirectory">
	<rdfs:subClassOf rdf:nodeID="genid166"/>
</rdf:Description>

<rdf:Description rdf:nodeID="genid166">
	<rdf:type rdf:resource="http://www.w3.org/2002/07/owl#Restriction"/>
	<owl:onProperty rdf:resource="http://cybox.mitre.org/objects/File#boundImport.virtualAddress"/>
	<owl:maxCardinality rdf:datatype="http://www.w3.org/2001/XMLSchema#nonNegativeInteger">1</owl:maxCardinality>
</rdf:Description>

<rdf:Description rdf:about="http://cybox.mitre.org/objects/File#PEDataDirectory">
	<rdfs:subClassOf rdf:nodeID="genid167"/>
</rdf:Description>

<rdf:Description rdf:nodeID="genid167">
	<rdf:type rdf:resource="http://www.w3.org/2002/07/owl#Restriction"/>
	<owl:onProperty rdf:resource="http://cybox.mitre.org/objects/File#certificateTable.size"/>
	<owl:maxCardinality rdf:datatype="http://www.w3.org/2001/XMLSchema#nonNegativeInteger">1</owl:maxCardinality>
</rdf:Description>

<rdf:Description rdf:about="http://cybox.mitre.org/objects/File#PEDataDirectory">
	<rdfs:subClassOf rdf:nodeID="genid168"/>
</rdf:Description>

<rdf:Description rdf:nodeID="genid168">
	<rdf:type rdf:resource="http://www.w3.org/2002/07/owl#Restriction"/>
	<owl:onProperty rdf:resource="http://cybox.mitre.org/objects/File#certificateTable.virtualAddress"/>
	<owl:maxCardinality rdf:datatype="http://www.w3.org/2001/XMLSchema#nonNegativeInteger">1</owl:maxCardinality>
</rdf:Description>

<rdf:Description rdf:about="http://cybox.mitre.org/objects/File#PEDataDirectory">
	<rdfs:subClassOf rdf:nodeID="genid169"/>
</rdf:Description>

<rdf:Description rdf:nodeID="genid169">
	<rdf:type rdf:resource="http://www.w3.org/2002/07/owl#Restriction"/>
	<owl:onProperty rdf:resource="http://cybox.mitre.org/objects/File#clrRuntimeHeader.size"/>
	<owl:maxCardinality rdf:datatype="http://www.w3.org/2001/XMLSchema#nonNegativeInteger">1</owl:maxCardinality>
</rdf:Description>

<rdf:Description rdf:about="http://cybox.mitre.org/objects/File#PEDataDirectory">
	<rdfs:subClassOf rdf:nodeID="genid170"/>
</rdf:Description>

<rdf:Description rdf:nodeID="genid170">
	<rdf:type rdf:resource="http://www.w3.org/2002/07/owl#Restriction"/>
	<owl:onProperty rdf:resource="http://cybox.mitre.org/objects/File#clrRuntimeHeader.virtualAddress"/>
	<owl:maxCardinality rdf:datatype="http://www.w3.org/2001/XMLSchema#nonNegativeInteger">1</owl:maxCardinality>
</rdf:Description>

<rdf:Description rdf:about="http://cybox.mitre.org/objects/File#PEDataDirectory">
	<rdfs:subClassOf rdf:nodeID="genid171"/>
</rdf:Description>

<rdf:Description rdf:nodeID="genid171">
	<rdf:type rdf:resource="http://www.w3.org/2002/07/owl#Restriction"/>
	<owl:onProperty rdf:resource="http://cybox.mitre.org/objects/File#debug.size"/>
	<owl:maxCardinality rdf:datatype="http://www.w3.org/2001/XMLSchema#nonNegativeInteger">1</owl:maxCardinality>
</rdf:Description>

<rdf:Description rdf:about="http://cybox.mitre.org/objects/File#PEDataDirectory">
	<rdfs:subClassOf rdf:nodeID="genid172"/>
</rdf:Description>

<rdf:Description rdf:nodeID="genid172">
	<rdf:type rdf:resource="http://www.w3.org/2002/07/owl#Restriction"/>
	<owl:onProperty rdf:resource="http://cybox.mitre.org/objects/File#debug.virtualAddress"/>
	<owl:maxCardinality rdf:datatype="http://www.w3.org/2001/XMLSchema#nonNegativeInteger">1</owl:maxCardinality>
</rdf:Description>

<rdf:Description rdf:about="http://cybox.mitre.org/objects/File#PEDataDirectory">
	<rdfs:subClassOf rdf:nodeID="genid173"/>
</rdf:Description>

<rdf:Description rdf:nodeID="genid173">
	<rdf:type rdf:resource="http://www.w3.org/2002/07/owl#Restriction"/>
	<owl:onProperty rdf:resource="http://cybox.mitre.org/objects/File#delayImportDescriptor.size"/>
	<owl:maxCardinality rdf:datatype="http://www.w3.org/2001/XMLSchema#nonNegativeInteger">1</owl:maxCardinality>
</rdf:Description>

<rdf:Description rdf:about="http://cybox.mitre.org/objects/File#PEDataDirectory">
	<rdfs:subClassOf rdf:nodeID="genid174"/>
</rdf:Description>

<rdf:Description rdf:nodeID="genid174">
	<rdf:type rdf:resource="http://www.w3.org/2002/07/owl#Restriction"/>
	<owl:onProperty rdf:resource="http://cybox.mitre.org/objects/File#delayImportDescriptor.virtualAddress"/>
	<owl:maxCardinality rdf:datatype="http://www.w3.org/2001/XMLSchema#nonNegativeInteger">1</owl:maxCardinality>
</rdf:Description>

<rdf:Description rdf:about="http://cybox.mitre.org/objects/File#PEDataDirectory">
	<rdfs:subClassOf rdf:nodeID="genid175"/>
</rdf:Description>

<rdf:Description rdf:nodeID="genid175">
	<rdf:type rdf:resource="http://www.w3.org/2002/07/owl#Restriction"/>
	<owl:onProperty rdf:resource="http://cybox.mitre.org/objects/File#exceptionTable.size"/>
	<owl:maxCardinality rdf:datatype="http://www.w3.org/2001/XMLSchema#nonNegativeInteger">1</owl:maxCardinality>
</rdf:Description>

<rdf:Description rdf:about="http://cybox.mitre.org/objects/File#PEDataDirectory">
	<rdfs:subClassOf rdf:nodeID="genid176"/>
</rdf:Description>

<rdf:Description rdf:nodeID="genid176">
	<rdf:type rdf:resource="http://www.w3.org/2002/07/owl#Restriction"/>
	<owl:onProperty rdf:resource="http://cybox.mitre.org/objects/File#exceptionTable.virtualAddress"/>
	<owl:maxCardinality rdf:datatype="http://www.w3.org/2001/XMLSchema#nonNegativeInteger">1</owl:maxCardinality>
</rdf:Description>

<rdf:Description rdf:about="http://cybox.mitre.org/objects/File#PEDataDirectory">
	<rdfs:subClassOf rdf:nodeID="genid177"/>
</rdf:Description>

<rdf:Description rdf:nodeID="genid177">
	<rdf:type rdf:resource="http://www.w3.org/2002/07/owl#Restriction"/>
	<owl:onProperty rdf:resource="http://cybox.mitre.org/objects/File#exportTable.size"/>
	<owl:maxCardinality rdf:datatype="http://www.w3.org/2001/XMLSchema#nonNegativeInteger">1</owl:maxCardinality>
</rdf:Description>

<rdf:Description rdf:about="http://cybox.mitre.org/objects/File#PEDataDirectory">
	<rdfs:subClassOf rdf:nodeID="genid178"/>
</rdf:Description>

<rdf:Description rdf:nodeID="genid178">
	<rdf:type rdf:resource="http://www.w3.org/2002/07/owl#Restriction"/>
	<owl:onProperty rdf:resource="http://cybox.mitre.org/objects/File#exportTable.virtualAddress"/>
	<owl:maxCardinality rdf:datatype="http://www.w3.org/2001/XMLSchema#nonNegativeInteger">1</owl:maxCardinality>
</rdf:Description>

<rdf:Description rdf:about="http://cybox.mitre.org/objects/File#PEDataDirectory">
	<rdfs:subClassOf rdf:nodeID="genid179"/>
</rdf:Description>

<rdf:Description rdf:nodeID="genid179">
	<rdf:type rdf:resource="http://www.w3.org/2002/07/owl#Restriction"/>
	<owl:onProperty rdf:resource="http://cybox.mitre.org/objects/File#globalPtr.size"/>
	<owl:maxCardinality rdf:datatype="http://www.w3.org/2001/XMLSchema#nonNegativeInteger">1</owl:maxCardinality>
</rdf:Description>

<rdf:Description rdf:about="http://cybox.mitre.org/objects/File#PEDataDirectory">
	<rdfs:subClassOf rdf:nodeID="genid180"/>
</rdf:Description>

<rdf:Description rdf:nodeID="genid180">
	<rdf:type rdf:resource="http://www.w3.org/2002/07/owl#Restriction"/>
	<owl:onProperty rdf:resource="http://cybox.mitre.org/objects/File#globalPtr.virtualAddress"/>
	<owl:maxCardinality rdf:datatype="http://www.w3.org/2001/XMLSchema#nonNegativeInteger">1</owl:maxCardinality>
</rdf:Description>

<rdf:Description rdf:about="http://cybox.mitre.org/objects/File#PEDataDirectory">
	<rdfs:subClassOf rdf:nodeID="genid181"/>
</rdf:Description>

<rdf:Description rdf:nodeID="genid181">
	<rdf:type rdf:resource="http://www.w3.org/2002/07/owl#Restriction"/>
	<owl:onProperty rdf:resource="http://cybox.mitre.org/objects/File#importAddressTable.size"/>
	<owl:maxCardinality rdf:datatype="http://www.w3.org/2001/XMLSchema#nonNegativeInteger">1</owl:maxCardinality>
</rdf:Description>

<rdf:Description rdf:about="http://cybox.mitre.org/objects/File#PEDataDirectory">
	<rdfs:subClassOf rdf:nodeID="genid182"/>
</rdf:Description>

<rdf:Description rdf:nodeID="genid182">
	<rdf:type rdf:resource="http://www.w3.org/2002/07/owl#Restriction"/>
	<owl:onProperty rdf:resource="http://cybox.mitre.org/objects/File#importAddressTable.virtualAddress"/>
	<owl:maxCardinality rdf:datatype="http://www.w3.org/2001/XMLSchema#nonNegativeInteger">1</owl:maxCardinality>
</rdf:Description>

<rdf:Description rdf:about="http://cybox.mitre.org/objects/File#PEDataDirectory">
	<rdfs:subClassOf rdf:nodeID="genid183"/>
</rdf:Description>

<rdf:Description rdf:nodeID="genid183">
	<rdf:type rdf:resource="http://www.w3.org/2002/07/owl#Restriction"/>
	<owl:onProperty rdf:resource="http://cybox.mitre.org/objects/File#importTable.size"/>
	<owl:maxCardinality rdf:datatype="http://www.w3.org/2001/XMLSchema#nonNegativeInteger">1</owl:maxCardinality>
</rdf:Description>

<rdf:Description rdf:about="http://cybox.mitre.org/objects/File#PEDataDirectory">
	<rdfs:subClassOf rdf:nodeID="genid184"/>
</rdf:Description>

<rdf:Description rdf:nodeID="genid184">
	<rdf:type rdf:resource="http://www.w3.org/2002/07/owl#Restriction"/>
	<owl:onProperty rdf:resource="http://cybox.mitre.org/objects/File#importTable.virtualAddress"/>
	<owl:maxCardinality rdf:datatype="http://www.w3.org/2001/XMLSchema#nonNegativeInteger">1</owl:maxCardinality>
</rdf:Description>

<rdf:Description rdf:about="http://cybox.mitre.org/objects/File#PEDataDirectory">
	<rdfs:subClassOf rdf:nodeID="genid185"/>
</rdf:Description>

<rdf:Description rdf:nodeID="genid185">
	<rdf:type rdf:resource="http://www.w3.org/2002/07/owl#Restriction"/>
	<owl:onProperty rdf:resource="http://cybox.mitre.org/objects/File#loadConfigTable.size"/>
	<owl:maxCardinality rdf:datatype="http://www.w3.org/2001/XMLSchema#nonNegativeInteger">1</owl:maxCardinality>
</rdf:Description>

<rdf:Description rdf:about="http://cybox.mitre.org/objects/File#PEDataDirectory">
	<rdfs:subClassOf rdf:nodeID="genid186"/>
</rdf:Description>

<rdf:Description rdf:nodeID="genid186">
	<rdf:type rdf:resource="http://www.w3.org/2002/07/owl#Restriction"/>
	<owl:onProperty rdf:resource="http://cybox.mitre.org/objects/File#loadConfigTable.virtualAddress"/>
	<owl:maxCardinality rdf:datatype="http://www.w3.org/2001/XMLSchema#nonNegativeInteger">1</owl:maxCardinality>
</rdf:Description>

<rdf:Description rdf:about="http://cybox.mitre.org/objects/File#PEDataDirectory">
	<rdfs:subClassOf rdf:nodeID="genid187"/>
</rdf:Description>

<rdf:Description rdf:nodeID="genid187">
	<rdf:type rdf:resource="http://www.w3.org/2002/07/owl#Restriction"/>
	<owl:onProperty rdf:resource="http://cybox.mitre.org/objects/File#reserved.size"/>
	<owl:maxCardinality rdf:datatype="http://www.w3.org/2001/XMLSchema#nonNegativeInteger">1</owl:maxCardinality>
</rdf:Description>

<rdf:Description rdf:about="http://cybox.mitre.org/objects/File#PEDataDirectory">
	<rdfs:subClassOf rdf:nodeID="genid188"/>
</rdf:Description>

<rdf:Description rdf:nodeID="genid188">
	<rdf:type rdf:resource="http://www.w3.org/2002/07/owl#Restriction"/>
	<owl:onProperty rdf:resource="http://cybox.mitre.org/objects/File#reserved.virtualAddress"/>
	<owl:maxCardinality rdf:datatype="http://www.w3.org/2001/XMLSchema#nonNegativeInteger">1</owl:maxCardinality>
</rdf:Description>

<rdf:Description rdf:about="http://cybox.mitre.org/objects/File#PEDataDirectory">
	<rdfs:subClassOf rdf:nodeID="genid189"/>
</rdf:Description>

<rdf:Description rdf:nodeID="genid189">
	<rdf:type rdf:resource="http://www.w3.org/2002/07/owl#Restriction"/>
	<owl:onProperty rdf:resource="http://cybox.mitre.org/objects/File#resourceTable.size"/>
	<owl:maxCardinality rdf:datatype="http://www.w3.org/2001/XMLSchema#nonNegativeInteger">1</owl:maxCardinality>
</rdf:Description>

<rdf:Description rdf:about="http://cybox.mitre.org/objects/File#PEDataDirectory">
	<rdfs:subClassOf rdf:nodeID="genid190"/>
</rdf:Description>

<rdf:Description rdf:nodeID="genid190">
	<rdf:type rdf:resource="http://www.w3.org/2002/07/owl#Restriction"/>
	<owl:onProperty rdf:resource="http://cybox.mitre.org/objects/File#resourceTable.virtualAddress"/>
	<owl:maxCardinality rdf:datatype="http://www.w3.org/2001/XMLSchema#nonNegativeInteger">1</owl:maxCardinality>
</rdf:Description>

<rdf:Description rdf:about="http://cybox.mitre.org/objects/File#PEDataDirectory">
	<rdfs:subClassOf rdf:nodeID="genid191"/>
</rdf:Description>

<rdf:Description rdf:nodeID="genid191">
	<rdf:type rdf:resource="http://www.w3.org/2002/07/owl#Restriction"/>
	<owl:onProperty rdf:resource="http://cybox.mitre.org/objects/File#tlsTable.size"/>
	<owl:maxCardinality rdf:datatype="http://www.w3.org/2001/XMLSchema#nonNegativeInteger">1</owl:maxCardinality>
</rdf:Description>

<rdf:Description rdf:about="http://cybox.mitre.org/objects/File#PEDataDirectory">
	<rdfs:subClassOf rdf:nodeID="genid192"/>
</rdf:Description>

<rdf:Description rdf:nodeID="genid192">
	<rdf:type rdf:resource="http://www.w3.org/2002/07/owl#Restriction"/>
	<owl:onProperty rdf:resource="http://cybox.mitre.org/objects/File#tlsTable.virtualAddress"/>
	<owl:maxCardinality rdf:datatype="http://www.w3.org/2001/XMLSchema#nonNegativeInteger">1</owl:maxCardinality>
</rdf:Description>

<rdf:Description rdf:about="http://cybox.mitre.org/objects/File#PEDataDirectory">
	<rdfs:comment>Characterizes the data directories that can appear in the PE file's optional header. The data directories, except the Certificate Table, are loaded into memory so they can be used at runtime.</rdfs:comment>
	<rdfs:isDefinedBy rdf:resource="http://cybox.mitre.org/objects/File"/>
	<rdfs:label>PE Data Directory</rdfs:label>
</rdf:Description>
<!--  -->
<!-- http://cybox.mitre.org/objects/File#PEExportedFunction -->

<rdf:Description rdf:about="http://cybox.mitre.org/objects/File#PEExportedFunction">
	<rdf:type rdf:resource="http://www.w3.org/2002/07/owl#Class"/>
	<rdfs:subClassOf rdf:nodeID="genid193"/>
</rdf:Description>

<rdf:Description rdf:nodeID="genid193">
	<rdf:type rdf:resource="http://www.w3.org/2002/07/owl#Restriction"/>
	<owl:onProperty rdf:resource="http://cybox.mitre.org/objects/File#functionName"/>
	<owl:cardinality rdf:datatype="http://www.w3.org/2001/XMLSchema#nonNegativeInteger">1</owl:cardinality>
</rdf:Description>

<rdf:Description rdf:about="http://cybox.mitre.org/objects/File#PEExportedFunction">
	<rdfs:subClassOf rdf:nodeID="genid194"/>
</rdf:Description>

<rdf:Description rdf:nodeID="genid194">
	<rdf:type rdf:resource="http://www.w3.org/2002/07/owl#Restriction"/>
	<owl:onProperty rdf:resource="http://cybox.mitre.org/objects/File#entryPoint"/>
	<owl:maxCardinality rdf:datatype="http://www.w3.org/2001/XMLSchema#nonNegativeInteger">1</owl:maxCardinality>
</rdf:Description>

<rdf:Description rdf:about="http://cybox.mitre.org/objects/File#PEExportedFunction">
	<rdfs:subClassOf rdf:nodeID="genid195"/>
</rdf:Description>

<rdf:Description rdf:nodeID="genid195">
	<rdf:type rdf:resource="http://www.w3.org/2002/07/owl#Restriction"/>
	<owl:onProperty rdf:resource="http://cybox.mitre.org/objects/File#ordinal"/>
	<owl:maxCardinality rdf:datatype="http://www.w3.org/2001/XMLSchema#nonNegativeInteger">1</owl:maxCardinality>
</rdf:Description>

<rdf:Description rdf:about="http://cybox.mitre.org/objects/File#PEExportedFunction">
	<rdfs:comment>Characterizes an exported function.</rdfs:comment>
	<rdfs:isDefinedBy rdf:resource="http://cybox.mitre.org/objects/File"/>
	<rdfs:label>PEExported Function</rdfs:label>
</rdf:Description>
<!--  -->
<!-- http://cybox.mitre.org/objects/File#PEExports -->

<rdf:Description rdf:about="http://cybox.mitre.org/objects/File#PEExports">
	<rdf:type rdf:resource="http://www.w3.org/2002/07/owl#Class"/>
	<rdfs:subClassOf rdf:nodeID="genid196"/>
</rdf:Description>

<rdf:Description rdf:nodeID="genid196">
	<rdf:type rdf:resource="http://www.w3.org/2002/07/owl#Restriction"/>
	<owl:onProperty rdf:resource="http://cybox.mitre.org/objects/File#peModuleName"/>
	<owl:cardinality rdf:datatype="http://www.w3.org/2001/XMLSchema#nonNegativeInteger">1</owl:cardinality>
</rdf:Description>

<rdf:Description rdf:about="http://cybox.mitre.org/objects/File#PEExports">
	<rdfs:subClassOf rdf:nodeID="genid197"/>
</rdf:Description>

<rdf:Description rdf:nodeID="genid197">
	<rdf:type rdf:resource="http://www.w3.org/2002/07/owl#Restriction"/>
	<owl:onProperty rdf:resource="http://cybox.mitre.org/objects/File#exportsTimestamp"/>
	<owl:maxCardinality rdf:datatype="http://www.w3.org/2001/XMLSchema#nonNegativeInteger">1</owl:maxCardinality>
</rdf:Description>

<rdf:Description rdf:about="http://cybox.mitre.org/objects/File#PEExports">
	<rdfs:subClassOf rdf:nodeID="genid198"/>
</rdf:Description>

<rdf:Description rdf:nodeID="genid198">
	<rdf:type rdf:resource="http://www.w3.org/2002/07/owl#Restriction"/>
	<owl:onProperty rdf:resource="http://cybox.mitre.org/objects/File#numberOfAddresses"/>
	<owl:maxCardinality rdf:datatype="http://www.w3.org/2001/XMLSchema#nonNegativeInteger">1</owl:maxCardinality>
</rdf:Description>

<rdf:Description rdf:about="http://cybox.mitre.org/objects/File#PEExports">
	<rdfs:subClassOf rdf:nodeID="genid199"/>
</rdf:Description>

<rdf:Description rdf:nodeID="genid199">
	<rdf:type rdf:resource="http://www.w3.org/2002/07/owl#Restriction"/>
	<owl:onProperty rdf:resource="http://cybox.mitre.org/objects/File#numberOfNames"/>
	<owl:maxCardinality rdf:datatype="http://www.w3.org/2001/XMLSchema#nonNegativeInteger">1</owl:maxCardinality>
</rdf:Description>

<rdf:Description rdf:about="http://cybox.mitre.org/objects/File#PEExports">
	<rdfs:subClassOf rdf:nodeID="genid200"/>
</rdf:Description>

<rdf:Description rdf:nodeID="genid200">
	<rdf:type rdf:resource="http://www.w3.org/2002/07/owl#Restriction"/>
	<owl:onProperty rdf:resource="http://cybox.mitre.org/objects/File#numberofFunctions"/>
	<owl:maxCardinality rdf:datatype="http://www.w3.org/2001/XMLSchema#nonNegativeInteger">1</owl:maxCardinality>
</rdf:Description>

<rdf:Description rdf:about="http://cybox.mitre.org/objects/File#PEExports">
	<rdfs:comment>Characterizes the PE File exports data section. &#xD;
&#xD;
The exports data section contains information about symbols exported by the PE File (a DLL) which can be dynamically loaded by other executables. This type abstracts, and its components, abstract the Windows structures.</rdfs:comment>
	<rdfs:isDefinedBy rdf:resource="http://cybox.mitre.org/objects/File"/>
	<rdfs:label>PEExports</rdfs:label>
</rdf:Description>
<!--  -->
<!-- http://cybox.mitre.org/objects/File#PEHeaders -->

<rdf:Description rdf:about="http://cybox.mitre.org/objects/File#PEHeaders">
	<rdf:type rdf:resource="http://www.w3.org/2002/07/owl#Class"/>
	<rdfs:subClassOf rdf:nodeID="genid201"/>
</rdf:Description>

<rdf:Description rdf:nodeID="genid201">
	<rdf:type rdf:resource="http://www.w3.org/2002/07/owl#Restriction"/>
	<owl:onProperty rdf:resource="http://cybox.mitre.org/objects/File#optionalHeader.dataDirectory"/>
	<owl:maxCardinality rdf:datatype="http://www.w3.org/2001/XMLSchema#nonNegativeInteger">1</owl:maxCardinality>
</rdf:Description>

<rdf:Description rdf:about="http://cybox.mitre.org/objects/File#PEHeaders">
	<rdfs:subClassOf rdf:nodeID="genid202"/>
</rdf:Description>

<rdf:Description rdf:nodeID="genid202">
	<rdf:type rdf:resource="http://www.w3.org/2002/07/owl#Restriction"/>
	<owl:onProperty rdf:resource="http://cybox.mitre.org/objects/File#dosHeader.e_cblp"/>
	<owl:maxCardinality rdf:datatype="http://www.w3.org/2001/XMLSchema#nonNegativeInteger">1</owl:maxCardinality>
</rdf:Description>

<rdf:Description rdf:about="http://cybox.mitre.org/objects/File#PEHeaders">
	<rdfs:subClassOf rdf:nodeID="genid203"/>
</rdf:Description>

<rdf:Description rdf:nodeID="genid203">
	<rdf:type rdf:resource="http://www.w3.org/2002/07/owl#Restriction"/>
	<owl:onProperty rdf:resource="http://cybox.mitre.org/objects/File#dosHeader.e_cp"/>
	<owl:maxCardinality rdf:datatype="http://www.w3.org/2001/XMLSchema#nonNegativeInteger">1</owl:maxCardinality>
</rdf:Description>

<rdf:Description rdf:about="http://cybox.mitre.org/objects/File#PEHeaders">
	<rdfs:subClassOf rdf:nodeID="genid204"/>
</rdf:Description>

<rdf:Description rdf:nodeID="genid204">
	<rdf:type rdf:resource="http://www.w3.org/2002/07/owl#Restriction"/>
	<owl:onProperty rdf:resource="http://cybox.mitre.org/objects/File#dosHeader.e_crlc"/>
	<owl:maxCardinality rdf:datatype="http://www.w3.org/2001/XMLSchema#nonNegativeInteger">1</owl:maxCardinality>
</rdf:Description>

<rdf:Description rdf:about="http://cybox.mitre.org/objects/File#PEHeaders">
	<rdfs:subClassOf rdf:nodeID="genid205"/>
</rdf:Description>

<rdf:Description rdf:nodeID="genid205">
	<rdf:type rdf:resource="http://www.w3.org/2002/07/owl#Restriction"/>
	<owl:onProperty rdf:resource="http://cybox.mitre.org/objects/File#dosHeader.e_cs"/>
	<owl:maxCardinality rdf:datatype="http://www.w3.org/2001/XMLSchema#nonNegativeInteger">1</owl:maxCardinality>
</rdf:Description>

<rdf:Description rdf:about="http://cybox.mitre.org/objects/File#PEHeaders">
	<rdfs:subClassOf rdf:nodeID="genid206"/>
</rdf:Description>

<rdf:Description rdf:nodeID="genid206">
	<rdf:type rdf:resource="http://www.w3.org/2002/07/owl#Restriction"/>
	<owl:onProperty rdf:resource="http://cybox.mitre.org/objects/File#dosHeader.e_csum"/>
	<owl:maxCardinality rdf:datatype="http://www.w3.org/2001/XMLSchema#nonNegativeInteger">1</owl:maxCardinality>
</rdf:Description>

<rdf:Description rdf:about="http://cybox.mitre.org/objects/File#PEHeaders">
	<rdfs:subClassOf rdf:nodeID="genid207"/>
</rdf:Description>

<rdf:Description rdf:nodeID="genid207">
	<rdf:type rdf:resource="http://www.w3.org/2002/07/owl#Restriction"/>
	<owl:onProperty rdf:resource="http://cybox.mitre.org/objects/File#dosHeader.e_ip"/>
	<owl:maxCardinality rdf:datatype="http://www.w3.org/2001/XMLSchema#nonNegativeInteger">1</owl:maxCardinality>
</rdf:Description>

<rdf:Description rdf:about="http://cybox.mitre.org/objects/File#PEHeaders">
	<rdfs:subClassOf rdf:nodeID="genid208"/>
</rdf:Description>

<rdf:Description rdf:nodeID="genid208">
	<rdf:type rdf:resource="http://www.w3.org/2002/07/owl#Restriction"/>
	<owl:onProperty rdf:resource="http://cybox.mitre.org/objects/File#dosHeader.e_lfanew"/>
	<owl:maxCardinality rdf:datatype="http://www.w3.org/2001/XMLSchema#nonNegativeInteger">1</owl:maxCardinality>
</rdf:Description>

<rdf:Description rdf:about="http://cybox.mitre.org/objects/File#PEHeaders">
	<rdfs:subClassOf rdf:nodeID="genid209"/>
</rdf:Description>

<rdf:Description rdf:nodeID="genid209">
	<rdf:type rdf:resource="http://www.w3.org/2002/07/owl#Restriction"/>
	<owl:onProperty rdf:resource="http://cybox.mitre.org/objects/File#dosHeader.e_lfarlc"/>
	<owl:maxCardinality rdf:datatype="http://www.w3.org/2001/XMLSchema#nonNegativeInteger">1</owl:maxCardinality>
</rdf:Description>

<rdf:Description rdf:about="http://cybox.mitre.org/objects/File#PEHeaders">
	<rdfs:subClassOf rdf:nodeID="genid210"/>
</rdf:Description>

<rdf:Description rdf:nodeID="genid210">
	<rdf:type rdf:resource="http://www.w3.org/2002/07/owl#Restriction"/>
	<owl:onProperty rdf:resource="http://cybox.mitre.org/objects/File#dosHeader.e_magic"/>
	<owl:maxCardinality rdf:datatype="http://www.w3.org/2001/XMLSchema#nonNegativeInteger">1</owl:maxCardinality>
</rdf:Description>

<rdf:Description rdf:about="http://cybox.mitre.org/objects/File#PEHeaders">
	<rdfs:subClassOf rdf:nodeID="genid211"/>
</rdf:Description>

<rdf:Description rdf:nodeID="genid211">
	<rdf:type rdf:resource="http://www.w3.org/2002/07/owl#Restriction"/>
	<owl:onProperty rdf:resource="http://cybox.mitre.org/objects/File#dosHeader.e_maxalloc"/>
	<owl:maxCardinality rdf:datatype="http://www.w3.org/2001/XMLSchema#nonNegativeInteger">1</owl:maxCardinality>
</rdf:Description>

<rdf:Description rdf:about="http://cybox.mitre.org/objects/File#PEHeaders">
	<rdfs:subClassOf rdf:nodeID="genid212"/>
</rdf:Description>

<rdf:Description rdf:nodeID="genid212">
	<rdf:type rdf:resource="http://www.w3.org/2002/07/owl#Restriction"/>
	<owl:onProperty rdf:resource="http://cybox.mitre.org/objects/File#dosHeader.e_minalloc"/>
	<owl:maxCardinality rdf:datatype="http://www.w3.org/2001/XMLSchema#nonNegativeInteger">1</owl:maxCardinality>
</rdf:Description>

<rdf:Description rdf:about="http://cybox.mitre.org/objects/File#PEHeaders">
	<rdfs:subClassOf rdf:nodeID="genid213"/>
</rdf:Description>

<rdf:Description rdf:nodeID="genid213">
	<rdf:type rdf:resource="http://www.w3.org/2002/07/owl#Restriction"/>
	<owl:onProperty rdf:resource="http://cybox.mitre.org/objects/File#dosHeader.e_oemid"/>
	<owl:maxCardinality rdf:datatype="http://www.w3.org/2001/XMLSchema#nonNegativeInteger">1</owl:maxCardinality>
</rdf:Description>

<rdf:Description rdf:about="http://cybox.mitre.org/objects/File#PEHeaders">
	<rdfs:subClassOf rdf:nodeID="genid214"/>
</rdf:Description>

<rdf:Description rdf:nodeID="genid214">
	<rdf:type rdf:resource="http://www.w3.org/2002/07/owl#Restriction"/>
	<owl:onProperty rdf:resource="http://cybox.mitre.org/objects/File#dosHeader.e_oeminfo"/>
	<owl:maxCardinality rdf:datatype="http://www.w3.org/2001/XMLSchema#nonNegativeInteger">1</owl:maxCardinality>
</rdf:Description>

<rdf:Description rdf:about="http://cybox.mitre.org/objects/File#PEHeaders">
	<rdfs:subClassOf rdf:nodeID="genid215"/>
</rdf:Description>

<rdf:Description rdf:nodeID="genid215">
	<rdf:type rdf:resource="http://www.w3.org/2002/07/owl#Restriction"/>
	<owl:onProperty rdf:resource="http://cybox.mitre.org/objects/File#dosHeader.e_ovro"/>
	<owl:maxCardinality rdf:datatype="http://www.w3.org/2001/XMLSchema#nonNegativeInteger">1</owl:maxCardinality>
</rdf:Description>

<rdf:Description rdf:about="http://cybox.mitre.org/objects/File#PEHeaders">
	<rdfs:subClassOf rdf:nodeID="genid216"/>
</rdf:Description>

<rdf:Description rdf:nodeID="genid216">
	<rdf:type rdf:resource="http://www.w3.org/2002/07/owl#Restriction"/>
	<owl:onProperty rdf:resource="http://cybox.mitre.org/objects/File#dosHeader.e_sp"/>
	<owl:maxCardinality rdf:datatype="http://www.w3.org/2001/XMLSchema#nonNegativeInteger">1</owl:maxCardinality>
</rdf:Description>

<rdf:Description rdf:about="http://cybox.mitre.org/objects/File#PEHeaders">
	<rdfs:subClassOf rdf:nodeID="genid217"/>
</rdf:Description>

<rdf:Description rdf:nodeID="genid217">
	<rdf:type rdf:resource="http://www.w3.org/2002/07/owl#Restriction"/>
	<owl:onProperty rdf:resource="http://cybox.mitre.org/objects/File#dosHeader.e_ss"/>
	<owl:maxCardinality rdf:datatype="http://www.w3.org/2001/XMLSchema#nonNegativeInteger">1</owl:maxCardinality>
</rdf:Description>

<rdf:Description rdf:about="http://cybox.mitre.org/objects/File#PEHeaders">
	<rdfs:subClassOf rdf:nodeID="genid218"/>
</rdf:Description>

<rdf:Description rdf:nodeID="genid218">
	<rdf:type rdf:resource="http://www.w3.org/2002/07/owl#Restriction"/>
	<owl:onProperty rdf:resource="http://cybox.mitre.org/objects/File#dosHeader.reserved1"/>
	<owl:maxCardinality rdf:datatype="http://www.w3.org/2001/XMLSchema#nonNegativeInteger">1</owl:maxCardinality>
</rdf:Description>

<rdf:Description rdf:about="http://cybox.mitre.org/objects/File#PEHeaders">
	<rdfs:subClassOf rdf:nodeID="genid219"/>
</rdf:Description>

<rdf:Description rdf:nodeID="genid219">
	<rdf:type rdf:resource="http://www.w3.org/2002/07/owl#Restriction"/>
	<owl:onProperty rdf:resource="http://cybox.mitre.org/objects/File#dosHeader.reserved2"/>
	<owl:maxCardinality rdf:datatype="http://www.w3.org/2001/XMLSchema#nonNegativeInteger">1</owl:maxCardinality>
</rdf:Description>

<rdf:Description rdf:about="http://cybox.mitre.org/objects/File#PEHeaders">
	<rdfs:subClassOf rdf:nodeID="genid220"/>
</rdf:Description>

<rdf:Description rdf:nodeID="genid220">
	<rdf:type rdf:resource="http://www.w3.org/2002/07/owl#Restriction"/>
	<owl:onProperty rdf:resource="http://cybox.mitre.org/objects/File#entropy.max"/>
	<owl:maxCardinality rdf:datatype="http://www.w3.org/2001/XMLSchema#nonNegativeInteger">1</owl:maxCardinality>
</rdf:Description>

<rdf:Description rdf:about="http://cybox.mitre.org/objects/File#PEHeaders">
	<rdfs:subClassOf rdf:nodeID="genid221"/>
</rdf:Description>

<rdf:Description rdf:nodeID="genid221">
	<rdf:type rdf:resource="http://www.w3.org/2002/07/owl#Restriction"/>
	<owl:onProperty rdf:resource="http://cybox.mitre.org/objects/File#entropy.min"/>
	<owl:maxCardinality rdf:datatype="http://www.w3.org/2001/XMLSchema#nonNegativeInteger">1</owl:maxCardinality>
</rdf:Description>

<rdf:Description rdf:about="http://cybox.mitre.org/objects/File#PEHeaders">
	<rdfs:subClassOf rdf:nodeID="genid222"/>
</rdf:Description>

<rdf:Description rdf:nodeID="genid222">
	<rdf:type rdf:resource="http://www.w3.org/2002/07/owl#Restriction"/>
	<owl:onProperty rdf:resource="http://cybox.mitre.org/objects/File#entropy.value"/>
	<owl:maxCardinality rdf:datatype="http://www.w3.org/2001/XMLSchema#nonNegativeInteger">1</owl:maxCardinality>
</rdf:Description>

<rdf:Description rdf:about="http://cybox.mitre.org/objects/File#PEHeaders">
	<rdfs:subClassOf rdf:nodeID="genid223"/>
</rdf:Description>

<rdf:Description rdf:nodeID="genid223">
	<rdf:type rdf:resource="http://www.w3.org/2002/07/owl#Restriction"/>
	<owl:onProperty rdf:resource="http://cybox.mitre.org/objects/File#fileHeader.characteristics"/>
	<owl:maxCardinality rdf:datatype="http://www.w3.org/2001/XMLSchema#nonNegativeInteger">1</owl:maxCardinality>
</rdf:Description>

<rdf:Description rdf:about="http://cybox.mitre.org/objects/File#PEHeaders">
	<rdfs:subClassOf rdf:nodeID="genid224"/>
</rdf:Description>

<rdf:Description rdf:nodeID="genid224">
	<rdf:type rdf:resource="http://www.w3.org/2002/07/owl#Restriction"/>
	<owl:onProperty rdf:resource="http://cybox.mitre.org/objects/File#fileHeader.machine"/>
	<owl:maxCardinality rdf:datatype="http://www.w3.org/2001/XMLSchema#nonNegativeInteger">1</owl:maxCardinality>
</rdf:Description>

<rdf:Description rdf:about="http://cybox.mitre.org/objects/File#PEHeaders">
	<rdfs:subClassOf rdf:nodeID="genid225"/>
</rdf:Description>

<rdf:Description rdf:nodeID="genid225">
	<rdf:type rdf:resource="http://www.w3.org/2002/07/owl#Restriction"/>
	<owl:onProperty rdf:resource="http://cybox.mitre.org/objects/File#fileHeader.numberOfSections"/>
	<owl:maxCardinality rdf:datatype="http://www.w3.org/2001/XMLSchema#nonNegativeInteger">1</owl:maxCardinality>
</rdf:Description>

<rdf:Description rdf:about="http://cybox.mitre.org/objects/File#PEHeaders">
	<rdfs:subClassOf rdf:nodeID="genid226"/>
</rdf:Description>

<rdf:Description rdf:nodeID="genid226">
	<rdf:type rdf:resource="http://www.w3.org/2002/07/owl#Restriction"/>
	<owl:onProperty rdf:resource="http://cybox.mitre.org/objects/File#fileHeader.numberOfSymbols"/>
	<owl:maxCardinality rdf:datatype="http://www.w3.org/2001/XMLSchema#nonNegativeInteger">1</owl:maxCardinality>
</rdf:Description>

<rdf:Description rdf:about="http://cybox.mitre.org/objects/File#PEHeaders">
	<rdfs:subClassOf rdf:nodeID="genid227"/>
</rdf:Description>

<rdf:Description rdf:nodeID="genid227">
	<rdf:type rdf:resource="http://www.w3.org/2002/07/owl#Restriction"/>
	<owl:onProperty rdf:resource="http://cybox.mitre.org/objects/File#fileHeader.pointerToSymbolTable"/>
	<owl:maxCardinality rdf:datatype="http://www.w3.org/2001/XMLSchema#nonNegativeInteger">1</owl:maxCardinality>
</rdf:Description>

<rdf:Description rdf:about="http://cybox.mitre.org/objects/File#PEHeaders">
	<rdfs:subClassOf rdf:nodeID="genid228"/>
</rdf:Description>

<rdf:Description rdf:nodeID="genid228">
	<rdf:type rdf:resource="http://www.w3.org/2002/07/owl#Restriction"/>
	<owl:onProperty rdf:resource="http://cybox.mitre.org/objects/File#fileHeader.sizeOfOptionalHeader"/>
	<owl:maxCardinality rdf:datatype="http://www.w3.org/2001/XMLSchema#nonNegativeInteger">1</owl:maxCardinality>
</rdf:Description>

<rdf:Description rdf:about="http://cybox.mitre.org/objects/File#PEHeaders">
	<rdfs:subClassOf rdf:nodeID="genid229"/>
</rdf:Description>

<rdf:Description rdf:nodeID="genid229">
	<rdf:type rdf:resource="http://www.w3.org/2002/07/owl#Restriction"/>
	<owl:onProperty rdf:resource="http://cybox.mitre.org/objects/File#fileHeader.timestamp"/>
	<owl:maxCardinality rdf:datatype="http://www.w3.org/2001/XMLSchema#nonNegativeInteger">1</owl:maxCardinality>
</rdf:Description>

<rdf:Description rdf:about="http://cybox.mitre.org/objects/File#PEHeaders">
	<rdfs:subClassOf rdf:nodeID="genid230"/>
</rdf:Description>

<rdf:Description rdf:nodeID="genid230">
	<rdf:type rdf:resource="http://www.w3.org/2002/07/owl#Restriction"/>
	<owl:onProperty rdf:resource="http://cybox.mitre.org/objects/File#optionalHeader.addressOfEntryPoint"/>
	<owl:maxCardinality rdf:datatype="http://www.w3.org/2001/XMLSchema#nonNegativeInteger">1</owl:maxCardinality>
</rdf:Description>

<rdf:Description rdf:about="http://cybox.mitre.org/objects/File#PEHeaders">
	<rdfs:subClassOf rdf:nodeID="genid231"/>
</rdf:Description>

<rdf:Description rdf:nodeID="genid231">
	<rdf:type rdf:resource="http://www.w3.org/2002/07/owl#Restriction"/>
	<owl:onProperty rdf:resource="http://cybox.mitre.org/objects/File#optionalHeader.baseOfCode"/>
	<owl:maxCardinality rdf:datatype="http://www.w3.org/2001/XMLSchema#nonNegativeInteger">1</owl:maxCardinality>
</rdf:Description>

<rdf:Description rdf:about="http://cybox.mitre.org/objects/File#PEHeaders">
	<rdfs:subClassOf rdf:nodeID="genid232"/>
</rdf:Description>

<rdf:Description rdf:nodeID="genid232">
	<rdf:type rdf:resource="http://www.w3.org/2002/07/owl#Restriction"/>
	<owl:onProperty rdf:resource="http://cybox.mitre.org/objects/File#optionalHeader.baseOfData"/>
	<owl:maxCardinality rdf:datatype="http://www.w3.org/2001/XMLSchema#nonNegativeInteger">1</owl:maxCardinality>
</rdf:Description>

<rdf:Description rdf:about="http://cybox.mitre.org/objects/File#PEHeaders">
	<rdfs:subClassOf rdf:nodeID="genid233"/>
</rdf:Description>

<rdf:Description rdf:nodeID="genid233">
	<rdf:type rdf:resource="http://www.w3.org/2002/07/owl#Restriction"/>
	<owl:onProperty rdf:resource="http://cybox.mitre.org/objects/File#optionalHeader.checksum"/>
	<owl:maxCardinality rdf:datatype="http://www.w3.org/2001/XMLSchema#nonNegativeInteger">1</owl:maxCardinality>
</rdf:Description>

<rdf:Description rdf:about="http://cybox.mitre.org/objects/File#PEHeaders">
	<rdfs:subClassOf rdf:nodeID="genid234"/>
</rdf:Description>

<rdf:Description rdf:nodeID="genid234">
	<rdf:type rdf:resource="http://www.w3.org/2002/07/owl#Restriction"/>
	<owl:onProperty rdf:resource="http://cybox.mitre.org/objects/File#optionalHeader.dllCharacteristics"/>
	<owl:maxCardinality rdf:datatype="http://www.w3.org/2001/XMLSchema#nonNegativeInteger">1</owl:maxCardinality>
</rdf:Description>

<rdf:Description rdf:about="http://cybox.mitre.org/objects/File#PEHeaders">
	<rdfs:subClassOf rdf:nodeID="genid235"/>
</rdf:Description>

<rdf:Description rdf:nodeID="genid235">
	<rdf:type rdf:resource="http://www.w3.org/2002/07/owl#Restriction"/>
	<owl:onProperty rdf:resource="http://cybox.mitre.org/objects/File#optionalHeader.fileAlignment"/>
	<owl:maxCardinality rdf:datatype="http://www.w3.org/2001/XMLSchema#nonNegativeInteger">1</owl:maxCardinality>
</rdf:Description>

<rdf:Description rdf:about="http://cybox.mitre.org/objects/File#PEHeaders">
	<rdfs:subClassOf rdf:nodeID="genid236"/>
</rdf:Description>

<rdf:Description rdf:nodeID="genid236">
	<rdf:type rdf:resource="http://www.w3.org/2002/07/owl#Restriction"/>
	<owl:onProperty rdf:resource="http://cybox.mitre.org/objects/File#optionalHeader.imageBase"/>
	<owl:maxCardinality rdf:datatype="http://www.w3.org/2001/XMLSchema#nonNegativeInteger">1</owl:maxCardinality>
</rdf:Description>

<rdf:Description rdf:about="http://cybox.mitre.org/objects/File#PEHeaders">
	<rdfs:subClassOf rdf:nodeID="genid237"/>
</rdf:Description>

<rdf:Description rdf:nodeID="genid237">
	<rdf:type rdf:resource="http://www.w3.org/2002/07/owl#Restriction"/>
	<owl:onProperty rdf:resource="http://cybox.mitre.org/objects/File#optionalHeader.loaderFlags"/>
	<owl:maxCardinality rdf:datatype="http://www.w3.org/2001/XMLSchema#nonNegativeInteger">1</owl:maxCardinality>
</rdf:Description>

<rdf:Description rdf:about="http://cybox.mitre.org/objects/File#PEHeaders">
	<rdfs:subClassOf rdf:nodeID="genid238"/>
</rdf:Description>

<rdf:Description rdf:nodeID="genid238">
	<rdf:type rdf:resource="http://www.w3.org/2002/07/owl#Restriction"/>
	<owl:onProperty rdf:resource="http://cybox.mitre.org/objects/File#optionalHeader.magic"/>
	<owl:maxCardinality rdf:datatype="http://www.w3.org/2001/XMLSchema#nonNegativeInteger">1</owl:maxCardinality>
</rdf:Description>

<rdf:Description rdf:about="http://cybox.mitre.org/objects/File#PEHeaders">
	<rdfs:subClassOf rdf:nodeID="genid239"/>
</rdf:Description>

<rdf:Description rdf:nodeID="genid239">
	<rdf:type rdf:resource="http://www.w3.org/2002/07/owl#Restriction"/>
	<owl:onProperty rdf:resource="http://cybox.mitre.org/objects/File#optionalHeader.majorImageVersion"/>
	<owl:maxCardinality rdf:datatype="http://www.w3.org/2001/XMLSchema#nonNegativeInteger">1</owl:maxCardinality>
</rdf:Description>

<rdf:Description rdf:about="http://cybox.mitre.org/objects/File#PEHeaders">
	<rdfs:subClassOf rdf:nodeID="genid240"/>
</rdf:Description>

<rdf:Description rdf:nodeID="genid240">
	<rdf:type rdf:resource="http://www.w3.org/2002/07/owl#Restriction"/>
	<owl:onProperty rdf:resource="http://cybox.mitre.org/objects/File#optionalHeader.majorLinkerVersion"/>
	<owl:maxCardinality rdf:datatype="http://www.w3.org/2001/XMLSchema#nonNegativeInteger">1</owl:maxCardinality>
</rdf:Description>

<rdf:Description rdf:about="http://cybox.mitre.org/objects/File#PEHeaders">
	<rdfs:subClassOf rdf:nodeID="genid241"/>
</rdf:Description>

<rdf:Description rdf:nodeID="genid241">
	<rdf:type rdf:resource="http://www.w3.org/2002/07/owl#Restriction"/>
	<owl:onProperty rdf:resource="http://cybox.mitre.org/objects/File#optionalHeader.majorOSVersion"/>
	<owl:maxCardinality rdf:datatype="http://www.w3.org/2001/XMLSchema#nonNegativeInteger">1</owl:maxCardinality>
</rdf:Description>

<rdf:Description rdf:about="http://cybox.mitre.org/objects/File#PEHeaders">
	<rdfs:subClassOf rdf:nodeID="genid242"/>
</rdf:Description>

<rdf:Description rdf:nodeID="genid242">
	<rdf:type rdf:resource="http://www.w3.org/2002/07/owl#Restriction"/>
	<owl:onProperty rdf:resource="http://cybox.mitre.org/objects/File#optionalHeader.majorSubsystemVersion"/>
	<owl:maxCardinality rdf:datatype="http://www.w3.org/2001/XMLSchema#nonNegativeInteger">1</owl:maxCardinality>
</rdf:Description>

<rdf:Description rdf:about="http://cybox.mitre.org/objects/File#PEHeaders">
	<rdfs:subClassOf rdf:nodeID="genid243"/>
</rdf:Description>

<rdf:Description rdf:nodeID="genid243">
	<rdf:type rdf:resource="http://www.w3.org/2002/07/owl#Restriction"/>
	<owl:onProperty rdf:resource="http://cybox.mitre.org/objects/File#optionalHeader.minorImageVersion"/>
	<owl:maxCardinality rdf:datatype="http://www.w3.org/2001/XMLSchema#nonNegativeInteger">1</owl:maxCardinality>
</rdf:Description>

<rdf:Description rdf:about="http://cybox.mitre.org/objects/File#PEHeaders">
	<rdfs:subClassOf rdf:nodeID="genid244"/>
</rdf:Description>

<rdf:Description rdf:nodeID="genid244">
	<rdf:type rdf:resource="http://www.w3.org/2002/07/owl#Restriction"/>
	<owl:onProperty rdf:resource="http://cybox.mitre.org/objects/File#optionalHeader.minorLinkerVersion"/>
	<owl:maxCardinality rdf:datatype="http://www.w3.org/2001/XMLSchema#nonNegativeInteger">1</owl:maxCardinality>
</rdf:Description>

<rdf:Description rdf:about="http://cybox.mitre.org/objects/File#PEHeaders">
	<rdfs:subClassOf rdf:nodeID="genid245"/>
</rdf:Description>

<rdf:Description rdf:nodeID="genid245">
	<rdf:type rdf:resource="http://www.w3.org/2002/07/owl#Restriction"/>
	<owl:onProperty rdf:resource="http://cybox.mitre.org/objects/File#optionalHeader.minorOSVersion"/>
	<owl:maxCardinality rdf:datatype="http://www.w3.org/2001/XMLSchema#nonNegativeInteger">1</owl:maxCardinality>
</rdf:Description>

<rdf:Description rdf:about="http://cybox.mitre.org/objects/File#PEHeaders">
	<rdfs:subClassOf rdf:nodeID="genid246"/>
</rdf:Description>

<rdf:Description rdf:nodeID="genid246">
	<rdf:type rdf:resource="http://www.w3.org/2002/07/owl#Restriction"/>
	<owl:onProperty rdf:resource="http://cybox.mitre.org/objects/File#optionalHeader.minorSubsystemVersion"/>
	<owl:maxCardinality rdf:datatype="http://www.w3.org/2001/XMLSchema#nonNegativeInteger">1</owl:maxCardinality>
</rdf:Description>

<rdf:Description rdf:about="http://cybox.mitre.org/objects/File#PEHeaders">
	<rdfs:subClassOf rdf:nodeID="genid247"/>
</rdf:Description>

<rdf:Description rdf:nodeID="genid247">
	<rdf:type rdf:resource="http://www.w3.org/2002/07/owl#Restriction"/>
	<owl:onProperty rdf:resource="http://cybox.mitre.org/objects/File#optionalHeader.numberOfRvaAndSizes"/>
	<owl:maxCardinality rdf:datatype="http://www.w3.org/2001/XMLSchema#nonNegativeInteger">1</owl:maxCardinality>
</rdf:Description>

<rdf:Description rdf:about="http://cybox.mitre.org/objects/File#PEHeaders">
	<rdfs:subClassOf rdf:nodeID="genid248"/>
</rdf:Description>

<rdf:Description rdf:nodeID="genid248">
	<rdf:type rdf:resource="http://www.w3.org/2002/07/owl#Restriction"/>
	<owl:onProperty rdf:resource="http://cybox.mitre.org/objects/File#optionalHeader.sectionAlignment"/>
	<owl:maxCardinality rdf:datatype="http://www.w3.org/2001/XMLSchema#nonNegativeInteger">1</owl:maxCardinality>
</rdf:Description>

<rdf:Description rdf:about="http://cybox.mitre.org/objects/File#PEHeaders">
	<rdfs:subClassOf rdf:nodeID="genid249"/>
</rdf:Description>

<rdf:Description rdf:nodeID="genid249">
	<rdf:type rdf:resource="http://www.w3.org/2002/07/owl#Restriction"/>
	<owl:onProperty rdf:resource="http://cybox.mitre.org/objects/File#optionalHeader.sizeOfCode"/>
	<owl:maxCardinality rdf:datatype="http://www.w3.org/2001/XMLSchema#nonNegativeInteger">1</owl:maxCardinality>
</rdf:Description>

<rdf:Description rdf:about="http://cybox.mitre.org/objects/File#PEHeaders">
	<rdfs:subClassOf rdf:nodeID="genid250"/>
</rdf:Description>

<rdf:Description rdf:nodeID="genid250">
	<rdf:type rdf:resource="http://www.w3.org/2002/07/owl#Restriction"/>
	<owl:onProperty rdf:resource="http://cybox.mitre.org/objects/File#optionalHeader.sizeOfHeaders"/>
	<owl:maxCardinality rdf:datatype="http://www.w3.org/2001/XMLSchema#nonNegativeInteger">1</owl:maxCardinality>
</rdf:Description>

<rdf:Description rdf:about="http://cybox.mitre.org/objects/File#PEHeaders">
	<rdfs:subClassOf rdf:nodeID="genid251"/>
</rdf:Description>

<rdf:Description rdf:nodeID="genid251">
	<rdf:type rdf:resource="http://www.w3.org/2002/07/owl#Restriction"/>
	<owl:onProperty rdf:resource="http://cybox.mitre.org/objects/File#optionalHeader.sizeOfHeapCommit"/>
	<owl:maxCardinality rdf:datatype="http://www.w3.org/2001/XMLSchema#nonNegativeInteger">1</owl:maxCardinality>
</rdf:Description>

<rdf:Description rdf:about="http://cybox.mitre.org/objects/File#PEHeaders">
	<rdfs:subClassOf rdf:nodeID="genid252"/>
</rdf:Description>

<rdf:Description rdf:nodeID="genid252">
	<rdf:type rdf:resource="http://www.w3.org/2002/07/owl#Restriction"/>
	<owl:onProperty rdf:resource="http://cybox.mitre.org/objects/File#optionalHeader.sizeOfHeapReserve"/>
	<owl:maxCardinality rdf:datatype="http://www.w3.org/2001/XMLSchema#nonNegativeInteger">1</owl:maxCardinality>
</rdf:Description>

<rdf:Description rdf:about="http://cybox.mitre.org/objects/File#PEHeaders">
	<rdfs:subClassOf rdf:nodeID="genid253"/>
</rdf:Description>

<rdf:Description rdf:nodeID="genid253">
	<rdf:type rdf:resource="http://www.w3.org/2002/07/owl#Restriction"/>
	<owl:onProperty rdf:resource="http://cybox.mitre.org/objects/File#optionalHeader.sizeOfImage"/>
	<owl:maxCardinality rdf:datatype="http://www.w3.org/2001/XMLSchema#nonNegativeInteger">1</owl:maxCardinality>
</rdf:Description>

<rdf:Description rdf:about="http://cybox.mitre.org/objects/File#PEHeaders">
	<rdfs:subClassOf rdf:nodeID="genid254"/>
</rdf:Description>

<rdf:Description rdf:nodeID="genid254">
	<rdf:type rdf:resource="http://www.w3.org/2002/07/owl#Restriction"/>
	<owl:onProperty rdf:resource="http://cybox.mitre.org/objects/File#optionalHeader.sizeOfInitializedData"/>
	<owl:maxCardinality rdf:datatype="http://www.w3.org/2001/XMLSchema#nonNegativeInteger">1</owl:maxCardinality>
</rdf:Description>

<rdf:Description rdf:about="http://cybox.mitre.org/objects/File#PEHeaders">
	<rdfs:subClassOf rdf:nodeID="genid255"/>
</rdf:Description>

<rdf:Description rdf:nodeID="genid255">
	<rdf:type rdf:resource="http://www.w3.org/2002/07/owl#Restriction"/>
	<owl:onProperty rdf:resource="http://cybox.mitre.org/objects/File#optionalHeader.sizeOfStackCommit"/>
	<owl:maxCardinality rdf:datatype="http://www.w3.org/2001/XMLSchema#nonNegativeInteger">1</owl:maxCardinality>
</rdf:Description>

<rdf:Description rdf:about="http://cybox.mitre.org/objects/File#PEHeaders">
	<rdfs:subClassOf rdf:nodeID="genid256"/>
</rdf:Description>

<rdf:Description rdf:nodeID="genid256">
	<rdf:type rdf:resource="http://www.w3.org/2002/07/owl#Restriction"/>
	<owl:onProperty rdf:resource="http://cybox.mitre.org/objects/File#optionalHeader.sizeOfStackReserve"/>
	<owl:maxCardinality rdf:datatype="http://www.w3.org/2001/XMLSchema#nonNegativeInteger">1</owl:maxCardinality>
</rdf:Description>

<rdf:Description rdf:about="http://cybox.mitre.org/objects/File#PEHeaders">
	<rdfs:subClassOf rdf:nodeID="genid257"/>
</rdf:Description>

<rdf:Description rdf:nodeID="genid257">
	<rdf:type rdf:resource="http://www.w3.org/2002/07/owl#Restriction"/>
	<owl:onProperty rdf:resource="http://cybox.mitre.org/objects/File#optionalHeader.sizeOfUninitializedData"/>
	<owl:maxCardinality rdf:datatype="http://www.w3.org/2001/XMLSchema#nonNegativeInteger">1</owl:maxCardinality>
</rdf:Description>

<rdf:Description rdf:about="http://cybox.mitre.org/objects/File#PEHeaders">
	<rdfs:subClassOf rdf:nodeID="genid258"/>
</rdf:Description>

<rdf:Description rdf:nodeID="genid258">
	<rdf:type rdf:resource="http://www.w3.org/2002/07/owl#Restriction"/>
	<owl:onProperty rdf:resource="http://cybox.mitre.org/objects/File#optionalHeader.subsystem"/>
	<owl:maxCardinality rdf:datatype="http://www.w3.org/2001/XMLSchema#nonNegativeInteger">1</owl:maxCardinality>
</rdf:Description>

<rdf:Description rdf:about="http://cybox.mitre.org/objects/File#PEHeaders">
	<rdfs:subClassOf rdf:nodeID="genid259"/>
</rdf:Description>

<rdf:Description rdf:nodeID="genid259">
	<rdf:type rdf:resource="http://www.w3.org/2002/07/owl#Restriction"/>
	<owl:onProperty rdf:resource="http://cybox.mitre.org/objects/File#optionalHeader.win32VersionValue"/>
	<owl:maxCardinality rdf:datatype="http://www.w3.org/2001/XMLSchema#nonNegativeInteger">1</owl:maxCardinality>
</rdf:Description>

<rdf:Description rdf:about="http://cybox.mitre.org/objects/File#PEHeaders">
	<rdfs:subClassOf rdf:nodeID="genid260"/>
</rdf:Description>

<rdf:Description rdf:nodeID="genid260">
	<rdf:type rdf:resource="http://www.w3.org/2002/07/owl#Restriction"/>
	<owl:onProperty rdf:resource="http://cybox.mitre.org/objects/File#peSignature"/>
	<owl:maxCardinality rdf:datatype="http://www.w3.org/2001/XMLSchema#nonNegativeInteger">1</owl:maxCardinality>
</rdf:Description>

<rdf:Description rdf:about="http://cybox.mitre.org/objects/File#PEHeaders">
	<rdfs:comment>Characterizes the headers found in PE and COFF files.</rdfs:comment>
	<rdfs:isDefinedBy rdf:resource="http://cybox.mitre.org/objects/File"/>
	<rdfs:label>PEHeaders</rdfs:label>
</rdf:Description>
<!--  -->
<!-- http://cybox.mitre.org/objects/File#PEImport -->

<rdf:Description rdf:about="http://cybox.mitre.org/objects/File#PEImport">
	<rdf:type rdf:resource="http://www.w3.org/2002/07/owl#Class"/>
	<rdfs:subClassOf rdf:nodeID="genid261"/>
</rdf:Description>

<rdf:Description rdf:nodeID="genid261">
	<rdf:type rdf:resource="http://www.w3.org/2002/07/owl#Restriction"/>
	<owl:onProperty rdf:resource="http://cybox.mitre.org/objects/File#importFile"/>
	<owl:maxCardinality rdf:datatype="http://www.w3.org/2001/XMLSchema#nonNegativeInteger">1</owl:maxCardinality>
</rdf:Description>

<rdf:Description rdf:about="http://cybox.mitre.org/objects/File#PEImport">
	<rdfs:subClassOf rdf:nodeID="genid262"/>
</rdf:Description>

<rdf:Description rdf:nodeID="genid262">
	<rdf:type rdf:resource="http://www.w3.org/2002/07/owl#Restriction"/>
	<owl:onProperty rdf:resource="http://cybox.mitre.org/objects/File#delayLoad"/>
	<owl:maxCardinality rdf:datatype="http://www.w3.org/2001/XMLSchema#nonNegativeInteger">1</owl:maxCardinality>
</rdf:Description>

<rdf:Description rdf:about="http://cybox.mitre.org/objects/File#PEImport">
	<rdfs:subClassOf rdf:nodeID="genid263"/>
</rdf:Description>

<rdf:Description rdf:nodeID="genid263">
	<rdf:type rdf:resource="http://www.w3.org/2002/07/owl#Restriction"/>
	<owl:onProperty rdf:resource="http://cybox.mitre.org/objects/File#importFileName"/>
	<owl:maxCardinality rdf:datatype="http://www.w3.org/2001/XMLSchema#nonNegativeInteger">1</owl:maxCardinality>
</rdf:Description>

<rdf:Description rdf:about="http://cybox.mitre.org/objects/File#PEImport">
	<rdfs:subClassOf rdf:nodeID="genid264"/>
</rdf:Description>

<rdf:Description rdf:nodeID="genid264">
	<rdf:type rdf:resource="http://www.w3.org/2002/07/owl#Restriction"/>
	<owl:onProperty rdf:resource="http://cybox.mitre.org/objects/File#importVirtualAddress"/>
	<owl:maxCardinality rdf:datatype="http://www.w3.org/2001/XMLSchema#nonNegativeInteger">1</owl:maxCardinality>
</rdf:Description>

<rdf:Description rdf:about="http://cybox.mitre.org/objects/File#PEImport">
	<rdfs:subClassOf rdf:nodeID="genid265"/>
</rdf:Description>

<rdf:Description rdf:nodeID="genid265">
	<rdf:type rdf:resource="http://www.w3.org/2002/07/owl#Restriction"/>
	<owl:onProperty rdf:resource="http://cybox.mitre.org/objects/File#initiallyVisible"/>
	<owl:maxCardinality rdf:datatype="http://www.w3.org/2001/XMLSchema#nonNegativeInteger">1</owl:maxCardinality>
</rdf:Description>

<rdf:Description rdf:about="http://cybox.mitre.org/objects/File#PEImport">
	<rdfs:comment>Characterizes the properties relevant to PE binary imports.</rdfs:comment>
	<rdfs:isDefinedBy rdf:resource="http://cybox.mitre.org/objects/File"/>
	<rdfs:label>PEImport</rdfs:label>
</rdf:Description>
<!--  -->
<!-- http://cybox.mitre.org/objects/File#PEImportedFunction -->

<rdf:Description rdf:about="http://cybox.mitre.org/objects/File#PEImportedFunction">
	<rdf:type rdf:resource="http://www.w3.org/2002/07/owl#Class"/>
	<rdfs:subClassOf rdf:nodeID="genid266"/>
</rdf:Description>

<rdf:Description rdf:nodeID="genid266">
	<rdf:type rdf:resource="http://www.w3.org/2002/07/owl#Restriction"/>
	<owl:onProperty rdf:resource="http://cybox.mitre.org/objects/File#functionName"/>
	<owl:cardinality rdf:datatype="http://www.w3.org/2001/XMLSchema#nonNegativeInteger">1</owl:cardinality>
</rdf:Description>

<rdf:Description rdf:about="http://cybox.mitre.org/objects/File#PEImportedFunction">
	<rdfs:subClassOf rdf:nodeID="genid267"/>
</rdf:Description>

<rdf:Description rdf:nodeID="genid267">
	<rdf:type rdf:resource="http://www.w3.org/2002/07/owl#Restriction"/>
	<owl:onProperty rdf:resource="http://cybox.mitre.org/objects/File#bound"/>
	<owl:maxCardinality rdf:datatype="http://www.w3.org/2001/XMLSchema#nonNegativeInteger">1</owl:maxCardinality>
</rdf:Description>

<rdf:Description rdf:about="http://cybox.mitre.org/objects/File#PEImportedFunction">
	<rdfs:subClassOf rdf:nodeID="genid268"/>
</rdf:Description>

<rdf:Description rdf:nodeID="genid268">
	<rdf:type rdf:resource="http://www.w3.org/2002/07/owl#Restriction"/>
	<owl:onProperty rdf:resource="http://cybox.mitre.org/objects/File#hint"/>
	<owl:maxCardinality rdf:datatype="http://www.w3.org/2001/XMLSchema#nonNegativeInteger">1</owl:maxCardinality>
</rdf:Description>

<rdf:Description rdf:about="http://cybox.mitre.org/objects/File#PEImportedFunction">
	<rdfs:subClassOf rdf:nodeID="genid269"/>
</rdf:Description>

<rdf:Description rdf:nodeID="genid269">
	<rdf:type rdf:resource="http://www.w3.org/2002/07/owl#Restriction"/>
	<owl:onProperty rdf:resource="http://cybox.mitre.org/objects/File#importOrdinal"/>
	<owl:maxCardinality rdf:datatype="http://www.w3.org/2001/XMLSchema#nonNegativeInteger">1</owl:maxCardinality>
</rdf:Description>

<rdf:Description rdf:about="http://cybox.mitre.org/objects/File#PEImportedFunction">
	<rdfs:subClassOf rdf:nodeID="genid270"/>
</rdf:Description>

<rdf:Description rdf:nodeID="genid270">
	<rdf:type rdf:resource="http://www.w3.org/2002/07/owl#Restriction"/>
	<owl:onProperty rdf:resource="http://cybox.mitre.org/objects/File#virtualAddress"/>
	<owl:maxCardinality rdf:datatype="http://www.w3.org/2001/XMLSchema#nonNegativeInteger">1</owl:maxCardinality>
</rdf:Description>

<rdf:Description rdf:about="http://cybox.mitre.org/objects/File#PEImportedFunction">
	<rdfs:comment>Characterizes  imported functions.</rdfs:comment>
	<rdfs:isDefinedBy rdf:resource="http://cybox.mitre.org/objects/File"/>
	<rdfs:label>PEImported function</rdfs:label>
</rdf:Description>
<!--  -->
<!-- http://cybox.mitre.org/objects/File#PEResource -->

<rdf:Description rdf:about="http://cybox.mitre.org/objects/File#PEResource">
	<rdf:type rdf:resource="http://www.w3.org/2002/07/owl#Class"/>
	<rdfs:subClassOf rdf:nodeID="genid271"/>
</rdf:Description>

<rdf:Description rdf:nodeID="genid271">
	<rdf:type rdf:resource="http://www.w3.org/2002/07/owl#Restriction"/>
	<owl:onProperty rdf:resource="http://cybox.mitre.org/objects/File#resourceName"/>
	<owl:cardinality rdf:datatype="http://www.w3.org/2001/XMLSchema#nonNegativeInteger">1</owl:cardinality>
</rdf:Description>

<rdf:Description rdf:about="http://cybox.mitre.org/objects/File#PEResource">
	<rdfs:subClassOf rdf:nodeID="genid272"/>
</rdf:Description>

<rdf:Description rdf:nodeID="genid272">
	<rdf:type rdf:resource="http://www.w3.org/2002/07/owl#Restriction"/>
	<owl:onProperty rdf:resource="http://cybox.mitre.org/objects/File#resourceType"/>
	<owl:cardinality rdf:datatype="http://www.w3.org/2001/XMLSchema#nonNegativeInteger">1</owl:cardinality>
</rdf:Description>

<rdf:Description rdf:about="http://cybox.mitre.org/objects/File#PEResource">
	<rdfs:subClassOf rdf:nodeID="genid273"/>
</rdf:Description>

<rdf:Description rdf:nodeID="genid273">
	<rdf:type rdf:resource="http://www.w3.org/2002/07/owl#Restriction"/>
	<owl:onProperty rdf:resource="http://cybox.mitre.org/objects/File#language"/>
	<owl:maxCardinality rdf:datatype="http://www.w3.org/2001/XMLSchema#nonNegativeInteger">1</owl:maxCardinality>
</rdf:Description>

<rdf:Description rdf:about="http://cybox.mitre.org/objects/File#PEResource">
	<rdfs:subClassOf rdf:nodeID="genid274"/>
</rdf:Description>

<rdf:Description rdf:nodeID="genid274">
	<rdf:type rdf:resource="http://www.w3.org/2002/07/owl#Restriction"/>
	<owl:onProperty rdf:resource="http://cybox.mitre.org/objects/File#resourceData"/>
	<owl:maxCardinality rdf:datatype="http://www.w3.org/2001/XMLSchema#nonNegativeInteger">1</owl:maxCardinality>
</rdf:Description>

<rdf:Description rdf:about="http://cybox.mitre.org/objects/File#PEResource">
	<rdfs:subClassOf rdf:nodeID="genid275"/>
</rdf:Description>

<rdf:Description rdf:nodeID="genid275">
	<rdf:type rdf:resource="http://www.w3.org/2002/07/owl#Restriction"/>
	<owl:onProperty rdf:resource="http://cybox.mitre.org/objects/File#resourceSize"/>
	<owl:maxCardinality rdf:datatype="http://www.w3.org/2001/XMLSchema#nonNegativeInteger">1</owl:maxCardinality>
</rdf:Description>

<rdf:Description rdf:about="http://cybox.mitre.org/objects/File#PEResource">
	<rdfs:subClassOf rdf:nodeID="genid276"/>
</rdf:Description>

<rdf:Description rdf:nodeID="genid276">
	<rdf:type rdf:resource="http://www.w3.org/2002/07/owl#Restriction"/>
	<owl:onProperty rdf:resource="http://cybox.mitre.org/objects/File#subLanguage"/>
	<owl:maxCardinality rdf:datatype="http://www.w3.org/2001/XMLSchema#nonNegativeInteger">1</owl:maxCardinality>
</rdf:Description>

<rdf:Description rdf:about="http://cybox.mitre.org/objects/File#PEResource">
	<rdfs:subClassOf rdf:nodeID="genid277"/>
</rdf:Description>

<rdf:Description rdf:nodeID="genid277">
	<rdf:type rdf:resource="http://www.w3.org/2002/07/owl#Restriction"/>
	<owl:onProperty rdf:resource="http://cybox.mitre.org/objects/File#virtualAddress"/>
	<owl:maxCardinality rdf:datatype="http://www.w3.org/2001/XMLSchema#nonNegativeInteger">1</owl:maxCardinality>
</rdf:Description>

<rdf:Description rdf:about="http://cybox.mitre.org/objects/File#PEResource">
	<rdfs:comment>Characterizes the properties relevant to PE binary resources.</rdfs:comment>
	<rdfs:isDefinedBy rdf:resource="http://cybox.mitre.org/objects/File"/>
	<rdfs:label>PEResource</rdfs:label>
</rdf:Description>
<!--  -->
<!-- http://cybox.mitre.org/objects/File#PESection -->

<rdf:Description rdf:about="http://cybox.mitre.org/objects/File#PESection">
	<rdf:type rdf:resource="http://www.w3.org/2002/07/owl#Class"/>
	<rdfs:subClassOf rdf:nodeID="genid278"/>
</rdf:Description>

<rdf:Description rdf:nodeID="genid278">
	<rdf:type rdf:resource="http://www.w3.org/2002/07/owl#Restriction"/>
	<owl:onProperty rdf:resource="http://cybox.mitre.org/objects/File#entropy.max"/>
	<owl:maxCardinality rdf:datatype="http://www.w3.org/2001/XMLSchema#nonNegativeInteger">1</owl:maxCardinality>
</rdf:Description>

<rdf:Description rdf:about="http://cybox.mitre.org/objects/File#PESection">
	<rdfs:subClassOf rdf:nodeID="genid279"/>
</rdf:Description>

<rdf:Description rdf:nodeID="genid279">
	<rdf:type rdf:resource="http://www.w3.org/2002/07/owl#Restriction"/>
	<owl:onProperty rdf:resource="http://cybox.mitre.org/objects/File#entropy.min"/>
	<owl:maxCardinality rdf:datatype="http://www.w3.org/2001/XMLSchema#nonNegativeInteger">1</owl:maxCardinality>
</rdf:Description>

<rdf:Description rdf:about="http://cybox.mitre.org/objects/File#PESection">
	<rdfs:subClassOf rdf:nodeID="genid280"/>
</rdf:Description>

<rdf:Description rdf:nodeID="genid280">
	<rdf:type rdf:resource="http://www.w3.org/2002/07/owl#Restriction"/>
	<owl:onProperty rdf:resource="http://cybox.mitre.org/objects/File#entropy.value"/>
	<owl:maxCardinality rdf:datatype="http://www.w3.org/2001/XMLSchema#nonNegativeInteger">1</owl:maxCardinality>
</rdf:Description>

<rdf:Description rdf:about="http://cybox.mitre.org/objects/File#PESection">
	<rdfs:subClassOf rdf:nodeID="genid281"/>
</rdf:Description>

<rdf:Description rdf:nodeID="genid281">
	<rdf:type rdf:resource="http://www.w3.org/2002/07/owl#Restriction"/>
	<owl:onProperty rdf:resource="http://cybox.mitre.org/objects/File#sectionHeader.characteristics"/>
	<owl:maxCardinality rdf:datatype="http://www.w3.org/2001/XMLSchema#nonNegativeInteger">1</owl:maxCardinality>
</rdf:Description>

<rdf:Description rdf:about="http://cybox.mitre.org/objects/File#PESection">
	<rdfs:subClassOf rdf:nodeID="genid282"/>
</rdf:Description>

<rdf:Description rdf:nodeID="genid282">
	<rdf:type rdf:resource="http://www.w3.org/2002/07/owl#Restriction"/>
	<owl:onProperty rdf:resource="http://cybox.mitre.org/objects/File#sectionHeader.name"/>
	<owl:maxCardinality rdf:datatype="http://www.w3.org/2001/XMLSchema#nonNegativeInteger">1</owl:maxCardinality>
</rdf:Description>

<rdf:Description rdf:about="http://cybox.mitre.org/objects/File#PESection">
	<rdfs:subClassOf rdf:nodeID="genid283"/>
</rdf:Description>

<rdf:Description rdf:nodeID="genid283">
	<rdf:type rdf:resource="http://www.w3.org/2002/07/owl#Restriction"/>
	<owl:onProperty rdf:resource="http://cybox.mitre.org/objects/File#sectionHeader.numberOfLinenumbers"/>
	<owl:maxCardinality rdf:datatype="http://www.w3.org/2001/XMLSchema#nonNegativeInteger">1</owl:maxCardinality>
</rdf:Description>

<rdf:Description rdf:about="http://cybox.mitre.org/objects/File#PESection">
	<rdfs:subClassOf rdf:nodeID="genid284"/>
</rdf:Description>

<rdf:Description rdf:nodeID="genid284">
	<rdf:type rdf:resource="http://www.w3.org/2002/07/owl#Restriction"/>
	<owl:onProperty rdf:resource="http://cybox.mitre.org/objects/File#sectionHeader.numberOfRelocations"/>
	<owl:maxCardinality rdf:datatype="http://www.w3.org/2001/XMLSchema#nonNegativeInteger">1</owl:maxCardinality>
</rdf:Description>

<rdf:Description rdf:about="http://cybox.mitre.org/objects/File#PESection">
	<rdfs:subClassOf rdf:nodeID="genid285"/>
</rdf:Description>

<rdf:Description rdf:nodeID="genid285">
	<rdf:type rdf:resource="http://www.w3.org/2002/07/owl#Restriction"/>
	<owl:onProperty rdf:resource="http://cybox.mitre.org/objects/File#sectionHeader.pointerToLinenumbers"/>
	<owl:maxCardinality rdf:datatype="http://www.w3.org/2001/XMLSchema#nonNegativeInteger">1</owl:maxCardinality>
</rdf:Description>

<rdf:Description rdf:about="http://cybox.mitre.org/objects/File#PESection">
	<rdfs:subClassOf rdf:nodeID="genid286"/>
</rdf:Description>

<rdf:Description rdf:nodeID="genid286">
	<rdf:type rdf:resource="http://www.w3.org/2002/07/owl#Restriction"/>
	<owl:onProperty rdf:resource="http://cybox.mitre.org/objects/File#sectionHeader.pointerToRawData"/>
	<owl:maxCardinality rdf:datatype="http://www.w3.org/2001/XMLSchema#nonNegativeInteger">1</owl:maxCardinality>
</rdf:Description>

<rdf:Description rdf:about="http://cybox.mitre.org/objects/File#PESection">
	<rdfs:subClassOf rdf:nodeID="genid287"/>
</rdf:Description>

<rdf:Description rdf:nodeID="genid287">
	<rdf:type rdf:resource="http://www.w3.org/2002/07/owl#Restriction"/>
	<owl:onProperty rdf:resource="http://cybox.mitre.org/objects/File#sectionHeader.pointerToRelocations"/>
	<owl:maxCardinality rdf:datatype="http://www.w3.org/2001/XMLSchema#nonNegativeInteger">1</owl:maxCardinality>
</rdf:Description>

<rdf:Description rdf:about="http://cybox.mitre.org/objects/File#PESection">
	<rdfs:subClassOf rdf:nodeID="genid288"/>
</rdf:Description>

<rdf:Description rdf:nodeID="genid288">
	<rdf:type rdf:resource="http://www.w3.org/2002/07/owl#Restriction"/>
	<owl:onProperty rdf:resource="http://cybox.mitre.org/objects/File#sectionHeader.sizeOfRawData"/>
	<owl:maxCardinality rdf:datatype="http://www.w3.org/2001/XMLSchema#nonNegativeInteger">1</owl:maxCardinality>
</rdf:Description>

<rdf:Description rdf:about="http://cybox.mitre.org/objects/File#PESection">
	<rdfs:subClassOf rdf:nodeID="genid289"/>
</rdf:Description>

<rdf:Description rdf:nodeID="genid289">
	<rdf:type rdf:resource="http://www.w3.org/2002/07/owl#Restriction"/>
	<owl:onProperty rdf:resource="http://cybox.mitre.org/objects/File#sectionHeader.virtualAddress"/>
	<owl:maxCardinality rdf:datatype="http://www.w3.org/2001/XMLSchema#nonNegativeInteger">1</owl:maxCardinality>
</rdf:Description>

<rdf:Description rdf:about="http://cybox.mitre.org/objects/File#PESection">
	<rdfs:subClassOf rdf:nodeID="genid290"/>
</rdf:Description>

<rdf:Description rdf:nodeID="genid290">
	<rdf:type rdf:resource="http://www.w3.org/2002/07/owl#Restriction"/>
	<owl:onProperty rdf:resource="http://cybox.mitre.org/objects/File#sectionHeader.virtualSize"/>
	<owl:maxCardinality rdf:datatype="http://www.w3.org/2001/XMLSchema#nonNegativeInteger">1</owl:maxCardinality>
</rdf:Description>

<rdf:Description rdf:about="http://cybox.mitre.org/objects/File#PESection">
	<rdfs:comment>Characterizes the properties relevant to PE binary sections. &#xD;
&#xD;
A PE Section consists of a header and data. The PESectionType contains properties that describe the Section Header and metadata computed about the section (e.g., hashes, entropy).</rdfs:comment>
	<rdfs:isDefinedBy rdf:resource="http://cybox.mitre.org/objects/File"/>
	<rdfs:label>PESection</rdfs:label>
</rdf:Description>
<!--  -->
<!-- http://cybox.mitre.org/objects/File#PEVersionResource -->

<rdf:Description rdf:about="http://cybox.mitre.org/objects/File#PEVersionResource">
	<rdf:type rdf:resource="http://www.w3.org/2002/07/owl#Class"/>
	<rdfs:subClassOf rdf:resource="http://cybox.mitre.org/objects/File#PEResource"/>
	<rdfs:subClassOf rdf:nodeID="genid291"/>
</rdf:Description>

<rdf:Description rdf:nodeID="genid291">
	<rdf:type rdf:resource="http://www.w3.org/2002/07/owl#Restriction"/>
	<owl:onProperty rdf:resource="http://cybox.mitre.org/objects/File#comments"/>
	<owl:maxCardinality rdf:datatype="http://www.w3.org/2001/XMLSchema#nonNegativeInteger">1</owl:maxCardinality>
</rdf:Description>

<rdf:Description rdf:about="http://cybox.mitre.org/objects/File#PEVersionResource">
	<rdfs:subClassOf rdf:nodeID="genid292"/>
</rdf:Description>

<rdf:Description rdf:nodeID="genid292">
	<rdf:type rdf:resource="http://www.w3.org/2002/07/owl#Restriction"/>
	<owl:onProperty rdf:resource="http://cybox.mitre.org/objects/File#companyName"/>
	<owl:maxCardinality rdf:datatype="http://www.w3.org/2001/XMLSchema#nonNegativeInteger">1</owl:maxCardinality>
</rdf:Description>

<rdf:Description rdf:about="http://cybox.mitre.org/objects/File#PEVersionResource">
	<rdfs:subClassOf rdf:nodeID="genid293"/>
</rdf:Description>

<rdf:Description rdf:nodeID="genid293">
	<rdf:type rdf:resource="http://www.w3.org/2002/07/owl#Restriction"/>
	<owl:onProperty rdf:resource="http://cybox.mitre.org/objects/File#fileDescription"/>
	<owl:maxCardinality rdf:datatype="http://www.w3.org/2001/XMLSchema#nonNegativeInteger">1</owl:maxCardinality>
</rdf:Description>

<rdf:Description rdf:about="http://cybox.mitre.org/objects/File#PEVersionResource">
	<rdfs:subClassOf rdf:nodeID="genid294"/>
</rdf:Description>

<rdf:Description rdf:nodeID="genid294">
	<rdf:type rdf:resource="http://www.w3.org/2002/07/owl#Restriction"/>
	<owl:onProperty rdf:resource="http://cybox.mitre.org/objects/File#fileVersion"/>
	<owl:maxCardinality rdf:datatype="http://www.w3.org/2001/XMLSchema#nonNegativeInteger">1</owl:maxCardinality>
</rdf:Description>

<rdf:Description rdf:about="http://cybox.mitre.org/objects/File#PEVersionResource">
	<rdfs:subClassOf rdf:nodeID="genid295"/>
</rdf:Description>

<rdf:Description rdf:nodeID="genid295">
	<rdf:type rdf:resource="http://www.w3.org/2002/07/owl#Restriction"/>
	<owl:onProperty rdf:resource="http://cybox.mitre.org/objects/File#internalName"/>
	<owl:maxCardinality rdf:datatype="http://www.w3.org/2001/XMLSchema#nonNegativeInteger">1</owl:maxCardinality>
</rdf:Description>

<rdf:Description rdf:about="http://cybox.mitre.org/objects/File#PEVersionResource">
	<rdfs:subClassOf rdf:nodeID="genid296"/>
</rdf:Description>

<rdf:Description rdf:nodeID="genid296">
	<rdf:type rdf:resource="http://www.w3.org/2002/07/owl#Restriction"/>
	<owl:onProperty rdf:resource="http://cybox.mitre.org/objects/File#langID"/>
	<owl:maxCardinality rdf:datatype="http://www.w3.org/2001/XMLSchema#nonNegativeInteger">1</owl:maxCardinality>
</rdf:Description>

<rdf:Description rdf:about="http://cybox.mitre.org/objects/File#PEVersionResource">
	<rdfs:subClassOf rdf:nodeID="genid297"/>
</rdf:Description>

<rdf:Description rdf:nodeID="genid297">
	<rdf:type rdf:resource="http://www.w3.org/2002/07/owl#Restriction"/>
	<owl:onProperty rdf:resource="http://cybox.mitre.org/objects/File#legalCopyright"/>
	<owl:maxCardinality rdf:datatype="http://www.w3.org/2001/XMLSchema#nonNegativeInteger">1</owl:maxCardinality>
</rdf:Description>

<rdf:Description rdf:about="http://cybox.mitre.org/objects/File#PEVersionResource">
	<rdfs:subClassOf rdf:nodeID="genid298"/>
</rdf:Description>

<rdf:Description rdf:nodeID="genid298">
	<rdf:type rdf:resource="http://www.w3.org/2002/07/owl#Restriction"/>
	<owl:onProperty rdf:resource="http://cybox.mitre.org/objects/File#legalTrademarks"/>
	<owl:maxCardinality rdf:datatype="http://www.w3.org/2001/XMLSchema#nonNegativeInteger">1</owl:maxCardinality>
</rdf:Description>

<rdf:Description rdf:about="http://cybox.mitre.org/objects/File#PEVersionResource">
	<rdfs:subClassOf rdf:nodeID="genid299"/>
</rdf:Description>

<rdf:Description rdf:nodeID="genid299">
	<rdf:type rdf:resource="http://www.w3.org/2002/07/owl#Restriction"/>
	<owl:onProperty rdf:resource="http://cybox.mitre.org/objects/File#originalFilename"/>
	<owl:maxCardinality rdf:datatype="http://www.w3.org/2001/XMLSchema#nonNegativeInteger">1</owl:maxCardinality>
</rdf:Description>

<rdf:Description rdf:about="http://cybox.mitre.org/objects/File#PEVersionResource">
	<rdfs:subClassOf rdf:nodeID="genid300"/>
</rdf:Description>

<rdf:Description rdf:nodeID="genid300">
	<rdf:type rdf:resource="http://www.w3.org/2002/07/owl#Restriction"/>
	<owl:onProperty rdf:resource="http://cybox.mitre.org/objects/File#privateBuild"/>
	<owl:maxCardinality rdf:datatype="http://www.w3.org/2001/XMLSchema#nonNegativeInteger">1</owl:maxCardinality>
</rdf:Description>

<rdf:Description rdf:about="http://cybox.mitre.org/objects/File#PEVersionResource">
	<rdfs:subClassOf rdf:nodeID="genid301"/>
</rdf:Description>

<rdf:Description rdf:nodeID="genid301">
	<rdf:type rdf:resource="http://www.w3.org/2002/07/owl#Restriction"/>
	<owl:onProperty rdf:resource="http://cybox.mitre.org/objects/File#productName"/>
	<owl:maxCardinality rdf:datatype="http://www.w3.org/2001/XMLSchema#nonNegativeInteger">1</owl:maxCardinality>
</rdf:Description>

<rdf:Description rdf:about="http://cybox.mitre.org/objects/File#PEVersionResource">
	<rdfs:subClassOf rdf:nodeID="genid302"/>
</rdf:Description>

<rdf:Description rdf:nodeID="genid302">
	<rdf:type rdf:resource="http://www.w3.org/2002/07/owl#Restriction"/>
	<owl:onProperty rdf:resource="http://cybox.mitre.org/objects/File#productVersion"/>
	<owl:maxCardinality rdf:datatype="http://www.w3.org/2001/XMLSchema#nonNegativeInteger">1</owl:maxCardinality>
</rdf:Description>

<rdf:Description rdf:about="http://cybox.mitre.org/objects/File#PEVersionResource">
	<rdfs:subClassOf rdf:nodeID="genid303"/>
</rdf:Description>

<rdf:Description rdf:nodeID="genid303">
	<rdf:type rdf:resource="http://www.w3.org/2002/07/owl#Restriction"/>
	<owl:onProperty rdf:resource="http://cybox.mitre.org/objects/File#specialBuild"/>
	<owl:maxCardinality rdf:datatype="http://www.w3.org/2001/XMLSchema#nonNegativeInteger">1</owl:maxCardinality>
</rdf:Description>

<rdf:Description rdf:about="http://cybox.mitre.org/objects/File#PEVersionResource">
	<rdfs:comment>Characterizes the special VERSIONINFO resource type. For more information please see: http://msdn.microsoft.com/en-us/library/windows/desktop/aa381058(v=vs.85).aspx.</rdfs:comment>
	<rdfs:isDefinedBy rdf:resource="http://cybox.mitre.org/objects/File"/>
	<rdfs:label>PE VERSIONINFO Resource</rdfs:label>
</rdf:Description>
<!--  -->
<!-- http://cybox.mitre.org/objects/File#Packer -->

<rdf:Description rdf:about="http://cybox.mitre.org/objects/File#Packer">
	<rdf:type rdf:resource="http://www.w3.org/2002/07/owl#Class"/>
</rdf:Description>


<rdf:Description rdf:about="http://cybox.mitre.org/objects/File#Packer">
	<rdfs:subClassOf rdf:nodeID="genid304"/>
</rdf:Description>

<rdf:Description rdf:nodeID="genid304">
	<rdf:type rdf:resource="http://www.w3.org/2002/07/owl#Restriction"/>
	<owl:onProperty rdf:resource="http://cybox.mitre.org/objects/File#packerName"/>
	<owl:cardinality rdf:datatype="http://www.w3.org/2001/XMLSchema#nonNegativeInteger">1</owl:cardinality>
</rdf:Description>

<rdf:Description rdf:about="http://cybox.mitre.org/objects/File#Packer">
	<rdfs:subClassOf rdf:nodeID="genid305"/>
</rdf:Description>

<rdf:Description rdf:nodeID="genid305">
	<rdf:type rdf:resource="http://www.w3.org/2002/07/owl#Restriction"/>
	<owl:onProperty rdf:resource="http://cybox.mitre.org/objects/File#entryPoint"/>
	<owl:maxCardinality rdf:datatype="http://www.w3.org/2001/XMLSchema#nonNegativeInteger">1</owl:maxCardinality>
</rdf:Description>

<rdf:Description rdf:about="http://cybox.mitre.org/objects/File#Packer">
	<rdfs:subClassOf rdf:nodeID="genid306"/>
</rdf:Description>

<rdf:Description rdf:nodeID="genid306">
	<rdf:type rdf:resource="http://www.w3.org/2002/07/owl#Restriction"/>
	<owl:onProperty rdf:resource="http://cybox.mitre.org/objects/File#epJumpCode.depth"/>
	<owl:maxCardinality rdf:datatype="http://www.w3.org/2001/XMLSchema#nonNegativeInteger">1</owl:maxCardinality>
</rdf:Description>

<rdf:Description rdf:about="http://cybox.mitre.org/objects/File#Packer">
	<rdfs:subClassOf rdf:nodeID="genid307"/>
</rdf:Description>

<rdf:Description rdf:nodeID="genid307">
	<rdf:type rdf:resource="http://www.w3.org/2002/07/owl#Restriction"/>
	<owl:onProperty rdf:resource="http://cybox.mitre.org/objects/File#epJumpCode.opCodes"/>
	<owl:maxCardinality rdf:datatype="http://www.w3.org/2001/XMLSchema#nonNegativeInteger">1</owl:maxCardinality>
</rdf:Description>

<rdf:Description rdf:about="http://cybox.mitre.org/objects/File#Packer">
	<rdfs:subClassOf rdf:nodeID="genid308"/>
</rdf:Description>

<rdf:Description rdf:nodeID="genid308">
	<rdf:type rdf:resource="http://www.w3.org/2002/07/owl#Restriction"/>
	<owl:onProperty rdf:resource="http://cybox.mitre.org/objects/File#packerType"/>
	<owl:maxCardinality rdf:datatype="http://www.w3.org/2001/XMLSchema#nonNegativeInteger">1</owl:maxCardinality>
</rdf:Description>

<rdf:Description rdf:about="http://cybox.mitre.org/objects/File#Packer">
	<rdfs:subClassOf rdf:nodeID="genid309"/>
</rdf:Description>

<rdf:Description rdf:nodeID="genid309">
	<rdf:type rdf:resource="http://www.w3.org/2002/07/owl#Restriction"/>
	<owl:onProperty rdf:resource="http://cybox.mitre.org/objects/File#packerVersion"/>
	<owl:maxCardinality rdf:datatype="http://www.w3.org/2001/XMLSchema#nonNegativeInteger">1</owl:maxCardinality>
</rdf:Description>

<rdf:Description rdf:about="http://cybox.mitre.org/objects/File#Packer">
	<rdfs:subClassOf rdf:nodeID="genid310"/>
</rdf:Description>

<rdf:Description rdf:nodeID="genid310">
	<rdf:type rdf:resource="http://www.w3.org/2002/07/owl#Restriction"/>
	<owl:onProperty rdf:resource="http://cybox.mitre.org/objects/File#signature"/>
	<owl:maxCardinality rdf:datatype="http://www.w3.org/2001/XMLSchema#nonNegativeInteger">1</owl:maxCardinality>
</rdf:Description>

<rdf:Description rdf:about="http://cybox.mitre.org/objects/File#Packer">
	<rdfs:comment>Characterize a particular file packer</rdfs:comment>
	<rdfs:isDefinedBy rdf:resource="http://cybox.mitre.org/objects/File"/>
	<rdfs:label>Packer</rdfs:label>
</rdf:Description>
<!--  -->
<!-- http://cybox.mitre.org/objects/File#UnixFile -->

<rdf:Description rdf:about="http://cybox.mitre.org/objects/File#UnixFile">
	<rdf:type rdf:resource="http://www.w3.org/2002/07/owl#Class"/>
	<rdfs:subClassOf rdf:resource="http://cybox.mitre.org/objects/File#File"/>
</rdf:Description>


<rdf:Description rdf:about="http://cybox.mitre.org/objects/File#UnixFile">
	<rdfs:subClassOf rdf:nodeID="genid311"/>
</rdf:Description>

<rdf:Description rdf:nodeID="genid311">
	<rdf:type rdf:resource="http://www.w3.org/2002/07/owl#Restriction"/>
	<owl:onProperty rdf:resource="http://cybox.mitre.org/objects/File#groupOwner"/>
	<owl:maxCardinality rdf:datatype="http://www.w3.org/2001/XMLSchema#nonNegativeInteger">1</owl:maxCardinality>
</rdf:Description>

<rdf:Description rdf:about="http://cybox.mitre.org/objects/File#UnixFile">
	<rdfs:subClassOf rdf:nodeID="genid312"/>
</rdf:Description>

<rdf:Description rdf:nodeID="genid312">
	<rdf:type rdf:resource="http://www.w3.org/2002/07/owl#Restriction"/>
	<owl:onProperty rdf:resource="http://cybox.mitre.org/objects/File#iNode"/>
	<owl:maxCardinality rdf:datatype="http://www.w3.org/2001/XMLSchema#nonNegativeInteger">1</owl:maxCardinality>
</rdf:Description>

<rdf:Description rdf:about="http://cybox.mitre.org/objects/File#UnixFile">
	<rdfs:comment>Characterize Unix files.</rdfs:comment>
	<rdfs:isDefinedBy rdf:resource="http://cybox.mitre.org/objects/File"/>
	<rdfs:label>Unix file</rdfs:label>
</rdf:Description>
<!--  -->
<!-- http://cybox.mitre.org/objects/File#UnixFilePermission -->

<rdf:Description rdf:about="http://cybox.mitre.org/objects/File#UnixFilePermission">
	<rdf:type rdf:resource="http://www.w3.org/2002/07/owl#Class"/>
	<rdfs:subClassOf rdf:resource="http://cybox.mitre.org/objects/File#FilePermission"/>
	<rdfs:subClassOf rdf:nodeID="genid313"/>
</rdf:Description>

<rdf:Description rdf:nodeID="genid313">
	<rdf:type rdf:resource="http://www.w3.org/2002/07/owl#Restriction"/>
	<owl:onProperty rdf:resource="http://cybox.mitre.org/objects/File#gexec"/>
	<owl:maxCardinality rdf:datatype="http://www.w3.org/2001/XMLSchema#nonNegativeInteger">1</owl:maxCardinality>
</rdf:Description>

<rdf:Description rdf:about="http://cybox.mitre.org/objects/File#UnixFilePermission">
	<rdfs:subClassOf rdf:nodeID="genid314"/>
</rdf:Description>

<rdf:Description rdf:nodeID="genid314">
	<rdf:type rdf:resource="http://www.w3.org/2002/07/owl#Restriction"/>
	<owl:onProperty rdf:resource="http://cybox.mitre.org/objects/File#gread"/>
	<owl:maxCardinality rdf:datatype="http://www.w3.org/2001/XMLSchema#nonNegativeInteger">1</owl:maxCardinality>
</rdf:Description>

<rdf:Description rdf:about="http://cybox.mitre.org/objects/File#UnixFilePermission">
	<rdfs:subClassOf rdf:nodeID="genid315"/>
</rdf:Description>

<rdf:Description rdf:nodeID="genid315">
	<rdf:type rdf:resource="http://www.w3.org/2002/07/owl#Restriction"/>
	<owl:onProperty rdf:resource="http://cybox.mitre.org/objects/File#gwrite"/>
	<owl:maxCardinality rdf:datatype="http://www.w3.org/2001/XMLSchema#nonNegativeInteger">1</owl:maxCardinality>
</rdf:Description>

<rdf:Description rdf:about="http://cybox.mitre.org/objects/File#UnixFilePermission">
	<rdfs:subClassOf rdf:nodeID="genid316"/>
</rdf:Description>

<rdf:Description rdf:nodeID="genid316">
	<rdf:type rdf:resource="http://www.w3.org/2002/07/owl#Restriction"/>
	<owl:onProperty rdf:resource="http://cybox.mitre.org/objects/File#oexec"/>
	<owl:maxCardinality rdf:datatype="http://www.w3.org/2001/XMLSchema#nonNegativeInteger">1</owl:maxCardinality>
</rdf:Description>

<rdf:Description rdf:about="http://cybox.mitre.org/objects/File#UnixFilePermission">
	<rdfs:subClassOf rdf:nodeID="genid317"/>
</rdf:Description>

<rdf:Description rdf:nodeID="genid317">
	<rdf:type rdf:resource="http://www.w3.org/2002/07/owl#Restriction"/>
	<owl:onProperty rdf:resource="http://cybox.mitre.org/objects/File#oread"/>
	<owl:maxCardinality rdf:datatype="http://www.w3.org/2001/XMLSchema#nonNegativeInteger">1</owl:maxCardinality>
</rdf:Description>

<rdf:Description rdf:about="http://cybox.mitre.org/objects/File#UnixFilePermission">
	<rdfs:subClassOf rdf:nodeID="genid318"/>
</rdf:Description>

<rdf:Description rdf:nodeID="genid318">
	<rdf:type rdf:resource="http://www.w3.org/2002/07/owl#Restriction"/>
	<owl:onProperty rdf:resource="http://cybox.mitre.org/objects/File#owrite"/>
	<owl:maxCardinality rdf:datatype="http://www.w3.org/2001/XMLSchema#nonNegativeInteger">1</owl:maxCardinality>
</rdf:Description>

<rdf:Description rdf:about="http://cybox.mitre.org/objects/File#UnixFilePermission">
	<rdfs:subClassOf rdf:nodeID="genid319"/>
</rdf:Description>

<rdf:Description rdf:nodeID="genid319">
	<rdf:type rdf:resource="http://www.w3.org/2002/07/owl#Restriction"/>
	<owl:onProperty rdf:resource="http://cybox.mitre.org/objects/File#sgid"/>
	<owl:maxCardinality rdf:datatype="http://www.w3.org/2001/XMLSchema#nonNegativeInteger">1</owl:maxCardinality>
</rdf:Description>

<rdf:Description rdf:about="http://cybox.mitre.org/objects/File#UnixFilePermission">
	<rdfs:subClassOf rdf:nodeID="genid320"/>
</rdf:Description>

<rdf:Description rdf:nodeID="genid320">
	<rdf:type rdf:resource="http://www.w3.org/2002/07/owl#Restriction"/>
	<owl:onProperty rdf:resource="http://cybox.mitre.org/objects/File#suid"/>
	<owl:maxCardinality rdf:datatype="http://www.w3.org/2001/XMLSchema#nonNegativeInteger">1</owl:maxCardinality>
</rdf:Description>

<rdf:Description rdf:about="http://cybox.mitre.org/objects/File#UnixFilePermission">
	<rdfs:subClassOf rdf:nodeID="genid321"/>
</rdf:Description>

<rdf:Description rdf:nodeID="genid321">
	<rdf:type rdf:resource="http://www.w3.org/2002/07/owl#Restriction"/>
	<owl:onProperty rdf:resource="http://cybox.mitre.org/objects/File#uexec"/>
	<owl:maxCardinality rdf:datatype="http://www.w3.org/2001/XMLSchema#nonNegativeInteger">1</owl:maxCardinality>
</rdf:Description>

<rdf:Description rdf:about="http://cybox.mitre.org/objects/File#UnixFilePermission">
	<rdfs:subClassOf rdf:nodeID="genid322"/>
</rdf:Description>

<rdf:Description rdf:nodeID="genid322">
	<rdf:type rdf:resource="http://www.w3.org/2002/07/owl#Restriction"/>
	<owl:onProperty rdf:resource="http://cybox.mitre.org/objects/File#uread"/>
	<owl:maxCardinality rdf:datatype="http://www.w3.org/2001/XMLSchema#nonNegativeInteger">1</owl:maxCardinality>
</rdf:Description>

<rdf:Description rdf:about="http://cybox.mitre.org/objects/File#UnixFilePermission">
	<rdfs:subClassOf rdf:nodeID="genid323"/>
</rdf:Description>

<rdf:Description rdf:nodeID="genid323">
	<rdf:type rdf:resource="http://www.w3.org/2002/07/owl#Restriction"/>
	<owl:onProperty rdf:resource="http://cybox.mitre.org/objects/File#uwrite"/>
	<owl:maxCardinality rdf:datatype="http://www.w3.org/2001/XMLSchema#nonNegativeInteger">1</owl:maxCardinality>
</rdf:Description>

<rdf:Description rdf:about="http://cybox.mitre.org/objects/File#UnixFilePermission">
	<rdfs:comment>Characterizes specific permissions used by the Unix family of operating systems.</rdfs:comment>
	<rdfs:isDefinedBy rdf:resource="http://cybox.mitre.org/objects/File"/>
	<rdfs:label>Unix File Permission</rdfs:label>
</rdf:Description>
<!--  -->
<!-- http://cybox.mitre.org/objects/File#WindowsDriver -->

<rdf:Description rdf:about="http://cybox.mitre.org/objects/File#WindowsDriver">
	<rdf:type rdf:resource="http://www.w3.org/2002/07/owl#Class"/>
	<rdfs:subClassOf rdf:resource="http://cybox.mitre.org/objects/File#WindowsExecutableFile"/>
	<rdfs:subClassOf rdf:nodeID="genid324"/>
</rdf:Description>

<rdf:Description rdf:nodeID="genid324">
	<rdf:type rdf:resource="http://www.w3.org/2002/07/owl#Restriction"/>
	<owl:onProperty rdf:resource="http://cybox.mitre.org/objects/File#driverName"/>
	<owl:cardinality rdf:datatype="http://www.w3.org/2001/XMLSchema#nonNegativeInteger">1</owl:cardinality>
</rdf:Description>

<rdf:Description rdf:about="http://cybox.mitre.org/objects/File#WindowsDriver">
	<rdfs:subClassOf rdf:nodeID="genid325"/>
</rdf:Description>

<rdf:Description rdf:nodeID="genid325">
	<rdf:type rdf:resource="http://www.w3.org/2002/07/owl#Restriction"/>
	<owl:onProperty rdf:resource="http://cybox.mitre.org/objects/File#IRP_MJ_CLEANUP"/>
	<owl:maxCardinality rdf:datatype="http://www.w3.org/2001/XMLSchema#nonNegativeInteger">1</owl:maxCardinality>
</rdf:Description>

<rdf:Description rdf:about="http://cybox.mitre.org/objects/File#WindowsDriver">
	<rdfs:subClassOf rdf:nodeID="genid326"/>
</rdf:Description>

<rdf:Description rdf:nodeID="genid326">
	<rdf:type rdf:resource="http://www.w3.org/2002/07/owl#Restriction"/>
	<owl:onProperty rdf:resource="http://cybox.mitre.org/objects/File#IRP_MJ_CLOSE"/>
	<owl:maxCardinality rdf:datatype="http://www.w3.org/2001/XMLSchema#nonNegativeInteger">1</owl:maxCardinality>
</rdf:Description>

<rdf:Description rdf:about="http://cybox.mitre.org/objects/File#WindowsDriver">
	<rdfs:subClassOf rdf:nodeID="genid327"/>
</rdf:Description>

<rdf:Description rdf:nodeID="genid327">
	<rdf:type rdf:resource="http://www.w3.org/2002/07/owl#Restriction"/>
	<owl:onProperty rdf:resource="http://cybox.mitre.org/objects/File#IRP_MJ_CREATE"/>
	<owl:maxCardinality rdf:datatype="http://www.w3.org/2001/XMLSchema#nonNegativeInteger">1</owl:maxCardinality>
</rdf:Description>

<rdf:Description rdf:about="http://cybox.mitre.org/objects/File#WindowsDriver">
	<rdfs:subClassOf rdf:nodeID="genid328"/>
</rdf:Description>

<rdf:Description rdf:nodeID="genid328">
	<rdf:type rdf:resource="http://www.w3.org/2002/07/owl#Restriction"/>
	<owl:onProperty rdf:resource="http://cybox.mitre.org/objects/File#IRP_MJ_CREATE_MAILSLOT"/>
	<owl:maxCardinality rdf:datatype="http://www.w3.org/2001/XMLSchema#nonNegativeInteger">1</owl:maxCardinality>
</rdf:Description>

<rdf:Description rdf:about="http://cybox.mitre.org/objects/File#WindowsDriver">
	<rdfs:subClassOf rdf:nodeID="genid329"/>
</rdf:Description>

<rdf:Description rdf:nodeID="genid329">
	<rdf:type rdf:resource="http://www.w3.org/2002/07/owl#Restriction"/>
	<owl:onProperty rdf:resource="http://cybox.mitre.org/objects/File#IRP_MJ_CREATE_NAMED_PIPE"/>
	<owl:maxCardinality rdf:datatype="http://www.w3.org/2001/XMLSchema#nonNegativeInteger">1</owl:maxCardinality>
</rdf:Description>

<rdf:Description rdf:about="http://cybox.mitre.org/objects/File#WindowsDriver">
	<rdfs:subClassOf rdf:nodeID="genid330"/>
</rdf:Description>

<rdf:Description rdf:nodeID="genid330">
	<rdf:type rdf:resource="http://www.w3.org/2002/07/owl#Restriction"/>
	<owl:onProperty rdf:resource="http://cybox.mitre.org/objects/File#IRP_MJ_DEVICE_CHANGE"/>
	<owl:maxCardinality rdf:datatype="http://www.w3.org/2001/XMLSchema#nonNegativeInteger">1</owl:maxCardinality>
</rdf:Description>

<rdf:Description rdf:about="http://cybox.mitre.org/objects/File#WindowsDriver">
	<rdfs:subClassOf rdf:nodeID="genid331"/>
</rdf:Description>

<rdf:Description rdf:nodeID="genid331">
	<rdf:type rdf:resource="http://www.w3.org/2002/07/owl#Restriction"/>
	<owl:onProperty rdf:resource="http://cybox.mitre.org/objects/File#IRP_MJ_DEVICE_CONTROL"/>
	<owl:maxCardinality rdf:datatype="http://www.w3.org/2001/XMLSchema#nonNegativeInteger">1</owl:maxCardinality>
</rdf:Description>

<rdf:Description rdf:about="http://cybox.mitre.org/objects/File#WindowsDriver">
	<rdfs:subClassOf rdf:nodeID="genid332"/>
</rdf:Description>

<rdf:Description rdf:nodeID="genid332">
	<rdf:type rdf:resource="http://www.w3.org/2002/07/owl#Restriction"/>
	<owl:onProperty rdf:resource="http://cybox.mitre.org/objects/File#IRP_MJ_DIRECTORY_CONTROL"/>
	<owl:maxCardinality rdf:datatype="http://www.w3.org/2001/XMLSchema#nonNegativeInteger">1</owl:maxCardinality>
</rdf:Description>

<rdf:Description rdf:about="http://cybox.mitre.org/objects/File#WindowsDriver">
	<rdfs:subClassOf rdf:nodeID="genid333"/>
</rdf:Description>

<rdf:Description rdf:nodeID="genid333">
	<rdf:type rdf:resource="http://www.w3.org/2002/07/owl#Restriction"/>
	<owl:onProperty rdf:resource="http://cybox.mitre.org/objects/File#IRP_MJ_FILE_SYSTEM_CONTROL"/>
	<owl:maxCardinality rdf:datatype="http://www.w3.org/2001/XMLSchema#nonNegativeInteger">1</owl:maxCardinality>
</rdf:Description>

<rdf:Description rdf:about="http://cybox.mitre.org/objects/File#WindowsDriver">
	<rdfs:subClassOf rdf:nodeID="genid334"/>
</rdf:Description>

<rdf:Description rdf:nodeID="genid334">
	<rdf:type rdf:resource="http://www.w3.org/2002/07/owl#Restriction"/>
	<owl:onProperty rdf:resource="http://cybox.mitre.org/objects/File#IRP_MJ_FLUSH_BUFFERS"/>
	<owl:maxCardinality rdf:datatype="http://www.w3.org/2001/XMLSchema#nonNegativeInteger">1</owl:maxCardinality>
</rdf:Description>

<rdf:Description rdf:about="http://cybox.mitre.org/objects/File#WindowsDriver">
	<rdfs:subClassOf rdf:nodeID="genid335"/>
</rdf:Description>

<rdf:Description rdf:nodeID="genid335">
	<rdf:type rdf:resource="http://www.w3.org/2002/07/owl#Restriction"/>
	<owl:onProperty rdf:resource="http://cybox.mitre.org/objects/File#IRP_MJ_INTERNAL_DEVICE_CONTROL"/>
	<owl:maxCardinality rdf:datatype="http://www.w3.org/2001/XMLSchema#nonNegativeInteger">1</owl:maxCardinality>
</rdf:Description>

<rdf:Description rdf:about="http://cybox.mitre.org/objects/File#WindowsDriver">
	<rdfs:subClassOf rdf:nodeID="genid336"/>
</rdf:Description>

<rdf:Description rdf:nodeID="genid336">
	<rdf:type rdf:resource="http://www.w3.org/2002/07/owl#Restriction"/>
	<owl:onProperty rdf:resource="http://cybox.mitre.org/objects/File#IRP_MJ_LOCK_CONTROL"/>
	<owl:maxCardinality rdf:datatype="http://www.w3.org/2001/XMLSchema#nonNegativeInteger">1</owl:maxCardinality>
</rdf:Description>

<rdf:Description rdf:about="http://cybox.mitre.org/objects/File#WindowsDriver">
	<rdfs:subClassOf rdf:nodeID="genid337"/>
</rdf:Description>

<rdf:Description rdf:nodeID="genid337">
	<rdf:type rdf:resource="http://www.w3.org/2002/07/owl#Restriction"/>
	<owl:onProperty rdf:resource="http://cybox.mitre.org/objects/File#IRP_MJ_PNP"/>
	<owl:maxCardinality rdf:datatype="http://www.w3.org/2001/XMLSchema#nonNegativeInteger">1</owl:maxCardinality>
</rdf:Description>

<rdf:Description rdf:about="http://cybox.mitre.org/objects/File#WindowsDriver">
	<rdfs:subClassOf rdf:nodeID="genid338"/>
</rdf:Description>

<rdf:Description rdf:nodeID="genid338">
	<rdf:type rdf:resource="http://www.w3.org/2002/07/owl#Restriction"/>
	<owl:onProperty rdf:resource="http://cybox.mitre.org/objects/File#IRP_MJ_POWER"/>
	<owl:maxCardinality rdf:datatype="http://www.w3.org/2001/XMLSchema#nonNegativeInteger">1</owl:maxCardinality>
</rdf:Description>

<rdf:Description rdf:about="http://cybox.mitre.org/objects/File#WindowsDriver">
	<rdfs:subClassOf rdf:nodeID="genid339"/>
</rdf:Description>

<rdf:Description rdf:nodeID="genid339">
	<rdf:type rdf:resource="http://www.w3.org/2002/07/owl#Restriction"/>
	<owl:onProperty rdf:resource="http://cybox.mitre.org/objects/File#IRP_MJ_QUERY_EA"/>
	<owl:maxCardinality rdf:datatype="http://www.w3.org/2001/XMLSchema#nonNegativeInteger">1</owl:maxCardinality>
</rdf:Description>

<rdf:Description rdf:about="http://cybox.mitre.org/objects/File#WindowsDriver">
	<rdfs:subClassOf rdf:nodeID="genid340"/>
</rdf:Description>

<rdf:Description rdf:nodeID="genid340">
	<rdf:type rdf:resource="http://www.w3.org/2002/07/owl#Restriction"/>
	<owl:onProperty rdf:resource="http://cybox.mitre.org/objects/File#IRP_MJ_QUERY_QUOTA"/>
	<owl:maxCardinality rdf:datatype="http://www.w3.org/2001/XMLSchema#nonNegativeInteger">1</owl:maxCardinality>
</rdf:Description>

<rdf:Description rdf:about="http://cybox.mitre.org/objects/File#WindowsDriver">
	<rdfs:subClassOf rdf:nodeID="genid341"/>
</rdf:Description>

<rdf:Description rdf:nodeID="genid341">
	<rdf:type rdf:resource="http://www.w3.org/2002/07/owl#Restriction"/>
	<owl:onProperty rdf:resource="http://cybox.mitre.org/objects/File#IRP_MJ_QUERY_SECURITY"/>
	<owl:maxCardinality rdf:datatype="http://www.w3.org/2001/XMLSchema#nonNegativeInteger">1</owl:maxCardinality>
</rdf:Description>

<rdf:Description rdf:about="http://cybox.mitre.org/objects/File#WindowsDriver">
	<rdfs:subClassOf rdf:nodeID="genid342"/>
</rdf:Description>

<rdf:Description rdf:nodeID="genid342">
	<rdf:type rdf:resource="http://www.w3.org/2002/07/owl#Restriction"/>
	<owl:onProperty rdf:resource="http://cybox.mitre.org/objects/File#IRP_MJ_QUERY_VOLUME_INFORMATION"/>
	<owl:maxCardinality rdf:datatype="http://www.w3.org/2001/XMLSchema#nonNegativeInteger">1</owl:maxCardinality>
</rdf:Description>

<rdf:Description rdf:about="http://cybox.mitre.org/objects/File#WindowsDriver">
	<rdfs:subClassOf rdf:nodeID="genid343"/>
</rdf:Description>

<rdf:Description rdf:nodeID="genid343">
	<rdf:type rdf:resource="http://www.w3.org/2002/07/owl#Restriction"/>
	<owl:onProperty rdf:resource="http://cybox.mitre.org/objects/File#IRP_MJ_READ"/>
	<owl:maxCardinality rdf:datatype="http://www.w3.org/2001/XMLSchema#nonNegativeInteger">1</owl:maxCardinality>
</rdf:Description>

<rdf:Description rdf:about="http://cybox.mitre.org/objects/File#WindowsDriver">
	<rdfs:subClassOf rdf:nodeID="genid344"/>
</rdf:Description>

<rdf:Description rdf:nodeID="genid344">
	<rdf:type rdf:resource="http://www.w3.org/2002/07/owl#Restriction"/>
	<owl:onProperty rdf:resource="http://cybox.mitre.org/objects/File#IRP_MJ_SET_EA"/>
	<owl:maxCardinality rdf:datatype="http://www.w3.org/2001/XMLSchema#nonNegativeInteger">1</owl:maxCardinality>
</rdf:Description>

<rdf:Description rdf:about="http://cybox.mitre.org/objects/File#WindowsDriver">
	<rdfs:subClassOf rdf:nodeID="genid345"/>
</rdf:Description>

<rdf:Description rdf:nodeID="genid345">
	<rdf:type rdf:resource="http://www.w3.org/2002/07/owl#Restriction"/>
	<owl:onProperty rdf:resource="http://cybox.mitre.org/objects/File#IRP_MJ_SET_INFORMATION"/>
	<owl:maxCardinality rdf:datatype="http://www.w3.org/2001/XMLSchema#nonNegativeInteger">1</owl:maxCardinality>
</rdf:Description>

<rdf:Description rdf:about="http://cybox.mitre.org/objects/File#WindowsDriver">
	<rdfs:subClassOf rdf:nodeID="genid346"/>
</rdf:Description>

<rdf:Description rdf:nodeID="genid346">
	<rdf:type rdf:resource="http://www.w3.org/2002/07/owl#Restriction"/>
	<owl:onProperty rdf:resource="http://cybox.mitre.org/objects/File#IRP_MJ_SET_QUOTA"/>
	<owl:maxCardinality rdf:datatype="http://www.w3.org/2001/XMLSchema#nonNegativeInteger">1</owl:maxCardinality>
</rdf:Description>

<rdf:Description rdf:about="http://cybox.mitre.org/objects/File#WindowsDriver">
	<rdfs:subClassOf rdf:nodeID="genid347"/>
</rdf:Description>

<rdf:Description rdf:nodeID="genid347">
	<rdf:type rdf:resource="http://www.w3.org/2002/07/owl#Restriction"/>
	<owl:onProperty rdf:resource="http://cybox.mitre.org/objects/File#IRP_MJ_SET_SECURITY"/>
	<owl:maxCardinality rdf:datatype="http://www.w3.org/2001/XMLSchema#nonNegativeInteger">1</owl:maxCardinality>
</rdf:Description>

<rdf:Description rdf:about="http://cybox.mitre.org/objects/File#WindowsDriver">
	<rdfs:subClassOf rdf:nodeID="genid348"/>
</rdf:Description>

<rdf:Description rdf:nodeID="genid348">
	<rdf:type rdf:resource="http://www.w3.org/2002/07/owl#Restriction"/>
	<owl:onProperty rdf:resource="http://cybox.mitre.org/objects/File#IRP_MJ_SET_VOLUME_INFORMATION"/>
	<owl:maxCardinality rdf:datatype="http://www.w3.org/2001/XMLSchema#nonNegativeInteger">1</owl:maxCardinality>
</rdf:Description>

<rdf:Description rdf:about="http://cybox.mitre.org/objects/File#WindowsDriver">
	<rdfs:subClassOf rdf:nodeID="genid349"/>
</rdf:Description>

<rdf:Description rdf:nodeID="genid349">
	<rdf:type rdf:resource="http://www.w3.org/2002/07/owl#Restriction"/>
	<owl:onProperty rdf:resource="http://cybox.mitre.org/objects/File#IRP_MJ_SHUTDOWN"/>
	<owl:maxCardinality rdf:datatype="http://www.w3.org/2001/XMLSchema#nonNegativeInteger">1</owl:maxCardinality>
</rdf:Description>

<rdf:Description rdf:about="http://cybox.mitre.org/objects/File#WindowsDriver">
	<rdfs:subClassOf rdf:nodeID="genid350"/>
</rdf:Description>

<rdf:Description rdf:nodeID="genid350">
	<rdf:type rdf:resource="http://www.w3.org/2002/07/owl#Restriction"/>
	<owl:onProperty rdf:resource="http://cybox.mitre.org/objects/File#IRP_MJ_SYSTEM_CONTROL"/>
	<owl:maxCardinality rdf:datatype="http://www.w3.org/2001/XMLSchema#nonNegativeInteger">1</owl:maxCardinality>
</rdf:Description>

<rdf:Description rdf:about="http://cybox.mitre.org/objects/File#WindowsDriver">
	<rdfs:subClassOf rdf:nodeID="genid351"/>
</rdf:Description>

<rdf:Description rdf:nodeID="genid351">
	<rdf:type rdf:resource="http://www.w3.org/2002/07/owl#Restriction"/>
	<owl:onProperty rdf:resource="http://cybox.mitre.org/objects/File#IRP_MJ_WRITE"/>
	<owl:maxCardinality rdf:datatype="http://www.w3.org/2001/XMLSchema#nonNegativeInteger">1</owl:maxCardinality>
</rdf:Description>

<rdf:Description rdf:about="http://cybox.mitre.org/objects/File#WindowsDriver">
	<rdfs:subClassOf rdf:nodeID="genid352"/>
</rdf:Description>

<rdf:Description rdf:nodeID="genid352">
	<rdf:type rdf:resource="http://www.w3.org/2002/07/owl#Restriction"/>
	<owl:onProperty rdf:resource="http://cybox.mitre.org/objects/File#buildInfo.compilerVersion"/>
	<owl:maxCardinality rdf:datatype="http://www.w3.org/2001/XMLSchema#nonNegativeInteger">1</owl:maxCardinality>
</rdf:Description>

<rdf:Description rdf:about="http://cybox.mitre.org/objects/File#WindowsDriver">
	<rdfs:subClassOf rdf:nodeID="genid353"/>
</rdf:Description>

<rdf:Description rdf:nodeID="genid353">
	<rdf:type rdf:resource="http://www.w3.org/2002/07/owl#Restriction"/>
	<owl:onProperty rdf:resource="http://cybox.mitre.org/objects/File#driverInit"/>
	<owl:maxCardinality rdf:datatype="http://www.w3.org/2001/XMLSchema#nonNegativeInteger">1</owl:maxCardinality>
</rdf:Description>

<rdf:Description rdf:about="http://cybox.mitre.org/objects/File#WindowsDriver">
	<rdfs:subClassOf rdf:nodeID="genid354"/>
</rdf:Description>

<rdf:Description rdf:nodeID="genid354">
	<rdf:type rdf:resource="http://www.w3.org/2002/07/owl#Restriction"/>
	<owl:onProperty rdf:resource="http://cybox.mitre.org/objects/File#driverObjectAddress"/>
	<owl:maxCardinality rdf:datatype="http://www.w3.org/2001/XMLSchema#nonNegativeInteger">1</owl:maxCardinality>
</rdf:Description>

<rdf:Description rdf:about="http://cybox.mitre.org/objects/File#WindowsDriver">
	<rdfs:subClassOf rdf:nodeID="genid355"/>
</rdf:Description>

<rdf:Description rdf:nodeID="genid355">
	<rdf:type rdf:resource="http://www.w3.org/2002/07/owl#Restriction"/>
	<owl:onProperty rdf:resource="http://cybox.mitre.org/objects/File#driverStartIO"/>
	<owl:maxCardinality rdf:datatype="http://www.w3.org/2001/XMLSchema#nonNegativeInteger">1</owl:maxCardinality>
</rdf:Description>

<rdf:Description rdf:about="http://cybox.mitre.org/objects/File#WindowsDriver">
	<rdfs:subClassOf rdf:nodeID="genid356"/>
</rdf:Description>

<rdf:Description rdf:nodeID="genid356">
	<rdf:type rdf:resource="http://www.w3.org/2002/07/owl#Restriction"/>
	<owl:onProperty rdf:resource="http://cybox.mitre.org/objects/File#driverUnload"/>
	<owl:maxCardinality rdf:datatype="http://www.w3.org/2001/XMLSchema#nonNegativeInteger">1</owl:maxCardinality>
</rdf:Description>

<rdf:Description rdf:about="http://cybox.mitre.org/objects/File#WindowsDriver">
	<rdfs:subClassOf rdf:nodeID="genid357"/>
</rdf:Description>

<rdf:Description rdf:nodeID="genid357">
	<rdf:type rdf:resource="http://www.w3.org/2002/07/owl#Restriction"/>
	<owl:onProperty rdf:resource="http://cybox.mitre.org/objects/File#imageBase"/>
	<owl:maxCardinality rdf:datatype="http://www.w3.org/2001/XMLSchema#nonNegativeInteger">1</owl:maxCardinality>
</rdf:Description>

<rdf:Description rdf:about="http://cybox.mitre.org/objects/File#WindowsDriver">
	<rdfs:subClassOf rdf:nodeID="genid358"/>
</rdf:Description>

<rdf:Description rdf:nodeID="genid358">
	<rdf:type rdf:resource="http://www.w3.org/2002/07/owl#Restriction"/>
	<owl:onProperty rdf:resource="http://cybox.mitre.org/objects/File#imageSize"/>
	<owl:maxCardinality rdf:datatype="http://www.w3.org/2001/XMLSchema#nonNegativeInteger">1</owl:maxCardinality>
</rdf:Description>

<rdf:Description rdf:about="http://cybox.mitre.org/objects/File#WindowsDriver">
	<rdfs:subClassOf rdf:nodeID="genid359"/>
</rdf:Description>

<rdf:Description rdf:nodeID="genid359">
	<rdf:type rdf:resource="http://www.w3.org/2002/07/owl#Restriction"/>
	<owl:onProperty rdf:resource="http://cybox.mitre.org/objects/File#peChecksum.computedAPI"/>
	<owl:maxCardinality rdf:datatype="http://www.w3.org/2001/XMLSchema#nonNegativeInteger">1</owl:maxCardinality>
</rdf:Description>

<rdf:Description rdf:about="http://cybox.mitre.org/objects/File#WindowsDriver">
	<rdfs:subClassOf rdf:nodeID="genid360"/>
</rdf:Description>

<rdf:Description rdf:nodeID="genid360">
	<rdf:type rdf:resource="http://www.w3.org/2002/07/owl#Restriction"/>
	<owl:onProperty rdf:resource="http://cybox.mitre.org/objects/File#peChecksum.fileAPI"/>
	<owl:maxCardinality rdf:datatype="http://www.w3.org/2001/XMLSchema#nonNegativeInteger">1</owl:maxCardinality>
</rdf:Description>

<rdf:Description rdf:about="http://cybox.mitre.org/objects/File#WindowsDriver">
	<rdfs:subClassOf rdf:nodeID="genid361"/>
</rdf:Description>

<rdf:Description rdf:nodeID="genid361">
	<rdf:type rdf:resource="http://www.w3.org/2002/07/owl#Restriction"/>
	<owl:onProperty rdf:resource="http://cybox.mitre.org/objects/File#peChecksum.fileRaw"/>
	<owl:maxCardinality rdf:datatype="http://www.w3.org/2001/XMLSchema#nonNegativeInteger">1</owl:maxCardinality>
</rdf:Description>

<rdf:Description rdf:about="http://cybox.mitre.org/objects/File#WindowsDriver">
	<rdfs:comment>Characterize Windows device drivers.</rdfs:comment>
	<rdfs:isDefinedBy rdf:resource="http://cybox.mitre.org/objects/File"/>
	<rdfs:label>Windows Driver</rdfs:label>
</rdf:Description>
<!--  -->
<!-- http://cybox.mitre.org/objects/File#WindowsExecutableFile -->

<rdf:Description rdf:about="http://cybox.mitre.org/objects/File#WindowsExecutableFile">
	<rdf:type rdf:resource="http://www.w3.org/2002/07/owl#Class"/>
	<rdfs:subClassOf rdf:resource="http://cybox.mitre.org/objects/File#WindowsFile"/>
	<rdfs:subClassOf rdf:nodeID="genid362"/>
</rdf:Description>

<rdf:Description rdf:nodeID="genid362">
	<rdf:type rdf:resource="http://www.w3.org/2002/07/owl#Restriction"/>
	<owl:onProperty rdf:resource="http://cybox.mitre.org/objects/File#digitalSignature"/>
	<owl:maxCardinality rdf:datatype="http://www.w3.org/2001/XMLSchema#nonNegativeInteger">1</owl:maxCardinality>
</rdf:Description>

<rdf:Description rdf:about="http://cybox.mitre.org/objects/File#WindowsExecutableFile">
	<rdfs:subClassOf rdf:nodeID="genid363"/>
</rdf:Description>

<rdf:Description rdf:nodeID="genid363">
	<rdf:type rdf:resource="http://www.w3.org/2002/07/owl#Restriction"/>
	<owl:onProperty rdf:resource="http://cybox.mitre.org/objects/File#exports"/>
	<owl:maxCardinality rdf:datatype="http://www.w3.org/2001/XMLSchema#nonNegativeInteger">1</owl:maxCardinality>
</rdf:Description>

<rdf:Description rdf:about="http://cybox.mitre.org/objects/File#WindowsExecutableFile">
	<rdfs:subClassOf rdf:nodeID="genid364"/>
</rdf:Description>

<rdf:Description rdf:nodeID="genid364">
	<rdf:type rdf:resource="http://www.w3.org/2002/07/owl#Restriction"/>
	<owl:onProperty rdf:resource="http://cybox.mitre.org/objects/File#headers"/>
	<owl:maxCardinality rdf:datatype="http://www.w3.org/2001/XMLSchema#nonNegativeInteger">1</owl:maxCardinality>
</rdf:Description>

<rdf:Description rdf:about="http://cybox.mitre.org/objects/File#WindowsExecutableFile">
	<rdfs:subClassOf rdf:nodeID="genid365"/>
</rdf:Description>

<rdf:Description rdf:nodeID="genid365">
	<rdf:type rdf:resource="http://www.w3.org/2002/07/owl#Restriction"/>
	<owl:onProperty rdf:resource="http://cybox.mitre.org/objects/File#buildInfo.compilerName"/>
	<owl:maxCardinality rdf:datatype="http://www.w3.org/2001/XMLSchema#nonNegativeInteger">1</owl:maxCardinality>
</rdf:Description>

<rdf:Description rdf:about="http://cybox.mitre.org/objects/File#WindowsExecutableFile">
	<rdfs:subClassOf rdf:nodeID="genid366"/>
</rdf:Description>

<rdf:Description rdf:nodeID="genid366">
	<rdf:type rdf:resource="http://www.w3.org/2002/07/owl#Restriction"/>
	<owl:onProperty rdf:resource="http://cybox.mitre.org/objects/File#buildInfo.linkerName"/>
	<owl:maxCardinality rdf:datatype="http://www.w3.org/2001/XMLSchema#nonNegativeInteger">1</owl:maxCardinality>
</rdf:Description>

<rdf:Description rdf:about="http://cybox.mitre.org/objects/File#WindowsExecutableFile">
	<rdfs:subClassOf rdf:nodeID="genid367"/>
</rdf:Description>

<rdf:Description rdf:nodeID="genid367">
	<rdf:type rdf:resource="http://www.w3.org/2002/07/owl#Restriction"/>
	<owl:onProperty rdf:resource="http://cybox.mitre.org/objects/File#buildInfo.linkerVersion"/>
	<owl:maxCardinality rdf:datatype="http://www.w3.org/2001/XMLSchema#nonNegativeInteger">1</owl:maxCardinality>
</rdf:Description>

<rdf:Description rdf:about="http://cybox.mitre.org/objects/File#WindowsExecutableFile">
	<rdfs:subClassOf rdf:nodeID="genid368"/>
</rdf:Description>

<rdf:Description rdf:nodeID="genid368">
	<rdf:type rdf:resource="http://www.w3.org/2002/07/owl#Restriction"/>
	<owl:onProperty rdf:resource="http://cybox.mitre.org/objects/File#extraneousBytes"/>
	<owl:maxCardinality rdf:datatype="http://www.w3.org/2001/XMLSchema#nonNegativeInteger">1</owl:maxCardinality>
</rdf:Description>

<rdf:Description rdf:about="http://cybox.mitre.org/objects/File#WindowsExecutableFile">
	<rdfs:subClassOf rdf:nodeID="genid369"/>
</rdf:Description>

<rdf:Description rdf:nodeID="genid369">
	<rdf:type rdf:resource="http://www.w3.org/2002/07/owl#Restriction"/>
	<owl:onProperty rdf:resource="http://cybox.mitre.org/objects/File#peChecksum.computedAPI"/>
	<owl:maxCardinality rdf:datatype="http://www.w3.org/2001/XMLSchema#nonNegativeInteger">1</owl:maxCardinality>
</rdf:Description>

<rdf:Description rdf:about="http://cybox.mitre.org/objects/File#WindowsExecutableFile">
	<rdfs:subClassOf rdf:nodeID="genid370"/>
</rdf:Description>

<rdf:Description rdf:nodeID="genid370">
	<rdf:type rdf:resource="http://www.w3.org/2002/07/owl#Restriction"/>
	<owl:onProperty rdf:resource="http://cybox.mitre.org/objects/File#peChecksum.fileRaw"/>
	<owl:maxCardinality rdf:datatype="http://www.w3.org/2001/XMLSchema#nonNegativeInteger">1</owl:maxCardinality>
</rdf:Description>

<rdf:Description rdf:about="http://cybox.mitre.org/objects/File#WindowsExecutableFile">
	<rdfs:subClassOf rdf:nodeID="genid371"/>
</rdf:Description>

<rdf:Description rdf:nodeID="genid371">
	<rdf:type rdf:resource="http://www.w3.org/2002/07/owl#Restriction"/>
	<owl:onProperty rdf:resource="http://cybox.mitre.org/objects/File#peType"/>
	<owl:maxCardinality rdf:datatype="http://www.w3.org/2001/XMLSchema#nonNegativeInteger">1</owl:maxCardinality>
</rdf:Description>

<rdf:Description rdf:about="http://cybox.mitre.org/objects/File#WindowsExecutableFile">
	<rdfs:comment>Characterizes Windows PE (Portable Executable) files.</rdfs:comment>
	<rdfs:isDefinedBy rdf:resource="http://cybox.mitre.org/objects/File"/>
	<rdfs:label>Windows Executable File</rdfs:label>
</rdf:Description>
<!--  -->
<!-- http://cybox.mitre.org/objects/File#WindowsFile -->

<rdf:Description rdf:about="http://cybox.mitre.org/objects/File#WindowsFile">
	<rdf:type rdf:resource="http://www.w3.org/2002/07/owl#Class"/>
	<rdfs:subClassOf rdf:resource="http://cybox.mitre.org/objects/File#File"/>
</rdf:Description>


<rdf:Description rdf:about="http://cybox.mitre.org/objects/File#WindowsFile">
</rdf:Description>


<rdf:Description rdf:about="http://cybox.mitre.org/objects/File#WindowsFile">
	<rdfs:subClassOf rdf:nodeID="genid372"/>
</rdf:Description>

<rdf:Description rdf:nodeID="genid372">
	<rdf:type rdf:resource="http://www.w3.org/2002/07/owl#Restriction"/>
	<owl:onProperty rdf:resource="http://cybox.mitre.org/objects/File#drive"/>
	<owl:maxCardinality rdf:datatype="http://www.w3.org/2001/XMLSchema#nonNegativeInteger">1</owl:maxCardinality>
</rdf:Description>

<rdf:Description rdf:about="http://cybox.mitre.org/objects/File#WindowsFile">
	<rdfs:subClassOf rdf:nodeID="genid373"/>
</rdf:Description>

<rdf:Description rdf:nodeID="genid373">
	<rdf:type rdf:resource="http://www.w3.org/2002/07/owl#Restriction"/>
	<owl:onProperty rdf:resource="http://cybox.mitre.org/objects/File#filenameAccessTime"/>
	<owl:maxCardinality rdf:datatype="http://www.w3.org/2001/XMLSchema#nonNegativeInteger">1</owl:maxCardinality>
</rdf:Description>

<rdf:Description rdf:about="http://cybox.mitre.org/objects/File#WindowsFile">
	<rdfs:subClassOf rdf:nodeID="genid374"/>
</rdf:Description>

<rdf:Description rdf:nodeID="genid374">
	<rdf:type rdf:resource="http://www.w3.org/2002/07/owl#Restriction"/>
	<owl:onProperty rdf:resource="http://cybox.mitre.org/objects/File#filenameCreatedTime"/>
	<owl:maxCardinality rdf:datatype="http://www.w3.org/2001/XMLSchema#nonNegativeInteger">1</owl:maxCardinality>
</rdf:Description>

<rdf:Description rdf:about="http://cybox.mitre.org/objects/File#WindowsFile">
	<rdfs:subClassOf rdf:nodeID="genid375"/>
</rdf:Description>

<rdf:Description rdf:nodeID="genid375">
	<rdf:type rdf:resource="http://www.w3.org/2002/07/owl#Restriction"/>
	<owl:onProperty rdf:resource="http://cybox.mitre.org/objects/File#filenameModifiedTime"/>
	<owl:maxCardinality rdf:datatype="http://www.w3.org/2001/XMLSchema#nonNegativeInteger">1</owl:maxCardinality>
</rdf:Description>

<rdf:Description rdf:about="http://cybox.mitre.org/objects/File#WindowsFile">
	<rdfs:comment>Characterize Windows files.</rdfs:comment>
	<rdfs:isDefinedBy rdf:resource="http://cybox.mitre.org/objects/File"/>
	<rdfs:label>Windows File</rdfs:label>
</rdf:Description>
<!--  -->
<!-- http://cybox.mitre.org/objects/File#WindowsFileAttribute -->

<rdf:Description rdf:about="http://cybox.mitre.org/objects/File#WindowsFileAttribute">
	<rdf:type rdf:resource="http://www.w3.org/2002/07/owl#Class"/>
	<rdfs:subClassOf rdf:resource="http://cybox.mitre.org/objects/File#FileAttribute"/>
	<rdfs:subClassOf rdf:nodeID="genid376"/>
</rdf:Description>

<rdf:Description rdf:nodeID="genid376">
	<rdf:type rdf:resource="http://www.w3.org/2002/07/owl#Restriction"/>
	<owl:onProperty rdf:resource="http://cybox.mitre.org/objects/File#archive"/>
	<owl:maxCardinality rdf:datatype="http://www.w3.org/2001/XMLSchema#nonNegativeInteger">1</owl:maxCardinality>
</rdf:Description>

<rdf:Description rdf:about="http://cybox.mitre.org/objects/File#WindowsFileAttribute">
	<rdfs:subClassOf rdf:nodeID="genid377"/>
</rdf:Description>

<rdf:Description rdf:nodeID="genid377">
	<rdf:type rdf:resource="http://www.w3.org/2002/07/owl#Restriction"/>
	<owl:onProperty rdf:resource="http://cybox.mitre.org/objects/File#compressed"/>
	<owl:maxCardinality rdf:datatype="http://www.w3.org/2001/XMLSchema#nonNegativeInteger">1</owl:maxCardinality>
</rdf:Description>

<rdf:Description rdf:about="http://cybox.mitre.org/objects/File#WindowsFileAttribute">
	<rdfs:subClassOf rdf:nodeID="genid378"/>
</rdf:Description>

<rdf:Description rdf:nodeID="genid378">
	<rdf:type rdf:resource="http://www.w3.org/2002/07/owl#Restriction"/>
	<owl:onProperty rdf:resource="http://cybox.mitre.org/objects/File#deleted"/>
	<owl:maxCardinality rdf:datatype="http://www.w3.org/2001/XMLSchema#nonNegativeInteger">1</owl:maxCardinality>
</rdf:Description>

<rdf:Description rdf:about="http://cybox.mitre.org/objects/File#WindowsFileAttribute">
	<rdfs:subClassOf rdf:nodeID="genid379"/>
</rdf:Description>

<rdf:Description rdf:nodeID="genid379">
	<rdf:type rdf:resource="http://www.w3.org/2002/07/owl#Restriction"/>
	<owl:onProperty rdf:resource="http://cybox.mitre.org/objects/File#device"/>
	<owl:maxCardinality rdf:datatype="http://www.w3.org/2001/XMLSchema#nonNegativeInteger">1</owl:maxCardinality>
</rdf:Description>

<rdf:Description rdf:about="http://cybox.mitre.org/objects/File#WindowsFileAttribute">
	<rdfs:subClassOf rdf:nodeID="genid380"/>
</rdf:Description>

<rdf:Description rdf:nodeID="genid380">
	<rdf:type rdf:resource="http://www.w3.org/2002/07/owl#Restriction"/>
	<owl:onProperty rdf:resource="http://cybox.mitre.org/objects/File#directory"/>
	<owl:maxCardinality rdf:datatype="http://www.w3.org/2001/XMLSchema#nonNegativeInteger">1</owl:maxCardinality>
</rdf:Description>

<rdf:Description rdf:about="http://cybox.mitre.org/objects/File#WindowsFileAttribute">
	<rdfs:subClassOf rdf:nodeID="genid381"/>
</rdf:Description>

<rdf:Description rdf:nodeID="genid381">
	<rdf:type rdf:resource="http://www.w3.org/2002/07/owl#Restriction"/>
	<owl:onProperty rdf:resource="http://cybox.mitre.org/objects/File#encrypted"/>
	<owl:maxCardinality rdf:datatype="http://www.w3.org/2001/XMLSchema#nonNegativeInteger">1</owl:maxCardinality>
</rdf:Description>

<rdf:Description rdf:about="http://cybox.mitre.org/objects/File#WindowsFileAttribute">
	<rdfs:subClassOf rdf:nodeID="genid382"/>
</rdf:Description>

<rdf:Description rdf:nodeID="genid382">
	<rdf:type rdf:resource="http://www.w3.org/2002/07/owl#Restriction"/>
	<owl:onProperty rdf:resource="http://cybox.mitre.org/objects/File#hidden"/>
	<owl:maxCardinality rdf:datatype="http://www.w3.org/2001/XMLSchema#nonNegativeInteger">1</owl:maxCardinality>
</rdf:Description>

<rdf:Description rdf:about="http://cybox.mitre.org/objects/File#WindowsFileAttribute">
	<rdfs:subClassOf rdf:nodeID="genid383"/>
</rdf:Description>

<rdf:Description rdf:nodeID="genid383">
	<rdf:type rdf:resource="http://www.w3.org/2002/07/owl#Restriction"/>
	<owl:onProperty rdf:resource="http://cybox.mitre.org/objects/File#integrityStream"/>
	<owl:maxCardinality rdf:datatype="http://www.w3.org/2001/XMLSchema#nonNegativeInteger">1</owl:maxCardinality>
</rdf:Description>

<rdf:Description rdf:about="http://cybox.mitre.org/objects/File#WindowsFileAttribute">
	<rdfs:subClassOf rdf:nodeID="genid384"/>
</rdf:Description>

<rdf:Description rdf:nodeID="genid384">
	<rdf:type rdf:resource="http://www.w3.org/2002/07/owl#Restriction"/>
	<owl:onProperty rdf:resource="http://cybox.mitre.org/objects/File#noScrubData"/>
	<owl:maxCardinality rdf:datatype="http://www.w3.org/2001/XMLSchema#nonNegativeInteger">1</owl:maxCardinality>
</rdf:Description>

<rdf:Description rdf:about="http://cybox.mitre.org/objects/File#WindowsFileAttribute">
	<rdfs:subClassOf rdf:nodeID="genid385"/>
</rdf:Description>

<rdf:Description rdf:nodeID="genid385">
	<rdf:type rdf:resource="http://www.w3.org/2002/07/owl#Restriction"/>
	<owl:onProperty rdf:resource="http://cybox.mitre.org/objects/File#normal"/>
	<owl:maxCardinality rdf:datatype="http://www.w3.org/2001/XMLSchema#nonNegativeInteger">1</owl:maxCardinality>
</rdf:Description>

<rdf:Description rdf:about="http://cybox.mitre.org/objects/File#WindowsFileAttribute">
	<rdfs:subClassOf rdf:nodeID="genid386"/>
</rdf:Description>

<rdf:Description rdf:nodeID="genid386">
	<rdf:type rdf:resource="http://www.w3.org/2002/07/owl#Restriction"/>
	<owl:onProperty rdf:resource="http://cybox.mitre.org/objects/File#notContentIndexed"/>
	<owl:maxCardinality rdf:datatype="http://www.w3.org/2001/XMLSchema#nonNegativeInteger">1</owl:maxCardinality>
</rdf:Description>

<rdf:Description rdf:about="http://cybox.mitre.org/objects/File#WindowsFileAttribute">
	<rdfs:subClassOf rdf:nodeID="genid387"/>
</rdf:Description>

<rdf:Description rdf:nodeID="genid387">
	<rdf:type rdf:resource="http://www.w3.org/2002/07/owl#Restriction"/>
	<owl:onProperty rdf:resource="http://cybox.mitre.org/objects/File#offline"/>
	<owl:maxCardinality rdf:datatype="http://www.w3.org/2001/XMLSchema#nonNegativeInteger">1</owl:maxCardinality>
</rdf:Description>

<rdf:Description rdf:about="http://cybox.mitre.org/objects/File#WindowsFileAttribute">
	<rdfs:subClassOf rdf:nodeID="genid388"/>
</rdf:Description>

<rdf:Description rdf:nodeID="genid388">
	<rdf:type rdf:resource="http://www.w3.org/2002/07/owl#Restriction"/>
	<owl:onProperty rdf:resource="http://cybox.mitre.org/objects/File#readOnly"/>
	<owl:maxCardinality rdf:datatype="http://www.w3.org/2001/XMLSchema#nonNegativeInteger">1</owl:maxCardinality>
</rdf:Description>

<rdf:Description rdf:about="http://cybox.mitre.org/objects/File#WindowsFileAttribute">
	<rdfs:subClassOf rdf:nodeID="genid389"/>
</rdf:Description>

<rdf:Description rdf:nodeID="genid389">
	<rdf:type rdf:resource="http://www.w3.org/2002/07/owl#Restriction"/>
	<owl:onProperty rdf:resource="http://cybox.mitre.org/objects/File#reparsePoint"/>
	<owl:maxCardinality rdf:datatype="http://www.w3.org/2001/XMLSchema#nonNegativeInteger">1</owl:maxCardinality>
</rdf:Description>

<rdf:Description rdf:about="http://cybox.mitre.org/objects/File#WindowsFileAttribute">
	<rdfs:subClassOf rdf:nodeID="genid390"/>
</rdf:Description>

<rdf:Description rdf:nodeID="genid390">
	<rdf:type rdf:resource="http://www.w3.org/2002/07/owl#Restriction"/>
	<owl:onProperty rdf:resource="http://cybox.mitre.org/objects/File#sparseFile"/>
	<owl:maxCardinality rdf:datatype="http://www.w3.org/2001/XMLSchema#nonNegativeInteger">1</owl:maxCardinality>
</rdf:Description>

<rdf:Description rdf:about="http://cybox.mitre.org/objects/File#WindowsFileAttribute">
	<rdfs:subClassOf rdf:nodeID="genid391"/>
</rdf:Description>

<rdf:Description rdf:nodeID="genid391">
	<rdf:type rdf:resource="http://www.w3.org/2002/07/owl#Restriction"/>
	<owl:onProperty rdf:resource="http://cybox.mitre.org/objects/File#system"/>
	<owl:maxCardinality rdf:datatype="http://www.w3.org/2001/XMLSchema#nonNegativeInteger">1</owl:maxCardinality>
</rdf:Description>

<rdf:Description rdf:about="http://cybox.mitre.org/objects/File#WindowsFileAttribute">
	<rdfs:subClassOf rdf:nodeID="genid392"/>
</rdf:Description>

<rdf:Description rdf:nodeID="genid392">
	<rdf:type rdf:resource="http://www.w3.org/2002/07/owl#Restriction"/>
	<owl:onProperty rdf:resource="http://cybox.mitre.org/objects/File#temporary"/>
	<owl:maxCardinality rdf:datatype="http://www.w3.org/2001/XMLSchema#nonNegativeInteger">1</owl:maxCardinality>
</rdf:Description>

<rdf:Description rdf:about="http://cybox.mitre.org/objects/File#WindowsFileAttribute">
	<rdfs:subClassOf rdf:nodeID="genid393"/>
</rdf:Description>

<rdf:Description rdf:nodeID="genid393">
	<rdf:type rdf:resource="http://www.w3.org/2002/07/owl#Restriction"/>
	<owl:onProperty rdf:resource="http://cybox.mitre.org/objects/File#virtual"/>
	<owl:maxCardinality rdf:datatype="http://www.w3.org/2001/XMLSchema#nonNegativeInteger">1</owl:maxCardinality>
</rdf:Description>

<rdf:Description rdf:about="http://cybox.mitre.org/objects/File#WindowsFileAttribute">
	<rdfs:comment>Chararactizes Windows File Attributes</rdfs:comment>
	<rdfs:isDefinedBy rdf:resource="http://cybox.mitre.org/objects/File"/>
	<rdfs:label>Windows File Attribute</rdfs:label>
</rdf:Description>
<!--  -->
<!-- http://cybox.mitre.org/objects/File#WindowsFilePermission -->

<rdf:Description rdf:about="http://cybox.mitre.org/objects/File#WindowsFilePermission">
	<rdf:type rdf:resource="http://www.w3.org/2002/07/owl#Class"/>
	<rdfs:subClassOf rdf:resource="http://cybox.mitre.org/objects/File#FilePermission"/>
	<rdfs:subClassOf rdf:nodeID="genid394"/>
</rdf:Description>

<rdf:Description rdf:nodeID="genid394">
	<rdf:type rdf:resource="http://www.w3.org/2002/07/owl#Restriction"/>
	<owl:onProperty rdf:resource="http://cybox.mitre.org/objects/File#fullControl"/>
	<owl:maxCardinality rdf:datatype="http://www.w3.org/2001/XMLSchema#nonNegativeInteger">1</owl:maxCardinality>
</rdf:Description>

<rdf:Description rdf:about="http://cybox.mitre.org/objects/File#WindowsFilePermission">
	<rdfs:subClassOf rdf:nodeID="genid395"/>
</rdf:Description>

<rdf:Description rdf:nodeID="genid395">
	<rdf:type rdf:resource="http://www.w3.org/2002/07/owl#Restriction"/>
	<owl:onProperty rdf:resource="http://cybox.mitre.org/objects/File#modify"/>
	<owl:maxCardinality rdf:datatype="http://www.w3.org/2001/XMLSchema#nonNegativeInteger">1</owl:maxCardinality>
</rdf:Description>

<rdf:Description rdf:about="http://cybox.mitre.org/objects/File#WindowsFilePermission">
	<rdfs:subClassOf rdf:nodeID="genid396"/>
</rdf:Description>

<rdf:Description rdf:nodeID="genid396">
	<rdf:type rdf:resource="http://www.w3.org/2002/07/owl#Restriction"/>
	<owl:onProperty rdf:resource="http://cybox.mitre.org/objects/File#read"/>
	<owl:maxCardinality rdf:datatype="http://www.w3.org/2001/XMLSchema#nonNegativeInteger">1</owl:maxCardinality>
</rdf:Description>

<rdf:Description rdf:about="http://cybox.mitre.org/objects/File#WindowsFilePermission">
	<rdfs:subClassOf rdf:nodeID="genid397"/>
</rdf:Description>

<rdf:Description rdf:nodeID="genid397">
	<rdf:type rdf:resource="http://www.w3.org/2002/07/owl#Restriction"/>
	<owl:onProperty rdf:resource="http://cybox.mitre.org/objects/File#readAndExecute"/>
	<owl:maxCardinality rdf:datatype="http://www.w3.org/2001/XMLSchema#nonNegativeInteger">1</owl:maxCardinality>
</rdf:Description>

<rdf:Description rdf:about="http://cybox.mitre.org/objects/File#WindowsFilePermission">
	<rdfs:subClassOf rdf:nodeID="genid398"/>
</rdf:Description>

<rdf:Description rdf:nodeID="genid398">
	<rdf:type rdf:resource="http://www.w3.org/2002/07/owl#Restriction"/>
	<owl:onProperty rdf:resource="http://cybox.mitre.org/objects/File#write"/>
	<owl:maxCardinality rdf:datatype="http://www.w3.org/2001/XMLSchema#nonNegativeInteger">1</owl:maxCardinality>
</rdf:Description>

<rdf:Description rdf:about="http://cybox.mitre.org/objects/File#WindowsFilePermission">
	<rdfs:comment>Characterizes Windows file permissions.</rdfs:comment>
	<rdfs:isDefinedBy rdf:resource="http://cybox.mitre.org/objects/File"/>
	<rdfs:label>Windows File Permissions</rdfs:label>
</rdf:Description>
<!--  -->
<!-- http://cybox.mitre.org/objects/File#WindowsStream -->



<rdf:Description rdf:about="http://cybox.mitre.org/objects/File#WindowsStream">
	<rdfs:subClassOf rdf:nodeID="genid399"/>
</rdf:Description>

<rdf:Description rdf:nodeID="genid399">
	<rdf:type rdf:resource="http://www.w3.org/2002/07/owl#Restriction"/>
	<owl:onProperty rdf:resource="http://cybox.mitre.org/objects/File#streamName"/>
	<owl:cardinality rdf:datatype="http://www.w3.org/2001/XMLSchema#nonNegativeInteger">1</owl:cardinality>
</rdf:Description>

<rdf:Description rdf:about="http://cybox.mitre.org/objects/File#WindowsStream">
	<rdfs:subClassOf rdf:nodeID="genid400"/>
</rdf:Description>

<rdf:Description rdf:nodeID="genid400">
	<rdf:type rdf:resource="http://www.w3.org/2002/07/owl#Restriction"/>
	<owl:onProperty rdf:resource="http://cybox.mitre.org/objects/File#sizeInBytes"/>
	<owl:maxCardinality rdf:datatype="http://www.w3.org/2001/XMLSchema#nonNegativeInteger">1</owl:maxCardinality>
</rdf:Description>

<rdf:Description rdf:about="http://cybox.mitre.org/objects/File#WindowsStream">
	<rdfs:comment>Characterize NTFS alternate data streams.</rdfs:comment>
	<rdfs:isDefinedBy rdf:resource="http://cybox.mitre.org/objects/File"/>
	<rdfs:label>Windows Stream</rdfs:label>
</rdf:Description>


<rdf:Description rdf:nodeID="genid401">
	<owl:cardinality rdf:datatype="http://www.w3.org/2001/XMLSchema#nonNegativeInteger">1</owl:cardinality>
</rdf:Description>

<rdf:Description rdf:nodeID="genid402">
	<owl:cardinality rdf:datatype="http://www.w3.org/2001/XMLSchema#nonNegativeInteger">1</owl:cardinality>
</rdf:Description>

<rdf:Description rdf:nodeID="genid403">
	<owl:cardinality rdf:datatype="http://www.w3.org/2001/XMLSchema#nonNegativeInteger">1</owl:cardinality>
</rdf:Description>

<rdf:Description rdf:nodeID="genid404">
	<owl:maxCardinality rdf:datatype="http://www.w3.org/2001/XMLSchema#nonNegativeInteger">1</owl:maxCardinality>
</rdf:Description>

<rdf:Description rdf:nodeID="genid405">
	<owl:maxCardinality rdf:datatype="http://www.w3.org/2001/XMLSchema#nonNegativeInteger">1</owl:maxCardinality>
</rdf:Description>

<rdf:Description rdf:nodeID="genid406">
	<owl:minCardinality rdf:datatype="http://www.w3.org/2001/XMLSchema#nonNegativeInteger">1</owl:minCardinality>
</rdf:Description>
<!-- Generated by the OWL API (version 4.2.6.20160910-2108) https://github.com/owlcs/owlapi -->

</rdf:RDF>