<?xml version="1.0"?>
<rdf:RDF xmlns="http://cybox.mitre.org/objects/UserSession#"
     xml:base="http://cybox.mitre.org/objects/UserSession"
     xmlns:rdf="http://www.w3.org/1999/02/22-rdf-syntax-ns#"
     xmlns:owl="http://www.w3.org/2002/07/owl#"
     xmlns:xml="http://www.w3.org/XML/1998/namespace"
     xmlns:xsd="http://www.w3.org/2001/XMLSchema#"
     xmlns:rdfs="http://www.w3.org/2000/01/rdf-schema#"
     xmlns:userSessionObj="http://cybox.mitre.org/objects/UserSession#">
    <owl:Ontology rdf:about="http://cybox.mitre.org/objects/UserSession">
        <owl:imports rdf:resource="http://cybox.mitre.org/cybox_core"/>
        <rdfs:label>Cyber Observable eXpression (CybOX) User Session Ontology {@en-US}Cyber Observable eXpression (CybOX) Account Ontology</rdfs:label>
        <owl:versionInfo rdf:datatype="http://www.w3.org/2001/XMLSchema#string">2.1.0-000</owl:versionInfo>
        <rdfs:comment>This ontology provides a vocabulary and representation of an User Session for the  Cyber Observable eXpression (CybOX).  

CybOX  provides a common mechansim (structure and content) to convey the full range of potential cyber observable information and strives to be fully expressive, flexible, extensible, automatable, and as human-readable as possible.

The ontology is based on the Cybox User Session object schema maintained by The MITRE Corporation copyright 2012-2014.  The version number of the ontology is kept in sync with the schema in order to more easily relate between the ontology and the corresponding schema version.

Copyright (c) 2014, DaedaFusion, LLC.  All rights reserved.</rdfs:comment>
    </owl:Ontology>
    


    <!-- 
    ///////////////////////////////////////////////////////////////////////////////////////
    //
    // Data properties
    //
    ///////////////////////////////////////////////////////////////////////////////////////
     -->

    


    <!-- http://cybox.mitre.org/objects/UserSession#effectiveGroup -->

    <owl:DatatypeProperty rdf:about="http://cybox.mitre.org/objects/UserSession#effectiveGroup">
        <rdfs:range rdf:resource="http://www.w3.org/2001/XMLSchema#string"/>
        <rdfs:comment>Specifies the name of the effective group used in the user session.</rdfs:comment>
        <rdfs:isDefinedBy rdf:resource="http://cybox.mitre.org/objects/UserSession"/>
        <rdfs:label>Effective Group</rdfs:label>
    </owl:DatatypeProperty>
    


    <!-- http://cybox.mitre.org/objects/UserSession#effectiveGroupID -->

    <owl:DatatypeProperty rdf:about="http://cybox.mitre.org/objects/UserSession#effectiveGroupID">
        <rdfs:range rdf:resource="http://www.w3.org/2001/XMLSchema#string"/>
        <rdfs:comment>Specifies the effective group ID of the group used in the user session.</rdfs:comment>
        <rdfs:isDefinedBy rdf:resource="http://cybox.mitre.org/objects/UserSession"/>
        <rdfs:label>Effective Group ID</rdfs:label>
    </owl:DatatypeProperty>
    


    <!-- http://cybox.mitre.org/objects/UserSession#effectiveUser -->

    <owl:DatatypeProperty rdf:about="http://cybox.mitre.org/objects/UserSession#effectiveUser">
        <rdfs:range rdf:resource="http://www.w3.org/2001/XMLSchema#string"/>
        <rdfs:comment>Specifies the effective username used in the user session.</rdfs:comment>
        <rdfs:isDefinedBy rdf:resource="http://cybox.mitre.org/objects/UserSession"/>
        <rdfs:label>Effective User</rdfs:label>
    </owl:DatatypeProperty>
    


    <!-- http://cybox.mitre.org/objects/UserSession#effectiveUserID -->

    <owl:DatatypeProperty rdf:about="http://cybox.mitre.org/objects/UserSession#effectiveUserID">
        <rdfs:range rdf:resource="http://www.w3.org/2001/XMLSchema#string"/>
        <rdfs:comment>Specifies the effective user ID of the user used in the user session.</rdfs:comment>
        <rdfs:isDefinedBy rdf:resource="http://cybox.mitre.org/objects/UserSession"/>
        <rdfs:label>Effective User ID</rdfs:label>
    </owl:DatatypeProperty>
    


    <!-- http://cybox.mitre.org/objects/UserSession#loginDateTime -->

    <owl:DatatypeProperty rdf:about="http://cybox.mitre.org/objects/UserSession#loginDateTime">
        <rdfs:range rdf:resource="http://www.w3.org/2001/XMLSchema#dateTime"/>
        <rdfs:comment>Specifies the date/time of the login for the user session.</rdfs:comment>
        <rdfs:isDefinedBy rdf:resource="http://cybox.mitre.org/objects/UserSession"/>
        <rdfs:label>Login Time</rdfs:label>
    </owl:DatatypeProperty>
    


    <!-- http://cybox.mitre.org/objects/UserSession#logoutDateTime -->

    <owl:DatatypeProperty rdf:about="http://cybox.mitre.org/objects/UserSession#logoutDateTime">
        <rdfs:range rdf:resource="http://www.w3.org/2001/XMLSchema#dateTime"/>
        <rdfs:comment>Specifies the date/time of the logout for the user session.</rdfs:comment>
        <rdfs:isDefinedBy rdf:resource="http://cybox.mitre.org/objects/UserSession"/>
        <rdfs:label>Logout Time</rdfs:label>
    </owl:DatatypeProperty>
    


    <!-- 
    ///////////////////////////////////////////////////////////////////////////////////////
    //
    // Classes
    //
    ///////////////////////////////////////////////////////////////////////////////////////
     -->

    


    <!-- http://cybox.mitre.org/cybox_core#Object -->

    <owl:Class rdf:about="http://cybox.mitre.org/cybox_core#Object"/>
    


    <!-- http://cybox.mitre.org/objects/UserSession#UserSession -->

    <owl:Class rdf:about="http://cybox.mitre.org/objects/UserSession#UserSession">
        <rdfs:subClassOf rdf:resource="http://cybox.mitre.org/cybox_core#Object"/>
        <rdfs:subClassOf>
            <owl:Restriction>
                <owl:onProperty rdf:resource="http://cybox.mitre.org/objects/UserSession#loginDateTime"/>
                <owl:cardinality rdf:datatype="http://www.w3.org/2001/XMLSchema#nonNegativeInteger">1</owl:cardinality>
            </owl:Restriction>
        </rdfs:subClassOf>
        <rdfs:subClassOf>
            <owl:Restriction>
                <owl:onProperty rdf:resource="http://cybox.mitre.org/objects/UserSession#logoutDateTime"/>
                <owl:cardinality rdf:datatype="http://www.w3.org/2001/XMLSchema#nonNegativeInteger">1</owl:cardinality>
            </owl:Restriction>
        </rdfs:subClassOf>
        <rdfs:subClassOf>
            <owl:Restriction>
                <owl:onProperty rdf:resource="http://cybox.mitre.org/objects/UserSession#effectiveGroup"/>
                <owl:maxCardinality rdf:datatype="http://www.w3.org/2001/XMLSchema#nonNegativeInteger">1</owl:maxCardinality>
            </owl:Restriction>
        </rdfs:subClassOf>
        <rdfs:subClassOf>
            <owl:Restriction>
                <owl:onProperty rdf:resource="http://cybox.mitre.org/objects/UserSession#effectiveGroupID"/>
                <owl:maxCardinality rdf:datatype="http://www.w3.org/2001/XMLSchema#nonNegativeInteger">1</owl:maxCardinality>
            </owl:Restriction>
        </rdfs:subClassOf>
        <rdfs:subClassOf>
            <owl:Restriction>
                <owl:onProperty rdf:resource="http://cybox.mitre.org/objects/UserSession#effectiveUser"/>
                <owl:maxCardinality rdf:datatype="http://www.w3.org/2001/XMLSchema#nonNegativeInteger">1</owl:maxCardinality>
            </owl:Restriction>
        </rdfs:subClassOf>
        <rdfs:subClassOf>
            <owl:Restriction>
                <owl:onProperty rdf:resource="http://cybox.mitre.org/objects/UserSession#effectiveUserID"/>
                <owl:maxCardinality rdf:datatype="http://www.w3.org/2001/XMLSchema#nonNegativeInteger">1</owl:maxCardinality>
            </owl:Restriction>
        </rdfs:subClassOf>
        <rdfs:comment>Characterize user sessions.</rdfs:comment>
        <rdfs:isDefinedBy rdf:resource="http://cybox.mitre.org/objects/UserSession"/>
        <rdfs:label>User Session</rdfs:label>
    </owl:Class>
</rdf:RDF>



<!-- Generated by the OWL API (version 4.2.6.20160910-2108) https://github.com/owlcs/owlapi -->

