<?xml version="1.0"?>
<rdf:RDF xmlns="http://cybox.mitre.org/objects/WindowsFilemapping#"
     xml:base="http://cybox.mitre.org/objects/WindowsFilemapping"
     xmlns:rdf="http://www.w3.org/1999/02/22-rdf-syntax-ns#"
     xmlns:owl="http://www.w3.org/2002/07/owl#"
     xmlns:xml="http://www.w3.org/XML/1998/namespace"
     xmlns:xsd="http://www.w3.org/2001/XMLSchema#"
     xmlns:rdfs="http://www.w3.org/2000/01/rdf-schema#"
     xmlns:winFilemappingObj="http://cybox.mitre.org/objects/WindowsFilemapping#">
    <owl:Ontology rdf:about="http://cybox.mitre.org/objects/WindowsFilemapping">
        <owl:imports rdf:resource="http://cybox.mitre.org/objects/WindowsHandle"/>
        <rdfs:comment>This ontology provides a vocabulary and representation of an Windows Filemapping for the Cyber Observable eXpression (CybOX).  

CybOX  provides a common mechansim (structure and content) to convey the full range of potential cyber observable information and strives to be fully expressive, flexible, extensible, automatable, and as human-readable as possible.

The ontology is based on the CybOX Windows Filemapping object schema maintained by The MITRE Corporation copyright 2012-2014.  The version number of the ontology is kept in sync with the schema in order to more easily relate between the ontology and the corresponding schema version.

Copyright (c) 2014, DaedaFusion, LLC.  All rights reserved.</rdfs:comment>
        <owl:versionInfo rdf:datatype="http://www.w3.org/2001/XMLSchema#string">2.1.0-000</owl:versionInfo>
        <rdfs:label>Cyber Observable eXpression (CybOX) Windows Filemapping Ontology</rdfs:label>
    </owl:Ontology>
    


    <!-- 
    ///////////////////////////////////////////////////////////////////////////////////////
    //
    // Object Properties
    //
    ///////////////////////////////////////////////////////////////////////////////////////
     -->

    


    <!-- http://cybox.mitre.org/objects/WindowsFilemapping#fileHandle -->

    <owl:ObjectProperty rdf:about="http://cybox.mitre.org/objects/WindowsFilemapping#fileHandle">
        <rdfs:domain rdf:resource="http://cybox.mitre.org/objects/WindowsFilemapping#WindowsFilemapping"/>
        <rdfs:range rdf:resource="http://cybox.mitre.org/objects/WindowsHandle#WindowsHandle"/>
        <rdfs:comment>Specifies the Windows handle to the file from which the file mapping was created.</rdfs:comment>
        <rdfs:isDefinedBy rdf:resource="http://cybox.mitre.org/objects/WindowsFilemapping"/>
        <rdfs:label>File Handle</rdfs:label>
    </owl:ObjectProperty>
    


    <!-- http://cybox.mitre.org/objects/WindowsFilemapping#handle -->

    <owl:ObjectProperty rdf:about="http://cybox.mitre.org/objects/WindowsFilemapping#handle">
        <rdfs:domain rdf:resource="http://cybox.mitre.org/objects/WindowsFilemapping#WindowsFilemapping"/>
        <rdfs:range rdf:resource="http://cybox.mitre.org/objects/WindowsHandle#WindowsHandle"/>
        <rdfs:comment>Specifies the Windows handle to the file mapping.</rdfs:comment>
        <rdfs:isDefinedBy rdf:resource="http://cybox.mitre.org/objects/WindowsFilemapping"/>
        <rdfs:label>Handle</rdfs:label>
    </owl:ObjectProperty>
    


    <!-- 
    ///////////////////////////////////////////////////////////////////////////////////////
    //
    // Data properties
    //
    ///////////////////////////////////////////////////////////////////////////////////////
     -->

    


    <!-- http://cybox.mitre.org/objects/WindowsFilemapping#actualSize -->

    <owl:DatatypeProperty rdf:about="http://cybox.mitre.org/objects/WindowsFilemapping#actualSize">
        <rdfs:domain rdf:resource="http://cybox.mitre.org/objects/WindowsFilemapping#WindowsFilemapping"/>
        <rdfs:range rdf:resource="http://www.w3.org/2001/XMLSchema#unsignedLong"/>
        <rdfs:comment>Specifies the actual size of the file mapping, in bytes.</rdfs:comment>
        <rdfs:isDefinedBy rdf:resource="http://cybox.mitre.org/objects/WindowsFilemapping"/>
        <rdfs:label>Actual Size</rdfs:label>
    </owl:DatatypeProperty>
    


    <!-- http://cybox.mitre.org/objects/WindowsFilemapping#filemappingName -->

    <owl:DatatypeProperty rdf:about="http://cybox.mitre.org/objects/WindowsFilemapping#filemappingName">
        <rdfs:domain rdf:resource="http://cybox.mitre.org/objects/WindowsFilemapping#WindowsFilemapping"/>
        <rdfs:range rdf:resource="http://www.w3.org/2001/XMLSchema#string"/>
        <rdfs:comment>Specifies the name of the file mapping.</rdfs:comment>
        <rdfs:isDefinedBy rdf:resource="http://cybox.mitre.org/objects/WindowsFilemapping"/>
        <rdfs:label>Filemapping Name</rdfs:label>
    </owl:DatatypeProperty>
    


    <!-- http://cybox.mitre.org/objects/WindowsFilemapping#maximumSize -->

    <owl:DatatypeProperty rdf:about="http://cybox.mitre.org/objects/WindowsFilemapping#maximumSize">
        <rdfs:domain rdf:resource="http://cybox.mitre.org/objects/WindowsFilemapping#WindowsFilemapping"/>
        <rdfs:range rdf:resource="http://www.w3.org/2001/XMLSchema#unsignedLong"/>
        <rdfs:comment>Specifies the maximum allowed size for the file mapping, in bytes. This value is typically initialized upon creation of the file mapping.</rdfs:comment>
        <rdfs:isDefinedBy rdf:resource="http://cybox.mitre.org/objects/WindowsFilemapping"/>
        <rdfs:label>Maximum Size</rdfs:label>
    </owl:DatatypeProperty>
    


    <!-- http://cybox.mitre.org/objects/WindowsFilemapping#pageProtectionAttribute -->

    <owl:DatatypeProperty rdf:about="http://cybox.mitre.org/objects/WindowsFilemapping#pageProtectionAttribute">
        <rdfs:domain rdf:resource="http://cybox.mitre.org/objects/WindowsFilemapping#WindowsFilemapping"/>
        <rdfs:range rdf:resource="http://www.w3.org/2001/XMLSchema#string"/>
        <rdfs:comment>Specifies a page protection attribute (i.e. SEC_) to be used in combination with the page protection value captured in the Page Protection Value field.</rdfs:comment>
        <rdfs:isDefinedBy rdf:resource="http://cybox.mitre.org/objects/WindowsFilemapping"/>
        <rdfs:label>Page Protection Attribute</rdfs:label>
    </owl:DatatypeProperty>
    


    <!-- http://cybox.mitre.org/objects/WindowsFilemapping#pageProtectionValue -->

    <owl:DatatypeProperty rdf:about="http://cybox.mitre.org/objects/WindowsFilemapping#pageProtectionValue">
        <rdfs:domain rdf:resource="http://cybox.mitre.org/objects/WindowsFilemapping#WindowsFilemapping"/>
        <rdfs:range rdf:resource="http://www.w3.org/2001/XMLSchema#string"/>
        <rdfs:comment>Specifies the page protection value (i.e. PAGE_) specified for the file mapping.</rdfs:comment>
        <rdfs:isDefinedBy rdf:resource="http://cybox.mitre.org/objects/WindowsFilemapping"/>
        <rdfs:label>Page Protection Value</rdfs:label>
    </owl:DatatypeProperty>
    


    <!-- http://cybox.mitre.org/objects/WindowsFilemapping#securityAttributes -->

    <owl:DatatypeProperty rdf:about="http://cybox.mitre.org/objects/WindowsFilemapping#securityAttributes">
        <rdfs:domain rdf:resource="http://cybox.mitre.org/objects/WindowsFilemapping#WindowsFilemapping"/>
        <rdfs:range rdf:resource="http://www.w3.org/2001/XMLSchema#string"/>
        <rdfs:comment>Specifies the Windows security attributes for the file mapping.</rdfs:comment>
        <rdfs:isDefinedBy rdf:resource="http://cybox.mitre.org/objects/WindowsFilemapping"/>
        <rdfs:label>Security Attributes</rdfs:label>
    </owl:DatatypeProperty>
    


    <!-- 
    ///////////////////////////////////////////////////////////////////////////////////////
    //
    // Classes
    //
    ///////////////////////////////////////////////////////////////////////////////////////
     -->

    

    <!-- http://cybox.mitre.org/objects/WindowsFilemapping#WindowsFilemapping -->

    <owl:Class rdf:about="http://cybox.mitre.org/objects/WindowsFilemapping#WindowsFilemapping">
        <rdfs:subClassOf rdf:resource="http://cybox.mitre.org/cybox_core#Object"/>
        <rdfs:subClassOf>
            <owl:Restriction>
                <owl:onProperty rdf:resource="http://cybox.mitre.org/objects/WindowsFilemapping#fileHandle"/>
                <owl:maxCardinality rdf:datatype="http://www.w3.org/2001/XMLSchema#nonNegativeInteger">1</owl:maxCardinality>
            </owl:Restriction>
        </rdfs:subClassOf>
        <rdfs:subClassOf>
            <owl:Restriction>
                <owl:onProperty rdf:resource="http://cybox.mitre.org/objects/WindowsFilemapping#handle"/>
                <owl:maxCardinality rdf:datatype="http://www.w3.org/2001/XMLSchema#nonNegativeInteger">1</owl:maxCardinality>
            </owl:Restriction>
        </rdfs:subClassOf>
        <rdfs:subClassOf>
            <owl:Restriction>
                <owl:onProperty rdf:resource="http://cybox.mitre.org/objects/WindowsFilemapping#filemappingName"/>
                <owl:cardinality rdf:datatype="http://www.w3.org/2001/XMLSchema#nonNegativeInteger">1</owl:cardinality>
            </owl:Restriction>
        </rdfs:subClassOf>
        <rdfs:subClassOf>
            <owl:Restriction>
                <owl:onProperty rdf:resource="http://cybox.mitre.org/objects/WindowsFilemapping#actualSize"/>
                <owl:maxCardinality rdf:datatype="http://www.w3.org/2001/XMLSchema#nonNegativeInteger">1</owl:maxCardinality>
            </owl:Restriction>
        </rdfs:subClassOf>
        <rdfs:subClassOf>
            <owl:Restriction>
                <owl:onProperty rdf:resource="http://cybox.mitre.org/objects/WindowsFilemapping#maximumSize"/>
                <owl:maxCardinality rdf:datatype="http://www.w3.org/2001/XMLSchema#nonNegativeInteger">1</owl:maxCardinality>
            </owl:Restriction>
        </rdfs:subClassOf>
        <rdfs:subClassOf>
            <owl:Restriction>
                <owl:onProperty rdf:resource="http://cybox.mitre.org/objects/WindowsFilemapping#pageProtectionValue"/>
                <owl:maxCardinality rdf:datatype="http://www.w3.org/2001/XMLSchema#nonNegativeInteger">1</owl:maxCardinality>
            </owl:Restriction>
        </rdfs:subClassOf>
        <rdfs:subClassOf>
            <owl:Restriction>
                <owl:onProperty rdf:resource="http://cybox.mitre.org/objects/WindowsFilemapping#securityAttributes"/>
                <owl:maxCardinality rdf:datatype="http://www.w3.org/2001/XMLSchema#nonNegativeInteger">1</owl:maxCardinality>
            </owl:Restriction>
        </rdfs:subClassOf>
        <rdfs:comment>Characterize Windows file mapping objects.</rdfs:comment>
        <rdfs:isDefinedBy rdf:resource="http://cybox.mitre.org/objects/WindowsFilemapping"/>
        <rdfs:label>Windows Filemapping</rdfs:label>
    </owl:Class>
    


</rdf:RDF>



<!-- Generated by the OWL API (version 4.2.6.20160910-2108) https://github.com/owlcs/owlapi -->

