<?xml version="1.0"?>
<rdf:RDF
    xmlns:rdf="http://www.w3.org/1999/02/22-rdf-syntax-ns#"
    xmlns:winPrefetchObj="http://cybox.mitre.org/objects/WindowsPrefetch#"
    xmlns:owl="http://www.w3.org/2002/07/owl#"
    xmlns:xsd="http://www.w3.org/2001/XMLSchema#"
    
    xmlns:rdfs="http://www.w3.org/2000/01/rdf-schema#"
  xml:base="http://cybox.mitre.org/objects/WindowsPrefetch">
  <owl:Ontology rdf:about="http://cybox.mitre.org/objects/WindowsPrefetch">
    <owl:versionInfo rdf:datatype="http://www.w3.org/2001/XMLSchema#string"
    >2.1.0-000</owl:versionInfo>
    <rdfs:comment >This ontology provides a vocabulary and representation of a Windows Prefetch for the  Cyber Observable eXpression (CybOX).  &#xD;
&#xD;
CybOX  provides a common mechansim (structure and content) to convey the full range of potential cyber observable information and strives to be fully expressive, flexible, extensible, automatable, and as human-readable as possible.&#xD;
&#xD;
The ontology is based on the CybOX Windows Prefetch object schema maintained by The MITRE Corporation copyright 2012-2014.  The version number of the ontology is kept in sync with the schema in order to more easily relate between the ontology and the corresponding schema version.&#xD;
&#xD;
Copyright (c) 2014, DaedaFusion, LLC.  All rights reserved.</rdfs:comment>
    <rdfs:label >Cyber Observable eXpression (CybOX) Windows Prefetch Ontology</rdfs:label>
    
    <owl:imports rdf:resource="http://cybox.mitre.org/cybox_core"/>
    <owl:imports rdf:resource="http://cybox.mitre.org/objects/Volume"/>
    <owl:imports rdf:resource="http://cybox.mitre.org/objects/Device"/>
    <owl:imports rdf:resource="http://cybox.mitre.org/objects/File"/>
  </owl:Ontology>
  <owl:Class rdf:ID="WindowsPrefetch">
    <rdfs:subClassOf>
      <owl:Restriction>
        <owl:onProperty>
          <owl:DatatypeProperty rdf:ID="lastRunDateTime"/>
        </owl:onProperty>
        <owl:maxCardinality rdf:datatype="http://www.w3.org/2001/XMLSchema#nonNegativeInteger"
        >1</owl:maxCardinality>
      </owl:Restriction>
    </rdfs:subClassOf>
    <rdfs:subClassOf rdf:resource="http://cybox.mitre.org/cybox_core#Object"/>
    <!-- <rdfs:subClassOf>
      <owl:Restriction>
        <owl:onProperty rdf:resource="http://cybox.mitre.org/cybox_core#physicalLocation"/>
        <owl:maxCardinality rdf:datatype="http://www.w3.org/2001/XMLSchema#nonNegativeInteger"
        >1</owl:maxCardinality>
      </owl:Restriction>
    </rdfs:subClassOf> -->
    
<!--     <rdfs:comment >Characterize entries in the Windows prefetch files. &#xD;
&#xD;
Starting with Windows XP, prefetching was introduced to speed up application startup. The prefetch object draws upon the descriptions and XML sample at http://www.forensicswiki.org/wiki/Prefetch_XML.</rdfs:comment>
    <rdfs:subClassOf>
      <owl:Restriction>
        <owl:onProperty rdf:resource="http://cybox.mitre.org/cybox_core#definedEffect"/>
        <owl:maxCardinality rdf:datatype="http://www.w3.org/2001/XMLSchema#nonNegativeInteger"
        >1</owl:maxCardinality>
      </owl:Restriction>
    </rdfs:subClassOf> -->
    
  <!--   <rdfs:subClassOf>
      <owl:Restriction>
        <owl:onProperty rdf:resource="http://cybox.mitre.org/cybox_core#hasChanged"/>
        <owl:maxCardinality rdf:datatype="http://www.w3.org/2001/XMLSchema#nonNegativeInteger"
        >1</owl:maxCardinality>
      </owl:Restriction>
    </rdfs:subClassOf> -->
    
    <rdfs:subClassOf>
      <owl:Restriction>
        <owl:onProperty>
          <owl:DatatypeProperty rdf:ID="applicationFilename"/>
        </owl:onProperty>
        <owl:cardinality rdf:datatype="http://www.w3.org/2001/XMLSchema#nonNegativeInteger"
        >1</owl:cardinality>
      </owl:Restriction>
    </rdfs:subClassOf>
    <rdfs:subClassOf>
      <owl:Restriction>
        <owl:onProperty>
          <owl:DatatypeProperty rdf:ID="prefetchHash"/>
        </owl:onProperty>
        <owl:cardinality rdf:datatype="http://www.w3.org/2001/XMLSchema#nonNegativeInteger"
        >1</owl:cardinality>
      </owl:Restriction>
    </rdfs:subClassOf>
    <rdfs:subClassOf>
      <owl:Restriction>
        <owl:onProperty>
          <owl:DatatypeProperty rdf:ID="timesExecuted"/>
        </owl:onProperty>
        <owl:maxCardinality rdf:datatype="http://www.w3.org/2001/XMLSchema#nonNegativeInteger"
        >1</owl:maxCardinality>
      </owl:Restriction>
    </rdfs:subClassOf>
   <!--  <rdfs:subClassOf>
      <owl:Restriction>
        <owl:onProperty rdf:resource="http://cybox.mitre.org/cybox_core#discoveryMethod"/>
        <owl:maxCardinality rdf:datatype="http://www.w3.org/2001/XMLSchema#nonNegativeInteger"
        >1</owl:maxCardinality>
      </owl:Restriction>
    </rdfs:subClassOf> -->
    <rdfs:subClassOf>
      <owl:Restriction>
        <owl:onProperty>
          <owl:DatatypeProperty rdf:ID="firstRunDateTime"/>
        </owl:onProperty>
        <owl:maxCardinality rdf:datatype="http://www.w3.org/2001/XMLSchema#nonNegativeInteger"
        >1</owl:maxCardinality>
      </owl:Restriction>
    </rdfs:subClassOf>
<!--     <rdfs:subClassOf>
      <owl:Restriction>
        <owl:onProperty rdf:resource="http://cybox.mitre.org/cybox_core#description"/>
        <owl:maxCardinality rdf:datatype="http://www.w3.org/2001/XMLSchema#nonNegativeInteger"
        >1</owl:maxCardinality>
      </owl:Restriction>
    </rdfs:subClassOf> -->
   <!--  <rdfs:subClassOf>
      <owl:Restriction>
        <owl:onProperty rdf:resource="http://cybox.mitre.org/cyboxCommon#id"/>
        <owl:cardinality rdf:datatype="http://www.w3.org/2001/XMLSchema#nonNegativeInteger"
        >1</owl:cardinality>
      </owl:Restriction>
    </rdfs:subClassOf> -->
<!--     <rdfs:label >Windows Prefetch</rdfs:label>
    <rdfs:isDefinedBy rdf:resource=""/> -->
   <!--  <rdfs:subClassOf>
      <owl:Restriction>
        <owl:onProperty rdf:resource="http://cybox.mitre.org/cybox_core#state"/>
        <owl:maxCardinality rdf:datatype="http://www.w3.org/2001/XMLSchema#nonNegativeInteger"
        >1</owl:maxCardinality>
      </owl:Restriction>
    </rdfs:subClassOf> -->
  </owl:Class>
  <owl:ObjectProperty rdf:ID="accessedFiles">
    <rdfs:comment >Specifies the files (e.g., DLLs and other support files) used by the application during startup.</rdfs:comment>
    <rdfs:label >Accessed Files</rdfs:label>
    
    <rdfs:isDefinedBy rdf:resource=""/>
    <rdfs:domain rdf:resource="#WindowsPrefetch"/>
    <rdfs:range rdf:resource="http://cybox.mitre.org/objects/File#WindowsFile"/>
  </owl:ObjectProperty>
  <owl:ObjectProperty rdf:ID="volume.deviceItems">
    <rdfs:range rdf:resource="http://cybox.mitre.org/objects/Device#Device"/>
    <rdfs:isDefinedBy rdf:resource=""/>
    <rdfs:domain rdf:resource="#WindowsPrefetch"/>
    
    <rdfs:comment >Specifies the device that the prefetch application was run from. The only item in the prefetch file is the device serial number.</rdfs:comment>
    <rdfs:label >Volume Device Items</rdfs:label>
  </owl:ObjectProperty>
  <owl:ObjectProperty rdf:ID="volume.volumeItems">
    
    <rdfs:isDefinedBy rdf:resource=""/>
    <rdfs:domain rdf:resource="#WindowsPrefetch"/>
    <rdfs:comment >Specifies the volume that the prefetch application was run from. The only item in the prefecth file is the volume name.</rdfs:comment>
    <rdfs:range rdf:resource="http://cybox.mitre.org/objects/Volume#WindowsVolume"/>
    <rdfs:label >Volume Items</rdfs:label>
  </owl:ObjectProperty>
  <owl:DatatypeProperty rdf:ID="accessedDirectories">
    <rdfs:label >Accessed Directories</rdfs:label>
    
    <rdfs:isDefinedBy rdf:resource=""/>
    <rdfs:range rdf:resource="http://www.w3.org/2001/XMLSchema#string"/>
    <rdfs:domain rdf:resource="#WindowsPrefetch"/>
    <rdfs:comment >Specifies the directories accessed by the prefetch application during startup.</rdfs:comment>
  </owl:DatatypeProperty>
  <owl:DatatypeProperty rdf:about="#applicationFilename">
    <rdfs:label >Application Filename</rdfs:label>
    
    <rdfs:isDefinedBy rdf:resource=""/>
    <rdfs:range rdf:resource="http://www.w3.org/2001/XMLSchema#string"/>
    <rdfs:domain rdf:resource="#WindowsPrefetch"/>
    <rdfs:comment >Specifies the name of the executable of the prefetch file.</rdfs:comment>
  </owl:DatatypeProperty>
  <owl:DatatypeProperty rdf:about="#prefetchHash">
    <rdfs:label >Prefetch Hash</rdfs:label>
    
    <rdfs:isDefinedBy rdf:resource=""/>
    <rdfs:range rdf:resource="http://www.w3.org/2001/XMLSchema#string"/>
    <rdfs:domain rdf:resource="#WindowsPrefetch"/>
    <rdfs:comment >Specifies an eight character hash of the location from which the application was run.</rdfs:comment>
  </owl:DatatypeProperty>
  <owl:DatatypeProperty rdf:about="#lastRunDateTime">
    <rdfs:comment >Specifies the timestamp of when the prefetch application was last run.</rdfs:comment>
    <rdfs:domain rdf:resource="#WindowsPrefetch"/>
    <rdfs:range rdf:resource="http://www.w3.org/2001/XMLSchema#dateTime"/>
    <rdfs:isDefinedBy rdf:resource=""/>
    
    <rdfs:label >Last Run</rdfs:label>
  </owl:DatatypeProperty>
  <owl:DatatypeProperty rdf:about="#firstRunDateTime">
    <rdfs:comment >Specifies a timestamp of when the prefetch application was first run.</rdfs:comment>
    <rdfs:domain rdf:resource="#WindowsPrefetch"/>
    <rdfs:range rdf:resource="http://www.w3.org/2001/XMLSchema#dateTime"/>
    <rdfs:isDefinedBy rdf:resource=""/>
    
    <rdfs:label >First Run</rdfs:label>
  </owl:DatatypeProperty>
  <owl:DatatypeProperty rdf:about="#timesExecuted">
    <rdfs:label >Times Executed</rdfs:label>
    
    <rdfs:isDefinedBy rdf:resource=""/>
    <rdfs:range rdf:resource="http://www.w3.org/2001/XMLSchema#long"/>
    <rdfs:domain rdf:resource="#WindowsPrefetch"/>
    <rdfs:comment >Specifies the number of times the prefetch application has executed.</rdfs:comment>
  </owl:DatatypeProperty>
</rdf:RDF>

<!-- Created with TopBraid -->
