<?xml version="1.0"?>
<rdf:RDF xmlns="http://cybox.mitre.org/objects/WindowsCriticalSection#"
     xml:base="http://cybox.mitre.org/objects/WindowsCriticalSection"
     xmlns:rdf="http://www.w3.org/1999/02/22-rdf-syntax-ns#"
     xmlns:owl="http://www.w3.org/2002/07/owl#"
     xmlns:xml="http://www.w3.org/XML/1998/namespace"
     xmlns:winCriticalSectionObj="http://cybox.mitre.org/objects/WindowsCriticalSection#"
     xmlns:xsd="http://www.w3.org/2001/XMLSchema#"
     xmlns:rdfs="http://www.w3.org/2000/01/rdf-schema#">
    <owl:Ontology rdf:about="http://cybox.mitre.org/objects/WindowsCriticalSection">
        <owl:imports rdf:resource="http://cybox.mitre.org/cybox_core"/>
        <owl:versionInfo rdf:datatype="http://www.w3.org/2001/XMLSchema#string">2.1.0-000</owl:versionInfo>
        <rdfs:comment>This ontology provides a vocabulary and representation of a Windows Critical Section for the  Cyber Observable eXpression (CybOX).  

CybOX provides a common mechansim (structure and content) to convey the full range of potential cyber observable information and strives to be fully expressive, flexible, extensible, automatable, and as human-readable as possible.

The ontology is based on the CybOX Windows Critical Section object schema maintained by The MITRE Corporation copyright 2012-2014.  The version number of the ontology is kept in sync with the schema in order to more easily relate between the ontology and the corresponding schema version.

Copyright (c) 2014, DaedaFusion, LLC.  All rights reserved.</rdfs:comment>
        <rdfs:label>Cyber Observable eXpression (CybOX) Windows Critical Section Ontology</rdfs:label>
    </owl:Ontology>
    


    <!-- 
    ///////////////////////////////////////////////////////////////////////////////////////
    //
    // Data properties
    //
    ///////////////////////////////////////////////////////////////////////////////////////
     -->

    


    <!-- http://cybox.mitre.org/objects/WindowsCriticalSection#address -->

    <owl:DatatypeProperty rdf:about="http://cybox.mitre.org/objects/WindowsCriticalSection#address">
        <rdfs:range rdf:resource="http://www.w3.org/2001/XMLSchema#hexBinary"/>
        <rdfs:comment>Specifies the address of the code that crated the critical section object.</rdfs:comment>
        <rdfs:isDefinedBy rdf:resource="http://cybox.mitre.org/objects/WindowsCriticalSection"/>
        <rdfs:label>Address</rdfs:label>
    </owl:DatatypeProperty>
    


    <!-- http://cybox.mitre.org/objects/WindowsCriticalSection#spinCount -->

    <owl:DatatypeProperty rdf:about="http://cybox.mitre.org/objects/WindowsCriticalSection#spinCount">
        <rdfs:range rdf:resource="http://www.w3.org/2001/XMLSchema#nonNegativeInteger"/>
        <rdfs:comment>Specifies the spin count value for the critical section object.</rdfs:comment>
        <rdfs:isDefinedBy rdf:resource="http://cybox.mitre.org/objects/WindowsCriticalSection"/>
        <rdfs:label>Spin Count</rdfs:label>
    </owl:DatatypeProperty>
    


    <!-- 
    ///////////////////////////////////////////////////////////////////////////////////////
    //
    // Classes
    //
    ///////////////////////////////////////////////////////////////////////////////////////
     -->

    


    <!-- http://cybox.mitre.org/objects/WindowsCriticalSection#WindowsCriticalSection -->

    <owl:Class rdf:about="http://cybox.mitre.org/objects/WindowsCriticalSection#WindowsCriticalSection">
        <rdfs:subClassOf>
            <owl:Restriction>
                <owl:onProperty rdf:resource="http://cybox.mitre.org/objects/WindowsCriticalSection#address"/>
                <owl:cardinality rdf:datatype="http://www.w3.org/2001/XMLSchema#nonNegativeInteger">1</owl:cardinality>
            </owl:Restriction>
        </rdfs:subClassOf>
        <rdfs:subClassOf>
            <owl:Restriction>
                <owl:onProperty rdf:resource="http://cybox.mitre.org/objects/WindowsCriticalSection#spinCount"/>
                <owl:maxCardinality rdf:datatype="http://www.w3.org/2001/XMLSchema#nonNegativeInteger">1</owl:maxCardinality>
            </owl:Restriction>
        </rdfs:subClassOf>
        <rdfs:comment>Characterizes a Windows Critical Section</rdfs:comment>
        <rdfs:isDefinedBy rdf:resource="http://cybox.mitre.org/objects/WindowsCriticalSection"/>
        <rdfs:label>Windows Critical Section</rdfs:label>
    </owl:Class>
</rdf:RDF>



<!-- Generated by the OWL API (version 4.2.6.20160910-2108) https://github.com/owlcs/owlapi -->

