<?xml version="1.0"?>
<rdf:RDF xmlns="http://cybox.mitre.org/objects/WindowsWaitableTimer#"
     xml:base="http://cybox.mitre.org/objects/WindowsWaitableTimer"
     xmlns:winWaitTimerObj="http://cybox.mitre.org/objects/WindowsWaitableTimer#"
     xmlns:rdf="http://www.w3.org/1999/02/22-rdf-syntax-ns#"
     xmlns:owl="http://www.w3.org/2002/07/owl#"
     xmlns:xml="http://www.w3.org/XML/1998/namespace"
     xmlns:xsd="http://www.w3.org/2001/XMLSchema#"
     xmlns:rdfs="http://www.w3.org/2000/01/rdf-schema#">
    <owl:Ontology rdf:about="http://cybox.mitre.org/objects/WindowsWaitableTimer">
        <owl:imports rdf:resource="http://cybox.mitre.org/cybox_core"/>
        <owl:imports rdf:resource="http://cybox.mitre.org/objects/WindowsHandle"/>
        <rdfs:label>Cyber Observable eXpression (CybOX) Windows Waitable Timer Ontology</rdfs:label>
        <owl:versionInfo rdf:datatype="http://www.w3.org/2001/XMLSchema#string">2.1.0-000</owl:versionInfo>
        <rdfs:comment>This ontology provides a vocabulary and representation of an Windows Waitable Timer for the  Cyber Observable eXpression (CybOX).  

CybOX  provides a common mechansim (structure and content) to convey the full range of potential cyber observable information and strives to be fully expressive, flexible, extensible, automatable, and as human-readable as possible.

The ontology is based on the CybOX Windows Waitable Timer object schema maintained by The MITRE Corporation copyright 2012-2014.  The version number of the ontology is kept in sync with the schema in order to more easily relate between the ontology and the corresponding schema version.

Copyright (c) 2014, DaedaFusion, LLC.  All rights reserved.</rdfs:comment>
    </owl:Ontology>
    


    <!-- 
    ///////////////////////////////////////////////////////////////////////////////////////
    //
    // Object Properties
    //
    ///////////////////////////////////////////////////////////////////////////////////////
     -->

    


    <!-- http://cybox.mitre.org/objects/WindowsWaitableTimer#handle -->

    <owl:ObjectProperty rdf:about="http://cybox.mitre.org/objects/WindowsWaitableTimer#handle">
        <rdfs:domain rdf:resource="http://cybox.mitre.org/objects/WindowsWaitableTimer#WindowsWaitableTimer"/>
        <rdfs:range rdf:resource="http://cybox.mitre.org/objects/WindowsHandle#WindowsHandle"/>
        <rdfs:comment>Specifies the handle to the Windows waitable timer object.</rdfs:comment>
        <rdfs:isDefinedBy rdf:datatype="http://www.w3.org/2001/XMLSchema#string">&lt;http://cybox.mitre.org/objects/WindowsWaitableTimer&gt;</rdfs:isDefinedBy>
        <rdfs:label>Handle</rdfs:label>
    </owl:ObjectProperty>
    


    <!-- 
    ///////////////////////////////////////////////////////////////////////////////////////
    //
    // Data properties
    //
    ///////////////////////////////////////////////////////////////////////////////////////
     -->

    


    <!-- http://cybox.mitre.org/objects/WindowsWaitableTimer#securityAttributes -->

    <owl:DatatypeProperty rdf:about="http://cybox.mitre.org/objects/WindowsWaitableTimer#securityAttributes">
        <rdfs:domain rdf:resource="http://cybox.mitre.org/objects/WindowsWaitableTimer#WindowsWaitableTimer"/>
        <rdfs:range rdf:resource="http://www.w3.org/2001/XMLSchema#string"/>
        <rdfs:comment>Specifies the security attributes for the Windows waitable timer object.</rdfs:comment>
        <rdfs:isDefinedBy rdf:resource="http://cybox.mitre.org/objects/WindowsWaitableTimer"/>
        <rdfs:label>Security Attributes</rdfs:label>
    </owl:DatatypeProperty>
    


    <!-- http://cybox.mitre.org/objects/WindowsWaitableTimer#waitableTimerName -->

    <owl:DatatypeProperty rdf:about="http://cybox.mitre.org/objects/WindowsWaitableTimer#waitableTimerName">
        <rdfs:domain rdf:resource="http://cybox.mitre.org/objects/WindowsWaitableTimer#WindowsWaitableTimer"/>
        <rdfs:range rdf:resource="http://www.w3.org/2001/XMLSchema#string"/>
        <rdfs:comment>Specifies the name of the Windows waitable timer object.</rdfs:comment>
        <rdfs:isDefinedBy rdf:resource="http://cybox.mitre.org/objects/WindowsWaitableTimer"/>
        <rdfs:label>Waitable Timer Name</rdfs:label>
    </owl:DatatypeProperty>
    


    <!-- http://cybox.mitre.org/objects/WindowsWaitableTimer#waitableTimerType -->

    <owl:DatatypeProperty rdf:about="http://cybox.mitre.org/objects/WindowsWaitableTimer#waitableTimerType">
        <rdfs:domain rdf:resource="http://cybox.mitre.org/objects/WindowsWaitableTimer#WindowsWaitableTimer"/>
        <rdfs:range rdf:resource="http://www.w3.org/2001/XMLSchema#string"/>
        <rdfs:comment>Specifies the type of the windows waitable timer object.</rdfs:comment>
        <rdfs:isDefinedBy rdf:resource="http://cybox.mitre.org/objects/WindowsWaitableTimer"/>
        <rdfs:label>Waitable Timer Type</rdfs:label>
    </owl:DatatypeProperty>
    


    <!-- 
    ///////////////////////////////////////////////////////////////////////////////////////
    //
    // Classes
    //
    ///////////////////////////////////////////////////////////////////////////////////////
     -->

    


   
    <!-- http://cybox.mitre.org/objects/WindowsWaitableTimer#WindowsWaitableTimer -->

    <owl:Class rdf:about="http://cybox.mitre.org/objects/WindowsWaitableTimer#WindowsWaitableTimer">
        <rdfs:subClassOf rdf:resource="http://cybox.mitre.org/cybox_core#Object"/>
        <rdfs:subClassOf>
            <owl:Restriction>
                <owl:onProperty rdf:resource="http://cybox.mitre.org/objects/WindowsWaitableTimer#handle"/>
                <owl:maxCardinality rdf:datatype="http://www.w3.org/2001/XMLSchema#nonNegativeInteger">1</owl:maxCardinality>
            </owl:Restriction>
        </rdfs:subClassOf>
        <rdfs:subClassOf>
            <owl:Restriction>
                <owl:onProperty rdf:resource="http://cybox.mitre.org/objects/WindowsWaitableTimer#waitableTimerName"/>
                <owl:cardinality rdf:datatype="http://www.w3.org/2001/XMLSchema#nonNegativeInteger">1</owl:cardinality>
            </owl:Restriction>
        </rdfs:subClassOf>
        <rdfs:subClassOf>
            <owl:Restriction>
                <owl:onProperty rdf:resource="http://cybox.mitre.org/objects/WindowsWaitableTimer#securityAttributes"/>
                <owl:maxCardinality rdf:datatype="http://www.w3.org/2001/XMLSchema#nonNegativeInteger">1</owl:maxCardinality>
            </owl:Restriction>
        </rdfs:subClassOf>
        <rdfs:subClassOf>
            <owl:Restriction>
                <owl:onProperty rdf:resource="http://cybox.mitre.org/objects/WindowsWaitableTimer#waitableTimerType"/>
                <owl:maxCardinality rdf:datatype="http://www.w3.org/2001/XMLSchema#nonNegativeInteger">1</owl:maxCardinality>
            </owl:Restriction>
        </rdfs:subClassOf>
        <rdfs:comment>Characterize Windows waitable timer (synchronization) objects.</rdfs:comment>
        <rdfs:isDefinedBy rdf:resource="http://cybox.mitre.org/objects/WindowsWaitableTimer"/>
        <rdfs:label>Windows Waitable Timer</rdfs:label>
    </owl:Class>
</rdf:RDF>



<!-- Generated by the OWL API (version 4.2.6.20160910-2108) https://github.com/owlcs/owlapi -->

