<?xml version="1.0"?>
<rdf:RDF xmlns="http://cybox.mitre.org/objects/WindowsNetworkShare#"
     xml:base="http://cybox.mitre.org/objects/WindowsNetworkShare"
     xmlns:winNetShareObj="http://cybox.mitre.org/objects/WindowsNetworkShare#"
     xmlns:rdf="http://www.w3.org/1999/02/22-rdf-syntax-ns#"
     xmlns:owl="http://www.w3.org/2002/07/owl#"
     xmlns:xml="http://www.w3.org/XML/1998/namespace"
     xmlns:xsd="http://www.w3.org/2001/XMLSchema#"
     xmlns:rdfs="http://www.w3.org/2000/01/rdf-schema#">
    <owl:Ontology rdf:about="http://cybox.mitre.org/objects/WindowsNetworkShare">
        <owl:imports rdf:resource="http://cybox.mitre.org/cybox_core"/>
        <owl:versionInfo rdf:datatype="http://www.w3.org/2001/XMLSchema#string">2.1.0-000</owl:versionInfo>
        <rdfs:label>Cyber Observable eXpression (CybOX) Windows Network Share Ontology</rdfs:label>
        <rdfs:comment>This ontology provides a vocabulary and representation of a Windows Network Share for the  Cyber Observable eXpression (CybOX).  

CybOX  provides a common mechansim (structure and content) to convey the full range of potential cyber observable information and strives to be fully expressive, flexible, extensible, automatable, and as human-readable as possible.

The ontology is based on the CybOX Windows Network Share object schema maintained by The MITRE Corporation copyright 2012-2014.  The version number of the ontology is kept in sync with the schema in order to more easily relate between the ontology and the corresponding schema version.

Copyright (c) 2014, DaedaFusion, LLC.  All rights reserved.</rdfs:comment>
    </owl:Ontology>
    


    <!-- 
    ///////////////////////////////////////////////////////////////////////////////////////
    //
    // Data properties
    //
    ///////////////////////////////////////////////////////////////////////////////////////
     -->

    


    <!-- http://cybox.mitre.org/objects/WindowsNetworkShare#currentUses -->

    <owl:DatatypeProperty rdf:about="http://cybox.mitre.org/objects/WindowsNetworkShare#currentUses">
        <rdfs:domain rdf:resource="http://cybox.mitre.org/objects/WindowsNetworkShare#WindowsNetworkShare"/>
        <rdfs:range rdf:resource="http://www.w3.org/2001/XMLSchema#nonNegativeInteger"/>
        <rdfs:comment>Specifies the current number of uses of the network share.</rdfs:comment>
        <rdfs:isDefinedBy rdf:resource="http://cybox.mitre.org/objects/WindowsNetworkShare"/>
        <rdfs:label>Current Uses</rdfs:label>
    </owl:DatatypeProperty>
    


    <!-- http://cybox.mitre.org/objects/WindowsNetworkShare#localPath -->

    <owl:DatatypeProperty rdf:about="http://cybox.mitre.org/objects/WindowsNetworkShare#localPath">
        <rdfs:domain rdf:resource="http://cybox.mitre.org/objects/WindowsNetworkShare#WindowsNetworkShare"/>
        <rdfs:range rdf:resource="http://www.w3.org/2001/XMLSchema#string"/>
        <rdfs:comment>Specifies the fully-qualified path on the local system to the network share.</rdfs:comment>
        <rdfs:isDefinedBy rdf:resource="http://cybox.mitre.org/objects/WindowsNetworkShare"/>
        <rdfs:label>Local Path</rdfs:label>
    </owl:DatatypeProperty>
    


    <!-- http://cybox.mitre.org/objects/WindowsNetworkShare#maxUses -->

    <owl:DatatypeProperty rdf:about="http://cybox.mitre.org/objects/WindowsNetworkShare#maxUses">
        <rdfs:domain rdf:resource="http://cybox.mitre.org/objects/WindowsNetworkShare#WindowsNetworkShare"/>
        <rdfs:range rdf:resource="http://www.w3.org/2001/XMLSchema#nonNegativeInteger"/>
        <rdfs:comment>Specifies the maximum number of concurrent connections to the network share.</rdfs:comment>
        <rdfs:isDefinedBy rdf:resource="http://cybox.mitre.org/objects/WindowsNetworkShare"/>
        <rdfs:label>Max Uses</rdfs:label>
    </owl:DatatypeProperty>
    


    <!-- http://cybox.mitre.org/objects/WindowsNetworkShare#netName -->

    <owl:DatatypeProperty rdf:about="http://cybox.mitre.org/objects/WindowsNetworkShare#netName">
        <rdfs:domain rdf:resource="http://cybox.mitre.org/objects/WindowsNetworkShare#WindowsNetworkShare"/>
        <rdfs:range rdf:resource="http://www.w3.org/2001/XMLSchema#string"/>
        <rdfs:comment>Specifies the network name of the network share.</rdfs:comment>
        <rdfs:isDefinedBy rdf:resource="http://cybox.mitre.org/objects/WindowsNetworkShare"/>
        <rdfs:label>Net Name</rdfs:label>
    </owl:DatatypeProperty>
    


    <!-- http://cybox.mitre.org/objects/WindowsNetworkShare#netShareType -->

    <owl:DatatypeProperty rdf:about="http://cybox.mitre.org/objects/WindowsNetworkShare#netShareType">
        <rdfs:domain rdf:resource="http://cybox.mitre.org/objects/WindowsNetworkShare#WindowsNetworkShare"/>
        <rdfs:range rdf:resource="http://www.w3.org/2001/XMLSchema#string"/>
        <rdfs:comment>Specifies the type of the network share.</rdfs:comment>
        <rdfs:isDefinedBy rdf:resource="http://cybox.mitre.org/objects/WindowsNetworkShare"/>
        <rdfs:label>Net Share Type</rdfs:label>
    </owl:DatatypeProperty>
    


    <!-- http://cybox.mitre.org/objects/WindowsNetworkShare#permission.ACCESS_ALL -->

    <owl:DatatypeProperty rdf:about="http://cybox.mitre.org/objects/WindowsNetworkShare#permission.ACCESS_ALL">
        <rdfs:domain rdf:resource="http://cybox.mitre.org/objects/WindowsNetworkShare#WindowsNetworkShare"/>
        <rdfs:range rdf:resource="http://www.w3.org/2001/XMLSchema#boolean"/>
        <rdfs:comment>Specifies the permission to read, write, create, execute, and delete resources, and to modify their attributes and permissions.</rdfs:comment>
        <rdfs:isDefinedBy rdf:resource="http://cybox.mitre.org/objects/WindowsNetworkShare"/>
        <rdfs:label>ACCESS_ALL</rdfs:label>
    </owl:DatatypeProperty>
    


    <!-- http://cybox.mitre.org/objects/WindowsNetworkShare#permission.ACCESS_ATRIB -->

    <owl:DatatypeProperty rdf:about="http://cybox.mitre.org/objects/WindowsNetworkShare#permission.ACCESS_ATRIB">
        <rdfs:domain rdf:resource="http://cybox.mitre.org/objects/WindowsNetworkShare#WindowsNetworkShare"/>
        <rdfs:range rdf:resource="http://www.w3.org/2001/XMLSchema#boolean"/>
        <rdfs:comment>Specifies the permission to modify the resource&apos;s attributes (such as the date and time when a file was last modified).</rdfs:comment>
        <rdfs:isDefinedBy rdf:resource="http://cybox.mitre.org/objects/WindowsNetworkShare"/>
        <rdfs:label>ACCESS_ATRIB</rdfs:label>
    </owl:DatatypeProperty>
    


    <!-- http://cybox.mitre.org/objects/WindowsNetworkShare#permission.ACCESS_CREATE -->

    <owl:DatatypeProperty rdf:about="http://cybox.mitre.org/objects/WindowsNetworkShare#permission.ACCESS_CREATE">
        <rdfs:domain rdf:resource="http://cybox.mitre.org/objects/WindowsNetworkShare#WindowsNetworkShare"/>
        <rdfs:range rdf:resource="http://www.w3.org/2001/XMLSchema#boolean"/>
        <rdfs:comment>Specifies the permission to create an instance of the resource (such as a file); data can be written to the resource as the resource is created.</rdfs:comment>
        <rdfs:isDefinedBy rdf:resource="http://cybox.mitre.org/objects/WindowsNetworkShare"/>
        <rdfs:label>ACCESS_CREATE</rdfs:label>
    </owl:DatatypeProperty>
    


    <!-- http://cybox.mitre.org/objects/WindowsNetworkShare#permission.ACCESS_DELETE -->

    <owl:DatatypeProperty rdf:about="http://cybox.mitre.org/objects/WindowsNetworkShare#permission.ACCESS_DELETE">
        <rdfs:domain rdf:resource="http://cybox.mitre.org/objects/WindowsNetworkShare#WindowsNetworkShare"/>
        <rdfs:range rdf:resource="http://www.w3.org/2001/XMLSchema#boolean"/>
        <rdfs:comment>Specifies the permission to delete the resource.</rdfs:comment>
        <rdfs:isDefinedBy rdf:resource="http://cybox.mitre.org/objects/WindowsNetworkShare"/>
        <rdfs:label>ACCESS_DELETE</rdfs:label>
    </owl:DatatypeProperty>
    


    <!-- http://cybox.mitre.org/objects/WindowsNetworkShare#permission.ACCESS_EXEC -->

    <owl:DatatypeProperty rdf:about="http://cybox.mitre.org/objects/WindowsNetworkShare#permission.ACCESS_EXEC">
        <rdfs:domain rdf:resource="http://cybox.mitre.org/objects/WindowsNetworkShare#WindowsNetworkShare"/>
        <rdfs:range rdf:resource="http://www.w3.org/2001/XMLSchema#boolean"/>
        <rdfs:comment>Specifies the permission to execute the resource.</rdfs:comment>
        <rdfs:isDefinedBy rdf:resource="http://cybox.mitre.org/objects/WindowsNetworkShare"/>
        <rdfs:label>ACCESS_EXEC</rdfs:label>
    </owl:DatatypeProperty>
    


    <!-- http://cybox.mitre.org/objects/WindowsNetworkShare#permission.ACCESS_PERM -->

    <owl:DatatypeProperty rdf:about="http://cybox.mitre.org/objects/WindowsNetworkShare#permission.ACCESS_PERM">
        <rdfs:domain rdf:resource="http://cybox.mitre.org/objects/WindowsNetworkShare#WindowsNetworkShare"/>
        <rdfs:range rdf:resource="http://www.w3.org/2001/XMLSchema#boolean"/>
        <rdfs:comment>Specifies the permission to modify the permissions (read, write, create, execute, and delete) assigned to a resource for a user or application.</rdfs:comment>
        <rdfs:isDefinedBy rdf:resource="http://cybox.mitre.org/objects/WindowsNetworkShare"/>
        <rdfs:label>ACCESS_PERM</rdfs:label>
    </owl:DatatypeProperty>
    


    <!-- http://cybox.mitre.org/objects/WindowsNetworkShare#permission.ACCESS_READ -->

    <owl:DatatypeProperty rdf:about="http://cybox.mitre.org/objects/WindowsNetworkShare#permission.ACCESS_READ">
        <rdfs:domain rdf:resource="http://cybox.mitre.org/objects/WindowsNetworkShare#WindowsNetworkShare"/>
        <rdfs:range rdf:resource="http://www.w3.org/2001/XMLSchema#boolean"/>
        <rdfs:comment>Specifies the permission to read data from a resource and, by default, to execute the resource.</rdfs:comment>
        <rdfs:isDefinedBy rdf:resource="http://cybox.mitre.org/objects/WindowsNetworkShare"/>
        <rdfs:label>ACCESS_READ</rdfs:label>
    </owl:DatatypeProperty>
    


    <!-- http://cybox.mitre.org/objects/WindowsNetworkShare#permission.ACCESS_WRITE -->

    <owl:DatatypeProperty rdf:about="http://cybox.mitre.org/objects/WindowsNetworkShare#permission.ACCESS_WRITE">
        <rdfs:domain rdf:resource="http://cybox.mitre.org/objects/WindowsNetworkShare#WindowsNetworkShare"/>
        <rdfs:range rdf:resource="http://www.w3.org/2001/XMLSchema#boolean"/>
        <rdfs:comment>specifies the permission to write data to the resource.</rdfs:comment>
        <rdfs:isDefinedBy rdf:resource="http://cybox.mitre.org/objects/WindowsNetworkShare"/>
        <rdfs:label>ACCESS_WRITE</rdfs:label>
    </owl:DatatypeProperty>
    


    <!-- 
    ///////////////////////////////////////////////////////////////////////////////////////
    //
    // Classes
    //
    ///////////////////////////////////////////////////////////////////////////////////////
     -->

    


    <!-- http://cybox.mitre.org/cybox_core#Object -->

    <owl:Class rdf:about="http://cybox.mitre.org/cybox_core#Object"/>
    


    <!-- http://cybox.mitre.org/objects/WindowsNetworkShare#WindowsNetworkShare -->

    <owl:Class rdf:about="http://cybox.mitre.org/objects/WindowsNetworkShare#WindowsNetworkShare">
        <rdfs:subClassOf rdf:resource="http://cybox.mitre.org/cybox_core#Object"/>
        <rdfs:subClassOf>
            <owl:Restriction>
                <owl:onProperty rdf:resource="http://cybox.mitre.org/objects/WindowsNetworkShare#localPath"/>
                <owl:cardinality rdf:datatype="http://www.w3.org/2001/XMLSchema#nonNegativeInteger">1</owl:cardinality>
            </owl:Restriction>
        </rdfs:subClassOf>
        <rdfs:subClassOf>
            <owl:Restriction>
                <owl:onProperty rdf:resource="http://cybox.mitre.org/objects/WindowsNetworkShare#netName"/>
                <owl:cardinality rdf:datatype="http://www.w3.org/2001/XMLSchema#nonNegativeInteger">1</owl:cardinality>
            </owl:Restriction>
        </rdfs:subClassOf>
        <rdfs:subClassOf>
            <owl:Restriction>
                <owl:onProperty rdf:resource="http://cybox.mitre.org/objects/WindowsNetworkShare#netShareType"/>
                <owl:cardinality rdf:datatype="http://www.w3.org/2001/XMLSchema#nonNegativeInteger">1</owl:cardinality>
            </owl:Restriction>
        </rdfs:subClassOf>
        <rdfs:subClassOf>
            <owl:Restriction>
                <owl:onProperty rdf:resource="http://cybox.mitre.org/objects/WindowsNetworkShare#currentUses"/>
                <owl:maxCardinality rdf:datatype="http://www.w3.org/2001/XMLSchema#nonNegativeInteger">1</owl:maxCardinality>
            </owl:Restriction>
        </rdfs:subClassOf>
        <rdfs:subClassOf>
            <owl:Restriction>
                <owl:onProperty rdf:resource="http://cybox.mitre.org/objects/WindowsNetworkShare#maxUses"/>
                <owl:maxCardinality rdf:datatype="http://www.w3.org/2001/XMLSchema#nonNegativeInteger">1</owl:maxCardinality>
            </owl:Restriction>
        </rdfs:subClassOf>
        <rdfs:subClassOf>
            <owl:Restriction>
                <owl:onProperty rdf:resource="http://cybox.mitre.org/objects/WindowsNetworkShare#permission.ACCESS_ALL"/>
                <owl:maxCardinality rdf:datatype="http://www.w3.org/2001/XMLSchema#nonNegativeInteger">1</owl:maxCardinality>
            </owl:Restriction>
        </rdfs:subClassOf>
        <rdfs:subClassOf>
            <owl:Restriction>
                <owl:onProperty rdf:resource="http://cybox.mitre.org/objects/WindowsNetworkShare#permission.ACCESS_ATRIB"/>
                <owl:maxCardinality rdf:datatype="http://www.w3.org/2001/XMLSchema#nonNegativeInteger">1</owl:maxCardinality>
            </owl:Restriction>
        </rdfs:subClassOf>
        <rdfs:subClassOf>
            <owl:Restriction>
                <owl:onProperty rdf:resource="http://cybox.mitre.org/objects/WindowsNetworkShare#permission.ACCESS_CREATE"/>
                <owl:maxCardinality rdf:datatype="http://www.w3.org/2001/XMLSchema#nonNegativeInteger">1</owl:maxCardinality>
            </owl:Restriction>
        </rdfs:subClassOf>
        <rdfs:subClassOf>
            <owl:Restriction>
                <owl:onProperty rdf:resource="http://cybox.mitre.org/objects/WindowsNetworkShare#permission.ACCESS_DELETE"/>
                <owl:maxCardinality rdf:datatype="http://www.w3.org/2001/XMLSchema#nonNegativeInteger">1</owl:maxCardinality>
            </owl:Restriction>
        </rdfs:subClassOf>
        <rdfs:subClassOf>
            <owl:Restriction>
                <owl:onProperty rdf:resource="http://cybox.mitre.org/objects/WindowsNetworkShare#permission.ACCESS_EXEC"/>
                <owl:maxCardinality rdf:datatype="http://www.w3.org/2001/XMLSchema#nonNegativeInteger">1</owl:maxCardinality>
            </owl:Restriction>
        </rdfs:subClassOf>
        <rdfs:subClassOf>
            <owl:Restriction>
                <owl:onProperty rdf:resource="http://cybox.mitre.org/objects/WindowsNetworkShare#permission.ACCESS_PERM"/>
                <owl:maxCardinality rdf:datatype="http://www.w3.org/2001/XMLSchema#nonNegativeInteger">1</owl:maxCardinality>
            </owl:Restriction>
        </rdfs:subClassOf>
        <rdfs:subClassOf>
            <owl:Restriction>
                <owl:onProperty rdf:resource="http://cybox.mitre.org/objects/WindowsNetworkShare#permission.ACCESS_READ"/>
                <owl:maxCardinality rdf:datatype="http://www.w3.org/2001/XMLSchema#nonNegativeInteger">1</owl:maxCardinality>
            </owl:Restriction>
        </rdfs:subClassOf>
        <rdfs:subClassOf>
            <owl:Restriction>
                <owl:onProperty rdf:resource="http://cybox.mitre.org/objects/WindowsNetworkShare#permission.ACCESS_WRITE"/>
                <owl:maxCardinality rdf:datatype="http://www.w3.org/2001/XMLSchema#nonNegativeInteger">1</owl:maxCardinality>
            </owl:Restriction>
        </rdfs:subClassOf>
        <rdfs:comment>Characterize Windows network shares.</rdfs:comment>
        <rdfs:label>Windows Network Share</rdfs:label>
    </owl:Class>
</rdf:RDF>



<!-- Generated by the OWL API (version 4.2.6.20160910-2108) https://github.com/owlcs/owlapi -->

