<?xml version="1.0"?>
<rdf:RDF xmlns="http://cybox.mitre.org/objects/WindowsPrefetch#"
     xml:base="http://cybox.mitre.org/objects/WindowsPrefetch"
     xmlns:rdf="http://www.w3.org/1999/02/22-rdf-syntax-ns#"
     xmlns:owl="http://www.w3.org/2002/07/owl#"
     xmlns:xml="http://www.w3.org/XML/1998/namespace"
     xmlns:xsd="http://www.w3.org/2001/XMLSchema#"
     xmlns:rdfs="http://www.w3.org/2000/01/rdf-schema#"
     xmlns:winPrefetchObj="http://cybox.mitre.org/objects/WindowsPrefetch#">
    <owl:Ontology rdf:about="http://cybox.mitre.org/objects/WindowsPrefetch">
        <owl:imports rdf:resource="http://cybox.mitre.org/cybox_core"/>
        <owl:imports rdf:resource="http://cybox.mitre.org/objects/File"/>
        <owl:imports rdf:resource="http://cybox.mitre.org/objects/Volume"/>
        <owl:imports rdf:resource="http://cybox.mitre.org/objects/Device"/>
        <rdfs:label>Cyber Observable eXpression (CybOX) Windows Prefetch Ontology</rdfs:label>
        <owl:versionInfo rdf:datatype="http://www.w3.org/2001/XMLSchema#string">2.1.0-000</owl:versionInfo>
        <rdfs:comment>This ontology provides a vocabulary and representation of a Windows Prefetch for the  Cyber Observable eXpression (CybOX).  

CybOX  provides a common mechansim (structure and content) to convey the full range of potential cyber observable information and strives to be fully expressive, flexible, extensible, automatable, and as human-readable as possible.

The ontology is based on the CybOX Windows Prefetch object schema maintained by The MITRE Corporation copyright 2012-2014.  The version number of the ontology is kept in sync with the schema in order to more easily relate between the ontology and the corresponding schema version.

Copyright (c) 2014, DaedaFusion, LLC.  All rights reserved.</rdfs:comment>
    </owl:Ontology>
    


    <!-- 
    ///////////////////////////////////////////////////////////////////////////////////////
    //
    // Object Properties
    //
    ///////////////////////////////////////////////////////////////////////////////////////
     -->

    


    <!-- http://cybox.mitre.org/objects/WindowsPrefetch#accessedFiles -->

    <owl:ObjectProperty rdf:about="http://cybox.mitre.org/objects/WindowsPrefetch#accessedFiles">
        <rdfs:domain rdf:resource="http://cybox.mitre.org/objects/WindowsPrefetch#WindowsPrefetch"/>
        <rdfs:range rdf:resource="http://cybox.mitre.org/objects/File#WindowsFile"/>
        <rdfs:comment>Specifies the files (e.g., DLLs and other support files) used by the application during startup.</rdfs:comment>
        <rdfs:isDefinedBy rdf:resource="http://cybox.mitre.org/objects/WindowsPrefetch"/>
        <rdfs:label>Accessed Files</rdfs:label>
    </owl:ObjectProperty>
    


    <!-- http://cybox.mitre.org/objects/WindowsPrefetch#volume.deviceItems -->

    <owl:ObjectProperty rdf:about="http://cybox.mitre.org/objects/WindowsPrefetch#volume.deviceItems">
        <rdfs:domain rdf:resource="http://cybox.mitre.org/objects/WindowsPrefetch#WindowsPrefetch"/>
        <rdfs:range rdf:resource="http://cybox.mitre.org/objects/Device#Device"/>
        <rdfs:comment>Specifies the device that the prefetch application was run from. The only item in the prefetch file is the device serial number.</rdfs:comment>
        <rdfs:isDefinedBy rdf:resource="http://cybox.mitre.org/objects/WindowsPrefetch"/>
        <rdfs:label>Volume Device Items</rdfs:label>
    </owl:ObjectProperty>
    


    <!-- http://cybox.mitre.org/objects/WindowsPrefetch#volume.volumeItems -->

    <owl:ObjectProperty rdf:about="http://cybox.mitre.org/objects/WindowsPrefetch#volume.volumeItems">
        <rdfs:domain rdf:resource="http://cybox.mitre.org/objects/WindowsPrefetch#WindowsPrefetch"/>
        <rdfs:range rdf:resource="http://cybox.mitre.org/objects/Volume#WindowsVolume"/>
        <rdfs:comment>Specifies the volume that the prefetch application was run from. The only item in the prefecth file is the volume name.</rdfs:comment>
        <rdfs:isDefinedBy rdf:resource="http://cybox.mitre.org/objects/WindowsPrefetch"/>
        <rdfs:label>Volume Items</rdfs:label>
    </owl:ObjectProperty>
    


    <!-- 
    ///////////////////////////////////////////////////////////////////////////////////////
    //
    // Data properties
    //
    ///////////////////////////////////////////////////////////////////////////////////////
     -->

    


    <!-- http://cybox.mitre.org/objects/WindowsPrefetch#accessedDirectories -->

    <owl:DatatypeProperty rdf:about="http://cybox.mitre.org/objects/WindowsPrefetch#accessedDirectories">
        <rdfs:domain rdf:resource="http://cybox.mitre.org/objects/WindowsPrefetch#WindowsPrefetch"/>
        <rdfs:range rdf:resource="http://www.w3.org/2001/XMLSchema#string"/>
        <rdfs:comment>Specifies the directories accessed by the prefetch application during startup.</rdfs:comment>
        <rdfs:isDefinedBy rdf:resource="http://cybox.mitre.org/objects/WindowsPrefetch"/>
        <rdfs:label>Accessed Directories</rdfs:label>
    </owl:DatatypeProperty>
    


    <!-- http://cybox.mitre.org/objects/WindowsPrefetch#applicationFilename -->

    <owl:DatatypeProperty rdf:about="http://cybox.mitre.org/objects/WindowsPrefetch#applicationFilename">
        <rdfs:domain rdf:resource="http://cybox.mitre.org/objects/WindowsPrefetch#WindowsPrefetch"/>
        <rdfs:range rdf:resource="http://www.w3.org/2001/XMLSchema#string"/>
        <rdfs:comment>Specifies the name of the executable of the prefetch file.</rdfs:comment>
        <rdfs:isDefinedBy rdf:resource="http://cybox.mitre.org/objects/WindowsPrefetch"/>
        <rdfs:label>Application Filename</rdfs:label>
    </owl:DatatypeProperty>
    


    <!-- http://cybox.mitre.org/objects/WindowsPrefetch#firstRunDateTime -->

    <owl:DatatypeProperty rdf:about="http://cybox.mitre.org/objects/WindowsPrefetch#firstRunDateTime">
        <rdfs:domain rdf:resource="http://cybox.mitre.org/objects/WindowsPrefetch#WindowsPrefetch"/>
        <rdfs:range rdf:resource="http://www.w3.org/2001/XMLSchema#dateTime"/>
        <rdfs:comment>Specifies a timestamp of when the prefetch application was first run.</rdfs:comment>
        <rdfs:isDefinedBy rdf:resource="http://cybox.mitre.org/objects/WindowsPrefetch"/>
        <rdfs:label>First Run</rdfs:label>
    </owl:DatatypeProperty>
    


    <!-- http://cybox.mitre.org/objects/WindowsPrefetch#lastRunDateTime -->

    <owl:DatatypeProperty rdf:about="http://cybox.mitre.org/objects/WindowsPrefetch#lastRunDateTime">
        <rdfs:domain rdf:resource="http://cybox.mitre.org/objects/WindowsPrefetch#WindowsPrefetch"/>
        <rdfs:range rdf:resource="http://www.w3.org/2001/XMLSchema#dateTime"/>
        <rdfs:comment>Specifies the timestamp of when the prefetch application was last run.</rdfs:comment>
        <rdfs:isDefinedBy rdf:resource="http://cybox.mitre.org/objects/WindowsPrefetch"/>
        <rdfs:label>Last Run</rdfs:label>
    </owl:DatatypeProperty>
    


    <!-- http://cybox.mitre.org/objects/WindowsPrefetch#prefetchHash -->

    <owl:DatatypeProperty rdf:about="http://cybox.mitre.org/objects/WindowsPrefetch#prefetchHash">
        <rdfs:domain rdf:resource="http://cybox.mitre.org/objects/WindowsPrefetch#WindowsPrefetch"/>
        <rdfs:range rdf:resource="http://www.w3.org/2001/XMLSchema#string"/>
        <rdfs:comment>Specifies an eight character hash of the location from which the application was run.</rdfs:comment>
        <rdfs:isDefinedBy rdf:resource="http://cybox.mitre.org/objects/WindowsPrefetch"/>
        <rdfs:label>Prefetch Hash</rdfs:label>
    </owl:DatatypeProperty>
    


    <!-- http://cybox.mitre.org/objects/WindowsPrefetch#timesExecuted -->

    <owl:DatatypeProperty rdf:about="http://cybox.mitre.org/objects/WindowsPrefetch#timesExecuted">
        <rdfs:domain rdf:resource="http://cybox.mitre.org/objects/WindowsPrefetch#WindowsPrefetch"/>
        <rdfs:range rdf:resource="http://www.w3.org/2001/XMLSchema#long"/>
        <rdfs:comment>Specifies the number of times the prefetch application has executed.</rdfs:comment>
        <rdfs:isDefinedBy rdf:resource="http://cybox.mitre.org/objects/WindowsPrefetch"/>
        <rdfs:label>Times Executed</rdfs:label>
    </owl:DatatypeProperty>
    


    <!-- 
    ///////////////////////////////////////////////////////////////////////////////////////
    //
    // Classes
    //
    ///////////////////////////////////////////////////////////////////////////////////////
     -->

    


    <!-- http://cybox.mitre.org/objects/WindowsPrefetch#WindowsPrefetch -->

    <owl:Class rdf:about="http://cybox.mitre.org/objects/WindowsPrefetch#WindowsPrefetch">
        <rdfs:subClassOf rdf:resource="http://cybox.mitre.org/cybox_core#Object"/>
        <rdfs:subClassOf>
            <owl:Restriction>
                <owl:onProperty rdf:resource="http://cybox.mitre.org/objects/WindowsPrefetch#applicationFilename"/>
                <owl:cardinality rdf:datatype="http://www.w3.org/2001/XMLSchema#nonNegativeInteger">1</owl:cardinality>
            </owl:Restriction>
        </rdfs:subClassOf>
        <rdfs:subClassOf>
            <owl:Restriction>
                <owl:onProperty rdf:resource="http://cybox.mitre.org/objects/WindowsPrefetch#prefetchHash"/>
                <owl:cardinality rdf:datatype="http://www.w3.org/2001/XMLSchema#nonNegativeInteger">1</owl:cardinality>
            </owl:Restriction>
        </rdfs:subClassOf>
        <rdfs:subClassOf>
            <owl:Restriction>
                <owl:onProperty rdf:resource="http://cybox.mitre.org/objects/WindowsPrefetch#firstRunDateTime"/>
                <owl:maxCardinality rdf:datatype="http://www.w3.org/2001/XMLSchema#nonNegativeInteger">1</owl:maxCardinality>
            </owl:Restriction>
        </rdfs:subClassOf>
        <rdfs:subClassOf>
            <owl:Restriction>
                <owl:onProperty rdf:resource="http://cybox.mitre.org/objects/WindowsPrefetch#lastRunDateTime"/>
                <owl:maxCardinality rdf:datatype="http://www.w3.org/2001/XMLSchema#nonNegativeInteger">1</owl:maxCardinality>
            </owl:Restriction>
        </rdfs:subClassOf>
        <rdfs:subClassOf>
            <owl:Restriction>
                <owl:onProperty rdf:resource="http://cybox.mitre.org/objects/WindowsPrefetch#timesExecuted"/>
                <owl:maxCardinality rdf:datatype="http://www.w3.org/2001/XMLSchema#nonNegativeInteger">1</owl:maxCardinality>
            </owl:Restriction>
        </rdfs:subClassOf>
    </owl:Class>
</rdf:RDF>



<!-- Generated by the OWL API (version 4.2.6.20160910-2108) https://github.com/owlcs/owlapi -->

