<?xml version="1.0"?>
<rdf:RDF xmlns="http://cybox.mitre.org/objects/WindowsTask#"
     xml:base="http://cybox.mitre.org/objects/WindowsTask"
     xmlns:rdf="http://www.w3.org/1999/02/22-rdf-syntax-ns#"
     xmlns:owl="http://www.w3.org/2002/07/owl#"
     xmlns:xml="http://www.w3.org/XML/1998/namespace"
     xmlns:winTaskObj="http://cybox.mitre.org/objects/WindowsTask#"
     xmlns:xsd="http://www.w3.org/2001/XMLSchema#"
     xmlns:rdfs="http://www.w3.org/2000/01/rdf-schema#">
    <owl:Ontology rdf:about="http://cybox.mitre.org/objects/WindowsTask">
        <owl:imports rdf:resource="http://cybox.mitre.org/objects/EmailMessage"/>
        <owl:imports rdf:resource="http://cybox.mitre.org/cybox_core"/>
        <owl:versionInfo rdf:datatype="http://www.w3.org/2001/XMLSchema#string">2.1.0-000</owl:versionInfo>
        <rdfs:comment>This ontology provides a vocabulary and representation of a Windows Task for the  Cyber Observable eXpression (CybOX).  

CybOX  provides a common mechansim (structure and content) to convey the full range of potential cyber observable information and strives to be fully expressive, flexible, extensible, automatable, and as human-readable as possible.

The ontology is based on the CybOX Winodws Task object schema maintained by The MITRE Corporation copyright 2012-2014.  The version number of the ontology is kept in sync with the schema in order to more easily relate between the ontology and the corresponding schema version.

Copyright (c) 2014, DaedaFusion, LLC.  All rights reserved.</rdfs:comment>
        <rdfs:label>Cyber Observable eXpression (CybOX) Windows Task Ontology</rdfs:label>
    </owl:Ontology>
    


    <!-- 
    ///////////////////////////////////////////////////////////////////////////////////////
    //
    // Datatypes
    //
    ///////////////////////////////////////////////////////////////////////////////////////
     -->

    


    <!-- http://www.w3.org/2001/XMLSchema#duration -->

    <rdfs:Datatype rdf:about="http://www.w3.org/2001/XMLSchema#duration"/>
    


    <!-- 
    ///////////////////////////////////////////////////////////////////////////////////////
    //
    // Object Properties
    //
    ///////////////////////////////////////////////////////////////////////////////////////
     -->

    


    <!-- http://cybox.mitre.org/objects/WindowsTask#action -->

    <owl:ObjectProperty rdf:about="http://cybox.mitre.org/objects/WindowsTask#action">
        <rdfs:domain rdf:resource="http://cybox.mitre.org/objects/WindowsTask#TaskAction"/>
        <rdfs:range>
            <owl:Class>
                <owl:unionOf rdf:parseType="Collection">
                    <rdf:Description rdf:about="http://cybox.mitre.org/objects/EmailMessage#EmailMessage"/>
                    <rdf:Description rdf:about="http://cybox.mitre.org/objects/WindowsTask#ICOMHandlerAction"/>
                    <rdf:Description rdf:about="http://cybox.mitre.org/objects/WindowsTask#IExecAction"/>
                    <rdf:Description rdf:about="http://cybox.mitre.org/objects/WindowsTask#IShowMessageAction"/>
                </owl:unionOf>
            </owl:Class>
        </rdfs:range>
        <rdfs:comment>Specifies the action(s) to be taken</rdfs:comment>
        <rdfs:isDefinedBy rdf:resource="http://cybox.mitre.org/objects/WindowsTask"/>
        <rdfs:label>action</rdfs:label>
    </owl:ObjectProperty>
    


    <!-- http://cybox.mitre.org/objects/WindowsTask#actionList -->

    <owl:ObjectProperty rdf:about="http://cybox.mitre.org/objects/WindowsTask#actionList">
        <rdfs:domain rdf:resource="http://cybox.mitre.org/objects/WindowsTask#WindowsTask"/>
        <rdfs:range rdf:resource="http://cybox.mitre.org/objects/WindowsTask#TaskAction"/>
        <rdfs:comment>Specifies a list of actions to be performed by the scheduled task.</rdfs:comment>
        <rdfs:isDefinedBy rdf:resource="http://cybox.mitre.org/objects/WindowsTask"/>
        <rdfs:label>Action List</rdfs:label>
    </owl:ObjectProperty>
    


    <!-- http://cybox.mitre.org/objects/WindowsTask#execProgramHash.details -->

    <owl:ObjectProperty rdf:about="http://cybox.mitre.org/objects/WindowsTask#execProgramHash.details">
        <rdfs:domain rdf:resource="http://cybox.mitre.org/objects/WindowsTask#IExecAction"/>
        <rdfs:range rdf:resource="http://cybox.mitre.org/cyboxCommon#Hash"/>
        <rdfs:comment>Specifies details about any hashes of the executable file launched by the action.</rdfs:comment>
        <rdfs:isDefinedBy rdf:resource="http://cybox.mitre.org/objects/WindowsTask"/>
        <rdfs:label>Exec Program Hash - Details</rdfs:label>
    </owl:ObjectProperty>
    


    <!-- http://cybox.mitre.org/objects/WindowsTask#triggerList -->

    <owl:ObjectProperty rdf:about="http://cybox.mitre.org/objects/WindowsTask#triggerList">
        <rdfs:domain rdf:resource="http://cybox.mitre.org/objects/WindowsTask#WindowsTask"/>
        <rdfs:range rdf:resource="http://cybox.mitre.org/objects/WindowsTask#Trigger"/>
        <rdfs:comment>Specifies a set of triggers used by the scheduled task. 

See also: http://msdn.microsoft.com/en-us/library/windows/desktop/aa383264(v=vs.85).aspx.</rdfs:comment>
        <rdfs:isDefinedBy rdf:resource="http://cybox.mitre.org/objects/WindowsTask"/>
        <rdfs:label>Trigger List</rdfs:label>
    </owl:ObjectProperty>
    


    <!-- 
    ///////////////////////////////////////////////////////////////////////////////////////
    //
    // Data properties
    //
    ///////////////////////////////////////////////////////////////////////////////////////
     -->

    


    <!-- http://cybox.mitre.org/objects/WindowsTask#accountLogonType -->

    <owl:DatatypeProperty rdf:about="http://cybox.mitre.org/objects/WindowsTask#accountLogonType">
        <rdfs:domain rdf:resource="http://cybox.mitre.org/objects/WindowsTask#WindowsTask"/>
        <rdfs:range rdf:resource="http://www.w3.org/2001/XMLSchema#string"/>
        <rdfs:comment>Specifies the security logon method required to run the tasks associated with the account. 

See also: http://msdn.microsoft.com/en-us/library/windows/desktop/aa383013(v=vs.85).aspx.</rdfs:comment>
        <rdfs:isDefinedBy rdf:resource="http://cybox.mitre.org/objects/WindowsTask"/>
        <rdfs:label>Account Logon Type</rdfs:label>
    </owl:DatatypeProperty>
    


    <!-- http://cybox.mitre.org/objects/WindowsTask#accountName -->

    <owl:DatatypeProperty rdf:about="http://cybox.mitre.org/objects/WindowsTask#accountName">
        <rdfs:domain rdf:resource="http://cybox.mitre.org/objects/WindowsTask#WindowsTask"/>
        <rdfs:range rdf:resource="http://www.w3.org/2001/XMLSchema#string"/>
        <rdfs:comment>Specifies the name of the account used to run the scheduled task. 

See also: http://msdn.microsoft.com/en-us/library/windows/desktop/aa381228(v=vs.85).aspx.</rdfs:comment>
        <rdfs:isDefinedBy rdf:resource="http://cybox.mitre.org/objects/WindowsTask"/>
        <rdfs:label>Account Name</rdfs:label>
    </owl:DatatypeProperty>
    


    <!-- http://cybox.mitre.org/objects/WindowsTask#accountRunLevel -->

    <owl:DatatypeProperty rdf:about="http://cybox.mitre.org/objects/WindowsTask#accountRunLevel">
        <rdfs:domain rdf:resource="http://cybox.mitre.org/objects/WindowsTask#WindowsTask"/>
        <rdfs:range rdf:resource="http://www.w3.org/2001/XMLSchema#string"/>
        <rdfs:comment>Specifies the permission level of the account that the task will be run at.</rdfs:comment>
        <rdfs:isDefinedBy rdf:resource="http://cybox.mitre.org/objects/WindowsTask"/>
        <rdfs:label>Account Run Level</rdfs:label>
    </owl:DatatypeProperty>
    


    <!-- http://cybox.mitre.org/objects/WindowsTask#actionID -->

    <owl:DatatypeProperty rdf:about="http://cybox.mitre.org/objects/WindowsTask#actionID">
        <rdfs:domain rdf:resource="http://cybox.mitre.org/objects/WindowsTask#TaskAction"/>
        <rdfs:range rdf:resource="http://www.w3.org/2001/XMLSchema#string"/>
        <rdfs:comment>Specifies the user-defined identifier for the action. This identifier is used by the Task Scheduler for logging purposes. 

See also: http://msdn.microsoft.com/en-us/library/windows/desktop/aa380590(v=vs.85).aspx.</rdfs:comment>
        <rdfs:isDefinedBy rdf:resource="http://cybox.mitre.org/objects/WindowsTask"/>
        <rdfs:label>Action ID</rdfs:label>
    </owl:DatatypeProperty>
    


    <!-- http://cybox.mitre.org/objects/WindowsTask#actionType -->

    <owl:DatatypeProperty rdf:about="http://cybox.mitre.org/objects/WindowsTask#actionType">
        <rdfs:domain rdf:resource="http://cybox.mitre.org/objects/WindowsTask#TaskAction"/>
        <rdfs:range rdf:resource="http://www.w3.org/2001/XMLSchema#string"/>
        <rdfs:comment>Specifies the type of the action. 

See also: http://msdn.microsoft.com/en-us/library/windows/desktop/aa380596(v=vs.85).aspx.</rdfs:comment>
        <rdfs:isDefinedBy rdf:resource="http://cybox.mitre.org/objects/WindowsTask"/>
        <rdfs:label>Action Type</rdfs:label>
    </owl:DatatypeProperty>
    


    <!-- http://cybox.mitre.org/objects/WindowsTask#applicationName -->

    <owl:DatatypeProperty rdf:about="http://cybox.mitre.org/objects/WindowsTask#applicationName">
        <rdfs:domain rdf:resource="http://cybox.mitre.org/objects/WindowsTask#WindowsTask"/>
        <rdfs:range rdf:resource="http://www.w3.org/2001/XMLSchema#string"/>
        <rdfs:comment>Specifies the application name associated with the task.</rdfs:comment>
        <rdfs:isDefinedBy rdf:resource="http://cybox.mitre.org/objects/WindowsTask"/>
        <rdfs:label>Application Name</rdfs:label>
    </owl:DatatypeProperty>
    


    <!-- http://cybox.mitre.org/objects/WindowsTask#body -->

    <owl:DatatypeProperty rdf:about="http://cybox.mitre.org/objects/WindowsTask#body">
        <rdfs:domain rdf:resource="http://cybox.mitre.org/objects/WindowsTask#IShowMessageAction"/>
        <rdfs:range rdf:resource="http://www.w3.org/2001/XMLSchema#string"/>
        <rdfs:comment>Specifies the message text that is displayed in the body of the message box by the action. 

See also: http://msdn.microsoft.com/en-us/library/windows/desktop/aa381302(v=vs.85).aspx.</rdfs:comment>
        <rdfs:isDefinedBy rdf:resource="http://cybox.mitre.org/objects/WindowsTask"/>
        <rdfs:label>Body</rdfs:label>
    </owl:DatatypeProperty>
    


    <!-- http://cybox.mitre.org/objects/WindowsTask#comClassID -->

    <owl:DatatypeProperty rdf:about="http://cybox.mitre.org/objects/WindowsTask#comClassID">
        <rdfs:domain rdf:resource="http://cybox.mitre.org/objects/WindowsTask#ICOMHandlerAction"/>
        <rdfs:range rdf:resource="http://www.w3.org/2001/XMLSchema#string"/>
        <rdfs:comment>Specifies the ID of the COM action. 

See also: http://msdn.microsoft.com/en-us/library/windows/desktop/aa380613(v=vs.85).aspx.</rdfs:comment>
        <rdfs:isDefinedBy rdf:resource="http://cybox.mitre.org/objects/WindowsTask"/>
        <rdfs:label>COM Class ID</rdfs:label>
    </owl:DatatypeProperty>
    


    <!-- http://cybox.mitre.org/objects/WindowsTask#comData -->

    <owl:DatatypeProperty rdf:about="http://cybox.mitre.org/objects/WindowsTask#comData">
        <rdfs:domain rdf:resource="http://cybox.mitre.org/objects/WindowsTask#ICOMHandlerAction"/>
        <rdfs:range rdf:resource="http://www.w3.org/2001/XMLSchema#string"/>
        <rdfs:comment>Specifies the data associated with the COM handler. 

See also: http://msdn.microsoft.com/en-us/library/windows/desktop/aa380613(v=vs.85).aspx..</rdfs:comment>
        <rdfs:isDefinedBy rdf:resource="http://cybox.mitre.org/objects/WindowsTask"/>
        <rdfs:label>COM Data</rdfs:label>
    </owl:DatatypeProperty>
    


    <!-- http://cybox.mitre.org/objects/WindowsTask#commandLineParameters -->

    <owl:DatatypeProperty rdf:about="http://cybox.mitre.org/objects/WindowsTask#commandLineParameters">
        <rdfs:domain rdf:resource="http://cybox.mitre.org/objects/WindowsTask#WindowsTask"/>
        <rdfs:range rdf:resource="http://www.w3.org/2001/XMLSchema#string"/>
        <rdfs:comment>Specifies the command line parameters used to launch the scheduled task. 

See also: http://msdn.microsoft.com/en-us/library/windows/desktop/aa381875(v=vs.85).aspx.</rdfs:comment>
        <rdfs:isDefinedBy rdf:resource="http://cybox.mitre.org/objects/WindowsTask"/>
        <rdfs:label>Command Line Parameters</rdfs:label>
    </owl:DatatypeProperty>
    


    <!-- http://cybox.mitre.org/objects/WindowsTask#comment -->

    <owl:DatatypeProperty rdf:about="http://cybox.mitre.org/objects/WindowsTask#comment">
        <rdfs:domain rdf:resource="http://cybox.mitre.org/objects/WindowsTask#WindowsTask"/>
        <rdfs:range rdf:resource="http://www.w3.org/2001/XMLSchema#string"/>
        <rdfs:comment>Specifies a comment for the scheduled task. 

See also: http://msdn.microsoft.com/en-us/library/windows/desktop/aa381232(v=vs.85).aspx.</rdfs:comment>
        <rdfs:isDefinedBy rdf:resource="http://cybox.mitre.org/objects/WindowsTask"/>
        <rdfs:label>Comment</rdfs:label>
    </owl:DatatypeProperty>
    


    <!-- http://cybox.mitre.org/objects/WindowsTask#creationDateTime -->

    <owl:DatatypeProperty rdf:about="http://cybox.mitre.org/objects/WindowsTask#creationDateTime">
        <rdfs:domain rdf:resource="http://cybox.mitre.org/objects/WindowsTask#WindowsTask"/>
        <rdfs:range rdf:resource="http://www.w3.org/2001/XMLSchema#dateTime"/>
        <rdfs:comment>Specifies the date and time that the task was registered. 

See also: http://msdn.microsoft.com/en-us/library/windows/desktop/aa382623(v=vs.85).aspx.</rdfs:comment>
        <rdfs:isDefinedBy rdf:resource="http://cybox.mitre.org/objects/WindowsTask"/>
        <rdfs:label>Creation Date</rdfs:label>
    </owl:DatatypeProperty>
    


    <!-- http://cybox.mitre.org/objects/WindowsTask#creator -->

    <owl:DatatypeProperty rdf:about="http://cybox.mitre.org/objects/WindowsTask#creator">
        <rdfs:domain rdf:resource="http://cybox.mitre.org/objects/WindowsTask#WindowsTask"/>
        <rdfs:range rdf:resource="http://www.w3.org/2001/XMLSchema#string"/>
        <rdfs:comment>Specifies the name of the creator of the scheduled task. 

See also: http://msdn.microsoft.com/en-us/library/windows/desktop/aa381235(v=vs.85).aspx.</rdfs:comment>
        <rdfs:isDefinedBy rdf:resource="http://cybox.mitre.org/objects/WindowsTask"/>
        <rdfs:label>Creator</rdfs:label>
    </owl:DatatypeProperty>
    


    <!-- http://cybox.mitre.org/objects/WindowsTask#execArguments -->

    <owl:DatatypeProperty rdf:about="http://cybox.mitre.org/objects/WindowsTask#execArguments">
        <rdfs:domain rdf:resource="http://cybox.mitre.org/objects/WindowsTask#IExecAction"/>
        <rdfs:range rdf:resource="http://www.w3.org/2001/XMLSchema#string"/>
        <rdfs:comment>pecifies the arguments associated with the command-line operation launched by the action. 

See also: http://msdn.microsoft.com/en-us/library/windows/desktop/aa380715(v=vs.85).aspx..</rdfs:comment>
        <rdfs:isDefinedBy rdf:resource="http://cybox.mitre.org/objects/WindowsTask"/>
        <rdfs:label>Executable Arguments</rdfs:label>
    </owl:DatatypeProperty>
    


    <!-- http://cybox.mitre.org/objects/WindowsTask#execProgramHash.value -->

    <owl:DatatypeProperty rdf:about="http://cybox.mitre.org/objects/WindowsTask#execProgramHash.value">
        <rdfs:domain rdf:resource="http://cybox.mitre.org/objects/WindowsTask#IExecAction"/>
        <rdfs:range rdf:resource="http://www.w3.org/2001/XMLSchema#string"/>
        <rdfs:comment>Specifies the values, in the format of &apos;hash-type&apos;:&apos;hash-value&apos;, for any hash computed for the executable file launched by the action.</rdfs:comment>
        <rdfs:isDefinedBy rdf:resource="http://cybox.mitre.org/objects/WindowsTask"/>
        <rdfs:label>Exec Program Hash - Value</rdfs:label>
    </owl:DatatypeProperty>
    


    <!-- http://cybox.mitre.org/objects/WindowsTask#execProgramPath -->

    <owl:DatatypeProperty rdf:about="http://cybox.mitre.org/objects/WindowsTask#execProgramPath">
        <rdfs:domain rdf:resource="http://cybox.mitre.org/objects/WindowsTask#IExecAction"/>
        <rdfs:range rdf:resource="http://www.w3.org/2001/XMLSchema#string"/>
        <rdfs:comment>Specifies the path to the executable file launched by the action. 

See also: http://msdn.microsoft.com/en-us/library/windows/desktop/aa380715(v=vs.85).aspx.</rdfs:comment>
        <rdfs:isDefinedBy rdf:resource="http://cybox.mitre.org/objects/WindowsTask"/>
        <rdfs:label>Executable Program Path</rdfs:label>
    </owl:DatatypeProperty>
    


    <!-- http://cybox.mitre.org/objects/WindowsTask#execWorkingDirectory -->

    <owl:DatatypeProperty rdf:about="http://cybox.mitre.org/objects/WindowsTask#execWorkingDirectory">
        <rdfs:domain rdf:resource="http://cybox.mitre.org/objects/WindowsTask#IExecAction"/>
        <rdfs:range rdf:resource="http://www.w3.org/2001/XMLSchema#string"/>
        <rdfs:comment>Specifies the directory that contains either the executable file or the files that are used by the executable file launched by the action. 

See also: http://msdn.microsoft.com/en-us/library/windows/desktop/aa380715(v=vs.85).aspx.</rdfs:comment>
        <rdfs:isDefinedBy rdf:resource="http://cybox.mitre.org/objects/WindowsTask"/>
        <rdfs:label>Executable Working Directory</rdfs:label>
    </owl:DatatypeProperty>
    


    <!-- http://cybox.mitre.org/objects/WindowsTask#exitCode -->

    <owl:DatatypeProperty rdf:about="http://cybox.mitre.org/objects/WindowsTask#exitCode">
        <rdfs:domain rdf:resource="http://cybox.mitre.org/objects/WindowsTask#WindowsTask"/>
        <rdfs:range rdf:resource="http://www.w3.org/2001/XMLSchema#long"/>
        <rdfs:comment>Specifies the last exit code of the scheduled task. 

See also: http://msdn.microsoft.com/en-us/library/windows/desktop/aa381245(v=vs.85).aspx.</rdfs:comment>
        <rdfs:isDefinedBy rdf:resource="http://cybox.mitre.org/objects/WindowsTask"/>
        <rdfs:label>Exit Code</rdfs:label>
    </owl:DatatypeProperty>
    


    <!-- http://cybox.mitre.org/objects/WindowsTask#maxRunTime -->

    <owl:DatatypeProperty rdf:about="http://cybox.mitre.org/objects/WindowsTask#maxRunTime">
        <rdfs:domain rdf:resource="http://cybox.mitre.org/objects/WindowsTask#WindowsTask"/>
        <rdfs:range rdf:resource="http://www.w3.org/2001/XMLSchema#unsignedLong"/>
        <rdfs:comment>Specifies the maximum run time of the scheduled task before terminating, in milliseconds. 

See also: http://msdn.microsoft.com/en-us/library/windows/desktop/aa381874(v=vs.85).aspx.</rdfs:comment>
        <rdfs:isDefinedBy rdf:resource="http://cybox.mitre.org/objects/WindowsTask"/>
        <rdfs:label>Max Run Time</rdfs:label>
    </owl:DatatypeProperty>
    


    <!-- http://cybox.mitre.org/objects/WindowsTask#mostRecentRunDateTime -->

    <owl:DatatypeProperty rdf:about="http://cybox.mitre.org/objects/WindowsTask#mostRecentRunDateTime">
        <rdfs:domain rdf:resource="http://cybox.mitre.org/objects/WindowsTask#WindowsTask"/>
        <rdfs:range rdf:resource="http://www.w3.org/2001/XMLSchema#dateTime"/>
        <rdfs:comment>Specifies the most recent run date/time of this scheduled task. 

See also: http://msdn.microsoft.com/en-us/library/windows/desktop/aa381254(v=vs.85).aspx.</rdfs:comment>
        <rdfs:isDefinedBy rdf:resource="http://cybox.mitre.org/objects/WindowsTask"/>
        <rdfs:label>Most Recent Run Time</rdfs:label>
    </owl:DatatypeProperty>
    


    <!-- http://cybox.mitre.org/objects/WindowsTask#nextRunDateTime -->

    <owl:DatatypeProperty rdf:about="http://cybox.mitre.org/objects/WindowsTask#nextRunDateTime">
        <rdfs:domain rdf:resource="http://cybox.mitre.org/objects/WindowsTask#WindowsTask"/>
        <rdfs:range rdf:resource="http://www.w3.org/2001/XMLSchema#dateTime"/>
        <rdfs:comment>Specifies the next run date/time of the scheduled task. 

See also: http://msdn.microsoft.com/en-us/library/windows/desktop/aa381257(v=vs.85).aspx.</rdfs:comment>
        <rdfs:isDefinedBy rdf:resource="http://cybox.mitre.org/objects/WindowsTask"/>
        <rdfs:label>Next Run Time</rdfs:label>
    </owl:DatatypeProperty>
    


    <!-- http://cybox.mitre.org/objects/WindowsTask#taskFlags -->

    <owl:DatatypeProperty rdf:about="http://cybox.mitre.org/objects/WindowsTask#taskFlags">
        <rdfs:domain rdf:resource="http://cybox.mitre.org/objects/WindowsTask#WindowsTask"/>
        <rdfs:range rdf:resource="http://www.w3.org/2001/XMLSchema#string"/>
        <rdfs:comment>Specifies any flags that modify the behavior of the scheduled task. 

See also: http://msdn.microsoft.com/en-us/library/windows/desktop/aa381248(v=vs.85).aspx.</rdfs:comment>
        <rdfs:isDefinedBy rdf:resource="http://cybox.mitre.org/objects/WindowsTask"/>
        <rdfs:label>Task Flags</rdfs:label>
    </owl:DatatypeProperty>
    


    <!-- http://cybox.mitre.org/objects/WindowsTask#taskName -->

    <owl:DatatypeProperty rdf:about="http://cybox.mitre.org/objects/WindowsTask#taskName">
        <rdfs:domain rdf:resource="http://cybox.mitre.org/objects/WindowsTask#WindowsTask"/>
        <rdfs:range rdf:resource="http://www.w3.org/2001/XMLSchema#string"/>
        <rdfs:comment>Specifies the name for the task.</rdfs:comment>
        <rdfs:isDefinedBy rdf:resource="http://cybox.mitre.org/objects/WindowsTask"/>
        <rdfs:label>Image Name</rdfs:label>
    </owl:DatatypeProperty>
    


    <!-- http://cybox.mitre.org/objects/WindowsTask#taskPriority -->

    <owl:DatatypeProperty rdf:about="http://cybox.mitre.org/objects/WindowsTask#taskPriority">
        <rdfs:domain rdf:resource="http://cybox.mitre.org/objects/WindowsTask#WindowsTask"/>
        <rdfs:range rdf:resource="http://www.w3.org/2001/XMLSchema#string"/>
        <rdfs:comment>Specifies the priority of the scheduled task. This can either be a free-form string or one the values in the TaskPriorityEnum enumeration. 

See also: http://msdn.microsoft.com/en-us/library/windows/desktop/aa381876(v=vs.85).aspx.</rdfs:comment>
        <rdfs:isDefinedBy rdf:resource="http://cybox.mitre.org/objects/WindowsTask"/>
        <rdfs:label>Task Priority</rdfs:label>
    </owl:DatatypeProperty>
    


    <!-- http://cybox.mitre.org/objects/WindowsTask#taskStatus -->

    <owl:DatatypeProperty rdf:about="http://cybox.mitre.org/objects/WindowsTask#taskStatus">
        <rdfs:domain rdf:resource="http://cybox.mitre.org/objects/WindowsTask#WindowsTask"/>
        <rdfs:range rdf:resource="http://www.w3.org/2001/XMLSchema#string"/>
        <rdfs:comment>Specifies the current status of the scheduled task. 

See also: http://msdn.microsoft.com/en-us/library/windows/desktop/aa381263(v=vs.85).aspx.</rdfs:comment>
        <rdfs:isDefinedBy rdf:resource="http://cybox.mitre.org/objects/WindowsTask"/>
        <rdfs:label>Task Status</rdfs:label>
    </owl:DatatypeProperty>
    


    <!-- http://cybox.mitre.org/objects/WindowsTask#title -->

    <owl:DatatypeProperty rdf:about="http://cybox.mitre.org/objects/WindowsTask#title">
        <rdfs:domain rdf:resource="http://cybox.mitre.org/objects/WindowsTask#IShowMessageAction"/>
        <rdfs:range rdf:resource="http://www.w3.org/2001/XMLSchema#string"/>
        <rdfs:comment>Specifies the title of the message box shown by the action. 

See also: http://msdn.microsoft.com/en-us/library/windows/desktop/aa381302(v=vs.85).aspx.</rdfs:comment>
        <rdfs:isDefinedBy rdf:resource="http://cybox.mitre.org/objects/WindowsTask"/>
        <rdfs:label>Title</rdfs:label>
    </owl:DatatypeProperty>
    


    <!-- http://cybox.mitre.org/objects/WindowsTask#triggerBeginDateTime -->

    <owl:DatatypeProperty rdf:about="http://cybox.mitre.org/objects/WindowsTask#triggerBeginDateTime">
        <rdfs:domain rdf:resource="http://cybox.mitre.org/objects/WindowsTask#Trigger"/>
        <rdfs:range rdf:resource="http://www.w3.org/2001/XMLSchema#dateTime"/>
        <rdfs:comment>Specifies the date/time that the trigger is activated.</rdfs:comment>
        <rdfs:isDefinedBy rdf:resource="http://cybox.mitre.org/objects/WindowsTask"/>
        <rdfs:label>Trigger Begin</rdfs:label>
    </owl:DatatypeProperty>
    


    <!-- http://cybox.mitre.org/objects/WindowsTask#triggerDelay -->

    <owl:DatatypeProperty rdf:about="http://cybox.mitre.org/objects/WindowsTask#triggerDelay">
        <rdfs:domain rdf:resource="http://cybox.mitre.org/objects/WindowsTask#Trigger"/>
        <rdfs:range rdf:resource="http://www.w3.org/2001/XMLSchema#duration"/>
        <rdfs:comment>Specifies the delay that takes place between when the task is registered and when the task is started.</rdfs:comment>
        <rdfs:isDefinedBy rdf:resource="http://cybox.mitre.org/objects/WindowsTask"/>
        <rdfs:label>Trigger Delay</rdfs:label>
    </owl:DatatypeProperty>
    


    <!-- http://cybox.mitre.org/objects/WindowsTask#triggerEnabled -->

    <owl:DatatypeProperty rdf:about="http://cybox.mitre.org/objects/WindowsTask#triggerEnabled">
        <rdfs:domain rdf:resource="http://cybox.mitre.org/objects/WindowsTask#Trigger"/>
        <rdfs:range rdf:resource="http://www.w3.org/2001/XMLSchema#boolean"/>
        <rdfs:comment>Specifies whether the trigger is enabled.</rdfs:comment>
        <rdfs:isDefinedBy rdf:resource="http://cybox.mitre.org/objects/WindowsTask"/>
        <rdfs:label>Enabled</rdfs:label>
    </owl:DatatypeProperty>
    


    <!-- http://cybox.mitre.org/objects/WindowsTask#triggerEndDateTime -->

    <owl:DatatypeProperty rdf:about="http://cybox.mitre.org/objects/WindowsTask#triggerEndDateTime">
        <rdfs:domain rdf:resource="http://cybox.mitre.org/objects/WindowsTask#Trigger"/>
        <rdfs:range rdf:resource="http://www.w3.org/2001/XMLSchema#dateTime"/>
        <rdfs:comment>Specifies the date/time that the trigger is deactivated.</rdfs:comment>
        <rdfs:isDefinedBy rdf:resource="http://cybox.mitre.org/objects/WindowsTask"/>
        <rdfs:label>Trigger End</rdfs:label>
    </owl:DatatypeProperty>
    


    <!-- http://cybox.mitre.org/objects/WindowsTask#triggerFrequency -->

    <owl:DatatypeProperty rdf:about="http://cybox.mitre.org/objects/WindowsTask#triggerFrequency">
        <rdfs:domain rdf:resource="http://cybox.mitre.org/objects/WindowsTask#Trigger"/>
        <rdfs:range rdf:resource="http://www.w3.org/2001/XMLSchema#string"/>
        <rdfs:comment>Specifies the frequency at which the trigger repeats.</rdfs:comment>
        <rdfs:isDefinedBy rdf:resource="http://cybox.mitre.org/objects/WindowsTask"/>
        <rdfs:label>Trigger Frequency</rdfs:label>
    </owl:DatatypeProperty>
    


    <!-- http://cybox.mitre.org/objects/WindowsTask#triggerMaxRunTime -->

    <owl:DatatypeProperty rdf:about="http://cybox.mitre.org/objects/WindowsTask#triggerMaxRunTime">
        <rdfs:domain rdf:resource="http://cybox.mitre.org/objects/WindowsTask#Trigger"/>
        <rdfs:range rdf:resource="http://www.w3.org/2001/XMLSchema#duration"/>
        <rdfs:comment>Specifies the maximum amount of time that the task launched by the trigger is allowed to run. 

See also: http://msdn.microsoft.com/en-us/library/windows/desktop/aa383868(v=vs.85).aspx.</rdfs:comment>
        <rdfs:isDefinedBy rdf:resource="http://cybox.mitre.org/objects/WindowsTask"/>
        <rdfs:label>Trigger Max Run Time</rdfs:label>
    </owl:DatatypeProperty>
    


    <!-- http://cybox.mitre.org/objects/WindowsTask#triggerSessionChangeType -->

    <owl:DatatypeProperty rdf:about="http://cybox.mitre.org/objects/WindowsTask#triggerSessionChangeType">
        <rdfs:domain rdf:resource="http://cybox.mitre.org/objects/WindowsTask#Trigger"/>
        <rdfs:range rdf:resource="http://www.w3.org/2001/XMLSchema#string"/>
        <rdfs:comment>Specifies the type of Terminal Server session change that would trigger a task launch. 

See also: http://msdn.microsoft.com/en-us/library/windows/desktop/aa381298(v=vs.85).aspx.</rdfs:comment>
        <rdfs:isDefinedBy rdf:resource="http://cybox.mitre.org/objects/WindowsTask"/>
        <rdfs:label>Trigger Session Change Type</rdfs:label>
    </owl:DatatypeProperty>
    


    <!-- http://cybox.mitre.org/objects/WindowsTask#triggerType -->

    <owl:DatatypeProperty rdf:about="http://cybox.mitre.org/objects/WindowsTask#triggerType">
        <rdfs:domain rdf:resource="http://cybox.mitre.org/objects/WindowsTask#Trigger"/>
        <rdfs:range rdf:resource="http://www.w3.org/2001/XMLSchema#string"/>
        <rdfs:comment>Specifies the type of the task trigger.</rdfs:comment>
        <rdfs:isDefinedBy rdf:resource="http://cybox.mitre.org/objects/WindowsTask"/>
        <rdfs:label>Trigger Type</rdfs:label>
    </owl:DatatypeProperty>
    


    <!-- http://cybox.mitre.org/objects/WindowsTask#workItemData -->

    <owl:DatatypeProperty rdf:about="http://cybox.mitre.org/objects/WindowsTask#workItemData">
        <rdfs:domain rdf:resource="http://cybox.mitre.org/objects/WindowsTask#WindowsTask"/>
        <rdfs:range rdf:resource="http://www.w3.org/2001/XMLSchema#base64Binary"/>
        <rdfs:comment>Specifies application defined data associated with the scheduled task. 

See also: http://msdn.microsoft.com/en-us/library/windows/desktop/aa381271(v=vs.85).aspx.</rdfs:comment>
        <rdfs:isDefinedBy rdf:resource="http://cybox.mitre.org/objects/WindowsTask"/>
        <rdfs:label>Work Item Data</rdfs:label>
    </owl:DatatypeProperty>
    


    <!-- http://cybox.mitre.org/objects/WindowsTask#workingDirectory -->

    <owl:DatatypeProperty rdf:about="http://cybox.mitre.org/objects/WindowsTask#workingDirectory">
        <rdfs:domain rdf:resource="http://cybox.mitre.org/objects/WindowsTask#WindowsTask"/>
        <rdfs:range rdf:resource="http://www.w3.org/2001/XMLSchema#string"/>
        <rdfs:comment>Specifies the working directory for the scheduled task. 

See also: http://msdn.microsoft.com/en-us/library/windows/desktop/aa381878(v=vs.85).aspx.</rdfs:comment>
        <rdfs:isDefinedBy rdf:resource="http://cybox.mitre.org/objects/WindowsTask"/>
        <rdfs:label>Working Directory</rdfs:label>
    </owl:DatatypeProperty>
    


    <!-- 
    ///////////////////////////////////////////////////////////////////////////////////////
    //
    // Classes
    //
    ///////////////////////////////////////////////////////////////////////////////////////
     -->

    


    <!-- http://cybox.mitre.org/cyboxCommon#Hash -->

    <owl:Class rdf:about="http://cybox.mitre.org/cyboxCommon#Hash"/>
    


    <!-- http://cybox.mitre.org/objects/EmailMessage#EmailMessage -->

    <owl:Class rdf:about="http://cybox.mitre.org/objects/EmailMessage#EmailMessage"/>
    


    <!-- http://cybox.mitre.org/objects/WindowsTask#ICOMHandlerAction -->

    <owl:Class rdf:about="http://cybox.mitre.org/objects/WindowsTask#ICOMHandlerAction">
        <rdfs:subClassOf>
            <owl:Restriction>
                <owl:onProperty rdf:resource="http://cybox.mitre.org/objects/WindowsTask#comClassID"/>
                <owl:cardinality rdf:datatype="http://www.w3.org/2001/XMLSchema#nonNegativeInteger">1</owl:cardinality>
            </owl:Restriction>
        </rdfs:subClassOf>
        <rdfs:subClassOf>
            <owl:Restriction>
                <owl:onProperty rdf:resource="http://cybox.mitre.org/objects/WindowsTask#comData"/>
                <owl:maxCardinality rdf:datatype="http://www.w3.org/2001/XMLSchema#nonNegativeInteger">1</owl:maxCardinality>
            </owl:Restriction>
        </rdfs:subClassOf>
        <rdfs:comment>Characterizes IComHandler actions.</rdfs:comment>
        <rdfs:isDefinedBy rdf:resource="http://cybox.mitre.org/objects/WindowsTask"/>
        <rdfs:label>ICOMHandler Action</rdfs:label>
    </owl:Class>
    


    <!-- http://cybox.mitre.org/objects/WindowsTask#IExecAction -->

    <owl:Class rdf:about="http://cybox.mitre.org/objects/WindowsTask#IExecAction">
        <rdfs:subClassOf>
            <owl:Restriction>
                <owl:onProperty rdf:resource="http://cybox.mitre.org/objects/WindowsTask#execProgramPath"/>
                <owl:cardinality rdf:datatype="http://www.w3.org/2001/XMLSchema#nonNegativeInteger">1</owl:cardinality>
            </owl:Restriction>
        </rdfs:subClassOf>
        <rdfs:subClassOf>
            <owl:Restriction>
                <owl:onProperty rdf:resource="http://cybox.mitre.org/objects/WindowsTask#execArguments"/>
                <owl:maxCardinality rdf:datatype="http://www.w3.org/2001/XMLSchema#nonNegativeInteger">1</owl:maxCardinality>
            </owl:Restriction>
        </rdfs:subClassOf>
        <rdfs:subClassOf>
            <owl:Restriction>
                <owl:onProperty rdf:resource="http://cybox.mitre.org/objects/WindowsTask#execWorkingDirectory"/>
                <owl:maxCardinality rdf:datatype="http://www.w3.org/2001/XMLSchema#nonNegativeInteger">1</owl:maxCardinality>
            </owl:Restriction>
        </rdfs:subClassOf>
        <rdfs:comment>Characterizes IExec actions.</rdfs:comment>
        <rdfs:isDefinedBy rdf:resource="http://cybox.mitre.org/objects/WindowsTask"/>
        <rdfs:label>IExec action</rdfs:label>
    </owl:Class>
    


    <!-- http://cybox.mitre.org/objects/WindowsTask#IShowMessageAction -->

    <owl:Class rdf:about="http://cybox.mitre.org/objects/WindowsTask#IShowMessageAction">
        <rdfs:subClassOf>
            <owl:Restriction>
                <owl:onProperty rdf:resource="http://cybox.mitre.org/objects/WindowsTask#title"/>
                <owl:cardinality rdf:datatype="http://www.w3.org/2001/XMLSchema#nonNegativeInteger">1</owl:cardinality>
            </owl:Restriction>
        </rdfs:subClassOf>
        <rdfs:subClassOf>
            <owl:Restriction>
                <owl:onProperty rdf:resource="http://cybox.mitre.org/objects/WindowsTask#body"/>
                <owl:maxCardinality rdf:datatype="http://www.w3.org/2001/XMLSchema#nonNegativeInteger">1</owl:maxCardinality>
            </owl:Restriction>
        </rdfs:subClassOf>
        <rdfs:comment>Characterizes IShowMessage actions.</rdfs:comment>
        <rdfs:isDefinedBy rdf:resource="http://cybox.mitre.org/objects/WindowsTask"/>
        <rdfs:label>IShowMessage Action</rdfs:label>
    </owl:Class>
    


    <!-- http://cybox.mitre.org/objects/WindowsTask#TaskAction -->

    <owl:Class rdf:about="http://cybox.mitre.org/objects/WindowsTask#TaskAction">
        <rdfs:subClassOf>
            <owl:Restriction>
                <owl:onProperty rdf:resource="http://cybox.mitre.org/objects/WindowsTask#action"/>
                <owl:maxCardinality rdf:datatype="http://www.w3.org/2001/XMLSchema#nonNegativeInteger">32</owl:maxCardinality>
            </owl:Restriction>
        </rdfs:subClassOf>
        <rdfs:subClassOf>
            <owl:Restriction>
                <owl:onProperty rdf:resource="http://cybox.mitre.org/objects/WindowsTask#actionID"/>
                <owl:cardinality rdf:datatype="http://www.w3.org/2001/XMLSchema#nonNegativeInteger">1</owl:cardinality>
            </owl:Restriction>
        </rdfs:subClassOf>
        <rdfs:subClassOf>
            <owl:Restriction>
                <owl:onProperty rdf:resource="http://cybox.mitre.org/objects/WindowsTask#actionType"/>
                <owl:cardinality rdf:datatype="http://www.w3.org/2001/XMLSchema#nonNegativeInteger">1</owl:cardinality>
            </owl:Restriction>
        </rdfs:subClassOf>
        <rdfs:comment>Characterizes scheduled task actions.</rdfs:comment>
        <rdfs:isDefinedBy rdf:resource="http://cybox.mitre.org/objects/WindowsTask"/>
        <rdfs:label>Task Action</rdfs:label>
    </owl:Class>
    


    <!-- http://cybox.mitre.org/objects/WindowsTask#Trigger -->

    <owl:Class rdf:about="http://cybox.mitre.org/objects/WindowsTask#Trigger">
        <rdfs:subClassOf>
            <owl:Restriction>
                <owl:onProperty rdf:resource="http://cybox.mitre.org/objects/WindowsTask#triggerBeginDateTime"/>
                <owl:cardinality rdf:datatype="http://www.w3.org/2001/XMLSchema#nonNegativeInteger">1</owl:cardinality>
            </owl:Restriction>
        </rdfs:subClassOf>
        <rdfs:subClassOf>
            <owl:Restriction>
                <owl:onProperty rdf:resource="http://cybox.mitre.org/objects/WindowsTask#triggerFrequency"/>
                <owl:cardinality rdf:datatype="http://www.w3.org/2001/XMLSchema#nonNegativeInteger">1</owl:cardinality>
            </owl:Restriction>
        </rdfs:subClassOf>
        <rdfs:subClassOf>
            <owl:Restriction>
                <owl:onProperty rdf:resource="http://cybox.mitre.org/objects/WindowsTask#triggerType"/>
                <owl:cardinality rdf:datatype="http://www.w3.org/2001/XMLSchema#nonNegativeInteger">1</owl:cardinality>
            </owl:Restriction>
        </rdfs:subClassOf>
        <rdfs:subClassOf>
            <owl:Restriction>
                <owl:onProperty rdf:resource="http://cybox.mitre.org/objects/WindowsTask#triggerDelay"/>
                <owl:maxCardinality rdf:datatype="http://www.w3.org/2001/XMLSchema#nonNegativeInteger">1</owl:maxCardinality>
            </owl:Restriction>
        </rdfs:subClassOf>
        <rdfs:subClassOf>
            <owl:Restriction>
                <owl:onProperty rdf:resource="http://cybox.mitre.org/objects/WindowsTask#triggerEnabled"/>
                <owl:maxCardinality rdf:datatype="http://www.w3.org/2001/XMLSchema#nonNegativeInteger">1</owl:maxCardinality>
            </owl:Restriction>
        </rdfs:subClassOf>
        <rdfs:subClassOf>
            <owl:Restriction>
                <owl:onProperty rdf:resource="http://cybox.mitre.org/objects/WindowsTask#triggerEndDateTime"/>
                <owl:maxCardinality rdf:datatype="http://www.w3.org/2001/XMLSchema#nonNegativeInteger">1</owl:maxCardinality>
            </owl:Restriction>
        </rdfs:subClassOf>
        <rdfs:subClassOf>
            <owl:Restriction>
                <owl:onProperty rdf:resource="http://cybox.mitre.org/objects/WindowsTask#triggerMaxRunTime"/>
                <owl:maxCardinality rdf:datatype="http://www.w3.org/2001/XMLSchema#nonNegativeInteger">1</owl:maxCardinality>
            </owl:Restriction>
        </rdfs:subClassOf>
        <rdfs:subClassOf>
            <owl:Restriction>
                <owl:onProperty rdf:resource="http://cybox.mitre.org/objects/WindowsTask#triggerSessionChangeType"/>
                <owl:maxCardinality rdf:datatype="http://www.w3.org/2001/XMLSchema#nonNegativeInteger">1</owl:maxCardinality>
            </owl:Restriction>
        </rdfs:subClassOf>
        <rdfs:comment>Characterizes task triggers.

See also: http://msdn.microsoft.com/en-us/library/windows/desktop/aa383868(v=vs.85).aspx.</rdfs:comment>
        <rdfs:isDefinedBy rdf:resource="http://cybox.mitre.org/objects/WindowsTask"/>
        <rdfs:label>Trigger</rdfs:label>
    </owl:Class>
    


    <!-- http://cybox.mitre.org/objects/WindowsTask#WindowsTask -->

    <owl:Class rdf:about="http://cybox.mitre.org/objects/WindowsTask#WindowsTask">
        <rdfs:subClassOf>
            <owl:Restriction>
                <owl:onProperty rdf:resource="http://cybox.mitre.org/objects/WindowsTask#taskName"/>
                <owl:cardinality rdf:datatype="http://www.w3.org/2001/XMLSchema#nonNegativeInteger">1</owl:cardinality>
            </owl:Restriction>
        </rdfs:subClassOf>
        <rdfs:subClassOf>
            <owl:Restriction>
                <owl:onProperty rdf:resource="http://cybox.mitre.org/objects/WindowsTask#accountLogonType"/>
                <owl:maxCardinality rdf:datatype="http://www.w3.org/2001/XMLSchema#nonNegativeInteger">1</owl:maxCardinality>
            </owl:Restriction>
        </rdfs:subClassOf>
        <rdfs:subClassOf>
            <owl:Restriction>
                <owl:onProperty rdf:resource="http://cybox.mitre.org/objects/WindowsTask#accountName"/>
                <owl:maxCardinality rdf:datatype="http://www.w3.org/2001/XMLSchema#nonNegativeInteger">1</owl:maxCardinality>
            </owl:Restriction>
        </rdfs:subClassOf>
        <rdfs:subClassOf>
            <owl:Restriction>
                <owl:onProperty rdf:resource="http://cybox.mitre.org/objects/WindowsTask#accountRunLevel"/>
                <owl:maxCardinality rdf:datatype="http://www.w3.org/2001/XMLSchema#nonNegativeInteger">1</owl:maxCardinality>
            </owl:Restriction>
        </rdfs:subClassOf>
        <rdfs:subClassOf>
            <owl:Restriction>
                <owl:onProperty rdf:resource="http://cybox.mitre.org/objects/WindowsTask#applicationName"/>
                <owl:maxCardinality rdf:datatype="http://www.w3.org/2001/XMLSchema#nonNegativeInteger">1</owl:maxCardinality>
            </owl:Restriction>
        </rdfs:subClassOf>
        <rdfs:subClassOf>
            <owl:Restriction>
                <owl:onProperty rdf:resource="http://cybox.mitre.org/objects/WindowsTask#commandLineParameters"/>
                <owl:maxCardinality rdf:datatype="http://www.w3.org/2001/XMLSchema#nonNegativeInteger">1</owl:maxCardinality>
            </owl:Restriction>
        </rdfs:subClassOf>
        <rdfs:subClassOf>
            <owl:Restriction>
                <owl:onProperty rdf:resource="http://cybox.mitre.org/objects/WindowsTask#comment"/>
                <owl:maxCardinality rdf:datatype="http://www.w3.org/2001/XMLSchema#nonNegativeInteger">1</owl:maxCardinality>
            </owl:Restriction>
        </rdfs:subClassOf>
        <rdfs:subClassOf>
            <owl:Restriction>
                <owl:onProperty rdf:resource="http://cybox.mitre.org/objects/WindowsTask#creationDateTime"/>
                <owl:maxCardinality rdf:datatype="http://www.w3.org/2001/XMLSchema#nonNegativeInteger">1</owl:maxCardinality>
            </owl:Restriction>
        </rdfs:subClassOf>
        <rdfs:subClassOf>
            <owl:Restriction>
                <owl:onProperty rdf:resource="http://cybox.mitre.org/objects/WindowsTask#creator"/>
                <owl:maxCardinality rdf:datatype="http://www.w3.org/2001/XMLSchema#nonNegativeInteger">1</owl:maxCardinality>
            </owl:Restriction>
        </rdfs:subClassOf>
        <rdfs:subClassOf>
            <owl:Restriction>
                <owl:onProperty rdf:resource="http://cybox.mitre.org/objects/WindowsTask#exitCode"/>
                <owl:maxCardinality rdf:datatype="http://www.w3.org/2001/XMLSchema#nonNegativeInteger">1</owl:maxCardinality>
            </owl:Restriction>
        </rdfs:subClassOf>
        <rdfs:subClassOf>
            <owl:Restriction>
                <owl:onProperty rdf:resource="http://cybox.mitre.org/objects/WindowsTask#maxRunTime"/>
                <owl:maxCardinality rdf:datatype="http://www.w3.org/2001/XMLSchema#nonNegativeInteger">1</owl:maxCardinality>
            </owl:Restriction>
        </rdfs:subClassOf>
        <rdfs:subClassOf>
            <owl:Restriction>
                <owl:onProperty rdf:resource="http://cybox.mitre.org/objects/WindowsTask#mostRecentRunDateTime"/>
                <owl:maxCardinality rdf:datatype="http://www.w3.org/2001/XMLSchema#nonNegativeInteger">1</owl:maxCardinality>
            </owl:Restriction>
        </rdfs:subClassOf>
        <rdfs:subClassOf>
            <owl:Restriction>
                <owl:onProperty rdf:resource="http://cybox.mitre.org/objects/WindowsTask#nextRunDateTime"/>
                <owl:maxCardinality rdf:datatype="http://www.w3.org/2001/XMLSchema#nonNegativeInteger">1</owl:maxCardinality>
            </owl:Restriction>
        </rdfs:subClassOf>
        <rdfs:subClassOf>
            <owl:Restriction>
                <owl:onProperty rdf:resource="http://cybox.mitre.org/objects/WindowsTask#taskFlags"/>
                <owl:maxCardinality rdf:datatype="http://www.w3.org/2001/XMLSchema#nonNegativeInteger">1</owl:maxCardinality>
            </owl:Restriction>
        </rdfs:subClassOf>
        <rdfs:subClassOf>
            <owl:Restriction>
                <owl:onProperty rdf:resource="http://cybox.mitre.org/objects/WindowsTask#taskPriority"/>
                <owl:maxCardinality rdf:datatype="http://www.w3.org/2001/XMLSchema#nonNegativeInteger">1</owl:maxCardinality>
            </owl:Restriction>
        </rdfs:subClassOf>
        <rdfs:subClassOf>
            <owl:Restriction>
                <owl:onProperty rdf:resource="http://cybox.mitre.org/objects/WindowsTask#taskStatus"/>
                <owl:maxCardinality rdf:datatype="http://www.w3.org/2001/XMLSchema#nonNegativeInteger">1</owl:maxCardinality>
            </owl:Restriction>
        </rdfs:subClassOf>
        <rdfs:subClassOf>
            <owl:Restriction>
                <owl:onProperty rdf:resource="http://cybox.mitre.org/objects/WindowsTask#workItemData"/>
                <owl:maxCardinality rdf:datatype="http://www.w3.org/2001/XMLSchema#nonNegativeInteger">1</owl:maxCardinality>
            </owl:Restriction>
        </rdfs:subClassOf>
        <rdfs:subClassOf>
            <owl:Restriction>
                <owl:onProperty rdf:resource="http://cybox.mitre.org/objects/WindowsTask#workingDirectory"/>
                <owl:maxCardinality rdf:datatype="http://www.w3.org/2001/XMLSchema#nonNegativeInteger">1</owl:maxCardinality>
            </owl:Restriction>
        </rdfs:subClassOf>
        <rdfs:comment>Characterize Windows task scheduler tasks. 

See Also: http://msdn.microsoft.com/en-us/library/windows/desktop/aa381311(v=vs.85).aspx.</rdfs:comment>
        <rdfs:isDefinedBy rdf:resource="http://cybox.mitre.org/objects/WindowsTask"/>
        <rdfs:label>Windows Task</rdfs:label>
    </owl:Class>
</rdf:RDF>



<!-- Generated by the OWL API (version 4.2.6.20160910-2108) https://github.com/owlcs/owlapi -->

