<?xml version="1.0"?>
<rdf:RDF
    xmlns:report="http://stix.mitre.org/Report#"
    xmlns:rdf="http://www.w3.org/1999/02/22-rdf-syntax-ns#"
    xmlns:owl="http://www.w3.org/2002/07/owl#"
    xmlns:xsd="http://www.w3.org/2001/XMLSchema#"
    
    xmlns:rdfs="http://www.w3.org/2000/01/rdf-schema#"
  xml:base="http://stix.mitre.org/Report">
  <owl:Ontology rdf:about="http://stix.mitre.org/Report">
    <owl:imports rdf:resource="http://data-marking.mitre.org/Data_Marking"/>
    <rdfs:label >STIX Report Ontology</rdfs:label>
    <rdfs:comment >This ontology provides a vocabulary and representation for the Structured Threat Information eXpression (STIX) Report.  The Report ontology provides a characterization of the context to a given grouping of STIX content.</rdfs:comment>
    <owl:imports rdf:resource="http://stix.mitre.org/stixCommon"/>
    <owl:imports rdf:resource="http://cybox.mitre.org/cybox_core"/>
    <owl:versionIRI rdf:resource="http://stix.mitre.org/Report/1.2"/>
    
    <owl:versionInfo rdf:datatype="http://www.w3.org/2001/XMLSchema#string"
    >1.2.0-000</owl:versionInfo>
  </owl:Ontology>
  <owl:Class rdf:ID="Report">
    <rdfs:subClassOf>
      <owl:Restriction>
        <owl:maxCardinality rdf:datatype="http://www.w3.org/2001/XMLSchema#nonNegativeInteger"
        >1</owl:maxCardinality>
        <owl:onProperty>
          <rdf:Description rdf:about="http://stix.mitre.org/stixCommon#informationSource">
            <rdfs:domain rdf:resource="#Report"/>
          </rdf:Description>
        </owl:onProperty>
      </owl:Restriction>
    </rdfs:subClassOf>
    <rdfs:subClassOf>
      <owl:Restriction>
        <owl:maxCardinality rdf:datatype="http://www.w3.org/2001/XMLSchema#nonNegativeInteger"
        >1</owl:maxCardinality>
        <owl:onProperty rdf:resource="http://stix.mitre.org/stixCommon#timestamp"/>
      </owl:Restriction>
    </rdfs:subClassOf>
    <rdfs:subClassOf rdf:resource="http://stix.mitre.org/stixCommon#ReportBase"/>
    <rdfs:isDefinedBy rdf:resource=""/>
    <rdfs:comment >Characterizes a contextual wrapper for a given group of STIX content.</rdfs:comment>
    <rdfs:label >Report</rdfs:label>
    <rdfs:subClassOf>
      <owl:Restriction>
        <owl:cardinality rdf:datatype="http://www.w3.org/2001/XMLSchema#nonNegativeInteger"
        >1</owl:cardinality>
        <owl:onProperty rdf:resource="http://stix.mitre.org/stixCommon#id"/>
      </owl:Restriction>
    </rdfs:subClassOf>
    
    <rdfs:subClassOf>
      <owl:Restriction>
        <owl:cardinality rdf:datatype="http://www.w3.org/2001/XMLSchema#nonNegativeInteger"
        >1</owl:cardinality>
        <owl:onProperty>
          <rdf:Description rdf:about="http://stix.mitre.org/stixCommon#title">
            <rdfs:domain rdf:resource="#Report"/>
          </rdf:Description>
        </owl:onProperty>
      </owl:Restriction>
    </rdfs:subClassOf>
  </owl:Class>
  <owl:ObjectProperty rdf:ID="relatedReports">
    <rdfs:comment >Specifies a reference to one or more related Reports</rdfs:comment>
    <rdfs:label >Related Reports</rdfs:label>
    <rdfs:isDefinedBy rdf:resource=""/>
    <rdfs:range rdf:resource="http://stix.mitre.org/stixCommon#ReportBase"/>
    
    <rdfs:domain rdf:resource="#Report"/>
  </owl:ObjectProperty>
  <owl:DatatypeProperty rdf:ID="reportIntent">
    <rdfs:comment >Specifies the intended purpose(s) or use(s) of this report. 

Examples of report intent include Threat Report, Indicators, PBX, and Campaign Characterization (these specific values are only provided to help explainthe property: they are neither recommended values nor necessarily part of any existing vocabulary).  The content creator may choose any arbitrary value or may constrain the set of possible values by referencing an externally-defined vocabulary or leveraging a formally defined vocabulary.

By default, the Report Intent Vocabulary is used to defined a restricted set of values.</rdfs:comment>
    
    <rdfs:label >Intent</rdfs:label>
    <rdfs:isDefinedBy rdf:resource=""/>
    <rdfs:domain rdf:resource="#Report"/>
    
    
    <rdfs:range rdf:resource="http://www.w3.org/2001/XMLSchema#string"/>
  </owl:DatatypeProperty>
  <rdf:Description rdf:about="http://stix.mitre.org/stixCommon#threatActors">
    <rdfs:domain rdf:resource="#Report"/>
  </rdf:Description>
  <rdf:Description rdf:about="http://stix.mitre.org/stixCommon#incidents">
    <rdfs:domain rdf:resource="#Report"/>
  </rdf:Description>
  <rdf:Description rdf:about="http://stix.mitre.org/stixCommon#observables">
    <rdfs:domain rdf:resource="#Report"/>
  </rdf:Description>
  <rdf:Description rdf:about="http://stix.mitre.org/stixCommon#shortDescription">
    <rdfs:domain rdf:resource="#Report"/>
  </rdf:Description>
  <rdf:Description rdf:about="http://stix.mitre.org/stixCommon#indicators">
    <rdfs:domain rdf:resource="#Report"/>
  </rdf:Description>
  <rdf:Description rdf:about="http://stix.mitre.org/stixCommon#campaigns">
    <rdfs:domain rdf:resource="#Report"/>
  </rdf:Description>
  <rdf:Description rdf:about="http://stix.mitre.org/stixCommon#TTPs">
    <rdfs:domain rdf:resource="#Report"/>
  </rdf:Description>
  <rdf:Description rdf:about="http://data-marking.mitre.org/Data_Marking#handling">
    <rdfs:domain rdf:resource="#Report"/>
  </rdf:Description>
  <rdf:Description rdf:about="http://stix.mitre.org/stixCommon#description">
    <rdfs:domain rdf:resource="#Report"/>
  </rdf:Description>
  <rdf:Description rdf:about="http://stix.mitre.org/stixCommon#coursesOfAction">
    <rdfs:domain rdf:resource="#Report"/>
  </rdf:Description>
  <rdf:Description rdf:about="http://stix.mitre.org/stixCommon#exploitTargets">
    <rdfs:domain rdf:resource="#Report"/>
  </rdf:Description>
</rdf:RDF>

<!-- Created with TopBraid -->
