<?xml version="1.0"?>
<rdf:RDF xmlns="http://stix.mitre.org/TTP#"
     xml:base="http://stix.mitre.org/TTP"
     xmlns:owl="http://www.w3.org/2002/07/owl#"
     xmlns:xsd="http://www.w3.org/2001/XMLSchema#"
     xmlns:rdfs="http://www.w3.org/2000/01/rdf-schema#"
     xmlns:cyboxCommon="http://cybox.mitre.org/cyboxCommon#"
     xmlns:maec_common="http://maec.mitre.org/maec_common#"
     xmlns:stixCommon="http://stix.mitre.org/stixCommon#"
     xmlns:ttp="http://stix.mitre.org/TTP#"
     xmlns:ciq_common="http://www.oasis-open.org/ciq_common#"
     xmlns:rdf="http://www.w3.org/1999/02/22-rdf-syntax-ns#"
     xmlns:xml="http://www.w3.org/XML/1998/namespace"
     xmlns:data_marking="http://data-marking.mitre.org/Data_Marking#"
     xmlns:wgs84_pos="http://www.w3.org/2003/01/geo/wgs84_pos#"
     xmlns:cybox_core="http://cybox.mitre.org/cybox_core#"
     xmlns:foaf="http://xmlns.com/foaf/0.1/"
     xmlns:dc="http://purl.org/dc/elements/1.1/">
    <owl:Ontology rdf:about="http://stix.mitre.org/TTP">
        <owl:versionIRI rdf:resource="http://stix.mitre.org/TTP/1.2"/>
        <owl:imports rdf:resource="http://data-marking.mitre.org/Data_Marking"/>
        <owl:imports rdf:resource="http://www.oasis-open.org/ciq_common"/>
        <owl:imports rdf:resource="http://stix.mitre.org/stixCommon"/>
        <owl:imports rdf:resource="http://maec.mitre.org/maec_package"/>
        <owl:versionInfo rdf:datatype="http://www.w3.org/2001/XMLSchema#string">1.2.0-000</owl:versionInfo>
        <rdfs:label>STIX Tactics, Techniques, and Procedures (TTPs) Ontology</rdfs:label>
        <rdfs:comment>This ontology provides a vocabulary and representation for the Structured Threat Information eXpression (STIX) TTP.  The STIX TTP ontology provides a characterization of a single STIX Tactic, Techiques, and Procedures (TTPs).

TTP is a military term that means &quot;tactics, techniques, and procedures&quot;. In STIX it is used to represent adversarial behavior, such as what victims they target, what attack patterns and malware they use, and what resources (infrastructure, tools, personas) they leverage. Because it describes adversary behavior, which is a big part of STIX, the TTP construct is one of the most commonly used and expressive constructs. In the STIX relationship structure, TTPs are referenced from indicators to describe which TTPs an indicator indicates, from campaigns and threat actors to describe the TTPs that are leveraged in a campaign or by a threat actor, in an incident to describe which TTPs were used in the execution of an attack, and to other TTPs to describe relationships of various sorts among TTPs. TTPs also use the exploit target construct to describe which exploit targets a TTP might exploit.</rdfs:comment>
    </owl:Ontology>
    




    <!-- 
    ///////////////////////////////////////////////////////////////////////////////////////
    //
    // Object Properties
    //
    ///////////////////////////////////////////////////////////////////////////////////////
     -->

    


    <!-- http://stix.mitre.org/TTP#behavior.attackPatterns -->

    <owl:ObjectProperty rdf:about="http://stix.mitre.org/TTP#behavior.attackPatterns">
        <rdfs:range>
            <owl:Class>
                <owl:unionOf rdf:parseType="Collection">
                    <rdf:Description rdf:about="http://capec.mitre.org/capec#AttackPattern"/>
                    <rdf:Description rdf:about="http://stix.mitre.org/TTP#AttackPattern"/>
                </owl:unionOf>
            </owl:Class>
        </rdfs:range>
        <rdfs:comment>Specifies a reference to one or more attack patterns that an adversary might leverage.</rdfs:comment>
        <rdfs:isDefinedBy rdf:resource="http://stix.mitre.org/TTP"/>
        <rdfs:label>Behavior Attack Patterns</rdfs:label>
    </owl:ObjectProperty>
    


    <!-- http://stix.mitre.org/TTP#behavior.exploits -->

    <owl:ObjectProperty rdf:about="http://stix.mitre.org/TTP#behavior.exploits">
        <rdfs:range rdf:resource="http://stix.mitre.org/TTP#Exploit"/>
        <rdfs:comment>Specifies a reference to a set of one or more exploits that an adversary may leverage.</rdfs:comment>
        <rdfs:isDefinedBy rdf:resource="http://stix.mitre.org/TTP"/>
        <rdfs:label>Behavior Exploits</rdfs:label>
    </owl:ObjectProperty>
    


    <!-- http://stix.mitre.org/TTP#behavior.malware -->

    <owl:ObjectProperty rdf:about="http://stix.mitre.org/TTP#behavior.malware">
        <rdfs:range rdf:resource="http://stix.mitre.org/TTP#MalwareInstance"/>
        <rdfs:comment>Specifies one or more instances of malware that the attacker leverages to execute this TTP.</rdfs:comment>
        <rdfs:isDefinedBy rdf:resource="http://stix.mitre.org/TTP"/>
        <rdfs:label>Behavior Malware</rdfs:label>
    </owl:ObjectProperty>
    


    <!-- http://stix.mitre.org/TTP#capecReference -->

    <owl:ObjectProperty rdf:about="http://stix.mitre.org/TTP#capecReference">
        <rdfs:range rdf:resource="http://capec.mitre.org/capec#AttackPattern"/>
        <rdfs:comment>Specifies a reference to a particular entry within the Common Attack Pattern Enumeration and Classification (CAPEC) registry.</rdfs:comment>
        <rdfs:isDefinedBy rdf:resource="http://stix.mitre.org/TTP"/>
        <rdfs:label>CAPEC Reference</rdfs:label>
    </owl:ObjectProperty>
    


    <!-- http://stix.mitre.org/TTP#exploitTargets -->

    <owl:ObjectProperty rdf:about="http://stix.mitre.org/TTP#exploitTargets">
        <rdfs:range rdf:resource="http://stix.mitre.org/stixCommon#ExploitTargetBase"/>
        <rdfs:comment>Specifies a reference to a set of one or more Exploit Targets potentially targeted by the TTP.</rdfs:comment>
        <rdfs:isDefinedBy rdf:resource="http://stix.mitre.org/TTP"/>
        <rdfs:label>Exploit Targets</rdfs:label>
    </owl:ObjectProperty>
    


    <!-- http://stix.mitre.org/TTP#intendedEffect -->

    <owl:ObjectProperty rdf:about="http://stix.mitre.org/TTP#intendedEffect">
        <rdfs:range rdf:resource="http://stix.mitre.org/stixCommon#IntendedEffectStatement"/>
        <rdfs:comment>Specifies the suspected intended effect for this TTP.</rdfs:comment>
        <rdfs:isDefinedBy rdf:resource="http://stix.mitre.org/TTP"/>
        <rdfs:label>Intended Effect</rdfs:label>
    </owl:ObjectProperty>
    


    <!-- http://stix.mitre.org/TTP#killChainPhases -->

    <owl:ObjectProperty rdf:about="http://stix.mitre.org/TTP#killChainPhases">
        <rdfs:range rdf:resource="http://stix.mitre.org/stixCommon#KillChainPhase"/>
        <rdfs:comment>Specifies a reference to a set of one or more kill chain phases (from one or more kill chains defined elsewhere) for which the TTP is asserted to be representative.</rdfs:comment>
        <rdfs:isDefinedBy rdf:resource="http://stix.mitre.org/TTP"/>
        <rdfs:label>Kill Chain Phases</rdfs:label>
    </owl:ObjectProperty>
    


    <!-- http://stix.mitre.org/TTP#killChains -->

    <owl:ObjectProperty rdf:about="http://stix.mitre.org/TTP#killChains">
        <rdfs:range rdf:resource="http://stix.mitre.org/stixCommon#KillChain"/>
        <rdfs:comment>Specifies a reference to a set of one or more specific kill chain definitions.</rdfs:comment>
        <rdfs:isDefinedBy rdf:resource="http://stix.mitre.org/TTP"/>
        <rdfs:label>Kill Chains</rdfs:label>
    </owl:ObjectProperty>
    


    <!-- http://stix.mitre.org/TTP#maecPackage -->

    <owl:ObjectProperty rdf:about="http://stix.mitre.org/TTP#maecPackage">
        <rdfs:range rdf:resource="http://maec.mitre.org/maec_package#Package"/>
        <rdfs:comment>Specifies a reference to the structured characterization of malware instances using the MAEC Package data model.</rdfs:comment>
        <rdfs:isDefinedBy rdf:resource="http://stix.mitre.org/TTP"/>
        <rdfs:label>Malware Characterization</rdfs:label>
    </owl:ObjectProperty>
    


    <!-- http://stix.mitre.org/TTP#observableCharacterization -->

    <owl:ObjectProperty rdf:about="http://stix.mitre.org/TTP#observableCharacterization">
        <rdfs:range rdf:resource="http://cybox.mitre.org/cybox_core#Observables"/>
        <rdfs:comment>Specifies a reference to the adversarial infrastructure through specification of a structured cyber Observables pattern.</rdfs:comment>
        <rdfs:isDefinedBy rdf:resource="http://stix.mitre.org/TTP"/>
        <rdfs:label>Observable Characterization</rdfs:label>
    </owl:ObjectProperty>
    


    <!-- http://stix.mitre.org/TTP#resources.infrastructure -->

    <owl:ObjectProperty rdf:about="http://stix.mitre.org/TTP#resources.infrastructure">
        <rdfs:range rdf:resource="http://stix.mitre.org/TTP#Infrastructure"/>
        <rdfs:comment>Specifies a reference to resources the adversary may leverage.</rdfs:comment>
        <rdfs:isDefinedBy rdf:resource="http://stix.mitre.org/TTP"/>
        <rdfs:label>Infrastructure Resource Utilized</rdfs:label>
    </owl:ObjectProperty>
    


    <!-- http://stix.mitre.org/TTP#resources.personas -->

    <owl:ObjectProperty rdf:about="http://stix.mitre.org/TTP#resources.personas">
        <rdfs:range>
            <owl:Class>
                <owl:unionOf rdf:parseType="Collection">
                    <rdf:Description rdf:about="http://stix.mitre.org/stixCommon#CIQIdentity"/>
                    <rdf:Description rdf:about="http://www.oasis-open.org/ciq_xpil#Organization"/>
                    <rdf:Description rdf:about="http://www.oasis-open.org/ciq_xpil#Party"/>
                    <rdf:Description rdf:about="http://www.oasis-open.org/ciq_xpil#Person"/>
                </owl:unionOf>
            </owl:Class>
        </rdfs:range>
        <rdfs:comment>Specific a reference to a set of one or more personas that an adversary may leverage. 

Different personas are often used as a method of masquerade.</rdfs:comment>
        <rdfs:isDefinedBy rdf:resource="http://stix.mitre.org/TTP"/>
        <rdfs:label>Persona Resources Utilized</rdfs:label>
    </owl:ObjectProperty>
    


    <!-- http://stix.mitre.org/TTP#resources.tools -->

    <owl:ObjectProperty rdf:about="http://stix.mitre.org/TTP#resources.tools">
        <rdfs:range rdf:resource="http://stix.mitre.org/stixCommon#ToolInformation"/>
        <rdfs:comment>Specifies the tools that the adversary uses to execute this TTP.</rdfs:comment>
        <rdfs:isDefinedBy rdf:resource="http://stix.mitre.org/TTP"/>
        <rdfs:label>Tool Resources Utilized</rdfs:label>
    </owl:ObjectProperty>
    


    <!-- http://stix.mitre.org/TTP#victimTargeting.identity -->

    <owl:ObjectProperty rdf:about="http://stix.mitre.org/TTP#victimTargeting.identity">
        <rdfs:range>
            <owl:Class>
                <owl:unionOf rdf:parseType="Collection">
                    <rdf:Description rdf:about="http://stix.mitre.org/stixCommon#CIQIdentity"/>
                    <rdf:Description rdf:about="http://www.oasis-open.org/ciq_xpil#Organization"/>
                    <rdf:Description rdf:about="http://www.oasis-open.org/ciq_xpil#Party"/>
                    <rdf:Description rdf:about="http://www.oasis-open.org/ciq_xpil#Person"/>
                </owl:unionOf>
            </owl:Class>
        </rdfs:range>
        <rdfs:comment>Specifies a reference to traits common to the people or organizations that are targeted.</rdfs:comment>
        <rdfs:isDefinedBy rdf:resource="http://stix.mitre.org/TTP"/>
        <rdfs:label>Victim Targeted Identity</rdfs:label>
    </owl:ObjectProperty>
    


    <!-- http://stix.mitre.org/TTP#victimTargeting.targetedTechnicalDetails -->

    <owl:ObjectProperty rdf:about="http://stix.mitre.org/TTP#victimTargeting.targetedTechnicalDetails">
        <rdfs:range rdf:resource="http://cybox.mitre.org/cybox_core#Observables"/>
        <rdfs:comment>Specifies a reference to details of specific technologies targeted by the adversary. 

It is implemented through specification of a structured cyber Observables pattern using the CybOX ObservablesType class.</rdfs:comment>
        <rdfs:isDefinedBy rdf:resource="http://stix.mitre.org/TTP"/>
        <rdfs:label>Victim Targeted Technical Details</rdfs:label>
    </owl:ObjectProperty>
    


    <!-- 
    ///////////////////////////////////////////////////////////////////////////////////////
    //
    // Data properties
    //
    ///////////////////////////////////////////////////////////////////////////////////////
     -->

    


    <!-- http://stix.mitre.org/TTP#capecID -->

    <owl:DatatypeProperty rdf:about="http://stix.mitre.org/TTP#capecID">
        <rdfs:range rdf:resource="http://www.w3.org/2001/XMLSchema#string"/>
        <rdfs:comment>Specifies an identifier to a particular entry within the Common Attack Pattern Enumeration and Classification (CAPEC)</rdfs:comment>
        <rdfs:isDefinedBy rdf:resource="http://stix.mitre.org/TTP"/>
        <rdfs:label>CAPEC ID</rdfs:label>
    </owl:DatatypeProperty>
    


    <!-- http://stix.mitre.org/TTP#infrastructureType -->

    <owl:DatatypeProperty rdf:about="http://stix.mitre.org/TTP#infrastructureType">
        <rdfs:range rdf:resource="http://www.w3.org/2001/XMLSchema#string"/>
        <rdfs:comment>Specifies the type of attacker infrastructure being described. 

Examples of types of attacker infrastructure include Anonymization, Domain Registration, Hosting, and Communications - Social Networks (these specific values are only provided to help explain the property: they are neither recommended values nor necessarily part of any existing vocabulary).  The content creator may choose any arbitrary value or may constrain the set of possible values by referencing an externally-defined vocabulary or leveraging a formally defined vocabulary.

By default, the Attack Infrastructure Type Vocabulary is used to defined a restricted set of values.</rdfs:comment>
        <rdfs:isDefinedBy rdf:resource="http://stix.mitre.org/TTP"/>
        <rdfs:label>Infrastructure Type</rdfs:label>
    </owl:DatatypeProperty>
    


    <!-- http://stix.mitre.org/TTP#malwareInstanceName -->

    <owl:DatatypeProperty rdf:about="http://stix.mitre.org/TTP#malwareInstanceName">
        <rdfs:range rdf:resource="http://www.w3.org/2001/XMLSchema#string"/>
        <rdfs:comment>Specifies a name associated with this MalwareInstance.</rdfs:comment>
        <rdfs:isDefinedBy rdf:resource="http://stix.mitre.org/TTP"/>
        <rdfs:label>Malware Instance Name</rdfs:label>
    </owl:DatatypeProperty>
    


    <!-- http://stix.mitre.org/TTP#malwareInstanceType -->

    <owl:DatatypeProperty rdf:about="http://stix.mitre.org/TTP#malwareInstanceType">
        <rdfs:range rdf:resource="http://www.w3.org/2001/XMLSchema#string"/>
        <rdfs:comment>Specifies the type of malware. 

Examples of types of malware include Adware, Exploit Kits, Ransomware, and Rootkit (these specific values are only provided to help explain the property: they are neither recommended values nor necessarily part of any existing vocabulary).  The content creator may choose any arbitrary value or may constrain the set of possible values by referencing an externally-defined vocabulary or leveraging a formally defined vocabulary.

By default, the Malware Type Vocabulary is used to defined a restricted set of values.</rdfs:comment>
        <rdfs:isDefinedBy rdf:resource="http://stix.mitre.org/TTP"/>
        <rdfs:label>Malware Instance Type</rdfs:label>
    </owl:DatatypeProperty>
    


    <!-- http://stix.mitre.org/TTP#vicitimTargeting.targetedSystems -->

    <owl:DatatypeProperty rdf:about="http://stix.mitre.org/TTP#vicitimTargeting.targetedSystems">
        <rdfs:range rdf:resource="http://www.w3.org/2001/XMLSchema#string"/>
        <rdfs:comment>Specifies the type of system that is targeted. 

Examples of types of systems include Enterprise Systems, Industrial Control Systems, Mobile Systems, and Users - Application And Software (these specific values are only provided to help explain the property: they are neither recommended values nor necessarily part of any existing vocabulary).  The content creator may choose any arbitrary value or may constrain the set of possible values by referencing an externally-defined vocabulary or leveraging a formally defined vocabulary.

By default, the System Type Vocabulary is used to defined a restricted set of values.</rdfs:comment>
        <rdfs:isDefinedBy rdf:resource="http://stix.mitre.org/TTP"/>
        <rdfs:label>Victim Targeted Systems</rdfs:label>
    </owl:DatatypeProperty>
    


    <!-- http://stix.mitre.org/TTP#victimTargeting.targetedInformation -->

    <owl:DatatypeProperty rdf:about="http://stix.mitre.org/TTP#victimTargeting.targetedInformation">
        <rdfs:range rdf:resource="http://www.w3.org/2001/XMLSchema#string"/>
        <rdfs:comment>Specifies a type of information that is targeted.

Examples of types of information include Information Assets, Information Assets - Customer PII, and Authentication Cookies (these specific values are only provided to help explain the property: they are neither recommended values nor necessarily part of any existing vocabulary).  The content creator may choose any arbitrary value or may constrain the set of possible values by referencing an externally-defined vocabulary or leveraging a formally defined vocabulary.

By default, the Information Type Vocabulary is used to defined a restricted set of values.</rdfs:comment>
        <rdfs:isDefinedBy rdf:resource="http://stix.mitre.org/TTP"/>
        <rdfs:label>Victim Targeted Information</rdfs:label>
    </owl:DatatypeProperty>
    


    <!-- 
    ///////////////////////////////////////////////////////////////////////////////////////
    //
    // Classes
    //
    ///////////////////////////////////////////////////////////////////////////////////////
     -->

    

    


    <!-- http://stix.mitre.org/TTP#AttackPattern -->

    <owl:Class rdf:about="http://stix.mitre.org/TTP#AttackPattern">
        <rdfs:subClassOf>
            <owl:Restriction>
                <owl:onProperty rdf:resource="http://stix.mitre.org/TTP#capecID"/>
                <owl:someValuesFrom rdf:resource="http://www.w3.org/2000/01/rdf-schema#Literal"/>
            </owl:Restriction>
        </rdfs:subClassOf>
        <rdfs:comment>Characterizes an individual attack pattern through the capture of information such as a textual description and a Common Attack Pattern Enumeration and Classification (CAPEC) reference.</rdfs:comment>
        <rdfs:isDefinedBy rdf:resource="http://stix.mitre.org/TTP"/>
        <rdfs:label>TTP Attack Pattern Synopsis</rdfs:label>
    </owl:Class>
    


    <!-- http://stix.mitre.org/TTP#Exploit -->

    <owl:Class rdf:about="http://stix.mitre.org/TTP#Exploit">
        <rdfs:comment>Characterizes an individual exploit instance through the capture of basic information such as the title and description of the exploit.</rdfs:comment>
        <rdfs:isDefinedBy rdf:resource="http://stix.mitre.org/TTP"/>
        <rdfs:label>Exploit</rdfs:label>
    </owl:Class>
    


    <!-- http://stix.mitre.org/TTP#Infrastructure -->

    <owl:Class rdf:about="http://stix.mitre.org/TTP#Infrastructure">
        <rdfs:subClassOf>
            <owl:Restriction>
                <owl:onProperty rdf:resource="http://stix.mitre.org/TTP#infrastructureType"/>
                <owl:someValuesFrom rdf:resource="http://www.w3.org/2000/01/rdf-schema#Literal"/>
            </owl:Restriction>
        </rdfs:subClassOf>
        <rdfs:comment>Characterizes adversarial infrastructure that an adversary may leverage.</rdfs:comment>
        <rdfs:isDefinedBy rdf:resource="http://stix.mitre.org/TTP"/>
        <rdfs:label>Infrastructure</rdfs:label>
    </owl:Class>
    


    <!-- http://stix.mitre.org/TTP#MalwareInstance -->

    <owl:Class rdf:about="http://stix.mitre.org/TTP#MalwareInstance">
        <rdfs:comment>Characterizes a malware instance through the capture of basic information such as the type, name, and description of the malware.

A malware instance may characterize anything from a specific malware sample to an entire family. .</rdfs:comment>
        <rdfs:isDefinedBy rdf:resource="http://stix.mitre.org/TTP"/>
        <rdfs:label>Malware instance</rdfs:label>
    </owl:Class>
    


    <!-- http://stix.mitre.org/TTP#TTP -->

    <owl:Class rdf:about="http://stix.mitre.org/TTP#TTP">
        <rdfs:subClassOf rdf:resource="http://stix.mitre.org/stixCommon#TTPBase"/>
        <rdfs:subClassOf>
            <owl:Restriction>
                <owl:onProperty rdf:resource="http://stix.mitre.org/TTP#resources.infrastructure"/>
                <owl:someValuesFrom rdf:resource="http://www.w3.org/2002/07/owl#Thing"/>
            </owl:Restriction>
        </rdfs:subClassOf>
        <rdfs:subClassOf>
            <owl:Restriction>
                <owl:onProperty rdf:resource="http://stix.mitre.org/TTP#victimTargeting.targetedTechnicalDetails"/>
                <owl:someValuesFrom rdf:resource="http://www.w3.org/2002/07/owl#Thing"/>
            </owl:Restriction>
        </rdfs:subClassOf>
        <rdfs:comment>Characterizes adversarial mode of operations (often referred to as the adversary’s “Tactics, Techniques, and Procedures”). 

The TTP class captures information that includes the victims targeted, the attack patterns and malware used, and the resources (infrastructure, tools, and personas) leveraged.</rdfs:comment>
        <rdfs:isDefinedBy rdf:resource="http://stix.mitre.org/TTP"/>
        <rdfs:label>TTP</rdfs:label>
    </owl:Class>
    


</rdf:RDF>



<!-- Generated by the OWL API (version 4.2.6.20160910-2108) https://github.com/owlcs/owlapi -->

