<?xml version="1.0"?>
<rdf:RDF xmlns="http://cwe.mitre.org/cwe#"
     xml:base="http://cwe.mitre.org/cwe"
     xmlns:capec="http://capec.mitre.org/capec#"
     xmlns:cwe="http://cwe.mitre.org/cwe#"
     xmlns:cve="http://nvd.nist.gov/cve#"
     xmlns:rdf="http://www.w3.org/1999/02/22-rdf-syntax-ns#"
     xmlns:owl="http://www.w3.org/2002/07/owl#"
     xmlns:xml="http://www.w3.org/XML/1998/namespace"
     xmlns:xsd="http://www.w3.org/2001/XMLSchema#"
     xmlns:rdfs="http://www.w3.org/2000/01/rdf-schema#">
    <owl:Ontology rdf:about="http://cwe.mitre.org/cwe">
        <owl:imports rdf:resource="http://cpe.mitre.org/cpe"/>
        <owl:imports rdf:resource="http://scap.nist.gov/scap_core"/>
        <owl:imports rdf:resource="http://capec.mitre.org/capec"/>
        <owl:imports rdf:resource="http://cybox.mitre.org/objects/NetworkProtocol"/>
        <owl:imports rdf:resource="http://nvd.nist.gov/cve"/>
        <rdfs:label>Common Weakness Enumeration (CWE) Ontology</rdfs:label>
        <rdfs:comment>This ontology provides a vocabulary and representation for the Common Weakness Enumeration (CWE) which provides a unified, measurable set of software weaknesses that is enabling more effective discussion, description, selection, and use of software security tools and services that can find these weaknesses in source code and operational systems as well as better understanding and management of software weaknesses related to architecture and design. 

Copyright (c) 2014, DaedaFusion, LLC.  All rights reserved.</rdfs:comment>
        <owl:versionInfo rdf:datatype="http://www.w3.org/2001/XMLSchema#string">v1.0.0-001</owl:versionInfo>
    </owl:Ontology>
    


    <!-- 
    ///////////////////////////////////////////////////////////////////////////////////////
    //
    // Annotation properties
    //
    ///////////////////////////////////////////////////////////////////////////////////////
     -->

    


    <!-- http://www.w3.org/2002/07/owl#maxCardinality -->

    <owl:AnnotationProperty rdf:about="http://www.w3.org/2002/07/owl#maxCardinality"/>
    


    <!-- 
    ///////////////////////////////////////////////////////////////////////////////////////
    //
    // Datatypes
    //
    ///////////////////////////////////////////////////////////////////////////////////////
     -->

    


    <!-- http://www.w3.org/2001/XMLSchema#date -->

    <rdfs:Datatype rdf:about="http://www.w3.org/2001/XMLSchema#date"/>
    


    <!-- http://www.w3.org/2001/XMLSchema#gYear -->

    <rdfs:Datatype rdf:about="http://www.w3.org/2001/XMLSchema#gYear"/>
    


    <!-- 
    ///////////////////////////////////////////////////////////////////////////////////////
    //
    // Object Properties
    //
    ///////////////////////////////////////////////////////////////////////////////////////
     -->

    


    <!-- http://cwe.mitre.org/cwe#alternateTerms -->

    <owl:ObjectProperty rdf:about="http://cwe.mitre.org/cwe#alternateTerms">
        <rdfs:domain rdf:resource="http://cwe.mitre.org/cwe#Category"/>
        <rdfs:domain rdf:resource="http://cwe.mitre.org/cwe#CompoundElement"/>
        <rdfs:domain rdf:resource="http://cwe.mitre.org/cwe#View"/>
        <rdfs:domain rdf:resource="http://cwe.mitre.org/cwe#Weakness"/>
        <rdfs:range rdf:resource="http://cwe.mitre.org/cwe#Term"/>
        <rdfs:comment>Defines zero or more  alternate terms by which this weakness may be known and a description to explain the context in which the term may be relevant</rdfs:comment>
        <rdfs:label>Alternate Terms</rdfs:label>
    </owl:ObjectProperty>
    


    <!-- http://cwe.mitre.org/cwe#applicableLanguages -->

    <owl:ObjectProperty rdf:about="http://cwe.mitre.org/cwe#applicableLanguages">
        <rdfs:domain rdf:resource="http://cwe.mitre.org/cwe#CompoundElement"/>
        <rdfs:domain rdf:resource="http://cwe.mitre.org/cwe#Mitigation"/>
        <rdfs:range rdf:resource="http://cwe.mitre.org/cwe#ProgrammingLanguage"/>
        <rdfs:comment>Defines one or more Languages which each represent a language in which this mitigation may exist.</rdfs:comment>
        <rdfs:label>Applicable Languages</rdfs:label>
    </owl:ObjectProperty>
    


    <!-- http://cwe.mitre.org/cwe#applicablePlatforms.ArchitectureParadigms -->

    <owl:ObjectProperty rdf:about="http://cwe.mitre.org/cwe#applicablePlatforms.ArchitectureParadigms">
        <rdfs:domain rdf:resource="http://cwe.mitre.org/cwe#Category"/>
        <rdfs:domain rdf:resource="http://cwe.mitre.org/cwe#CompoundElement"/>
        <rdfs:domain rdf:resource="http://cwe.mitre.org/cwe#Weakness"/>
        <rdfs:range rdf:resource="http://cwe.mitre.org/cwe#ArchitectureParadigm"/>
        <rdfs:comment>Defines one or more Architectural Paradigms  represent an architecture on which this weakness is likely to exist.</rdfs:comment>
        <rdfs:label>Applicable Architecture Paradigms</rdfs:label>
    </owl:ObjectProperty>
    


    <!-- http://cwe.mitre.org/cwe#applicablePlatforms.CommonPlatformReferences -->

    <owl:ObjectProperty rdf:about="http://cwe.mitre.org/cwe#applicablePlatforms.CommonPlatformReferences">
        <rdfs:domain rdf:resource="http://cwe.mitre.org/cwe#Category"/>
        <rdfs:domain rdf:resource="http://cwe.mitre.org/cwe#CompoundElement"/>
        <rdfs:domain rdf:resource="http://cwe.mitre.org/cwe#Weakness"/>
        <rdfs:range rdf:resource="http://cpe.mitre.org/cpe#CPE"/>
        <rdfs:comment>Defines references to the Common Platform Enumeration, CPE, which will identify common platforms on which this weakness may occur. It has one or more Common_Platform elements as children and each child will point to a single CPE entry which is associated with this weakness.</rdfs:comment>
        <rdfs:label>Common Platform References</rdfs:label>
    </owl:ObjectProperty>
    


    <!-- http://cwe.mitre.org/cwe#applicablePlatforms.Environments -->

    <owl:ObjectProperty rdf:about="http://cwe.mitre.org/cwe#applicablePlatforms.Environments">
        <rdfs:domain rdf:resource="http://cwe.mitre.org/cwe#Category"/>
        <rdfs:domain rdf:resource="http://cwe.mitre.org/cwe#CompoundElement"/>
        <rdfs:domain rdf:resource="http://cwe.mitre.org/cwe#Weakness"/>
        <rdfs:range rdf:resource="http://cwe.mitre.org/cwe#Environment"/>
        <rdfs:comment>Defines one or more Environments which each represent an environment in which this weakness may exist.</rdfs:comment>
        <rdfs:label>Applicable Environments</rdfs:label>
    </owl:ObjectProperty>
    


    <!-- http://cwe.mitre.org/cwe#applicablePlatforms.HardwareArchitecture -->

    <owl:ObjectProperty rdf:about="http://cwe.mitre.org/cwe#applicablePlatforms.HardwareArchitecture">
        <rdfs:domain rdf:resource="http://cwe.mitre.org/cwe#Category"/>
        <rdfs:domain rdf:resource="http://cwe.mitre.org/cwe#CompoundElement"/>
        <rdfs:domain rdf:resource="http://cwe.mitre.org/cwe#Weakness"/>
        <rdfs:range rdf:resource="http://cwe.mitre.org/cwe#HardwareArchitecture"/>
        <rdfs:comment>Defines one or more Hardware Architectures which each represent an architecture in which this weakness is likely to exist.</rdfs:comment>
        <rdfs:label>Applicable Hardware Architectures</rdfs:label>
    </owl:ObjectProperty>
    


    <!-- http://cwe.mitre.org/cwe#applicablePlatforms.Languages -->

    <owl:ObjectProperty rdf:about="http://cwe.mitre.org/cwe#applicablePlatforms.Languages">
        <rdfs:domain rdf:resource="http://cwe.mitre.org/cwe#Category"/>
        <rdfs:domain rdf:resource="http://cwe.mitre.org/cwe#Weakness"/>
        <rdfs:range rdf:resource="http://cwe.mitre.org/cwe#ProgrammingLanguage"/>
        <rdfs:comment>Specifies a contains one or more Language elements which each represent a language in which this weakness may exist.</rdfs:comment>
        <rdfs:label>Applicable Programming Languages</rdfs:label>
    </owl:ObjectProperty>
    


    <!-- http://cwe.mitre.org/cwe#applicablePlatforms.OperatingSystems -->

    <owl:ObjectProperty rdf:about="http://cwe.mitre.org/cwe#applicablePlatforms.OperatingSystems">
        <rdfs:domain rdf:resource="http://cwe.mitre.org/cwe#Category"/>
        <rdfs:domain rdf:resource="http://cwe.mitre.org/cwe#CompoundElement"/>
        <rdfs:domain rdf:resource="http://cwe.mitre.org/cwe#Weakness"/>
        <rdfs:range rdf:resource="http://cwe.mitre.org/cwe#OperatingSystem"/>
        <rdfs:comment>Defines one or more Operating System in which this weakness is likely to exist.</rdfs:comment>
        <rdfs:label>Applicable Operating Systems</rdfs:label>
    </owl:ObjectProperty>
    


    <!-- http://cwe.mitre.org/cwe#applicablePlatforms.PlatformNotes -->

    <owl:ObjectProperty rdf:about="http://cwe.mitre.org/cwe#applicablePlatforms.PlatformNotes">
        <rdfs:domain rdf:resource="http://cwe.mitre.org/cwe#Category"/>
        <rdfs:domain rdf:resource="http://cwe.mitre.org/cwe#CompoundElement"/>
        <rdfs:domain rdf:resource="http://cwe.mitre.org/cwe#Weakness"/>
        <rdfs:range rdf:resource="http://cwe.mitre.org/cwe#Note"/>
        <rdfs:comment>Defines a additional information related to the applicable platforms of a weakness if needed.</rdfs:comment>
        <rdfs:label>Platform Notes</rdfs:label>
    </owl:ObjectProperty>
    


    <!-- http://cwe.mitre.org/cwe#applicablePlatforms.TechnologyClasses -->

    <owl:ObjectProperty rdf:about="http://cwe.mitre.org/cwe#applicablePlatforms.TechnologyClasses">
        <rdfs:domain rdf:resource="http://cwe.mitre.org/cwe#Category"/>
        <rdfs:domain rdf:resource="http://cwe.mitre.org/cwe#CompoundElement"/>
        <rdfs:domain rdf:resource="http://cwe.mitre.org/cwe#Weakness"/>
        <rdfs:range rdf:resource="http://cwe.mitre.org/cwe#TechnologyClass"/>
        <rdfs:comment>Defines one or more individual Technology Class which each represent a technology class in which this weakness is likely to exist.</rdfs:comment>
        <rdfs:label>Applicable Technology Classes</rdfs:label>
    </owl:ObjectProperty>
    


    <!-- http://cwe.mitre.org/cwe#audience -->

    <owl:ObjectProperty rdf:about="http://cwe.mitre.org/cwe#audience">
        <rdfs:domain rdf:resource="http://cwe.mitre.org/cwe#View"/>
        <rdfs:range rdf:resource="http://cwe.mitre.org/cwe#Audience"/>
        <rdfs:comment>Specifies a reference to the targeted audiences or groups for this view.</rdfs:comment>
        <rdfs:label>Audience</rdfs:label>
    </owl:ObjectProperty>
    


    <!-- http://cwe.mitre.org/cwe#author -->

    <owl:ObjectProperty rdf:about="http://cwe.mitre.org/cwe#author">
        <rdfs:domain rdf:resource="http://cwe.mitre.org/cwe#HistoryRecord"/>
        <rdfs:range>
            <owl:Class>
                <owl:unionOf rdf:parseType="Collection">
                    <rdf:Description rdf:about="http://www.oasis-open.org/ciq_xpil#Organization"/>
                    <rdf:Description rdf:about="http://www.oasis-open.org/ciq_xpil#Party"/>
                    <rdf:Description rdf:about="http://www.oasis-open.org/ciq_xpil#Person"/>
                </owl:unionOf>
            </owl:Class>
        </rdfs:range>
        <rdfs:comment>Specifies references to one or more individuals that authored the submitted, contributed, or modified the Weakness, View, Category, or CompoundElement.</rdfs:comment>
        <rdfs:label>Author</rdfs:label>
    </owl:ObjectProperty>
    


    <!-- http://cwe.mitre.org/cwe#authorOrganization -->

    <owl:ObjectProperty rdf:about="http://cwe.mitre.org/cwe#authorOrganization">
        <rdfs:domain rdf:resource="http://cwe.mitre.org/cwe#HistoryRecord"/>
        <rdfs:range rdf:resource="http://www.oasis-open.org/ciq_xpil#Organization"/>
        <rdfs:comment>Specifies one or more references tothe organization which submitted, contributed, or modified the Weakness, View, Category, or CompoundElement</rdfs:comment>
        <rdfs:label>Author Organization</rdfs:label>
    </owl:ObjectProperty>
    


    <!-- http://cwe.mitre.org/cwe#backgroundDetails -->

    <owl:ObjectProperty rdf:about="http://cwe.mitre.org/cwe#backgroundDetails">
        <rdfs:domain rdf:resource="http://cwe.mitre.org/cwe#Category"/>
        <rdfs:domain rdf:resource="http://cwe.mitre.org/cwe#CompoundElement"/>
        <rdfs:domain rdf:resource="http://cwe.mitre.org/cwe#Weakness"/>
        <rdfs:range rdf:resource="http://cwe.mitre.org/cwe#BackgroundDetail"/>
        <rdfs:comment>Specifies one or more Background Details, each of which holds information regarding the entry or any technologies that are related to it, where the background information is not related to the nature of the entry itself. It should be filled out where appropriate.</rdfs:comment>
        <rdfs:label>Background Details</rdfs:label>
    </owl:ObjectProperty>
    


    <!-- http://cwe.mitre.org/cwe#blackBoxDefinitons -->

    <owl:ObjectProperty rdf:about="http://cwe.mitre.org/cwe#blackBoxDefinitons">
        <rdfs:domain rdf:resource="http://cwe.mitre.org/cwe#Category"/>
        <rdfs:domain rdf:resource="http://cwe.mitre.org/cwe#CompoundElement"/>
        <rdfs:domain rdf:resource="http://cwe.mitre.org/cwe#Weakness"/>
        <rdfs:range rdf:resource="http://cwe.mitre.org/cwe#BlackBoxDefinition"/>
        <rdfs:comment>Defines  one or more Black Box Definitions, each of which describes the weakness from an external perspective, 	meaning that the view includes no knowledge of how the software is processing data other than what can be inferred from observing the software&apos;s behavior.</rdfs:comment>
        <rdfs:label>Black Box Definitions</rdfs:label>
    </owl:ObjectProperty>
    


    <!-- http://cwe.mitre.org/cwe#block -->

    <owl:ObjectProperty rdf:about="http://cwe.mitre.org/cwe#block">
        <rdfs:domain rdf:resource="http://cwe.mitre.org/cwe#StructuredText"/>
        <rdfs:range rdf:resource="http://cwe.mitre.org/cwe#Block"/>
        <rdfs:comment>Defines a block of text</rdfs:comment>
        <rdfs:label>Block</rdfs:label>
    </owl:ObjectProperty>
    


    <!-- http://cwe.mitre.org/cwe#categories -->

    <owl:ObjectProperty rdf:about="http://cwe.mitre.org/cwe#categories">
        <rdfs:domain rdf:resource="http://cwe.mitre.org/cwe#WeaknessCatalog"/>
        <rdfs:range rdf:resource="http://cwe.mitre.org/cwe#Category"/>
        <rdfs:comment>Defines  zero or more Category 	elements. Each Category element represents what used to be referred to in CWE as a &quot;Grouping&quot; entry. That is, a category is now a collection of 	weaknesses based on a common attribute, such as CWE-310 Cryptographic Issues or CWE-355 User Interface Security Issues.</rdfs:comment>
        <rdfs:label>Categories</rdfs:label>
    </owl:ObjectProperty>
    


    <!-- http://cwe.mitre.org/cwe#chains -->

    <owl:ObjectProperty rdf:about="http://cwe.mitre.org/cwe#chains">
        <rdfs:domain rdf:resource="http://cwe.mitre.org/cwe#RelationshipStatement"/>
        <rdfs:range rdf:resource="http://cwe.mitre.org/cwe#CompoundElement"/>
        <rdfs:comment>Specifes a list of the individual Chains this relationship pertains to.</rdfs:comment>
        <rdfs:label>Chains</rdfs:label>
    </owl:ObjectProperty>
    


    <!-- http://cwe.mitre.org/cwe#commonConsequences -->

    <owl:ObjectProperty rdf:about="http://cwe.mitre.org/cwe#commonConsequences">
        <rdfs:domain rdf:resource="http://cwe.mitre.org/cwe#Category"/>
        <rdfs:domain rdf:resource="http://cwe.mitre.org/cwe#CompoundElement"/>
        <rdfs:domain rdf:resource="http://cwe.mitre.org/cwe#Weakness"/>
        <rdfs:range rdf:resource="http://cwe.mitre.org/cwe#Consequence"/>
        <rdfs:comment>Defines zero or more  the common consequences associated with this weakness.  This should be included and completed as much as possible for all weaknesses.</rdfs:comment>
        <rdfs:label>Common Consequences</rdfs:label>
    </owl:ObjectProperty>
    


    <!-- http://cwe.mitre.org/cwe#compoundElements -->

    <owl:ObjectProperty rdf:about="http://cwe.mitre.org/cwe#compoundElements">
        <rdfs:domain rdf:resource="http://cwe.mitre.org/cwe#WeaknessCatalog"/>
        <rdfs:range rdf:resource="http://cwe.mitre.org/cwe#CompoundElement"/>
        <rdfs:comment>Defines  zero or more Compound_Element elements. 
Each Compound_Element represents a meaningful 	aggregation of several weaknesses, as in a chain like CWE-690: CWE-252 Unchecked Return Value can result in CWE-476 NULL Pointer Dereference or as in a composite like CWE-352 Cross-Site Request Forgery.</rdfs:comment>
        <rdfs:label>CompoundElements</rdfs:label>
    </owl:ObjectProperty>
    


    <!-- http://cwe.mitre.org/cwe#consequenceNote -->

    <owl:ObjectProperty rdf:about="http://cwe.mitre.org/cwe#consequenceNote">
        <rdfs:domain rdf:resource="http://cwe.mitre.org/cwe#Consequence"/>
        <rdfs:range rdf:resource="http://cwe.mitre.org/cwe#Note"/>
        <rdfs:comment>Defines additional commentary about this consequence.</rdfs:comment>
        <rdfs:label>Consequence Note</rdfs:label>
    </owl:ObjectProperty>
    


    <!-- http://cwe.mitre.org/cwe#consequenceTechnicalImpact -->

    <owl:ObjectProperty rdf:about="http://cwe.mitre.org/cwe#consequenceTechnicalImpact">
        <rdfs:domain rdf:resource="http://cwe.mitre.org/cwe#Consequence"/>
        <rdfs:range rdf:resource="http://cwe.mitre.org/cwe#TechnicalImpact"/>
        <rdfs:comment>Defines the technical impacts that can arise if an attacker attempts to exploit this weakness.</rdfs:comment>
        <rdfs:label>Technical Impact</rdfs:label>
    </owl:ObjectProperty>
    


    <!-- http://cwe.mitre.org/cwe#contentHistory -->

    <owl:ObjectProperty rdf:about="http://cwe.mitre.org/cwe#contentHistory">
        <rdfs:domain rdf:resource="http://cwe.mitre.org/cwe#Category"/>
        <rdfs:domain rdf:resource="http://cwe.mitre.org/cwe#CompoundElement"/>
        <rdfs:domain rdf:resource="http://cwe.mitre.org/cwe#View"/>
        <rdfs:domain rdf:resource="http://cwe.mitre.org/cwe#Weakness"/>
        <rdfs:range rdf:resource="http://cwe.mitre.org/cwe#HistoryRecord"/>
        <rdfs:comment>Defines zero or more Content History elements used to keep track of the author of the weakness entry and anyone who has made modifications to the content.</rdfs:comment>
        <rdfs:label>Content History</rdfs:label>
    </owl:ObjectProperty>
    


    <!-- http://cwe.mitre.org/cwe#demoExampleRefs -->

    <owl:ObjectProperty rdf:about="http://cwe.mitre.org/cwe#demoExampleRefs">
        <rdfs:domain rdf:resource="http://cwe.mitre.org/cwe#DemonstrativeExample"/>
        <rdfs:range rdf:resource="http://cwe.mitre.org/cwe#Reference"/>
        <rdfs:comment>Defines one or more References, each of which provide further reading and insight into this demonstrative example. This should be filled out when appropriate.</rdfs:comment>
        <rdfs:label>References</rdfs:label>
    </owl:ObjectProperty>
    


    <!-- http://cwe.mitre.org/cwe#demonstrativeExamples -->

    <owl:ObjectProperty rdf:about="http://cwe.mitre.org/cwe#demonstrativeExamples">
        <rdfs:domain rdf:resource="http://cwe.mitre.org/cwe#Category"/>
        <rdfs:domain rdf:resource="http://cwe.mitre.org/cwe#CompoundElement"/>
        <rdfs:domain rdf:resource="http://cwe.mitre.org/cwe#Weakness"/>
        <rdfs:range rdf:resource="http://cwe.mitre.org/cwe#DemonstrativeExample"/>
        <rdfs:comment>Defines one or more Demonstrative Examples, each of which should contain an example illustrating the problem being described in this weakness.</rdfs:comment>
        <rdfs:label>Demonstrative Examples</rdfs:label>
    </owl:ObjectProperty>
    


    <!-- http://cwe.mitre.org/cwe#detectionMethods -->

    <owl:ObjectProperty rdf:about="http://cwe.mitre.org/cwe#detectionMethods">
        <rdfs:domain rdf:resource="http://cwe.mitre.org/cwe#Category"/>
        <rdfs:domain rdf:resource="http://cwe.mitre.org/cwe#CompoundElement"/>
        <rdfs:domain rdf:resource="http://cwe.mitre.org/cwe#Weakness"/>
        <rdfs:range rdf:resource="http://cwe.mitre.org/cwe#DetectionMethod"/>
        <rdfs:comment>Defines a one or more 	Detection Method which identify methods that may be employed to detect this weakness.</rdfs:comment>
        <rdfs:label>Detection Methods</rdfs:label>
    </owl:ObjectProperty>
    


    <!-- http://cwe.mitre.org/cwe#enablingExploitationFactors -->

    <owl:ObjectProperty rdf:about="http://cwe.mitre.org/cwe#enablingExploitationFactors">
        <rdfs:domain rdf:resource="http://cwe.mitre.org/cwe#Category"/>
        <rdfs:domain rdf:resource="http://cwe.mitre.org/cwe#CompoundElement"/>
        <rdfs:domain rdf:resource="http://cwe.mitre.org/cwe#Weakness"/>
        <rdfs:range rdf:resource="http://cwe.mitre.org/cwe#ExploitationFactor"/>
        <rdfs:comment>Defines one or more Enabling Factor for Exploitation, each of which points out conditions or factors that could increase the likelihood of exploit for this weakness. This should be filled out for most weakness bases.</rdfs:comment>
        <rdfs:label>Enableing Factors for Exploitation</rdfs:label>
    </owl:ObjectProperty>
    


    <!-- http://cwe.mitre.org/cwe#extendedDescription -->

    <owl:ObjectProperty rdf:about="http://cwe.mitre.org/cwe#extendedDescription">
        <rdfs:domain rdf:resource="http://cwe.mitre.org/cwe#Category"/>
        <rdfs:domain rdf:resource="http://cwe.mitre.org/cwe#CompoundElement"/>
        <rdfs:domain rdf:resource="http://cwe.mitre.org/cwe#Weakness"/>
        <rdfs:range rdf:resource="http://cwe.mitre.org/cwe#StructuredText"/>
        <rdfs:comment>Specifies a place for details important to the description of this entry  to be included that are not necessary to convery the fundamental concept behind the entry.</rdfs:comment>
        <rdfs:label>Extended Description</rdfs:label>
    </owl:ObjectProperty>
    


    <!-- http://cwe.mitre.org/cwe#maintenanceNotes -->

    <owl:ObjectProperty rdf:about="http://cwe.mitre.org/cwe#maintenanceNotes">
        <rdfs:domain rdf:resource="http://cwe.mitre.org/cwe#Category"/>
        <rdfs:domain rdf:resource="http://cwe.mitre.org/cwe#CompoundElement"/>
        <rdfs:domain rdf:resource="http://cwe.mitre.org/cwe#View"/>
        <rdfs:domain rdf:resource="http://cwe.mitre.org/cwe#Weakness"/>
        <rdfs:range rdf:resource="http://cwe.mitre.org/cwe#Note"/>
        <rdfs:comment>Defines zero or more maintenance notes associated with the View.</rdfs:comment>
        <rdfs:label>Maintenance Notes</rdfs:label>
    </owl:ObjectProperty>
    


    <!-- http://cwe.mitre.org/cwe#methodEffectivenessNotes -->

    <owl:ObjectProperty rdf:about="http://cwe.mitre.org/cwe#methodEffectivenessNotes">
        <rdfs:domain rdf:resource="http://cwe.mitre.org/cwe#DetectionMethod"/>
        <rdfs:range rdf:resource="http://cwe.mitre.org/cwe#Note"/>
        <rdfs:comment>Defines a description of the strengths and shortcomings of this detection method. This should be filled out for some weakness classes and bases.</rdfs:comment>
        <rdfs:label>Method Effectiveness Notes</rdfs:label>
    </owl:ObjectProperty>
    


    <!-- http://cwe.mitre.org/cwe#mitigationEffectivenessNotes -->

    <owl:ObjectProperty rdf:about="http://cwe.mitre.org/cwe#mitigationEffectivenessNotes">
        <rdfs:domain rdf:resource="http://cwe.mitre.org/cwe#Mitigation"/>
        <rdfs:range rdf:resource="http://cwe.mitre.org/cwe#Note"/>
        <rdfs:comment>Defines the strengths and shortcomings of this mitigation on a specific weakness.</rdfs:comment>
        <rdfs:label>Mitigation Effectiveness Notes</rdfs:label>
    </owl:ObjectProperty>
    


    <!-- http://cwe.mitre.org/cwe#modesOfIntroduction -->

    <owl:ObjectProperty rdf:about="http://cwe.mitre.org/cwe#modesOfIntroduction">
        <rdfs:domain rdf:resource="http://cwe.mitre.org/cwe#Category"/>
        <rdfs:domain rdf:resource="http://cwe.mitre.org/cwe#CompoundElement"/>
        <rdfs:domain rdf:resource="http://cwe.mitre.org/cwe#Weakness"/>
        <rdfs:range rdf:resource="http://cwe.mitre.org/cwe#IntroductionMode"/>
        <rdfs:comment>Defines the typical scenarios under which this weakness can be introduced into the software. It should be filled out as needed.</rdfs:comment>
        <rdfs:label>Modes of Introduction</rdfs:label>
    </owl:ObjectProperty>
    


    <!-- http://cwe.mitre.org/cwe#nonPrimaryViews -->

    <owl:ObjectProperty rdf:about="http://cwe.mitre.org/cwe#nonPrimaryViews">
        <rdfs:domain rdf:resource="http://cwe.mitre.org/cwe#RelationshipStatement"/>
        <rdfs:range rdf:resource="http://cwe.mitre.org/cwe#View"/>
        <rdfs:comment>Specifies the list of non-ChildOf Views to which this relationship pertains.</rdfs:comment>
        <rdfs:label>Relationship Views</rdfs:label>
    </owl:ObjectProperty>
    


    <!-- http://cwe.mitre.org/cwe#objective -->

    <owl:ObjectProperty rdf:about="http://cwe.mitre.org/cwe#objective">
        <rdfs:domain rdf:resource="http://cwe.mitre.org/cwe#View"/>
        <rdfs:range rdf:resource="http://cwe.mitre.org/cwe#ViewObjective"/>
        <rdfs:comment>Defines a description the perspective from which this View is constructed.</rdfs:comment>
        <rdfs:label>Objective</rdfs:label>
    </owl:ObjectProperty>
    


    <!-- http://cwe.mitre.org/cwe#observedExamples -->

    <owl:ObjectProperty rdf:about="http://cwe.mitre.org/cwe#observedExamples">
        <rdfs:domain rdf:resource="http://cwe.mitre.org/cwe#Category"/>
        <rdfs:domain rdf:resource="http://cwe.mitre.org/cwe#CompoundElement"/>
        <rdfs:domain rdf:resource="http://cwe.mitre.org/cwe#Weakness"/>
        <rdfs:range rdf:resource="http://cwe.mitre.org/cwe#ObservedExample"/>
        <rdfs:comment>Specifies one or more ObservedExample elements, each of which is a reference to a specific observed instance of this weakness in the real world; typically this will be a CVE reference.</rdfs:comment>
        <rdfs:label>Observed Examples</rdfs:label>
    </owl:ObjectProperty>
    


    <!-- http://cwe.mitre.org/cwe#otherNotes -->

    <owl:ObjectProperty rdf:about="http://cwe.mitre.org/cwe#otherNotes">
        <rdfs:domain rdf:resource="http://cwe.mitre.org/cwe#Category"/>
        <rdfs:domain rdf:resource="http://cwe.mitre.org/cwe#CompoundElement"/>
        <rdfs:domain rdf:resource="http://cwe.mitre.org/cwe#View"/>
        <rdfs:domain rdf:resource="http://cwe.mitre.org/cwe#Weakness"/>
        <rdfs:range rdf:resource="http://cwe.mitre.org/cwe#Note"/>
        <rdfs:comment>Defines zero or ore other notes assoicated with the View.</rdfs:comment>
        <rdfs:label>Other Notes</rdfs:label>
    </owl:ObjectProperty>
    


    <!-- http://cwe.mitre.org/cwe#potentialMitigations -->

    <owl:ObjectProperty rdf:about="http://cwe.mitre.org/cwe#potentialMitigations">
        <rdfs:domain rdf:resource="http://cwe.mitre.org/cwe#Category"/>
        <rdfs:domain rdf:resource="http://cwe.mitre.org/cwe#CompoundElement"/>
        <rdfs:domain rdf:resource="http://cwe.mitre.org/cwe#Weakness"/>
        <rdfs:range rdf:resource="http://cwe.mitre.org/cwe#Mitigation"/>
        <rdfs:comment>Defines the potential mitigations associated with this weakness. It contains one or more mitigation subelements which each represent individual mitigations for this weakness. This should be included and completed to the extent possible for all weakness bases and variants.</rdfs:comment>
        <rdfs:label>Potential Mitigations</rdfs:label>
    </owl:ObjectProperty>
    


    <!-- http://cwe.mitre.org/cwe#primaryViews -->

    <owl:ObjectProperty rdf:about="http://cwe.mitre.org/cwe#primaryViews">
        <rdfs:domain rdf:resource="http://cwe.mitre.org/cwe#RelationshipStatement"/>
        <rdfs:range rdf:resource="http://cwe.mitre.org/cwe#View"/>
        <rdfs:comment>Specifies the list of Views to which this relationship pertains, where the relationship represents the primary ChildOf relationship for this weakness entry.</rdfs:comment>
        <rdfs:label>Primary Parent/Child Views</rdfs:label>
    </owl:ObjectProperty>
    


    <!-- http://cwe.mitre.org/cwe#referenceAuthor -->

    <owl:ObjectProperty rdf:about="http://cwe.mitre.org/cwe#referenceAuthor">
        <rdfs:domain rdf:resource="http://cwe.mitre.org/cwe#Reference"/>
        <rdfs:range>
            <owl:Class>
                <owl:unionOf rdf:parseType="Collection">
                    <rdf:Description rdf:about="http://www.oasis-open.org/ciq_xpil#Organization"/>
                    <rdf:Description rdf:about="http://www.oasis-open.org/ciq_xpil#Party"/>
                    <rdf:Description rdf:about="http://www.oasis-open.org/ciq_xpil#Person"/>
                </owl:unionOf>
            </owl:Class>
        </rdfs:range>
        <rdfs:comment>Specifies a reference to one or more individuals or organizations that authored the material</rdfs:comment>
        <rdfs:label>Reference Author</rdfs:label>
    </owl:ObjectProperty>
    


    <!-- http://cwe.mitre.org/cwe#referencePublisher -->

    <owl:ObjectProperty rdf:about="http://cwe.mitre.org/cwe#referencePublisher">
        <rdfs:domain rdf:resource="http://cwe.mitre.org/cwe#Reference"/>
        <rdfs:range rdf:resource="http://www.oasis-open.org/ciq_xpil#Organization"/>
        <rdfs:comment>Specifies the publisher of the reference material, if one exists</rdfs:comment>
        <rdfs:label>Reference Publisher</rdfs:label>
    </owl:ObjectProperty>
    


    <!-- http://cwe.mitre.org/cwe#references -->

    <owl:ObjectProperty rdf:about="http://cwe.mitre.org/cwe#references">
        <rdfs:domain rdf:resource="http://cwe.mitre.org/cwe#Category"/>
        <rdfs:domain rdf:resource="http://cwe.mitre.org/cwe#CompoundElement"/>
        <rdfs:domain rdf:resource="http://cwe.mitre.org/cwe#Mitigation"/>
        <rdfs:domain rdf:resource="http://cwe.mitre.org/cwe#View"/>
        <rdfs:domain rdf:resource="http://cwe.mitre.org/cwe#Weakness"/>
        <rdfs:range rdf:resource="http://cwe.mitre.org/cwe#Reference"/>
        <rdfs:comment>Defines zero or more sources from which more information and deeper insight can be obtained, such as a 	research paper or an excerpt from a publication</rdfs:comment>
        <rdfs:label>References</rdfs:label>
    </owl:ObjectProperty>
    


    <!-- http://cwe.mitre.org/cwe#relatedAttackPatterns -->

    <owl:ObjectProperty rdf:about="http://cwe.mitre.org/cwe#relatedAttackPatterns">
        <rdfs:domain rdf:resource="http://cwe.mitre.org/cwe#Category"/>
        <rdfs:domain rdf:resource="http://cwe.mitre.org/cwe#CompoundElement"/>
        <rdfs:domain rdf:resource="http://cwe.mitre.org/cwe#Weakness"/>
        <rdfs:range rdf:resource="http://capec.mitre.org/capec#AttackPattern"/>
        <rdfs:comment>Specifies one or more references to CAPEC entries which will identify related attack patterns to this weakness. This should be filled out to the extent possible for most weaknesses.</rdfs:comment>
        <rdfs:label>Related Attack Patterns</rdfs:label>
    </owl:ObjectProperty>
    


    <!-- http://cwe.mitre.org/cwe#relationshipNotes -->

    <owl:ObjectProperty rdf:about="http://cwe.mitre.org/cwe#relationshipNotes">
        <rdfs:domain rdf:resource="http://cwe.mitre.org/cwe#Category"/>
        <rdfs:domain rdf:resource="http://cwe.mitre.org/cwe#CompoundElement"/>
        <rdfs:domain rdf:resource="http://cwe.mitre.org/cwe#View"/>
        <rdfs:domain rdf:resource="http://cwe.mitre.org/cwe#Weakness"/>
        <rdfs:range rdf:resource="http://cwe.mitre.org/cwe#Note"/>
        <rdfs:comment>Defines zero or more relationship notes associated with the View</rdfs:comment>
        <rdfs:label>Relationship Notes</rdfs:label>
    </owl:ObjectProperty>
    


    <!-- http://cwe.mitre.org/cwe#relationships -->

    <owl:ObjectProperty rdf:about="http://cwe.mitre.org/cwe#relationships">
        <rdfs:domain rdf:resource="http://cwe.mitre.org/cwe#Category"/>
        <rdfs:domain rdf:resource="http://cwe.mitre.org/cwe#CompoundElement"/>
        <rdfs:domain rdf:resource="http://cwe.mitre.org/cwe#View"/>
        <rdfs:domain rdf:resource="http://cwe.mitre.org/cwe#Weakness"/>
        <rdfs:range rdf:resource="http://cwe.mitre.org/cwe#Category"/>
        <rdfs:range rdf:resource="http://cwe.mitre.org/cwe#CompoundElement"/>
        <rdfs:range rdf:resource="http://cwe.mitre.org/cwe#View"/>
        <rdfs:range rdf:resource="http://cwe.mitre.org/cwe#Weakness"/>
        <rdfs:comment>Specifies one or more associations between this structure, whether it is a Weakness, Category, or Compound_Element and another structure.</rdfs:comment>
        <rdfs:label>Relationships</rdfs:label>
    </owl:ObjectProperty>
    


    <!-- http://cwe.mitre.org/cwe#researchGaps -->

    <owl:ObjectProperty rdf:about="http://cwe.mitre.org/cwe#researchGaps">
        <rdfs:domain rdf:resource="http://cwe.mitre.org/cwe#Category"/>
        <rdfs:domain rdf:resource="http://cwe.mitre.org/cwe#CompoundElement"/>
        <rdfs:domain rdf:resource="http://cwe.mitre.org/cwe#View"/>
        <rdfs:domain rdf:resource="http://cwe.mitre.org/cwe#Weakness"/>
        <rdfs:range rdf:resource="http://cwe.mitre.org/cwe#ResearchGap"/>
        <rdfs:comment>Defines zero or more gaps in the research associated with this Weakness, Category, View, or Compound Element</rdfs:comment>
        <rdfs:label>Research Gaps</rdfs:label>
    </owl:ObjectProperty>
    


    <!-- http://cwe.mitre.org/cwe#subMitigations -->

    <owl:ObjectProperty rdf:about="http://cwe.mitre.org/cwe#subMitigations">
        <rdfs:domain rdf:resource="http://cwe.mitre.org/cwe#Mitigation"/>
        <rdfs:range rdf:resource="http://cwe.mitre.org/cwe#Mitigation"/>
        <rdfs:comment>Defines one or more sub-mitigations</rdfs:comment>
        <rdfs:label>Submitigations</rdfs:label>
    </owl:ObjectProperty>
    


    <!-- http://cwe.mitre.org/cwe#taxonomyMappings -->

    <owl:ObjectProperty rdf:about="http://cwe.mitre.org/cwe#taxonomyMappings">
        <rdfs:domain rdf:resource="http://cwe.mitre.org/cwe#Category"/>
        <rdfs:domain rdf:resource="http://cwe.mitre.org/cwe#CompoundElement"/>
        <rdfs:domain rdf:resource="http://cwe.mitre.org/cwe#Weakness"/>
        <rdfs:range rdf:resource="http://cwe.mitre.org/cwe#TaxonomyMapping"/>
        <rdfs:comment>Defines one or more Taxonomy Mappings which provide a mapping from this entry to an entry in a different taxonomy.</rdfs:comment>
        <rdfs:label>Taxonomy Mappings</rdfs:label>
    </owl:ObjectProperty>
    


    <!-- http://cwe.mitre.org/cwe#terminologyNotes -->

    <owl:ObjectProperty rdf:about="http://cwe.mitre.org/cwe#terminologyNotes">
        <rdfs:domain rdf:resource="http://cwe.mitre.org/cwe#Category"/>
        <rdfs:domain rdf:resource="http://cwe.mitre.org/cwe#CompoundElement"/>
        <rdfs:domain rdf:resource="http://cwe.mitre.org/cwe#Weakness"/>
        <rdfs:range rdf:resource="http://cwe.mitre.org/cwe#Note"/>
        <rdfs:comment>Specifies zero or more notes that contain a discussion of terminology issues related to this weakness.   It is different from Alternate Terms, which is focused on discussion of specific terms that are commonly used. It should be filled out in any entry for which there is no established terminology, or if there are multiple uses of the same key term.</rdfs:comment>
        <rdfs:label>Terminology Notes</rdfs:label>
    </owl:ObjectProperty>
    


    <!-- http://cwe.mitre.org/cwe#theoreticalNotes -->

    <owl:ObjectProperty rdf:about="http://cwe.mitre.org/cwe#theoreticalNotes">
        <rdfs:domain rdf:resource="http://cwe.mitre.org/cwe#Category"/>
        <rdfs:domain rdf:resource="http://cwe.mitre.org/cwe#CompoundElement"/>
        <rdfs:domain rdf:resource="http://cwe.mitre.org/cwe#Weakness"/>
        <rdfs:range rdf:resource="http://cwe.mitre.org/cwe#Note"/>
        <rdfs:comment>Specifies one or more Theoretical Notes that each describe the weakness using vulnerability theory concepts. It should be filled out as needed, especially in cases where the application of 	vulnerability theory is not necessarily obvious for the weakness.</rdfs:comment>
        <rdfs:label>Theoretical Notes</rdfs:label>
    </owl:ObjectProperty>
    


    <!-- http://cwe.mitre.org/cwe#views -->

    <owl:ObjectProperty rdf:about="http://cwe.mitre.org/cwe#views">
        <rdfs:domain rdf:resource="http://cwe.mitre.org/cwe#WeaknessCatalog"/>
        <rdfs:range rdf:resource="http://cwe.mitre.org/cwe#View"/>
        <rdfs:comment>Defines  zero or more View elements.  Each View element represents a perspective with which one might look at the weaknesses in CWE. CWE-699 Development View and CWE-1000 Research View are two examples of Views.</rdfs:comment>
        <rdfs:label>Views</rdfs:label>
    </owl:ObjectProperty>
    


    <!-- http://cwe.mitre.org/cwe#vulnerabilityReference -->

    <owl:ObjectProperty rdf:about="http://cwe.mitre.org/cwe#vulnerabilityReference">
        <rdfs:domain rdf:resource="http://cwe.mitre.org/cwe#ObservedExample"/>
        <rdfs:range rdf:resource="http://nvd.nist.gov/cve#Vulnerability"/>
        <rdfs:comment>Specifies a reference to a vulnerability entity, typically as a Common Vulnerabilty Enumeration (CVE) entry</rdfs:comment>
        <rdfs:label>Vulnerability Reference</rdfs:label>
    </owl:ObjectProperty>
    


    <!-- http://cwe.mitre.org/cwe#weaknessOrdinality -->

    <owl:ObjectProperty rdf:about="http://cwe.mitre.org/cwe#weaknessOrdinality">
        <rdfs:domain rdf:resource="http://cwe.mitre.org/cwe#Category"/>
        <rdfs:domain rdf:resource="http://cwe.mitre.org/cwe#CompoundElement"/>
        <rdfs:domain rdf:resource="http://cwe.mitre.org/cwe#Weakness"/>
        <rdfs:range rdf:resource="http://cwe.mitre.org/cwe#WeaknessOrdinality"/>
        <rdfs:comment>Specifies when this entry is primary - where the weakness exists independent of other weaknesses, or when this entry might be resultant - where the weakness is typically related to the presence of some other weaknesses. This should be filled out for all Weakness Base and 	Variant entries.</rdfs:comment>
        <rdfs:label>Weakness Ordinality</rdfs:label>
    </owl:ObjectProperty>
    


    <!-- http://cwe.mitre.org/cwe#weaknesses -->

    <owl:ObjectProperty rdf:about="http://cwe.mitre.org/cwe#weaknesses">
        <rdfs:domain rdf:resource="http://cwe.mitre.org/cwe#WeaknessCatalog"/>
        <rdfs:range rdf:resource="http://cwe.mitre.org/cwe#Weakness"/>
        <rdfs:comment>Defines zero or more Weakness entities that represents an actual weakness entry in CWE, such as CWE-311 Failure to Encrypt Sensitive Data or CWE-326 Weak Encryption.</rdfs:comment>
        <rdfs:label>Weakness</rdfs:label>
    </owl:ObjectProperty>
    


    <!-- http://cwe.mitre.org/cwe#whiteBoxDefinitions -->

    <owl:ObjectProperty rdf:about="http://cwe.mitre.org/cwe#whiteBoxDefinitions">
        <rdfs:domain rdf:resource="http://cwe.mitre.org/cwe#Category"/>
        <rdfs:domain rdf:resource="http://cwe.mitre.org/cwe#CompoundElement"/>
        <rdfs:domain rdf:resource="http://cwe.mitre.org/cwe#Weakness"/>
        <rdfs:range rdf:resource="http://cwe.mitre.org/cwe#WhiteBoxDefinition"/>
        <rdfs:comment>Defines one or more White Box Definitions, each of which describes the weakness from a white box perspective, meaning that the view includes the knowledge of control flow, data flow, and all other inner workings of the software in which the weakness exists.</rdfs:comment>
        <rdfs:label>White Box Definitions</rdfs:label>
    </owl:ObjectProperty>
    


    <!-- 
    ///////////////////////////////////////////////////////////////////////////////////////
    //
    // Data properties
    //
    ///////////////////////////////////////////////////////////////////////////////////////
     -->

    


    <!-- http://cwe.mitre.org/cwe#abstraction -->

    <owl:DatatypeProperty rdf:about="http://cwe.mitre.org/cwe#abstraction">
        <rdfs:domain rdf:resource="http://cwe.mitre.org/cwe#CompoundElement"/>
        <rdfs:domain rdf:resource="http://cwe.mitre.org/cwe#Weakness"/>
        <rdfs:range>
            <rdfs:Datatype>
                <owl:oneOf>
                    <rdf:Description>
                        <rdf:type rdf:resource="http://www.w3.org/1999/02/22-rdf-syntax-ns#List"/>
                        <rdf:first rdf:datatype="http://www.w3.org/2001/XMLSchema#string">Base</rdf:first>
                        <rdf:rest>
                            <rdf:Description>
                                <rdf:type rdf:resource="http://www.w3.org/1999/02/22-rdf-syntax-ns#List"/>
                                <rdf:first rdf:datatype="http://www.w3.org/2001/XMLSchema#string">Class</rdf:first>
                                <rdf:rest>
                                    <rdf:Description>
                                        <rdf:type rdf:resource="http://www.w3.org/1999/02/22-rdf-syntax-ns#List"/>
                                        <rdf:first rdf:datatype="http://www.w3.org/2001/XMLSchema#string">Variant</rdf:first>
                                        <rdf:rest rdf:resource="http://www.w3.org/1999/02/22-rdf-syntax-ns#nil"/>
                                    </rdf:Description>
                                </rdf:rest>
                            </rdf:Description>
                        </rdf:rest>
                    </rdf:Description>
                </owl:oneOf>
            </rdfs:Datatype>
        </rdfs:range>
        <rdfs:comment>Specifies the abstraction level for this weakness.  The abstractions levels for Compound Elements and Weaknesses are the same. For example, if the Compound Element is a chain, and all elements of the chain are Class level, then the Compound Element Abstraction attribute is Class. 

Acceptable values are &quot;Class&quot;, which is the most abstract type of Weakness such as CWE-362 Race Conditions, &quot;Base&quot; which is a more specific type of weakness that is still mostly independent of a specific resource or technology such as CWE-567 Unsynchronized Access to 	Shared Data, and &quot;Variant&quot; which is a weakness specific to a particular resource, technology or context.</rdfs:comment>
        <rdfs:label>Abstraction</rdfs:label>
    </owl:DatatypeProperty>
    


    <!-- http://cwe.mitre.org/cwe#affectedResources -->

    <owl:DatatypeProperty rdf:about="http://cwe.mitre.org/cwe#affectedResources">
        <rdfs:domain rdf:resource="http://cwe.mitre.org/cwe#Category"/>
        <rdfs:domain rdf:resource="http://cwe.mitre.org/cwe#CompoundElement"/>
        <rdfs:domain rdf:resource="http://cwe.mitre.org/cwe#Weakness"/>
        <rdfs:range>
            <rdfs:Datatype>
                <owl:oneOf>
                    <rdf:Description>
                        <rdf:type rdf:resource="http://www.w3.org/1999/02/22-rdf-syntax-ns#List"/>
                        <rdf:first rdf:datatype="http://www.w3.org/2001/XMLSchema#string">CPU</rdf:first>
                        <rdf:rest>
                            <rdf:Description>
                                <rdf:type rdf:resource="http://www.w3.org/1999/02/22-rdf-syntax-ns#List"/>
                                <rdf:first rdf:datatype="http://www.w3.org/2001/XMLSchema#string">File/Directory</rdf:first>
                                <rdf:rest>
                                    <rdf:Description>
                                        <rdf:type rdf:resource="http://www.w3.org/1999/02/22-rdf-syntax-ns#List"/>
                                        <rdf:first rdf:datatype="http://www.w3.org/2001/XMLSchema#string">Memory</rdf:first>
                                        <rdf:rest>
                                            <rdf:Description>
                                                <rdf:type rdf:resource="http://www.w3.org/1999/02/22-rdf-syntax-ns#List"/>
                                                <rdf:first rdf:datatype="http://www.w3.org/2001/XMLSchema#string">System Process</rdf:first>
                                                <rdf:rest rdf:resource="http://www.w3.org/1999/02/22-rdf-syntax-ns#nil"/>
                                            </rdf:Description>
                                        </rdf:rest>
                                    </rdf:Description>
                                </rdf:rest>
                            </rdf:Description>
                        </rdf:rest>
                    </rdf:Description>
                </owl:oneOf>
            </rdfs:Datatype>
        </rdfs:range>
        <rdfs:comment>Defines one or more system resources affected by this 	entry.</rdfs:comment>
        <rdfs:label>Affected Resources</rdfs:label>
    </owl:DatatypeProperty>
    


    <!-- http://cwe.mitre.org/cwe#authorName -->

    <owl:DatatypeProperty rdf:about="http://cwe.mitre.org/cwe#authorName">
        <rdfs:domain rdf:resource="http://cwe.mitre.org/cwe#HistoryRecord"/>
        <rdfs:range rdf:resource="http://www.w3.org/2001/XMLSchema#string"/>
        <rdfs:comment>Specifies the names of one or more individuals that authored the submitted, contributed, or modified the Weakness, View, Category, or CompoundElement.</rdfs:comment>
        <rdfs:label>Author Name</rdfs:label>
    </owl:DatatypeProperty>
    


    <!-- http://cwe.mitre.org/cwe#authorOrganizationName -->

    <owl:DatatypeProperty rdf:about="http://cwe.mitre.org/cwe#authorOrganizationName">
        <rdfs:domain rdf:resource="http://cwe.mitre.org/cwe#HistoryRecord"/>
        <rdfs:range rdf:resource="http://www.w3.org/2001/XMLSchema#string"/>
        <rdfs:comment>Specifies the name of the organization which submitted, contributed, or modified the Weakness, View, Category, or CompoundElement</rdfs:comment>
        <rdfs:label>Author Organization Name</rdfs:label>
    </owl:DatatypeProperty>
    


    <!-- http://cwe.mitre.org/cwe#blockNature -->

    <owl:DatatypeProperty rdf:about="http://cwe.mitre.org/cwe#blockNature">
        <rdfs:domain rdf:resource="http://cwe.mitre.org/cwe#Block"/>
        <rdfs:range>
            <rdfs:Datatype>
                <owl:oneOf>
                    <rdf:Description>
                        <rdf:type rdf:resource="http://www.w3.org/1999/02/22-rdf-syntax-ns#List"/>
                        <rdf:first rdf:datatype="http://www.w3.org/2001/XMLSchema#string">Attack</rdf:first>
                        <rdf:rest>
                            <rdf:Description>
                                <rdf:type rdf:resource="http://www.w3.org/1999/02/22-rdf-syntax-ns#List"/>
                                <rdf:first rdf:datatype="http://www.w3.org/2001/XMLSchema#string">Bad_Code</rdf:first>
                                <rdf:rest>
                                    <rdf:Description>
                                        <rdf:type rdf:resource="http://www.w3.org/1999/02/22-rdf-syntax-ns#List"/>
                                        <rdf:first rdf:datatype="http://www.w3.org/2001/XMLSchema#string">Good_Code</rdf:first>
                                        <rdf:rest>
                                            <rdf:Description>
                                                <rdf:type rdf:resource="http://www.w3.org/1999/02/22-rdf-syntax-ns#List"/>
                                                <rdf:first rdf:datatype="http://www.w3.org/2001/XMLSchema#string">List</rdf:first>
                                                <rdf:rest>
                                                    <rdf:Description>
                                                        <rdf:type rdf:resource="http://www.w3.org/1999/02/22-rdf-syntax-ns#List"/>
                                                        <rdf:first rdf:datatype="http://www.w3.org/2001/XMLSchema#string">Mitigation_Code</rdf:first>
                                                        <rdf:rest>
                                                            <rdf:Description>
                                                                <rdf:type rdf:resource="http://www.w3.org/1999/02/22-rdf-syntax-ns#List"/>
                                                                <rdf:first rdf:datatype="http://www.w3.org/2001/XMLSchema#string">Numeric_List</rdf:first>
                                                                <rdf:rest>
                                                                    <rdf:Description>
                                                                        <rdf:type rdf:resource="http://www.w3.org/1999/02/22-rdf-syntax-ns#List"/>
                                                                        <rdf:first rdf:datatype="http://www.w3.org/2001/XMLSchema#string">Result</rdf:first>
                                                                        <rdf:rest rdf:resource="http://www.w3.org/1999/02/22-rdf-syntax-ns#nil"/>
                                                                    </rdf:Description>
                                                                </rdf:rest>
                                                            </rdf:Description>
                                                        </rdf:rest>
                                                    </rdf:Description>
                                                </rdf:rest>
                                            </rdf:Description>
                                        </rdf:rest>
                                    </rdf:Description>
                                </rdf:rest>
                            </rdf:Description>
                        </rdf:rest>
                    </rdf:Description>
                </owl:oneOf>
            </rdfs:Datatype>
        </rdfs:range>
        <rdfs:comment>Defines the nature of the content contained within the Block.</rdfs:comment>
        <rdfs:label>Block Nature</rdfs:label>
    </owl:DatatypeProperty>
    


    <!-- http://cwe.mitre.org/cwe#casualNature -->

    <owl:DatatypeProperty rdf:about="http://cwe.mitre.org/cwe#casualNature">
        <rdfs:domain rdf:resource="http://cwe.mitre.org/cwe#Weakness"/>
        <rdfs:range>
            <rdfs:Datatype>
                <owl:oneOf>
                    <rdf:Description>
                        <rdf:type rdf:resource="http://www.w3.org/1999/02/22-rdf-syntax-ns#List"/>
                        <rdf:first rdf:datatype="http://www.w3.org/2001/XMLSchema#string">Explicit</rdf:first>
                        <rdf:rest>
                            <rdf:Description>
                                <rdf:type rdf:resource="http://www.w3.org/1999/02/22-rdf-syntax-ns#List"/>
                                <rdf:first rdf:datatype="http://www.w3.org/2001/XMLSchema#string">Implicit</rdf:first>
                                <rdf:rest rdf:resource="http://www.w3.org/1999/02/22-rdf-syntax-ns#nil"/>
                            </rdf:Description>
                        </rdf:rest>
                    </rdf:Description>
                </owl:oneOf>
            </rdfs:Datatype>
        </rdfs:range>
        <rdfs:comment>Specifies the nature of the underlying cause of the weakness. Is it an implicit underlying weakness or is it an issue of behavior on the part of the software developer? Appropriate values are 	either Implicit, occurring regardless of developer behavior, or Explicit, an explicit weakness resulting from behavior of the developer.</rdfs:comment>
        <rdfs:label>Casual Nature</rdfs:label>
    </owl:DatatypeProperty>
    


    <!-- http://cwe.mitre.org/cwe#categoryName -->

    <owl:DatatypeProperty rdf:about="http://cwe.mitre.org/cwe#categoryName">
        <rdfs:domain rdf:resource="http://cwe.mitre.org/cwe#Category"/>
        <rdfs:range rdf:resource="http://www.w3.org/2001/XMLSchema#string"/>
        <rdfs:comment>Specifies a descriptive name used to give the reader an idea of what the commonality is amongst the children of this category.  All words in the name should be capitalized except for articles and prepositions unless they begin or end the name.  Subsequent words in a hyphenated chain are also not capitalized.</rdfs:comment>
        <rdfs:label>Category Name</rdfs:label>
    </owl:DatatypeProperty>
    


    <!-- http://cwe.mitre.org/cwe#causalNature -->

    <owl:DatatypeProperty rdf:about="http://cwe.mitre.org/cwe#causalNature">
        <rdfs:domain rdf:resource="http://cwe.mitre.org/cwe#Category"/>
        <rdfs:domain rdf:resource="http://cwe.mitre.org/cwe#CompoundElement"/>
        <rdfs:domain rdf:resource="http://cwe.mitre.org/cwe#Weakness"/>
        <rdfs:range>
            <rdfs:Datatype>
                <owl:oneOf>
                    <rdf:Description>
                        <rdf:type rdf:resource="http://www.w3.org/1999/02/22-rdf-syntax-ns#List"/>
                        <rdf:first rdf:datatype="http://www.w3.org/2001/XMLSchema#string">Explicit</rdf:first>
                        <rdf:rest>
                            <rdf:Description>
                                <rdf:type rdf:resource="http://www.w3.org/1999/02/22-rdf-syntax-ns#List"/>
                                <rdf:first rdf:datatype="http://www.w3.org/2001/XMLSchema#string">Implicit</rdf:first>
                                <rdf:rest rdf:resource="http://www.w3.org/1999/02/22-rdf-syntax-ns#nil"/>
                            </rdf:Description>
                        </rdf:rest>
                    </rdf:Description>
                </owl:oneOf>
            </rdfs:Datatype>
        </rdfs:range>
        <rdfs:comment>Defines the nature of the underlying cause of the weakness. Is it an implicit underlying weakness or is it an issue of behavior on the part of the software developer? Appropriate values are either Implicit, occurring regardless of developer behavior, or Explicit, an explicit weakness resulting from behavior of the developer.</rdfs:comment>
        <rdfs:label>Nature of Cause</rdfs:label>
    </owl:DatatypeProperty>
    


    <!-- http://cwe.mitre.org/cwe#code -->

    <owl:DatatypeProperty rdf:about="http://cwe.mitre.org/cwe#code">
        <rdfs:domain rdf:resource="http://cwe.mitre.org/cwe#StructuredText"/>
        <rdfs:range rdf:resource="http://www.w3.org/2001/XMLSchema#string"/>
        <rdfs:comment>Defines a line of code.</rdfs:comment>
        <rdfs:label>Code</rdfs:label>
    </owl:DatatypeProperty>
    


    <!-- http://cwe.mitre.org/cwe#codeExampleLanguage -->

    <owl:DatatypeProperty rdf:about="http://cwe.mitre.org/cwe#codeExampleLanguage">
        <rdfs:domain rdf:resource="http://cwe.mitre.org/cwe#StructuredText"/>
        <rdfs:range rdf:resource="http://www.w3.org/2001/XMLSchema#string"/>
        <rdfs:comment>Specifies the programming language being used in the following block of Code</rdfs:comment>
        <rdfs:label>Code Language</rdfs:label>
    </owl:DatatypeProperty>
    


    <!-- http://cwe.mitre.org/cwe#comment -->

    <owl:DatatypeProperty rdf:about="http://cwe.mitre.org/cwe#comment">
        <rdfs:domain rdf:resource="http://cwe.mitre.org/cwe#StructuredText"/>
        <rdfs:range rdf:resource="http://www.w3.org/2001/XMLSchema#string"/>
        <rdfs:comment>Defines a comment in code</rdfs:comment>
        <rdfs:label>Comment</rdfs:label>
    </owl:DatatypeProperty>
    


    <!-- http://cwe.mitre.org/cwe#compoundElementName -->

    <owl:DatatypeProperty rdf:about="http://cwe.mitre.org/cwe#compoundElementName">
        <rdfs:domain rdf:resource="http://cwe.mitre.org/cwe#CompoundElement"/>
        <rdfs:range rdf:resource="http://www.w3.org/2001/XMLSchema#string"/>
        <rdfs:comment>Specifies a descriptive name used to give the reader an idea of the meaning behind the compound weakness structure. 

All words in the name should be capitalized except for articles and prepositions unless they begin or end the name. Subsequent words in a hyphenated chain are also not capitalized.</rdfs:comment>
        <rdfs:label>Compound Element Name</rdfs:label>
    </owl:DatatypeProperty>
    


    <!-- http://cwe.mitre.org/cwe#compoundElementStructure -->

    <owl:DatatypeProperty rdf:about="http://cwe.mitre.org/cwe#compoundElementStructure">
        <rdfs:domain rdf:resource="http://cwe.mitre.org/cwe#CompoundElement"/>
        <rdfs:range>
            <rdfs:Datatype>
                <owl:oneOf>
                    <rdf:Description>
                        <rdf:type rdf:resource="http://www.w3.org/1999/02/22-rdf-syntax-ns#List"/>
                        <rdf:first rdf:datatype="http://www.w3.org/2001/XMLSchema#string">Chain</rdf:first>
                        <rdf:rest>
                            <rdf:Description>
                                <rdf:type rdf:resource="http://www.w3.org/1999/02/22-rdf-syntax-ns#List"/>
                                <rdf:first rdf:datatype="http://www.w3.org/2001/XMLSchema#string">Composite</rdf:first>
                                <rdf:rest rdf:resource="http://www.w3.org/1999/02/22-rdf-syntax-ns#nil"/>
                            </rdf:Description>
                        </rdf:rest>
                    </rdf:Description>
                </owl:oneOf>
            </rdfs:Datatype>
        </rdfs:range>
        <rdfs:comment>Specifies the structural nature of this compound element - that is, composed of other weaknesses concurrently, as in a composite, or consecutively, as in a chain.</rdfs:comment>
        <rdfs:label>Compound Element Structure</rdfs:label>
    </owl:DatatypeProperty>
    


    <!-- http://cwe.mitre.org/cwe#consequenceId -->

    <owl:DatatypeProperty rdf:about="http://cwe.mitre.org/cwe#consequenceId">
        <rdfs:domain rdf:resource="http://cwe.mitre.org/cwe#Consequence"/>
        <rdfs:range rdf:resource="http://www.w3.org/2001/XMLSchema#string"/>
        <rdfs:comment>Specifies the value for the related Common Consequence entry identifier. However, Common Consequences across CWE with the same ID should only vary in small details.</rdfs:comment>
        <rdfs:label>Consequence Identifier</rdfs:label>
    </owl:DatatypeProperty>
    


    <!-- http://cwe.mitre.org/cwe#consequenceScope -->

    <owl:DatatypeProperty rdf:about="http://cwe.mitre.org/cwe#consequenceScope">
        <rdfs:domain rdf:resource="http://cwe.mitre.org/cwe#Consequence"/>
        <rdfs:range rdf:resource="http://www.w3.org/2001/XMLSchema#string"/>
        <rdfs:comment>Defines an individual consequence that may be associated with this weakness. Possible effects are detailed in 	Consequence Effect.</rdfs:comment>
        <rdfs:label>Consequence Scope</rdfs:label>
    </owl:DatatypeProperty>
    


    <!-- http://cwe.mitre.org/cwe#contributionMode -->

    <owl:DatatypeProperty rdf:about="http://cwe.mitre.org/cwe#contributionMode">
        <rdfs:domain rdf:resource="http://cwe.mitre.org/cwe#HistoryRecord"/>
        <rdfs:range>
            <rdfs:Datatype>
                <owl:oneOf>
                    <rdf:Description>
                        <rdf:type rdf:resource="http://www.w3.org/1999/02/22-rdf-syntax-ns#List"/>
                        <rdf:first rdf:datatype="http://www.w3.org/2001/XMLSchema#string">Content</rdf:first>
                        <rdf:rest>
                            <rdf:Description>
                                <rdf:type rdf:resource="http://www.w3.org/1999/02/22-rdf-syntax-ns#List"/>
                                <rdf:first rdf:datatype="http://www.w3.org/2001/XMLSchema#string">Feedback</rdf:first>
                                <rdf:rest rdf:resource="http://www.w3.org/1999/02/22-rdf-syntax-ns#nil"/>
                            </rdf:Description>
                        </rdf:rest>
                    </rdf:Description>
                </owl:oneOf>
            </rdfs:Datatype>
        </rdfs:range>
        <rdfs:comment>Defines whether the contribution was part of feedback given to the CWE team or actual content that was donated.</rdfs:comment>
        <rdfs:label>Contribution Mode</rdfs:label>
    </owl:DatatypeProperty>
    


    <!-- http://cwe.mitre.org/cwe#demoExampleId -->

    <owl:DatatypeProperty rdf:about="http://cwe.mitre.org/cwe#demoExampleId">
        <rdfs:domain rdf:resource="http://cwe.mitre.org/cwe#DemonstrativeExample"/>
        <rdfs:range rdf:resource="http://www.w3.org/2001/XMLSchema#string"/>
        <rdfs:comment>Defines  the identifier for the related Demonstrative Example. Only one Demonstrative Example ID can exist for each Demonstrative Example (ex: DX-1). However, Demonstrative Examples across CWE with the same ID should only vary in small details.</rdfs:comment>
        <rdfs:label>Demonstration Example Identifier</rdfs:label>
    </owl:DatatypeProperty>
    


    <!-- http://cwe.mitre.org/cwe#descriptionSummary -->

    <owl:DatatypeProperty rdf:about="http://cwe.mitre.org/cwe#descriptionSummary">
        <rdfs:domain rdf:resource="http://cwe.mitre.org/cwe#Category"/>
        <rdfs:domain rdf:resource="http://cwe.mitre.org/cwe#CompoundElement"/>
        <rdfs:domain rdf:resource="http://cwe.mitre.org/cwe#Weakness"/>
        <rdfs:range rdf:resource="http://www.w3.org/2001/XMLSchema#string"/>
        <rdfs:comment>Defines a minimalistic description which provides the information necessary to understand the primary focus of this entry.  The description text should be short and should limit itself to describing the key points that define this entry.  Further explanation can be included in the extended description element.</rdfs:comment>
        <rdfs:label>Description Summary</rdfs:label>
    </owl:DatatypeProperty>
    


    <!-- http://cwe.mitre.org/cwe#detectionMethodId -->

    <owl:DatatypeProperty rdf:about="http://cwe.mitre.org/cwe#detectionMethodId">
        <rdfs:domain rdf:resource="http://cwe.mitre.org/cwe#DetectionMethod"/>
        <rdfs:range rdf:resource="http://www.w3.org/2001/XMLSchema#string"/>
        <rdfs:comment>Defines an identifier for the related Detection Method. Only one Detection_Method_ID element can exist for each Detection Method element (ex: DM-1). However, Detection Methods across CWE with the same ID should only vary in small details.</rdfs:comment>
        <rdfs:label>Identifier</rdfs:label>
    </owl:DatatypeProperty>
    


    <!-- http://cwe.mitre.org/cwe#dictionaryLink -->

    <owl:DatatypeProperty rdf:about="http://cwe.mitre.org/cwe#dictionaryLink">
        <rdfs:domain rdf:resource="http://cwe.mitre.org/cwe#Weakness"/>
        <rdfs:range rdf:resource="http://www.w3.org/2001/XMLSchema#anyURI"/>
        <rdfs:comment>Specifies an external link to the weakness contained at the Common Weakness Enumeration (CWE) dictionary.  The link should be in the following form:  http://cwe.mitre.org/data/definitions/{weakness-id}.html, where {weakness-id) should be the integer Identifier of the specific weakness.</rdfs:comment>
        <rdfs:label>Dictionary Link</rdfs:label>
    </owl:DatatypeProperty>
    


    <!-- http://cwe.mitre.org/cwe#entryComment -->

    <owl:DatatypeProperty rdf:about="http://cwe.mitre.org/cwe#entryComment">
        <rdfs:domain rdf:resource="http://cwe.mitre.org/cwe#HistoryRecord"/>
        <rdfs:range rdf:resource="http://www.w3.org/2001/XMLSchema#string"/>
        <rdfs:comment>Defines any comments regarding the content of this weakness entry, such as assumptions made, reasons for omitting 	elements, contact information, pending questions, etc.</rdfs:comment>
        <rdfs:label>Comments</rdfs:label>
    </owl:DatatypeProperty>
    


    <!-- http://cwe.mitre.org/cwe#entryDate -->

    <owl:DatatypeProperty rdf:about="http://cwe.mitre.org/cwe#entryDate">
        <rdfs:domain rdf:resource="http://cwe.mitre.org/cwe#HistoryRecord"/>
        <rdfs:range rdf:resource="http://www.w3.org/2001/XMLSchema#date"/>
        <rdfs:comment>Defines the date on which the content was authored, contributed, or modified in YYYY-MM-DD format.</rdfs:comment>
        <rdfs:label>Entry Date</rdfs:label>
    </owl:DatatypeProperty>
    


    <!-- http://cwe.mitre.org/cwe#entryType -->

    <owl:DatatypeProperty rdf:about="http://cwe.mitre.org/cwe#entryType">
        <rdfs:domain rdf:resource="http://cwe.mitre.org/cwe#HistoryRecord"/>
        <rdfs:range>
            <rdfs:Datatype>
                <owl:oneOf>
                    <rdf:Description>
                        <rdf:type rdf:resource="http://www.w3.org/1999/02/22-rdf-syntax-ns#List"/>
                        <rdf:first rdf:datatype="http://www.w3.org/2001/XMLSchema#string">Contribution</rdf:first>
                        <rdf:rest>
                            <rdf:Description>
                                <rdf:type rdf:resource="http://www.w3.org/1999/02/22-rdf-syntax-ns#List"/>
                                <rdf:first rdf:datatype="http://www.w3.org/2001/XMLSchema#string">Modification</rdf:first>
                                <rdf:rest>
                                    <rdf:Description>
                                        <rdf:type rdf:resource="http://www.w3.org/1999/02/22-rdf-syntax-ns#List"/>
                                        <rdf:first rdf:datatype="http://www.w3.org/2001/XMLSchema#string">NameChange</rdf:first>
                                        <rdf:rest>
                                            <rdf:Description>
                                                <rdf:type rdf:resource="http://www.w3.org/1999/02/22-rdf-syntax-ns#List"/>
                                                <rdf:first rdf:datatype="http://www.w3.org/2001/XMLSchema#string">Submission</rdf:first>
                                                <rdf:rest rdf:resource="http://www.w3.org/1999/02/22-rdf-syntax-ns#nil"/>
                                            </rdf:Description>
                                        </rdf:rest>
                                    </rdf:Description>
                                </rdf:rest>
                            </rdf:Description>
                        </rdf:rest>
                    </rdf:Description>
                </owl:oneOf>
            </rdfs:Datatype>
        </rdfs:range>
        <rdfs:comment>Defines the type of the Content History.</rdfs:comment>
        <rdfs:label>Entry Type</rdfs:label>
    </owl:DatatypeProperty>
    


    <!-- http://cwe.mitre.org/cwe#environmentName -->

    <owl:DatatypeProperty rdf:about="http://cwe.mitre.org/cwe#environmentName">
        <rdfs:domain rdf:resource="http://cwe.mitre.org/cwe#Environment"/>
        <rdfs:range rdf:resource="http://www.w3.org/2001/XMLSchema#string"/>
        <rdfs:comment>Specifies the name of the Environment we are identifying.</rdfs:comment>
        <rdfs:label>Environment Name</rdfs:label>
    </owl:DatatypeProperty>
    


    <!-- http://cwe.mitre.org/cwe#exampleBody -->

    <owl:DatatypeProperty rdf:about="http://cwe.mitre.org/cwe#exampleBody">
        <rdfs:domain rdf:resource="http://cwe.mitre.org/cwe#DemonstrativeExample"/>
        <rdfs:range rdf:resource="http://www.w3.org/2001/XMLSchema#string"/>
        <rdfs:comment>Defines a description which should hold  the code and some explanatory information for the reader.</rdfs:comment>
        <rdfs:label>Example Body</rdfs:label>
    </owl:DatatypeProperty>
    


    <!-- http://cwe.mitre.org/cwe#externalLink -->

    <owl:DatatypeProperty rdf:about="http://cwe.mitre.org/cwe#externalLink">
        <rdfs:domain rdf:resource="http://cwe.mitre.org/cwe#ObservedExample"/>
        <rdfs:range rdf:resource="http://www.w3.org/2001/XMLSchema#anyURI"/>
        <rdfs:comment>Specifies a valid URL where more information regarding this example can be obtained.</rdfs:comment>
        <rdfs:label>Reference Link</rdfs:label>
    </owl:DatatypeProperty>
    


    <!-- http://cwe.mitre.org/cwe#form -->

    <owl:DatatypeProperty rdf:about="http://cwe.mitre.org/cwe#form">
        <rdfs:domain rdf:resource="http://cwe.mitre.org/cwe#RelationshipStatement"/>
        <rdfs:domain rdf:resource="http://cwe.mitre.org/cwe#Weakness"/>
        <rdfs:range>
            <rdfs:Datatype>
                <owl:oneOf>
                    <rdf:Description>
                        <rdf:type rdf:resource="http://www.w3.org/1999/02/22-rdf-syntax-ns#List"/>
                        <rdf:first rdf:datatype="http://www.w3.org/2001/XMLSchema#string">Category</rdf:first>
                        <rdf:rest>
                            <rdf:Description>
                                <rdf:type rdf:resource="http://www.w3.org/1999/02/22-rdf-syntax-ns#List"/>
                                <rdf:first rdf:datatype="http://www.w3.org/2001/XMLSchema#string">CompoundElements</rdf:first>
                                <rdf:rest>
                                    <rdf:Description>
                                        <rdf:type rdf:resource="http://www.w3.org/1999/02/22-rdf-syntax-ns#List"/>
                                        <rdf:first rdf:datatype="http://www.w3.org/2001/XMLSchema#string">View</rdf:first>
                                        <rdf:rest>
                                            <rdf:Description>
                                                <rdf:type rdf:resource="http://www.w3.org/1999/02/22-rdf-syntax-ns#List"/>
                                                <rdf:first rdf:datatype="http://www.w3.org/2001/XMLSchema#string">Weakness</rdf:first>
                                                <rdf:rest rdf:resource="http://www.w3.org/1999/02/22-rdf-syntax-ns#nil"/>
                                            </rdf:Description>
                                        </rdf:rest>
                                    </rdf:Description>
                                </rdf:rest>
                            </rdf:Description>
                        </rdf:rest>
                    </rdf:Description>
                </owl:oneOf>
            </rdfs:Datatype>
        </rdfs:range>
        <rdfs:comment>Specifies the form of the weakness.

A Compound Element represents a meaningful aggregation of several weaknesses, as in a chain like CWE-690: CWE-252 Unchecked Return Value can result in CWE-476 NULL Pointer Dereference or as in a composite like CWE-352 Cross-Site Request Forgery.  

A Category represents a collection of weaknesses sharing a common attribute, such as CWE-310 Cryptographic Issues or CWE-355 User Interface Security Issues. The shared attribute may any number of things including, but not limited to, environment (J2EE, .NET), functional area (authentication, cryptography) and the relevant resource (credentials management, certificate issues).</rdfs:comment>
        <rdfs:label>Form</rdfs:label>
    </owl:DatatypeProperty>
    


    <!-- http://cwe.mitre.org/cwe#formattedIdentifier -->

    <owl:DatatypeProperty rdf:about="http://cwe.mitre.org/cwe#formattedIdentifier">
        <rdfs:domain rdf:resource="http://cwe.mitre.org/cwe#Category"/>
        <rdfs:domain rdf:resource="http://cwe.mitre.org/cwe#CompoundElement"/>
        <rdfs:domain rdf:resource="http://cwe.mitre.org/cwe#View"/>
        <rdfs:domain rdf:resource="http://cwe.mitre.org/cwe#Weakness"/>
        <rdfs:range rdf:resource="http://www.w3.org/2001/XMLSchema#string"/>
        <rdfs:comment>Specifies the Common Weakness Enumeration (CWE) identifier associated with the weakness.  The weakness identifier should follow the CWE identifier pattern of &quot;CWE-nnnn&quot; where &apos;nnnnn&apos; specifies an numerically incrementing number.</rdfs:comment>
        <rdfs:label>Common Weakness Enumeration (CWE) identifier</rdfs:label>
    </owl:DatatypeProperty>
    


    <!-- http://cwe.mitre.org/cwe#functionalAreas -->

    <owl:DatatypeProperty rdf:about="http://cwe.mitre.org/cwe#functionalAreas">
        <rdfs:domain rdf:resource="http://cwe.mitre.org/cwe#Category"/>
        <rdfs:domain rdf:resource="http://cwe.mitre.org/cwe#CompoundElement"/>
        <rdfs:domain rdf:resource="http://cwe.mitre.org/cwe#Weakness"/>
        <rdfs:range rdf:resource="http://www.w3.org/2001/XMLSchema#string"/>
        <rdfs:comment>Defines one or more descriptions of the functional area of the software in which the 	weakness is most likely to occur. For example,  CWE-178 Failure to Resolve Case Sensitivity is likely to occur in functional areas of software related to file processing and credentials.</rdfs:comment>
        <rdfs:label>Functional Areas</rdfs:label>
    </owl:DatatypeProperty>
    


    <!-- http://cwe.mitre.org/cwe#hardwareArchitectureClassDescription -->

    <owl:DatatypeProperty rdf:about="http://cwe.mitre.org/cwe#hardwareArchitectureClassDescription">
        <rdfs:domain rdf:resource="http://cwe.mitre.org/cwe#HardwareArchitecture"/>
        <rdfs:range rdf:resource="http://www.w3.org/2001/XMLSchema#string"/>
        <rdfs:comment>Defines architectures in which this weakness is likely to exist.</rdfs:comment>
        <rdfs:label>Architecture Class Description</rdfs:label>
    </owl:DatatypeProperty>
    


    <!-- http://cwe.mitre.org/cwe#hardwareArchitectureName -->

    <owl:DatatypeProperty rdf:about="http://cwe.mitre.org/cwe#hardwareArchitectureName">
        <rdfs:domain rdf:resource="http://cwe.mitre.org/cwe#HardwareArchitecture"/>
        <rdfs:range>
            <rdfs:Datatype>
                <owl:oneOf>
                    <rdf:Description>
                        <rdf:type rdf:resource="http://www.w3.org/1999/02/22-rdf-syntax-ns#List"/>
                        <rdf:first rdf:datatype="http://www.w3.org/2001/XMLSchema#string">PowerPC</rdf:first>
                        <rdf:rest>
                            <rdf:Description>
                                <rdf:type rdf:resource="http://www.w3.org/1999/02/22-rdf-syntax-ns#List"/>
                                <rdf:first rdf:datatype="http://www.w3.org/2001/XMLSchema#string">SPARC</rdf:first>
                                <rdf:rest>
                                    <rdf:Description>
                                        <rdf:type rdf:resource="http://www.w3.org/1999/02/22-rdf-syntax-ns#List"/>
                                        <rdf:first rdf:datatype="http://www.w3.org/2001/XMLSchema#string">x86</rdf:first>
                                        <rdf:rest rdf:resource="http://www.w3.org/1999/02/22-rdf-syntax-ns#nil"/>
                                    </rdf:Description>
                                </rdf:rest>
                            </rdf:Description>
                        </rdf:rest>
                    </rdf:Description>
                </owl:oneOf>
            </rdfs:Datatype>
        </rdfs:range>
        <rdfs:comment>Defines  the name of the hardware architectures on which this weakness is likely to exist.</rdfs:comment>
        <rdfs:label>Name</rdfs:label>
    </owl:DatatypeProperty>
    


    <!-- http://cwe.mitre.org/cwe#id -->

    <owl:DatatypeProperty rdf:about="http://cwe.mitre.org/cwe#id">
        <rdfs:domain rdf:resource="http://cwe.mitre.org/cwe#Category"/>
        <rdfs:domain rdf:resource="http://cwe.mitre.org/cwe#CompoundElement"/>
        <rdfs:domain rdf:resource="http://cwe.mitre.org/cwe#View"/>
        <rdfs:domain rdf:resource="http://cwe.mitre.org/cwe#Weakness"/>
        <rdfs:range rdf:resource="http://www.w3.org/2001/XMLSchema#string"/>
        <rdfs:comment>Specifies the Common Weakness Enumeration (CWE) Identifier for this entry.   It will be static for the lifetime of the entry. In the event that this entry becomes deprecated, the ID will not be reused and a pointer will be left in this entry to the replacement.</rdfs:comment>
        <rdfs:label>Common Weakness Enumeration (CWE) Identifier</rdfs:label>
    </owl:DatatypeProperty>
    


    <!-- http://cwe.mitre.org/cwe#impactDescription -->

    <owl:DatatypeProperty rdf:about="http://cwe.mitre.org/cwe#impactDescription">
        <rdfs:domain rdf:resource="http://cwe.mitre.org/cwe#TechnicalImpact"/>
        <rdfs:range rdf:resource="http://www.w3.org/2001/XMLSchema#string"/>
        <rdfs:comment>Defines a description of the technical impact</rdfs:comment>
        <rdfs:label>Impact Description</rdfs:label>
    </owl:DatatypeProperty>
    


    <!-- http://cwe.mitre.org/cwe#impactType -->

    <owl:DatatypeProperty rdf:about="http://cwe.mitre.org/cwe#impactType">
        <rdfs:domain rdf:resource="http://cwe.mitre.org/cwe#TechnicalImpact"/>
        <rdfs:range rdf:resource="http://www.w3.org/2001/XMLSchema#string"/>
        <rdfs:comment>Specifies the type of impact</rdfs:comment>
        <rdfs:label>Impact Type</rdfs:label>
    </owl:DatatypeProperty>
    


    <!-- http://cwe.mitre.org/cwe#introText -->

    <owl:DatatypeProperty rdf:about="http://cwe.mitre.org/cwe#introText">
        <rdfs:domain rdf:resource="http://cwe.mitre.org/cwe#DemonstrativeExample"/>
        <rdfs:range rdf:resource="http://www.w3.org/2001/XMLSchema#string"/>
        <rdfs:comment>Defines the context and setting surrounding the example to add clarity for the reader.</rdfs:comment>
        <rdfs:label>Intro text</rdfs:label>
    </owl:DatatypeProperty>
    


    <!-- http://cwe.mitre.org/cwe#langClass -->

    <owl:DatatypeProperty rdf:about="http://cwe.mitre.org/cwe#langClass">
        <rdfs:domain rdf:resource="http://cwe.mitre.org/cwe#ProgrammingLanguage"/>
        <rdfs:range rdf:resource="http://www.w3.org/2001/XMLSchema#string"/>
        <rdfs:comment>Specifies a description of a type of language in which this entry is likely to exist. The type may be specified by a common property, such as Languages with Automated Memory Management or Languages which support Format Strings, or it may describe a more general class of language such as All Interpreted Languages or Pseudo Code.</rdfs:comment>
        <rdfs:label>Language Class</rdfs:label>
    </owl:DatatypeProperty>
    


    <!-- http://cwe.mitre.org/cwe#langName -->

    <owl:DatatypeProperty rdf:about="http://cwe.mitre.org/cwe#langName">
        <rdfs:domain rdf:resource="http://cwe.mitre.org/cwe#ProgrammingLanguage"/>
        <rdfs:range rdf:resource="http://www.w3.org/2001/XMLSchema#string"/>
        <rdfs:comment>Defines  the name of the  programming language in which this entry may occur.</rdfs:comment>
        <rdfs:label>Language Name</rdfs:label>
    </owl:DatatypeProperty>
    


    <!-- http://cwe.mitre.org/cwe#likelihood -->

    <owl:DatatypeProperty rdf:about="http://cwe.mitre.org/cwe#likelihood">
        <rdfs:domain rdf:resource="http://cwe.mitre.org/cwe#Category"/>
        <rdfs:domain rdf:resource="http://cwe.mitre.org/cwe#CompoundElement"/>
        <rdfs:domain rdf:resource="http://cwe.mitre.org/cwe#TechnicalImpact"/>
        <rdfs:domain rdf:resource="http://cwe.mitre.org/cwe#Weakness"/>
        <rdfs:range rdf:resource="http://www.w3.org/2001/XMLSchema#string"/>
        <rdfs:comment>Specifies a rough estimate at the likelihood of exploitation of an exposed weakness. Many factors can impact this value which is why it should only be regarded as an approximation.</rdfs:comment>
        <rdfs:label rdf:datatype="http://www.w3.org/2001/XMLSchema#string">Likelihood@en-US}</rdfs:label>
    </owl:DatatypeProperty>
    


    <!-- http://cwe.mitre.org/cwe#localReferenceId -->

    <owl:DatatypeProperty rdf:about="http://cwe.mitre.org/cwe#localReferenceId">
        <rdfs:domain rdf:resource="http://cwe.mitre.org/cwe#Reference"/>
        <rdfs:range rdf:resource="http://www.w3.org/2001/XMLSchema#string"/>
        <rdfs:comment>Specifies an identifier for the related Local	Reference. Only one Local Reference ID element can exist for each Reference element (ex: R.78.1). Text citing this reference should use the format [R.78.1] where &quot;78&quot; is the CWE identifier and &quot;1&quot; is the ordinal value of the reference (e.g., 1 being the first, 2 being the second).</rdfs:comment>
        <rdfs:label>Local Reference Identifier</rdfs:label>
    </owl:DatatypeProperty>
    


    <!-- http://cwe.mitre.org/cwe#mappedNodeId -->

    <owl:DatatypeProperty rdf:about="http://cwe.mitre.org/cwe#mappedNodeId">
        <rdfs:domain rdf:resource="http://cwe.mitre.org/cwe#TaxonomyMapping"/>
        <rdfs:range rdf:resource="http://www.w3.org/2001/XMLSchema#string"/>
        <rdfs:comment>Defines the ID of the entry to which this weakness is being mapped in taxonomy Taxonomy Name.</rdfs:comment>
        <rdfs:label>Mapped Node Identifier</rdfs:label>
    </owl:DatatypeProperty>
    


    <!-- http://cwe.mitre.org/cwe#mappedNodeName -->

    <owl:DatatypeProperty rdf:about="http://cwe.mitre.org/cwe#mappedNodeName">
        <rdfs:domain rdf:resource="http://cwe.mitre.org/cwe#TaxonomyMapping"/>
        <rdfs:range rdf:resource="http://www.w3.org/2001/XMLSchema#string"/>
        <rdfs:comment>Defines athe name of the entry to which this weakness is being mapped in taxonomy Taxonomy_Name.</rdfs:comment>
        <rdfs:label>Mapped Node Name</rdfs:label>
    </owl:DatatypeProperty>
    


    <!-- http://cwe.mitre.org/cwe#mappingFit -->

    <owl:DatatypeProperty rdf:about="http://cwe.mitre.org/cwe#mappingFit">
        <rdfs:domain rdf:resource="http://cwe.mitre.org/cwe#TaxonomyMapping"/>
        <rdfs:range>
            <rdfs:Datatype>
                <owl:oneOf>
                    <rdf:Description>
                        <rdf:type rdf:resource="http://www.w3.org/1999/02/22-rdf-syntax-ns#List"/>
                        <rdf:first rdf:datatype="http://www.w3.org/2001/XMLSchema#string">CWE_More_Abstract</rdf:first>
                        <rdf:rest>
                            <rdf:Description>
                                <rdf:type rdf:resource="http://www.w3.org/1999/02/22-rdf-syntax-ns#List"/>
                                <rdf:first rdf:datatype="http://www.w3.org/2001/XMLSchema#string">CWE_More_Specific</rdf:first>
                                <rdf:rest>
                                    <rdf:Description>
                                        <rdf:type rdf:resource="http://www.w3.org/1999/02/22-rdf-syntax-ns#List"/>
                                        <rdf:first rdf:datatype="http://www.w3.org/2001/XMLSchema#string">Exact</rdf:first>
                                        <rdf:rest>
                                            <rdf:Description>
                                                <rdf:type rdf:resource="http://www.w3.org/1999/02/22-rdf-syntax-ns#List"/>
                                                <rdf:first rdf:datatype="http://www.w3.org/2001/XMLSchema#string">Imprecise</rdf:first>
                                                <rdf:rest>
                                                    <rdf:Description>
                                                        <rdf:type rdf:resource="http://www.w3.org/1999/02/22-rdf-syntax-ns#List"/>
                                                        <rdf:first rdf:datatype="http://www.w3.org/2001/XMLSchema#string">Perspective</rdf:first>
                                                        <rdf:rest rdf:resource="http://www.w3.org/1999/02/22-rdf-syntax-ns#nil"/>
                                                    </rdf:Description>
                                                </rdf:rest>
                                            </rdf:Description>
                                        </rdf:rest>
                                    </rdf:Description>
                                </rdf:rest>
                            </rdf:Description>
                        </rdf:rest>
                    </rdf:Description>
                </owl:oneOf>
            </rdfs:Datatype>
        </rdfs:range>
        <rdfs:comment>Defines how close to the original taxonomy this node was mapped.</rdfs:comment>
        <rdfs:label>Mapping Fit</rdfs:label>
    </owl:DatatypeProperty>
    


    <!-- http://cwe.mitre.org/cwe#methodDescription -->

    <owl:DatatypeProperty rdf:about="http://cwe.mitre.org/cwe#methodDescription">
        <rdfs:domain rdf:resource="http://cwe.mitre.org/cwe#DetectionMethod"/>
        <rdfs:range rdf:resource="http://www.w3.org/2001/XMLSchema#string"/>
        <rdfs:comment>Defines some context of how this Detection Method can be applied to a specific weakness. This should be filled out for some 	weakness classes and bases.</rdfs:comment>
        <rdfs:label>Method Description</rdfs:label>
    </owl:DatatypeProperty>
    


    <!-- http://cwe.mitre.org/cwe#methodEffectiveness -->

    <owl:DatatypeProperty rdf:about="http://cwe.mitre.org/cwe#methodEffectiveness">
        <rdfs:domain rdf:resource="http://cwe.mitre.org/cwe#DetectionMethod"/>
        <rdfs:range>
            <rdfs:Datatype>
                <owl:oneOf>
                    <rdf:Description>
                        <rdf:type rdf:resource="http://www.w3.org/1999/02/22-rdf-syntax-ns#List"/>
                        <rdf:first rdf:datatype="http://www.w3.org/2001/XMLSchema#string">High</rdf:first>
                        <rdf:rest>
                            <rdf:Description>
                                <rdf:type rdf:resource="http://www.w3.org/1999/02/22-rdf-syntax-ns#List"/>
                                <rdf:first rdf:datatype="http://www.w3.org/2001/XMLSchema#string">Limited</rdf:first>
                                <rdf:rest>
                                    <rdf:Description>
                                        <rdf:type rdf:resource="http://www.w3.org/1999/02/22-rdf-syntax-ns#List"/>
                                        <rdf:first rdf:datatype="http://www.w3.org/2001/XMLSchema#string">Moderate</rdf:first>
                                        <rdf:rest>
                                            <rdf:Description>
                                                <rdf:type rdf:resource="http://www.w3.org/1999/02/22-rdf-syntax-ns#List"/>
                                                <rdf:first rdf:datatype="http://www.w3.org/2001/XMLSchema#string">None/Rare</rdf:first>
                                                <rdf:rest>
                                                    <rdf:Description>
                                                        <rdf:type rdf:resource="http://www.w3.org/1999/02/22-rdf-syntax-ns#List"/>
                                                        <rdf:first rdf:datatype="http://www.w3.org/2001/XMLSchema#string">Opportunistic</rdf:first>
                                                        <rdf:rest>
                                                            <rdf:Description>
                                                                <rdf:type rdf:resource="http://www.w3.org/1999/02/22-rdf-syntax-ns#List"/>
                                                                <rdf:first rdf:datatype="http://www.w3.org/2001/XMLSchema#string">SOAR High</rdf:first>
                                                                <rdf:rest>
                                                                    <rdf:Description>
                                                                        <rdf:type rdf:resource="http://www.w3.org/1999/02/22-rdf-syntax-ns#List"/>
                                                                        <rdf:first rdf:datatype="http://www.w3.org/2001/XMLSchema#string">SOAR Partial</rdf:first>
                                                                        <rdf:rest rdf:resource="http://www.w3.org/1999/02/22-rdf-syntax-ns#nil"/>
                                                                    </rdf:Description>
                                                                </rdf:rest>
                                                            </rdf:Description>
                                                        </rdf:rest>
                                                    </rdf:Description>
                                                </rdf:rest>
                                            </rdf:Description>
                                        </rdf:rest>
                                    </rdf:Description>
                                </rdf:rest>
                            </rdf:Description>
                        </rdf:rest>
                    </rdf:Description>
                </owl:oneOf>
            </rdfs:Datatype>
        </rdfs:range>
        <rdfs:comment>Defines how effective the detection method may be in detecting the associated weakness. This assumes the use of best-of-breed tools, analysts, and methods. There is limited consideration for financial costs, labor, or 	time.</rdfs:comment>
        <rdfs:label>Method Effectiveness</rdfs:label>
    </owl:DatatypeProperty>
    


    <!-- http://cwe.mitre.org/cwe#methodName -->

    <owl:DatatypeProperty rdf:about="http://cwe.mitre.org/cwe#methodName">
        <rdfs:domain rdf:resource="http://cwe.mitre.org/cwe#DetectionMethod"/>
        <rdfs:range rdf:resource="http://www.w3.org/2001/XMLSchema#string"/>
        <rdfs:comment>Specifies a name for the particular weakness detection method. This should be filled out for some weakness classes and bases.</rdfs:comment>
        <rdfs:label>Method Name</rdfs:label>
    </owl:DatatypeProperty>
    


    <!-- http://cwe.mitre.org/cwe#mitigationDescription -->

    <owl:DatatypeProperty rdf:about="http://cwe.mitre.org/cwe#mitigationDescription">
        <rdfs:domain rdf:resource="http://cwe.mitre.org/cwe#Mitigation"/>
        <rdfs:range rdf:resource="http://www.w3.org/2001/XMLSchema#string"/>
        <rdfs:comment>Defines the description of this individual mitigation.</rdfs:comment>
        <rdfs:label>Mitigation Description</rdfs:label>
    </owl:DatatypeProperty>
    


    <!-- http://cwe.mitre.org/cwe#mitigationEffectiveness -->

    <owl:DatatypeProperty rdf:about="http://cwe.mitre.org/cwe#mitigationEffectiveness">
        <rdfs:domain rdf:resource="http://cwe.mitre.org/cwe#Mitigation"/>
        <rdfs:range>
            <rdfs:Datatype>
                <owl:oneOf>
                    <rdf:Description>
                        <rdf:type rdf:resource="http://www.w3.org/1999/02/22-rdf-syntax-ns#List"/>
                        <rdf:first rdf:datatype="http://www.w3.org/2001/XMLSchema#string">Defense in Depth</rdf:first>
                        <rdf:rest>
                            <rdf:Description>
                                <rdf:type rdf:resource="http://www.w3.org/1999/02/22-rdf-syntax-ns#List"/>
                                <rdf:first rdf:datatype="http://www.w3.org/2001/XMLSchema#string">High</rdf:first>
                                <rdf:rest>
                                    <rdf:Description>
                                        <rdf:type rdf:resource="http://www.w3.org/1999/02/22-rdf-syntax-ns#List"/>
                                        <rdf:first rdf:datatype="http://www.w3.org/2001/XMLSchema#string">Incidental</rdf:first>
                                        <rdf:rest>
                                            <rdf:Description>
                                                <rdf:type rdf:resource="http://www.w3.org/1999/02/22-rdf-syntax-ns#List"/>
                                                <rdf:first rdf:datatype="http://www.w3.org/2001/XMLSchema#string">Limited</rdf:first>
                                                <rdf:rest>
                                                    <rdf:Description>
                                                        <rdf:type rdf:resource="http://www.w3.org/1999/02/22-rdf-syntax-ns#List"/>
                                                        <rdf:first rdf:datatype="http://www.w3.org/2001/XMLSchema#string">Moderate</rdf:first>
                                                        <rdf:rest>
                                                            <rdf:Description>
                                                                <rdf:type rdf:resource="http://www.w3.org/1999/02/22-rdf-syntax-ns#List"/>
                                                                <rdf:first rdf:datatype="http://www.w3.org/2001/XMLSchema#string">None</rdf:first>
                                                                <rdf:rest rdf:resource="http://www.w3.org/1999/02/22-rdf-syntax-ns#nil"/>
                                                            </rdf:Description>
                                                        </rdf:rest>
                                                    </rdf:Description>
                                                </rdf:rest>
                                            </rdf:Description>
                                        </rdf:rest>
                                    </rdf:Description>
                                </rdf:rest>
                            </rdf:Description>
                        </rdf:rest>
                    </rdf:Description>
                </owl:oneOf>
            </rdfs:Datatype>
        </rdfs:range>
        <rdfs:comment>Defines how effective the mitigation may be in preventing the weakness.</rdfs:comment>
        <rdfs:label>Mitigation Effectiveness</rdfs:label>
    </owl:DatatypeProperty>
    


    <!-- http://cwe.mitre.org/cwe#mitigationId -->

    <owl:DatatypeProperty rdf:about="http://cwe.mitre.org/cwe#mitigationId">
        <rdfs:domain rdf:resource="http://cwe.mitre.org/cwe#Mitigation"/>
        <rdfs:range rdf:resource="http://www.w3.org/2001/XMLSchema#string"/>
        <rdfs:comment>Defines the value for the related Mitigation entry identifier as a string. Only one Mitigation_ID element can exist for each Mitigation element (ex: MIT-1). However, Mitigations across CWE with the same ID should only vary in small details.</rdfs:comment>
        <rdfs:label>Mitigation Identifier</rdfs:label>
    </owl:DatatypeProperty>
    


    <!-- http://cwe.mitre.org/cwe#mitigationPhase -->

    <owl:DatatypeProperty rdf:about="http://cwe.mitre.org/cwe#mitigationPhase">
        <rdfs:domain rdf:resource="http://cwe.mitre.org/cwe#Mitigation"/>
        <rdfs:range rdf:resource="http://www.w3.org/2001/XMLSchema#string"/>
        <rdfs:comment>Defines  the development life cycle phase during which this particular mitigation may be applied.</rdfs:comment>
        <rdfs:label>Mitigation Phase</rdfs:label>
    </owl:DatatypeProperty>
    


    <!-- http://cwe.mitre.org/cwe#mitigationStrategy -->

    <owl:DatatypeProperty rdf:about="http://cwe.mitre.org/cwe#mitigationStrategy">
        <rdfs:domain rdf:resource="http://cwe.mitre.org/cwe#Mitigation"/>
        <rdfs:range>
            <rdfs:Datatype>
                <owl:oneOf>
                    <rdf:Description>
                        <rdf:type rdf:resource="http://www.w3.org/1999/02/22-rdf-syntax-ns#List"/>
                        <rdf:first rdf:datatype="http://www.w3.org/2001/XMLSchema#string">Compilation or Build Hardening</rdf:first>
                        <rdf:rest>
                            <rdf:Description>
                                <rdf:type rdf:resource="http://www.w3.org/1999/02/22-rdf-syntax-ns#List"/>
                                <rdf:first rdf:datatype="http://www.w3.org/2001/XMLSchema#string">Enforcement by Conversion</rdf:first>
                                <rdf:rest>
                                    <rdf:Description>
                                        <rdf:type rdf:resource="http://www.w3.org/1999/02/22-rdf-syntax-ns#List"/>
                                        <rdf:first rdf:datatype="http://www.w3.org/2001/XMLSchema#string">Environment Hardening</rdf:first>
                                        <rdf:rest>
                                            <rdf:Description>
                                                <rdf:type rdf:resource="http://www.w3.org/1999/02/22-rdf-syntax-ns#List"/>
                                                <rdf:first rdf:datatype="http://www.w3.org/2001/XMLSchema#string">Firewall</rdf:first>
                                                <rdf:rest>
                                                    <rdf:Description>
                                                        <rdf:type rdf:resource="http://www.w3.org/1999/02/22-rdf-syntax-ns#List"/>
                                                        <rdf:first rdf:datatype="http://www.w3.org/2001/XMLSchema#string">Identify and Reduce Attack Surface</rdf:first>
                                                        <rdf:rest>
                                                            <rdf:Description>
                                                                <rdf:type rdf:resource="http://www.w3.org/1999/02/22-rdf-syntax-ns#List"/>
                                                                <rdf:first rdf:datatype="http://www.w3.org/2001/XMLSchema#string">Input Validation</rdf:first>
                                                                <rdf:rest>
                                                                    <rdf:Description>
                                                                        <rdf:type rdf:resource="http://www.w3.org/1999/02/22-rdf-syntax-ns#List"/>
                                                                        <rdf:first rdf:datatype="http://www.w3.org/2001/XMLSchema#string">Language Selection</rdf:first>
                                                                        <rdf:rest>
                                                                            <rdf:Description>
                                                                                <rdf:type rdf:resource="http://www.w3.org/1999/02/22-rdf-syntax-ns#List"/>
                                                                                <rdf:first rdf:datatype="http://www.w3.org/2001/XMLSchema#string">Libraries or Frameworks</rdf:first>
                                                                                <rdf:rest>
                                                                                    <rdf:Description>
                                                                                        <rdf:type rdf:resource="http://www.w3.org/1999/02/22-rdf-syntax-ns#List"/>
                                                                                        <rdf:first rdf:datatype="http://www.w3.org/2001/XMLSchema#string">Limit Resource Consumption</rdf:first>
                                                                                        <rdf:rest>
                                                                                            <rdf:Description>
                                                                                                <rdf:type rdf:resource="http://www.w3.org/1999/02/22-rdf-syntax-ns#List"/>
                                                                                                <rdf:first rdf:datatype="http://www.w3.org/2001/XMLSchema#string">Output Encoding</rdf:first>
                                                                                                <rdf:rest>
                                                                                                    <rdf:Description>
                                                                                                        <rdf:type rdf:resource="http://www.w3.org/1999/02/22-rdf-syntax-ns#List"/>
                                                                                                        <rdf:first rdf:datatype="http://www.w3.org/2001/XMLSchema#string">Parameterization</rdf:first>
                                                                                                        <rdf:rest>
                                                                                                            <rdf:Description>
                                                                                                                <rdf:type rdf:resource="http://www.w3.org/1999/02/22-rdf-syntax-ns#List"/>
                                                                                                                <rdf:first rdf:datatype="http://www.w3.org/2001/XMLSchema#string">Refactoring</rdf:first>
                                                                                                                <rdf:rest>
                                                                                                                    <rdf:Description>
                                                                                                                        <rdf:type rdf:resource="http://www.w3.org/1999/02/22-rdf-syntax-ns#List"/>
                                                                                                                        <rdf:first rdf:datatype="http://www.w3.org/2001/XMLSchema#string">Sandbox or Jail</rdf:first>
                                                                                                                        <rdf:rest>
                                                                                                                            <rdf:Description>
                                                                                                                                <rdf:type rdf:resource="http://www.w3.org/1999/02/22-rdf-syntax-ns#List"/>
                                                                                                                                <rdf:first rdf:datatype="http://www.w3.org/2001/XMLSchema#string">Separation of Privilege</rdf:first>
                                                                                                                                <rdf:rest>
                                                                                                                                    <rdf:Description>
                                                                                                                                        <rdf:type rdf:resource="http://www.w3.org/1999/02/22-rdf-syntax-ns#List"/>
                                                                                                                                        <rdf:first rdf:datatype="http://www.w3.org/2001/XMLSchema#string">Threat Modeling</rdf:first>
                                                                                                                                        <rdf:rest rdf:resource="http://www.w3.org/1999/02/22-rdf-syntax-ns#nil"/>
                                                                                                                                    </rdf:Description>
                                                                                                                                </rdf:rest>
                                                                                                                            </rdf:Description>
                                                                                                                        </rdf:rest>
                                                                                                                    </rdf:Description>
                                                                                                                </rdf:rest>
                                                                                                            </rdf:Description>
                                                                                                        </rdf:rest>
                                                                                                    </rdf:Description>
                                                                                                </rdf:rest>
                                                                                            </rdf:Description>
                                                                                        </rdf:rest>
                                                                                    </rdf:Description>
                                                                                </rdf:rest>
                                                                            </rdf:Description>
                                                                        </rdf:rest>
                                                                    </rdf:Description>
                                                                </rdf:rest>
                                                            </rdf:Description>
                                                        </rdf:rest>
                                                    </rdf:Description>
                                                </rdf:rest>
                                            </rdf:Description>
                                        </rdf:rest>
                                    </rdf:Description>
                                </rdf:rest>
                            </rdf:Description>
                        </rdf:rest>
                    </rdf:Description>
                </owl:oneOf>
            </rdfs:Datatype>
        </rdfs:range>
        <rdfs:comment>Defines a general strategy for protecting a system to which this mitigation contributes</rdfs:comment>
        <rdfs:label>Mitigation Strategy</rdfs:label>
    </owl:DatatypeProperty>
    


    <!-- http://cwe.mitre.org/cwe#modificationImportance -->

    <owl:DatatypeProperty rdf:about="http://cwe.mitre.org/cwe#modificationImportance">
        <rdfs:domain rdf:resource="http://cwe.mitre.org/cwe#HistoryRecord"/>
        <rdfs:range>
            <rdfs:Datatype>
                <owl:oneOf>
                    <rdf:Description>
                        <rdf:type rdf:resource="http://www.w3.org/1999/02/22-rdf-syntax-ns#List"/>
                        <rdf:first rdf:datatype="http://www.w3.org/2001/XMLSchema#string">Critical</rdf:first>
                        <rdf:rest>
                            <rdf:Description>
                                <rdf:type rdf:resource="http://www.w3.org/1999/02/22-rdf-syntax-ns#List"/>
                                <rdf:first rdf:datatype="http://www.w3.org/2001/XMLSchema#string">Noramal</rdf:first>
                                <rdf:rest rdf:resource="http://www.w3.org/1999/02/22-rdf-syntax-ns#nil"/>
                            </rdf:Description>
                        </rdf:rest>
                    </rdf:Description>
                </owl:oneOf>
            </rdfs:Datatype>
        </rdfs:range>
        <rdfs:comment>Defines how significant the modification is to the weakness with regard to the meaning and interpretation of the weakness.  If a modification has a value of Critical, then the meaning of the entry or how it might be interpreted has changed and requires attention from anyone previously dependent on the weakness.</rdfs:comment>
        <rdfs:label>Modification Importance</rdfs:label>
    </owl:DatatypeProperty>
    


    <!-- http://cwe.mitre.org/cwe#modificationSource -->

    <owl:DatatypeProperty rdf:about="http://cwe.mitre.org/cwe#modificationSource">
        <rdfs:domain rdf:resource="http://cwe.mitre.org/cwe#HistoryRecord"/>
        <rdfs:range>
            <rdfs:Datatype>
                <owl:oneOf>
                    <rdf:Description>
                        <rdf:type rdf:resource="http://www.w3.org/1999/02/22-rdf-syntax-ns#List"/>
                        <rdf:first rdf:datatype="http://www.w3.org/2001/XMLSchema#string">External</rdf:first>
                        <rdf:rest>
                            <rdf:Description>
                                <rdf:type rdf:resource="http://www.w3.org/1999/02/22-rdf-syntax-ns#List"/>
                                <rdf:first rdf:datatype="http://www.w3.org/2001/XMLSchema#string">Internal</rdf:first>
                                <rdf:rest rdf:resource="http://www.w3.org/1999/02/22-rdf-syntax-ns#nil"/>
                            </rdf:Description>
                        </rdf:rest>
                    </rdf:Description>
                </owl:oneOf>
            </rdfs:Datatype>
        </rdfs:range>
        <rdfs:comment>Defines whether this modification was created by a CWE team member or provided by an external party.</rdfs:comment>
        <rdfs:label>Modification Source</rdfs:label>
    </owl:DatatypeProperty>
    


    <!-- http://cwe.mitre.org/cwe#noteType -->

    <owl:DatatypeProperty rdf:about="http://cwe.mitre.org/cwe#noteType">
        <rdfs:domain rdf:resource="http://cwe.mitre.org/cwe#Note"/>
        <rdfs:range>
            <rdfs:Datatype>
                <owl:oneOf>
                    <rdf:Description>
                        <rdf:type rdf:resource="http://www.w3.org/1999/02/22-rdf-syntax-ns#List"/>
                        <rdf:first rdf:datatype="http://www.w3.org/2001/XMLSchema#string">Consequence</rdf:first>
                        <rdf:rest>
                            <rdf:Description>
                                <rdf:type rdf:resource="http://www.w3.org/1999/02/22-rdf-syntax-ns#List"/>
                                <rdf:first rdf:datatype="http://www.w3.org/2001/XMLSchema#string">Maintenance</rdf:first>
                                <rdf:rest>
                                    <rdf:Description>
                                        <rdf:type rdf:resource="http://www.w3.org/1999/02/22-rdf-syntax-ns#List"/>
                                        <rdf:first rdf:datatype="http://www.w3.org/2001/XMLSchema#string">MethodEffectivenessNote</rdf:first>
                                        <rdf:rest>
                                            <rdf:Description>
                                                <rdf:type rdf:resource="http://www.w3.org/1999/02/22-rdf-syntax-ns#List"/>
                                                <rdf:first rdf:datatype="http://www.w3.org/2001/XMLSchema#string">Other</rdf:first>
                                                <rdf:rest>
                                                    <rdf:Description>
                                                        <rdf:type rdf:resource="http://www.w3.org/1999/02/22-rdf-syntax-ns#List"/>
                                                        <rdf:first rdf:datatype="http://www.w3.org/2001/XMLSchema#string">Platform</rdf:first>
                                                        <rdf:rest>
                                                            <rdf:Description>
                                                                <rdf:type rdf:resource="http://www.w3.org/1999/02/22-rdf-syntax-ns#List"/>
                                                                <rdf:first rdf:datatype="http://www.w3.org/2001/XMLSchema#string">Relationship</rdf:first>
                                                                <rdf:rest>
                                                                    <rdf:Description>
                                                                        <rdf:type rdf:resource="http://www.w3.org/1999/02/22-rdf-syntax-ns#List"/>
                                                                        <rdf:first rdf:datatype="http://www.w3.org/2001/XMLSchema#string">Terminology</rdf:first>
                                                                        <rdf:rest>
                                                                            <rdf:Description>
                                                                                <rdf:type rdf:resource="http://www.w3.org/1999/02/22-rdf-syntax-ns#List"/>
                                                                                <rdf:first rdf:datatype="http://www.w3.org/2001/XMLSchema#string">Theoretical</rdf:first>
                                                                                <rdf:rest rdf:resource="http://www.w3.org/1999/02/22-rdf-syntax-ns#nil"/>
                                                                            </rdf:Description>
                                                                        </rdf:rest>
                                                                    </rdf:Description>
                                                                </rdf:rest>
                                                            </rdf:Description>
                                                        </rdf:rest>
                                                    </rdf:Description>
                                                </rdf:rest>
                                            </rdf:Description>
                                        </rdf:rest>
                                    </rdf:Description>
                                </rdf:rest>
                            </rdf:Description>
                        </rdf:rest>
                    </rdf:Description>
                </owl:oneOf>
            </rdfs:Datatype>
        </rdfs:range>
        <rdfs:comment>Defines the type of Note.</rdfs:comment>
        <rdfs:label>Note Type</rdfs:label>
    </owl:DatatypeProperty>
    


    <!-- http://cwe.mitre.org/cwe#observationDescription -->

    <owl:DatatypeProperty rdf:about="http://cwe.mitre.org/cwe#observationDescription">
        <rdfs:domain rdf:resource="http://cwe.mitre.org/cwe#ObservedExample"/>
        <rdfs:range rdf:resource="http://www.w3.org/2001/XMLSchema#string"/>
        <rdfs:comment>Specifies a product independent description of the example being cited. The description should present an unambiguous correlation between the example being described and the weakness which it is meant to exemplify. It should also be short and easy to understand.</rdfs:comment>
        <rdfs:label>Description</rdfs:label>
    </owl:DatatypeProperty>
    


    <!-- http://cwe.mitre.org/cwe#ordinality -->

    <owl:DatatypeProperty rdf:about="http://cwe.mitre.org/cwe#ordinality">
        <rdfs:domain rdf:resource="http://cwe.mitre.org/cwe#WeaknessOrdinality"/>
        <rdfs:range>
            <rdfs:Datatype>
                <owl:oneOf>
                    <rdf:Description>
                        <rdf:type rdf:resource="http://www.w3.org/1999/02/22-rdf-syntax-ns#List"/>
                        <rdf:first rdf:datatype="http://www.w3.org/2001/XMLSchema#string">Primary</rdf:first>
                        <rdf:rest>
                            <rdf:Description>
                                <rdf:type rdf:resource="http://www.w3.org/1999/02/22-rdf-syntax-ns#List"/>
                                <rdf:first rdf:datatype="http://www.w3.org/2001/XMLSchema#string">Resultant</rdf:first>
                                <rdf:rest rdf:resource="http://www.w3.org/1999/02/22-rdf-syntax-ns#nil"/>
                            </rdf:Description>
                        </rdf:rest>
                    </rdf:Description>
                </owl:oneOf>
            </rdfs:Datatype>
        </rdfs:range>
        <rdfs:comment>Specifies whether this weakness exists independent of other weaknesses, 	Primary, or whether it is the result of the presence of some other weaknesses, Resultant.</rdfs:comment>
        <rdfs:label>Ordinality</rdfs:label>
    </owl:DatatypeProperty>
    


    <!-- http://cwe.mitre.org/cwe#ordinalityDescription -->

    <owl:DatatypeProperty rdf:about="http://cwe.mitre.org/cwe#ordinalityDescription">
        <rdfs:domain rdf:resource="http://cwe.mitre.org/cwe#WeaknessOrdinality"/>
        <rdfs:range rdf:resource="http://www.w3.org/2001/XMLSchema#string"/>
        <rdfs:comment>Specifies context in which this entry is either Primary or Resultant, depending on the corresponding value for Ordinality.</rdfs:comment>
        <rdfs:label>Description</rdfs:label>
    </owl:DatatypeProperty>
    


    <!-- http://cwe.mitre.org/cwe#osClass -->

    <owl:DatatypeProperty rdf:about="http://cwe.mitre.org/cwe#osClass">
        <rdfs:domain rdf:resource="http://cwe.mitre.org/cwe#OperatingSystem"/>
        <rdfs:range rdf:resource="http://www.w3.org/2001/XMLSchema#string"/>
        <rdfs:comment>Defines families or groups of operating systems in which this weakness is likely to exist. Do not fill this in if a specific Operating System was specified.</rdfs:comment>
        <rdfs:label>Operating System Class Description</rdfs:label>
    </owl:DatatypeProperty>
    


    <!-- http://cwe.mitre.org/cwe#osName -->

    <owl:DatatypeProperty rdf:about="http://cwe.mitre.org/cwe#osName">
        <rdfs:domain rdf:resource="http://cwe.mitre.org/cwe#OperatingSystem"/>
        <rdfs:range>
            <rdfs:Datatype>
                <owl:oneOf>
                    <rdf:Description>
                        <rdf:type rdf:resource="http://www.w3.org/1999/02/22-rdf-syntax-ns#List"/>
                        <rdf:first rdf:datatype="http://www.w3.org/2001/XMLSchema#string">FreeBSD</rdf:first>
                        <rdf:rest>
                            <rdf:Description>
                                <rdf:type rdf:resource="http://www.w3.org/1999/02/22-rdf-syntax-ns#List"/>
                                <rdf:first rdf:datatype="http://www.w3.org/2001/XMLSchema#string">MAC OS X</rdf:first>
                                <rdf:rest>
                                    <rdf:Description>
                                        <rdf:type rdf:resource="http://www.w3.org/1999/02/22-rdf-syntax-ns#List"/>
                                        <rdf:first rdf:datatype="http://www.w3.org/2001/XMLSchema#string">NetBSD</rdf:first>
                                        <rdf:rest>
                                            <rdf:Description>
                                                <rdf:type rdf:resource="http://www.w3.org/1999/02/22-rdf-syntax-ns#List"/>
                                                <rdf:first rdf:datatype="http://www.w3.org/2001/XMLSchema#string">OpenBSD</rdf:first>
                                                <rdf:rest>
                                                    <rdf:Description>
                                                        <rdf:type rdf:resource="http://www.w3.org/1999/02/22-rdf-syntax-ns#List"/>
                                                        <rdf:first rdf:datatype="http://www.w3.org/2001/XMLSchema#string">Red Hat Linux</rdf:first>
                                                        <rdf:rest>
                                                            <rdf:Description>
                                                                <rdf:type rdf:resource="http://www.w3.org/1999/02/22-rdf-syntax-ns#List"/>
                                                                <rdf:first rdf:datatype="http://www.w3.org/2001/XMLSchema#string">SUSE Linux</rdf:first>
                                                                <rdf:rest>
                                                                    <rdf:Description>
                                                                        <rdf:type rdf:resource="http://www.w3.org/1999/02/22-rdf-syntax-ns#List"/>
                                                                        <rdf:first rdf:datatype="http://www.w3.org/2001/XMLSchema#string">Solaris</rdf:first>
                                                                        <rdf:rest>
                                                                            <rdf:Description>
                                                                                <rdf:type rdf:resource="http://www.w3.org/1999/02/22-rdf-syntax-ns#List"/>
                                                                                <rdf:first rdf:datatype="http://www.w3.org/2001/XMLSchema#string">Ubuntu Linux</rdf:first>
                                                                                <rdf:rest>
                                                                                    <rdf:Description>
                                                                                        <rdf:type rdf:resource="http://www.w3.org/1999/02/22-rdf-syntax-ns#List"/>
                                                                                        <rdf:first rdf:datatype="http://www.w3.org/2001/XMLSchema#string">Windows 2000</rdf:first>
                                                                                        <rdf:rest>
                                                                                            <rdf:Description>
                                                                                                <rdf:type rdf:resource="http://www.w3.org/1999/02/22-rdf-syntax-ns#List"/>
                                                                                                <rdf:first rdf:datatype="http://www.w3.org/2001/XMLSchema#string">Windows 7</rdf:first>
                                                                                                <rdf:rest>
                                                                                                    <rdf:Description>
                                                                                                        <rdf:type rdf:resource="http://www.w3.org/1999/02/22-rdf-syntax-ns#List"/>
                                                                                                        <rdf:first rdf:datatype="http://www.w3.org/2001/XMLSchema#string">Windows Vista</rdf:first>
                                                                                                        <rdf:rest>
                                                                                                            <rdf:Description>
                                                                                                                <rdf:type rdf:resource="http://www.w3.org/1999/02/22-rdf-syntax-ns#List"/>
                                                                                                                <rdf:first rdf:datatype="http://www.w3.org/2001/XMLSchema#string">Windows XP</rdf:first>
                                                                                                                <rdf:rest rdf:resource="http://www.w3.org/1999/02/22-rdf-syntax-ns#nil"/>
                                                                                                            </rdf:Description>
                                                                                                        </rdf:rest>
                                                                                                    </rdf:Description>
                                                                                                </rdf:rest>
                                                                                            </rdf:Description>
                                                                                        </rdf:rest>
                                                                                    </rdf:Description>
                                                                                </rdf:rest>
                                                                            </rdf:Description>
                                                                        </rdf:rest>
                                                                    </rdf:Description>
                                                                </rdf:rest>
                                                            </rdf:Description>
                                                        </rdf:rest>
                                                    </rdf:Description>
                                                </rdf:rest>
                                            </rdf:Description>
                                        </rdf:rest>
                                    </rdf:Description>
                                </rdf:rest>
                            </rdf:Description>
                        </rdf:rest>
                    </rdf:Description>
                </owl:oneOf>
            </rdfs:Datatype>
        </rdfs:range>
        <rdfs:comment>Defines the name of the operating systems in which this weakness is likely to exist.</rdfs:comment>
        <rdfs:label>Name</rdfs:label>
    </owl:DatatypeProperty>
    


    <!-- http://cwe.mitre.org/cwe#paradigmName -->

    <owl:DatatypeProperty rdf:about="http://cwe.mitre.org/cwe#paradigmName">
        <rdfs:domain rdf:resource="http://cwe.mitre.org/cwe#ArchitectureParadigm"/>
        <rdfs:range>
            <rdfs:Datatype>
                <owl:oneOf>
                    <rdf:Description>
                        <rdf:type rdf:resource="http://www.w3.org/1999/02/22-rdf-syntax-ns#List"/>
                        <rdf:first rdf:datatype="http://www.w3.org/2001/XMLSchema#string">Client-Server</rdf:first>
                        <rdf:rest>
                            <rdf:Description>
                                <rdf:type rdf:resource="http://www.w3.org/1999/02/22-rdf-syntax-ns#List"/>
                                <rdf:first rdf:datatype="http://www.w3.org/2001/XMLSchema#string">Concurrent Systems Operating on Shared Resources</rdf:first>
                                <rdf:rest>
                                    <rdf:Description>
                                        <rdf:type rdf:resource="http://www.w3.org/1999/02/22-rdf-syntax-ns#List"/>
                                        <rdf:first rdf:datatype="http://www.w3.org/2001/XMLSchema#string">Mainframe</rdf:first>
                                        <rdf:rest>
                                            <rdf:Description>
                                                <rdf:type rdf:resource="http://www.w3.org/1999/02/22-rdf-syntax-ns#List"/>
                                                <rdf:first rdf:datatype="http://www.w3.org/2001/XMLSchema#string">Mobile Application</rdf:first>
                                                <rdf:rest>
                                                    <rdf:Description>
                                                        <rdf:type rdf:resource="http://www.w3.org/1999/02/22-rdf-syntax-ns#List"/>
                                                        <rdf:first rdf:datatype="http://www.w3.org/2001/XMLSchema#string">SOA</rdf:first>
                                                        <rdf:rest>
                                                            <rdf:Description>
                                                                <rdf:type rdf:resource="http://www.w3.org/1999/02/22-rdf-syntax-ns#List"/>
                                                                <rdf:first rdf:datatype="http://www.w3.org/2001/XMLSchema#string">Web-based</rdf:first>
                                                                <rdf:rest>
                                                                    <rdf:Description>
                                                                        <rdf:type rdf:resource="http://www.w3.org/1999/02/22-rdf-syntax-ns#List"/>
                                                                        <rdf:first rdf:datatype="http://www.w3.org/2001/XMLSchema#string">n-Tier</rdf:first>
                                                                        <rdf:rest rdf:resource="http://www.w3.org/1999/02/22-rdf-syntax-ns#nil"/>
                                                                    </rdf:Description>
                                                                </rdf:rest>
                                                            </rdf:Description>
                                                        </rdf:rest>
                                                    </rdf:Description>
                                                </rdf:rest>
                                            </rdf:Description>
                                        </rdf:rest>
                                    </rdf:Description>
                                </rdf:rest>
                            </rdf:Description>
                        </rdf:rest>
                    </rdf:Description>
                </owl:oneOf>
            </rdfs:Datatype>
        </rdfs:range>
        <rdfs:comment>Defines the name of the architecture  paradigm.</rdfs:comment>
        <rdfs:label>Paradigm Name</rdfs:label>
    </owl:DatatypeProperty>
    


    <!-- http://cwe.mitre.org/cwe#prevalence -->

    <owl:DatatypeProperty rdf:about="http://cwe.mitre.org/cwe#prevalence">
        <rdfs:domain rdf:resource="http://cwe.mitre.org/cwe#ArchitectureParadigm"/>
        <rdfs:domain rdf:resource="http://cwe.mitre.org/cwe#Environment"/>
        <rdfs:domain rdf:resource="http://cwe.mitre.org/cwe#HardwareArchitecture"/>
        <rdfs:domain rdf:resource="http://cwe.mitre.org/cwe#OperatingSystem"/>
        <rdfs:domain rdf:resource="http://cwe.mitre.org/cwe#ProgrammingLanguage"/>
        <rdfs:domain rdf:resource="http://cwe.mitre.org/cwe#TechnologyClass"/>
        <rdfs:range>
            <rdfs:Datatype>
                <owl:oneOf>
                    <rdf:Description>
                        <rdf:type rdf:resource="http://www.w3.org/1999/02/22-rdf-syntax-ns#List"/>
                        <rdf:first rdf:datatype="http://www.w3.org/2001/XMLSchema#string">Often</rdf:first>
                        <rdf:rest>
                            <rdf:Description>
                                <rdf:type rdf:resource="http://www.w3.org/1999/02/22-rdf-syntax-ns#List"/>
                                <rdf:first rdf:datatype="http://www.w3.org/2001/XMLSchema#string">Rarely</rdf:first>
                                <rdf:rest>
                                    <rdf:Description>
                                        <rdf:type rdf:resource="http://www.w3.org/1999/02/22-rdf-syntax-ns#List"/>
                                        <rdf:first rdf:datatype="http://www.w3.org/2001/XMLSchema#string">Sometimes</rdf:first>
                                        <rdf:rest rdf:resource="http://www.w3.org/1999/02/22-rdf-syntax-ns#nil"/>
                                    </rdf:Description>
                                </rdf:rest>
                            </rdf:Description>
                        </rdf:rest>
                    </rdf:Description>
                </owl:oneOf>
            </rdfs:Datatype>
        </rdfs:range>
        <rdfs:comment>Defines the prevalence with which this weakness may occur within code.</rdfs:comment>
        <rdfs:label>Prevalence</rdfs:label>
    </owl:DatatypeProperty>
    


    <!-- http://cwe.mitre.org/cwe#previousEntryName -->

    <owl:DatatypeProperty rdf:about="http://cwe.mitre.org/cwe#previousEntryName">
        <rdfs:domain rdf:resource="http://cwe.mitre.org/cwe#HistoryRecord"/>
        <rdfs:range rdf:resource="http://www.w3.org/2001/XMLSchema#string"/>
        <rdfs:comment>Specifies the name by which this entry was previously known.</rdfs:comment>
        <rdfs:label>Previous Names</rdfs:label>
    </owl:DatatypeProperty>
    


    <!-- http://cwe.mitre.org/cwe#referenceAuthorName -->

    <owl:DatatypeProperty rdf:about="http://cwe.mitre.org/cwe#referenceAuthorName">
        <rdfs:domain rdf:resource="http://cwe.mitre.org/cwe#Reference"/>
        <rdfs:range rdf:resource="http://www.w3.org/2001/XMLSchema#string"/>
        <rdfs:comment>Specifies the names of one or more an individuals that authored the material being referenced.</rdfs:comment>
        <rdfs:label>Author Name</rdfs:label>
    </owl:DatatypeProperty>
    


    <!-- http://cwe.mitre.org/cwe#referenceDate -->

    <owl:DatatypeProperty rdf:about="http://cwe.mitre.org/cwe#referenceDate">
        <rdfs:domain rdf:resource="http://cwe.mitre.org/cwe#Reference"/>
        <rdfs:range rdf:resource="http://www.w3.org/2001/XMLSchema#date"/>
        <rdfs:comment>Defines the date when the reference was 	included in the entry. This provides the reader with a time line for when the material in the reference, usually the link, was valid. The date should be of the format YYYY-MM-DD.</rdfs:comment>
        <rdfs:label>Date</rdfs:label>
    </owl:DatatypeProperty>
    


    <!-- http://cwe.mitre.org/cwe#referenceEdition -->

    <owl:DatatypeProperty rdf:about="http://cwe.mitre.org/cwe#referenceEdition">
        <rdfs:domain rdf:resource="http://cwe.mitre.org/cwe#Reference"/>
        <rdfs:range rdf:resource="http://www.w3.org/2001/XMLSchema#string"/>
        <rdfs:comment>Defines the edition of the material being 	referenced in the event that multiple editions of the material exist. This will usually only be useful for book references.</rdfs:comment>
        <rdfs:label>Edition</rdfs:label>
    </owl:DatatypeProperty>
    


    <!-- http://cwe.mitre.org/cwe#referenceId -->

    <owl:DatatypeProperty rdf:about="http://cwe.mitre.org/cwe#referenceId">
        <rdfs:domain rdf:resource="http://cwe.mitre.org/cwe#Reference"/>
        <rdfs:range rdf:resource="http://www.w3.org/2001/XMLSchema#string"/>
        <rdfs:comment>Defines the identifier for the related Reference  entry identifier as a string. Only one Reference_ID element can exist for each Reference element (ex: REF-1). However, References across CWE with the same ID should only vary in small details. Text citing this reference should use the local reference ID, as this ID is only for reference library related consistency checking and maintenance.</rdfs:comment>
        <rdfs:label>Reference Identifier</rdfs:label>
    </owl:DatatypeProperty>
    


    <!-- http://cwe.mitre.org/cwe#referenceIdentifier -->

    <owl:DatatypeProperty rdf:about="http://cwe.mitre.org/cwe#referenceIdentifier">
        <rdfs:domain rdf:resource="http://cwe.mitre.org/cwe#ObservedExample"/>
        <rdfs:range rdf:resource="http://www.w3.org/2001/XMLSchema#string"/>
        <rdfs:comment>Specifies  the identifier for the example being cited. For example, if a CVE is being cited it should be of the standard CVE identifier format, such as CVE-2005-1951 or CVE-1999-0046.</rdfs:comment>
        <rdfs:label>Reference Identifier</rdfs:label>
    </owl:DatatypeProperty>
    


    <!-- http://cwe.mitre.org/cwe#referenceLink -->

    <owl:DatatypeProperty rdf:about="http://cwe.mitre.org/cwe#referenceLink">
        <rdfs:domain rdf:resource="http://cwe.mitre.org/cwe#Reference"/>
        <rdfs:range rdf:resource="http://www.w3.org/2001/XMLSchema#anyURI"/>
        <rdfs:comment>Defines the URL for the material being 	referenced, if one exists. This should always be used for web references, and may optionally be used for book and other publication references.</rdfs:comment>
        <rdfs:label>Reference Link</rdfs:label>
    </owl:DatatypeProperty>
    


    <!-- http://cwe.mitre.org/cwe#referencePubDate -->

    <owl:DatatypeProperty rdf:about="http://cwe.mitre.org/cwe#referencePubDate">
        <rdfs:domain rdf:resource="http://cwe.mitre.org/cwe#Reference"/>
        <rdfs:range rdf:resource="http://www.w3.org/2001/XMLSchema#gYear"/>
        <rdfs:comment>Defines  the date when the reference was published YYYY.</rdfs:comment>
        <rdfs:label>Published Date</rdfs:label>
    </owl:DatatypeProperty>
    


    <!-- http://cwe.mitre.org/cwe#referencePublication -->

    <owl:DatatypeProperty rdf:about="http://cwe.mitre.org/cwe#referencePublication">
        <rdfs:domain rdf:resource="http://cwe.mitre.org/cwe#Reference"/>
        <rdfs:range rdf:resource="http://www.w3.org/2001/XMLSchema#string"/>
        <rdfs:comment>Defines the publication source of the reference material, if one exists.</rdfs:comment>
        <rdfs:label>Publication</rdfs:label>
    </owl:DatatypeProperty>
    


    <!-- http://cwe.mitre.org/cwe#referencePublisherName -->

    <owl:DatatypeProperty rdf:about="http://cwe.mitre.org/cwe#referencePublisherName">
        <rdfs:domain rdf:resource="http://cwe.mitre.org/cwe#Reference"/>
        <rdfs:range rdf:resource="http://www.w3.org/2001/XMLSchema#string"/>
        <rdfs:comment>Defines the publisher of the reference material, if one exists.</rdfs:comment>
        <rdfs:label>Publisher</rdfs:label>
    </owl:DatatypeProperty>
    


    <!-- http://cwe.mitre.org/cwe#referenceSection -->

    <owl:DatatypeProperty rdf:about="http://cwe.mitre.org/cwe#referenceSection">
        <rdfs:domain rdf:resource="http://cwe.mitre.org/cwe#Reference"/>
        <rdfs:range rdf:resource="http://www.w3.org/2001/XMLSchema#string"/>
        <rdfs:comment>Defines a means of identifying the exact location of the material inside of the publication source, such as the relevant pages of a research paper, the appropriate chapters from a book, etc. This is useful for both book references and internet references.</rdfs:comment>
        <rdfs:label>Section</rdfs:label>
    </owl:DatatypeProperty>
    


    <!-- http://cwe.mitre.org/cwe#referenceTitle -->

    <owl:DatatypeProperty rdf:about="http://cwe.mitre.org/cwe#referenceTitle">
        <rdfs:domain rdf:resource="http://cwe.mitre.org/cwe#Reference"/>
        <rdfs:range rdf:resource="http://www.w3.org/2001/XMLSchema#string"/>
        <rdfs:comment>Defines the title of the material being referenced. It is not required if the material does not have a title.</rdfs:comment>
        <rdfs:label>Title</rdfs:label>
    </owl:DatatypeProperty>
    


    <!-- http://cwe.mitre.org/cwe#relationshipNature -->

    <owl:DatatypeProperty rdf:about="http://cwe.mitre.org/cwe#relationshipNature">
        <rdfs:domain rdf:resource="http://cwe.mitre.org/cwe#RelationshipStatement"/>
        <rdfs:range>
            <rdfs:Datatype>
                <owl:oneOf>
                    <rdf:Description>
                        <rdf:type rdf:resource="http://www.w3.org/1999/02/22-rdf-syntax-ns#List"/>
                        <rdf:first rdf:datatype="http://www.w3.org/2001/XMLSchema#string">CanAlsoBe</rdf:first>
                        <rdf:rest>
                            <rdf:Description>
                                <rdf:type rdf:resource="http://www.w3.org/1999/02/22-rdf-syntax-ns#List"/>
                                <rdf:first rdf:datatype="http://www.w3.org/2001/XMLSchema#string">CanFollow</rdf:first>
                                <rdf:rest>
                                    <rdf:Description>
                                        <rdf:type rdf:resource="http://www.w3.org/1999/02/22-rdf-syntax-ns#List"/>
                                        <rdf:first rdf:datatype="http://www.w3.org/2001/XMLSchema#string">CanProceed</rdf:first>
                                        <rdf:rest>
                                            <rdf:Description>
                                                <rdf:type rdf:resource="http://www.w3.org/1999/02/22-rdf-syntax-ns#List"/>
                                                <rdf:first rdf:datatype="http://www.w3.org/2001/XMLSchema#string">ChildOf</rdf:first>
                                                <rdf:rest>
                                                    <rdf:Description>
                                                        <rdf:type rdf:resource="http://www.w3.org/1999/02/22-rdf-syntax-ns#List"/>
                                                        <rdf:first rdf:datatype="http://www.w3.org/2001/XMLSchema#string">HasMember</rdf:first>
                                                        <rdf:rest>
                                                            <rdf:Description>
                                                                <rdf:type rdf:resource="http://www.w3.org/1999/02/22-rdf-syntax-ns#List"/>
                                                                <rdf:first rdf:datatype="http://www.w3.org/2001/XMLSchema#string">MemberOf</rdf:first>
                                                                <rdf:rest>
                                                                    <rdf:Description>
                                                                        <rdf:type rdf:resource="http://www.w3.org/1999/02/22-rdf-syntax-ns#List"/>
                                                                        <rdf:first rdf:datatype="http://www.w3.org/2001/XMLSchema#string">ParentOf</rdf:first>
                                                                        <rdf:rest>
                                                                            <rdf:Description>
                                                                                <rdf:type rdf:resource="http://www.w3.org/1999/02/22-rdf-syntax-ns#List"/>
                                                                                <rdf:first rdf:datatype="http://www.w3.org/2001/XMLSchema#string">PeerOf</rdf:first>
                                                                                <rdf:rest>
                                                                                    <rdf:Description>
                                                                                        <rdf:type rdf:resource="http://www.w3.org/1999/02/22-rdf-syntax-ns#List"/>
                                                                                        <rdf:first rdf:datatype="http://www.w3.org/2001/XMLSchema#string">RequiredBy</rdf:first>
                                                                                        <rdf:rest>
                                                                                            <rdf:Description>
                                                                                                <rdf:type rdf:resource="http://www.w3.org/1999/02/22-rdf-syntax-ns#List"/>
                                                                                                <rdf:first rdf:datatype="http://www.w3.org/2001/XMLSchema#string">Requires</rdf:first>
                                                                                                <rdf:rest>
                                                                                                    <rdf:Description>
                                                                                                        <rdf:type rdf:resource="http://www.w3.org/1999/02/22-rdf-syntax-ns#List"/>
                                                                                                        <rdf:first rdf:datatype="http://www.w3.org/2001/XMLSchema#string">StartsChain</rdf:first>
                                                                                                        <rdf:rest>
                                                                                                            <rdf:Description>
                                                                                                                <rdf:type rdf:resource="http://www.w3.org/1999/02/22-rdf-syntax-ns#List"/>
                                                                                                                <rdf:first rdf:datatype="http://www.w3.org/2001/XMLSchema#string">StartsWith</rdf:first>
                                                                                                                <rdf:rest rdf:resource="http://www.w3.org/1999/02/22-rdf-syntax-ns#nil"/>
                                                                                                            </rdf:Description>
                                                                                                        </rdf:rest>
                                                                                                    </rdf:Description>
                                                                                                </rdf:rest>
                                                                                            </rdf:Description>
                                                                                        </rdf:rest>
                                                                                    </rdf:Description>
                                                                                </rdf:rest>
                                                                            </rdf:Description>
                                                                        </rdf:rest>
                                                                    </rdf:Description>
                                                                </rdf:rest>
                                                            </rdf:Description>
                                                        </rdf:rest>
                                                    </rdf:Description>
                                                </rdf:rest>
                                            </rdf:Description>
                                        </rdf:rest>
                                    </rdf:Description>
                                </rdf:rest>
                            </rdf:Description>
                        </rdf:rest>
                    </rdf:Description>
                </owl:oneOf>
            </rdfs:Datatype>
        </rdfs:range>
        <rdfs:comment>Specifies the nature of the relationship between this element and the target element, such as ChildOf, HasMember or Requires to name a few.</rdfs:comment>
        <rdfs:label>Relationship Nature</rdfs:label>
    </owl:DatatypeProperty>
    


    <!-- http://cwe.mitre.org/cwe#relativeId -->

    <owl:DatatypeProperty rdf:about="http://cwe.mitre.org/cwe#relativeId">
        <rdfs:domain rdf:resource="http://cwe.mitre.org/cwe#Consequence"/>
        <rdfs:domain rdf:resource="http://cwe.mitre.org/cwe#DemonstrativeExample"/>
        <rdfs:domain rdf:resource="http://cwe.mitre.org/cwe#HistoryRecord"/>
        <rdfs:domain rdf:resource="http://cwe.mitre.org/cwe#Mitigation"/>
        <rdfs:domain rdf:resource="http://cwe.mitre.org/cwe#ObservedExample"/>
        <rdfs:domain rdf:resource="http://cwe.mitre.org/cwe#TaxonomyMapping"/>
        <rdfs:range rdf:resource="http://www.w3.org/2001/XMLSchema#string"/>
        <rdfs:comment>Specifies an identifier for the related entity.  Only one relative ID element can exist for each entity (ex: R.78.1). Text citing this reference should use the format [R.78.1] where &quot;78&quot; is the entity identifier and &quot;1&quot; is the ordinal value of the reference (e.g., 1 being the first, 2 being the second)</rdfs:comment>
        <rdfs:label>Relative ID</rdfs:label>
    </owl:DatatypeProperty>
    


    <!-- http://cwe.mitre.org/cwe#relevantProperties -->

    <owl:DatatypeProperty rdf:about="http://cwe.mitre.org/cwe#relevantProperties">
        <rdfs:domain rdf:resource="http://cwe.mitre.org/cwe#Category"/>
        <rdfs:domain rdf:resource="http://cwe.mitre.org/cwe#CompoundElement"/>
        <rdfs:domain rdf:resource="http://cwe.mitre.org/cwe#Weakness"/>
        <rdfs:range>
            <rdfs:Datatype>
                <owl:oneOf>
                    <rdf:Description>
                        <rdf:type rdf:resource="http://www.w3.org/1999/02/22-rdf-syntax-ns#List"/>
                        <rdf:first rdf:datatype="http://www.w3.org/2001/XMLSchema#string">Accessibility</rdf:first>
                        <rdf:rest>
                            <rdf:Description>
                                <rdf:type rdf:resource="http://www.w3.org/1999/02/22-rdf-syntax-ns#List"/>
                                <rdf:first rdf:datatype="http://www.w3.org/2001/XMLSchema#string">Equivalence</rdf:first>
                                <rdf:rest>
                                    <rdf:Description>
                                        <rdf:type rdf:resource="http://www.w3.org/1999/02/22-rdf-syntax-ns#List"/>
                                        <rdf:first rdf:datatype="http://www.w3.org/2001/XMLSchema#string">Mutability</rdf:first>
                                        <rdf:rest>
                                            <rdf:Description>
                                                <rdf:type rdf:resource="http://www.w3.org/1999/02/22-rdf-syntax-ns#List"/>
                                                <rdf:first rdf:datatype="http://www.w3.org/2001/XMLSchema#string">Predictability</rdf:first>
                                                <rdf:rest>
                                                    <rdf:Description>
                                                        <rdf:type rdf:resource="http://www.w3.org/1999/02/22-rdf-syntax-ns#List"/>
                                                        <rdf:first rdf:datatype="http://www.w3.org/2001/XMLSchema#string">Trustability</rdf:first>
                                                        <rdf:rest>
                                                            <rdf:Description>
                                                                <rdf:type rdf:resource="http://www.w3.org/1999/02/22-rdf-syntax-ns#List"/>
                                                                <rdf:first rdf:datatype="http://www.w3.org/2001/XMLSchema#string">Uniqueness</rdf:first>
                                                                <rdf:rest>
                                                                    <rdf:Description>
                                                                        <rdf:type rdf:resource="http://www.w3.org/1999/02/22-rdf-syntax-ns#List"/>
                                                                        <rdf:first rdf:datatype="http://www.w3.org/2001/XMLSchema#string">Validty</rdf:first>
                                                                        <rdf:rest rdf:resource="http://www.w3.org/1999/02/22-rdf-syntax-ns#nil"/>
                                                                    </rdf:Description>
                                                                </rdf:rest>
                                                            </rdf:Description>
                                                        </rdf:rest>
                                                    </rdf:Description>
                                                </rdf:rest>
                                            </rdf:Description>
                                        </rdf:rest>
                                    </rdf:Description>
                                </rdf:rest>
                            </rdf:Description>
                        </rdf:rest>
                    </rdf:Description>
                </owl:oneOf>
            </rdfs:Datatype>
        </rdfs:range>
        <rdfs:comment>Defines one or more Relevant Property.  Each Relevant Property element identifies a property that is required by the code or a resource in order to function as specified.  Correctly labeling all of the relevant properties can help to figure out 	what the root cause of a vulnerability might be.</rdfs:comment>
        <rdfs:label>Relevant Properties</rdfs:label>
    </owl:DatatypeProperty>
    


    <!-- http://cwe.mitre.org/cwe#stakeholder -->

    <owl:DatatypeProperty rdf:about="http://cwe.mitre.org/cwe#stakeholder">
        <rdfs:domain rdf:resource="http://cwe.mitre.org/cwe#Audience"/>
        <rdfs:range rdf:resource="http://www.w3.org/2001/XMLSchema#string"/>
        <rdfs:comment>Specifies what types of members of the CWE community might be interested in this view.</rdfs:comment>
        <rdfs:label>Stakeholder</rdfs:label>
    </owl:DatatypeProperty>
    


    <!-- http://cwe.mitre.org/cwe#stakeholderDescription -->

    <owl:DatatypeProperty rdf:about="http://cwe.mitre.org/cwe#stakeholderDescription">
        <rdfs:domain rdf:resource="http://cwe.mitre.org/cwe#Audience"/>
        <rdfs:range rdf:resource="http://www.w3.org/2001/XMLSchema#string"/>
        <rdfs:comment>Specifies a description of what properties of this View this particular Stakeholder might find useful.</rdfs:comment>
        <rdfs:label>Description</rdfs:label>
    </owl:DatatypeProperty>
    


    <!-- http://cwe.mitre.org/cwe#status -->

    <owl:DatatypeProperty rdf:about="http://cwe.mitre.org/cwe#status">
        <rdfs:domain rdf:resource="http://cwe.mitre.org/cwe#Category"/>
        <rdfs:domain rdf:resource="http://cwe.mitre.org/cwe#CompoundElement"/>
        <rdfs:domain rdf:resource="http://cwe.mitre.org/cwe#View"/>
        <rdfs:domain rdf:resource="http://cwe.mitre.org/cwe#Weakness"/>
        <rdfs:range>
            <rdfs:Datatype>
                <owl:oneOf>
                    <rdf:Description>
                        <rdf:type rdf:resource="http://www.w3.org/1999/02/22-rdf-syntax-ns#List"/>
                        <rdf:first rdf:datatype="http://www.w3.org/2001/XMLSchema#string">Deprecated</rdf:first>
                        <rdf:rest>
                            <rdf:Description>
                                <rdf:type rdf:resource="http://www.w3.org/1999/02/22-rdf-syntax-ns#List"/>
                                <rdf:first rdf:datatype="http://www.w3.org/2001/XMLSchema#string">Draft</rdf:first>
                                <rdf:rest>
                                    <rdf:Description>
                                        <rdf:type rdf:resource="http://www.w3.org/1999/02/22-rdf-syntax-ns#List"/>
                                        <rdf:first rdf:datatype="http://www.w3.org/2001/XMLSchema#string">Incomplete</rdf:first>
                                        <rdf:rest>
                                            <rdf:Description>
                                                <rdf:type rdf:resource="http://www.w3.org/1999/02/22-rdf-syntax-ns#List"/>
                                                <rdf:first rdf:datatype="http://www.w3.org/2001/XMLSchema#string">Stable</rdf:first>
                                                <rdf:rest>
                                                    <rdf:Description>
                                                        <rdf:type rdf:resource="http://www.w3.org/1999/02/22-rdf-syntax-ns#List"/>
                                                        <rdf:first rdf:datatype="http://www.w3.org/2001/XMLSchema#string">Usable</rdf:first>
                                                        <rdf:rest rdf:resource="http://www.w3.org/1999/02/22-rdf-syntax-ns#nil"/>
                                                    </rdf:Description>
                                                </rdf:rest>
                                            </rdf:Description>
                                        </rdf:rest>
                                    </rdf:Description>
                                </rdf:rest>
                            </rdf:Description>
                        </rdf:rest>
                    </rdf:Description>
                </owl:oneOf>
            </rdfs:Datatype>
        </rdfs:range>
        <rdfs:comment>Specifies the status level for this weakness.</rdfs:comment>
        <rdfs:label>Status</rdfs:label>
    </owl:DatatypeProperty>
    


    <!-- http://cwe.mitre.org/cwe#structureType -->

    <owl:DatatypeProperty rdf:about="http://cwe.mitre.org/cwe#structureType">
        <rdfs:domain rdf:resource="http://cwe.mitre.org/cwe#View"/>
        <rdfs:range>
            <rdfs:Datatype>
                <owl:oneOf>
                    <rdf:Description>
                        <rdf:type rdf:resource="http://www.w3.org/1999/02/22-rdf-syntax-ns#List"/>
                        <rdf:first rdf:datatype="http://www.w3.org/2001/XMLSchema#string">Explicit_Slice</rdf:first>
                        <rdf:rest>
                            <rdf:Description>
                                <rdf:type rdf:resource="http://www.w3.org/1999/02/22-rdf-syntax-ns#List"/>
                                <rdf:first rdf:datatype="http://www.w3.org/2001/XMLSchema#string">Graph</rdf:first>
                                <rdf:rest>
                                    <rdf:Description>
                                        <rdf:type rdf:resource="http://www.w3.org/1999/02/22-rdf-syntax-ns#List"/>
                                        <rdf:first rdf:datatype="http://www.w3.org/2001/XMLSchema#string">Implicit_Slice</rdf:first>
                                        <rdf:rest rdf:resource="http://www.w3.org/1999/02/22-rdf-syntax-ns#nil"/>
                                    </rdf:Description>
                                </rdf:rest>
                            </rdf:Description>
                        </rdf:rest>
                    </rdf:Description>
                </owl:oneOf>
            </rdfs:Datatype>
        </rdfs:range>
        <rdfs:comment>Specifies how this view is being constructed. 

Valid values are: Implicit Slice = a slice based on a filter criteria; Explicit Slice = a slice based on arbitrary membership, as defined by specific relationships between entries; Graph = a bounded graphical slice based on ChildOf relationships</rdfs:comment>
        <rdfs:label>Structure Type</rdfs:label>
    </owl:DatatypeProperty>
    


    <!-- http://cwe.mitre.org/cwe#submissionSource -->

    <owl:DatatypeProperty rdf:about="http://cwe.mitre.org/cwe#submissionSource">
        <rdfs:domain rdf:resource="http://cwe.mitre.org/cwe#HistoryRecord"/>
        <rdfs:range>
            <rdfs:Datatype>
                <owl:oneOf>
                    <rdf:Description>
                        <rdf:type rdf:resource="http://www.w3.org/1999/02/22-rdf-syntax-ns#List"/>
                        <rdf:first rdf:datatype="http://www.w3.org/2001/XMLSchema#string">External_Submission</rdf:first>
                        <rdf:rest>
                            <rdf:Description>
                                <rdf:type rdf:resource="http://www.w3.org/1999/02/22-rdf-syntax-ns#List"/>
                                <rdf:first rdf:datatype="http://www.w3.org/2001/XMLSchema#string">Externally_Mined</rdf:first>
                                <rdf:rest>
                                    <rdf:Description>
                                        <rdf:type rdf:resource="http://www.w3.org/1999/02/22-rdf-syntax-ns#List"/>
                                        <rdf:first rdf:datatype="http://www.w3.org/2001/XMLSchema#string">Internal_CWE_Team</rdf:first>
                                        <rdf:rest>
                                            <rdf:Description>
                                                <rdf:type rdf:resource="http://www.w3.org/1999/02/22-rdf-syntax-ns#List"/>
                                                <rdf:first rdf:datatype="http://www.w3.org/2001/XMLSchema#string">NDA</rdf:first>
                                                <rdf:rest rdf:resource="http://www.w3.org/1999/02/22-rdf-syntax-ns#nil"/>
                                            </rdf:Description>
                                        </rdf:rest>
                                    </rdf:Description>
                                </rdf:rest>
                            </rdf:Description>
                        </rdf:rest>
                    </rdf:Description>
                </owl:oneOf>
            </rdfs:Datatype>
        </rdfs:range>
        <rdfs:comment>Defines how the initial information for this entry was obtained.</rdfs:comment>
        <rdfs:label>Submission Source</rdfs:label>
    </owl:DatatypeProperty>
    


    <!-- http://cwe.mitre.org/cwe#taxonomyName -->

    <owl:DatatypeProperty rdf:about="http://cwe.mitre.org/cwe#taxonomyName">
        <rdfs:domain rdf:resource="http://cwe.mitre.org/cwe#TaxonomyMapping"/>
        <rdfs:range>
            <rdfs:Datatype>
                <owl:oneOf>
                    <rdf:Description>
                        <rdf:type rdf:resource="http://www.w3.org/1999/02/22-rdf-syntax-ns#List"/>
                        <rdf:first rdf:datatype="http://www.w3.org/2001/XMLSchema#string">19 Deadly Sins</rdf:first>
                        <rdf:rest>
                            <rdf:Description>
                                <rdf:type rdf:resource="http://www.w3.org/1999/02/22-rdf-syntax-ns#List"/>
                                <rdf:first rdf:datatype="http://www.w3.org/2001/XMLSchema#string">7 Pernicious Kingdoms</rdf:first>
                                <rdf:rest>
                                    <rdf:Description>
                                        <rdf:type rdf:resource="http://www.w3.org/1999/02/22-rdf-syntax-ns#List"/>
                                        <rdf:first rdf:datatype="http://www.w3.org/2001/XMLSchema#string">Anonymous Tool Vendor (under NDA)</rdf:first>
                                        <rdf:rest>
                                            <rdf:Description>
                                                <rdf:type rdf:resource="http://www.w3.org/1999/02/22-rdf-syntax-ns#List"/>
                                                <rdf:first rdf:datatype="http://www.w3.org/2001/XMLSchema#string">Aslam</rdf:first>
                                                <rdf:rest>
                                                    <rdf:Description>
                                                        <rdf:type rdf:resource="http://www.w3.org/1999/02/22-rdf-syntax-ns#List"/>
                                                        <rdf:first rdf:datatype="http://www.w3.org/2001/XMLSchema#string">Bishop</rdf:first>
                                                        <rdf:rest>
                                                            <rdf:Description>
                                                                <rdf:type rdf:resource="http://www.w3.org/1999/02/22-rdf-syntax-ns#List"/>
                                                                <rdf:first rdf:datatype="http://www.w3.org/2001/XMLSchema#string">CERT C Secure Coding</rdf:first>
                                                                <rdf:rest>
                                                                    <rdf:Description>
                                                                        <rdf:type rdf:resource="http://www.w3.org/1999/02/22-rdf-syntax-ns#List"/>
                                                                        <rdf:first rdf:datatype="http://www.w3.org/2001/XMLSchema#string">CERT C++ Secure Coding</rdf:first>
                                                                        <rdf:rest>
                                                                            <rdf:Description>
                                                                                <rdf:type rdf:resource="http://www.w3.org/1999/02/22-rdf-syntax-ns#List"/>
                                                                                <rdf:first rdf:datatype="http://www.w3.org/2001/XMLSchema#string">CERT Java Secure Coding</rdf:first>
                                                                                <rdf:rest>
                                                                                    <rdf:Description>
                                                                                        <rdf:type rdf:resource="http://www.w3.org/1999/02/22-rdf-syntax-ns#List"/>
                                                                                        <rdf:first rdf:datatype="http://www.w3.org/2001/XMLSchema#string">CLASP</rdf:first>
                                                                                        <rdf:rest>
                                                                                            <rdf:Description>
                                                                                                <rdf:type rdf:resource="http://www.w3.org/1999/02/22-rdf-syntax-ns#List"/>
                                                                                                <rdf:first rdf:datatype="http://www.w3.org/2001/XMLSchema#string">Landwehr</rdf:first>
                                                                                                <rdf:rest>
                                                                                                    <rdf:Description>
                                                                                                        <rdf:type rdf:resource="http://www.w3.org/1999/02/22-rdf-syntax-ns#List"/>
                                                                                                        <rdf:first rdf:datatype="http://www.w3.org/2001/XMLSchema#string">OWASP Top Ten 2004</rdf:first>
                                                                                                        <rdf:rest>
                                                                                                            <rdf:Description>
                                                                                                                <rdf:type rdf:resource="http://www.w3.org/1999/02/22-rdf-syntax-ns#List"/>
                                                                                                                <rdf:first rdf:datatype="http://www.w3.org/2001/XMLSchema#string">OWASP Top Ten 2007</rdf:first>
                                                                                                                <rdf:rest>
                                                                                                                    <rdf:Description>
                                                                                                                        <rdf:type rdf:resource="http://www.w3.org/1999/02/22-rdf-syntax-ns#List"/>
                                                                                                                        <rdf:first rdf:datatype="http://www.w3.org/2001/XMLSchema#string">PLOVER</rdf:first>
                                                                                                                        <rdf:rest>
                                                                                                                            <rdf:Description>
                                                                                                                                <rdf:type rdf:resource="http://www.w3.org/1999/02/22-rdf-syntax-ns#List"/>
                                                                                                                                <rdf:first rdf:datatype="http://www.w3.org/2001/XMLSchema#string">Protection Analysis</rdf:first>
                                                                                                                                <rdf:rest>
                                                                                                                                    <rdf:Description>
                                                                                                                                        <rdf:type rdf:resource="http://www.w3.org/1999/02/22-rdf-syntax-ns#List"/>
                                                                                                                                        <rdf:first rdf:datatype="http://www.w3.org/2001/XMLSchema#string">RISOS</rdf:first>
                                                                                                                                        <rdf:rest>
                                                                                                                                            <rdf:Description>
                                                                                                                                                <rdf:type rdf:resource="http://www.w3.org/1999/02/22-rdf-syntax-ns#List"/>
                                                                                                                                                <rdf:first rdf:datatype="http://www.w3.org/2001/XMLSchema#string">Software Fault Patterns</rdf:first>
                                                                                                                                                <rdf:rest>
                                                                                                                                                    <rdf:Description>
                                                                                                                                                        <rdf:type rdf:resource="http://www.w3.org/1999/02/22-rdf-syntax-ns#List"/>
                                                                                                                                                        <rdf:first rdf:datatype="http://www.w3.org/2001/XMLSchema#string">WASC</rdf:first>
                                                                                                                                                        <rdf:rest>
                                                                                                                                                            <rdf:Description>
                                                                                                                                                                <rdf:type rdf:resource="http://www.w3.org/1999/02/22-rdf-syntax-ns#List"/>
                                                                                                                                                                <rdf:first rdf:datatype="http://www.w3.org/2001/XMLSchema#string">Weber, Karger, Paradkar</rdf:first>
                                                                                                                                                                <rdf:rest rdf:resource="http://www.w3.org/1999/02/22-rdf-syntax-ns#nil"/>
                                                                                                                                                            </rdf:Description>
                                                                                                                                                        </rdf:rest>
                                                                                                                                                    </rdf:Description>
                                                                                                                                                </rdf:rest>
                                                                                                                                            </rdf:Description>
                                                                                                                                        </rdf:rest>
                                                                                                                                    </rdf:Description>
                                                                                                                                </rdf:rest>
                                                                                                                            </rdf:Description>
                                                                                                                        </rdf:rest>
                                                                                                                    </rdf:Description>
                                                                                                                </rdf:rest>
                                                                                                            </rdf:Description>
                                                                                                        </rdf:rest>
                                                                                                    </rdf:Description>
                                                                                                </rdf:rest>
                                                                                            </rdf:Description>
                                                                                        </rdf:rest>
                                                                                    </rdf:Description>
                                                                                </rdf:rest>
                                                                            </rdf:Description>
                                                                        </rdf:rest>
                                                                    </rdf:Description>
                                                                </rdf:rest>
                                                            </rdf:Description>
                                                        </rdf:rest>
                                                    </rdf:Description>
                                                </rdf:rest>
                                            </rdf:Description>
                                        </rdf:rest>
                                    </rdf:Description>
                                </rdf:rest>
                            </rdf:Description>
                        </rdf:rest>
                    </rdf:Description>
                </owl:oneOf>
            </rdfs:Datatype>
        </rdfs:range>
        <rdfs:comment>Defines the taxonomy to which this weakness has a similar or equivalent entry.</rdfs:comment>
        <rdfs:label>Taxonomy Name</rdfs:label>
    </owl:DatatypeProperty>
    


    <!-- http://cwe.mitre.org/cwe#techName -->

    <owl:DatatypeProperty rdf:about="http://cwe.mitre.org/cwe#techName">
        <rdfs:domain rdf:resource="http://cwe.mitre.org/cwe#TechnologyClass"/>
        <rdfs:range>
            <rdfs:Datatype>
                <owl:oneOf>
                    <rdf:Description>
                        <rdf:type rdf:resource="http://www.w3.org/1999/02/22-rdf-syntax-ns#List"/>
                        <rdf:first rdf:datatype="http://www.w3.org/2001/XMLSchema#string">Database-Client</rdf:first>
                        <rdf:rest>
                            <rdf:Description>
                                <rdf:type rdf:resource="http://www.w3.org/1999/02/22-rdf-syntax-ns#List"/>
                                <rdf:first rdf:datatype="http://www.w3.org/2001/XMLSchema#string">Database-Server</rdf:first>
                                <rdf:rest>
                                    <rdf:Description>
                                        <rdf:type rdf:resource="http://www.w3.org/1999/02/22-rdf-syntax-ns#List"/>
                                        <rdf:first rdf:datatype="http://www.w3.org/2001/XMLSchema#string">Web-Client</rdf:first>
                                        <rdf:rest>
                                            <rdf:Description>
                                                <rdf:type rdf:resource="http://www.w3.org/1999/02/22-rdf-syntax-ns#List"/>
                                                <rdf:first rdf:datatype="http://www.w3.org/2001/XMLSchema#string">Web-Server</rdf:first>
                                                <rdf:rest rdf:resource="http://www.w3.org/1999/02/22-rdf-syntax-ns#nil"/>
                                            </rdf:Description>
                                        </rdf:rest>
                                    </rdf:Description>
                                </rdf:rest>
                            </rdf:Description>
                        </rdf:rest>
                    </rdf:Description>
                </owl:oneOf>
            </rdfs:Datatype>
        </rdfs:range>
        <rdfs:comment>Defines a technology class in which this weakness is likely to exist.</rdfs:comment>
        <rdfs:label>Technology Name</rdfs:label>
    </owl:DatatypeProperty>
    


    <!-- http://cwe.mitre.org/cwe#termDescription -->

    <owl:DatatypeProperty rdf:about="http://cwe.mitre.org/cwe#termDescription">
        <rdfs:domain rdf:resource="http://cwe.mitre.org/cwe#Term"/>
        <rdfs:range rdf:resource="http://www.w3.org/2001/XMLSchema#string"/>
        <rdfs:comment>Specifies a short description providing context to the term.</rdfs:comment>
        <rdfs:label>Term Description</rdfs:label>
    </owl:DatatypeProperty>
    


    <!-- http://cwe.mitre.org/cwe#termName -->

    <owl:DatatypeProperty rdf:about="http://cwe.mitre.org/cwe#termName">
        <rdfs:domain rdf:resource="http://cwe.mitre.org/cwe#Term"/>
        <rdfs:range rdf:resource="http://www.w3.org/2001/XMLSchema#string"/>
        <rdfs:comment>Defines the actual term. Each term should follow the same 	conventions as the entry Name attribute.</rdfs:comment>
        <rdfs:label>Term</rdfs:label>
    </owl:DatatypeProperty>
    


    <!-- http://cwe.mitre.org/cwe#text -->

    <owl:DatatypeProperty rdf:about="http://cwe.mitre.org/cwe#text">
        <rdfs:domain rdf:resource="http://cwe.mitre.org/cwe#StructuredText"/>
        <rdfs:range rdf:resource="http://www.w3.org/2001/XMLSchema#string"/>
        <rdfs:comment>Defines a paragraph of text.</rdfs:comment>
        <rdfs:label>Text</rdfs:label>
    </owl:DatatypeProperty>
    


    <!-- http://cwe.mitre.org/cwe#textTitle -->

    <owl:DatatypeProperty rdf:about="http://cwe.mitre.org/cwe#textTitle">
        <rdfs:domain rdf:resource="http://cwe.mitre.org/cwe#StructuredText"/>
        <rdfs:range rdf:resource="http://www.w3.org/2001/XMLSchema#string"/>
        <rdfs:comment>Defines a bold-faced title for a subsequent block of text.</rdfs:comment>
        <rdfs:label>Text Title</rdfs:label>
    </owl:DatatypeProperty>
    


    <!-- http://cwe.mitre.org/cwe#timeOfIntroduction -->

    <owl:DatatypeProperty rdf:about="http://cwe.mitre.org/cwe#timeOfIntroduction">
        <rdfs:domain rdf:resource="http://cwe.mitre.org/cwe#Category"/>
        <rdfs:domain rdf:resource="http://cwe.mitre.org/cwe#Weakness"/>
        <rdfs:range rdf:resource="http://www.w3.org/2001/XMLSchema#string"/>
        <rdfs:comment>Specifies the points of time in the software life cycle at which the weakness may be introduced. If there are multiple points of time at which the weakness may be introduced, then separate Introduction elements should be included for each.</rdfs:comment>
        <rdfs:label>Time of Introduction</rdfs:label>
    </owl:DatatypeProperty>
    


    <!-- http://cwe.mitre.org/cwe#viewFilter -->

    <owl:DatatypeProperty rdf:about="http://cwe.mitre.org/cwe#viewFilter">
        <rdfs:domain rdf:resource="http://cwe.mitre.org/cwe#View"/>
        <rdfs:range rdf:resource="http://www.w3.org/2001/XMLSchema#string"/>
        <rdfs:comment>Defines an XSL query for identifying 	which elements are members of an implicit slice. This should only be present for implicit slices.</rdfs:comment>
        <rdfs:label>View Filter</rdfs:label>
    </owl:DatatypeProperty>
    


    <!-- http://cwe.mitre.org/cwe#viewName -->

    <owl:DatatypeProperty rdf:about="http://cwe.mitre.org/cwe#viewName">
        <rdfs:domain rdf:resource="http://cwe.mitre.org/cwe#View"/>
        <rdfs:range rdf:resource="http://www.w3.org/2001/XMLSchema#string"/>
        <rdfs:comment>Specifies a descriptive name used to give the reader an idea of what perspective this view represents. 

All words in the name should be capitalized except for articles and prepositions unless they begin or end the name. Subsequent words in a hyphenated chain are also not capitalized.</rdfs:comment>
        <rdfs:label>Name</rdfs:label>
    </owl:DatatypeProperty>
    


    <!-- http://cwe.mitre.org/cwe#weaknessName -->

    <owl:DatatypeProperty rdf:about="http://cwe.mitre.org/cwe#weaknessName">
        <rdfs:domain rdf:resource="http://cwe.mitre.org/cwe#Weakness"/>
        <rdfs:range rdf:resource="http://www.w3.org/2001/XMLSchema#string"/>
        <rdfs:comment>Specifies a name which identifies the entry. 

The name should focus on the weakness being described in the entry and should 	avoid focusing on the attack which exploits the weakness or the consequences of exploiting the weakness. All words in the entry name should be capitalized except for articles and prepositions unless they begin or end the name. Subsequent words in a hyphenated chain are also not capitalized.</rdfs:comment>
        <rdfs:label>Name</rdfs:label>
    </owl:DatatypeProperty>
    


    <!-- 
    ///////////////////////////////////////////////////////////////////////////////////////
    //
    // Classes
    //
    ///////////////////////////////////////////////////////////////////////////////////////
     -->

    


    <!-- http://capec.mitre.org/capec#AttackPattern -->

    <owl:Class rdf:about="http://capec.mitre.org/capec#AttackPattern"/>
    


    <!-- http://cpe.mitre.org/cpe#CPE -->

    <owl:Class rdf:about="http://cpe.mitre.org/cpe#CPE"/>
    


    <!-- http://cwe.mitre.org/cwe#ArchitectureParadigm -->

    <owl:Class rdf:about="http://cwe.mitre.org/cwe#ArchitectureParadigm">
        <rdfs:subClassOf>
            <owl:Restriction>
                <owl:onProperty rdf:resource="http://cwe.mitre.org/cwe#paradigmName"/>
                <owl:cardinality rdf:datatype="http://www.w3.org/2001/XMLSchema#nonNegativeInteger">1</owl:cardinality>
            </owl:Restriction>
        </rdfs:subClassOf>
        <rdfs:subClassOf>
            <owl:Restriction>
                <owl:onProperty rdf:resource="http://cwe.mitre.org/cwe#prevalence"/>
                <owl:maxCardinality rdf:datatype="http://www.w3.org/2001/XMLSchema#nonNegativeInteger">1</owl:maxCardinality>
            </owl:Restriction>
        </rdfs:subClassOf>
        <rdfs:comment>Characterizes a single Architectural Paradigm in which this entry may exist and with what frequency in the specified paradigm.</rdfs:comment>
        <rdfs:isDefinedBy rdf:resource="http://cwe.mitre.org/cwe"/>
        <rdfs:label>Architecture Paradigm</rdfs:label>
    </owl:Class>
    


    <!-- http://cwe.mitre.org/cwe#Audience -->

    <owl:Class rdf:about="http://cwe.mitre.org/cwe#Audience">
        <rdfs:subClassOf>
            <owl:Restriction>
                <owl:onProperty rdf:resource="http://cwe.mitre.org/cwe#stakeholder"/>
                <owl:cardinality rdf:datatype="http://www.w3.org/2001/XMLSchema#nonNegativeInteger">1</owl:cardinality>
            </owl:Restriction>
        </rdfs:subClassOf>
        <rdfs:subClassOf>
            <owl:Restriction>
                <owl:onProperty rdf:resource="http://cwe.mitre.org/cwe#stakeholderDescription"/>
                <owl:maxCardinality rdf:datatype="http://www.w3.org/2001/XMLSchema#nonNegativeInteger">1</owl:maxCardinality>
            </owl:Restriction>
        </rdfs:subClassOf>
        <rdfs:comment>Characterizes a target audience or group for this view.</rdfs:comment>
        <rdfs:isDefinedBy rdf:resource="http://cwe.mitre.org/cwe"/>
        <rdfs:label>Audience</rdfs:label>
    </owl:Class>
    


    <!-- http://cwe.mitre.org/cwe#BackgroundDetail -->

    <owl:Class rdf:about="http://cwe.mitre.org/cwe#BackgroundDetail">
        <rdfs:subClassOf rdf:resource="http://cwe.mitre.org/cwe#StructuredText"/>
        <rdfs:comment>Defines background information regarding the entry or any technologies that are related to it, where the background information is not related to the nature of the weakness itself. It should be filled out where appropriate.</rdfs:comment>
        <rdfs:isDefinedBy rdf:resource="http://cwe.mitre.org/cwe"/>
        <rdfs:label>Background Detail</rdfs:label>
    </owl:Class>
    


    <!-- http://cwe.mitre.org/cwe#BlackBoxDefinition -->

    <owl:Class rdf:about="http://cwe.mitre.org/cwe#BlackBoxDefinition">
        <rdfs:subClassOf rdf:resource="http://cwe.mitre.org/cwe#StructuredText"/>
        <rdfs:comment>Defines one or more Black Box Definitions, each of which describes the weakness from an external perspective, 	meaning that the view includes no knowledge of how the software is processing data other than what can be inferred from observing the software&apos;s behavior.</rdfs:comment>
        <rdfs:isDefinedBy rdf:resource="http://cwe.mitre.org/cwe"/>
        <rdfs:label>Black Box Definition</rdfs:label>
    </owl:Class>
    


    <!-- http://cwe.mitre.org/cwe#Block -->

    <owl:Class rdf:about="http://cwe.mitre.org/cwe#Block">
        <rdfs:subClassOf rdf:resource="http://cwe.mitre.org/cwe#StructuredText"/>
        <rdfs:comment>Defines a  Block of structured text</rdfs:comment>
        <rdfs:isDefinedBy rdf:resource="http://cwe.mitre.org/cwe"/>
        <rdfs:label>Block</rdfs:label>
    </owl:Class>
    


    <!-- http://cwe.mitre.org/cwe#Category -->

    <owl:Class rdf:about="http://cwe.mitre.org/cwe#Category">
        <rdfs:subClassOf>
            <owl:Restriction>
                <owl:onProperty rdf:resource="http://cwe.mitre.org/cwe#extendedDescription"/>
                <owl:maxCardinality rdf:datatype="http://www.w3.org/2001/XMLSchema#nonNegativeInteger">1</owl:maxCardinality>
            </owl:Restriction>
        </rdfs:subClassOf>
        <rdfs:subClassOf>
            <owl:Restriction>
                <owl:onProperty rdf:resource="http://cwe.mitre.org/cwe#categoryName"/>
                <owl:cardinality rdf:datatype="http://www.w3.org/2001/XMLSchema#nonNegativeInteger">1</owl:cardinality>
            </owl:Restriction>
        </rdfs:subClassOf>
        <rdfs:subClassOf>
            <owl:Restriction>
                <owl:onProperty rdf:resource="http://cwe.mitre.org/cwe#descriptionSummary"/>
                <owl:cardinality rdf:datatype="http://www.w3.org/2001/XMLSchema#nonNegativeInteger">1</owl:cardinality>
            </owl:Restriction>
        </rdfs:subClassOf>
        <rdfs:subClassOf>
            <owl:Restriction>
                <owl:onProperty rdf:resource="http://cwe.mitre.org/cwe#formattedIdentifier"/>
                <owl:cardinality rdf:datatype="http://www.w3.org/2001/XMLSchema#nonNegativeInteger">1</owl:cardinality>
            </owl:Restriction>
        </rdfs:subClassOf>
        <rdfs:subClassOf>
            <owl:Restriction>
                <owl:onProperty rdf:resource="http://cwe.mitre.org/cwe#id"/>
                <owl:cardinality rdf:datatype="http://www.w3.org/2001/XMLSchema#nonNegativeInteger">1</owl:cardinality>
            </owl:Restriction>
        </rdfs:subClassOf>
        <rdfs:subClassOf>
            <owl:Restriction>
                <owl:onProperty rdf:resource="http://cwe.mitre.org/cwe#weaknessName"/>
                <owl:cardinality rdf:datatype="http://www.w3.org/2001/XMLSchema#nonNegativeInteger">1</owl:cardinality>
            </owl:Restriction>
        </rdfs:subClassOf>
        <rdfs:subClassOf>
            <owl:Restriction>
                <owl:onProperty rdf:resource="http://cwe.mitre.org/cwe#likelihood"/>
                <owl:maxCardinality rdf:datatype="http://www.w3.org/2001/XMLSchema#nonNegativeInteger">1</owl:maxCardinality>
            </owl:Restriction>
        </rdfs:subClassOf>
        <rdfs:subClassOf>
            <owl:Restriction>
                <owl:onProperty rdf:resource="http://cwe.mitre.org/cwe#status"/>
                <owl:maxCardinality rdf:datatype="http://www.w3.org/2001/XMLSchema#nonNegativeInteger">1</owl:maxCardinality>
            </owl:Restriction>
        </rdfs:subClassOf>
        <rdfs:subClassOf>
            <owl:Restriction>
                <owl:onProperty rdf:resource="http://cwe.mitre.org/cwe#timeOfIntroduction"/>
                <owl:maxCardinality rdf:datatype="http://www.w3.org/2001/XMLSchema#nonNegativeInteger">1</owl:maxCardinality>
            </owl:Restriction>
        </rdfs:subClassOf>
        <rdfs:comment>Characterizes a category entity that represents a collection of weaknesses based on a common attribute, such as CWE-310 Cryptographic Issues or CWE-355 User Interface Security Issues.</rdfs:comment>
        <rdfs:isDefinedBy rdf:resource="http://cwe.mitre.org/cwe"/>
        <rdfs:label>Weakness Category</rdfs:label>
    </owl:Class>
    


    <!-- http://cwe.mitre.org/cwe#CompoundElement -->

    <owl:Class rdf:about="http://cwe.mitre.org/cwe#CompoundElement">
        <rdfs:subClassOf>
            <owl:Restriction>
                <owl:onProperty rdf:resource="http://cwe.mitre.org/cwe#extendedDescription"/>
                <owl:maxCardinality rdf:datatype="http://www.w3.org/2001/XMLSchema#nonNegativeInteger">1</owl:maxCardinality>
            </owl:Restriction>
        </rdfs:subClassOf>
        <rdfs:subClassOf>
            <owl:Restriction>
                <owl:onProperty rdf:resource="http://cwe.mitre.org/cwe#abstraction"/>
                <owl:cardinality rdf:datatype="http://www.w3.org/2001/XMLSchema#nonNegativeInteger">1</owl:cardinality>
            </owl:Restriction>
        </rdfs:subClassOf>
        <rdfs:subClassOf>
            <owl:Restriction>
                <owl:onProperty rdf:resource="http://cwe.mitre.org/cwe#compoundElementName"/>
                <owl:cardinality rdf:datatype="http://www.w3.org/2001/XMLSchema#nonNegativeInteger">1</owl:cardinality>
            </owl:Restriction>
        </rdfs:subClassOf>
        <rdfs:subClassOf>
            <owl:Restriction>
                <owl:onProperty rdf:resource="http://cwe.mitre.org/cwe#compoundElementStructure"/>
                <owl:cardinality rdf:datatype="http://www.w3.org/2001/XMLSchema#nonNegativeInteger">1</owl:cardinality>
            </owl:Restriction>
        </rdfs:subClassOf>
        <rdfs:subClassOf>
            <owl:Restriction>
                <owl:onProperty rdf:resource="http://cwe.mitre.org/cwe#descriptionSummary"/>
                <owl:cardinality rdf:datatype="http://www.w3.org/2001/XMLSchema#nonNegativeInteger">1</owl:cardinality>
            </owl:Restriction>
        </rdfs:subClassOf>
        <rdfs:subClassOf>
            <owl:Restriction>
                <owl:onProperty rdf:resource="http://cwe.mitre.org/cwe#formattedIdentifier"/>
                <owl:cardinality rdf:datatype="http://www.w3.org/2001/XMLSchema#nonNegativeInteger">1</owl:cardinality>
            </owl:Restriction>
        </rdfs:subClassOf>
        <rdfs:subClassOf>
            <owl:Restriction>
                <owl:onProperty rdf:resource="http://cwe.mitre.org/cwe#id"/>
                <owl:cardinality rdf:datatype="http://www.w3.org/2001/XMLSchema#nonNegativeInteger">1</owl:cardinality>
            </owl:Restriction>
        </rdfs:subClassOf>
        <rdfs:subClassOf>
            <owl:Restriction>
                <owl:onProperty rdf:resource="http://cwe.mitre.org/cwe#status"/>
                <owl:cardinality rdf:datatype="http://www.w3.org/2001/XMLSchema#nonNegativeInteger">1</owl:cardinality>
            </owl:Restriction>
        </rdfs:subClassOf>
        <rdfs:subClassOf>
            <owl:Restriction>
                <owl:onProperty rdf:resource="http://cwe.mitre.org/cwe#causalNature"/>
                <owl:maxCardinality rdf:datatype="http://www.w3.org/2001/XMLSchema#nonNegativeInteger">1</owl:maxCardinality>
            </owl:Restriction>
        </rdfs:subClassOf>
        <rdfs:subClassOf>
            <owl:Restriction>
                <owl:onProperty rdf:resource="http://cwe.mitre.org/cwe#likelihood"/>
                <owl:maxCardinality rdf:datatype="http://www.w3.org/2001/XMLSchema#nonNegativeInteger">1</owl:maxCardinality>
            </owl:Restriction>
        </rdfs:subClassOf>
        <rdfs:comment>Characterizes a meaningful aggregation of several weaknesses, as in a chain like CWE-690: CWE-252 Unchecked Return Value can result in CWE-476 NULL Pointer Dereference or as in a composite like CWE-352 Cross-Site Request Forgery.</rdfs:comment>
        <rdfs:isDefinedBy rdf:resource="http://cwe.mitre.org/cwe"/>
        <rdfs:label>CompoundElement</rdfs:label>
    </owl:Class>
    


    <!-- http://cwe.mitre.org/cwe#Consequence -->

    <owl:Class rdf:about="http://cwe.mitre.org/cwe#Consequence">
        <rdfs:subClassOf>
            <owl:Restriction>
                <owl:onProperty rdf:resource="http://cwe.mitre.org/cwe#consequenceNote"/>
                <owl:maxCardinality rdf:datatype="http://www.w3.org/2001/XMLSchema#nonNegativeInteger">1</owl:maxCardinality>
            </owl:Restriction>
        </rdfs:subClassOf>
        <rdfs:subClassOf>
            <owl:Restriction>
                <owl:onProperty rdf:resource="http://cwe.mitre.org/cwe#consequenceId"/>
                <owl:cardinality rdf:datatype="http://www.w3.org/2001/XMLSchema#nonNegativeInteger">1</owl:cardinality>
            </owl:Restriction>
        </rdfs:subClassOf>
        <rdfs:subClassOf>
            <owl:Restriction>
                <owl:onProperty rdf:resource="http://cwe.mitre.org/cwe#relativeId"/>
                <owl:cardinality rdf:datatype="http://www.w3.org/2001/XMLSchema#nonNegativeInteger">1</owl:cardinality>
            </owl:Restriction>
        </rdfs:subClassOf>
        <rdfs:comment>Characterizes a consequence that may be associated with the Weakness, Category, View, or Compound Element.</rdfs:comment>
        <rdfs:isDefinedBy rdf:resource="http://cwe.mitre.org/cwe"/>
        <rdfs:label>Consequence</rdfs:label>
    </owl:Class>
    


    <!-- http://cwe.mitre.org/cwe#DemonstrativeExample -->

    <owl:Class rdf:about="http://cwe.mitre.org/cwe#DemonstrativeExample">
        <rdfs:subClassOf>
            <owl:Restriction>
                <owl:onProperty rdf:resource="http://cwe.mitre.org/cwe#demoExampleId"/>
                <owl:cardinality rdf:datatype="http://www.w3.org/2001/XMLSchema#nonNegativeInteger">1</owl:cardinality>
            </owl:Restriction>
        </rdfs:subClassOf>
        <rdfs:subClassOf>
            <owl:Restriction>
                <owl:onProperty rdf:resource="http://cwe.mitre.org/cwe#introText"/>
                <owl:cardinality rdf:datatype="http://www.w3.org/2001/XMLSchema#nonNegativeInteger">1</owl:cardinality>
            </owl:Restriction>
        </rdfs:subClassOf>
        <rdfs:subClassOf>
            <owl:Restriction>
                <owl:onProperty rdf:resource="http://cwe.mitre.org/cwe#relativeId"/>
                <owl:cardinality rdf:datatype="http://www.w3.org/2001/XMLSchema#nonNegativeInteger">1</owl:cardinality>
            </owl:Restriction>
        </rdfs:subClassOf>
        <rdfs:subClassOf>
            <owl:Restriction>
                <owl:onProperty rdf:resource="http://cwe.mitre.org/cwe#exampleBody"/>
                <owl:maxCardinality rdf:datatype="http://www.w3.org/2001/XMLSchema#nonNegativeInteger">1</owl:maxCardinality>
            </owl:Restriction>
        </rdfs:subClassOf>
        <rdfs:comment>Characterizes a Demonstrative Example which should contain an example illustrating the problem being described in this weakness.</rdfs:comment>
        <rdfs:isDefinedBy rdf:resource="http://cwe.mitre.org/cwe"/>
        <rdfs:label>Demonstrative Example</rdfs:label>
    </owl:Class>
    


    <!-- http://cwe.mitre.org/cwe#DetectionMethod -->

    <owl:Class rdf:about="http://cwe.mitre.org/cwe#DetectionMethod">
        <rdfs:subClassOf>
            <owl:Restriction>
                <owl:onProperty rdf:resource="http://cwe.mitre.org/cwe#methodName"/>
                <owl:cardinality rdf:datatype="http://www.w3.org/2001/XMLSchema#nonNegativeInteger">1</owl:cardinality>
            </owl:Restriction>
        </rdfs:subClassOf>
        <rdfs:subClassOf>
            <owl:Restriction>
                <owl:onProperty rdf:resource="http://cwe.mitre.org/cwe#detectionMethodId"/>
                <owl:maxCardinality rdf:datatype="http://www.w3.org/2001/XMLSchema#nonNegativeInteger">1</owl:maxCardinality>
            </owl:Restriction>
        </rdfs:subClassOf>
        <rdfs:comment>Characterizes  information on different techniques that can be used to detect a weakness, including their strengths and limitations.  This should be filled out for some weakness classes and bases.</rdfs:comment>
        <rdfs:isDefinedBy rdf:resource="http://cwe.mitre.org/cwe"/>
        <rdfs:label>Detection Method</rdfs:label>
    </owl:Class>
    


    <!-- http://cwe.mitre.org/cwe#Environment -->

    <owl:Class rdf:about="http://cwe.mitre.org/cwe#Environment">
        <rdfs:subClassOf>
            <owl:Restriction>
                <owl:onProperty rdf:resource="http://cwe.mitre.org/cwe#environmentName"/>
                <owl:cardinality rdf:datatype="http://www.w3.org/2001/XMLSchema#nonNegativeInteger">1</owl:cardinality>
            </owl:Restriction>
        </rdfs:subClassOf>
        <rdfs:subClassOf>
            <owl:Restriction>
                <owl:onProperty rdf:resource="http://cwe.mitre.org/cwe#prevalence"/>
                <owl:maxCardinality rdf:datatype="http://www.w3.org/2001/XMLSchema#nonNegativeInteger">1</owl:maxCardinality>
            </owl:Restriction>
        </rdfs:subClassOf>
        <rdfs:comment>Characterizes a single Environment in which this entry may exist and with what frequency in the specified environment.</rdfs:comment>
        <rdfs:isDefinedBy rdf:resource="http://cwe.mitre.org/cwe"/>
        <rdfs:label>Environment</rdfs:label>
    </owl:Class>
    


    <!-- http://cwe.mitre.org/cwe#ExploitationFactor -->

    <owl:Class rdf:about="http://cwe.mitre.org/cwe#ExploitationFactor">
        <rdfs:subClassOf rdf:resource="http://cwe.mitre.org/cwe#StructuredText"/>
        <rdfs:comment>Defines a condition or factor tha could increase the likelihood of exploit for this weakness.</rdfs:comment>
        <rdfs:isDefinedBy rdf:resource="http://cwe.mitre.org/cwe"/>
        <rdfs:label>Exploitation Factor</rdfs:label>
    </owl:Class>
    


    <!-- http://cwe.mitre.org/cwe#HardwareArchitecture -->

    <owl:Class rdf:about="http://cwe.mitre.org/cwe#HardwareArchitecture">
        <rdfs:subClassOf>
            <owl:Restriction>
                <owl:onProperty rdf:resource="http://cwe.mitre.org/cwe#hardwareArchitectureClassDescription"/>
                <owl:maxCardinality rdf:datatype="http://www.w3.org/2001/XMLSchema#nonNegativeInteger">1</owl:maxCardinality>
            </owl:Restriction>
        </rdfs:subClassOf>
        <rdfs:subClassOf>
            <owl:Restriction>
                <owl:onProperty rdf:resource="http://cwe.mitre.org/cwe#hardwareArchitectureName"/>
                <owl:maxCardinality rdf:datatype="http://www.w3.org/2001/XMLSchema#nonNegativeInteger">1</owl:maxCardinality>
            </owl:Restriction>
        </rdfs:subClassOf>
        <rdfs:subClassOf>
            <owl:Restriction>
                <owl:onProperty rdf:resource="http://cwe.mitre.org/cwe#prevalence"/>
                <owl:maxCardinality rdf:datatype="http://www.w3.org/2001/XMLSchema#nonNegativeInteger">1</owl:maxCardinality>
            </owl:Restriction>
        </rdfs:subClassOf>
        <rdfs:comment>Characterizes a hardware achitecture on which this entry may exist and with what frequency on the specified architecture.</rdfs:comment>
        <rdfs:isDefinedBy rdf:resource="http://cwe.mitre.org/cwe"/>
        <rdfs:label>Hardware Architecture</rdfs:label>
    </owl:Class>
    


    <!-- http://cwe.mitre.org/cwe#HistoryRecord -->

    <owl:Class rdf:about="http://cwe.mitre.org/cwe#HistoryRecord">
        <rdfs:subClassOf>
            <owl:Restriction>
                <owl:onProperty rdf:resource="http://cwe.mitre.org/cwe#authorOrganization"/>
                <owl:maxCardinality rdf:datatype="http://www.w3.org/2001/XMLSchema#nonNegativeInteger">1</owl:maxCardinality>
            </owl:Restriction>
        </rdfs:subClassOf>
        <rdfs:subClassOf>
            <owl:Restriction>
                <owl:onProperty rdf:resource="http://cwe.mitre.org/cwe#entryType"/>
                <owl:cardinality rdf:datatype="http://www.w3.org/2001/XMLSchema#nonNegativeInteger">1</owl:cardinality>
            </owl:Restriction>
        </rdfs:subClassOf>
        <rdfs:subClassOf>
            <owl:Restriction>
                <owl:onProperty rdf:resource="http://cwe.mitre.org/cwe#relativeId"/>
                <owl:cardinality rdf:datatype="http://www.w3.org/2001/XMLSchema#nonNegativeInteger">1</owl:cardinality>
            </owl:Restriction>
        </rdfs:subClassOf>
        <rdfs:subClassOf>
            <owl:Restriction>
                <owl:onProperty rdf:resource="http://cwe.mitre.org/cwe#authorName"/>
                <owl:maxCardinality rdf:datatype="http://www.w3.org/2001/XMLSchema#nonNegativeInteger">1</owl:maxCardinality>
            </owl:Restriction>
        </rdfs:subClassOf>
        <rdfs:subClassOf>
            <owl:Restriction>
                <owl:onProperty rdf:resource="http://cwe.mitre.org/cwe#authorOrganizationName"/>
                <owl:maxCardinality rdf:datatype="http://www.w3.org/2001/XMLSchema#nonNegativeInteger">1</owl:maxCardinality>
            </owl:Restriction>
        </rdfs:subClassOf>
        <rdfs:subClassOf>
            <owl:Restriction>
                <owl:onProperty rdf:resource="http://cwe.mitre.org/cwe#contributionMode"/>
                <owl:maxCardinality rdf:datatype="http://www.w3.org/2001/XMLSchema#nonNegativeInteger">1</owl:maxCardinality>
            </owl:Restriction>
        </rdfs:subClassOf>
        <rdfs:subClassOf>
            <owl:Restriction>
                <owl:onProperty rdf:resource="http://cwe.mitre.org/cwe#entryDate"/>
                <owl:maxCardinality rdf:datatype="http://www.w3.org/2001/XMLSchema#nonNegativeInteger">1</owl:maxCardinality>
            </owl:Restriction>
        </rdfs:subClassOf>
        <rdfs:subClassOf>
            <owl:Restriction>
                <owl:onProperty rdf:resource="http://cwe.mitre.org/cwe#modificationImportance"/>
                <owl:maxCardinality rdf:datatype="http://www.w3.org/2001/XMLSchema#nonNegativeInteger">1</owl:maxCardinality>
            </owl:Restriction>
        </rdfs:subClassOf>
        <rdfs:subClassOf>
            <owl:Restriction>
                <owl:onProperty rdf:resource="http://cwe.mitre.org/cwe#modificationSource"/>
                <owl:maxCardinality rdf:datatype="http://www.w3.org/2001/XMLSchema#nonNegativeInteger">1</owl:maxCardinality>
            </owl:Restriction>
        </rdfs:subClassOf>
        <rdfs:subClassOf>
            <owl:Restriction>
                <owl:onProperty rdf:resource="http://cwe.mitre.org/cwe#submissionSource"/>
                <owl:maxCardinality rdf:datatype="http://www.w3.org/2001/XMLSchema#nonNegativeInteger">1</owl:maxCardinality>
            </owl:Restriction>
        </rdfs:subClassOf>
        <rdfs:comment>Characterizes a record of history to keep track of the author of the weakness entry and anyone who has made modifications to the content. This provides a means of contacting the authors and modifiers for clarifying ambiguities,  merging overlapping contributions, etc. This should be filled out for all entries.</rdfs:comment>
        <rdfs:isDefinedBy rdf:resource="http://cwe.mitre.org/cwe"/>
        <rdfs:label>Content History</rdfs:label>
    </owl:Class>
    


    <!-- http://cwe.mitre.org/cwe#IntroductionMode -->

    <owl:Class rdf:about="http://cwe.mitre.org/cwe#IntroductionMode">
        <rdfs:subClassOf rdf:resource="http://cwe.mitre.org/cwe#StructuredText"/>
        <rdfs:comment>Defines the mode in which the weakness can be introduced.</rdfs:comment>
        <rdfs:isDefinedBy rdf:resource="http://cwe.mitre.org/cwe"/>
        <rdfs:label>Introduction Mode</rdfs:label>
    </owl:Class>
    


    <!-- http://cwe.mitre.org/cwe#Mitigation -->

    <owl:Class rdf:about="http://cwe.mitre.org/cwe#Mitigation">
        <rdfs:subClassOf>
            <owl:Restriction>
                <owl:onProperty rdf:resource="http://cwe.mitre.org/cwe#relativeId"/>
                <owl:cardinality rdf:datatype="http://www.w3.org/2001/XMLSchema#nonNegativeInteger">1</owl:cardinality>
            </owl:Restriction>
        </rdfs:subClassOf>
        <rdfs:subClassOf>
            <owl:Restriction>
                <owl:onProperty rdf:resource="http://cwe.mitre.org/cwe#mitigationEffectiveness"/>
                <owl:maxCardinality rdf:datatype="http://www.w3.org/2001/XMLSchema#nonNegativeInteger">1</owl:maxCardinality>
            </owl:Restriction>
        </rdfs:subClassOf>
        <rdfs:subClassOf>
            <owl:Restriction>
                <owl:onProperty rdf:resource="http://cwe.mitre.org/cwe#mitigationId"/>
                <owl:maxCardinality rdf:datatype="http://www.w3.org/2001/XMLSchema#nonNegativeInteger">1</owl:maxCardinality>
            </owl:Restriction>
        </rdfs:subClassOf>
        <rdfs:comment>Characterizes a method for mitigating a weakness.</rdfs:comment>
        <rdfs:isDefinedBy rdf:resource="http://cwe.mitre.org/cwe"/>
        <rdfs:label>Mitigation</rdfs:label>
    </owl:Class>
    


    <!-- http://cwe.mitre.org/cwe#Note -->

    <owl:Class rdf:about="http://cwe.mitre.org/cwe#Note">
        <rdfs:subClassOf rdf:resource="http://cwe.mitre.org/cwe#StructuredText"/>
        <rdfs:subClassOf>
            <owl:Restriction>
                <owl:onProperty rdf:resource="http://cwe.mitre.org/cwe#noteType"/>
                <owl:cardinality rdf:datatype="http://www.w3.org/2001/XMLSchema#nonNegativeInteger">1</owl:cardinality>
            </owl:Restriction>
        </rdfs:subClassOf>
        <rdfs:comment>Defines one or more Relationship Note elements, which each contain details regarding the relationships between CWE entries.</rdfs:comment>
        <rdfs:isDefinedBy rdf:resource="http://cwe.mitre.org/cwe"/>
        <rdfs:label>Note</rdfs:label>
    </owl:Class>
    


    <!-- http://cwe.mitre.org/cwe#ObservedExample -->

    <owl:Class rdf:about="http://cwe.mitre.org/cwe#ObservedExample">
        <rdfs:subClassOf>
            <owl:Restriction>
                <owl:onProperty rdf:resource="http://cwe.mitre.org/cwe#relativeId"/>
                <owl:cardinality rdf:datatype="http://www.w3.org/2001/XMLSchema#nonNegativeInteger">1</owl:cardinality>
            </owl:Restriction>
        </rdfs:subClassOf>
        <rdfs:comment>Characterizes an observed instance of this weakness in the real-world; typically this will be a CVE reference.  If the reference identifier is for a CVE reference, the cveReference should also be completed. This element should be filled out for as many entries as possible.</rdfs:comment>
        <rdfs:isDefinedBy rdf:resource="http://cwe.mitre.org/cwe"/>
        <rdfs:label>Observed Example</rdfs:label>
    </owl:Class>
    


    <!-- http://cwe.mitre.org/cwe#OperatingSystem -->

    <owl:Class rdf:about="http://cwe.mitre.org/cwe#OperatingSystem">
        <rdfs:subClassOf>
            <owl:Restriction>
                <owl:onProperty rdf:resource="http://cwe.mitre.org/cwe#osClass"/>
                <owl:maxCardinality rdf:datatype="http://www.w3.org/2001/XMLSchema#nonNegativeInteger">1</owl:maxCardinality>
            </owl:Restriction>
        </rdfs:subClassOf>
        <rdfs:subClassOf>
            <owl:Restriction>
                <owl:onProperty rdf:resource="http://cwe.mitre.org/cwe#osName"/>
                <owl:maxCardinality rdf:datatype="http://www.w3.org/2001/XMLSchema#nonNegativeInteger">1</owl:maxCardinality>
            </owl:Restriction>
        </rdfs:subClassOf>
        <rdfs:subClassOf>
            <owl:Restriction>
                <owl:onProperty rdf:resource="http://cwe.mitre.org/cwe#prevalence"/>
                <owl:maxCardinality rdf:datatype="http://www.w3.org/2001/XMLSchema#nonNegativeInteger">1</owl:maxCardinality>
            </owl:Restriction>
        </rdfs:subClassOf>
        <rdfs:comment>Characterizes an Operating System in which this entry may exist and with what frequency on the specified OS.</rdfs:comment>
        <rdfs:isDefinedBy rdf:resource="http://cwe.mitre.org/cwe"/>
        <rdfs:label>Operating System</rdfs:label>
    </owl:Class>
    


    <!-- http://cwe.mitre.org/cwe#ProgrammingLanguage -->

    <owl:Class rdf:about="http://cwe.mitre.org/cwe#ProgrammingLanguage">
        <rdfs:subClassOf>
            <owl:Restriction>
                <owl:onProperty rdf:resource="http://cwe.mitre.org/cwe#langName"/>
                <owl:cardinality rdf:datatype="http://www.w3.org/2001/XMLSchema#nonNegativeInteger">1</owl:cardinality>
            </owl:Restriction>
        </rdfs:subClassOf>
        <rdfs:subClassOf>
            <owl:Restriction>
                <owl:onProperty rdf:resource="http://cwe.mitre.org/cwe#langClass"/>
                <owl:maxCardinality rdf:datatype="http://www.w3.org/2001/XMLSchema#nonNegativeInteger">1</owl:maxCardinality>
            </owl:Restriction>
        </rdfs:subClassOf>
        <rdfs:subClassOf>
            <owl:Restriction>
                <owl:onProperty rdf:resource="http://cwe.mitre.org/cwe#prevalence"/>
                <owl:maxCardinality rdf:datatype="http://www.w3.org/2001/XMLSchema#nonNegativeInteger">1</owl:maxCardinality>
            </owl:Restriction>
        </rdfs:subClassOf>
        <rdfs:comment>Characterizes a Programming Language in which this weakness may exist. 

Do not fill this in if a specific Programming Language was specified.</rdfs:comment>
        <rdfs:isDefinedBy rdf:resource="http://cwe.mitre.org/cwe"/>
        <rdfs:label>Programming Language</rdfs:label>
    </owl:Class>
    


    <!-- http://cwe.mitre.org/cwe#Reference -->

    <owl:Class rdf:about="http://cwe.mitre.org/cwe#Reference">
        <rdfs:subClassOf>
            <owl:Restriction>
                <owl:onProperty rdf:resource="http://cwe.mitre.org/cwe#localReferenceId"/>
                <owl:cardinality rdf:datatype="http://www.w3.org/2001/XMLSchema#nonNegativeInteger">1</owl:cardinality>
            </owl:Restriction>
        </rdfs:subClassOf>
        <rdfs:subClassOf>
            <owl:Restriction>
                <owl:onProperty rdf:resource="http://cwe.mitre.org/cwe#referenceDate"/>
                <owl:maxCardinality rdf:datatype="http://www.w3.org/2001/XMLSchema#nonNegativeInteger">1</owl:maxCardinality>
            </owl:Restriction>
        </rdfs:subClassOf>
        <rdfs:subClassOf>
            <owl:Restriction>
                <owl:onProperty rdf:resource="http://cwe.mitre.org/cwe#referenceEdition"/>
                <owl:maxCardinality rdf:datatype="http://www.w3.org/2001/XMLSchema#nonNegativeInteger">1</owl:maxCardinality>
            </owl:Restriction>
        </rdfs:subClassOf>
        <rdfs:subClassOf>
            <owl:Restriction>
                <owl:onProperty rdf:resource="http://cwe.mitre.org/cwe#referenceId"/>
                <owl:maxCardinality rdf:datatype="http://www.w3.org/2001/XMLSchema#nonNegativeInteger">1</owl:maxCardinality>
            </owl:Restriction>
        </rdfs:subClassOf>
        <rdfs:subClassOf>
            <owl:Restriction>
                <owl:onProperty rdf:resource="http://cwe.mitre.org/cwe#referenceLink"/>
                <owl:maxCardinality rdf:datatype="http://www.w3.org/2001/XMLSchema#nonNegativeInteger">1</owl:maxCardinality>
            </owl:Restriction>
        </rdfs:subClassOf>
        <rdfs:subClassOf>
            <owl:Restriction>
                <owl:onProperty rdf:resource="http://cwe.mitre.org/cwe#referencePubDate"/>
                <owl:maxCardinality rdf:datatype="http://www.w3.org/2001/XMLSchema#nonNegativeInteger">1</owl:maxCardinality>
            </owl:Restriction>
        </rdfs:subClassOf>
        <rdfs:subClassOf>
            <owl:Restriction>
                <owl:onProperty rdf:resource="http://cwe.mitre.org/cwe#referencePublication"/>
                <owl:maxCardinality rdf:datatype="http://www.w3.org/2001/XMLSchema#nonNegativeInteger">1</owl:maxCardinality>
            </owl:Restriction>
        </rdfs:subClassOf>
        <rdfs:subClassOf>
            <owl:Restriction>
                <owl:onProperty rdf:resource="http://cwe.mitre.org/cwe#referencePublisherName"/>
                <owl:maxCardinality rdf:datatype="http://www.w3.org/2001/XMLSchema#nonNegativeInteger">1</owl:maxCardinality>
            </owl:Restriction>
        </rdfs:subClassOf>
        <rdfs:subClassOf>
            <owl:Restriction>
                <owl:onProperty rdf:resource="http://cwe.mitre.org/cwe#referenceSection"/>
                <owl:maxCardinality rdf:datatype="http://www.w3.org/2001/XMLSchema#nonNegativeInteger">1</owl:maxCardinality>
            </owl:Restriction>
        </rdfs:subClassOf>
        <rdfs:subClassOf>
            <owl:Restriction>
                <owl:onProperty rdf:resource="http://cwe.mitre.org/cwe#referenceTitle"/>
                <owl:maxCardinality rdf:datatype="http://www.w3.org/2001/XMLSchema#nonNegativeInteger">1</owl:maxCardinality>
            </owl:Restriction>
        </rdfs:subClassOf>
        <rdfs:comment>Characterizes  a source from which more information and deeper insight can be obtained, such as a 	research paper or an excerpt from a publication.</rdfs:comment>
        <rdfs:isDefinedBy rdf:resource="http://cwe.mitre.org/cwe"/>
        <rdfs:label>Reference</rdfs:label>
    </owl:Class>
    


    <!-- http://cwe.mitre.org/cwe#RelationshipStatement -->

    <owl:Class rdf:about="http://cwe.mitre.org/cwe#RelationshipStatement">
        <rdfs:subClassOf rdf:resource="http://www.w3.org/1999/02/22-rdf-syntax-ns#Statement"/>
        <rdfs:subClassOf>
            <owl:Restriction>
                <owl:onProperty rdf:resource="http://cwe.mitre.org/cwe#chains"/>
                <owl:cardinality rdf:datatype="http://www.w3.org/2001/XMLSchema#nonNegativeInteger">1</owl:cardinality>
            </owl:Restriction>
        </rdfs:subClassOf>
        <rdfs:subClassOf>
            <owl:Restriction>
                <owl:onProperty rdf:resource="http://cwe.mitre.org/cwe#views"/>
                <owl:cardinality rdf:datatype="http://www.w3.org/2001/XMLSchema#nonNegativeInteger">1</owl:cardinality>
            </owl:Restriction>
        </rdfs:subClassOf>
        <rdfs:subClassOf>
            <owl:Restriction>
                <owl:onProperty rdf:resource="http://cwe.mitre.org/cwe#form"/>
                <owl:cardinality rdf:datatype="http://www.w3.org/2001/XMLSchema#nonNegativeInteger">1</owl:cardinality>
            </owl:Restriction>
        </rdfs:subClassOf>
        <rdfs:subClassOf>
            <owl:Restriction>
                <owl:onProperty rdf:resource="http://cwe.mitre.org/cwe#relationshipNature"/>
                <owl:cardinality rdf:datatype="http://www.w3.org/2001/XMLSchema#nonNegativeInteger">1</owl:cardinality>
            </owl:Restriction>
        </rdfs:subClassOf>
        <rdfs:comment>Characterizes an association between this structure, whether it is a Weakness, Category, or Compound_Element and another structure. The relationship also identifies the views under which the relationship is applicable.</rdfs:comment>
        <rdfs:isDefinedBy rdf:resource="http://cwe.mitre.org/cwe"/>
        <rdfs:label>Relationship</rdfs:label>
    </owl:Class>
    


    <!-- http://cwe.mitre.org/cwe#ResearchGap -->

    <owl:Class rdf:about="http://cwe.mitre.org/cwe#ResearchGap">
        <rdfs:subClassOf rdf:resource="http://cwe.mitre.org/cwe#StructuredText"/>
        <rdfs:comment>Defines a potential opportunity for the vulnerability research community to conduct further exploration of issues related to this weakness. It is intended to highlight parts of 	CWE that have not received sufficient attention from researchers. This 	should be filled out where appropriate for weaknesses and categories.</rdfs:comment>
        <rdfs:isDefinedBy rdf:resource="http://cwe.mitre.org/cwe"/>
        <rdfs:label>Research Gap</rdfs:label>
    </owl:Class>
    


    <!-- http://cwe.mitre.org/cwe#StructuredText -->

    <owl:Class rdf:about="http://cwe.mitre.org/cwe#StructuredText">
        <rdfs:subClassOf>
            <owl:Restriction>
                <owl:onProperty rdf:resource="http://cwe.mitre.org/cwe#text"/>
                <owl:cardinality rdf:datatype="http://www.w3.org/2001/XMLSchema#nonNegativeInteger">1</owl:cardinality>
            </owl:Restriction>
        </rdfs:subClassOf>
        <rdfs:subClassOf>
            <owl:Restriction>
                <owl:onProperty rdf:resource="http://cwe.mitre.org/cwe#textTitle"/>
                <owl:cardinality rdf:datatype="http://www.w3.org/2001/XMLSchema#nonNegativeInteger">1</owl:cardinality>
            </owl:Restriction>
        </rdfs:subClassOf>
        <rdfs:comment>Characterizes a structured description text that can include a title, text, comments, code examples, and blocks of text.</rdfs:comment>
        <rdfs:isDefinedBy rdf:resource="http://cwe.mitre.org/cwe"/>
        <rdfs:label>Structured Text</rdfs:label>
    </owl:Class>
    


    <!-- http://cwe.mitre.org/cwe#TaxonomyMapping -->

    <owl:Class rdf:about="http://cwe.mitre.org/cwe#TaxonomyMapping">
        <rdfs:subClassOf>
            <owl:Restriction>
                <owl:onProperty rdf:resource="http://cwe.mitre.org/cwe#relativeId"/>
                <owl:cardinality rdf:datatype="http://www.w3.org/2001/XMLSchema#nonNegativeInteger">1</owl:cardinality>
            </owl:Restriction>
        </rdfs:subClassOf>
        <rdfs:subClassOf>
            <owl:Restriction>
                <owl:onProperty rdf:resource="http://cwe.mitre.org/cwe#taxonomyName"/>
                <owl:cardinality rdf:datatype="http://www.w3.org/2001/XMLSchema#nonNegativeInteger">1</owl:cardinality>
            </owl:Restriction>
        </rdfs:subClassOf>
        <rdfs:subClassOf>
            <owl:Restriction>
                <owl:onProperty rdf:resource="http://cwe.mitre.org/cwe#mappedNodeId"/>
                <owl:maxCardinality rdf:datatype="http://www.w3.org/2001/XMLSchema#nonNegativeInteger">1</owl:maxCardinality>
            </owl:Restriction>
        </rdfs:subClassOf>
        <rdfs:subClassOf>
            <owl:Restriction>
                <owl:onProperty rdf:resource="http://cwe.mitre.org/cwe#mappedNodeName"/>
                <owl:maxCardinality rdf:datatype="http://www.w3.org/2001/XMLSchema#nonNegativeInteger">1</owl:maxCardinality>
            </owl:Restriction>
        </rdfs:subClassOf>
        <rdfs:subClassOf>
            <owl:Restriction>
                <owl:onProperty rdf:resource="http://cwe.mitre.org/cwe#mappingFit"/>
                <owl:maxCardinality rdf:datatype="http://www.w3.org/2001/XMLSchema#nonNegativeInteger">1</owl:maxCardinality>
            </owl:Restriction>
        </rdfs:subClassOf>
        <rdfs:comment>Characterizes mappings to nodes of other taxonomies that are similar in meaning to this node.  

Although this may sound similar to Source  Taxonomy, Source Taxonomy is designed to provide a history and pedigree for the entry, whereas Taxonomy Mapping allows similar nodes in other collections to be identified as matching concepts with this weakness. For example, Taxonomy Mapping should be used to map the CWE entries to their OWASP Top 10 equivalents.</rdfs:comment>
        <rdfs:isDefinedBy rdf:resource="http://cwe.mitre.org/cwe"/>
        <rdfs:label>TaxonomyMapping</rdfs:label>
    </owl:Class>
    


    <!-- http://cwe.mitre.org/cwe#TechnicalImpact -->

    <owl:Class rdf:about="http://cwe.mitre.org/cwe#TechnicalImpact">
        <rdfs:subClassOf>
            <owl:Restriction>
                <owl:onProperty rdf:resource="http://cwe.mitre.org/cwe#impactType"/>
                <owl:cardinality rdf:datatype="http://www.w3.org/2001/XMLSchema#nonNegativeInteger">1</owl:cardinality>
            </owl:Restriction>
        </rdfs:subClassOf>
        <rdfs:subClassOf>
            <owl:Restriction>
                <owl:onProperty rdf:resource="http://cwe.mitre.org/cwe#impactDescription"/>
                <owl:maxCardinality rdf:datatype="http://www.w3.org/2001/XMLSchema#nonNegativeInteger">1</owl:maxCardinality>
            </owl:Restriction>
        </rdfs:subClassOf>
        <rdfs:subClassOf>
            <owl:Restriction>
                <owl:onProperty rdf:resource="http://cwe.mitre.org/cwe#likelihood"/>
                <owl:maxCardinality rdf:datatype="http://www.w3.org/2001/XMLSchema#nonNegativeInteger">1</owl:maxCardinality>
            </owl:Restriction>
        </rdfs:subClassOf>
        <rdfs:comment>Characterizes a technical impact that can arise if an attacker attempts to exploit this weakness.</rdfs:comment>
        <rdfs:isDefinedBy rdf:resource="http://cwe.mitre.org/cwe"/>
        <rdfs:label>Technical Impact</rdfs:label>
    </owl:Class>
    


    <!-- http://cwe.mitre.org/cwe#TechnologyClass -->

    <owl:Class rdf:about="http://cwe.mitre.org/cwe#TechnologyClass">
        <rdfs:subClassOf>
            <owl:Restriction>
                <owl:onProperty rdf:resource="http://cwe.mitre.org/cwe#techName"/>
                <owl:cardinality rdf:datatype="http://www.w3.org/2001/XMLSchema#nonNegativeInteger">1</owl:cardinality>
            </owl:Restriction>
        </rdfs:subClassOf>
        <rdfs:subClassOf>
            <owl:Restriction>
                <owl:onProperty rdf:resource="http://cwe.mitre.org/cwe#prevalence"/>
                <owl:maxCardinality rdf:datatype="http://www.w3.org/2001/XMLSchema#nonNegativeInteger">1</owl:maxCardinality>
            </owl:Restriction>
        </rdfs:subClassOf>
        <rdfs:comment>Characterizes a class of technology in which this entry may exist and with what frequency in the specified class.</rdfs:comment>
        <rdfs:isDefinedBy rdf:resource="http://cwe.mitre.org/cwe"/>
        <rdfs:label>Technoloy Class</rdfs:label>
    </owl:Class>
    


    <!-- http://cwe.mitre.org/cwe#Term -->

    <owl:Class rdf:about="http://cwe.mitre.org/cwe#Term">
        <rdfs:subClassOf>
            <owl:Restriction>
                <owl:onProperty rdf:resource="http://cwe.mitre.org/cwe#termName"/>
                <owl:cardinality rdf:datatype="http://www.w3.org/2001/XMLSchema#nonNegativeInteger">1</owl:cardinality>
            </owl:Restriction>
        </rdfs:subClassOf>
        <rdfs:subClassOf>
            <owl:Restriction>
                <owl:onProperty rdf:resource="http://cwe.mitre.org/cwe#termDescription"/>
                <owl:maxCardinality rdf:datatype="http://www.w3.org/2001/XMLSchema#nonNegativeInteger">1</owl:maxCardinality>
            </owl:Restriction>
        </rdfs:subClassOf>
        <rdfs:comment>Defines term by which an entity may be known and a description to explain the context in which the term may be relevant. For example, CWE-181 Incorrect Behavior Order: Validate Before Filter, has the alternate terms value &quot;Validate-before-cleanse&quot;.</rdfs:comment>
        <rdfs:isDefinedBy rdf:resource="http://cwe.mitre.org/cwe"/>
        <rdfs:label>Term</rdfs:label>
    </owl:Class>
    


    <!-- http://cwe.mitre.org/cwe#View -->

    <owl:Class rdf:about="http://cwe.mitre.org/cwe#View">
        <rdfs:subClassOf>
            <owl:Restriction>
                <owl:onProperty rdf:resource="http://cwe.mitre.org/cwe#objective"/>
                <owl:cardinality rdf:datatype="http://www.w3.org/2001/XMLSchema#nonNegativeInteger">1</owl:cardinality>
            </owl:Restriction>
        </rdfs:subClassOf>
        <rdfs:subClassOf>
            <owl:Restriction>
                <owl:onProperty rdf:resource="http://cwe.mitre.org/cwe#formattedIdentifier"/>
                <owl:cardinality rdf:datatype="http://www.w3.org/2001/XMLSchema#nonNegativeInteger">1</owl:cardinality>
            </owl:Restriction>
        </rdfs:subClassOf>
        <rdfs:subClassOf>
            <owl:Restriction>
                <owl:onProperty rdf:resource="http://cwe.mitre.org/cwe#id"/>
                <owl:cardinality rdf:datatype="http://www.w3.org/2001/XMLSchema#nonNegativeInteger">1</owl:cardinality>
            </owl:Restriction>
        </rdfs:subClassOf>
        <rdfs:subClassOf>
            <owl:Restriction>
                <owl:onProperty rdf:resource="http://cwe.mitre.org/cwe#status"/>
                <owl:cardinality rdf:datatype="http://www.w3.org/2001/XMLSchema#nonNegativeInteger">1</owl:cardinality>
            </owl:Restriction>
        </rdfs:subClassOf>
        <rdfs:subClassOf>
            <owl:Restriction>
                <owl:onProperty rdf:resource="http://cwe.mitre.org/cwe#structureType"/>
                <owl:cardinality rdf:datatype="http://www.w3.org/2001/XMLSchema#nonNegativeInteger">1</owl:cardinality>
            </owl:Restriction>
        </rdfs:subClassOf>
        <rdfs:subClassOf>
            <owl:Restriction>
                <owl:onProperty rdf:resource="http://cwe.mitre.org/cwe#viewName"/>
                <owl:cardinality rdf:datatype="http://www.w3.org/2001/XMLSchema#nonNegativeInteger">1</owl:cardinality>
            </owl:Restriction>
        </rdfs:subClassOf>
        <rdfs:subClassOf>
            <owl:Restriction>
                <owl:onProperty rdf:resource="http://cwe.mitre.org/cwe#weaknessName"/>
                <owl:cardinality rdf:datatype="http://www.w3.org/2001/XMLSchema#nonNegativeInteger">1</owl:cardinality>
            </owl:Restriction>
        </rdfs:subClassOf>
        <rdfs:comment>Characterizes a perspective with which one might look at the weaknesses in CWE. CWE-699 Development Concepts, CWE-1000 Research Concepts and are two examples of Views.</rdfs:comment>
        <rdfs:isDefinedBy rdf:resource="http://cwe.mitre.org/cwe"/>
        <rdfs:label>View</rdfs:label>
    </owl:Class>
    


    <!-- http://cwe.mitre.org/cwe#ViewObjective -->

    <owl:Class rdf:about="http://cwe.mitre.org/cwe#ViewObjective">
        <rdfs:subClassOf rdf:resource="http://cwe.mitre.org/cwe#StructuredText"/>
        <rdfs:comment>Defines the perspective from which this View is constructed.</rdfs:comment>
        <rdfs:isDefinedBy rdf:resource="http://cwe.mitre.org/cwe"/>
        <rdfs:label>View Objective</rdfs:label>
    </owl:Class>
    


    <!-- http://cwe.mitre.org/cwe#Weakness -->

    <owl:Class rdf:about="http://cwe.mitre.org/cwe#Weakness">
        <rdfs:subClassOf>
            <owl:Restriction>
                <owl:onProperty rdf:resource="http://cwe.mitre.org/cwe#extendedDescription"/>
                <owl:maxCardinality rdf:datatype="http://www.w3.org/2001/XMLSchema#nonNegativeInteger">1</owl:maxCardinality>
            </owl:Restriction>
        </rdfs:subClassOf>
        <rdfs:subClassOf>
            <owl:Restriction>
                <owl:onProperty rdf:resource="http://cwe.mitre.org/cwe#abstraction"/>
                <owl:cardinality rdf:datatype="http://www.w3.org/2001/XMLSchema#nonNegativeInteger">1</owl:cardinality>
            </owl:Restriction>
        </rdfs:subClassOf>
        <rdfs:subClassOf>
            <owl:Restriction>
                <owl:onProperty rdf:resource="http://cwe.mitre.org/cwe#descriptionSummary"/>
                <owl:cardinality rdf:datatype="http://www.w3.org/2001/XMLSchema#nonNegativeInteger">1</owl:cardinality>
            </owl:Restriction>
        </rdfs:subClassOf>
        <rdfs:subClassOf>
            <owl:Restriction>
                <owl:onProperty rdf:resource="http://cwe.mitre.org/cwe#dictionaryLink"/>
                <owl:cardinality rdf:datatype="http://www.w3.org/2001/XMLSchema#nonNegativeInteger">1</owl:cardinality>
            </owl:Restriction>
        </rdfs:subClassOf>
        <rdfs:subClassOf>
            <owl:Restriction>
                <owl:onProperty rdf:resource="http://cwe.mitre.org/cwe#formattedIdentifier"/>
                <owl:cardinality rdf:datatype="http://www.w3.org/2001/XMLSchema#nonNegativeInteger">1</owl:cardinality>
            </owl:Restriction>
        </rdfs:subClassOf>
        <rdfs:subClassOf>
            <owl:Restriction>
                <owl:onProperty rdf:resource="http://cwe.mitre.org/cwe#id"/>
                <owl:cardinality rdf:datatype="http://www.w3.org/2001/XMLSchema#nonNegativeInteger">1</owl:cardinality>
            </owl:Restriction>
        </rdfs:subClassOf>
        <rdfs:subClassOf>
            <owl:Restriction>
                <owl:onProperty rdf:resource="http://cwe.mitre.org/cwe#status"/>
                <owl:cardinality rdf:datatype="http://www.w3.org/2001/XMLSchema#nonNegativeInteger">1</owl:cardinality>
            </owl:Restriction>
        </rdfs:subClassOf>
        <rdfs:subClassOf>
            <owl:Restriction>
                <owl:onProperty rdf:resource="http://cwe.mitre.org/cwe#weaknessName"/>
                <owl:cardinality rdf:datatype="http://www.w3.org/2001/XMLSchema#nonNegativeInteger">1</owl:cardinality>
            </owl:Restriction>
        </rdfs:subClassOf>
        <rdfs:comment>Characterizes an actual weakness entry in the Common Weakness Enumeration dictionary</rdfs:comment>
        <rdfs:isDefinedBy rdf:resource="http://cwe.mitre.org/cwe"/>
        <rdfs:label>Weakness</rdfs:label>
    </owl:Class>
    


    <!-- http://cwe.mitre.org/cwe#WeaknessCatalog -->

    <owl:Class rdf:about="http://cwe.mitre.org/cwe#WeaknessCatalog">
        <rdfs:subClassOf rdf:resource="http://org.semanticweb.owlapi/error#Error1"/>
        <rdfs:subClassOf rdf:resource="http://scap.nist.gov/scap_core#Catalog"/>
        <rdfs:comment>Characterizes a collection of software security issues (flaws, faults, bugs, vulnerabilities, weaknesses, etc).  The name used by CWE is usually &quot;CWE&quot;.  However, if this collection is a subset of CWE, then a more appropriate name should be used.</rdfs:comment>
        <rdfs:isDefinedBy rdf:resource="http://cwe.mitre.org/cwe"/>
        <rdfs:label>Weakness Catalog</rdfs:label>
    </owl:Class>
    


    <!-- http://cwe.mitre.org/cwe#WeaknessOrdinality -->

    <owl:Class rdf:about="http://cwe.mitre.org/cwe#WeaknessOrdinality">
        <rdfs:subClassOf>
            <owl:Restriction>
                <owl:onProperty rdf:resource="http://cwe.mitre.org/cwe#ordinality"/>
                <owl:cardinality rdf:datatype="http://www.w3.org/2001/XMLSchema#nonNegativeInteger">1</owl:cardinality>
            </owl:Restriction>
        </rdfs:subClassOf>
        <rdfs:subClassOf>
            <owl:Restriction>
                <owl:onProperty rdf:resource="http://cwe.mitre.org/cwe#ordinalityDescription"/>
                <owl:maxCardinality rdf:datatype="http://www.w3.org/2001/XMLSchema#nonNegativeInteger">1</owl:maxCardinality>
            </owl:Restriction>
        </rdfs:subClassOf>
        <rdfs:comment>Characterizes a Weakness Ordinality and indicates when this entry is primary - where the weakness exists independent of other weaknesses, or when this entry might be resultant - where the weakness is typically related to the presence of some other weaknesses.</rdfs:comment>
        <rdfs:isDefinedBy rdf:resource="http://cwe.mitre.org/cwe"/>
        <rdfs:label>Weakness Ordinality</rdfs:label>
    </owl:Class>
    


    <!-- http://cwe.mitre.org/cwe#WhiteBoxDefinition -->

    <owl:Class rdf:about="http://cwe.mitre.org/cwe#WhiteBoxDefinition">
        <rdfs:subClassOf rdf:resource="http://cwe.mitre.org/cwe#StructuredText"/>
        <rdfs:comment>Defines the weakness from a white box perspective, meaning that the view includes the knowledge of control flow, data flow, and all other inner workings of the software in which the weakness exists.</rdfs:comment>
        <rdfs:isDefinedBy rdf:resource="http://cwe.mitre.org/cwe"/>
        <rdfs:label>WhiteBox Definition</rdfs:label>
    </owl:Class>
    


    <!-- http://nvd.nist.gov/cve#Vulnerability -->

    <owl:Class rdf:about="http://nvd.nist.gov/cve#Vulnerability"/>
    


    <!-- http://org.semanticweb.owlapi/error#Error1 -->

    <owl:Class rdf:about="http://org.semanticweb.owlapi/error#Error1"/>
    


    <!-- http://scap.nist.gov/scap_core#Catalog -->

    <owl:Class rdf:about="http://scap.nist.gov/scap_core#Catalog"/>
    


    <!-- http://www.oasis-open.org/ciq_xpil#Organization -->

    <owl:Class rdf:about="http://www.oasis-open.org/ciq_xpil#Organization"/>
    


    <!-- http://www.oasis-open.org/ciq_xpil#Party -->

    <owl:Class rdf:about="http://www.oasis-open.org/ciq_xpil#Party"/>
    


    <!-- http://www.oasis-open.org/ciq_xpil#Person -->

    <owl:Class rdf:about="http://www.oasis-open.org/ciq_xpil#Person"/>
    


    <!-- http://www.w3.org/1999/02/22-rdf-syntax-ns#Statement -->

    <owl:Class rdf:about="http://www.w3.org/1999/02/22-rdf-syntax-ns#Statement"/>
    <rdf:Description>
        <owl:maxCardinality rdf:datatype="http://www.w3.org/2001/XMLSchema#nonNegativeInteger">1</owl:maxCardinality>
    </rdf:Description>
</rdf:RDF>



<!-- Generated by the OWL API (version 4.2.6.20160910-2108) https://github.com/owlcs/owlapi -->

