<?xml version="1.0"?>
<rdf:RDF xmlns="http://capec.mitre.org/capec#"
     xml:base="http://capec.mitre.org/capec"
     xmlns:capec="http://capec.mitre.org/capec#"
     xmlns:rdf="http://www.w3.org/1999/02/22-rdf-syntax-ns#"
     xmlns:owl="http://www.w3.org/2002/07/owl#"
     xmlns:xml="http://www.w3.org/XML/1998/namespace"
     xmlns:xsd="http://www.w3.org/2001/XMLSchema#"
     xmlns:rdfs="http://www.w3.org/2000/01/rdf-schema#">
    <owl:Ontology rdf:about="http://capec.mitre.org/capec">
        <owl:imports rdf:resource="http://cybox.mitre.org/objects/URI"/>
        <owl:imports rdf:resource="http://scap.nist.gov/scap_core"/>
        <owl:imports rdf:resource="http://cybox.mitre.org/cybox_core"/>
        <owl:imports rdf:resource="http://cybox.mitre.org/objects/NetworkProtocol"/>
        <owl:imports rdf:resource="http://nvd.nist.gov/cve"/>
        <rdfs:comment>This ontology provides a vocabulary and representation for the Common Attack Pattern Enumeration and Classification (CAPEC) which provides a publicly available, community-developed list of common attack patterns along with a comprehensive schema and classification taxonomy. Attack patterns are descriptions of common methods for exploiting software systems. They derive from the concept of design patterns applied in a destructive rather than constructive context and are generated from in-depth analysis of specific real-world exploit examples.

Copyright (c) 2014, DaedaFusion, LLC.  All rights reserved.</rdfs:comment>
        <owl:versionInfo rdf:datatype="http://www.w3.org/2001/XMLSchema#string">v1.0.0-001</owl:versionInfo>
        <rdfs:label>Common Attack Pattern Enumeration and Classification (CAPEC) Ontology</rdfs:label>
    </owl:Ontology>
    


    <!-- 
    ///////////////////////////////////////////////////////////////////////////////////////
    //
    // Annotation properties
    //
    ///////////////////////////////////////////////////////////////////////////////////////
     -->

    


    <!-- http://www.w3.org/2002/07/owl#maxCardinality -->

    <owl:AnnotationProperty rdf:about="http://www.w3.org/2002/07/owl#maxCardinality"/>
    


    <!-- 
    ///////////////////////////////////////////////////////////////////////////////////////
    //
    // Datatypes
    //
    ///////////////////////////////////////////////////////////////////////////////////////
     -->

    


    <!-- http://capec.mitre.org/capec#structuredText -->

    <rdfs:Datatype rdf:about="http://capec.mitre.org/capec#structuredText"/>
    


    <!-- http://www.w3.org/2001/XMLSchema#date -->

    <rdfs:Datatype rdf:about="http://www.w3.org/2001/XMLSchema#date"/>
    


    <!-- http://www.w3.org/2001/XMLSchema#gYear -->

    <rdfs:Datatype rdf:about="http://www.w3.org/2001/XMLSchema#gYear"/>
    


    <!-- 
    ///////////////////////////////////////////////////////////////////////////////////////
    //
    // Object Properties
    //
    ///////////////////////////////////////////////////////////////////////////////////////
     -->

    


    <!-- http://capec.mitre.org/capec#alternateTerms -->

    <owl:ObjectProperty rdf:about="http://capec.mitre.org/capec#alternateTerms">
        <rdfs:domain rdf:resource="http://capec.mitre.org/capec#AttackPattern"/>
        <rdfs:domain rdf:resource="http://capec.mitre.org/capec#Category"/>
        <rdfs:domain rdf:resource="http://capec.mitre.org/capec#CompoundElement"/>
        <rdfs:domain rdf:resource="http://capec.mitre.org/capec#View"/>
        <rdfs:range rdf:resource="http://capec.mitre.org/capec#Term"/>
        <rdfs:comment>Specifies zero or more Alternate Terms, each ofwhich contains other names used to describe this attack pattern.</rdfs:comment>
        <rdfs:label>Alternate Terms</rdfs:label>
    </owl:ObjectProperty>
    


    <!-- http://capec.mitre.org/capec#attackExecutionFlow -->

    <owl:ObjectProperty rdf:about="http://capec.mitre.org/capec#attackExecutionFlow">
        <rdfs:domain rdf:resource="http://capec.mitre.org/capec#AttackPattern"/>
        <rdfs:range rdf:resource="http://capec.mitre.org/capec#AttackPhase"/>
        <rdfs:comment>Specifies a detailed description of the attack including the chain of actions taken by the attacker. More comprehensive descriptions could include relevant attack trees and/or exploit graphs to more clearly elaborate this type of attack.</rdfs:comment>
        <rdfs:label>Attack Execution Flow</rdfs:label>
    </owl:ObjectProperty>
    


    <!-- http://capec.mitre.org/capec#attackMotivationConsequences -->

    <owl:ObjectProperty rdf:about="http://capec.mitre.org/capec#attackMotivationConsequences">
        <rdfs:domain rdf:resource="http://capec.mitre.org/capec#AttackPattern"/>
        <rdfs:domain rdf:resource="http://capec.mitre.org/capec#Category"/>
        <rdfs:range rdf:resource="http://capec.mitre.org/capec#Consequence"/>
        <rdfs:comment>Specifies what the attacker is trying to achieve by using this attack.  This is not the end business/mission goal of the attack within the target context but rather the specific technical result desired that 	could be leveraged to achieve the end business/mission objective. This information is useful for aligning attack patterns to threat models and for determining which attack patterns are relevant for a given context.</rdfs:comment>
        <rdfs:label>Attack Motivation Consequences</rdfs:label>
    </owl:ObjectProperty>
    


    <!-- http://capec.mitre.org/capec#attackPatterns -->

    <owl:ObjectProperty rdf:about="http://capec.mitre.org/capec#attackPatterns">
        <rdfs:domain rdf:resource="http://capec.mitre.org/capec#AttackPatternCatalog"/>
        <rdfs:range rdf:resource="http://capec.mitre.org/capec#AttackPattern"/>
        <rdfs:comment>Specifies a collection of attack patterns</rdfs:comment>
        <rdfs:label>Attack Patterns</rdfs:label>
    </owl:ObjectProperty>
    


    <!-- http://capec.mitre.org/capec#attackSteps -->

    <owl:ObjectProperty rdf:about="http://capec.mitre.org/capec#attackSteps">
        <rdfs:domain rdf:resource="http://capec.mitre.org/capec#AttackPhase"/>
        <rdfs:range rdf:resource="http://capec.mitre.org/capec#AttackStep"/>
        <rdfs:comment>Specifies the steps of the attack pattern</rdfs:comment>
        <rdfs:label>Attack Steps</rdfs:label>
    </owl:ObjectProperty>
    


    <!-- http://capec.mitre.org/capec#attackTechniques -->

    <owl:ObjectProperty rdf:about="http://capec.mitre.org/capec#attackTechniques">
        <rdfs:domain rdf:resource="http://capec.mitre.org/capec#AttackStep"/>
        <rdfs:range rdf:resource="http://capec.mitre.org/capec#AttackStepTechnique"/>
        <rdfs:comment>Specifies various techniques that the attacker can use to achieve the attack step’s goal. For example, an attacker may use tools such as WebScarab and Tamper Data in the experimentation phase of a SQL Injection attack pattern. The techniques include references to environments, because not all techniques work in all environments</rdfs:comment>
        <rdfs:label>Techniques</rdfs:label>
    </owl:ObjectProperty>
    


    <!-- http://capec.mitre.org/capec#attackerKnowledgeRequired -->

    <owl:ObjectProperty rdf:about="http://capec.mitre.org/capec#attackerKnowledgeRequired">
        <rdfs:domain rdf:resource="http://capec.mitre.org/capec#AttackPattern"/>
        <rdfs:domain rdf:resource="http://capec.mitre.org/capec#Category"/>
        <rdfs:range rdf:resource="http://capec.mitre.org/capec#Knowlege"/>
        <rdfs:comment>Specifies  the level of skills or specific knowledge required by an attacker to execute this type of attack.</rdfs:comment>
        <rdfs:label>Attacker Skill or Knowledge Required</rdfs:label>
    </owl:ObjectProperty>
    


    <!-- http://capec.mitre.org/capec#audience -->

    <owl:ObjectProperty rdf:about="http://capec.mitre.org/capec#audience">
        <rdfs:domain rdf:resource="http://capec.mitre.org/capec#View"/>
        <rdfs:range rdf:resource="http://capec.mitre.org/capec#Audience"/>
        <rdfs:comment>Specifies a reference to the targeted audiences or groups for this view.</rdfs:comment>
        <rdfs:label>Audience</rdfs:label>
    </owl:ObjectProperty>
    


    <!-- http://capec.mitre.org/capec#author -->

    <owl:ObjectProperty rdf:about="http://capec.mitre.org/capec#author">
        <rdfs:domain rdf:resource="http://capec.mitre.org/capec#HistoryRecord"/>
        <rdfs:range>
            <owl:Class>
                <owl:unionOf rdf:parseType="Collection">
                    <rdf:Description rdf:about="http://www.oasis-open.org/ciq_xpil#Organization"/>
                    <rdf:Description rdf:about="http://www.oasis-open.org/ciq_xpil#Party"/>
                    <rdf:Description rdf:about="http://www.oasis-open.org/ciq_xpil#Person"/>
                </owl:unionOf>
            </owl:Class>
        </rdfs:range>
        <rdfs:comment>Specifies the author</rdfs:comment>
        <rdfs:label>Author</rdfs:label>
    </owl:ObjectProperty>
    


    <!-- http://capec.mitre.org/capec#authorOrganization -->

    <owl:ObjectProperty rdf:about="http://capec.mitre.org/capec#authorOrganization">
        <rdfs:domain rdf:resource="http://capec.mitre.org/capec#HistoryRecord"/>
        <rdfs:range rdf:resource="http://www.oasis-open.org/ciq_xpil#Organization"/>
        <rdfs:comment>Specifies the author&apos;s organization</rdfs:comment>
        <rdfs:label>Author&apos;s Organization</rdfs:label>
    </owl:ObjectProperty>
    


    <!-- http://capec.mitre.org/capec#categories -->

    <owl:ObjectProperty rdf:about="http://capec.mitre.org/capec#categories">
        <rdfs:domain rdf:resource="http://capec.mitre.org/capec#AttackPatternCatalog"/>
        <rdfs:range rdf:resource="http://capec.mitre.org/capec#Category"/>
        <rdfs:comment>Specifies  a collection of attack patterns sharing a common attribute. The shared attribute may any number of things.</rdfs:comment>
        <rdfs:label>Categories</rdfs:label>
    </owl:ObjectProperty>
    


    <!-- http://capec.mitre.org/capec#commonAttackSteps -->

    <owl:ObjectProperty rdf:about="http://capec.mitre.org/capec#commonAttackSteps">
        <rdfs:domain rdf:resource="http://capec.mitre.org/capec#AttackPatternCatalog"/>
        <rdfs:range rdf:resource="http://capec.mitre.org/capec#AttackStep"/>
        <rdfs:comment>Specifies a collection of attack steps</rdfs:comment>
        <rdfs:label>Common Attack Steps</rdfs:label>
    </owl:ObjectProperty>
    


    <!-- http://capec.mitre.org/capec#comonAttackSurfaces -->

    <owl:ObjectProperty rdf:about="http://capec.mitre.org/capec#comonAttackSurfaces">
        <rdfs:domain rdf:resource="http://capec.mitre.org/capec#AttackPatternCatalog"/>
        <rdfs:range rdf:resource="http://capec.mitre.org/capec#TargetAttackSurfaceDescription"/>
        <rdfs:comment>Specifies a collection of common attack surfaces</rdfs:comment>
        <rdfs:label>Comon Attack Surfaces</rdfs:label>
    </owl:ObjectProperty>
    


    <!-- http://capec.mitre.org/capec#compoundElements -->

    <owl:ObjectProperty rdf:about="http://capec.mitre.org/capec#compoundElements">
        <rdfs:domain rdf:resource="http://capec.mitre.org/capec#AttackPatternCatalog"/>
        <rdfs:range rdf:resource="http://capec.mitre.org/capec#CompoundElement"/>
        <rdfs:comment>Specifies a meaningful aggregation of several attack patterns.</rdfs:comment>
        <rdfs:label>Compound Elements</rdfs:label>
    </owl:ObjectProperty>
    


    <!-- http://capec.mitre.org/capec#consequenceTechnicalImpact -->

    <owl:ObjectProperty rdf:about="http://capec.mitre.org/capec#consequenceTechnicalImpact">
        <rdfs:domain rdf:resource="http://capec.mitre.org/capec#Consequence"/>
        <rdfs:range rdf:resource="http://capec.mitre.org/capec#TechnicalImpact"/>
        <rdfs:comment>Specifies the technical impacts that can result from successful execution of this attack pattern.</rdfs:comment>
        <rdfs:label>Technical Impact</rdfs:label>
    </owl:ObjectProperty>
    


    <!-- http://capec.mitre.org/capec#contentHistory -->

    <owl:ObjectProperty rdf:about="http://capec.mitre.org/capec#contentHistory">
        <rdfs:domain rdf:resource="http://capec.mitre.org/capec#AttackPattern"/>
        <rdfs:domain rdf:resource="http://capec.mitre.org/capec#Category"/>
        <rdfs:domain rdf:resource="http://capec.mitre.org/capec#CompoundElement"/>
        <rdfs:domain rdf:resource="http://capec.mitre.org/capec#View"/>
        <rdfs:range rdf:resource="http://capec.mitre.org/capec#HistoryRecord"/>
        <rdfs:comment>Specifies one or more history records  used to keep track of the author of the attack pattern entry and anyone who has made modifications to the content. This provides a means of contacting the authors and  modifiers for clarifying ambiguities, merging overlapping contributions, etc. This should be filled out for all entries.</rdfs:comment>
        <rdfs:label>Content History</rdfs:label>
    </owl:ObjectProperty>
    


    <!-- http://capec.mitre.org/capec#environments -->

    <owl:ObjectProperty rdf:about="http://capec.mitre.org/capec#environments">
        <rdfs:domain rdf:resource="http://capec.mitre.org/capec#AttackPatternCatalog"/>
        <rdfs:domain rdf:resource="http://capec.mitre.org/capec#AttackStepTechnique"/>
        <rdfs:domain rdf:resource="http://capec.mitre.org/capec#SusceptabiltyIndicator"/>
        <rdfs:range rdf:resource="http://capec.mitre.org/capec#Environment"/>
        <rdfs:comment>Specifies the environments where an attack step technique is applicable.</rdfs:comment>
        <rdfs:label>Environments</rdfs:label>
    </owl:ObjectProperty>
    


    <!-- http://capec.mitre.org/capec#exampleInstances -->

    <owl:ObjectProperty rdf:about="http://capec.mitre.org/capec#exampleInstances">
        <rdfs:domain rdf:resource="http://capec.mitre.org/capec#AttackPattern"/>
        <rdfs:range rdf:resource="http://capec.mitre.org/capec#ExampleInstance"/>
        <rdfs:comment>Specifies explanatory examples or demonstrative exploit instances of this attack, which are intended to help the reader understand the nature, context and variability of the attack in more practical and concrete terms.</rdfs:comment>
        <rdfs:label>Examples Instances</rdfs:label>
    </owl:ObjectProperty>
    


    <!-- http://capec.mitre.org/capec#indicatorWarningOfAttack -->

    <owl:ObjectProperty rdf:about="http://capec.mitre.org/capec#indicatorWarningOfAttack">
        <rdfs:domain rdf:resource="http://capec.mitre.org/capec#AttackPattern"/>
        <rdfs:range rdf:resource="http://capec.mitre.org/capec#IndicatorWarning"/>
        <rdfs:comment>Specifies one or more indicator warning of attack. Indicator warning of attack describes activities, events,	conditions or behaviors that may indicate that an attack of this type is imminent, in progress or has occurred.</rdfs:comment>
        <rdfs:label>Indicator-Wwarning of Attack</rdfs:label>
    </owl:ObjectProperty>
    


    <!-- http://capec.mitre.org/capec#indicators -->

    <owl:ObjectProperty rdf:about="http://capec.mitre.org/capec#indicators">
        <rdfs:domain rdf:resource="http://capec.mitre.org/capec#AttackStep"/>
        <rdfs:range rdf:resource="http://capec.mitre.org/capec#SusceptabiltyIndicator"/>
        <rdfs:comment>Specifies indicators that the application may or may not be susceptible to the given attack step (not necessarily the pattern as a whole).</rdfs:comment>
        <rdfs:label>Indicators</rdfs:label>
    </owl:ObjectProperty>
    


    <!-- http://capec.mitre.org/capec#leveragedAttackPatterns -->

    <owl:ObjectProperty rdf:about="http://capec.mitre.org/capec#leveragedAttackPatterns">
        <rdfs:domain rdf:resource="http://capec.mitre.org/capec#AttackStepTechnique"/>
        <rdfs:range rdf:resource="http://capec.mitre.org/capec#AttackPattern"/>
        <rdfs:comment>Specifies any attack patterns which are leveraged</rdfs:comment>
        <rdfs:label>Leveraged Attack Patterns</rdfs:label>
    </owl:ObjectProperty>
    


    <!-- http://capec.mitre.org/capec#nonPrimaryViews -->

    <owl:ObjectProperty rdf:about="http://capec.mitre.org/capec#nonPrimaryViews">
        <rdfs:domain rdf:resource="http://capec.mitre.org/capec#RelationshipStatement"/>
        <rdfs:range rdf:resource="http://capec.mitre.org/capec#View"/>
        <rdfs:comment>Specifies a list of the individual Views to which this relationship pertains.</rdfs:comment>
        <rdfs:label>Non-Primary Related Views</rdfs:label>
    </owl:ObjectProperty>
    


    <!-- http://capec.mitre.org/capec#obfuscationTechniques -->

    <owl:ObjectProperty rdf:about="http://capec.mitre.org/capec#obfuscationTechniques">
        <rdfs:domain rdf:resource="http://capec.mitre.org/capec#AttackPattern"/>
        <rdfs:range rdf:resource="http://capec.mitre.org/capec#ObfuscationTechnique"/>
        <rdfs:comment>Specifies one or more obfuscation techniques. An obfuscation technique can be used to disguise the fact that an attack of this type is imminent, in progress or has occurred.</rdfs:comment>
        <rdfs:label>Obfuscation Techniques</rdfs:label>
    </owl:ObjectProperty>
    


    <!-- http://capec.mitre.org/capec#observableEvidenceIfNotPresent -->

    <owl:ObjectProperty rdf:about="http://capec.mitre.org/capec#observableEvidenceIfNotPresent">
        <rdfs:domain rdf:resource="http://capec.mitre.org/capec#SecurityControl"/>
        <rdfs:range rdf:resource="http://cybox.mitre.org/cybox_core#Observables"/>
        <rdfs:comment>Specifies observable evidence, if not present</rdfs:comment>
        <rdfs:label>Observable Evidence If Not Present</rdfs:label>
    </owl:ObjectProperty>
    


    <!-- http://capec.mitre.org/capec#observableEvidenceIfPresent -->

    <owl:ObjectProperty rdf:about="http://capec.mitre.org/capec#observableEvidenceIfPresent">
        <rdfs:domain rdf:resource="http://capec.mitre.org/capec#SecurityControl"/>
        <rdfs:range rdf:resource="http://cybox.mitre.org/cybox_core#Observables"/>
        <rdfs:comment>Specifies observable evidence, if present</rdfs:comment>
        <rdfs:label>Observable Evidence If Present</rdfs:label>
    </owl:ObjectProperty>
    


    <!-- http://capec.mitre.org/capec#observables -->

    <owl:ObjectProperty rdf:about="http://capec.mitre.org/capec#observables">
        <rdfs:domain rdf:resource="http://capec.mitre.org/capec#AttackStep"/>
        <rdfs:domain rdf:resource="http://capec.mitre.org/capec#AttackStepTechnique"/>
        <rdfs:domain rdf:resource="http://capec.mitre.org/capec#IndicatorWarning"/>
        <rdfs:domain rdf:resource="http://capec.mitre.org/capec#ObfuscationTechnique"/>
        <rdfs:domain rdf:resource="http://capec.mitre.org/capec#Outcome"/>
        <rdfs:domain rdf:resource="http://capec.mitre.org/capec#ProbingTechnique"/>
        <rdfs:domain rdf:resource="http://capec.mitre.org/capec#SusceptabiltyIndicator"/>
        <rdfs:range rdf:resource="http://cybox.mitre.org/cybox_core#Observables"/>
        <rdfs:comment>Specifies observable behaviors</rdfs:comment>
        <rdfs:label>Observables</rdfs:label>
    </owl:ObjectProperty>
    


    <!-- http://capec.mitre.org/capec#outcomes -->

    <owl:ObjectProperty rdf:about="http://capec.mitre.org/capec#outcomes">
        <rdfs:domain rdf:resource="http://capec.mitre.org/capec#AttackStep"/>
        <rdfs:range rdf:resource="http://capec.mitre.org/capec#Outcome"/>
        <rdfs:comment>Specifies possible outcomes for this attack step.</rdfs:comment>
        <rdfs:label>Outcomes</rdfs:label>
    </owl:ObjectProperty>
    


    <!-- http://capec.mitre.org/capec#patternSpecificOverrides -->

    <owl:ObjectProperty rdf:about="http://capec.mitre.org/capec#patternSpecificOverrides">
        <rdfs:domain rdf:resource="http://capec.mitre.org/capec#CommonAttackSurfaceDescription"/>
        <rdfs:range rdf:resource="http://capec.mitre.org/capec#TargetAttackSurfaceDescription"/>
        <rdfs:comment>Specifies pattern-specific overrides for a target attack surface</rdfs:comment>
        <rdfs:label>Pattern-Specific Overrides</rdfs:label>
    </owl:ObjectProperty>
    


    <!-- http://capec.mitre.org/capec#payloadActivationImpact.observables -->

    <owl:ObjectProperty rdf:about="http://capec.mitre.org/capec#payloadActivationImpact.observables">
        <rdfs:domain rdf:resource="http://capec.mitre.org/capec#AttackPattern"/>
        <rdfs:range rdf:resource="http://cybox.mitre.org/cybox_core#Observables"/>
        <rdfs:comment>Specifies detailed cyber observable patterns for potential detection of the payload activation impact.</rdfs:comment>
        <rdfs:isDefinedBy rdf:resource="http://capec.mitre.org/capec"/>
        <rdfs:label>Payload Activation Impact Observables</rdfs:label>
    </owl:ObjectProperty>
    


    <!-- http://capec.mitre.org/capec#primaryViews -->

    <owl:ObjectProperty rdf:about="http://capec.mitre.org/capec#primaryViews">
        <rdfs:domain rdf:resource="http://capec.mitre.org/capec#RelationshipStatement"/>
        <rdfs:range rdf:resource="http://capec.mitre.org/capec#View"/>
        <rdfs:comment>Specifies a list of the individual Views to which this relationship pertains</rdfs:comment>
        <rdfs:isDefinedBy rdf:resource="http://capec.mitre.org/capec"/>
        <rdfs:label>Primary Related Views</rdfs:label>
    </owl:ObjectProperty>
    


    <!-- http://capec.mitre.org/capec#probingTechniques -->

    <owl:ObjectProperty rdf:about="http://capec.mitre.org/capec#probingTechniques">
        <rdfs:domain rdf:resource="http://capec.mitre.org/capec#AttackPattern"/>
        <rdfs:range rdf:resource="http://capec.mitre.org/capec#ProbingTechnique"/>
        <rdfs:comment>Specifies one or more probing techniques. A probing technique describes a method used to probe and reconnoiter a potential target to determine vulnerability and/or to prepare for this type of attack.</rdfs:comment>
        <rdfs:label>Probing Techniques</rdfs:label>
    </owl:ObjectProperty>
    


    <!-- http://capec.mitre.org/capec#protocol -->

    <owl:ObjectProperty rdf:about="http://capec.mitre.org/capec#protocol">
        <rdfs:domain rdf:resource="http://capec.mitre.org/capec#TargetedProtocol"/>
        <rdfs:range rdf:resource="http://cybox.mitre.org/objects/NetworkProtocol#NetworkProtocol"/>
        <rdfs:comment>Specifies a reference to a Protocol</rdfs:comment>
        <rdfs:label>Protocol</rdfs:label>
    </owl:ObjectProperty>
    


    <!-- http://capec.mitre.org/capec#referenceAuthor -->

    <owl:ObjectProperty rdf:about="http://capec.mitre.org/capec#referenceAuthor">
        <rdfs:domain rdf:resource="http://capec.mitre.org/capec#Reference"/>
        <rdfs:range>
            <owl:Class>
                <owl:unionOf rdf:parseType="Collection">
                    <rdf:Description rdf:about="http://www.oasis-open.org/ciq_xpil#Organization"/>
                    <rdf:Description rdf:about="http://www.oasis-open.org/ciq_xpil#Party"/>
                    <rdf:Description rdf:about="http://www.oasis-open.org/ciq_xpil#Person"/>
                </owl:unionOf>
            </owl:Class>
        </rdfs:range>
        <rdfs:comment>Specifies a reference to one or more authors of the material being referenced.</rdfs:comment>
        <rdfs:label>Reference Author</rdfs:label>
    </owl:ObjectProperty>
    


    <!-- http://capec.mitre.org/capec#referencePublisher -->

    <owl:ObjectProperty rdf:about="http://capec.mitre.org/capec#referencePublisher">
        <rdfs:domain rdf:resource="http://capec.mitre.org/capec#Reference"/>
        <rdfs:range rdf:resource="http://www.oasis-open.org/ciq_xpil#Organization"/>
        <rdfs:comment>Specifies the publisher of the reference material, if one exists.</rdfs:comment>
        <rdfs:label>Reference Publisher</rdfs:label>
    </owl:ObjectProperty>
    


    <!-- http://capec.mitre.org/capec#references -->

    <owl:ObjectProperty rdf:about="http://capec.mitre.org/capec#references">
        <rdfs:domain rdf:resource="http://capec.mitre.org/capec#AttackPattern"/>
        <rdfs:domain rdf:resource="http://capec.mitre.org/capec#Category"/>
        <rdfs:domain rdf:resource="http://capec.mitre.org/capec#CompoundElement"/>
        <rdfs:domain rdf:resource="http://capec.mitre.org/capec#View"/>
        <rdfs:range rdf:resource="http://capec.mitre.org/capec#Reference"/>
        <rdfs:comment>Specifies one or more references.</rdfs:comment>
        <rdfs:label>References</rdfs:label>
    </owl:ObjectProperty>
    


    <!-- http://capec.mitre.org/capec#relatedAttackPatterns -->

    <owl:ObjectProperty rdf:about="http://capec.mitre.org/capec#relatedAttackPatterns">
        <rdfs:domain rdf:resource="http://capec.mitre.org/capec#AttackPattern"/>
        <rdfs:range rdf:resource="http://capec.mitre.org/capec#AttackPattern"/>
        <rdfs:comment>Specifies one or more related attack patterns. A related attack pattern refers to an attack pattern that is dependent on or applied in conjunction with this attack pattern.</rdfs:comment>
        <rdfs:label>Related Attack Patterns</rdfs:label>
    </owl:ObjectProperty>
    


    <!-- http://capec.mitre.org/capec#relatedProtocols -->

    <owl:ObjectProperty rdf:about="http://capec.mitre.org/capec#relatedProtocols">
        <rdfs:domain rdf:resource="http://capec.mitre.org/capec#TargetedProtocol"/>
        <rdfs:range rdf:resource="http://cybox.mitre.org/objects/NetworkProtocol#NetworkProtocol"/>
        <rdfs:comment>Specifies zero or more protocols related to the existing protocol</rdfs:comment>
        <rdfs:label>Related Protocols</rdfs:label>
    </owl:ObjectProperty>
    


    <!-- http://capec.mitre.org/capec#relatedVulnerabilities -->

    <owl:ObjectProperty rdf:about="http://capec.mitre.org/capec#relatedVulnerabilities">
        <rdfs:domain rdf:resource="http://capec.mitre.org/capec#AttackPattern"/>
        <rdfs:range rdf:resource="http://nvd.nist.gov/cve#Vulnerability"/>
        <rdfs:comment>Specifies  one or more related vulnerabilities. A related vulnerability refers to a specific instance vulnerability targeted for exploit by this attack pattern. 

USAGE: This element is used to identify specific vulnerabilities by their 	industry-standard Common Vulnerabilities and Exposures (CVE) numbers and/or US-CERT numbers. As vulnerabilities are much more specific and localized than weaknesses, it is uncommon that an attack pattern would target a specific vulnerability. This would most likely occur if the attack pattern were targeting vulnerabilities in the underlying platform, framework, or software library.</rdfs:comment>
        <rdfs:label>Related Vulnerability</rdfs:label>
    </owl:ObjectProperty>
    


    <!-- http://capec.mitre.org/capec#relatedWeaknesses -->

    <owl:ObjectProperty rdf:about="http://capec.mitre.org/capec#relatedWeaknesses">
        <rdfs:domain rdf:resource="http://capec.mitre.org/capec#AttackPattern"/>
        <rdfs:domain rdf:resource="http://capec.mitre.org/capec#Category"/>
        <rdfs:range>
            <owl:Class>
                <owl:unionOf rdf:parseType="Collection">
                    <rdf:Description rdf:about="http://cwe.mitre.org/cwe#Category"/>
                    <rdf:Description rdf:about="http://cwe.mitre.org/cwe#CompoundElement"/>
                    <rdf:Description rdf:about="http://cwe.mitre.org/cwe#View"/>
                    <rdf:Description rdf:about="http://cwe.mitre.org/cwe#Weakness"/>
                </owl:unionOf>
            </owl:Class>
        </rdfs:range>
        <rdfs:comment>Specifies the specific weaknesses the attack targets and leverages.

Specific weaknesses (underlying issues that may cause vulnerabilities) reference the industry-standard Common Weakness 	Enumeration (CWE). This list should include not only those weaknesses that are directly targeted by the attack but also those whose presence can directly increase the likelihood of the attack succeeding or the impact if it does succeed.</rdfs:comment>
        <rdfs:label>Related Weaknesses</rdfs:label>
    </owl:ObjectProperty>
    


    <!-- http://capec.mitre.org/capec#relationshipChains -->

    <owl:ObjectProperty rdf:about="http://capec.mitre.org/capec#relationshipChains">
        <rdfs:domain rdf:resource="http://capec.mitre.org/capec#RelationshipStatement"/>
        <rdfs:range rdf:resource="http://capec.mitre.org/capec#CompoundElement"/>
        <rdfs:comment>Specifies a list of the individual Chains this relationship pertains to.</rdfs:comment>
        <rdfs:label>Relationship Chains</rdfs:label>
    </owl:ObjectProperty>
    


    <!-- http://capec.mitre.org/capec#relationships -->

    <owl:ObjectProperty rdf:about="http://capec.mitre.org/capec#relationships">
        <rdfs:domain rdf:resource="http://capec.mitre.org/capec#Category"/>
        <rdfs:domain rdf:resource="http://capec.mitre.org/capec#CompoundElement"/>
        <rdfs:domain rdf:resource="http://capec.mitre.org/capec#View"/>
        <rdfs:range>
            <owl:Class>
                <owl:unionOf rdf:parseType="Collection">
                    <rdf:Description rdf:about="http://capec.mitre.org/capec#AttackPattern"/>
                    <rdf:Description rdf:about="http://capec.mitre.org/capec#Category"/>
                    <rdf:Description rdf:about="http://capec.mitre.org/capec#CompoundElement"/>
                    <rdf:Description rdf:about="http://capec.mitre.org/capec#View"/>
                </owl:unionOf>
            </owl:Class>
        </rdfs:range>
        <rdfs:comment>Specfies one or more Relationship elements, each of which identifies an association between this structure, whether it is a Attack Pattern, Category, or Compound_Element and another structure.</rdfs:comment>
        <rdfs:label>Relationships</rdfs:label>
    </owl:ObjectProperty>
    


    <!-- http://capec.mitre.org/capec#relevantCommandStructures -->

    <owl:ObjectProperty rdf:about="http://capec.mitre.org/capec#relevantCommandStructures">
        <rdfs:domain rdf:resource="http://capec.mitre.org/capec#CommonAttackSurfaceDescription"/>
        <rdfs:range rdf:resource="http://capec.mitre.org/capec#CommandStructure"/>
        <rdfs:comment>Specifies command structures that are relevant to this attack surface</rdfs:comment>
        <rdfs:label>Relevant Command Structures</rdfs:label>
    </owl:ObjectProperty>
    


    <!-- http://capec.mitre.org/capec#relevantFunctionalServices -->

    <owl:ObjectProperty rdf:about="http://capec.mitre.org/capec#relevantFunctionalServices">
        <rdfs:domain rdf:resource="http://capec.mitre.org/capec#CommonAttackSurfaceDescription"/>
        <rdfs:range rdf:resource="http://capec.mitre.org/capec#FunctionalService"/>
        <rdfs:comment>Specifies the functional services that are relevant to this attack surface</rdfs:comment>
        <rdfs:label>Relevant Functional Services</rdfs:label>
    </owl:ObjectProperty>
    


    <!-- http://capec.mitre.org/capec#relevantProtocolHeaders -->

    <owl:ObjectProperty rdf:about="http://capec.mitre.org/capec#relevantProtocolHeaders">
        <rdfs:domain rdf:resource="http://capec.mitre.org/capec#CommonAttackSurfaceDescription"/>
        <rdfs:comment>Specifies protocol headers that a relevant to this attack surface</rdfs:comment>
        <rdfs:label>Relevant Protocl Headers</rdfs:label>
    </owl:ObjectProperty>
    


    <!-- http://capec.mitre.org/capec#relevantProtocols -->

    <owl:ObjectProperty rdf:about="http://capec.mitre.org/capec#relevantProtocols">
        <rdfs:domain rdf:resource="http://capec.mitre.org/capec#CommonAttackSurfaceDescription"/>
        <rdfs:range rdf:resource="http://capec.mitre.org/capec#TargetedProtocol"/>
        <rdfs:comment>Specifies protocols that are relevant to this attack surface area.</rdfs:comment>
        <rdfs:label>Relevant Protocols</rdfs:label>
    </owl:ObjectProperty>
    


    <!-- http://capec.mitre.org/capec#securityControls -->

    <owl:ObjectProperty rdf:about="http://capec.mitre.org/capec#securityControls">
        <rdfs:domain rdf:resource="http://capec.mitre.org/capec#AttackStep"/>
        <rdfs:range rdf:resource="http://capec.mitre.org/capec#SecurityControl"/>
        <rdfs:comment>Specifies security controls for this attack step that describe ways in which the attack step can be detected, corrected, or prevented. These are presented from a defender’s point of view, where the defender may be a developer, tester, operations administrator, or other resource resisting the attacker.</rdfs:comment>
        <rdfs:label>Security Controls</rdfs:label>
    </owl:ObjectProperty>
    


    <!-- http://capec.mitre.org/capec#targetAttackSurface -->

    <owl:ObjectProperty rdf:about="http://capec.mitre.org/capec#targetAttackSurface">
        <rdfs:domain rdf:resource="http://capec.mitre.org/capec#AttackPattern"/>
        <rdfs:range>
            <owl:Class>
                <owl:unionOf rdf:parseType="Collection">
                    <rdf:Description rdf:about="http://capec.mitre.org/capec#CommonAttackSurfaceDescription"/>
                    <rdf:Description rdf:about="http://capec.mitre.org/capec#TargetAttackSurfaceDescription"/>
                </owl:unionOf>
            </owl:Class>
        </rdfs:range>
        <rdfs:comment>Specifies the locations where an attacker interacts with the target system</rdfs:comment>
        <rdfs:label>Target Attack Surface</rdfs:label>
    </owl:ObjectProperty>
    


    <!-- http://capec.mitre.org/capec#targetFunctionalServices -->

    <owl:ObjectProperty rdf:about="http://capec.mitre.org/capec#targetFunctionalServices">
        <rdfs:domain rdf:resource="http://capec.mitre.org/capec#TargetAttackSurfaceDescription"/>
        <rdfs:range rdf:resource="http://capec.mitre.org/capec#FunctionalService"/>
        <rdfs:comment>Specifies Functional Services that are part of the target attack surface</rdfs:comment>
        <rdfs:label>Attack Surface Target Functional Services</rdfs:label>
    </owl:ObjectProperty>
    


    <!-- http://capec.mitre.org/capec#targetedCommandStructures -->

    <owl:ObjectProperty rdf:about="http://capec.mitre.org/capec#targetedCommandStructures">
        <rdfs:domain rdf:resource="http://capec.mitre.org/capec#TargetedProtocol"/>
        <rdfs:range rdf:resource="http://capec.mitre.org/capec#CommandStructure"/>
        <rdfs:comment>Specifies the protocol&apos;s command structures that are being targeted by the attack pattern</rdfs:comment>
        <rdfs:label>TargetedCommand Structures</rdfs:label>
    </owl:ObjectProperty>
    


    <!-- http://capec.mitre.org/capec#targetedProtocolFields -->

    <owl:ObjectProperty rdf:about="http://capec.mitre.org/capec#targetedProtocolFields">
        <rdfs:domain rdf:resource="http://capec.mitre.org/capec#TargetedProtocol"/>
        <rdfs:comment>Specifies zero or more specific fields of the protocol being utilized</rdfs:comment>
        <rdfs:label>Targeted Protocol Fields</rdfs:label>
    </owl:ObjectProperty>
    


    <!-- http://capec.mitre.org/capec#targetedProtocols -->

    <owl:ObjectProperty rdf:about="http://capec.mitre.org/capec#targetedProtocols">
        <rdfs:domain rdf:resource="http://capec.mitre.org/capec#FunctionalService"/>
        <rdfs:domain rdf:resource="http://capec.mitre.org/capec#TargetAttackSurfaceDescription"/>
        <rdfs:range rdf:resource="http://capec.mitre.org/capec#TargetedProtocol"/>
        <rdfs:comment>Specifies one or more protocols associated with the Functional Service that an attack pattern specifically targets aspects of the protocol</rdfs:comment>
        <rdfs:label>Targeted Protocols</rdfs:label>
    </owl:ObjectProperty>
    


    <!-- http://capec.mitre.org/capec#usesProtocols -->

    <owl:ObjectProperty rdf:about="http://capec.mitre.org/capec#usesProtocols">
        <rdfs:domain rdf:resource="http://capec.mitre.org/capec#FunctionalService"/>
        <rdfs:comment>Specifies one or more protocols associated with the Functional Service that are generally targeted by an attack pattern</rdfs:comment>
        <rdfs:label>Uses Protocols</rdfs:label>
    </owl:ObjectProperty>
    


    <!-- http://capec.mitre.org/capec#views -->

    <owl:ObjectProperty rdf:about="http://capec.mitre.org/capec#views">
        <rdfs:domain rdf:resource="http://capec.mitre.org/capec#AttackPatternCatalog"/>
        <rdfs:range rdf:resource="http://capec.mitre.org/capec#View"/>
        <rdfs:comment>Specifies a reference to one or more Attack Pattern Views</rdfs:comment>
        <rdfs:label>Views</rdfs:label>
    </owl:ObjectProperty>
    


    <!-- http://capec.mitre.org/capec#vulnerability -->

    <owl:ObjectProperty rdf:about="http://capec.mitre.org/capec#vulnerability">
        <rdfs:domain rdf:resource="http://capec.mitre.org/capec#ExampleInstance"/>
        <rdfs:range rdf:resource="http://nvd.nist.gov/cve#Vulnerability"/>
        <rdfs:comment>Specifies the vulnerability</rdfs:comment>
        <rdfs:label>Vulnerability</rdfs:label>
    </owl:ObjectProperty>
    


    <!-- 
    ///////////////////////////////////////////////////////////////////////////////////////
    //
    // Data properties
    //
    ///////////////////////////////////////////////////////////////////////////////////////
     -->

    


    <!-- http://capec.mitre.org/capec#activationZone -->

    <owl:DatatypeProperty rdf:about="http://capec.mitre.org/capec#activationZone">
        <rdfs:domain rdf:resource="http://capec.mitre.org/capec#AttackPattern"/>
        <rdfs:range rdf:resource="http://capec.mitre.org/capec#structuredText"/>
        <rdfs:comment>Specifies the area within the target software that is capable of executing or otherwise activating the payload of an injection-based attack of this type. The activation zone is where the intent of the attacker is put into action. The activation zone may be a command interpreter, some active machine code in a buffer, a client browser, a system API call, etc.</rdfs:comment>
        <rdfs:label>Activation Zone</rdfs:label>
    </owl:DatatypeProperty>
    


    <!-- http://capec.mitre.org/capec#attackPrerequisites -->

    <owl:DatatypeProperty rdf:about="http://capec.mitre.org/capec#attackPrerequisites">
        <rdfs:domain rdf:resource="http://capec.mitre.org/capec#AttackPattern"/>
        <rdfs:domain rdf:resource="http://capec.mitre.org/capec#Category"/>
        <rdfs:range rdf:resource="http://capec.mitre.org/capec#structuredText"/>
        <rdfs:comment>Specifies the conditions that must exist or the functionality and characteristics that the target software must have or behavior it must exhibit for an attack of this type to succeed.</rdfs:comment>
        <rdfs:label>Attack Prerequisites</rdfs:label>
    </owl:DatatypeProperty>
    


    <!-- http://capec.mitre.org/capec#attackSurfaceId -->

    <owl:DatatypeProperty rdf:about="http://capec.mitre.org/capec#attackSurfaceId">
        <rdfs:domain rdf:resource="http://capec.mitre.org/capec#CommonAttackSurface"/>
        <rdfs:domain rdf:resource="http://capec.mitre.org/capec#CommonAttackSurfaceDescription"/>
        <rdfs:range rdf:resource="http://www.w3.org/2001/XMLSchema#string"/>
        <rdfs:comment>Specifies an identifier for the attack surface</rdfs:comment>
        <rdfs:label>Attack Surface Identifier</rdfs:label>
    </owl:DatatypeProperty>
    


    <!-- http://capec.mitre.org/capec#authorName -->

    <owl:DatatypeProperty rdf:about="http://capec.mitre.org/capec#authorName">
        <rdfs:domain rdf:resource="http://capec.mitre.org/capec#HistoryRecord"/>
        <rdfs:range rdf:resource="http://www.w3.org/2001/XMLSchema#string"/>
        <rdfs:comment>Specifies the name of the author for this entry</rdfs:comment>
        <rdfs:label>Author Name</rdfs:label>
    </owl:DatatypeProperty>
    


    <!-- http://capec.mitre.org/capec#authorOganizationName -->

    <owl:DatatypeProperty rdf:about="http://capec.mitre.org/capec#authorOganizationName">
        <rdfs:domain rdf:resource="http://capec.mitre.org/capec#HistoryRecord"/>
        <rdfs:range rdf:resource="http://www.w3.org/2001/XMLSchema#string"/>
        <rdfs:comment>Specifies the name of the author&apos;s organization</rdfs:comment>
        <rdfs:label>Author&apos;s Oganization Name</rdfs:label>
    </owl:DatatypeProperty>
    


    <!-- http://capec.mitre.org/capec#backgroundDetails -->

    <owl:DatatypeProperty rdf:about="http://capec.mitre.org/capec#backgroundDetails">
        <rdfs:domain rdf:resource="http://capec.mitre.org/capec#Category"/>
        <rdfs:domain rdf:resource="http://capec.mitre.org/capec#CompoundElement"/>
        <rdfs:range rdf:resource="http://capec.mitre.org/capec#structuredText"/>
        <rdfs:comment>Speicfies information regarding the entry or any technologies that are related to it, where the background information is 	not related to the nature of the entry itself. It should be filled out where appropriate.</rdfs:comment>
        <rdfs:label>Background Details</rdfs:label>
    </owl:DatatypeProperty>
    


    <!-- http://capec.mitre.org/capec#categoryName -->

    <owl:DatatypeProperty rdf:about="http://capec.mitre.org/capec#categoryName">
        <rdfs:domain rdf:resource="http://capec.mitre.org/capec#Category"/>
        <rdfs:range rdf:resource="http://www.w3.org/2001/XMLSchema#string"/>
        <rdfs:comment>Specifies a descriptive name used to give the reader an idea of what the commonality is amongst the children of this category. 

All words in the name should be capitalized except for articles and prepositions unless they begin or end the name. Subsequent words in a hyphenated chain are also not capitalized.</rdfs:comment>
        <rdfs:label>Category Name</rdfs:label>
    </owl:DatatypeProperty>
    


    <!-- http://capec.mitre.org/capec#code -->

    <owl:DatatypeProperty rdf:about="http://capec.mitre.org/capec#code">
        <rdfs:range rdf:resource="http://www.w3.org/2001/XMLSchema#string"/>
        <rdfs:comment>Specifies a line of code.</rdfs:comment>
        <rdfs:label>Code</rdfs:label>
    </owl:DatatypeProperty>
    


    <!-- http://capec.mitre.org/capec#codeComment -->

    <owl:DatatypeProperty rdf:about="http://capec.mitre.org/capec#codeComment">
        <rdfs:range rdf:resource="http://www.w3.org/2001/XMLSchema#string"/>
        <rdfs:comment>Specifies a comment in code.</rdfs:comment>
        <rdfs:label>Comment</rdfs:label>
    </owl:DatatypeProperty>
    


    <!-- http://capec.mitre.org/capec#codeExampleLanguage -->

    <owl:DatatypeProperty rdf:about="http://capec.mitre.org/capec#codeExampleLanguage">
        <rdfs:range rdf:resource="http://www.w3.org/2001/XMLSchema#string"/>
        <rdfs:comment>Specifies the programming language being used in the following block of Code</rdfs:comment>
        <rdfs:label>Code Example Language</rdfs:label>
    </owl:DatatypeProperty>
    


    <!-- http://capec.mitre.org/capec#commandDescription -->

    <owl:DatatypeProperty rdf:about="http://capec.mitre.org/capec#commandDescription">
        <rdfs:domain rdf:resource="http://capec.mitre.org/capec#CommandStructure"/>
        <rdfs:range rdf:resource="http://www.w3.org/2001/XMLSchema#string"/>
        <rdfs:comment>Specifies a brief description of the command structure</rdfs:comment>
        <rdfs:label>Description</rdfs:label>
    </owl:DatatypeProperty>
    


    <!-- http://capec.mitre.org/capec#commandGroupLabel -->

    <owl:DatatypeProperty rdf:about="http://capec.mitre.org/capec#commandGroupLabel">
        <rdfs:domain rdf:resource="http://capec.mitre.org/capec#CommandStructure"/>
        <rdfs:range rdf:resource="http://www.w3.org/2001/XMLSchema#string"/>
        <rdfs:comment>Specifies the group label for the command structure</rdfs:comment>
        <rdfs:label>Group Label</rdfs:label>
    </owl:DatatypeProperty>
    


    <!-- http://capec.mitre.org/capec#commandStructureId -->

    <owl:DatatypeProperty rdf:about="http://capec.mitre.org/capec#commandStructureId">
        <rdfs:domain rdf:resource="http://capec.mitre.org/capec#CommandStructure"/>
        <rdfs:range rdf:resource="http://www.w3.org/2001/XMLSchema#integer"/>
        <rdfs:comment>Specifies the identifier for a Command Structure</rdfs:comment>
        <rdfs:label>Command Structure Identifier</rdfs:label>
    </owl:DatatypeProperty>
    


    <!-- http://capec.mitre.org/capec#commandStructureName -->

    <owl:DatatypeProperty rdf:about="http://capec.mitre.org/capec#commandStructureName">
        <rdfs:domain rdf:resource="http://capec.mitre.org/capec#CommandStructure"/>
        <rdfs:range rdf:resource="http://www.w3.org/2001/XMLSchema#string"/>
        <rdfs:comment>Specifies a name associated with the Command Structure</rdfs:comment>
        <rdfs:label>Name</rdfs:label>
    </owl:DatatypeProperty>
    


    <!-- http://capec.mitre.org/capec#commandType -->

    <owl:DatatypeProperty rdf:about="http://capec.mitre.org/capec#commandType">
        <rdfs:domain rdf:resource="http://capec.mitre.org/capec#CommandStructure"/>
        <rdfs:range rdf:resource="http://www.w3.org/2001/XMLSchema#string"/>
        <rdfs:comment>Specifies the type of the command structure</rdfs:comment>
        <rdfs:label>Type</rdfs:label>
    </owl:DatatypeProperty>
    


    <!-- http://capec.mitre.org/capec#compoundElementAbstraction -->

    <owl:DatatypeProperty rdf:about="http://capec.mitre.org/capec#compoundElementAbstraction">
        <rdfs:domain rdf:resource="http://capec.mitre.org/capec#CompoundElement"/>
        <rdfs:range>
            <rdfs:Datatype>
                <owl:oneOf>
                    <rdf:Description>
                        <rdf:type rdf:resource="http://www.w3.org/1999/02/22-rdf-syntax-ns#List"/>
                        <rdf:first rdf:datatype="http://www.w3.org/2001/XMLSchema#string">Detailed</rdf:first>
                        <rdf:rest>
                            <rdf:Description>
                                <rdf:type rdf:resource="http://www.w3.org/1999/02/22-rdf-syntax-ns#List"/>
                                <rdf:first rdf:datatype="http://www.w3.org/2001/XMLSchema#string">Meta</rdf:first>
                                <rdf:rest>
                                    <rdf:Description>
                                        <rdf:type rdf:resource="http://www.w3.org/1999/02/22-rdf-syntax-ns#List"/>
                                        <rdf:first rdf:datatype="http://www.w3.org/2001/XMLSchema#string">Standard</rdf:first>
                                        <rdf:rest rdf:resource="http://www.w3.org/1999/02/22-rdf-syntax-ns#nil"/>
                                    </rdf:Description>
                                </rdf:rest>
                            </rdf:Description>
                        </rdf:rest>
                    </rdf:Description>
                </owl:oneOf>
            </rdfs:Datatype>
        </rdfs:range>
        <rdfs:comment>Specifies the abstraction level for this attack pattern. The abstraction levels for Compound Elements and Attack Patterns 	are the same. For example, if the Compound Element is a chain, and all elements of the chain are Meta level, then the Compound Element Abstraction attribute is Meta.</rdfs:comment>
        <rdfs:label>Compound Element Abstraction</rdfs:label>
    </owl:DatatypeProperty>
    


    <!-- http://capec.mitre.org/capec#compoundElementCompleteness -->

    <owl:DatatypeProperty rdf:about="http://capec.mitre.org/capec#compoundElementCompleteness">
        <rdfs:domain rdf:resource="http://capec.mitre.org/capec#CompoundElement"/>
        <rdfs:range>
            <rdfs:Datatype>
                <owl:oneOf>
                    <rdf:Description>
                        <rdf:type rdf:resource="http://www.w3.org/1999/02/22-rdf-syntax-ns#List"/>
                        <rdf:first rdf:datatype="http://www.w3.org/2001/XMLSchema#string">Complete</rdf:first>
                        <rdf:rest>
                            <rdf:Description>
                                <rdf:type rdf:resource="http://www.w3.org/1999/02/22-rdf-syntax-ns#List"/>
                                <rdf:first rdf:datatype="http://www.w3.org/2001/XMLSchema#string">Hook</rdf:first>
                                <rdf:rest>
                                    <rdf:Description>
                                        <rdf:type rdf:resource="http://www.w3.org/1999/02/22-rdf-syntax-ns#List"/>
                                        <rdf:first rdf:datatype="http://www.w3.org/2001/XMLSchema#string">Stub</rdf:first>
                                        <rdf:rest rdf:resource="http://www.w3.org/1999/02/22-rdf-syntax-ns#nil"/>
                                    </rdf:Description>
                                </rdf:rest>
                            </rdf:Description>
                        </rdf:rest>
                    </rdf:Description>
                </owl:oneOf>
            </rdfs:Datatype>
        </rdfs:range>
        <rdfs:comment>Specifies the completeness of the Compound Element</rdfs:comment>
        <rdfs:label>Compound Element Completeness</rdfs:label>
    </owl:DatatypeProperty>
    


    <!-- http://capec.mitre.org/capec#compoundElementStructure -->

    <owl:DatatypeProperty rdf:about="http://capec.mitre.org/capec#compoundElementStructure">
        <rdfs:domain rdf:resource="http://capec.mitre.org/capec#CompoundElement"/>
        <rdfs:range>
            <rdfs:Datatype>
                <owl:oneOf>
                    <rdf:Description>
                        <rdf:type rdf:resource="http://www.w3.org/1999/02/22-rdf-syntax-ns#List"/>
                        <rdf:first rdf:datatype="http://www.w3.org/2001/XMLSchema#string">Chain</rdf:first>
                        <rdf:rest>
                            <rdf:Description>
                                <rdf:type rdf:resource="http://www.w3.org/1999/02/22-rdf-syntax-ns#List"/>
                                <rdf:first rdf:datatype="http://www.w3.org/2001/XMLSchema#string">Composite</rdf:first>
                                <rdf:rest rdf:resource="http://www.w3.org/1999/02/22-rdf-syntax-ns#nil"/>
                            </rdf:Description>
                        </rdf:rest>
                    </rdf:Description>
                </owl:oneOf>
            </rdfs:Datatype>
        </rdfs:range>
        <rdfs:comment>Specifies  the structural nature of this Compound Element - that is, composed of other attack patterns concurrently,	as in a composite, or consecutively, as in a chain.</rdfs:comment>
        <rdfs:label>Compound Element Structure</rdfs:label>
    </owl:DatatypeProperty>
    


    <!-- http://capec.mitre.org/capec#consequenceId -->

    <owl:DatatypeProperty rdf:about="http://capec.mitre.org/capec#consequenceId">
        <rdfs:domain rdf:resource="http://capec.mitre.org/capec#Consequence"/>
        <rdfs:range rdf:resource="http://www.w3.org/2001/XMLSchema#string"/>
        <rdfs:comment>Specifies the value for the related Common_Consequence entry identifier as a string.  Only one Common Consequence Identifier can exist for each Consequence element (ex: CC-1).  However, Consequences across CAPEC with the same ID should only vary in small details.</rdfs:comment>
        <rdfs:label>Consequence Identifier</rdfs:label>
    </owl:DatatypeProperty>
    


    <!-- http://capec.mitre.org/capec#consequenceNote -->

    <owl:DatatypeProperty rdf:about="http://capec.mitre.org/capec#consequenceNote">
        <rdfs:domain rdf:resource="http://capec.mitre.org/capec#Consequence"/>
        <rdfs:range rdf:resource="http://capec.mitre.org/capec#structuredText"/>
        <rdfs:comment>Specifies additional commentary about this consequence.</rdfs:comment>
        <rdfs:label>Consequence Note</rdfs:label>
    </owl:DatatypeProperty>
    


    <!-- http://capec.mitre.org/capec#consequenceScope -->

    <owl:DatatypeProperty rdf:about="http://capec.mitre.org/capec#consequenceScope">
        <rdfs:domain rdf:resource="http://capec.mitre.org/capec#Consequence"/>
        <rdfs:range rdf:resource="http://www.w3.org/2001/XMLSchema#string"/>
        <rdfs:comment>Specifies an individual consequence that may result from this attack pattern.</rdfs:comment>
        <rdfs:label>Scope</rdfs:label>
    </owl:DatatypeProperty>
    


    <!-- http://capec.mitre.org/capec#contributionImportance -->

    <owl:DatatypeProperty rdf:about="http://capec.mitre.org/capec#contributionImportance">
        <rdfs:domain rdf:resource="http://capec.mitre.org/capec#HistoryRecord"/>
        <rdfs:range>
            <rdfs:Datatype>
                <owl:oneOf>
                    <rdf:Description>
                        <rdf:type rdf:resource="http://www.w3.org/1999/02/22-rdf-syntax-ns#List"/>
                        <rdf:first rdf:datatype="http://www.w3.org/2001/XMLSchema#string">Critical</rdf:first>
                        <rdf:rest>
                            <rdf:Description>
                                <rdf:type rdf:resource="http://www.w3.org/1999/02/22-rdf-syntax-ns#List"/>
                                <rdf:first rdf:datatype="http://www.w3.org/2001/XMLSchema#string">Normal</rdf:first>
                                <rdf:rest rdf:resource="http://www.w3.org/1999/02/22-rdf-syntax-ns#nil"/>
                            </rdf:Description>
                        </rdf:rest>
                    </rdf:Description>
                </owl:oneOf>
            </rdfs:Datatype>
        </rdfs:range>
        <rdfs:comment>Specifies how significant the modification is with regard to the meaning and interpretation of the associated entity.  If a modification has a value of Critical, then the meaning of the entry or how it might be interpreted has changed and requires attention from anyone previously dependent on the associated entity.</rdfs:comment>
        <rdfs:label>Contribution Importance</rdfs:label>
    </owl:DatatypeProperty>
    


    <!-- http://capec.mitre.org/capec#contributionMode -->

    <owl:DatatypeProperty rdf:about="http://capec.mitre.org/capec#contributionMode">
        <rdfs:domain rdf:resource="http://capec.mitre.org/capec#HistoryRecord"/>
        <rdfs:range>
            <rdfs:Datatype>
                <owl:oneOf>
                    <rdf:Description>
                        <rdf:type rdf:resource="http://www.w3.org/1999/02/22-rdf-syntax-ns#List"/>
                        <rdf:first rdf:datatype="http://www.w3.org/2001/XMLSchema#string">Content</rdf:first>
                        <rdf:rest>
                            <rdf:Description>
                                <rdf:type rdf:resource="http://www.w3.org/1999/02/22-rdf-syntax-ns#List"/>
                                <rdf:first rdf:datatype="http://www.w3.org/2001/XMLSchema#string">Feedback</rdf:first>
                                <rdf:rest rdf:resource="http://www.w3.org/1999/02/22-rdf-syntax-ns#nil"/>
                            </rdf:Description>
                        </rdf:rest>
                    </rdf:Description>
                </owl:oneOf>
            </rdfs:Datatype>
        </rdfs:range>
        <rdfs:comment>Specifies whether the contribution was part of feedback given or actual content that was donated.</rdfs:comment>
        <rdfs:label>Contribution Mode</rdfs:label>
    </owl:DatatypeProperty>
    


    <!-- http://capec.mitre.org/capec#contributionSource -->

    <owl:DatatypeProperty rdf:about="http://capec.mitre.org/capec#contributionSource">
        <rdfs:domain rdf:resource="http://capec.mitre.org/capec#HistoryRecord"/>
        <rdfs:range>
            <rdfs:Datatype>
                <owl:oneOf>
                    <rdf:Description>
                        <rdf:type rdf:resource="http://www.w3.org/1999/02/22-rdf-syntax-ns#List"/>
                        <rdf:first rdf:datatype="http://www.w3.org/2001/XMLSchema#string">External</rdf:first>
                        <rdf:rest>
                            <rdf:Description>
                                <rdf:type rdf:resource="http://www.w3.org/1999/02/22-rdf-syntax-ns#List"/>
                                <rdf:first rdf:datatype="http://www.w3.org/2001/XMLSchema#string">Internal</rdf:first>
                                <rdf:rest rdf:resource="http://www.w3.org/1999/02/22-rdf-syntax-ns#nil"/>
                            </rdf:Description>
                        </rdf:rest>
                    </rdf:Description>
                </owl:oneOf>
            </rdfs:Datatype>
        </rdfs:range>
        <rdfs:comment>Specifies whether this contirbution was created by a CAPEC team member or provided by an external party.</rdfs:comment>
        <rdfs:label>Contribution Source</rdfs:label>
    </owl:DatatypeProperty>
    


    <!-- http://capec.mitre.org/capec#description -->

    <owl:DatatypeProperty rdf:about="http://capec.mitre.org/capec#description">
        <rdfs:domain rdf:resource="http://capec.mitre.org/capec#AttackPattern"/>
        <rdfs:domain rdf:resource="http://capec.mitre.org/capec#Category"/>
        <rdfs:domain rdf:resource="http://capec.mitre.org/capec#CompoundElement"/>
        <rdfs:domain rdf:resource="http://capec.mitre.org/capec#View"/>
        <rdfs:range rdf:resource="http://www.w3.org/2001/XMLSchema#string"/>
        <rdfs:comment>Specifies a minimalistic description which provides the information necessary to understand the primary focus of this entry.  The description text should be short and should limit itself to describing the key points that define this entry.  Further explanation can be included in the extended description element</rdfs:comment>
        <rdfs:label>Description Summary</rdfs:label>
    </owl:DatatypeProperty>
    


    <!-- http://capec.mitre.org/capec#dictionaryLink -->

    <owl:DatatypeProperty rdf:about="http://capec.mitre.org/capec#dictionaryLink">
        <rdfs:domain rdf:resource="http://capec.mitre.org/capec#AttackPattern"/>
        <rdfs:range rdf:resource="http://www.w3.org/2001/XMLSchema#anyURI"/>
        <rdfs:comment>Specifies an external link to the specific attack pattern contained at the Common Attack Pattern Enumeration and Characterizaton (CAPEC) dictionary.  The link should be in the following form:  http://capec.mitre.org/data/definitions/{attack-pattern-id}.html, where {attack-pattern-id) should be the integer Identifier of the specific attack pattern.</rdfs:comment>
        <rdfs:label>Dictionary Link</rdfs:label>
    </owl:DatatypeProperty>
    


    <!-- http://capec.mitre.org/capec#encryptionType -->

    <owl:DatatypeProperty rdf:about="http://capec.mitre.org/capec#encryptionType">
        <rdfs:domain rdf:resource="http://capec.mitre.org/capec#TargetedProtocol"/>
        <rdfs:range rdf:resource="http://www.w3.org/2001/XMLSchema#string"/>
        <rdfs:comment>Specifies the type of encryption</rdfs:comment>
        <rdfs:label>Encryption Type</rdfs:label>
    </owl:DatatypeProperty>
    


    <!-- http://capec.mitre.org/capec#encryptionUsed -->

    <owl:DatatypeProperty rdf:about="http://capec.mitre.org/capec#encryptionUsed">
        <rdfs:domain rdf:resource="http://capec.mitre.org/capec#TargetedProtocol"/>
        <rdfs:range rdf:resource="http://www.w3.org/2001/XMLSchema#boolean"/>
        <rdfs:comment>Specifies whether the encryption was utilized</rdfs:comment>
        <rdfs:label>Encryption</rdfs:label>
    </owl:DatatypeProperty>
    


    <!-- http://capec.mitre.org/capec#entryComment -->

    <owl:DatatypeProperty rdf:about="http://capec.mitre.org/capec#entryComment">
        <rdfs:domain rdf:resource="http://capec.mitre.org/capec#HistoryRecord"/>
        <rdfs:range rdf:resource="http://www.w3.org/2001/XMLSchema#string"/>
        <rdfs:comment>Specifies any comments regarding the content of this attack pattern entry, such as assumptions made, reasons for omitting elements, contact information, pending questions, etc.</rdfs:comment>
        <rdfs:label>Comment</rdfs:label>
    </owl:DatatypeProperty>
    


    <!-- http://capec.mitre.org/capec#entryDate -->

    <owl:DatatypeProperty rdf:about="http://capec.mitre.org/capec#entryDate">
        <rdfs:domain rdf:resource="http://capec.mitre.org/capec#HistoryRecord"/>
        <rdfs:range rdf:resource="http://www.w3.org/2001/XMLSchema#date"/>
        <rdfs:comment>Specifies the date on which the content was authored.</rdfs:comment>
        <rdfs:label>Date</rdfs:label>
    </owl:DatatypeProperty>
    


    <!-- http://capec.mitre.org/capec#entryNameChangeDate -->

    <owl:DatatypeProperty rdf:about="http://capec.mitre.org/capec#entryNameChangeDate">
        <rdfs:domain rdf:resource="http://capec.mitre.org/capec#HistoryRecord"/>
        <rdfs:range rdf:resource="http://www.w3.org/2001/XMLSchema#date"/>
        <rdfs:comment>Specifies the date on which the name was changed to something else.</rdfs:comment>
        <rdfs:label>Date of Name Change</rdfs:label>
    </owl:DatatypeProperty>
    


    <!-- http://capec.mitre.org/capec#entryType -->

    <owl:DatatypeProperty rdf:about="http://capec.mitre.org/capec#entryType">
        <rdfs:domain rdf:resource="http://capec.mitre.org/capec#HistoryRecord"/>
        <rdfs:range>
            <rdfs:Datatype>
                <owl:oneOf>
                    <rdf:Description>
                        <rdf:type rdf:resource="http://www.w3.org/1999/02/22-rdf-syntax-ns#List"/>
                        <rdf:first rdf:datatype="http://www.w3.org/2001/XMLSchema#string">Contributions</rdf:first>
                        <rdf:rest>
                            <rdf:Description>
                                <rdf:type rdf:resource="http://www.w3.org/1999/02/22-rdf-syntax-ns#List"/>
                                <rdf:first rdf:datatype="http://www.w3.org/2001/XMLSchema#string">Modification</rdf:first>
                                <rdf:rest>
                                    <rdf:Description>
                                        <rdf:type rdf:resource="http://www.w3.org/1999/02/22-rdf-syntax-ns#List"/>
                                        <rdf:first rdf:datatype="http://www.w3.org/2001/XMLSchema#string">Submission</rdf:first>
                                        <rdf:rest rdf:resource="http://www.w3.org/1999/02/22-rdf-syntax-ns#nil"/>
                                    </rdf:Description>
                                </rdf:rest>
                            </rdf:Description>
                        </rdf:rest>
                    </rdf:Description>
                </owl:oneOf>
            </rdfs:Datatype>
        </rdfs:range>
        <rdfs:comment>Specifies the type of history records.</rdfs:comment>
        <rdfs:label>Entry Type</rdfs:label>
    </owl:DatatypeProperty>
    


    <!-- http://capec.mitre.org/capec#environmentDescription -->

    <owl:DatatypeProperty rdf:about="http://capec.mitre.org/capec#environmentDescription">
        <rdfs:domain rdf:resource="http://capec.mitre.org/capec#Environment"/>
        <rdfs:range rdf:resource="http://www.w3.org/2001/XMLSchema#string"/>
        <rdfs:comment>Specifies a description of the environment</rdfs:comment>
        <rdfs:label>Description</rdfs:label>
    </owl:DatatypeProperty>
    


    <!-- http://capec.mitre.org/capec#environmentId -->

    <owl:DatatypeProperty rdf:about="http://capec.mitre.org/capec#environmentId">
        <rdfs:domain rdf:resource="http://capec.mitre.org/capec#Environment"/>
        <rdfs:range rdf:resource="http://www.w3.org/2001/XMLSchema#string"/>
        <rdfs:comment>Specifies a globally unique Identifier for a kind of environment</rdfs:comment>
        <rdfs:label>Environment Identifier</rdfs:label>
    </owl:DatatypeProperty>
    


    <!-- http://capec.mitre.org/capec#environmentTitle -->

    <owl:DatatypeProperty rdf:about="http://capec.mitre.org/capec#environmentTitle">
        <rdfs:domain rdf:resource="http://capec.mitre.org/capec#Environment"/>
        <rdfs:range rdf:resource="http://www.w3.org/2001/XMLSchema#string"/>
        <rdfs:comment>Specifies a short descriptive title for the environment</rdfs:comment>
        <rdfs:label>Title</rdfs:label>
    </owl:DatatypeProperty>
    


    <!-- http://capec.mitre.org/capec#exampleInstanceDescription -->

    <owl:DatatypeProperty rdf:about="http://capec.mitre.org/capec#exampleInstanceDescription">
        <rdfs:domain rdf:resource="http://capec.mitre.org/capec#ExampleInstance"/>
        <rdfs:range rdf:resource="http://capec.mitre.org/capec#structuredText"/>
        <rdfs:comment>Specifies in detail a specific example or exploit instance of this attack. It should outline the context of the attack, the targeted software, the targeted weaknesses or vulnerabilities, the specific set of actions involved in the attack and the resulting impact of the attacks success or failure (in the case of counterexamples).</rdfs:comment>
        <rdfs:label>Description</rdfs:label>
    </owl:DatatypeProperty>
    


    <!-- http://capec.mitre.org/capec#extendedDescription -->

    <owl:DatatypeProperty rdf:about="http://capec.mitre.org/capec#extendedDescription">
        <rdfs:domain rdf:resource="http://capec.mitre.org/capec#Audience"/>
        <rdfs:domain rdf:resource="http://capec.mitre.org/capec#Category"/>
        <rdfs:domain rdf:resource="http://capec.mitre.org/capec#CompoundElement"/>
        <rdfs:domain rdf:resource="http://capec.mitre.org/capec#IndicatorWarning"/>
        <rdfs:domain rdf:resource="http://capec.mitre.org/capec#ObfuscationTechnique"/>
        <rdfs:domain rdf:resource="http://capec.mitre.org/capec#ProbingTechnique"/>
        <rdfs:domain rdf:resource="http://capec.mitre.org/capec#Term"/>
        <rdfs:range rdf:resource="http://capec.mitre.org/capec#structuredText"/>
        <rdfs:comment>Specifies a short description</rdfs:comment>
        <rdfs:label>Description</rdfs:label>
    </owl:DatatypeProperty>
    


    <!-- http://capec.mitre.org/capec#formattedIdentifier -->

    <owl:DatatypeProperty rdf:about="http://capec.mitre.org/capec#formattedIdentifier">
        <rdfs:domain rdf:resource="http://capec.mitre.org/capec#AttackPattern"/>
        <rdfs:domain rdf:resource="http://capec.mitre.org/capec#Category"/>
        <rdfs:domain rdf:resource="http://capec.mitre.org/capec#CompoundElement"/>
        <rdfs:domain rdf:resource="http://capec.mitre.org/capec#View"/>
        <rdfs:range rdf:resource="http://www.w3.org/2001/XMLSchema#string"/>
        <rdfs:comment>Specifies the Common Attack Pattern Enumeration and Classification (CAPEC) identifier associated with the entity.  The identifier should follow the CAPEC identifier pattern of &quot;CAPEC-nnnn&quot; where &apos;nnnnn&apos; specifies an numerically incrementing number.</rdfs:comment>
        <rdfs:label>Common Attack Pattern Enumeration and Classification (CAPEC) Identifier</rdfs:label>
    </owl:DatatypeProperty>
    


    <!-- http://capec.mitre.org/capec#functionalServiceId -->

    <owl:DatatypeProperty rdf:about="http://capec.mitre.org/capec#functionalServiceId">
        <rdfs:domain rdf:resource="http://capec.mitre.org/capec#FunctionalService"/>
        <rdfs:range rdf:resource="http://www.w3.org/2001/XMLSchema#integer"/>
        <rdfs:comment>Specifies the identifier for the Funcational Service</rdfs:comment>
        <rdfs:label>Functional Service Identifier</rdfs:label>
    </owl:DatatypeProperty>
    


    <!-- http://capec.mitre.org/capec#functionalServiceName -->

    <owl:DatatypeProperty rdf:about="http://capec.mitre.org/capec#functionalServiceName">
        <rdfs:domain rdf:resource="http://capec.mitre.org/capec#FunctionalService"/>
        <rdfs:range rdf:resource="http://www.w3.org/2001/XMLSchema#string"/>
        <rdfs:comment>Specifies the name associated with the Functional Service</rdfs:comment>
        <rdfs:label>Name</rdfs:label>
    </owl:DatatypeProperty>
    


    <!-- http://capec.mitre.org/capec#id -->

    <owl:DatatypeProperty rdf:about="http://capec.mitre.org/capec#id">
        <rdfs:domain rdf:resource="http://capec.mitre.org/capec#AttackPattern"/>
        <rdfs:domain rdf:resource="http://capec.mitre.org/capec#Category"/>
        <rdfs:domain rdf:resource="http://capec.mitre.org/capec#CompoundElement"/>
        <rdfs:domain rdf:resource="http://capec.mitre.org/capec#View"/>
        <rdfs:range rdf:resource="http://www.w3.org/2001/XMLSchema#integer"/>
        <rdfs:comment>Specifies the identifer of the Attack Pattern, Category, View</rdfs:comment>
        <rdfs:label>Attack Pattern Identifier</rdfs:label>
    </owl:DatatypeProperty>
    


    <!-- http://capec.mitre.org/capec#imageLocation -->

    <owl:DatatypeProperty rdf:about="http://capec.mitre.org/capec#imageLocation">
        <rdfs:range rdf:resource="http://www.w3.org/2001/XMLSchema#string"/>
        <rdfs:comment>Specifies the location of the image file</rdfs:comment>
        <rdfs:label>Image Location</rdfs:label>
    </owl:DatatypeProperty>
    


    <!-- http://capec.mitre.org/capec#imageTitle -->

    <owl:DatatypeProperty rdf:about="http://capec.mitre.org/capec#imageTitle">
        <rdfs:range rdf:resource="http://www.w3.org/2001/XMLSchema#string"/>
        <rdfs:comment>Specifies a brief title associated with the image</rdfs:comment>
        <rdfs:label>Image Title</rdfs:label>
    </owl:DatatypeProperty>
    


    <!-- http://capec.mitre.org/capec#impact.availability -->

    <owl:DatatypeProperty rdf:about="http://capec.mitre.org/capec#impact.availability">
        <rdfs:domain rdf:resource="http://capec.mitre.org/capec#AttackPattern"/>
        <rdfs:range rdf:resource="http://www.w3.org/2001/XMLSchema#string"/>
        <rdfs:comment>Specifies the typical impact of this pattern on the availability characteristics of the targeted 	software and related data.</rdfs:comment>
        <rdfs:label>Availability Impact</rdfs:label>
    </owl:DatatypeProperty>
    


    <!-- http://capec.mitre.org/capec#impact.confidentiality -->

    <owl:DatatypeProperty rdf:about="http://capec.mitre.org/capec#impact.confidentiality">
        <rdfs:domain rdf:resource="http://capec.mitre.org/capec#AttackPattern"/>
        <rdfs:range rdf:resource="http://www.w3.org/2001/XMLSchema#string"/>
        <rdfs:comment>Specifies the typical impact of this pattern on the confidentiality characteristics of the targeted software and related data.</rdfs:comment>
        <rdfs:label>Confidentiality Impact</rdfs:label>
    </owl:DatatypeProperty>
    


    <!-- http://capec.mitre.org/capec#impact.integrity -->

    <owl:DatatypeProperty rdf:about="http://capec.mitre.org/capec#impact.integrity">
        <rdfs:domain rdf:resource="http://capec.mitre.org/capec#AttackPattern"/>
        <rdfs:range rdf:resource="http://www.w3.org/2001/XMLSchema#string"/>
        <rdfs:comment>Specifies  the typical impact of this pattern on the integrity characteristics of the targeted software and related data.</rdfs:comment>
        <rdfs:label>Integrity Impact</rdfs:label>
    </owl:DatatypeProperty>
    


    <!-- http://capec.mitre.org/capec#impactDescription -->

    <owl:DatatypeProperty rdf:about="http://capec.mitre.org/capec#impactDescription">
        <rdfs:domain rdf:resource="http://capec.mitre.org/capec#TechnicalImpact"/>
        <rdfs:range rdf:resource="http://www.w3.org/2001/XMLSchema#string"/>
        <rdfs:comment></rdfs:comment>
        <rdfs:label>impact description</rdfs:label>
    </owl:DatatypeProperty>
    


    <!-- http://capec.mitre.org/capec#impactLikelihood -->

    <owl:DatatypeProperty rdf:about="http://capec.mitre.org/capec#impactLikelihood">
        <rdfs:domain rdf:resource="http://capec.mitre.org/capec#TechnicalImpact"/>
        <rdfs:range rdf:resource="http://www.w3.org/2001/XMLSchema#string"/>
        <rdfs:comment>Specifies a rough estimate of the likelihood of the attack pattern having an impact.</rdfs:comment>
        <rdfs:label>Impact Likelihood</rdfs:label>
    </owl:DatatypeProperty>
    


    <!-- http://capec.mitre.org/capec#impactType -->

    <owl:DatatypeProperty rdf:about="http://capec.mitre.org/capec#impactType">
        <rdfs:domain rdf:resource="http://capec.mitre.org/capec#TechnicalImpact"/>
        <rdfs:range rdf:resource="http://www.w3.org/2001/XMLSchema#string"/>
        <rdfs:comment>Specifies the technical impacts that can result from successful execution of this attack pattern</rdfs:comment>
        <rdfs:label>impact type</rdfs:label>
    </owl:DatatypeProperty>
    


    <!-- http://capec.mitre.org/capec#indicatorDescription -->

    <owl:DatatypeProperty rdf:about="http://capec.mitre.org/capec#indicatorDescription">
        <rdfs:domain rdf:resource="http://capec.mitre.org/capec#SusceptabiltyIndicator"/>
        <rdfs:range rdf:resource="http://capec.mitre.org/capec#structuredText"/>
        <rdfs:comment>Specifies a brief description of the indicator.</rdfs:comment>
        <rdfs:label>Description</rdfs:label>
    </owl:DatatypeProperty>
    


    <!-- http://capec.mitre.org/capec#indicatorId -->

    <owl:DatatypeProperty rdf:about="http://capec.mitre.org/capec#indicatorId">
        <rdfs:domain rdf:resource="http://capec.mitre.org/capec#SusceptabiltyIndicator"/>
        <rdfs:range rdf:resource="http://www.w3.org/2001/XMLSchema#integer"/>
        <rdfs:comment>Specifies an identifier for the Indicator</rdfs:comment>
        <rdfs:label>Indicator Identifier</rdfs:label>
    </owl:DatatypeProperty>
    


    <!-- http://capec.mitre.org/capec#indicatorType -->

    <owl:DatatypeProperty rdf:about="http://capec.mitre.org/capec#indicatorType">
        <rdfs:domain rdf:resource="http://capec.mitre.org/capec#SusceptabiltyIndicator"/>
        <rdfs:range>
            <rdfs:Datatype>
                <owl:oneOf>
                    <rdf:Description>
                        <rdf:type rdf:resource="http://www.w3.org/1999/02/22-rdf-syntax-ns#List"/>
                        <rdf:first rdf:datatype="http://www.w3.org/2001/XMLSchema#string">Inconclusive</rdf:first>
                        <rdf:rest>
                            <rdf:Description>
                                <rdf:type rdf:resource="http://www.w3.org/1999/02/22-rdf-syntax-ns#List"/>
                                <rdf:first rdf:datatype="http://www.w3.org/2001/XMLSchema#string">Negative</rdf:first>
                                <rdf:rest>
                                    <rdf:Description>
                                        <rdf:type rdf:resource="http://www.w3.org/1999/02/22-rdf-syntax-ns#List"/>
                                        <rdf:first rdf:datatype="http://www.w3.org/2001/XMLSchema#string">Positive</rdf:first>
                                        <rdf:rest rdf:resource="http://www.w3.org/1999/02/22-rdf-syntax-ns#nil"/>
                                    </rdf:Description>
                                </rdf:rest>
                            </rdf:Description>
                        </rdf:rest>
                    </rdf:Description>
                </owl:oneOf>
            </rdfs:Datatype>
        </rdfs:range>
        <rdfs:comment>Specifies a mandatory type that can be one of the values “Positive,” “Negative,” or “Inconclusive.” 

For example, a positive indicator of susceptibility to parameter tampering is the existence of parameters in the URL. Although it does not guarantee susceptibility, it indicates a cause for further examination. A negative indicator for the technique of privilege escalation is a lack of credentials and user identifiers in an application. Again, this is not a conclusive measure of resistance to attack, but an indicator that the attack step technique is unlikely to bear significant fruit. An inconclusive indicator of susceptibility to dynamic code injection is a page whose URL ends in .jsp, .asp, or .do but which has no visible explicit parameters. Such URLs typically indicate dynamic processing, but since no visible parameters are passed, it is inconclusive whether dynamic code could be injected into the application.</rdfs:comment>
        <rdfs:label>Indicator Type</rdfs:label>
    </owl:DatatypeProperty>
    


    <!-- http://capec.mitre.org/capec#injectionVector -->

    <owl:DatatypeProperty rdf:about="http://capec.mitre.org/capec#injectionVector">
        <rdfs:domain rdf:resource="http://capec.mitre.org/capec#AttackPattern"/>
        <rdfs:range rdf:resource="http://capec.mitre.org/capec#structuredText"/>
        <rdfs:comment>Specifies the mechanism and format of an input-driven attack of this type. Injection vectors take into account the grammar of an attack, the syntax accepted by the system, the position of various fields, and the ranges of data that are acceptable.</rdfs:comment>
        <rdfs:label>Injection Vector</rdfs:label>
    </owl:DatatypeProperty>
    


    <!-- http://capec.mitre.org/capec#keywords -->

    <owl:DatatypeProperty rdf:about="http://capec.mitre.org/capec#keywords">
        <rdfs:domain rdf:resource="http://capec.mitre.org/capec#AttackPattern"/>
        <rdfs:range rdf:resource="http://www.w3.org/2001/XMLSchema#string"/>
        <rdfs:comment>Specifies one or more keywords.  Keyword correspond to text strings used to tag and search CAPEC catalog data.</rdfs:comment>
        <rdfs:label>keywords</rdfs:label>
    </owl:DatatypeProperty>
    


    <!-- http://capec.mitre.org/capec#localReferenceId -->

    <owl:DatatypeProperty rdf:about="http://capec.mitre.org/capec#localReferenceId">
        <rdfs:domain rdf:resource="http://capec.mitre.org/capec#Reference"/>
        <rdfs:range rdf:resource="http://www.w3.org/2001/XMLSchema#string"/>
        <rdfs:comment>Specifies the local reference identifier for the reference</rdfs:comment>
        <rdfs:isDefinedBy rdf:datatype="http://www.w3.org/2001/XMLSchema#string">&lt;http://capec.mitre.org/capec&gt;</rdfs:isDefinedBy>
        <rdfs:label>local reference id</rdfs:label>
    </owl:DatatypeProperty>
    


    <!-- http://capec.mitre.org/capec#maintenanceNotes -->

    <owl:DatatypeProperty rdf:about="http://capec.mitre.org/capec#maintenanceNotes">
        <rdfs:domain rdf:resource="http://capec.mitre.org/capec#AttackPattern"/>
        <rdfs:domain rdf:resource="http://capec.mitre.org/capec#Category"/>
        <rdfs:domain rdf:resource="http://capec.mitre.org/capec#CompoundElement"/>
        <rdfs:domain rdf:resource="http://capec.mitre.org/capec#View"/>
        <rdfs:range rdf:resource="http://capec.mitre.org/capec#structuredText"/>
        <rdfs:comment>Specifies one or more maintenance notes which each contain significant maintenance tasks within this entry that still need to be addressed, such as clarifying the concepts involved or improving relationships. It should be filled out in any entry that is still undergoing significant review by the CAPEC team.</rdfs:comment>
        <rdfs:label>Maintenance Notes</rdfs:label>
    </owl:DatatypeProperty>
    


    <!-- http://capec.mitre.org/capec#methodsOfAttack -->

    <owl:DatatypeProperty rdf:about="http://capec.mitre.org/capec#methodsOfAttack">
        <rdfs:domain rdf:resource="http://capec.mitre.org/capec#AttackPattern"/>
        <rdfs:domain rdf:resource="http://capec.mitre.org/capec#Category"/>
        <rdfs:range rdf:resource="http://www.w3.org/2001/XMLSchema#string"/>
        <rdfs:comment>Specifies the mechanism of attack used by this pattern. This field can help define the applicable attack surface required for this attack.</rdfs:comment>
        <rdfs:label>Methods of Attack</rdfs:label>
    </owl:DatatypeProperty>
    


    <!-- http://capec.mitre.org/capec#otherNotes -->

    <owl:DatatypeProperty rdf:about="http://capec.mitre.org/capec#otherNotes">
        <rdfs:domain rdf:resource="http://capec.mitre.org/capec#AttackPattern"/>
        <rdfs:domain rdf:resource="http://capec.mitre.org/capec#Category"/>
        <rdfs:domain rdf:resource="http://capec.mitre.org/capec#CompoundElement"/>
        <rdfs:domain rdf:resource="http://capec.mitre.org/capec#View"/>
        <rdfs:range rdf:resource="http://capec.mitre.org/capec#structuredText"/>
        <rdfs:comment>Specifies one or more Note elements, each of which provide any additional notes or comments that cannot be captured using other elements. New elements might be defined in the future to contain this information. It should be filled out where needed.</rdfs:comment>
        <rdfs:label>Other Notes</rdfs:label>
    </owl:DatatypeProperty>
    


    <!-- http://capec.mitre.org/capec#outcomeDescription -->

    <owl:DatatypeProperty rdf:about="http://capec.mitre.org/capec#outcomeDescription">
        <rdfs:domain rdf:resource="http://capec.mitre.org/capec#Outcome"/>
        <rdfs:range rdf:resource="http://www.w3.org/2001/XMLSchema#string"/>
        <rdfs:comment>Specifies a brief description of the outcome</rdfs:comment>
        <rdfs:label>Description</rdfs:label>
    </owl:DatatypeProperty>
    


    <!-- http://capec.mitre.org/capec#outcomeId -->

    <owl:DatatypeProperty rdf:about="http://capec.mitre.org/capec#outcomeId">
        <rdfs:domain rdf:resource="http://capec.mitre.org/capec#Outcome"/>
        <rdfs:range rdf:resource="http://www.w3.org/2001/XMLSchema#integer"/>
        <rdfs:comment>Specifies a unique integer identifier for the outcome.</rdfs:comment>
        <rdfs:label>Outcome Identifier</rdfs:label>
    </owl:DatatypeProperty>
    


    <!-- http://capec.mitre.org/capec#outcomeType -->

    <owl:DatatypeProperty rdf:about="http://capec.mitre.org/capec#outcomeType">
        <rdfs:domain rdf:resource="http://capec.mitre.org/capec#Outcome"/>
        <rdfs:range>
            <rdfs:Datatype>
                <owl:oneOf>
                    <rdf:Description>
                        <rdf:type rdf:resource="http://www.w3.org/1999/02/22-rdf-syntax-ns#List"/>
                        <rdf:first rdf:datatype="http://www.w3.org/2001/XMLSchema#string">Failure</rdf:first>
                        <rdf:rest>
                            <rdf:Description>
                                <rdf:type rdf:resource="http://www.w3.org/1999/02/22-rdf-syntax-ns#List"/>
                                <rdf:first rdf:datatype="http://www.w3.org/2001/XMLSchema#string">Inconclusive</rdf:first>
                                <rdf:rest>
                                    <rdf:Description>
                                        <rdf:type rdf:resource="http://www.w3.org/1999/02/22-rdf-syntax-ns#List"/>
                                        <rdf:first rdf:datatype="http://www.w3.org/2001/XMLSchema#string">Success</rdf:first>
                                        <rdf:rest rdf:resource="http://www.w3.org/1999/02/22-rdf-syntax-ns#nil"/>
                                    </rdf:Description>
                                </rdf:rest>
                            </rdf:Description>
                        </rdf:rest>
                    </rdf:Description>
                </owl:oneOf>
            </rdfs:Datatype>
        </rdfs:range>
        <rdfs:comment>Specifies what results of executing the attack step techniques should be considered &quot;success&quot;, which should be considered &quot;failure&quot;, and which ones are &quot;inconclusive&quot;.  Outcomes’ successes are determined relative to the attacker’s point of view. It is a success if the attack step got the attacker closer to his goal of attacking the application. It is a failure if the attacker got no closer to his goal.</rdfs:comment>
        <rdfs:label>Outcome Type</rdfs:label>
    </owl:DatatypeProperty>
    


    <!-- http://capec.mitre.org/capec#patternAbstraction -->

    <owl:DatatypeProperty rdf:about="http://capec.mitre.org/capec#patternAbstraction">
        <rdfs:domain rdf:resource="http://capec.mitre.org/capec#AttackPattern"/>
        <rdfs:range>
            <rdfs:Datatype>
                <owl:oneOf>
                    <rdf:Description>
                        <rdf:type rdf:resource="http://www.w3.org/1999/02/22-rdf-syntax-ns#List"/>
                        <rdf:first rdf:datatype="http://www.w3.org/2001/XMLSchema#string">Detailed</rdf:first>
                        <rdf:rest>
                            <rdf:Description>
                                <rdf:type rdf:resource="http://www.w3.org/1999/02/22-rdf-syntax-ns#List"/>
                                <rdf:first rdf:datatype="http://www.w3.org/2001/XMLSchema#string">Meta</rdf:first>
                                <rdf:rest>
                                    <rdf:Description>
                                        <rdf:type rdf:resource="http://www.w3.org/1999/02/22-rdf-syntax-ns#List"/>
                                        <rdf:first rdf:datatype="http://www.w3.org/2001/XMLSchema#string">Standard</rdf:first>
                                        <rdf:rest rdf:resource="http://www.w3.org/1999/02/22-rdf-syntax-ns#nil"/>
                                    </rdf:Description>
                                </rdf:rest>
                            </rdf:Description>
                        </rdf:rest>
                    </rdf:Description>
                </owl:oneOf>
            </rdfs:Datatype>
        </rdfs:range>
        <rdfs:comment>Specifies an abstraction level for the pattern which helps guide the appropriate information needed forits definition aswell aswhere and how it is most usefully leveraged.

Acceptable values are &quot;Meta&quot; which is technology and functional context non-specific and often defines approachesto thinking on how to violate assumptions made in software , &quot;Standard&quot; which is typically functional context-specific but technology context nonspecific and often defines actionable approach to exploiting specific weaknesses in software, and &quot;Detailed&quot; which is technology and/or functional context specific and often defines specific delivery vector and/or attack content.</rdfs:comment>
        <rdfs:label>Pattern Abstraction Level</rdfs:label>
    </owl:DatatypeProperty>
    


    <!-- http://capec.mitre.org/capec#patternCompleteness -->

    <owl:DatatypeProperty rdf:about="http://capec.mitre.org/capec#patternCompleteness">
        <rdfs:domain rdf:resource="http://capec.mitre.org/capec#AttackPattern"/>
        <rdfs:range>
            <rdfs:Datatype>
                <owl:oneOf>
                    <rdf:Description>
                        <rdf:type rdf:resource="http://www.w3.org/1999/02/22-rdf-syntax-ns#List"/>
                        <rdf:first rdf:datatype="http://www.w3.org/2001/XMLSchema#string">Complete</rdf:first>
                        <rdf:rest>
                            <rdf:Description>
                                <rdf:type rdf:resource="http://www.w3.org/1999/02/22-rdf-syntax-ns#List"/>
                                <rdf:first rdf:datatype="http://www.w3.org/2001/XMLSchema#string">Hook</rdf:first>
                                <rdf:rest>
                                    <rdf:Description>
                                        <rdf:type rdf:resource="http://www.w3.org/1999/02/22-rdf-syntax-ns#List"/>
                                        <rdf:first rdf:datatype="http://www.w3.org/2001/XMLSchema#string">Stub</rdf:first>
                                        <rdf:rest rdf:resource="http://www.w3.org/1999/02/22-rdf-syntax-ns#nil"/>
                                    </rdf:Description>
                                </rdf:rest>
                            </rdf:Description>
                        </rdf:rest>
                    </rdf:Description>
                </owl:oneOf>
            </rdfs:Datatype>
        </rdfs:range>
        <rdfs:comment>Specifies the completeness of the attack pattern</rdfs:comment>
        <rdfs:label>Pattern Completeness</rdfs:label>
    </owl:DatatypeProperty>
    


    <!-- http://capec.mitre.org/capec#payload -->

    <owl:DatatypeProperty rdf:about="http://capec.mitre.org/capec#payload">
        <rdfs:domain rdf:resource="http://capec.mitre.org/capec#AttackPattern"/>
        <rdfs:range rdf:resource="http://capec.mitre.org/capec#structuredText"/>
        <rdfs:comment>Specifies the code, configuration or other data to be executed or otherwise activated as part of an injection-based attack of this type.</rdfs:comment>
        <rdfs:label>Payload</rdfs:label>
    </owl:DatatypeProperty>
    


    <!-- http://capec.mitre.org/capec#payloadActivationImpact.description -->

    <owl:DatatypeProperty rdf:about="http://capec.mitre.org/capec#payloadActivationImpact.description">
        <rdfs:domain rdf:resource="http://capec.mitre.org/capec#AttackPattern"/>
        <rdfs:range rdf:resource="http://capec.mitre.org/capec#structuredText"/>
        <rdfs:comment>Specifies an explanatory description of the payload activation impact.</rdfs:comment>
        <rdfs:isDefinedBy rdf:resource="http://capec.mitre.org/capec"/>
        <rdfs:label>Payload Activation Impact Description</rdfs:label>
    </owl:DatatypeProperty>
    


    <!-- http://capec.mitre.org/capec#phaseId -->

    <owl:DatatypeProperty rdf:about="http://capec.mitre.org/capec#phaseId">
        <rdfs:domain rdf:resource="http://capec.mitre.org/capec#AttackPhase"/>
        <rdfs:range rdf:resource="http://www.w3.org/2001/XMLSchema#integer"/>
        <rdfs:comment>Specifies the identifier of the attack phase</rdfs:comment>
        <rdfs:label>Attack Phase Id</rdfs:label>
    </owl:DatatypeProperty>
    


    <!-- http://capec.mitre.org/capec#phaseName -->

    <owl:DatatypeProperty rdf:about="http://capec.mitre.org/capec#phaseName">
        <rdfs:domain rdf:resource="http://capec.mitre.org/capec#AttackPhase"/>
        <rdfs:range>
            <rdfs:Datatype>
                <owl:oneOf>
                    <rdf:Description>
                        <rdf:type rdf:resource="http://www.w3.org/1999/02/22-rdf-syntax-ns#List"/>
                        <rdf:first rdf:datatype="http://www.w3.org/2001/XMLSchema#string">Experiment</rdf:first>
                        <rdf:rest>
                            <rdf:Description>
                                <rdf:type rdf:resource="http://www.w3.org/1999/02/22-rdf-syntax-ns#List"/>
                                <rdf:first rdf:datatype="http://www.w3.org/2001/XMLSchema#string">Exploit</rdf:first>
                                <rdf:rest>
                                    <rdf:Description>
                                        <rdf:type rdf:resource="http://www.w3.org/1999/02/22-rdf-syntax-ns#List"/>
                                        <rdf:first rdf:datatype="http://www.w3.org/2001/XMLSchema#string">Explore</rdf:first>
                                        <rdf:rest rdf:resource="http://www.w3.org/1999/02/22-rdf-syntax-ns#nil"/>
                                    </rdf:Description>
                                </rdf:rest>
                            </rdf:Description>
                        </rdf:rest>
                    </rdf:Description>
                </owl:oneOf>
            </rdfs:Datatype>
        </rdfs:range>
        <rdfs:comment>Specifies the name of the attack phase</rdfs:comment>
        <rdfs:label>Attack Phase Name</rdfs:label>
    </owl:DatatypeProperty>
    


    <!-- http://capec.mitre.org/capec#previousEntryName -->

    <owl:DatatypeProperty rdf:about="http://capec.mitre.org/capec#previousEntryName">
        <rdfs:domain rdf:resource="http://capec.mitre.org/capec#HistoryRecord"/>
        <rdfs:range rdf:resource="http://www.w3.org/2001/XMLSchema#string"/>
        <rdfs:comment>Specifies the previous name for this entry.</rdfs:comment>
        <rdfs:label>Previous Name</rdfs:label>
    </owl:DatatypeProperty>
    


    <!-- http://capec.mitre.org/capec#purposes -->

    <owl:DatatypeProperty rdf:about="http://capec.mitre.org/capec#purposes">
        <rdfs:domain rdf:resource="http://capec.mitre.org/capec#AttackPattern"/>
        <rdfs:range>
            <rdfs:Datatype>
                <owl:oneOf>
                    <rdf:Description>
                        <rdf:type rdf:resource="http://www.w3.org/1999/02/22-rdf-syntax-ns#List"/>
                        <rdf:first rdf:datatype="http://www.w3.org/2001/XMLSchema#string">Exploitation</rdf:first>
                        <rdf:rest>
                            <rdf:Description>
                                <rdf:type rdf:resource="http://www.w3.org/1999/02/22-rdf-syntax-ns#List"/>
                                <rdf:first rdf:datatype="http://www.w3.org/2001/XMLSchema#string">Obfuscation</rdf:first>
                                <rdf:rest>
                                    <rdf:Description>
                                        <rdf:type rdf:resource="http://www.w3.org/1999/02/22-rdf-syntax-ns#List"/>
                                        <rdf:first rdf:datatype="http://www.w3.org/2001/XMLSchema#string">Penetration</rdf:first>
                                        <rdf:rest>
                                            <rdf:Description>
                                                <rdf:type rdf:resource="http://www.w3.org/1999/02/22-rdf-syntax-ns#List"/>
                                                <rdf:first rdf:datatype="http://www.w3.org/2001/XMLSchema#string">Reconnaissance</rdf:first>
                                                <rdf:rest rdf:resource="http://www.w3.org/1999/02/22-rdf-syntax-ns#nil"/>
                                            </rdf:Description>
                                        </rdf:rest>
                                    </rdf:Description>
                                </rdf:rest>
                            </rdf:Description>
                        </rdf:rest>
                    </rdf:Description>
                </owl:oneOf>
            </rdfs:Datatype>
        </rdfs:range>
        <rdfs:comment>Specifies one or more purposes.  Purpose refers to the intended purpose behind the attack pattern relative to an enumerated list of attack objectives. 

USAGE: This element is used to capture pattern composibility and assist with normalization and classification of attack patterns within the CAPEC catalog.</rdfs:comment>
        <rdfs:label>Purposes</rdfs:label>
    </owl:DatatypeProperty>
    


    <!-- http://capec.mitre.org/capec#referenceAuthorName -->

    <owl:DatatypeProperty rdf:about="http://capec.mitre.org/capec#referenceAuthorName">
        <rdfs:domain rdf:resource="http://capec.mitre.org/capec#Reference"/>
        <rdfs:range rdf:resource="http://www.w3.org/2001/XMLSchema#string"/>
        <rdfs:comment>Specifies the name of an individual author of the material being referenced. It is not required, but may be repeated sequentially in order to identify multiple authors for a single piece of material.</rdfs:comment>
        <rdfs:label>Reference Author</rdfs:label>
    </owl:DatatypeProperty>
    


    <!-- http://capec.mitre.org/capec#referenceDate -->

    <owl:DatatypeProperty rdf:about="http://capec.mitre.org/capec#referenceDate">
        <rdfs:domain rdf:resource="http://capec.mitre.org/capec#Reference"/>
        <rdfs:range rdf:resource="http://www.w3.org/2001/XMLSchema#date"/>
        <rdfs:comment>Specifies the date when the reference was included in the entry. This provides the reader with a time line for when the material in the reference, usually the link, was valid. The date should be of the format YYYY-MM-DD.</rdfs:comment>
        <rdfs:label>Reference Date</rdfs:label>
    </owl:DatatypeProperty>
    


    <!-- http://capec.mitre.org/capec#referenceDescription -->

    <owl:DatatypeProperty rdf:about="http://capec.mitre.org/capec#referenceDescription">
        <rdfs:domain rdf:resource="http://capec.mitre.org/capec#Reference"/>
        <rdfs:range rdf:resource="http://www.w3.org/2001/XMLSchema#string"/>
        <rdfs:comment>Specifies a brief description of the reference</rdfs:comment>
        <rdfs:label>Reference Description</rdfs:label>
    </owl:DatatypeProperty>
    


    <!-- http://capec.mitre.org/capec#referenceEdition -->

    <owl:DatatypeProperty rdf:about="http://capec.mitre.org/capec#referenceEdition">
        <rdfs:domain rdf:resource="http://capec.mitre.org/capec#Reference"/>
        <rdfs:range rdf:resource="http://www.w3.org/2001/XMLSchema#string"/>
        <rdfs:comment>Specifies the edition of the material being referenced in the event that multiple editions of the material exist. This will usually only be useful for book references.</rdfs:comment>
        <rdfs:label>Reference Edition</rdfs:label>
    </owl:DatatypeProperty>
    


    <!-- http://capec.mitre.org/capec#referenceId -->

    <owl:DatatypeProperty rdf:about="http://capec.mitre.org/capec#referenceId">
        <rdfs:domain rdf:resource="http://capec.mitre.org/capec#Reference"/>
        <rdfs:range rdf:resource="http://www.w3.org/2001/XMLSchema#string"/>
        <rdfs:comment>Specifies a mechanism forciting text in the entry. If an id is provided, it is placed between brackets and precedes this reference and the matching id should be used inside of the text for the attack pattern itself where this reference is applicable. All reference ids assigned within an entry must be unique.</rdfs:comment>
        <rdfs:label>Reference Identifier</rdfs:label>
    </owl:DatatypeProperty>
    


    <!-- http://capec.mitre.org/capec#referenceLink -->

    <owl:DatatypeProperty rdf:about="http://capec.mitre.org/capec#referenceLink">
        <rdfs:domain rdf:resource="http://capec.mitre.org/capec#Reference"/>
        <rdfs:range rdf:resource="http://www.w3.org/2001/XMLSchema#anyURI"/>
        <rdfs:comment>Specifies the URL for the material being referenced, if one exists. This should always be used for web references, and may optionally be used for book and other publication references.</rdfs:comment>
        <rdfs:label>Reference Link</rdfs:label>
    </owl:DatatypeProperty>
    


    <!-- http://capec.mitre.org/capec#referencePubDate -->

    <owl:DatatypeProperty rdf:about="http://capec.mitre.org/capec#referencePubDate">
        <rdfs:domain rdf:resource="http://capec.mitre.org/capec#Reference"/>
        <rdfs:range rdf:resource="http://www.w3.org/2001/XMLSchema#gYear"/>
        <rdfs:comment>Specifies the date when the reference was published YYYY.</rdfs:comment>
        <rdfs:label>Publication Date</rdfs:label>
    </owl:DatatypeProperty>
    


    <!-- http://capec.mitre.org/capec#referencePublication -->

    <owl:DatatypeProperty rdf:about="http://capec.mitre.org/capec#referencePublication">
        <rdfs:domain rdf:resource="http://capec.mitre.org/capec#Reference"/>
        <rdfs:range rdf:resource="http://www.w3.org/2001/XMLSchema#string"/>
        <rdfs:comment>Specifies the publication source of the reference material, if one exists.</rdfs:comment>
        <rdfs:label>Publication</rdfs:label>
    </owl:DatatypeProperty>
    


    <!-- http://capec.mitre.org/capec#referencePublisherName -->

    <owl:DatatypeProperty rdf:about="http://capec.mitre.org/capec#referencePublisherName">
        <rdfs:domain rdf:resource="http://capec.mitre.org/capec#Reference"/>
        <rdfs:range rdf:resource="http://www.w3.org/2001/XMLSchema#string"/>
        <rdfs:comment>Specifies the name of the publisher of the reference material, if one exists.</rdfs:comment>
        <rdfs:label>Publisher</rdfs:label>
    </owl:DatatypeProperty>
    


    <!-- http://capec.mitre.org/capec#referenceSection -->

    <owl:DatatypeProperty rdf:about="http://capec.mitre.org/capec#referenceSection">
        <rdfs:domain rdf:resource="http://capec.mitre.org/capec#Reference"/>
        <rdfs:range rdf:resource="http://www.w3.org/2001/XMLSchema#string"/>
        <rdfs:comment>Specifies a means of identifying the exact location of the material inside of the publication source, such as the relevant pages of a research paper, the appropriate chapters from a book, etc. This is useful for both book references and internet references.</rdfs:comment>
        <rdfs:label>Section</rdfs:label>
    </owl:DatatypeProperty>
    


    <!-- http://capec.mitre.org/capec#referenceTitle -->

    <owl:DatatypeProperty rdf:about="http://capec.mitre.org/capec#referenceTitle">
        <rdfs:domain rdf:resource="http://capec.mitre.org/capec#Reference"/>
        <rdfs:range rdf:resource="http://www.w3.org/2001/XMLSchema#string"/>
        <rdfs:comment>Specifies the title of the material beingreferenced. It is not required if the material does not have a title.</rdfs:comment>
        <rdfs:label>Title</rdfs:label>
    </owl:DatatypeProperty>
    


    <!-- http://capec.mitre.org/capec#relatedGuidelines -->

    <owl:DatatypeProperty rdf:about="http://capec.mitre.org/capec#relatedGuidelines">
        <rdfs:domain rdf:resource="http://capec.mitre.org/capec#AttackPattern"/>
        <rdfs:range rdf:resource="http://capec.mitre.org/capec#structuredText"/>
        <rdfs:comment>Specifies one or more related guidelines. A related guideline represents a security guideline that is relevant to identifying or mitigating this type of attack. 

USAGE: It would be helpful to provide a usage reference.  However links to security principle and guideline documentation on the BSI site appear to be broken. NIST SP 800-27 uses the terms principle and guideline interchangeably.</rdfs:comment>
        <rdfs:label>Related Guidelines</rdfs:label>
    </owl:DatatypeProperty>
    


    <!-- http://capec.mitre.org/capec#relatedSecurityPrinciples -->

    <owl:DatatypeProperty rdf:about="http://capec.mitre.org/capec#relatedSecurityPrinciples">
        <rdfs:domain rdf:resource="http://capec.mitre.org/capec#AttackPattern"/>
        <rdfs:range rdf:resource="http://capec.mitre.org/capec#structuredText"/>
        <rdfs:comment>Specifies one or more related security principles. A principle is defined as a rule or standard for good behavior. A related security principle is a security rule or practice that impedes this attack pattern. 

USAGE: Usage defined in NIST SP 800-27A, &quot;Engineering Principles for Information Technology Security&quot;, Revision A.</rdfs:comment>
        <rdfs:label>Related Security Principles</rdfs:label>
    </owl:DatatypeProperty>
    


    <!-- http://capec.mitre.org/capec#relationshipDescription -->

    <owl:DatatypeProperty rdf:about="http://capec.mitre.org/capec#relationshipDescription">
        <rdfs:domain rdf:resource="http://capec.mitre.org/capec#RelationshipStatement"/>
        <rdfs:range rdf:resource="http://capec.mitre.org/capec#structuredText"/>
        <rdfs:comment>Specifies a short description of the relationship.</rdfs:comment>
        <rdfs:label>Relationship Description</rdfs:label>
    </owl:DatatypeProperty>
    


    <!-- http://capec.mitre.org/capec#relationshipNature -->

    <owl:DatatypeProperty rdf:about="http://capec.mitre.org/capec#relationshipNature">
        <rdfs:domain rdf:resource="http://capec.mitre.org/capec#RelationshipStatement"/>
        <rdfs:range>
            <rdfs:Datatype>
                <owl:oneOf>
                    <rdf:Description>
                        <rdf:type rdf:resource="http://www.w3.org/1999/02/22-rdf-syntax-ns#List"/>
                        <rdf:first rdf:datatype="http://www.w3.org/2001/XMLSchema#string">CanAlsoBe</rdf:first>
                        <rdf:rest>
                            <rdf:Description>
                                <rdf:type rdf:resource="http://www.w3.org/1999/02/22-rdf-syntax-ns#List"/>
                                <rdf:first rdf:datatype="http://www.w3.org/2001/XMLSchema#string">CanFollow</rdf:first>
                                <rdf:rest>
                                    <rdf:Description>
                                        <rdf:type rdf:resource="http://www.w3.org/1999/02/22-rdf-syntax-ns#List"/>
                                        <rdf:first rdf:datatype="http://www.w3.org/2001/XMLSchema#string">CanPrecede</rdf:first>
                                        <rdf:rest>
                                            <rdf:Description>
                                                <rdf:type rdf:resource="http://www.w3.org/1999/02/22-rdf-syntax-ns#List"/>
                                                <rdf:first rdf:datatype="http://www.w3.org/2001/XMLSchema#string">ChildOf</rdf:first>
                                                <rdf:rest>
                                                    <rdf:Description>
                                                        <rdf:type rdf:resource="http://www.w3.org/1999/02/22-rdf-syntax-ns#List"/>
                                                        <rdf:first rdf:datatype="http://www.w3.org/2001/XMLSchema#string">HasMember</rdf:first>
                                                        <rdf:rest>
                                                            <rdf:Description>
                                                                <rdf:type rdf:resource="http://www.w3.org/1999/02/22-rdf-syntax-ns#List"/>
                                                                <rdf:first rdf:datatype="http://www.w3.org/2001/XMLSchema#string">MemberOf</rdf:first>
                                                                <rdf:rest>
                                                                    <rdf:Description>
                                                                        <rdf:type rdf:resource="http://www.w3.org/1999/02/22-rdf-syntax-ns#List"/>
                                                                        <rdf:first rdf:datatype="http://www.w3.org/2001/XMLSchema#string">ParentOf</rdf:first>
                                                                        <rdf:rest>
                                                                            <rdf:Description>
                                                                                <rdf:type rdf:resource="http://www.w3.org/1999/02/22-rdf-syntax-ns#List"/>
                                                                                <rdf:first rdf:datatype="http://www.w3.org/2001/XMLSchema#string">PeerOf</rdf:first>
                                                                                <rdf:rest>
                                                                                    <rdf:Description>
                                                                                        <rdf:type rdf:resource="http://www.w3.org/1999/02/22-rdf-syntax-ns#List"/>
                                                                                        <rdf:first rdf:datatype="http://www.w3.org/2001/XMLSchema#string">RequiredBy</rdf:first>
                                                                                        <rdf:rest>
                                                                                            <rdf:Description>
                                                                                                <rdf:type rdf:resource="http://www.w3.org/1999/02/22-rdf-syntax-ns#List"/>
                                                                                                <rdf:first rdf:datatype="http://www.w3.org/2001/XMLSchema#string">Requires</rdf:first>
                                                                                                <rdf:rest>
                                                                                                    <rdf:Description>
                                                                                                        <rdf:type rdf:resource="http://www.w3.org/1999/02/22-rdf-syntax-ns#List"/>
                                                                                                        <rdf:first rdf:datatype="http://www.w3.org/2001/XMLSchema#string">StartsChain</rdf:first>
                                                                                                        <rdf:rest>
                                                                                                            <rdf:Description>
                                                                                                                <rdf:type rdf:resource="http://www.w3.org/1999/02/22-rdf-syntax-ns#List"/>
                                                                                                                <rdf:first rdf:datatype="http://www.w3.org/2001/XMLSchema#string">StartsWith</rdf:first>
                                                                                                                <rdf:rest rdf:resource="http://www.w3.org/1999/02/22-rdf-syntax-ns#nil"/>
                                                                                                            </rdf:Description>
                                                                                                        </rdf:rest>
                                                                                                    </rdf:Description>
                                                                                                </rdf:rest>
                                                                                            </rdf:Description>
                                                                                        </rdf:rest>
                                                                                    </rdf:Description>
                                                                                </rdf:rest>
                                                                            </rdf:Description>
                                                                        </rdf:rest>
                                                                    </rdf:Description>
                                                                </rdf:rest>
                                                            </rdf:Description>
                                                        </rdf:rest>
                                                    </rdf:Description>
                                                </rdf:rest>
                                            </rdf:Description>
                                        </rdf:rest>
                                    </rdf:Description>
                                </rdf:rest>
                            </rdf:Description>
                        </rdf:rest>
                    </rdf:Description>
                </owl:oneOf>
            </rdfs:Datatype>
        </rdfs:range>
        <rdfs:comment>Specifies the nature of the relationship between this element and the target element, such as ChildOf, HasMember or Requires to name a few.</rdfs:comment>
        <rdfs:label>relationship nature</rdfs:label>
    </owl:DatatypeProperty>
    


    <!-- http://capec.mitre.org/capec#relationshipNotes -->

    <owl:DatatypeProperty rdf:about="http://capec.mitre.org/capec#relationshipNotes">
        <rdfs:domain rdf:resource="http://capec.mitre.org/capec#Category"/>
        <rdfs:domain rdf:resource="http://capec.mitre.org/capec#CompoundElement"/>
        <rdfs:domain rdf:resource="http://capec.mitre.org/capec#View"/>
        <rdfs:range rdf:resource="http://capec.mitre.org/capec#structuredText"/>
        <rdfs:comment>Specifies details regarding the relationships between CAPEC entries.</rdfs:comment>
        <rdfs:label>Relationship Notes</rdfs:label>
    </owl:DatatypeProperty>
    


    <!-- http://capec.mitre.org/capec#relationshipTargetForm -->

    <owl:DatatypeProperty rdf:about="http://capec.mitre.org/capec#relationshipTargetForm">
        <rdfs:domain rdf:resource="http://capec.mitre.org/capec#RelationshipStatement"/>
        <rdfs:range>
            <rdfs:Datatype>
                <owl:oneOf>
                    <rdf:Description>
                        <rdf:type rdf:resource="http://www.w3.org/1999/02/22-rdf-syntax-ns#List"/>
                        <rdf:first rdf:datatype="http://www.w3.org/2001/XMLSchema#string">Attack Pattern</rdf:first>
                        <rdf:rest>
                            <rdf:Description>
                                <rdf:type rdf:resource="http://www.w3.org/1999/02/22-rdf-syntax-ns#List"/>
                                <rdf:first rdf:datatype="http://www.w3.org/2001/XMLSchema#string">Category</rdf:first>
                                <rdf:rest>
                                    <rdf:Description>
                                        <rdf:type rdf:resource="http://www.w3.org/1999/02/22-rdf-syntax-ns#List"/>
                                        <rdf:first rdf:datatype="http://www.w3.org/2001/XMLSchema#string">Compound Element</rdf:first>
                                        <rdf:rest>
                                            <rdf:Description>
                                                <rdf:type rdf:resource="http://www.w3.org/1999/02/22-rdf-syntax-ns#List"/>
                                                <rdf:first rdf:datatype="http://www.w3.org/2001/XMLSchema#string">View</rdf:first>
                                                <rdf:rest rdf:resource="http://www.w3.org/1999/02/22-rdf-syntax-ns#nil"/>
                                            </rdf:Description>
                                        </rdf:rest>
                                    </rdf:Description>
                                </rdf:rest>
                            </rdf:Description>
                        </rdf:rest>
                    </rdf:Description>
                </owl:oneOf>
            </rdfs:Datatype>
        </rdfs:range>
        <rdfs:comment>Specifies the form of the target of this relationship, such as Category, Attack Pattern, View or Compound_Element.</rdfs:comment>
        <rdfs:label>relationship target form</rdfs:label>
    </owl:DatatypeProperty>
    


    <!-- http://capec.mitre.org/capec#relationshipType -->

    <owl:DatatypeProperty rdf:about="http://capec.mitre.org/capec#relationshipType">
        <rdfs:domain rdf:resource="http://capec.mitre.org/capec#RelatedProtocolStatement"/>
        <rdfs:range>
            <rdfs:Datatype>
                <owl:oneOf>
                    <rdf:Description>
                        <rdf:type rdf:resource="http://www.w3.org/1999/02/22-rdf-syntax-ns#List"/>
                        <rdf:first rdf:datatype="http://www.w3.org/2001/XMLSchema#string">Is a command of</rdf:first>
                        <rdf:rest>
                            <rdf:Description>
                                <rdf:type rdf:resource="http://www.w3.org/1999/02/22-rdf-syntax-ns#List"/>
                                <rdf:first rdf:datatype="http://www.w3.org/2001/XMLSchema#string">Is a refinement of</rdf:first>
                                <rdf:rest>
                                    <rdf:Description>
                                        <rdf:type rdf:resource="http://www.w3.org/1999/02/22-rdf-syntax-ns#List"/>
                                        <rdf:first rdf:datatype="http://www.w3.org/2001/XMLSchema#string">Is a service of</rdf:first>
                                        <rdf:rest>
                                            <rdf:Description>
                                                <rdf:type rdf:resource="http://www.w3.org/1999/02/22-rdf-syntax-ns#List"/>
                                                <rdf:first rdf:datatype="http://www.w3.org/2001/XMLSchema#string">Is an abstraction of</rdf:first>
                                                <rdf:rest>
                                                    <rdf:Description>
                                                        <rdf:type rdf:resource="http://www.w3.org/1999/02/22-rdf-syntax-ns#List"/>
                                                        <rdf:first rdf:datatype="http://www.w3.org/2001/XMLSchema#string">Is an alternative to</rdf:first>
                                                        <rdf:rest>
                                                            <rdf:Description>
                                                                <rdf:type rdf:resource="http://www.w3.org/1999/02/22-rdf-syntax-ns#List"/>
                                                                <rdf:first rdf:datatype="http://www.w3.org/2001/XMLSchema#string">Uses Protocol</rdf:first>
                                                                <rdf:rest rdf:resource="http://www.w3.org/1999/02/22-rdf-syntax-ns#nil"/>
                                                            </rdf:Description>
                                                        </rdf:rest>
                                                    </rdf:Description>
                                                </rdf:rest>
                                            </rdf:Description>
                                        </rdf:rest>
                                    </rdf:Description>
                                </rdf:rest>
                            </rdf:Description>
                        </rdf:rest>
                    </rdf:Description>
                </owl:oneOf>
            </rdfs:Datatype>
        </rdfs:range>
        <rdfs:comment>Specifies the type of relationship</rdfs:comment>
        <rdfs:label>Relationship Type</rdfs:label>
    </owl:DatatypeProperty>
    


    <!-- http://capec.mitre.org/capec#relationshipViewOrdinal -->

    <owl:DatatypeProperty rdf:about="http://capec.mitre.org/capec#relationshipViewOrdinal">
        <rdfs:range>
            <rdfs:Datatype>
                <owl:oneOf>
                    <rdf:Description>
                        <rdf:type rdf:resource="http://www.w3.org/1999/02/22-rdf-syntax-ns#List"/>
                        <rdf:first rdf:datatype="http://www.w3.org/2001/XMLSchema#string">Primary</rdf:first>
                        <rdf:rest rdf:resource="http://www.w3.org/1999/02/22-rdf-syntax-ns#nil"/>
                    </rdf:Description>
                </owl:oneOf>
            </rdfs:Datatype>
        </rdfs:range>
        <rdfs:comment>Specifies if this relationship is the primary ChildOf relationship for this entry for a given RelationshipView element.. This attribute can only have the value &quot;Primary&quot; and should only be included for the primary parent/child relationship.</rdfs:comment>
        <rdfs:label>Relationship View Ordinal</rdfs:label>
    </owl:DatatypeProperty>
    


    <!-- http://capec.mitre.org/capec#relativeId -->

    <owl:DatatypeProperty rdf:about="http://capec.mitre.org/capec#relativeId">
        <rdfs:domain rdf:resource="http://capec.mitre.org/capec#AttackPhase"/>
        <rdfs:domain rdf:resource="http://capec.mitre.org/capec#AttackStep"/>
        <rdfs:domain rdf:resource="http://capec.mitre.org/capec#AttackStepTechnique"/>
        <rdfs:domain rdf:resource="http://capec.mitre.org/capec#CommonAttackSurfaceDescription"/>
        <rdfs:domain rdf:resource="http://capec.mitre.org/capec#Consequence"/>
        <rdfs:domain rdf:resource="http://capec.mitre.org/capec#ExampleInstance"/>
        <rdfs:domain rdf:resource="http://capec.mitre.org/capec#HistoryRecord"/>
        <rdfs:domain rdf:resource="http://capec.mitre.org/capec#IndicatorWarning"/>
        <rdfs:domain rdf:resource="http://capec.mitre.org/capec#Knowlege"/>
        <rdfs:domain rdf:resource="http://capec.mitre.org/capec#ObfuscationTechnique"/>
        <rdfs:domain rdf:resource="http://capec.mitre.org/capec#Outcome"/>
        <rdfs:domain rdf:resource="http://capec.mitre.org/capec#ProbingTechnique"/>
        <rdfs:domain rdf:resource="http://capec.mitre.org/capec#SecurityControl"/>
        <rdfs:domain rdf:resource="http://capec.mitre.org/capec#SusceptabiltyIndicator"/>
        <rdfs:domain rdf:resource="http://capec.mitre.org/capec#TargetAttackSurfaceDescription"/>
        <rdfs:domain rdf:resource="http://capec.mitre.org/capec#TargetedProtocol"/>
        <rdfs:range rdf:resource="http://www.w3.org/2001/XMLSchema#string"/>
        <rdfs:comment>Specifies an identifier for the related entity.  Only one relative ID element can exist for each entity (ex: R.78.1). Text citing this reference should use the format [R.78.1] where &quot;R&quot; is some identifier, &quot;78&quot; is the entity identifier and &quot;1&quot; is the ordinal value of the reference (e.g., 1 being the first, 2 being the second)</rdfs:comment>
        <rdfs:label>relative id</rdfs:label>
    </owl:DatatypeProperty>
    


    <!-- http://capec.mitre.org/capec#relevantDesignPatterns.nonRecommended -->

    <owl:DatatypeProperty rdf:about="http://capec.mitre.org/capec#relevantDesignPatterns.nonRecommended">
        <rdfs:domain rdf:resource="http://capec.mitre.org/capec#AttackPattern"/>
        <rdfs:range rdf:resource="http://capec.mitre.org/capec#structuredText"/>
        <rdfs:comment>Specifies one or more non-recommended design patterns. A non-recommended design can decrease a sofware&apos;s resistence or resilience to this type of attack, leaving the system more susceptible.</rdfs:comment>
        <rdfs:label>Non-Recommended Design Patterns</rdfs:label>
    </owl:DatatypeProperty>
    


    <!-- http://capec.mitre.org/capec#relevantDesignPatterns.recommended -->

    <owl:DatatypeProperty rdf:about="http://capec.mitre.org/capec#relevantDesignPatterns.recommended">
        <rdfs:domain rdf:resource="http://capec.mitre.org/capec#AttackPattern"/>
        <rdfs:range rdf:resource="http://capec.mitre.org/capec#structuredText"/>
        <rdfs:comment>Specifies one or more recommended design patterns. A recommended design pattern increases the software&apos;s resistance or resilience to this type of attack.</rdfs:comment>
        <rdfs:label>Recommended Design Patterns</rdfs:label>
    </owl:DatatypeProperty>
    


    <!-- http://capec.mitre.org/capec#relevantSecurityPatterns -->

    <owl:DatatypeProperty rdf:about="http://capec.mitre.org/capec#relevantSecurityPatterns">
        <rdfs:domain rdf:resource="http://capec.mitre.org/capec#AttackPattern"/>
        <rdfs:range rdf:resource="http://capec.mitre.org/capec#structuredText"/>
        <rdfs:comment>Specifies one or more relevant security patterns. A relevant security pattern provides resistance or resilience to this type of attack.</rdfs:comment>
        <rdfs:label>relevant security patterns</rdfs:label>
    </owl:DatatypeProperty>
    


    <!-- http://capec.mitre.org/capec#relevantSecurityRequirements -->

    <owl:DatatypeProperty rdf:about="http://capec.mitre.org/capec#relevantSecurityRequirements">
        <rdfs:domain rdf:resource="http://capec.mitre.org/capec#AttackPattern"/>
        <rdfs:range rdf:resource="http://capec.mitre.org/capec#structuredText"/>
        <rdfs:comment>Specifies  one or more relevant security requirements. A relevant security requirement is a general security requirement that is relevant to this type of attack.</rdfs:comment>
        <rdfs:label>Relevant Security Requirements</rdfs:label>
    </owl:DatatypeProperty>
    


    <!-- http://capec.mitre.org/capec#researchGaps -->

    <owl:DatatypeProperty rdf:about="http://capec.mitre.org/capec#researchGaps">
        <rdfs:domain rdf:resource="http://capec.mitre.org/capec#Category"/>
        <rdfs:domain rdf:resource="http://capec.mitre.org/capec#CompoundElement"/>
        <rdfs:domain rdf:resource="http://capec.mitre.org/capec#View"/>
        <rdfs:range rdf:resource="http://capec.mitre.org/capec#structuredText"/>
        <rdfs:comment>Specifies zero or more Research gap elements, each of which identifies potential opportunities for the vulnerability research community to conduct further exploration of issues related to this attack pattern.  It is intended to highlight parts of CAPEC that have not received sufficient attention from researchers. This should be filled out where appropriate for attack patterns and categories.</rdfs:comment>
        <rdfs:label>Research Gaps</rdfs:label>
    </owl:DatatypeProperty>
    


    <!-- http://capec.mitre.org/capec#resourcesRequired -->

    <owl:DatatypeProperty rdf:about="http://capec.mitre.org/capec#resourcesRequired">
        <rdfs:domain rdf:resource="http://capec.mitre.org/capec#AttackPattern"/>
        <rdfs:domain rdf:resource="http://capec.mitre.org/capec#Category"/>
        <rdfs:range rdf:resource="http://capec.mitre.org/capec#structuredText"/>
        <rdfs:comment>Specifies the resources (CPU cycles, IP 	addresses, tools, etc.) required by an attacker to effectively execute this type of attack.</rdfs:comment>
        <rdfs:label>Resources Required</rdfs:label>
    </owl:DatatypeProperty>
    


    <!-- http://capec.mitre.org/capec#rfc -->

    <owl:DatatypeProperty rdf:about="http://capec.mitre.org/capec#rfc">
        <rdfs:range rdf:resource="http://www.w3.org/2001/XMLSchema#string"/>
        <rdfs:comment>Specifies the Request For Comment (RFC) associated with the protocol</rdfs:comment>
        <rdfs:label>RFC</rdfs:label>
    </owl:DatatypeProperty>
    


    <!-- http://capec.mitre.org/capec#securityControlDescription -->

    <owl:DatatypeProperty rdf:about="http://capec.mitre.org/capec#securityControlDescription">
        <rdfs:domain rdf:resource="http://capec.mitre.org/capec#SecurityControl"/>
        <rdfs:range rdf:resource="http://www.w3.org/2001/XMLSchema#string"/>
        <rdfs:comment>Specifies a brief description of the Security Control</rdfs:comment>
        <rdfs:label>Description</rdfs:label>
    </owl:DatatypeProperty>
    


    <!-- http://capec.mitre.org/capec#securityControlId -->

    <owl:DatatypeProperty rdf:about="http://capec.mitre.org/capec#securityControlId">
        <rdfs:domain rdf:resource="http://capec.mitre.org/capec#SecurityControl"/>
        <rdfs:range rdf:resource="http://www.w3.org/2001/XMLSchema#integer"/>
        <rdfs:comment>Specifies a unique integer identifier for the security control.</rdfs:comment>
        <rdfs:label>Security Control Identifier</rdfs:label>
    </owl:DatatypeProperty>
    


    <!-- http://capec.mitre.org/capec#securityControlType -->

    <owl:DatatypeProperty rdf:about="http://capec.mitre.org/capec#securityControlType">
        <rdfs:domain rdf:resource="http://capec.mitre.org/capec#SecurityControl"/>
        <rdfs:range>
            <rdfs:Datatype>
                <owl:oneOf>
                    <rdf:Description>
                        <rdf:type rdf:resource="http://www.w3.org/1999/02/22-rdf-syntax-ns#List"/>
                        <rdf:first rdf:datatype="http://www.w3.org/2001/XMLSchema#string">Corrective</rdf:first>
                        <rdf:rest>
                            <rdf:Description>
                                <rdf:type rdf:resource="http://www.w3.org/1999/02/22-rdf-syntax-ns#List"/>
                                <rdf:first rdf:datatype="http://www.w3.org/2001/XMLSchema#string">Detective</rdf:first>
                                <rdf:rest>
                                    <rdf:Description>
                                        <rdf:type rdf:resource="http://www.w3.org/1999/02/22-rdf-syntax-ns#List"/>
                                        <rdf:first rdf:datatype="http://www.w3.org/2001/XMLSchema#string">Preventative</rdf:first>
                                        <rdf:rest rdf:resource="http://www.w3.org/1999/02/22-rdf-syntax-ns#nil"/>
                                    </rdf:Description>
                                </rdf:rest>
                            </rdf:Description>
                        </rdf:rest>
                    </rdf:Description>
                </owl:oneOf>
            </rdfs:Datatype>
        </rdfs:range>
        <rdfs:comment>Specifies the type of the Security Control as “Detective,” “Corrective,” or “Preventative.” Detective controls detect an attacker’s activities in the attack step, whether the activities are successful or not. Corrective controls attempt to mitigate an attacker’s success by responding to a successful outcome. They are not related to or normalized against outcomes. Preventative controls are those that make the attack step unlikely or impossible to succeed.</rdfs:comment>
        <rdfs:label>Security Control Type</rdfs:label>
    </owl:DatatypeProperty>
    


    <!-- http://capec.mitre.org/capec#skillKnowledgeDescription -->

    <owl:DatatypeProperty rdf:about="http://capec.mitre.org/capec#skillKnowledgeDescription">
        <rdfs:domain rdf:resource="http://capec.mitre.org/capec#Knowlege"/>
        <rdfs:range rdf:resource="http://capec.mitre.org/capec#structuredText"/>
        <rdfs:comment>Specifies contextual detail for the skill or knowledge level.</rdfs:comment>
        <rdfs:label>Skill or Knowledge Description</rdfs:label>
    </owl:DatatypeProperty>
    


    <!-- http://capec.mitre.org/capec#skillKnowledgeLevel -->

    <owl:DatatypeProperty rdf:about="http://capec.mitre.org/capec#skillKnowledgeLevel">
        <rdfs:domain rdf:resource="http://capec.mitre.org/capec#Knowlege"/>
        <rdfs:range>
            <rdfs:Datatype>
                <owl:oneOf>
                    <rdf:Description>
                        <rdf:type rdf:resource="http://www.w3.org/1999/02/22-rdf-syntax-ns#List"/>
                        <rdf:first rdf:datatype="http://www.w3.org/2001/XMLSchema#string">High</rdf:first>
                        <rdf:rest>
                            <rdf:Description>
                                <rdf:type rdf:resource="http://www.w3.org/1999/02/22-rdf-syntax-ns#List"/>
                                <rdf:first rdf:datatype="http://www.w3.org/2001/XMLSchema#string">Low</rdf:first>
                                <rdf:rest>
                                    <rdf:Description>
                                        <rdf:type rdf:resource="http://www.w3.org/1999/02/22-rdf-syntax-ns#List"/>
                                        <rdf:first rdf:datatype="http://www.w3.org/2001/XMLSchema#string">Medium</rdf:first>
                                        <rdf:rest rdf:resource="http://www.w3.org/1999/02/22-rdf-syntax-ns#nil"/>
                                    </rdf:Description>
                                </rdf:rest>
                            </rdf:Description>
                        </rdf:rest>
                    </rdf:Description>
                </owl:oneOf>
            </rdfs:Datatype>
        </rdfs:range>
        <rdfs:comment>Specifies the level of skill or knowledge required by the attacker communicated on a rough scale.

 For example: Low - Basic computer familiarity,  Low - Basic SQL knowledge ; 
                         Medium - Moderate scripting and shell experience and ability to disassemble and decompile;
                         High - Expert knowledge of LINUX kernel, High - Detailed knowledge of target software development practices and business context (former employee)</rdfs:comment>
        <rdfs:label>Skill or Knowledge Level</rdfs:label>
    </owl:DatatypeProperty>
    


    <!-- http://capec.mitre.org/capec#solutionsAndMitigations -->

    <owl:DatatypeProperty rdf:about="http://capec.mitre.org/capec#solutionsAndMitigations">
        <rdfs:domain rdf:resource="http://capec.mitre.org/capec#AttackPattern"/>
        <rdfs:range rdf:resource="http://capec.mitre.org/capec#structuredText"/>
        <rdfs:comment>Specifies one or more solutions or mitigations. A solution or mitigation describes actions or approaches to prevent or mitigate the risk of this attack by improving the resilience of the target system, reduce its attack surface or to reduce the impact of the attack if it is successful.</rdfs:comment>
        <rdfs:label>Solutions and Mitigations</rdfs:label>
    </owl:DatatypeProperty>
    


    <!-- http://capec.mitre.org/capec#stakeholder -->

    <owl:DatatypeProperty rdf:about="http://capec.mitre.org/capec#stakeholder">
        <rdfs:domain rdf:resource="http://capec.mitre.org/capec#Audience"/>
        <rdfs:range>
            <rdfs:Datatype>
                <owl:oneOf>
                    <rdf:Description>
                        <rdf:type rdf:resource="http://www.w3.org/1999/02/22-rdf-syntax-ns#List"/>
                        <rdf:first rdf:datatype="http://www.w3.org/2001/XMLSchema#string">Academic_Researchers</rdf:first>
                        <rdf:rest>
                            <rdf:Description>
                                <rdf:type rdf:resource="http://www.w3.org/1999/02/22-rdf-syntax-ns#List"/>
                                <rdf:first rdf:datatype="http://www.w3.org/2001/XMLSchema#string">Applied_Researchers</rdf:first>
                                <rdf:rest>
                                    <rdf:Description>
                                        <rdf:type rdf:resource="http://www.w3.org/1999/02/22-rdf-syntax-ns#List"/>
                                        <rdf:first rdf:datatype="http://www.w3.org/2001/XMLSchema#string">Assessment_Customers</rdf:first>
                                        <rdf:rest>
                                            <rdf:Description>
                                                <rdf:type rdf:resource="http://www.w3.org/1999/02/22-rdf-syntax-ns#List"/>
                                                <rdf:first rdf:datatype="http://www.w3.org/2001/XMLSchema#string">Assessment_Vendors</rdf:first>
                                                <rdf:rest>
                                                    <rdf:Description>
                                                        <rdf:type rdf:resource="http://www.w3.org/1999/02/22-rdf-syntax-ns#List"/>
                                                        <rdf:first rdf:datatype="http://www.w3.org/2001/XMLSchema#string">CAPEC_Formalization</rdf:first>
                                                        <rdf:rest>
                                                            <rdf:Description>
                                                                <rdf:type rdf:resource="http://www.w3.org/1999/02/22-rdf-syntax-ns#List"/>
                                                                <rdf:first rdf:datatype="http://www.w3.org/2001/XMLSchema#string">CAPEC_Team</rdf:first>
                                                                <rdf:rest>
                                                                    <rdf:Description>
                                                                        <rdf:type rdf:resource="http://www.w3.org/1999/02/22-rdf-syntax-ns#List"/>
                                                                        <rdf:first rdf:datatype="http://www.w3.org/2001/XMLSchema#string">Developers</rdf:first>
                                                                        <rdf:rest>
                                                                            <rdf:Description>
                                                                                <rdf:type rdf:resource="http://www.w3.org/1999/02/22-rdf-syntax-ns#List"/>
                                                                                <rdf:first rdf:datatype="http://www.w3.org/2001/XMLSchema#string">Educators</rdf:first>
                                                                                <rdf:rest>
                                                                                    <rdf:Description>
                                                                                        <rdf:type rdf:resource="http://www.w3.org/1999/02/22-rdf-syntax-ns#List"/>
                                                                                        <rdf:first rdf:datatype="http://www.w3.org/2001/XMLSchema#string">Information_Providers</rdf:first>
                                                                                        <rdf:rest>
                                                                                            <rdf:Description>
                                                                                                <rdf:type rdf:resource="http://www.w3.org/1999/02/22-rdf-syntax-ns#List"/>
                                                                                                <rdf:first rdf:datatype="http://www.w3.org/2001/XMLSchema#string">OWGV</rdf:first>
                                                                                                <rdf:rest>
                                                                                                    <rdf:Description>
                                                                                                        <rdf:type rdf:resource="http://www.w3.org/1999/02/22-rdf-syntax-ns#List"/>
                                                                                                        <rdf:first rdf:datatype="http://www.w3.org/2001/XMLSchema#string">SAMATE</rdf:first>
                                                                                                        <rdf:rest>
                                                                                                            <rdf:Description>
                                                                                                                <rdf:type rdf:resource="http://www.w3.org/1999/02/22-rdf-syntax-ns#List"/>
                                                                                                                <rdf:first rdf:datatype="http://www.w3.org/2001/XMLSchema#string">Software_Customers</rdf:first>
                                                                                                                <rdf:rest>
                                                                                                                    <rdf:Description>
                                                                                                                        <rdf:type rdf:resource="http://www.w3.org/1999/02/22-rdf-syntax-ns#List"/>
                                                                                                                        <rdf:first rdf:datatype="http://www.w3.org/2001/XMLSchema#string">Software_Vendors</rdf:first>
                                                                                                                        <rdf:rest rdf:resource="http://www.w3.org/1999/02/22-rdf-syntax-ns#nil"/>
                                                                                                                    </rdf:Description>
                                                                                                                </rdf:rest>
                                                                                                            </rdf:Description>
                                                                                                        </rdf:rest>
                                                                                                    </rdf:Description>
                                                                                                </rdf:rest>
                                                                                            </rdf:Description>
                                                                                        </rdf:rest>
                                                                                    </rdf:Description>
                                                                                </rdf:rest>
                                                                            </rdf:Description>
                                                                        </rdf:rest>
                                                                    </rdf:Description>
                                                                </rdf:rest>
                                                            </rdf:Description>
                                                        </rdf:rest>
                                                    </rdf:Description>
                                                </rdf:rest>
                                            </rdf:Description>
                                        </rdf:rest>
                                    </rdf:Description>
                                </rdf:rest>
                            </rdf:Description>
                        </rdf:rest>
                    </rdf:Description>
                </owl:oneOf>
            </rdfs:Datatype>
        </rdfs:range>
        <rdfs:comment>Specifies what types of members of the Cyber Security community might be interested in this view.</rdfs:comment>
        <rdfs:label>Stakeholder</rdfs:label>
    </owl:DatatypeProperty>
    


    <!-- http://capec.mitre.org/capec#status -->

    <owl:DatatypeProperty rdf:about="http://capec.mitre.org/capec#status">
        <rdfs:domain rdf:resource="http://capec.mitre.org/capec#AttackPattern"/>
        <rdfs:domain rdf:resource="http://capec.mitre.org/capec#Category"/>
        <rdfs:domain rdf:resource="http://capec.mitre.org/capec#CompoundElement"/>
        <rdfs:domain rdf:resource="http://capec.mitre.org/capec#View"/>
        <rdfs:range>
            <rdfs:Datatype>
                <owl:oneOf>
                    <rdf:Description>
                        <rdf:type rdf:resource="http://www.w3.org/1999/02/22-rdf-syntax-ns#List"/>
                        <rdf:first rdf:datatype="http://www.w3.org/2001/XMLSchema#string">Depreciated</rdf:first>
                        <rdf:rest>
                            <rdf:Description>
                                <rdf:type rdf:resource="http://www.w3.org/1999/02/22-rdf-syntax-ns#List"/>
                                <rdf:first rdf:datatype="http://www.w3.org/2001/XMLSchema#string">Draft</rdf:first>
                                <rdf:rest>
                                    <rdf:Description>
                                        <rdf:type rdf:resource="http://www.w3.org/1999/02/22-rdf-syntax-ns#List"/>
                                        <rdf:first rdf:datatype="http://www.w3.org/2001/XMLSchema#string">Incomplete</rdf:first>
                                        <rdf:rest>
                                            <rdf:Description>
                                                <rdf:type rdf:resource="http://www.w3.org/1999/02/22-rdf-syntax-ns#List"/>
                                                <rdf:first rdf:datatype="http://www.w3.org/2001/XMLSchema#string">Stable</rdf:first>
                                                <rdf:rest>
                                                    <rdf:Description>
                                                        <rdf:type rdf:resource="http://www.w3.org/1999/02/22-rdf-syntax-ns#List"/>
                                                        <rdf:first rdf:datatype="http://www.w3.org/2001/XMLSchema#string">Usable</rdf:first>
                                                        <rdf:rest rdf:resource="http://www.w3.org/1999/02/22-rdf-syntax-ns#nil"/>
                                                    </rdf:Description>
                                                </rdf:rest>
                                            </rdf:Description>
                                        </rdf:rest>
                                    </rdf:Description>
                                </rdf:rest>
                            </rdf:Description>
                        </rdf:rest>
                    </rdf:Description>
                </owl:oneOf>
            </rdfs:Datatype>
        </rdfs:range>
        <rdfs:comment>Specifies the status</rdfs:comment>
        <rdfs:label>Status</rdfs:label>
    </owl:DatatypeProperty>
    


    <!-- http://capec.mitre.org/capec#stepDescription -->

    <owl:DatatypeProperty rdf:about="http://capec.mitre.org/capec#stepDescription">
        <rdfs:domain rdf:resource="http://capec.mitre.org/capec#AttackStep"/>
        <rdfs:range rdf:resource="http://capec.mitre.org/capec#structuredText"/>
        <rdfs:comment>Specifies a brief description of the attack step.</rdfs:comment>
        <rdfs:label>Description</rdfs:label>
    </owl:DatatypeProperty>
    


    <!-- http://capec.mitre.org/capec#stepId -->

    <owl:DatatypeProperty rdf:about="http://capec.mitre.org/capec#stepId">
        <rdfs:domain rdf:resource="http://capec.mitre.org/capec#AttackStep"/>
        <rdfs:range rdf:resource="http://www.w3.org/2001/XMLSchema#integer"/>
        <rdfs:comment>Specifies an identifier which indicates the particular step in the overall set of steps of the attack</rdfs:comment>
        <rdfs:label>Attack Phase Step Identifier</rdfs:label>
    </owl:DatatypeProperty>
    


    <!-- http://capec.mitre.org/capec#structureType -->

    <owl:DatatypeProperty rdf:about="http://capec.mitre.org/capec#structureType">
        <rdfs:domain rdf:resource="http://capec.mitre.org/capec#View"/>
        <rdfs:range>
            <rdfs:Datatype>
                <owl:oneOf>
                    <rdf:Description>
                        <rdf:type rdf:resource="http://www.w3.org/1999/02/22-rdf-syntax-ns#List"/>
                        <rdf:first rdf:datatype="http://www.w3.org/2001/XMLSchema#string">Explicit_Slice</rdf:first>
                        <rdf:rest>
                            <rdf:Description>
                                <rdf:type rdf:resource="http://www.w3.org/1999/02/22-rdf-syntax-ns#List"/>
                                <rdf:first rdf:datatype="http://www.w3.org/2001/XMLSchema#string">Graph</rdf:first>
                                <rdf:rest>
                                    <rdf:Description>
                                        <rdf:type rdf:resource="http://www.w3.org/1999/02/22-rdf-syntax-ns#List"/>
                                        <rdf:first rdf:datatype="http://www.w3.org/2001/XMLSchema#string">Implicit_Slice</rdf:first>
                                        <rdf:rest rdf:resource="http://www.w3.org/1999/02/22-rdf-syntax-ns#nil"/>
                                    </rdf:Description>
                                </rdf:rest>
                            </rdf:Description>
                        </rdf:rest>
                    </rdf:Description>
                </owl:oneOf>
            </rdfs:Datatype>
        </rdfs:range>
        <rdfs:comment>Specifies how this view is being constructed. 

Valid values are: Implicit Slice = a slice based on a filter criteria; Explicit Slice = a slice based on arbitrary membership, as defined by specific relationships between entries; Graph = a bounded graphical slice based on ChildOf relationships.</rdfs:comment>
        <rdfs:label>View Structure</rdfs:label>
    </owl:DatatypeProperty>
    


    <!-- http://capec.mitre.org/capec#submissionSource -->

    <owl:DatatypeProperty rdf:about="http://capec.mitre.org/capec#submissionSource">
        <rdfs:domain rdf:resource="http://capec.mitre.org/capec#HistoryRecord"/>
        <rdfs:range>
            <rdfs:Datatype>
                <owl:oneOf>
                    <rdf:Description>
                        <rdf:type rdf:resource="http://www.w3.org/1999/02/22-rdf-syntax-ns#List"/>
                        <rdf:first rdf:datatype="http://www.w3.org/2001/XMLSchema#string">External_Submission</rdf:first>
                        <rdf:rest>
                            <rdf:Description>
                                <rdf:type rdf:resource="http://www.w3.org/1999/02/22-rdf-syntax-ns#List"/>
                                <rdf:first rdf:datatype="http://www.w3.org/2001/XMLSchema#string">Externally_Mined</rdf:first>
                                <rdf:rest>
                                    <rdf:Description>
                                        <rdf:type rdf:resource="http://www.w3.org/1999/02/22-rdf-syntax-ns#List"/>
                                        <rdf:first rdf:datatype="http://www.w3.org/2001/XMLSchema#string">Internal_CAPEC_Team</rdf:first>
                                        <rdf:rest>
                                            <rdf:Description>
                                                <rdf:type rdf:resource="http://www.w3.org/1999/02/22-rdf-syntax-ns#List"/>
                                                <rdf:first rdf:datatype="http://www.w3.org/2001/XMLSchema#string">Internal_CWE_Team</rdf:first>
                                                <rdf:rest>
                                                    <rdf:Description>
                                                        <rdf:type rdf:resource="http://www.w3.org/1999/02/22-rdf-syntax-ns#List"/>
                                                        <rdf:first rdf:datatype="http://www.w3.org/2001/XMLSchema#string">NDA</rdf:first>
                                                        <rdf:rest rdf:resource="http://www.w3.org/1999/02/22-rdf-syntax-ns#nil"/>
                                                    </rdf:Description>
                                                </rdf:rest>
                                            </rdf:Description>
                                        </rdf:rest>
                                    </rdf:Description>
                                </rdf:rest>
                            </rdf:Description>
                        </rdf:rest>
                    </rdf:Description>
                </owl:oneOf>
            </rdfs:Datatype>
        </rdfs:range>
        <rdfs:comment>Specifies how the initial information for this entry was obtained.</rdfs:comment>
        <rdfs:label>submission source</rdfs:label>
    </owl:DatatypeProperty>
    


    <!-- http://capec.mitre.org/capec#targetAttackSurfaceLocalities -->

    <owl:DatatypeProperty rdf:about="http://capec.mitre.org/capec#targetAttackSurfaceLocalities">
        <rdfs:domain rdf:resource="http://capec.mitre.org/capec#TargetAttackSurfaceDescription"/>
        <rdfs:range>
            <rdfs:Datatype>
                <owl:oneOf>
                    <rdf:Description>
                        <rdf:type rdf:resource="http://www.w3.org/1999/02/22-rdf-syntax-ns#List"/>
                        <rdf:first rdf:datatype="http://www.w3.org/2001/XMLSchema#string">Client-side</rdf:first>
                        <rdf:rest>
                            <rdf:Description>
                                <rdf:type rdf:resource="http://www.w3.org/1999/02/22-rdf-syntax-ns#List"/>
                                <rdf:first rdf:datatype="http://www.w3.org/2001/XMLSchema#string">Server-side</rdf:first>
                                <rdf:rest rdf:resource="http://www.w3.org/1999/02/22-rdf-syntax-ns#nil"/>
                            </rdf:Description>
                        </rdf:rest>
                    </rdf:Description>
                </owl:oneOf>
            </rdfs:Datatype>
        </rdfs:range>
        <rdfs:comment>Specifies the localities, as &quot;client-side&quot; or &quot;server-side&quot;, of the targeted attack surface</rdfs:comment>
        <rdfs:label>Targeted Attack Surface Localities</rdfs:label>
    </owl:DatatypeProperty>
    


    <!-- http://capec.mitre.org/capec#targetAttackSurfaceTypes -->

    <owl:DatatypeProperty rdf:about="http://capec.mitre.org/capec#targetAttackSurfaceTypes">
        <rdfs:domain rdf:resource="http://capec.mitre.org/capec#TargetAttackSurfaceDescription"/>
        <rdfs:range>
            <rdfs:Datatype>
                <owl:oneOf>
                    <rdf:Description>
                        <rdf:type rdf:resource="http://www.w3.org/1999/02/22-rdf-syntax-ns#List"/>
                        <rdf:first rdf:datatype="http://www.w3.org/2001/XMLSchema#string">Firewall</rdf:first>
                        <rdf:rest>
                            <rdf:Description>
                                <rdf:type rdf:resource="http://www.w3.org/1999/02/22-rdf-syntax-ns#List"/>
                                <rdf:first rdf:datatype="http://www.w3.org/2001/XMLSchema#string">Host</rdf:first>
                                <rdf:rest>
                                    <rdf:Description>
                                        <rdf:type rdf:resource="http://www.w3.org/1999/02/22-rdf-syntax-ns#List"/>
                                        <rdf:first rdf:datatype="http://www.w3.org/2001/XMLSchema#string">Network</rdf:first>
                                        <rdf:rest>
                                            <rdf:Description>
                                                <rdf:type rdf:resource="http://www.w3.org/1999/02/22-rdf-syntax-ns#List"/>
                                                <rdf:first rdf:datatype="http://www.w3.org/2001/XMLSchema#string">Non-Web Application</rdf:first>
                                                <rdf:rest>
                                                    <rdf:Description>
                                                        <rdf:type rdf:resource="http://www.w3.org/1999/02/22-rdf-syntax-ns#List"/>
                                                        <rdf:first rdf:datatype="http://www.w3.org/2001/XMLSchema#string">Service</rdf:first>
                                                        <rdf:rest>
                                                            <rdf:Description>
                                                                <rdf:type rdf:resource="http://www.w3.org/1999/02/22-rdf-syntax-ns#List"/>
                                                                <rdf:first rdf:datatype="http://www.w3.org/2001/XMLSchema#string">Web Application</rdf:first>
                                                                <rdf:rest rdf:resource="http://www.w3.org/1999/02/22-rdf-syntax-ns#nil"/>
                                                            </rdf:Description>
                                                        </rdf:rest>
                                                    </rdf:Description>
                                                </rdf:rest>
                                            </rdf:Description>
                                        </rdf:rest>
                                    </rdf:Description>
                                </rdf:rest>
                            </rdf:Description>
                        </rdf:rest>
                    </rdf:Description>
                </owl:oneOf>
            </rdfs:Datatype>
        </rdfs:range>
        <rdfs:comment>Specifies one or more values that indicate the type of the targeted attack surface</rdfs:comment>
        <rdfs:label>Target Attack Surface Types</rdfs:label>
    </owl:DatatypeProperty>
    


    <!-- http://capec.mitre.org/capec#targetProtocolId -->

    <owl:DatatypeProperty rdf:about="http://capec.mitre.org/capec#targetProtocolId">
        <rdfs:domain rdf:resource="http://capec.mitre.org/capec#TargetedProtocol"/>
        <rdfs:range rdf:resource="http://www.w3.org/2001/XMLSchema#integer"/>
        <rdfs:comment>Specifies the identifier associated with the protocol being targeted</rdfs:comment>
        <rdfs:label>Protocol Identifier</rdfs:label>
    </owl:DatatypeProperty>
    


    <!-- http://capec.mitre.org/capec#targetProtocolName -->

    <owl:DatatypeProperty rdf:about="http://capec.mitre.org/capec#targetProtocolName">
        <rdfs:domain rdf:resource="http://capec.mitre.org/capec#TargetedProtocol"/>
        <rdfs:range rdf:resource="http://www.w3.org/2001/XMLSchema#string"/>
        <rdfs:comment>Specifies the name associated with the protocol being targeted</rdfs:comment>
        <rdfs:label>Protocol Name</rdfs:label>
    </owl:DatatypeProperty>
    


    <!-- http://capec.mitre.org/capec#targetedOSILayers -->

    <owl:DatatypeProperty rdf:about="http://capec.mitre.org/capec#targetedOSILayers">
        <rdfs:domain rdf:resource="http://capec.mitre.org/capec#TargetAttackSurfaceDescription"/>
        <rdfs:range>
            <rdfs:Datatype>
                <owl:oneOf>
                    <rdf:Description>
                        <rdf:type rdf:resource="http://www.w3.org/1999/02/22-rdf-syntax-ns#List"/>
                        <rdf:first rdf:datatype="http://www.w3.org/2001/XMLSchema#string">Application Layer</rdf:first>
                        <rdf:rest>
                            <rdf:Description>
                                <rdf:type rdf:resource="http://www.w3.org/1999/02/22-rdf-syntax-ns#List"/>
                                <rdf:first rdf:datatype="http://www.w3.org/2001/XMLSchema#string">Data Link Layer</rdf:first>
                                <rdf:rest>
                                    <rdf:Description>
                                        <rdf:type rdf:resource="http://www.w3.org/1999/02/22-rdf-syntax-ns#List"/>
                                        <rdf:first rdf:datatype="http://www.w3.org/2001/XMLSchema#string">Network Layer</rdf:first>
                                        <rdf:rest>
                                            <rdf:Description>
                                                <rdf:type rdf:resource="http://www.w3.org/1999/02/22-rdf-syntax-ns#List"/>
                                                <rdf:first rdf:datatype="http://www.w3.org/2001/XMLSchema#string">Physical Layer</rdf:first>
                                                <rdf:rest>
                                                    <rdf:Description>
                                                        <rdf:type rdf:resource="http://www.w3.org/1999/02/22-rdf-syntax-ns#List"/>
                                                        <rdf:first rdf:datatype="http://www.w3.org/2001/XMLSchema#string">Presentation Layer</rdf:first>
                                                        <rdf:rest>
                                                            <rdf:Description>
                                                                <rdf:type rdf:resource="http://www.w3.org/1999/02/22-rdf-syntax-ns#List"/>
                                                                <rdf:first rdf:datatype="http://www.w3.org/2001/XMLSchema#string">Session Layer</rdf:first>
                                                                <rdf:rest>
                                                                    <rdf:Description>
                                                                        <rdf:type rdf:resource="http://www.w3.org/1999/02/22-rdf-syntax-ns#List"/>
                                                                        <rdf:first rdf:datatype="http://www.w3.org/2001/XMLSchema#string">Transport Layer</rdf:first>
                                                                        <rdf:rest rdf:resource="http://www.w3.org/1999/02/22-rdf-syntax-ns#nil"/>
                                                                    </rdf:Description>
                                                                </rdf:rest>
                                                            </rdf:Description>
                                                        </rdf:rest>
                                                    </rdf:Description>
                                                </rdf:rest>
                                            </rdf:Description>
                                        </rdf:rest>
                                    </rdf:Description>
                                </rdf:rest>
                            </rdf:Description>
                        </rdf:rest>
                    </rdf:Description>
                </owl:oneOf>
            </rdfs:Datatype>
        </rdfs:range>
        <rdfs:comment>Specifies the OSI Layers that are part of the targeted Attack Surface</rdfs:comment>
        <rdfs:label>Targeted Attack Surface OSI Layers</rdfs:label>
    </owl:DatatypeProperty>
    


    <!-- http://capec.mitre.org/capec#technicalContext.architecturalParadigms -->

    <owl:DatatypeProperty rdf:about="http://capec.mitre.org/capec#technicalContext.architecturalParadigms">
        <rdfs:domain rdf:resource="http://capec.mitre.org/capec#AttackPattern"/>
        <rdfs:range>
            <rdfs:Datatype>
                <owl:oneOf>
                    <rdf:Description>
                        <rdf:type rdf:resource="http://www.w3.org/1999/02/22-rdf-syntax-ns#List"/>
                        <rdf:first rdf:datatype="http://www.w3.org/2001/XMLSchema#string">All</rdf:first>
                        <rdf:rest>
                            <rdf:Description>
                                <rdf:type rdf:resource="http://www.w3.org/1999/02/22-rdf-syntax-ns#List"/>
                                <rdf:first rdf:datatype="http://www.w3.org/2001/XMLSchema#string">Client-Server</rdf:first>
                                <rdf:rest>
                                    <rdf:Description>
                                        <rdf:type rdf:resource="http://www.w3.org/1999/02/22-rdf-syntax-ns#List"/>
                                        <rdf:first rdf:datatype="http://www.w3.org/2001/XMLSchema#string">Mainframe</rdf:first>
                                        <rdf:rest>
                                            <rdf:Description>
                                                <rdf:type rdf:resource="http://www.w3.org/1999/02/22-rdf-syntax-ns#List"/>
                                                <rdf:first rdf:datatype="http://www.w3.org/2001/XMLSchema#string">Other</rdf:first>
                                                <rdf:rest>
                                                    <rdf:Description>
                                                        <rdf:type rdf:resource="http://www.w3.org/1999/02/22-rdf-syntax-ns#List"/>
                                                        <rdf:first rdf:datatype="http://www.w3.org/2001/XMLSchema#string">SOA</rdf:first>
                                                        <rdf:rest>
                                                            <rdf:Description>
                                                                <rdf:type rdf:resource="http://www.w3.org/1999/02/22-rdf-syntax-ns#List"/>
                                                                <rdf:first rdf:datatype="http://www.w3.org/2001/XMLSchema#string">Web</rdf:first>
                                                                <rdf:rest>
                                                                    <rdf:Description>
                                                                        <rdf:type rdf:resource="http://www.w3.org/1999/02/22-rdf-syntax-ns#List"/>
                                                                        <rdf:first rdf:datatype="http://www.w3.org/2001/XMLSchema#string">n-Tier</rdf:first>
                                                                        <rdf:rest rdf:resource="http://www.w3.org/1999/02/22-rdf-syntax-ns#nil"/>
                                                                    </rdf:Description>
                                                                </rdf:rest>
                                                            </rdf:Description>
                                                        </rdf:rest>
                                                    </rdf:Description>
                                                </rdf:rest>
                                            </rdf:Description>
                                        </rdf:rest>
                                    </rdf:Description>
                                </rdf:rest>
                            </rdf:Description>
                        </rdf:rest>
                    </rdf:Description>
                </owl:oneOf>
            </rdfs:Datatype>
        </rdfs:range>
        <rdfs:comment>Specifies the technical context where this pattern is applicable.</rdfs:comment>
        <rdfs:label>Technical Context</rdfs:label>
    </owl:DatatypeProperty>
    


    <!-- http://capec.mitre.org/capec#technicalContext.frameworks -->

    <owl:DatatypeProperty rdf:about="http://capec.mitre.org/capec#technicalContext.frameworks">
        <rdfs:domain rdf:resource="http://capec.mitre.org/capec#AttackPattern"/>
        <rdfs:range>
            <rdfs:Datatype>
                <owl:oneOf>
                    <rdf:Description>
                        <rdf:type rdf:resource="http://www.w3.org/1999/02/22-rdf-syntax-ns#List"/>
                        <rdf:first rdf:datatype="http://www.w3.org/2001/XMLSchema#string">.NET</rdf:first>
                        <rdf:rest>
                            <rdf:Description>
                                <rdf:type rdf:resource="http://www.w3.org/1999/02/22-rdf-syntax-ns#List"/>
                                <rdf:first rdf:datatype="http://www.w3.org/2001/XMLSchema#string">All</rdf:first>
                                <rdf:rest>
                                    <rdf:Description>
                                        <rdf:type rdf:resource="http://www.w3.org/1999/02/22-rdf-syntax-ns#List"/>
                                        <rdf:first rdf:datatype="http://www.w3.org/2001/XMLSchema#string">Hibernate</rdf:first>
                                        <rdf:rest>
                                            <rdf:Description>
                                                <rdf:type rdf:resource="http://www.w3.org/1999/02/22-rdf-syntax-ns#List"/>
                                                <rdf:first rdf:datatype="http://www.w3.org/2001/XMLSchema#string">J2EE</rdf:first>
                                                <rdf:rest>
                                                    <rdf:Description>
                                                        <rdf:type rdf:resource="http://www.w3.org/1999/02/22-rdf-syntax-ns#List"/>
                                                        <rdf:first rdf:datatype="http://www.w3.org/2001/XMLSchema#string">Other</rdf:first>
                                                        <rdf:rest>
                                                            <rdf:Description>
                                                                <rdf:type rdf:resource="http://www.w3.org/1999/02/22-rdf-syntax-ns#List"/>
                                                                <rdf:first rdf:datatype="http://www.w3.org/2001/XMLSchema#string">Spring</rdf:first>
                                                                <rdf:rest>
                                                                    <rdf:Description>
                                                                        <rdf:type rdf:resource="http://www.w3.org/1999/02/22-rdf-syntax-ns#List"/>
                                                                        <rdf:first rdf:datatype="http://www.w3.org/2001/XMLSchema#string">Struts</rdf:first>
                                                                        <rdf:rest rdf:resource="http://www.w3.org/1999/02/22-rdf-syntax-ns#nil"/>
                                                                    </rdf:Description>
                                                                </rdf:rest>
                                                            </rdf:Description>
                                                        </rdf:rest>
                                                    </rdf:Description>
                                                </rdf:rest>
                                            </rdf:Description>
                                        </rdf:rest>
                                    </rdf:Description>
                                </rdf:rest>
                            </rdf:Description>
                        </rdf:rest>
                    </rdf:Description>
                </owl:oneOf>
            </rdfs:Datatype>
        </rdfs:range>
        <rdfs:comment>Specifies  one or more frameworks in which this attack pattern is possible and relevant. Frameworks characterizes the target using an enumerated list of frameworks utilized by the target.</rdfs:comment>
        <rdfs:label>Frameworks</rdfs:label>
    </owl:DatatypeProperty>
    


    <!-- http://capec.mitre.org/capec#technicalContext.languages -->

    <owl:DatatypeProperty rdf:about="http://capec.mitre.org/capec#technicalContext.languages">
        <rdfs:domain rdf:resource="http://capec.mitre.org/capec#AttackPattern"/>
        <rdfs:range rdf:resource="http://www.w3.org/2001/XMLSchema#string"/>
        <rdfs:comment>Specifies one or more languages in which this attack pattern is possible and relevant.  Languages characterizes the target using an enumerated list of languages utilized by the target.</rdfs:comment>
        <rdfs:label>Languages</rdfs:label>
    </owl:DatatypeProperty>
    


    <!-- http://capec.mitre.org/capec#technicalContext.platforms -->

    <owl:DatatypeProperty rdf:about="http://capec.mitre.org/capec#technicalContext.platforms">
        <rdfs:domain rdf:resource="http://capec.mitre.org/capec#AttackPattern"/>
        <rdfs:range>
            <rdfs:Datatype>
                <owl:oneOf>
                    <rdf:Description>
                        <rdf:type rdf:resource="http://www.w3.org/1999/02/22-rdf-syntax-ns#List"/>
                        <rdf:first rdf:datatype="http://www.w3.org/2001/XMLSchema#string">All</rdf:first>
                        <rdf:rest>
                            <rdf:Description>
                                <rdf:type rdf:resource="http://www.w3.org/1999/02/22-rdf-syntax-ns#List"/>
                                <rdf:first rdf:datatype="http://www.w3.org/2001/XMLSchema#string">Other</rdf:first>
                                <rdf:rest>
                                    <rdf:Description>
                                        <rdf:type rdf:resource="http://www.w3.org/1999/02/22-rdf-syntax-ns#List"/>
                                        <rdf:first rdf:datatype="http://www.w3.org/2001/XMLSchema#string">Solaris</rdf:first>
                                        <rdf:rest>
                                            <rdf:Description>
                                                <rdf:type rdf:resource="http://www.w3.org/1999/02/22-rdf-syntax-ns#List"/>
                                                <rdf:first rdf:datatype="http://www.w3.org/2001/XMLSchema#string">UNIX-LINUX</rdf:first>
                                                <rdf:rest>
                                                    <rdf:Description>
                                                        <rdf:type rdf:resource="http://www.w3.org/1999/02/22-rdf-syntax-ns#List"/>
                                                        <rdf:first rdf:datatype="http://www.w3.org/2001/XMLSchema#string">Windows</rdf:first>
                                                        <rdf:rest rdf:resource="http://www.w3.org/1999/02/22-rdf-syntax-ns#nil"/>
                                                    </rdf:Description>
                                                </rdf:rest>
                                            </rdf:Description>
                                        </rdf:rest>
                                    </rdf:Description>
                                </rdf:rest>
                            </rdf:Description>
                        </rdf:rest>
                    </rdf:Description>
                </owl:oneOf>
            </rdfs:Datatype>
        </rdfs:range>
        <rdfs:comment>Specifies one or more platforms in which this attack pattern is possible and relevant. Platforms characterizes the target using an enumerated list of platforms utilized by the target.</rdfs:comment>
        <rdfs:label>Platforms</rdfs:label>
    </owl:DatatypeProperty>
    


    <!-- http://capec.mitre.org/capec#techniqueDescription -->

    <owl:DatatypeProperty rdf:about="http://capec.mitre.org/capec#techniqueDescription">
        <rdfs:domain rdf:resource="http://capec.mitre.org/capec#AttackStepTechnique"/>
        <rdfs:range rdf:resource="http://capec.mitre.org/capec#structuredText"/>
        <rdfs:comment>Specifies a brief description of the attack step technique</rdfs:comment>
        <rdfs:label>Description</rdfs:label>
    </owl:DatatypeProperty>
    


    <!-- http://capec.mitre.org/capec#techniqueId -->

    <owl:DatatypeProperty rdf:about="http://capec.mitre.org/capec#techniqueId">
        <rdfs:domain rdf:resource="http://capec.mitre.org/capec#AttackStepTechnique"/>
        <rdfs:range rdf:resource="http://www.w3.org/2001/XMLSchema#integer"/>
        <rdfs:comment>Specifies an identifier for the technique</rdfs:comment>
        <rdfs:label>Technique Identifier</rdfs:label>
    </owl:DatatypeProperty>
    


    <!-- http://capec.mitre.org/capec#techniqueName -->

    <owl:DatatypeProperty rdf:about="http://capec.mitre.org/capec#techniqueName">
        <rdfs:domain rdf:resource="http://capec.mitre.org/capec#ObfuscationTechnique"/>
        <rdfs:domain rdf:resource="http://capec.mitre.org/capec#ProbingTechnique"/>
        <rdfs:range rdf:resource="http://www.w3.org/2001/XMLSchema#string"/>
        <rdfs:comment>Specifies a name associated with the technique</rdfs:comment>
        <rdfs:label>Technique Name</rdfs:label>
    </owl:DatatypeProperty>
    


    <!-- http://capec.mitre.org/capec#term -->

    <owl:DatatypeProperty rdf:about="http://capec.mitre.org/capec#term">
        <rdfs:domain rdf:resource="http://capec.mitre.org/capec#Term"/>
        <rdfs:range rdf:resource="http://www.w3.org/2001/XMLSchema#string"/>
        <rdfs:comment>Specifies the actual term.  Each term should follow the same conventions as they entry Name attribute.</rdfs:comment>
        <rdfs:isDefinedBy rdf:datatype="http://www.w3.org/2001/XMLSchema#string">&lt;http://capec.mitre.org/capec&gt;</rdfs:isDefinedBy>
        <rdfs:label>Term</rdfs:label>
    </owl:DatatypeProperty>
    


    <!-- http://capec.mitre.org/capec#text -->

    <owl:DatatypeProperty rdf:about="http://capec.mitre.org/capec#text">
        <rdfs:range rdf:resource="http://www.w3.org/2001/XMLSchema#string"/>
        <rdfs:comment>Specifies a paragraph of text.</rdfs:comment>
        <rdfs:label>Text</rdfs:label>
    </owl:DatatypeProperty>
    


    <!-- http://capec.mitre.org/capec#textTitle -->

    <owl:DatatypeProperty rdf:about="http://capec.mitre.org/capec#textTitle">
        <rdfs:range rdf:resource="http://www.w3.org/2001/XMLSchema#string"/>
        <rdfs:comment>Specifies a title for a subsequent block of text.</rdfs:comment>
        <rdfs:label>Text Title</rdfs:label>
    </owl:DatatypeProperty>
    


    <!-- http://capec.mitre.org/capec#title -->

    <owl:DatatypeProperty rdf:about="http://capec.mitre.org/capec#title">
        <rdfs:domain rdf:resource="http://capec.mitre.org/capec#AttackPattern"/>
        <rdfs:domain rdf:resource="http://capec.mitre.org/capec#AttackStep"/>
        <rdfs:range rdf:resource="http://www.w3.org/2001/XMLSchema#string"/>
        <rdfs:comment>Specifies a short descriptive title. It should be kept as short as possible but also clearly convey the nature of what is being described</rdfs:comment>
        <rdfs:label>Title</rdfs:label>
    </owl:DatatypeProperty>
    


    <!-- http://capec.mitre.org/capec#typicalLikelihoodOfExploit -->

    <owl:DatatypeProperty rdf:about="http://capec.mitre.org/capec#typicalLikelihoodOfExploit">
        <rdfs:domain rdf:resource="http://capec.mitre.org/capec#AttackPattern"/>
        <rdfs:range rdf:resource="http://www.w3.org/2001/XMLSchema#string"/>
        <rdfs:comment>Specifies on a rough scale (Very Low, Low Medium,  High, Very High), what is the overall likelihood of this type of attack typically succeeding considering the attack prerequisites, targeted weakness attack surface, skill required and resources required as well as available and likely implemented blocking solutions? The likelihood of exploit of a specific attack instance can vary greatly depending on the specific context of the target software under attack. This field is intended to capture an overall typical average value for this type of attack with the understanding that it will not be completely accurate for all attacks.</rdfs:comment>
        <rdfs:label>Typical Likelihood of Exploit</rdfs:label>
    </owl:DatatypeProperty>
    


    <!-- http://capec.mitre.org/capec#typicalLikelyhoodOfExploit.explanation -->

    <owl:DatatypeProperty rdf:about="http://capec.mitre.org/capec#typicalLikelyhoodOfExploit.explanation">
        <rdfs:domain rdf:resource="http://capec.mitre.org/capec#AttackPattern"/>
        <rdfs:range rdf:resource="http://capec.mitre.org/capec#structuredText"/>
        <rdfs:comment>Speifies an explanation for the likelihood of Exploit</rdfs:comment>
        <rdfs:label>Likelyhood of Exploit Explanation</rdfs:label>
    </owl:DatatypeProperty>
    


    <!-- http://capec.mitre.org/capec#typicalSeverity -->

    <owl:DatatypeProperty rdf:about="http://capec.mitre.org/capec#typicalSeverity">
        <rdfs:domain rdf:resource="http://capec.mitre.org/capec#AttackPattern"/>
        <rdfs:range>
            <rdfs:Datatype>
                <owl:oneOf>
                    <rdf:Description>
                        <rdf:type rdf:resource="http://www.w3.org/1999/02/22-rdf-syntax-ns#List"/>
                        <rdf:first rdf:datatype="http://www.w3.org/2001/XMLSchema#string">High</rdf:first>
                        <rdf:rest>
                            <rdf:Description>
                                <rdf:type rdf:resource="http://www.w3.org/1999/02/22-rdf-syntax-ns#List"/>
                                <rdf:first rdf:datatype="http://www.w3.org/2001/XMLSchema#string">Low</rdf:first>
                                <rdf:rest>
                                    <rdf:Description>
                                        <rdf:type rdf:resource="http://www.w3.org/1999/02/22-rdf-syntax-ns#List"/>
                                        <rdf:first rdf:datatype="http://www.w3.org/2001/XMLSchema#string">Medium</rdf:first>
                                        <rdf:rest>
                                            <rdf:Description>
                                                <rdf:type rdf:resource="http://www.w3.org/1999/02/22-rdf-syntax-ns#List"/>
                                                <rdf:first rdf:datatype="http://www.w3.org/2001/XMLSchema#string">Very High</rdf:first>
                                                <rdf:rest>
                                                    <rdf:Description>
                                                        <rdf:type rdf:resource="http://www.w3.org/1999/02/22-rdf-syntax-ns#List"/>
                                                        <rdf:first rdf:datatype="http://www.w3.org/2001/XMLSchema#string">Very Low</rdf:first>
                                                        <rdf:rest rdf:resource="http://www.w3.org/1999/02/22-rdf-syntax-ns#nil"/>
                                                    </rdf:Description>
                                                </rdf:rest>
                                            </rdf:Description>
                                        </rdf:rest>
                                    </rdf:Description>
                                </rdf:rest>
                            </rdf:Description>
                        </rdf:rest>
                    </rdf:Description>
                </owl:oneOf>
            </rdfs:Datatype>
        </rdfs:range>
        <rdfs:comment>Specifies on a rough scale (Very Low, Low, Medium, High, Very high), what is the typical severity of impact to the targeted software if this attack occurs? The severity of a specific attack instance can vary greatly depending on the specific context of the target software under attack. This field is intended to capture an overall typical average value for this type of attack with the understanding that it will not be completely accurate for all attacks.</rdfs:comment>
        <rdfs:label>Typical Severity</rdfs:label>
    </owl:DatatypeProperty>
    


    <!-- http://capec.mitre.org/capec#viewFilter -->

    <owl:DatatypeProperty rdf:about="http://capec.mitre.org/capec#viewFilter">
        <rdfs:domain rdf:resource="http://capec.mitre.org/capec#View"/>
        <rdfs:range rdf:resource="http://www.w3.org/2001/XMLSchema#string"/>
        <rdfs:comment>Specifies an XSL query for identifying 	which elements are members of an implicit slice. This should only be present for implicit slices</rdfs:comment>
        <rdfs:label>View Filter</rdfs:label>
    </owl:DatatypeProperty>
    


    <!-- http://capec.mitre.org/capec#viewName -->

    <owl:DatatypeProperty rdf:about="http://capec.mitre.org/capec#viewName">
        <rdfs:domain rdf:resource="http://capec.mitre.org/capec#View"/>
        <rdfs:range rdf:resource="http://www.w3.org/2001/XMLSchema#string"/>
        <rdfs:comment>Specifies a descriptive attribute used to give the reader an idea of what perspective this view represents. All words in the name should be capitalized except for articles and prepositions unless they begin or end the name. Subsequent words in a hyphenated chain are also not capitalized.</rdfs:comment>
        <rdfs:label>view name</rdfs:label>
    </owl:DatatypeProperty>
    


    <!-- http://capec.mitre.org/capec#viewObjective -->

    <owl:DatatypeProperty rdf:about="http://capec.mitre.org/capec#viewObjective">
        <rdfs:domain rdf:resource="http://capec.mitre.org/capec#View"/>
        <rdfs:range rdf:resource="http://capec.mitre.org/capec#structuredText"/>
        <rdfs:comment>Specifies the perspective from which this View is constructed.</rdfs:comment>
        <rdfs:label>View Objective</rdfs:label>
    </owl:DatatypeProperty>
    


    <!-- http://capec.mitre.org/capec#vulnerabilityDescription -->

    <owl:DatatypeProperty rdf:about="http://capec.mitre.org/capec#vulnerabilityDescription">
        <rdfs:domain rdf:resource="http://capec.mitre.org/capec#ExampleInstance"/>
        <rdfs:domain rdf:resource="http://capec.mitre.org/capec#RelatedVulnerabilityStatement"/>
        <rdfs:range rdf:resource="http://capec.mitre.org/capec#structuredText"/>
        <rdfs:comment>Specifies a short textual description of the specific related vulnerability taken from the industry standard vulnerability listing.</rdfs:comment>
        <rdfs:label>Vulnerability Description</rdfs:label>
    </owl:DatatypeProperty>
    


    <!-- http://capec.mitre.org/capec#vulnerabilityId -->

    <owl:DatatypeProperty rdf:about="http://capec.mitre.org/capec#vulnerabilityId">
        <rdfs:range rdf:resource="http://www.w3.org/2001/XMLSchema#string"/>
        <rdfs:comment>Specifies the vulnerability identifier, such as Common Vulnerabilities and Explosures (CVE), Common Attack Pattern Enumeration and Classification (CAPEC), US-CERT number, or vendor-specific identifier that identifies the vulnerability.</rdfs:comment>
        <rdfs:label>Vulnerability Id</rdfs:label>
    </owl:DatatypeProperty>
    


    <!-- http://capec.mitre.org/capec#weaknessId -->

    <owl:DatatypeProperty rdf:about="http://capec.mitre.org/capec#weaknessId">
        <rdfs:range rdf:resource="http://www.w3.org/2001/XMLSchema#string"/>
        <rdfs:comment>Specifies the identifer, in the form &apos;CWE-xxxx&apos; of the weakness as enumerated in Common Weakness Enumeration (CWE).</rdfs:comment>
        <rdfs:label>Weakness ID</rdfs:label>
    </owl:DatatypeProperty>
    


    <!-- http://capec.mitre.org/capec#weaknessRelationshipType -->

    <owl:DatatypeProperty rdf:about="http://capec.mitre.org/capec#weaknessRelationshipType">
        <rdfs:domain rdf:resource="http://capec.mitre.org/capec#RelatedWeaknessStatement"/>
        <rdfs:range>
            <rdfs:Datatype>
                <owl:oneOf>
                    <rdf:Description>
                        <rdf:type rdf:resource="http://www.w3.org/1999/02/22-rdf-syntax-ns#List"/>
                        <rdf:first rdf:datatype="http://www.w3.org/2001/XMLSchema#string">Secondary</rdf:first>
                        <rdf:rest>
                            <rdf:Description>
                                <rdf:type rdf:resource="http://www.w3.org/1999/02/22-rdf-syntax-ns#List"/>
                                <rdf:first rdf:datatype="http://www.w3.org/2001/XMLSchema#string">Targeted</rdf:first>
                                <rdf:rest rdf:resource="http://www.w3.org/1999/02/22-rdf-syntax-ns#nil"/>
                            </rdf:Description>
                        </rdf:rest>
                    </rdf:Description>
                </owl:oneOf>
            </rdfs:Datatype>
        </rdfs:range>
        <rdfs:comment>Specifies the nature of the relationship between this weakness and the 	attack pattern. Weaknesses that are specifically targeted by the attack are of type “Targeted”.  Weaknesses which are not specifically targeted but whose presence may increase the likelihood of the attack succeeding or the impact of the attack if it does succeed are of type “Secondary”.</rdfs:comment>
        <rdfs:label>Relationship Type</rdfs:label>
    </owl:DatatypeProperty>
    


    <!-- 
    ///////////////////////////////////////////////////////////////////////////////////////
    //
    // Classes
    //
    ///////////////////////////////////////////////////////////////////////////////////////
     -->

    


    <!-- http://capec.mitre.org/capec#AttackPattern -->

    <owl:Class rdf:about="http://capec.mitre.org/capec#AttackPattern">
        <rdfs:subClassOf>
            <owl:Restriction>
                <owl:onProperty rdf:resource="http://capec.mitre.org/capec#attackExecutionFlow"/>
                <owl:maxCardinality rdf:datatype="http://www.w3.org/2001/XMLSchema#nonNegativeInteger">1</owl:maxCardinality>
            </owl:Restriction>
        </rdfs:subClassOf>
        <rdfs:subClassOf>
            <owl:Restriction>
                <owl:onProperty rdf:resource="http://capec.mitre.org/capec#payloadActivationImpact.observables"/>
                <owl:maxCardinality rdf:datatype="http://www.w3.org/2001/XMLSchema#nonNegativeInteger">1</owl:maxCardinality>
            </owl:Restriction>
        </rdfs:subClassOf>
        <rdfs:subClassOf>
            <owl:Restriction>
                <owl:onProperty rdf:resource="http://capec.mitre.org/capec#description"/>
                <owl:cardinality rdf:datatype="http://www.w3.org/2001/XMLSchema#nonNegativeInteger">1</owl:cardinality>
            </owl:Restriction>
        </rdfs:subClassOf>
        <rdfs:subClassOf>
            <owl:Restriction>
                <owl:onProperty rdf:resource="http://capec.mitre.org/capec#dictionaryLink"/>
                <owl:cardinality rdf:datatype="http://www.w3.org/2001/XMLSchema#nonNegativeInteger">1</owl:cardinality>
            </owl:Restriction>
        </rdfs:subClassOf>
        <rdfs:subClassOf>
            <owl:Restriction>
                <owl:onProperty rdf:resource="http://capec.mitre.org/capec#id"/>
                <owl:cardinality rdf:datatype="http://www.w3.org/2001/XMLSchema#nonNegativeInteger">1</owl:cardinality>
            </owl:Restriction>
        </rdfs:subClassOf>
        <rdfs:subClassOf>
            <owl:Restriction>
                <owl:onProperty rdf:resource="http://capec.mitre.org/capec#status"/>
                <owl:cardinality rdf:datatype="http://www.w3.org/2001/XMLSchema#nonNegativeInteger">1</owl:cardinality>
            </owl:Restriction>
        </rdfs:subClassOf>
        <rdfs:subClassOf>
            <owl:Restriction>
                <owl:onProperty rdf:resource="http://capec.mitre.org/capec#title"/>
                <owl:cardinality rdf:datatype="http://www.w3.org/2001/XMLSchema#nonNegativeInteger">1</owl:cardinality>
            </owl:Restriction>
        </rdfs:subClassOf>
        <rdfs:subClassOf>
            <owl:Restriction>
                <owl:onProperty rdf:resource="http://capec.mitre.org/capec#impact.availability"/>
                <owl:maxCardinality rdf:datatype="http://www.w3.org/2001/XMLSchema#nonNegativeInteger">1</owl:maxCardinality>
            </owl:Restriction>
        </rdfs:subClassOf>
        <rdfs:subClassOf>
            <owl:Restriction>
                <owl:onProperty rdf:resource="http://capec.mitre.org/capec#impact.confidentiality"/>
                <owl:maxCardinality rdf:datatype="http://www.w3.org/2001/XMLSchema#nonNegativeInteger">1</owl:maxCardinality>
            </owl:Restriction>
        </rdfs:subClassOf>
        <rdfs:subClassOf>
            <owl:Restriction>
                <owl:onProperty rdf:resource="http://capec.mitre.org/capec#impact.integrity"/>
                <owl:maxCardinality rdf:datatype="http://www.w3.org/2001/XMLSchema#nonNegativeInteger">1</owl:maxCardinality>
            </owl:Restriction>
        </rdfs:subClassOf>
        <rdfs:subClassOf>
            <owl:Restriction>
                <owl:onProperty rdf:resource="http://capec.mitre.org/capec#injectionVector"/>
                <owl:maxCardinality rdf:datatype="http://www.w3.org/2001/XMLSchema#nonNegativeInteger">1</owl:maxCardinality>
            </owl:Restriction>
        </rdfs:subClassOf>
        <rdfs:subClassOf>
            <owl:Restriction>
                <owl:onProperty rdf:resource="http://capec.mitre.org/capec#payloadActivationImpact.description"/>
                <owl:maxCardinality rdf:datatype="http://www.w3.org/2001/XMLSchema#nonNegativeInteger">1</owl:maxCardinality>
            </owl:Restriction>
        </rdfs:subClassOf>
        <rdfs:comment>Characterizes an Attack Pattern</rdfs:comment>
        <rdfs:isDefinedBy rdf:resource="http://capec.mitre.org/capec"/>
        <rdfs:label>Attack Pattern</rdfs:label>
    </owl:Class>
    


    <!-- http://capec.mitre.org/capec#AttackPatternCatalog -->

    <owl:Class rdf:about="http://capec.mitre.org/capec#AttackPatternCatalog">
        <rdfs:subClassOf rdf:resource="http://scap.nist.gov/scap_core#Catalog"/>
        <rdfs:comment>Characterizes a catalog of Attack Patterns</rdfs:comment>
        <rdfs:isDefinedBy rdf:resource="http://capec.mitre.org/capec"/>
        <rdfs:label>Attack Pattern Catalog</rdfs:label>
    </owl:Class>
    


    <!-- http://capec.mitre.org/capec#AttackPhase -->

    <owl:Class rdf:about="http://capec.mitre.org/capec#AttackPhase">
        <rdfs:subClassOf>
            <owl:Restriction>
                <owl:onProperty rdf:resource="http://capec.mitre.org/capec#attackSteps"/>
                <owl:minCardinality rdf:datatype="http://www.w3.org/2001/XMLSchema#nonNegativeInteger">1</owl:minCardinality>
            </owl:Restriction>
        </rdfs:subClassOf>
        <rdfs:subClassOf>
            <owl:Restriction>
                <owl:onProperty rdf:resource="http://capec.mitre.org/capec#phaseId"/>
                <owl:cardinality rdf:datatype="http://www.w3.org/2001/XMLSchema#nonNegativeInteger">1</owl:cardinality>
            </owl:Restriction>
        </rdfs:subClassOf>
        <rdfs:subClassOf>
            <owl:Restriction>
                <owl:onProperty rdf:resource="http://capec.mitre.org/capec#phaseName"/>
                <owl:cardinality rdf:datatype="http://www.w3.org/2001/XMLSchema#nonNegativeInteger">1</owl:cardinality>
            </owl:Restriction>
        </rdfs:subClassOf>
        <rdfs:subClassOf>
            <owl:Restriction>
                <owl:onProperty rdf:resource="http://capec.mitre.org/capec#relativeId"/>
                <owl:cardinality rdf:datatype="http://www.w3.org/2001/XMLSchema#nonNegativeInteger">1</owl:cardinality>
            </owl:Restriction>
        </rdfs:subClassOf>
        <rdfs:comment>Represents a segment the attack steps into the various phases of attack. One of three phases &quot;Explore,&quot; &quot;Experiment,&quot; or &quot;Exploit.&quot;  Each phase should appear at most once, and attack steps should be grouped by what kind of activities the attacker is carrying out. The exploration and experimentation phases may or may not occur during a particular attack, because the attacker may already know exactly how to exploit a system</rdfs:comment>
        <rdfs:isDefinedBy rdf:resource="http://capec.mitre.org/capec"/>
        <rdfs:label>Attack Phase</rdfs:label>
    </owl:Class>
    


    <!-- http://capec.mitre.org/capec#AttackStep -->

    <owl:Class rdf:about="http://capec.mitre.org/capec#AttackStep">
        <rdfs:subClassOf>
            <owl:Restriction>
                <owl:onProperty rdf:resource="http://capec.mitre.org/capec#relativeId"/>
                <owl:cardinality rdf:datatype="http://www.w3.org/2001/XMLSchema#nonNegativeInteger">1</owl:cardinality>
            </owl:Restriction>
        </rdfs:subClassOf>
        <rdfs:subClassOf>
            <owl:Restriction>
                <owl:onProperty rdf:resource="http://capec.mitre.org/capec#stepId"/>
                <owl:cardinality rdf:datatype="http://www.w3.org/2001/XMLSchema#nonNegativeInteger">1</owl:cardinality>
            </owl:Restriction>
        </rdfs:subClassOf>
        <rdfs:subClassOf>
            <owl:Restriction>
                <owl:onProperty rdf:resource="http://capec.mitre.org/capec#title"/>
                <owl:cardinality rdf:datatype="http://www.w3.org/2001/XMLSchema#nonNegativeInteger">1</owl:cardinality>
            </owl:Restriction>
        </rdfs:subClassOf>
        <rdfs:subClassOf>
            <owl:Restriction>
                <owl:onProperty rdf:resource="http://capec.mitre.org/capec#stepDescription"/>
                <owl:maxCardinality rdf:datatype="http://www.w3.org/2001/XMLSchema#nonNegativeInteger">1</owl:maxCardinality>
            </owl:Restriction>
        </rdfs:subClassOf>
        <rdfs:comment>Specifies a brief description of an individual action step</rdfs:comment>
        <rdfs:isDefinedBy rdf:resource="http://capec.mitre.org/capec"/>
        <rdfs:label>Attack Step</rdfs:label>
    </owl:Class>
    


    <!-- http://capec.mitre.org/capec#AttackStepOverrideStatement -->

    <owl:Class rdf:about="http://capec.mitre.org/capec#AttackStepOverrideStatement">
        <rdfs:subClassOf rdf:resource="http://capec.mitre.org/capec#AttackStep"/>
        <rdfs:subClassOf rdf:resource="http://www.w3.org/1999/02/22-rdf-syntax-ns#Statement"/>
        <rdfs:comment>Characterizes the pattern-specific overrides applied to an Attack Step</rdfs:comment>
        <rdfs:isDefinedBy rdf:resource="http://capec.mitre.org/capec"/>
        <rdfs:label>Attack step override statement</rdfs:label>
    </owl:Class>
    


    <!-- http://capec.mitre.org/capec#AttackStepTechnique -->

    <owl:Class rdf:about="http://capec.mitre.org/capec#AttackStepTechnique">
        <rdfs:subClassOf>
            <owl:Restriction>
                <owl:onProperty rdf:resource="http://capec.mitre.org/capec#relativeId"/>
                <owl:cardinality rdf:datatype="http://www.w3.org/2001/XMLSchema#nonNegativeInteger">1</owl:cardinality>
            </owl:Restriction>
        </rdfs:subClassOf>
        <rdfs:subClassOf>
            <owl:Restriction>
                <owl:onProperty rdf:resource="http://capec.mitre.org/capec#techniqueId"/>
                <owl:cardinality rdf:datatype="http://www.w3.org/2001/XMLSchema#nonNegativeInteger">1</owl:cardinality>
            </owl:Restriction>
        </rdfs:subClassOf>
        <rdfs:comment>Characterizes a particular technique that may accomplish this attack step</rdfs:comment>
        <rdfs:isDefinedBy rdf:resource="http://capec.mitre.org/capec"/>
        <rdfs:label>Attack Step Technique</rdfs:label>
    </owl:Class>
    


    <!-- http://capec.mitre.org/capec#Audience -->

    <owl:Class rdf:about="http://capec.mitre.org/capec#Audience">
        <rdfs:subClassOf>
            <owl:Restriction>
                <owl:onProperty rdf:resource="http://capec.mitre.org/capec#extendedDescription"/>
                <owl:minCardinality rdf:datatype="http://www.w3.org/2001/XMLSchema#nonNegativeInteger">1</owl:minCardinality>
            </owl:Restriction>
        </rdfs:subClassOf>
        <rdfs:subClassOf>
            <owl:Restriction>
                <owl:onProperty rdf:resource="http://capec.mitre.org/capec#stakeholder"/>
                <owl:cardinality rdf:datatype="http://www.w3.org/2001/XMLSchema#nonNegativeInteger">1</owl:cardinality>
            </owl:Restriction>
        </rdfs:subClassOf>
        <rdfs:comment>Characterizes a reference to the target audience or group for this view.</rdfs:comment>
        <rdfs:isDefinedBy rdf:resource="http://capec.mitre.org/capec"/>
        <rdfs:label>Audience</rdfs:label>
    </owl:Class>
    


    <!-- http://capec.mitre.org/capec#Category -->

    <owl:Class rdf:about="http://capec.mitre.org/capec#Category">
        <rdfs:subClassOf>
            <owl:Restriction>
                <owl:onProperty rdf:resource="http://capec.mitre.org/capec#categoryName"/>
                <owl:cardinality rdf:datatype="http://www.w3.org/2001/XMLSchema#nonNegativeInteger">1</owl:cardinality>
            </owl:Restriction>
        </rdfs:subClassOf>
        <rdfs:subClassOf>
            <owl:Restriction>
                <owl:onProperty rdf:resource="http://capec.mitre.org/capec#description"/>
                <owl:cardinality rdf:datatype="http://www.w3.org/2001/XMLSchema#nonNegativeInteger">1</owl:cardinality>
            </owl:Restriction>
        </rdfs:subClassOf>
        <rdfs:subClassOf>
            <owl:Restriction>
                <owl:onProperty rdf:resource="http://capec.mitre.org/capec#id"/>
                <owl:cardinality rdf:datatype="http://www.w3.org/2001/XMLSchema#nonNegativeInteger">1</owl:cardinality>
            </owl:Restriction>
        </rdfs:subClassOf>
        <rdfs:subClassOf>
            <owl:Restriction>
                <owl:onProperty rdf:resource="http://capec.mitre.org/capec#status"/>
                <owl:cardinality rdf:datatype="http://www.w3.org/2001/XMLSchema#nonNegativeInteger">1</owl:cardinality>
            </owl:Restriction>
        </rdfs:subClassOf>
        <rdfs:subClassOf>
            <owl:Restriction>
                <owl:onProperty rdf:resource="http://capec.mitre.org/capec#extendedDescription"/>
                <owl:maxCardinality rdf:datatype="http://www.w3.org/2001/XMLSchema#nonNegativeInteger">1</owl:maxCardinality>
            </owl:Restriction>
        </rdfs:subClassOf>
        <rdfs:subClassOf>
            <owl:Restriction>
                <owl:onProperty rdf:resource="http://capec.mitre.org/capec#resourcesRequired"/>
                <owl:maxCardinality rdf:datatype="http://www.w3.org/2001/XMLSchema#nonNegativeInteger">1</owl:maxCardinality>
            </owl:Restriction>
        </rdfs:subClassOf>
        <rdfs:comment>Characterizes  a collection of attack patterns sharing a common attribute.</rdfs:comment>
        <rdfs:isDefinedBy rdf:resource="http://capec.mitre.org/capec"/>
        <rdfs:label>Category</rdfs:label>
    </owl:Class>
    


    <!-- http://capec.mitre.org/capec#CommandStructure -->

    <owl:Class rdf:about="http://capec.mitre.org/capec#CommandStructure">
        <rdfs:subClassOf>
            <owl:Restriction>
                <owl:onProperty rdf:resource="http://capec.mitre.org/capec#commandStructureId"/>
                <owl:cardinality rdf:datatype="http://www.w3.org/2001/XMLSchema#nonNegativeInteger">1</owl:cardinality>
            </owl:Restriction>
        </rdfs:subClassOf>
        <rdfs:subClassOf>
            <owl:Restriction>
                <owl:onProperty rdf:resource="http://capec.mitre.org/capec#commandStructureName"/>
                <owl:cardinality rdf:datatype="http://www.w3.org/2001/XMLSchema#nonNegativeInteger">1</owl:cardinality>
            </owl:Restriction>
        </rdfs:subClassOf>
        <rdfs:subClassOf>
            <owl:Restriction>
                <owl:onProperty rdf:resource="http://capec.mitre.org/capec#commandDescription"/>
                <owl:maxCardinality rdf:datatype="http://www.w3.org/2001/XMLSchema#nonNegativeInteger">1</owl:maxCardinality>
            </owl:Restriction>
        </rdfs:subClassOf>
        <rdfs:subClassOf>
            <owl:Restriction>
                <owl:onProperty rdf:resource="http://capec.mitre.org/capec#commandGroupLabel"/>
                <owl:maxCardinality rdf:datatype="http://www.w3.org/2001/XMLSchema#nonNegativeInteger">1</owl:maxCardinality>
            </owl:Restriction>
        </rdfs:subClassOf>
        <rdfs:subClassOf>
            <owl:Restriction>
                <owl:onProperty rdf:resource="http://capec.mitre.org/capec#commandType"/>
                <owl:maxCardinality rdf:datatype="http://www.w3.org/2001/XMLSchema#nonNegativeInteger">1</owl:maxCardinality>
            </owl:Restriction>
        </rdfs:subClassOf>
        <rdfs:comment>Represents a protocol&apos;s Command Structure</rdfs:comment>
        <rdfs:isDefinedBy rdf:resource="http://capec.mitre.org/capec"/>
        <rdfs:label>Command Structure</rdfs:label>
    </owl:Class>
    


    <!-- http://capec.mitre.org/capec#CommonAttackSurface -->

    <owl:Class rdf:about="http://capec.mitre.org/capec#CommonAttackSurface">
        <rdfs:subClassOf rdf:resource="http://capec.mitre.org/capec#TargetAttackSurfaceDescription"/>
        <rdfs:comment>Characterizes a common Attack Surface</rdfs:comment>
        <rdfs:isDefinedBy rdf:resource="http://capec.mitre.org/capec"/>
        <rdfs:label>Common Attack Surface</rdfs:label>
    </owl:Class>
    


    <!-- http://capec.mitre.org/capec#CommonAttackSurfaceDescription -->

    <owl:Class rdf:about="http://capec.mitre.org/capec#CommonAttackSurfaceDescription">
        <rdfs:subClassOf>
            <owl:Restriction>
                <owl:onProperty rdf:resource="http://capec.mitre.org/capec#patternSpecificOverrides"/>
                <owl:maxCardinality rdf:datatype="http://www.w3.org/2001/XMLSchema#nonNegativeInteger">1</owl:maxCardinality>
            </owl:Restriction>
        </rdfs:subClassOf>
        <rdfs:subClassOf>
            <owl:Restriction>
                <owl:onProperty rdf:resource="http://capec.mitre.org/capec#attackSurfaceId"/>
                <owl:cardinality rdf:datatype="http://www.w3.org/2001/XMLSchema#nonNegativeInteger">1</owl:cardinality>
            </owl:Restriction>
        </rdfs:subClassOf>
        <rdfs:subClassOf>
            <owl:Restriction>
                <owl:onProperty rdf:resource="http://capec.mitre.org/capec#relativeId"/>
                <owl:cardinality rdf:datatype="http://www.w3.org/2001/XMLSchema#nonNegativeInteger">1</owl:cardinality>
            </owl:Restriction>
        </rdfs:subClassOf>
        <rdfs:comment>Characterizes a description of a Common Attack Surface</rdfs:comment>
        <rdfs:isDefinedBy rdf:resource="http://capec.mitre.org/capec"/>
        <rdfs:label>Relevant attack surface</rdfs:label>
    </owl:Class>
    


    <!-- http://capec.mitre.org/capec#CompoundElement -->

    <owl:Class rdf:about="http://capec.mitre.org/capec#CompoundElement">
        <rdfs:subClassOf>
            <owl:Restriction>
                <owl:onProperty rdf:resource="http://capec.mitre.org/capec#compoundElementAbstraction"/>
                <owl:cardinality rdf:datatype="http://www.w3.org/2001/XMLSchema#nonNegativeInteger">1</owl:cardinality>
            </owl:Restriction>
        </rdfs:subClassOf>
        <rdfs:subClassOf>
            <owl:Restriction>
                <owl:onProperty rdf:resource="http://capec.mitre.org/capec#compoundElementCompleteness"/>
                <owl:cardinality rdf:datatype="http://www.w3.org/2001/XMLSchema#nonNegativeInteger">1</owl:cardinality>
            </owl:Restriction>
        </rdfs:subClassOf>
        <rdfs:subClassOf>
            <owl:Restriction>
                <owl:onProperty rdf:resource="http://capec.mitre.org/capec#compoundElementStructure"/>
                <owl:cardinality rdf:datatype="http://www.w3.org/2001/XMLSchema#nonNegativeInteger">1</owl:cardinality>
            </owl:Restriction>
        </rdfs:subClassOf>
        <rdfs:subClassOf>
            <owl:Restriction>
                <owl:onProperty rdf:resource="http://capec.mitre.org/capec#description"/>
                <owl:cardinality rdf:datatype="http://www.w3.org/2001/XMLSchema#nonNegativeInteger">1</owl:cardinality>
            </owl:Restriction>
        </rdfs:subClassOf>
        <rdfs:subClassOf>
            <owl:Restriction>
                <owl:onProperty rdf:resource="http://capec.mitre.org/capec#formattedIdentifier"/>
                <owl:cardinality rdf:datatype="http://www.w3.org/2001/XMLSchema#nonNegativeInteger">1</owl:cardinality>
            </owl:Restriction>
        </rdfs:subClassOf>
        <rdfs:subClassOf>
            <owl:Restriction>
                <owl:onProperty rdf:resource="http://capec.mitre.org/capec#id"/>
                <owl:cardinality rdf:datatype="http://www.w3.org/2001/XMLSchema#nonNegativeInteger">1</owl:cardinality>
            </owl:Restriction>
        </rdfs:subClassOf>
        <rdfs:subClassOf>
            <owl:Restriction>
                <owl:onProperty rdf:resource="http://capec.mitre.org/capec#status"/>
                <owl:cardinality rdf:datatype="http://www.w3.org/2001/XMLSchema#nonNegativeInteger">1</owl:cardinality>
            </owl:Restriction>
        </rdfs:subClassOf>
        <rdfs:subClassOf>
            <owl:Restriction>
                <owl:onProperty rdf:resource="http://capec.mitre.org/capec#extendedDescription"/>
                <owl:maxCardinality rdf:datatype="http://www.w3.org/2001/XMLSchema#nonNegativeInteger">1</owl:maxCardinality>
            </owl:Restriction>
        </rdfs:subClassOf>
        <rdfs:comment>Characterizes a meaningful aggregation of several attack patterns, as in a chain.</rdfs:comment>
        <rdfs:isDefinedBy rdf:resource="http://capec.mitre.org/capec"/>
        <rdfs:label>Compound Element</rdfs:label>
    </owl:Class>
    


    <!-- http://capec.mitre.org/capec#Consequence -->

    <owl:Class rdf:about="http://capec.mitre.org/capec#Consequence">
        <rdfs:subClassOf>
            <owl:Restriction>
                <owl:onProperty rdf:resource="http://capec.mitre.org/capec#consequenceId"/>
                <owl:cardinality rdf:datatype="http://www.w3.org/2001/XMLSchema#nonNegativeInteger">1</owl:cardinality>
            </owl:Restriction>
        </rdfs:subClassOf>
        <rdfs:subClassOf>
            <owl:Restriction>
                <owl:onProperty rdf:resource="http://capec.mitre.org/capec#relativeId"/>
                <owl:cardinality rdf:datatype="http://www.w3.org/2001/XMLSchema#nonNegativeInteger">1</owl:cardinality>
            </owl:Restriction>
        </rdfs:subClassOf>
        <rdfs:subClassOf>
            <owl:Restriction>
                <owl:onProperty rdf:resource="http://capec.mitre.org/capec#consequenceNote"/>
                <owl:maxCardinality rdf:datatype="http://www.w3.org/2001/XMLSchema#nonNegativeInteger">1</owl:maxCardinality>
            </owl:Restriction>
        </rdfs:subClassOf>
        <rdfs:comment>Characterizes a motivation and consequences that may be associated.</rdfs:comment>
        <rdfs:isDefinedBy rdf:resource="http://capec.mitre.org/capec"/>
        <rdfs:label>Consequence</rdfs:label>
    </owl:Class>
    


    <!-- http://capec.mitre.org/capec#Environment -->

    <owl:Class rdf:about="http://capec.mitre.org/capec#Environment">
        <rdfs:subClassOf>
            <owl:Restriction>
                <owl:onProperty rdf:resource="http://capec.mitre.org/capec#environmentId"/>
                <owl:cardinality rdf:datatype="http://www.w3.org/2001/XMLSchema#nonNegativeInteger">1</owl:cardinality>
            </owl:Restriction>
        </rdfs:subClassOf>
        <rdfs:subClassOf>
            <owl:Restriction>
                <owl:onProperty rdf:resource="http://capec.mitre.org/capec#environmentTitle"/>
                <owl:cardinality rdf:datatype="http://www.w3.org/2001/XMLSchema#nonNegativeInteger">1</owl:cardinality>
            </owl:Restriction>
        </rdfs:subClassOf>
        <rdfs:subClassOf>
            <owl:Restriction>
                <owl:onProperty rdf:resource="http://capec.mitre.org/capec#environmentDescription"/>
                <owl:maxCardinality rdf:datatype="http://www.w3.org/2001/XMLSchema#nonNegativeInteger">1</owl:maxCardinality>
            </owl:Restriction>
        </rdfs:subClassOf>
        <rdfs:comment>Represents a kind of environment or context that is required. Used in Attack Steps, Indicators of Susceptibility, and Security Controls, etc.</rdfs:comment>
        <rdfs:isDefinedBy rdf:resource="http://capec.mitre.org/capec"/>
        <rdfs:label>Environment</rdfs:label>
    </owl:Class>
    


    <!-- http://capec.mitre.org/capec#ExampleInstance -->

    <owl:Class rdf:about="http://capec.mitre.org/capec#ExampleInstance">
        <rdfs:subClassOf>
            <owl:Restriction>
                <owl:onProperty rdf:resource="http://capec.mitre.org/capec#exampleInstanceDescription"/>
                <owl:cardinality rdf:datatype="http://www.w3.org/2001/XMLSchema#nonNegativeInteger">1</owl:cardinality>
            </owl:Restriction>
        </rdfs:subClassOf>
        <rdfs:subClassOf>
            <owl:Restriction>
                <owl:onProperty rdf:resource="http://capec.mitre.org/capec#relativeId"/>
                <owl:cardinality rdf:datatype="http://www.w3.org/2001/XMLSchema#nonNegativeInteger">1</owl:cardinality>
            </owl:Restriction>
        </rdfs:subClassOf>
        <rdfs:comment>Represents an individual example or exploit instance.</rdfs:comment>
        <rdfs:isDefinedBy rdf:resource="http://capec.mitre.org/capec"/>
        <rdfs:label>Example Instance</rdfs:label>
    </owl:Class>
    


    <!-- http://capec.mitre.org/capec#FunctionalService -->

    <owl:Class rdf:about="http://capec.mitre.org/capec#FunctionalService">
        <rdfs:subClassOf>
            <owl:Restriction>
                <owl:onProperty rdf:resource="http://capec.mitre.org/capec#functionalServiceId"/>
                <owl:cardinality rdf:datatype="http://www.w3.org/2001/XMLSchema#nonNegativeInteger">1</owl:cardinality>
            </owl:Restriction>
        </rdfs:subClassOf>
        <rdfs:subClassOf>
            <owl:Restriction>
                <owl:onProperty rdf:resource="http://capec.mitre.org/capec#functionalServiceName"/>
                <owl:cardinality rdf:datatype="http://www.w3.org/2001/XMLSchema#nonNegativeInteger">1</owl:cardinality>
            </owl:Restriction>
        </rdfs:subClassOf>
        <rdfs:comment>Characterizes a Functional Service associated with an attack pattern</rdfs:comment>
        <rdfs:isDefinedBy rdf:resource="http://capec.mitre.org/capec"/>
        <rdfs:label>Functional Service</rdfs:label>
    </owl:Class>
    


    <!-- http://capec.mitre.org/capec#HistoryRecord -->

    <owl:Class rdf:about="http://capec.mitre.org/capec#HistoryRecord">
        <rdfs:subClassOf>
            <owl:Restriction>
                <owl:onProperty rdf:resource="http://capec.mitre.org/capec#contributionMode"/>
                <owl:cardinality rdf:datatype="http://www.w3.org/2001/XMLSchema#nonNegativeInteger">1</owl:cardinality>
            </owl:Restriction>
        </rdfs:subClassOf>
        <rdfs:subClassOf>
            <owl:Restriction>
                <owl:onProperty rdf:resource="http://capec.mitre.org/capec#entryType"/>
                <owl:cardinality rdf:datatype="http://www.w3.org/2001/XMLSchema#nonNegativeInteger">1</owl:cardinality>
            </owl:Restriction>
        </rdfs:subClassOf>
        <rdfs:subClassOf>
            <owl:Restriction>
                <owl:onProperty rdf:resource="http://capec.mitre.org/capec#relativeId"/>
                <owl:cardinality rdf:datatype="http://www.w3.org/2001/XMLSchema#nonNegativeInteger">1</owl:cardinality>
            </owl:Restriction>
        </rdfs:subClassOf>
        <rdfs:subClassOf>
            <owl:Restriction>
                <owl:onProperty rdf:resource="http://capec.mitre.org/capec#contributionMode"/>
                <owl:maxCardinality rdf:datatype="http://www.w3.org/2001/XMLSchema#nonNegativeInteger">1</owl:maxCardinality>
            </owl:Restriction>
        </rdfs:subClassOf>
        <rdfs:subClassOf>
            <owl:Restriction>
                <owl:onProperty rdf:resource="http://capec.mitre.org/capec#contributionSource"/>
                <owl:maxCardinality rdf:datatype="http://www.w3.org/2001/XMLSchema#nonNegativeInteger">1</owl:maxCardinality>
            </owl:Restriction>
        </rdfs:subClassOf>
        <rdfs:subClassOf>
            <owl:Restriction>
                <owl:onProperty rdf:resource="http://capec.mitre.org/capec#entryDate"/>
                <owl:maxCardinality rdf:datatype="http://www.w3.org/2001/XMLSchema#nonNegativeInteger">1</owl:maxCardinality>
            </owl:Restriction>
        </rdfs:subClassOf>
        <rdfs:subClassOf>
            <owl:Restriction>
                <owl:onProperty rdf:resource="http://capec.mitre.org/capec#entryNameChangeDate"/>
                <owl:maxCardinality rdf:datatype="http://www.w3.org/2001/XMLSchema#nonNegativeInteger">1</owl:maxCardinality>
            </owl:Restriction>
        </rdfs:subClassOf>
        <rdfs:subClassOf>
            <owl:Restriction>
                <owl:onProperty rdf:resource="http://capec.mitre.org/capec#previousEntryName"/>
                <owl:maxCardinality rdf:datatype="http://www.w3.org/2001/XMLSchema#nonNegativeInteger">1</owl:maxCardinality>
            </owl:Restriction>
        </rdfs:subClassOf>
        <rdfs:subClassOf>
            <owl:Restriction>
                <owl:onProperty rdf:resource="http://capec.mitre.org/capec#submissionSource"/>
                <owl:maxCardinality rdf:datatype="http://www.w3.org/2001/XMLSchema#nonNegativeInteger">1</owl:maxCardinality>
            </owl:Restriction>
        </rdfs:subClassOf>
        <rdfs:comment>Characterizes a record of submissions, contributions, modifications, and changes to an entity.  It is used to keep track of the author of an entry and anyone who has made modifications to the content. This provides a means of contacting the authors and modifiers for clarifying ambiguities, merging overlapping 	contributions, etc. This should be filled out for all entries.</rdfs:comment>
        <rdfs:isDefinedBy rdf:resource="http://capec.mitre.org/capec"/>
        <rdfs:label>History Record</rdfs:label>
    </owl:Class>
    


    <!-- http://capec.mitre.org/capec#IndicatorWarning -->

    <owl:Class rdf:about="http://capec.mitre.org/capec#IndicatorWarning">
        <rdfs:subClassOf>
            <owl:Restriction>
                <owl:onProperty rdf:resource="http://capec.mitre.org/capec#observables"/>
                <owl:maxCardinality rdf:datatype="http://www.w3.org/2001/XMLSchema#nonNegativeInteger">1</owl:maxCardinality>
            </owl:Restriction>
        </rdfs:subClassOf>
        <rdfs:subClassOf>
            <owl:Restriction>
                <owl:onProperty rdf:resource="http://capec.mitre.org/capec#relativeId"/>
                <owl:cardinality rdf:datatype="http://www.w3.org/2001/XMLSchema#nonNegativeInteger">1</owl:cardinality>
            </owl:Restriction>
        </rdfs:subClassOf>
        <rdfs:subClassOf>
            <owl:Restriction>
                <owl:onProperty rdf:resource="http://capec.mitre.org/capec#extendedDescription"/>
                <owl:maxCardinality rdf:datatype="http://www.w3.org/2001/XMLSchema#nonNegativeInteger">1</owl:maxCardinality>
            </owl:Restriction>
        </rdfs:subClassOf>
        <rdfs:comment>Characterizes an Indicator Warning for an attack</rdfs:comment>
        <rdfs:isDefinedBy rdf:resource="http://capec.mitre.org/capec"/>
        <rdfs:label>Indicator Warning</rdfs:label>
    </owl:Class>
    


    <!-- http://capec.mitre.org/capec#Knowlege -->

    <owl:Class rdf:about="http://capec.mitre.org/capec#Knowlege">
        <rdfs:subClassOf>
            <owl:Restriction>
                <owl:onProperty rdf:resource="http://capec.mitre.org/capec#relativeId"/>
                <owl:cardinality rdf:datatype="http://www.w3.org/2001/XMLSchema#nonNegativeInteger">1</owl:cardinality>
            </owl:Restriction>
        </rdfs:subClassOf>
        <rdfs:subClassOf>
            <owl:Restriction>
                <owl:onProperty rdf:resource="http://capec.mitre.org/capec#skillKnowledgeDescription"/>
                <owl:cardinality rdf:datatype="http://www.w3.org/2001/XMLSchema#nonNegativeInteger">1</owl:cardinality>
            </owl:Restriction>
        </rdfs:subClassOf>
        <rdfs:subClassOf>
            <owl:Restriction>
                <owl:onProperty rdf:resource="http://capec.mitre.org/capec#skillKnowledgeLevel"/>
                <owl:cardinality rdf:datatype="http://www.w3.org/2001/XMLSchema#nonNegativeInteger">1</owl:cardinality>
            </owl:Restriction>
        </rdfs:subClassOf>
        <rdfs:comment>Characterizes a skill or knowledge</rdfs:comment>
        <rdfs:isDefinedBy rdf:resource="http://capec.mitre.org/capec"/>
        <rdfs:label>Knowlege</rdfs:label>
    </owl:Class>
    


    <!-- http://capec.mitre.org/capec#ObfuscationTechnique -->

    <owl:Class rdf:about="http://capec.mitre.org/capec#ObfuscationTechnique">
        <rdfs:subClassOf>
            <owl:Restriction>
                <owl:onProperty rdf:resource="http://capec.mitre.org/capec#observables"/>
                <owl:maxCardinality rdf:datatype="http://www.w3.org/2001/XMLSchema#nonNegativeInteger">1</owl:maxCardinality>
            </owl:Restriction>
        </rdfs:subClassOf>
        <rdfs:subClassOf>
            <owl:Restriction>
                <owl:onProperty rdf:resource="http://capec.mitre.org/capec#relativeId"/>
                <owl:cardinality rdf:datatype="http://www.w3.org/2001/XMLSchema#nonNegativeInteger">1</owl:cardinality>
            </owl:Restriction>
        </rdfs:subClassOf>
        <rdfs:subClassOf>
            <owl:Restriction>
                <owl:onProperty rdf:resource="http://capec.mitre.org/capec#extendedDescription"/>
                <owl:maxCardinality rdf:datatype="http://www.w3.org/2001/XMLSchema#nonNegativeInteger">1</owl:maxCardinality>
            </owl:Restriction>
        </rdfs:subClassOf>
        <rdfs:subClassOf>
            <owl:Restriction>
                <owl:onProperty rdf:resource="http://capec.mitre.org/capec#techniqueName"/>
                <owl:maxCardinality rdf:datatype="http://www.w3.org/2001/XMLSchema#nonNegativeInteger">1</owl:maxCardinality>
            </owl:Restriction>
        </rdfs:subClassOf>
        <rdfs:comment>Characterizes a technique used to obfuscate an attackers actions</rdfs:comment>
        <rdfs:isDefinedBy rdf:resource="http://capec.mitre.org/capec"/>
        <rdfs:label>Obfuscation Technique</rdfs:label>
    </owl:Class>
    


    <!-- http://capec.mitre.org/capec#Outcome -->

    <owl:Class rdf:about="http://capec.mitre.org/capec#Outcome">
        <rdfs:subClassOf>
            <owl:Restriction>
                <owl:onProperty rdf:resource="http://capec.mitre.org/capec#outcomeDescription"/>
                <owl:cardinality rdf:datatype="http://www.w3.org/2001/XMLSchema#nonNegativeInteger">1</owl:cardinality>
            </owl:Restriction>
        </rdfs:subClassOf>
        <rdfs:subClassOf>
            <owl:Restriction>
                <owl:onProperty rdf:resource="http://capec.mitre.org/capec#outcomeId"/>
                <owl:cardinality rdf:datatype="http://www.w3.org/2001/XMLSchema#nonNegativeInteger">1</owl:cardinality>
            </owl:Restriction>
        </rdfs:subClassOf>
        <rdfs:subClassOf>
            <owl:Restriction>
                <owl:onProperty rdf:resource="http://capec.mitre.org/capec#outcomeType"/>
                <owl:cardinality rdf:datatype="http://www.w3.org/2001/XMLSchema#nonNegativeInteger">1</owl:cardinality>
            </owl:Restriction>
        </rdfs:subClassOf>
        <rdfs:subClassOf>
            <owl:Restriction>
                <owl:onProperty rdf:resource="http://capec.mitre.org/capec#relativeId"/>
                <owl:cardinality rdf:datatype="http://www.w3.org/2001/XMLSchema#nonNegativeInteger">1</owl:cardinality>
            </owl:Restriction>
        </rdfs:subClassOf>
        <rdfs:comment>Represents a possible Outcome for an attack step</rdfs:comment>
        <rdfs:isDefinedBy rdf:resource="http://capec.mitre.org/capec"/>
        <rdfs:label>Outcome</rdfs:label>
    </owl:Class>
    


    <!-- http://capec.mitre.org/capec#ProbingTechnique -->

    <owl:Class rdf:about="http://capec.mitre.org/capec#ProbingTechnique">
        <rdfs:subClassOf>
            <owl:Restriction>
                <owl:onProperty rdf:resource="http://capec.mitre.org/capec#relativeId"/>
                <owl:cardinality rdf:datatype="http://www.w3.org/2001/XMLSchema#nonNegativeInteger">1</owl:cardinality>
            </owl:Restriction>
        </rdfs:subClassOf>
        <rdfs:subClassOf>
            <owl:Restriction>
                <owl:onProperty rdf:resource="http://capec.mitre.org/capec#extendedDescription"/>
                <owl:maxCardinality rdf:datatype="http://www.w3.org/2001/XMLSchema#nonNegativeInteger">1</owl:maxCardinality>
            </owl:Restriction>
        </rdfs:subClassOf>
        <rdfs:subClassOf>
            <owl:Restriction>
                <owl:onProperty rdf:resource="http://capec.mitre.org/capec#techniqueName"/>
                <owl:maxCardinality rdf:datatype="http://www.w3.org/2001/XMLSchema#nonNegativeInteger">1</owl:maxCardinality>
            </owl:Restriction>
        </rdfs:subClassOf>
        <rdfs:comment>Characterizes the technique used to probe a target</rdfs:comment>
        <rdfs:isDefinedBy rdf:resource="http://capec.mitre.org/capec"/>
        <rdfs:label>Probing Technique</rdfs:label>
    </owl:Class>
    


    <!-- http://capec.mitre.org/capec#Reference -->

    <owl:Class rdf:about="http://capec.mitre.org/capec#Reference">
        <rdfs:subClassOf>
            <owl:Restriction>
                <owl:onProperty rdf:resource="http://capec.mitre.org/capec#referencePublisher"/>
                <owl:maxCardinality rdf:datatype="http://www.w3.org/2001/XMLSchema#nonNegativeInteger">1</owl:maxCardinality>
            </owl:Restriction>
        </rdfs:subClassOf>
        <rdfs:subClassOf>
            <owl:Restriction>
                <owl:onProperty rdf:resource="http://capec.mitre.org/capec#localReferenceId"/>
                <owl:cardinality rdf:datatype="http://www.w3.org/2001/XMLSchema#nonNegativeInteger">1</owl:cardinality>
            </owl:Restriction>
        </rdfs:subClassOf>
        <rdfs:subClassOf>
            <owl:Restriction>
                <owl:onProperty rdf:resource="http://capec.mitre.org/capec#referenceDescription"/>
                <owl:maxCardinality rdf:datatype="http://www.w3.org/2001/XMLSchema#nonNegativeInteger">1</owl:maxCardinality>
            </owl:Restriction>
        </rdfs:subClassOf>
        <rdfs:subClassOf>
            <owl:Restriction>
                <owl:onProperty rdf:resource="http://capec.mitre.org/capec#referenceEdition"/>
                <owl:maxCardinality rdf:datatype="http://www.w3.org/2001/XMLSchema#nonNegativeInteger">1</owl:maxCardinality>
            </owl:Restriction>
        </rdfs:subClassOf>
        <rdfs:subClassOf>
            <owl:Restriction>
                <owl:onProperty rdf:resource="http://capec.mitre.org/capec#referenceId"/>
                <owl:maxCardinality rdf:datatype="http://www.w3.org/2001/XMLSchema#nonNegativeInteger">1</owl:maxCardinality>
            </owl:Restriction>
        </rdfs:subClassOf>
        <rdfs:subClassOf>
            <owl:Restriction>
                <owl:onProperty rdf:resource="http://capec.mitre.org/capec#referencePublication"/>
                <owl:maxCardinality rdf:datatype="http://www.w3.org/2001/XMLSchema#nonNegativeInteger">1</owl:maxCardinality>
            </owl:Restriction>
        </rdfs:subClassOf>
        <rdfs:subClassOf>
            <owl:Restriction>
                <owl:onProperty rdf:resource="http://capec.mitre.org/capec#referencePublisherName"/>
                <owl:maxCardinality rdf:datatype="http://www.w3.org/2001/XMLSchema#nonNegativeInteger">1</owl:maxCardinality>
            </owl:Restriction>
        </rdfs:subClassOf>
        <rdfs:subClassOf>
            <owl:Restriction>
                <owl:onProperty rdf:resource="http://capec.mitre.org/capec#referenceSection"/>
                <owl:maxCardinality rdf:datatype="http://www.w3.org/2001/XMLSchema#nonNegativeInteger">1</owl:maxCardinality>
            </owl:Restriction>
        </rdfs:subClassOf>
        <rdfs:subClassOf>
            <owl:Restriction>
                <owl:onProperty rdf:resource="http://capec.mitre.org/capec#referenceTitle"/>
                <owl:maxCardinality rdf:datatype="http://www.w3.org/2001/XMLSchema#nonNegativeInteger">1</owl:maxCardinality>
            </owl:Restriction>
        </rdfs:subClassOf>
        <rdfs:comment>Represents a Reference</rdfs:comment>
        <rdfs:isDefinedBy rdf:resource="http://capec.mitre.org/capec"/>
        <rdfs:label>Reference</rdfs:label>
    </owl:Class>
    


    <!-- http://capec.mitre.org/capec#RelatedProtocolStatement -->

    <owl:Class rdf:about="http://capec.mitre.org/capec#RelatedProtocolStatement">
        <rdfs:subClassOf rdf:resource="http://www.w3.org/1999/02/22-rdf-syntax-ns#Statement"/>
        <rdfs:comment>Represents a Related Protocol</rdfs:comment>
        <rdfs:isDefinedBy rdf:resource="http://capec.mitre.org/capec"/>
        <rdfs:label>Related Protocol</rdfs:label>
    </owl:Class>
    


    <!-- http://capec.mitre.org/capec#RelatedVulnerabilityStatement -->

    <owl:Class rdf:about="http://capec.mitre.org/capec#RelatedVulnerabilityStatement">
        <rdfs:subClassOf rdf:resource="http://www.w3.org/1999/02/22-rdf-syntax-ns#Statement"/>
        <rdfs:subClassOf>
            <owl:Restriction>
                <owl:onProperty rdf:resource="http://capec.mitre.org/capec#vulnerability"/>
                <owl:maxCardinality rdf:datatype="http://www.w3.org/2001/XMLSchema#nonNegativeInteger">1</owl:maxCardinality>
            </owl:Restriction>
        </rdfs:subClassOf>
        <rdfs:subClassOf>
            <owl:Restriction>
                <owl:onProperty rdf:resource="http://capec.mitre.org/capec#vulnerabilityId"/>
                <owl:cardinality rdf:datatype="http://www.w3.org/2001/XMLSchema#nonNegativeInteger">1</owl:cardinality>
            </owl:Restriction>
        </rdfs:subClassOf>
        <rdfs:subClassOf>
            <owl:Restriction>
                <owl:onProperty rdf:resource="http://capec.mitre.org/capec#vulnerabilityDescription"/>
                <owl:maxCardinality rdf:datatype="http://www.w3.org/2001/XMLSchema#nonNegativeInteger">1</owl:maxCardinality>
            </owl:Restriction>
        </rdfs:subClassOf>
        <rdfs:comment>Characterizes the relationship to a Vulnerability</rdfs:comment>
        <rdfs:isDefinedBy rdf:resource="http://capec.mitre.org/capec"/>
        <rdfs:label>Related Vulnerability</rdfs:label>
    </owl:Class>
    


    <!-- http://capec.mitre.org/capec#RelatedWeaknessStatement -->

    <owl:Class rdf:about="http://capec.mitre.org/capec#RelatedWeaknessStatement">
        <rdfs:subClassOf rdf:resource="http://www.w3.org/1999/02/22-rdf-syntax-ns#Statement"/>
        <rdfs:subClassOf>
            <owl:Restriction>
                <owl:onProperty rdf:resource="http://capec.mitre.org/capec#weaknessId"/>
                <owl:cardinality rdf:datatype="http://www.w3.org/2001/XMLSchema#nonNegativeInteger">1</owl:cardinality>
            </owl:Restriction>
        </rdfs:subClassOf>
        <rdfs:subClassOf>
            <owl:Restriction>
                <owl:onProperty rdf:resource="http://capec.mitre.org/capec#weaknessRelationshipType"/>
                <owl:cardinality rdf:datatype="http://www.w3.org/2001/XMLSchema#nonNegativeInteger">1</owl:cardinality>
            </owl:Restriction>
        </rdfs:subClassOf>
        <rdfs:comment>Characterizes the relationship to the related weakness</rdfs:comment>
        <rdfs:isDefinedBy rdf:resource="http://capec.mitre.org/capec"/>
        <rdfs:label>Related weakness</rdfs:label>
    </owl:Class>
    


    <!-- http://capec.mitre.org/capec#RelationshipStatement -->

    <owl:Class rdf:about="http://capec.mitre.org/capec#RelationshipStatement">
        <rdfs:subClassOf rdf:resource="http://www.w3.org/1999/02/22-rdf-syntax-ns#Statement"/>
        <rdfs:subClassOf>
            <owl:Restriction>
                <owl:onProperty rdf:resource="http://capec.mitre.org/capec#relationshipNature"/>
                <owl:minCardinality rdf:datatype="http://www.w3.org/2001/XMLSchema#nonNegativeInteger">1</owl:minCardinality>
            </owl:Restriction>
        </rdfs:subClassOf>
        <rdfs:subClassOf>
            <owl:Restriction>
                <owl:onProperty rdf:resource="http://capec.mitre.org/capec#relationshipTargetForm"/>
                <owl:cardinality rdf:datatype="http://www.w3.org/2001/XMLSchema#nonNegativeInteger">1</owl:cardinality>
            </owl:Restriction>
        </rdfs:subClassOf>
        <rdfs:subClassOf>
            <owl:Restriction>
                <owl:onProperty rdf:resource="http://capec.mitre.org/capec#relationshipViewOrdinal"/>
                <owl:maxCardinality rdf:datatype="http://www.w3.org/2001/XMLSchema#nonNegativeInteger">1</owl:maxCardinality>
            </owl:Restriction>
        </rdfs:subClassOf>
        <rdfs:comment>Characterizes a list of the individual Views to which this relationship pertains.</rdfs:comment>
        <rdfs:isDefinedBy rdf:resource="http://capec.mitre.org/capec"/>
        <rdfs:label>Relationship</rdfs:label>
    </owl:Class>
    


    <!-- http://capec.mitre.org/capec#SecurityControl -->

    <owl:Class rdf:about="http://capec.mitre.org/capec#SecurityControl">
        <rdfs:subClassOf>
            <owl:Restriction>
                <owl:onProperty rdf:resource="http://capec.mitre.org/capec#relativeId"/>
                <owl:cardinality rdf:datatype="http://www.w3.org/2001/XMLSchema#nonNegativeInteger">1</owl:cardinality>
            </owl:Restriction>
        </rdfs:subClassOf>
        <rdfs:subClassOf>
            <owl:Restriction>
                <owl:onProperty rdf:resource="http://capec.mitre.org/capec#securityControlId"/>
                <owl:cardinality rdf:datatype="http://www.w3.org/2001/XMLSchema#nonNegativeInteger">1</owl:cardinality>
            </owl:Restriction>
        </rdfs:subClassOf>
        <rdfs:subClassOf>
            <owl:Restriction>
                <owl:onProperty rdf:resource="http://capec.mitre.org/capec#securityControlType"/>
                <owl:cardinality rdf:datatype="http://www.w3.org/2001/XMLSchema#nonNegativeInteger">1</owl:cardinality>
            </owl:Restriction>
        </rdfs:subClassOf>
        <rdfs:comment>Represents a security control for an attack step that describe ways in which the attack step can be detected, corrected, or prevented.  Security Controls are presented from a defender’s point of view, where the defender may be a developer, tester, operations administrator, or other resource resisting the attacker.</rdfs:comment>
        <rdfs:isDefinedBy rdf:resource="http://capec.mitre.org/capec"/>
        <rdfs:label>Security Control</rdfs:label>
    </owl:Class>
    


    <!-- http://capec.mitre.org/capec#SusceptabiltyIndicator -->

    <owl:Class rdf:about="http://capec.mitre.org/capec#SusceptabiltyIndicator">
        <rdfs:subClassOf>
            <owl:Restriction>
                <owl:onProperty rdf:resource="http://capec.mitre.org/capec#indicatorId"/>
                <owl:cardinality rdf:datatype="http://www.w3.org/2001/XMLSchema#nonNegativeInteger">1</owl:cardinality>
            </owl:Restriction>
        </rdfs:subClassOf>
        <rdfs:subClassOf>
            <owl:Restriction>
                <owl:onProperty rdf:resource="http://capec.mitre.org/capec#indicatorType"/>
                <owl:cardinality rdf:datatype="http://www.w3.org/2001/XMLSchema#nonNegativeInteger">1</owl:cardinality>
            </owl:Restriction>
        </rdfs:subClassOf>
        <rdfs:subClassOf>
            <owl:Restriction>
                <owl:onProperty rdf:resource="http://capec.mitre.org/capec#relativeId"/>
                <owl:cardinality rdf:datatype="http://www.w3.org/2001/XMLSchema#nonNegativeInteger">1</owl:cardinality>
            </owl:Restriction>
        </rdfs:subClassOf>
        <rdfs:comment>Characterizes an indicator that the application may or may not be susceptible to the given attack step (not necessarily the pattern as a whole).</rdfs:comment>
        <rdfs:isDefinedBy rdf:resource="http://capec.mitre.org/capec"/>
        <rdfs:label>Indicator</rdfs:label>
    </owl:Class>
    


    <!-- http://capec.mitre.org/capec#TargetAttackSurfaceDescription -->

    <owl:Class rdf:about="http://capec.mitre.org/capec#TargetAttackSurfaceDescription">
        <rdfs:subClassOf>
            <owl:Restriction>
                <owl:onProperty rdf:resource="http://capec.mitre.org/capec#targetAttackSurfaceLocalities"/>
                <owl:minCardinality rdf:datatype="http://www.w3.org/2001/XMLSchema#nonNegativeInteger">1</owl:minCardinality>
            </owl:Restriction>
        </rdfs:subClassOf>
        <rdfs:subClassOf>
            <owl:Restriction>
                <owl:onProperty rdf:resource="http://capec.mitre.org/capec#targetAttackSurfaceTypes"/>
                <owl:minCardinality rdf:datatype="http://www.w3.org/2001/XMLSchema#nonNegativeInteger">1</owl:minCardinality>
            </owl:Restriction>
        </rdfs:subClassOf>
        <rdfs:subClassOf>
            <owl:Restriction>
                <owl:onProperty rdf:resource="http://capec.mitre.org/capec#targetedOSILayers"/>
                <owl:minCardinality rdf:datatype="http://www.w3.org/2001/XMLSchema#nonNegativeInteger">1</owl:minCardinality>
            </owl:Restriction>
        </rdfs:subClassOf>
        <rdfs:subClassOf>
            <owl:Restriction>
                <owl:onProperty rdf:resource="http://capec.mitre.org/capec#attackSurfaceId"/>
                <owl:cardinality rdf:datatype="http://www.w3.org/2001/XMLSchema#nonNegativeInteger">1</owl:cardinality>
            </owl:Restriction>
        </rdfs:subClassOf>
        <rdfs:subClassOf>
            <owl:Restriction>
                <owl:onProperty rdf:resource="http://capec.mitre.org/capec#relativeId"/>
                <owl:cardinality rdf:datatype="http://www.w3.org/2001/XMLSchema#nonNegativeInteger">1</owl:cardinality>
            </owl:Restriction>
        </rdfs:subClassOf>
        <rdfs:comment>Characterizes an Attack Surface</rdfs:comment>
        <rdfs:isDefinedBy rdf:resource="http://capec.mitre.org/capec"/>
        <rdfs:label>Attack Surface</rdfs:label>
    </owl:Class>
    


    <!-- http://capec.mitre.org/capec#TargetedProtocol -->

    <owl:Class rdf:about="http://capec.mitre.org/capec#TargetedProtocol">
        <rdfs:subClassOf>
            <owl:Restriction>
                <owl:onProperty rdf:resource="http://capec.mitre.org/capec#protocol"/>
                <owl:maxCardinality rdf:datatype="http://www.w3.org/2001/XMLSchema#nonNegativeInteger">1</owl:maxCardinality>
            </owl:Restriction>
        </rdfs:subClassOf>
        <rdfs:subClassOf>
            <owl:Restriction>
                <owl:onProperty rdf:resource="http://capec.mitre.org/capec#encryptionUsed"/>
                <owl:cardinality rdf:datatype="http://www.w3.org/2001/XMLSchema#nonNegativeInteger">1</owl:cardinality>
            </owl:Restriction>
        </rdfs:subClassOf>
        <rdfs:subClassOf>
            <owl:Restriction>
                <owl:onProperty rdf:resource="http://capec.mitre.org/capec#relativeId"/>
                <owl:cardinality rdf:datatype="http://www.w3.org/2001/XMLSchema#nonNegativeInteger">1</owl:cardinality>
            </owl:Restriction>
        </rdfs:subClassOf>
        <rdfs:subClassOf>
            <owl:Restriction>
                <owl:onProperty rdf:resource="http://capec.mitre.org/capec#targetProtocolId"/>
                <owl:cardinality rdf:datatype="http://www.w3.org/2001/XMLSchema#nonNegativeInteger">1</owl:cardinality>
            </owl:Restriction>
        </rdfs:subClassOf>
        <rdfs:subClassOf>
            <owl:Restriction>
                <owl:onProperty rdf:resource="http://capec.mitre.org/capec#targetProtocolName"/>
                <owl:cardinality rdf:datatype="http://www.w3.org/2001/XMLSchema#nonNegativeInteger">1</owl:cardinality>
            </owl:Restriction>
        </rdfs:subClassOf>
        <rdfs:subClassOf>
            <owl:Restriction>
                <owl:onProperty rdf:resource="http://capec.mitre.org/capec#rfc"/>
                <owl:maxCardinality rdf:datatype="http://www.w3.org/2001/XMLSchema#nonNegativeInteger">1</owl:maxCardinality>
            </owl:Restriction>
        </rdfs:subClassOf>
        <rdfs:comment>Characterizes a Protocol</rdfs:comment>
        <rdfs:isDefinedBy rdf:resource="http://capec.mitre.org/capec"/>
        <rdfs:label>Protocol</rdfs:label>
    </owl:Class>
    


    <!-- http://capec.mitre.org/capec#TechnicalImpact -->

    <owl:Class rdf:about="http://capec.mitre.org/capec#TechnicalImpact">
        <rdfs:subClassOf>
            <owl:Restriction>
                <owl:onProperty rdf:resource="http://capec.mitre.org/capec#impactType"/>
                <owl:cardinality rdf:datatype="http://www.w3.org/2001/XMLSchema#nonNegativeInteger">1</owl:cardinality>
            </owl:Restriction>
        </rdfs:subClassOf>
        <rdfs:subClassOf>
            <owl:Restriction>
                <owl:onProperty rdf:resource="http://capec.mitre.org/capec#impactDescription"/>
                <owl:maxCardinality rdf:datatype="http://www.w3.org/2001/XMLSchema#nonNegativeInteger">1</owl:maxCardinality>
            </owl:Restriction>
        </rdfs:subClassOf>
        <rdfs:subClassOf>
            <owl:Restriction>
                <owl:onProperty rdf:resource="http://capec.mitre.org/capec#impactLikelihood"/>
                <owl:maxCardinality rdf:datatype="http://www.w3.org/2001/XMLSchema#nonNegativeInteger">1</owl:maxCardinality>
            </owl:Restriction>
        </rdfs:subClassOf>
        <rdfs:comment>Characterizes a technical impact that can result from successful execution of this attack pattern</rdfs:comment>
        <rdfs:isDefinedBy rdf:resource="http://capec.mitre.org/capec"/>
        <rdfs:label>Technical Impact</rdfs:label>
    </owl:Class>
    


    <!-- http://capec.mitre.org/capec#Term -->

    <owl:Class rdf:about="http://capec.mitre.org/capec#Term">
        <rdfs:subClassOf>
            <owl:Restriction>
                <owl:onProperty rdf:resource="http://capec.mitre.org/capec#term"/>
                <owl:cardinality rdf:datatype="http://www.w3.org/2001/XMLSchema#nonNegativeInteger">1</owl:cardinality>
            </owl:Restriction>
        </rdfs:subClassOf>
        <rdfs:subClassOf>
            <owl:Restriction>
                <owl:onProperty rdf:resource="http://capec.mitre.org/capec#extendedDescription"/>
                <owl:maxCardinality rdf:datatype="http://www.w3.org/2001/XMLSchema#nonNegativeInteger">1</owl:maxCardinality>
            </owl:Restriction>
        </rdfs:subClassOf>
        <rdfs:comment>Characterizes a term by which an attack pattern may be known and a description to explain the context in which the term may be relevant. This is not required for all entries and should only be included where appropriate.</rdfs:comment>
        <rdfs:isDefinedBy rdf:resource="http://capec.mitre.org/capec"/>
        <rdfs:label>Term</rdfs:label>
    </owl:Class>
    


    <!-- http://capec.mitre.org/capec#View -->

    <owl:Class rdf:about="http://capec.mitre.org/capec#View">
        <rdfs:subClassOf>
            <owl:Restriction>
                <owl:onProperty rdf:resource="http://capec.mitre.org/capec#id"/>
                <owl:cardinality rdf:datatype="http://www.w3.org/2001/XMLSchema#nonNegativeInteger">1</owl:cardinality>
            </owl:Restriction>
        </rdfs:subClassOf>
        <rdfs:subClassOf>
            <owl:Restriction>
                <owl:onProperty rdf:resource="http://capec.mitre.org/capec#status"/>
                <owl:cardinality rdf:datatype="http://www.w3.org/2001/XMLSchema#nonNegativeInteger">1</owl:cardinality>
            </owl:Restriction>
        </rdfs:subClassOf>
        <rdfs:subClassOf>
            <owl:Restriction>
                <owl:onProperty rdf:resource="http://capec.mitre.org/capec#structureType"/>
                <owl:cardinality rdf:datatype="http://www.w3.org/2001/XMLSchema#nonNegativeInteger">1</owl:cardinality>
            </owl:Restriction>
        </rdfs:subClassOf>
        <rdfs:subClassOf>
            <owl:Restriction>
                <owl:onProperty rdf:resource="http://capec.mitre.org/capec#viewName"/>
                <owl:cardinality rdf:datatype="http://www.w3.org/2001/XMLSchema#nonNegativeInteger">1</owl:cardinality>
            </owl:Restriction>
        </rdfs:subClassOf>
        <rdfs:subClassOf>
            <owl:Restriction>
                <owl:onProperty rdf:resource="http://capec.mitre.org/capec#viewFilter"/>
                <owl:maxCardinality rdf:datatype="http://www.w3.org/2001/XMLSchema#nonNegativeInteger">1</owl:maxCardinality>
            </owl:Restriction>
        </rdfs:subClassOf>
        <rdfs:subClassOf>
            <owl:Restriction>
                <owl:onProperty rdf:resource="http://capec.mitre.org/capec#viewObjective"/>
                <owl:maxCardinality rdf:datatype="http://www.w3.org/2001/XMLSchema#nonNegativeInteger">1</owl:maxCardinality>
            </owl:Restriction>
        </rdfs:subClassOf>
        <rdfs:comment>Represents a perspective with which one might look at the attack patterns in CAPEC</rdfs:comment>
        <rdfs:isDefinedBy rdf:resource="http://capec.mitre.org/capec"/>
        <rdfs:label>View</rdfs:label>
    </owl:Class>
    
    


    <!-- 
    ///////////////////////////////////////////////////////////////////////////////////////
    //
    // Annotations
    //
    ///////////////////////////////////////////////////////////////////////////////////////
     -->

    <rdf:Description rdf:about="http://capec.mitre.org/capec#structuredText">
        <rdfs:comment>Specifies that the text description is formatted utilizing some encoding scheme.</rdfs:comment>
        <rdfs:isDefinedBy rdf:resource="http://capec.mitre.org/capec"/>
        <rdfs:label>Structured Text</rdfs:label>
    </rdf:Description>
</rdf:RDF>



<!-- Generated by the OWL API (version 4.2.6.20160910-2108) https://github.com/owlcs/owlapi -->

