<?xml version="1.0"?>
<rdf:RDF xmlns="http://cce.mitre.org/cce#"
     xml:base="http://cce.mitre.org/cce"
     xmlns:cce="http://cce.mitre.org/cce#"
     xmlns:rdf="http://www.w3.org/1999/02/22-rdf-syntax-ns#"
     xmlns:owl="http://www.w3.org/2002/07/owl#"
     xmlns:xml="http://www.w3.org/XML/1998/namespace"
     xmlns:xsd="http://www.w3.org/2001/XMLSchema#"
     xmlns:rdfs="http://www.w3.org/2000/01/rdf-schema#">
    <owl:Ontology rdf:about="http://cce.mitre.org/cce">
        <owl:imports rdf:resource="http://cpe.mitre.org/cpe"/>
        <owl:imports rdf:resource="http://scap.nist.gov/scap_core"/>
        <rdfs:comment>This ontology provides a vocabulary and representation for the Common Configuration Enumeration (CCE) which provides unique identifiers to system configuration issues in order to facility fast and accurate correlation of configuration data across multiple information sources and tools.  This ontology is compatible with the version 5 format of the Common Configuration Enumeration XML schema.

Copyright (c) 2014, DaedaFusion, LLC.  All rights reserved.</rdfs:comment>
        <owl:versionInfo rdf:datatype="http://www.w3.org/2001/XMLSchema#string">v1.0.0-001</owl:versionInfo>
        <rdfs:label>Common Configuration Enumeration (CCE) Ontology</rdfs:label>
    </owl:Ontology>
    


    <!-- 
    ///////////////////////////////////////////////////////////////////////////////////////
    //
    // Annotation properties
    //
    ///////////////////////////////////////////////////////////////////////////////////////
     -->

    


    <!-- http://www.w3.org/2002/07/owl#maxCardinality -->

    <owl:AnnotationProperty rdf:about="http://www.w3.org/2002/07/owl#maxCardinality"/>
    


    <!-- 
    ///////////////////////////////////////////////////////////////////////////////////////
    //
    // Datatypes
    //
    ///////////////////////////////////////////////////////////////////////////////////////
     -->

    


    <!-- http://www.w3.org/2001/XMLSchema#date -->

    <rdfs:Datatype rdf:about="http://www.w3.org/2001/XMLSchema#date"/>
    


    <!-- 
    ///////////////////////////////////////////////////////////////////////////////////////
    //
    // Object Properties
    //
    ///////////////////////////////////////////////////////////////////////////////////////
     -->

    


    <!-- http://cce.mitre.org/cce#configurationIssues -->

    <owl:ObjectProperty rdf:about="http://cce.mitre.org/cce#configurationIssues">
        <rdfs:domain rdf:resource="http://cce.mitre.org/cce#ConfigurationIssueCatalog"/>
        <rdfs:range rdf:resource="http://cce.mitre.org/cce#CCE"/>
        <rdfs:comment>Specifies the CCE Name entries contained within the Configuration Issue Catalog.</rdfs:comment>
        <rdfs:isDefinedBy rdf:resource="http://cce.mitre.org/cce"/>
        <rdfs:label>Configuration Issues</rdfs:label>
    </owl:ObjectProperty>
    


    <!-- http://cce.mitre.org/cce#creator -->

    <owl:ObjectProperty rdf:about="http://cce.mitre.org/cce#creator">
        <rdfs:domain rdf:resource="http://cce.mitre.org/cce#CceResource"/>
        <rdfs:comment>Specifies the creator of the resource document</rdfs:comment>
        <rdfs:label>Creator</rdfs:label>
    </owl:ObjectProperty>
    


    <!-- http://cce.mitre.org/cce#platform -->

    <owl:ObjectProperty rdf:about="http://cce.mitre.org/cce#platform">
        <rdfs:domain rdf:resource="http://cce.mitre.org/cce#CCE"/>
        <rdfs:range rdf:resource="http://cpe.mitre.org/cpe#CPE"/>
        <rdfs:comment>Specifies the platform associated with this configuration control</rdfs:comment>
        <rdfs:label>Platform</rdfs:label>
    </owl:ObjectProperty>
    


    <!-- http://cce.mitre.org/cce#publisher -->

    <owl:ObjectProperty rdf:about="http://cce.mitre.org/cce#publisher">
        <rdfs:domain rdf:resource="http://cce.mitre.org/cce#CceResource"/>
        <rdfs:comment>Specifies the publisher of the resource, typically an organization</rdfs:comment>
        <rdfs:label>Publisher</rdfs:label>
    </owl:ObjectProperty>
    


    <!-- http://cce.mitre.org/cce#references -->

    <owl:ObjectProperty rdf:about="http://cce.mitre.org/cce#references">
        <rdfs:domain rdf:resource="http://cce.mitre.org/cce#CCE"/>
        <rdfs:range rdf:resource="http://cce.mitre.org/cce#CceReference"/>
        <rdfs:comment>Specifies a set of references from published configuration guidance documents such as the NSA Security Guides, the Center for Internet Security Benchmarks, and the DISA STIGs. Authoritative vendor documentation such as Microsoftâ€™s Security Compliance Manager represents acceptable reference material as well.</rdfs:comment>
        <rdfs:label>Resource References</rdfs:label>
    </owl:ObjectProperty>
    


    <!-- http://cce.mitre.org/cce#resource -->

    <owl:ObjectProperty rdf:about="http://cce.mitre.org/cce#resource">
        <rdfs:domain rdf:resource="http://cce.mitre.org/cce#CceReference"/>
        <rdfs:range rdf:resource="http://cce.mitre.org/cce#CceResource"/>
        <rdfs:comment>Specifies the Resource assoicated with the reference</rdfs:comment>
        <rdfs:label>Resource</rdfs:label>
    </owl:ObjectProperty>
    


    <!-- http://cce.mitre.org/cce#resources -->

    <owl:ObjectProperty rdf:about="http://cce.mitre.org/cce#resources">
        <rdfs:domain rdf:resource="http://cce.mitre.org/cce#ConfigurationIssueCatalog"/>
        <rdfs:range rdf:resource="http://cce.mitre.org/cce#CceResource"/>
        <rdfs:comment>Specifies the Configuration Issue Resources contained within the Configuration Issue Catalog.</rdfs:comment>
        <rdfs:isDefinedBy rdf:resource="http://cce.mitre.org/cce"/>
        <rdfs:label>Resources</rdfs:label>
    </owl:ObjectProperty>
    


    <!-- 
    ///////////////////////////////////////////////////////////////////////////////////////
    //
    // Data properties
    //
    ///////////////////////////////////////////////////////////////////////////////////////
     -->

    


    <!-- http://cce.mitre.org/cce#cceId -->

    <owl:DatatypeProperty rdf:about="http://cce.mitre.org/cce#cceId">
        <rdfs:domain rdf:resource="http://cce.mitre.org/cce#CCE"/>
        <rdfs:range rdf:resource="http://www.w3.org/2001/XMLSchema#string"/>
        <rdfs:comment>Specifies pseudorandom identifier tag assigned to the CCE entry</rdfs:comment>
        <rdfs:label>CCE Identifier</rdfs:label>
    </owl:DatatypeProperty>
    


    <!-- http://cce.mitre.org/cce#cceResourceId -->

    <owl:DatatypeProperty rdf:about="http://cce.mitre.org/cce#cceResourceId">
        <rdfs:domain rdf:resource="http://cce.mitre.org/cce#CceResource"/>
        <rdfs:range rdf:resource="http://www.w3.org/2001/XMLSchema#string"/>
        <rdfs:comment>Specifies the identifier for the Common Configuration Enumeration resource</rdfs:comment>
        <rdfs:label>Resource Identifier</rdfs:label>
    </owl:DatatypeProperty>
    


    <!-- http://cce.mitre.org/cce#creatorName -->

    <owl:DatatypeProperty rdf:about="http://cce.mitre.org/cce#creatorName">
        <rdfs:domain rdf:resource="http://cce.mitre.org/cce#CceResource"/>
        <rdfs:range rdf:resource="http://www.w3.org/2001/XMLSchema#string"/>
        <rdfs:comment>Specifies the name of the creator(s) of the resource document</rdfs:comment>
        <rdfs:isDefinedBy rdf:resource="http://cce.mitre.org/cce"/>
        <rdfs:label>Creator Name</rdfs:label>
    </owl:DatatypeProperty>
    


    <!-- http://cce.mitre.org/cce#deprecated -->

    <owl:DatatypeProperty rdf:about="http://cce.mitre.org/cce#deprecated">
        <rdfs:domain rdf:resource="http://cce.mitre.org/cce#CCE"/>
        <rdfs:range rdf:resource="http://www.w3.org/2001/XMLSchema#boolean"/>
        <rdfs:comment>Specifies whether the CCE entry is depreciated</rdfs:comment>
        <rdfs:label>Deprecated</rdfs:label>
    </owl:DatatypeProperty>
    


    <!-- http://cce.mitre.org/cce#description -->

    <owl:DatatypeProperty rdf:about="http://cce.mitre.org/cce#description">
        <rdfs:domain rdf:resource="http://cce.mitre.org/cce#CCE"/>
        <rdfs:range rdf:resource="http://www.w3.org/2001/XMLSchema#string"/>
        <rdfs:comment>Specifies a humanly understandable description of the configuration control. This description describes the control and allows an analyst to quickly and accurately recognize an entry.</rdfs:comment>
        <rdfs:label>Description</rdfs:label>
    </owl:DatatypeProperty>
    


    <!-- http://cce.mitre.org/cce#format -->

    <owl:DatatypeProperty rdf:about="http://cce.mitre.org/cce#format">
        <rdfs:domain rdf:resource="http://cce.mitre.org/cce#CceResource"/>
        <rdfs:range rdf:resource="http://www.w3.org/2001/XMLSchema#string"/>
        <rdfs:comment>Specifies the format of the resource</rdfs:comment>
        <rdfs:label>Format</rdfs:label>
    </owl:DatatypeProperty>
    


    <!-- http://cce.mitre.org/cce#issuedDate -->

    <owl:DatatypeProperty rdf:about="http://cce.mitre.org/cce#issuedDate">
        <rdfs:domain rdf:resource="http://cce.mitre.org/cce#CceResource"/>
        <rdfs:range rdf:resource="http://www.w3.org/2001/XMLSchema#date"/>
        <rdfs:comment>Specifies the date of formal issuance (e.g., publication) of the resource.</rdfs:comment>
        <rdfs:label>Issued</rdfs:label>
    </owl:DatatypeProperty>
    


    <!-- http://cce.mitre.org/cce#lastModifiedDate -->

    <owl:DatatypeProperty rdf:about="http://cce.mitre.org/cce#lastModifiedDate">
        <rdfs:domain rdf:resource="http://cce.mitre.org/cce#CCE"/>
        <rdfs:domain rdf:resource="http://cce.mitre.org/cce#CceReference"/>
        <rdfs:range rdf:resource="http://www.w3.org/2001/XMLSchema#date"/>
        <rdfs:comment>Specifies the date the configuration control was last modified</rdfs:comment>
        <rdfs:label>Last Modified</rdfs:label>
    </owl:DatatypeProperty>
    


    <!-- http://cce.mitre.org/cce#notes -->

    <owl:DatatypeProperty rdf:about="http://cce.mitre.org/cce#notes">
        <rdfs:domain rdf:resource="http://cce.mitre.org/cce#CceResource"/>
        <rdfs:range rdf:resource="http://www.w3.org/2001/XMLSchema#string"/>
        <rdfs:comment>Specifies a note associated with the resource</rdfs:comment>
        <rdfs:label>Notes</rdfs:label>
    </owl:DatatypeProperty>
    


    <!-- http://cce.mitre.org/cce#parameters -->

    <owl:DatatypeProperty rdf:about="http://cce.mitre.org/cce#parameters">
        <rdfs:domain rdf:resource="http://cce.mitre.org/cce#CCE"/>
        <rdfs:range rdf:resource="http://www.w3.org/2001/XMLSchema#string"/>
        <rdfs:comment>Specifies parameters that would need to be specified in order to implement a CCE on a system.</rdfs:comment>
        <rdfs:label>Parameters</rdfs:label>
    </owl:DatatypeProperty>
    


    <!-- http://cce.mitre.org/cce#publisherName -->

    <owl:DatatypeProperty rdf:about="http://cce.mitre.org/cce#publisherName">
        <rdfs:domain rdf:resource="http://cce.mitre.org/cce#CceResource"/>
        <rdfs:range rdf:resource="http://www.w3.org/2001/XMLSchema#string"/>
        <rdfs:comment>Specifies the name of the publisher of the resource, typically an organization</rdfs:comment>
        <rdfs:isDefinedBy rdf:resource="http://cce.mitre.org/cce"/>
        <rdfs:label>Publisher Name</rdfs:label>
    </owl:DatatypeProperty>
    


    <!-- http://cce.mitre.org/cce#resourceId -->

    <owl:DatatypeProperty rdf:about="http://cce.mitre.org/cce#resourceId">
        <rdfs:domain rdf:resource="http://cce.mitre.org/cce#CceReference"/>
        <rdfs:range rdf:resource="http://www.w3.org/2001/XMLSchema#string"/>
        <rdfs:comment>Specifies the identifier of the resource</rdfs:comment>
        <rdfs:isDefinedBy rdf:resource="http://cce.mitre.org/cce"/>
        <rdfs:label>Resource Id</rdfs:label>
    </owl:DatatypeProperty>
    


    <!-- http://cce.mitre.org/cce#section -->

    <owl:DatatypeProperty rdf:about="http://cce.mitre.org/cce#section">
        <rdfs:domain rdf:resource="http://cce.mitre.org/cce#CceReference"/>
        <rdfs:range rdf:resource="http://www.w3.org/2001/XMLSchema#string"/>
        <rdfs:comment>Specifies a specific section contained within the resource referenced that is applicable to this configuration control</rdfs:comment>
        <rdfs:label>Section</rdfs:label>
    </owl:DatatypeProperty>
    


    <!-- http://cce.mitre.org/cce#technicalMechanism -->

    <owl:DatatypeProperty rdf:about="http://cce.mitre.org/cce#technicalMechanism">
        <rdfs:domain rdf:resource="http://cce.mitre.org/cce#CCE"/>
        <rdfs:range rdf:resource="http://www.w3.org/2001/XMLSchema#string"/>
        <rdfs:comment>Specifies for any given configuration issue there may be one or more ways to implement the desired result.</rdfs:comment>
        <rdfs:label>Technical Mechanisms</rdfs:label>
    </owl:DatatypeProperty>
    


    <!-- http://cce.mitre.org/cce#title -->

    <owl:DatatypeProperty rdf:about="http://cce.mitre.org/cce#title">
        <rdfs:domain rdf:resource="http://cce.mitre.org/cce#CceResource"/>
        <rdfs:range rdf:resource="http://www.w3.org/2001/XMLSchema#string"/>
        <rdfs:comment>Specifies the title of the resource document</rdfs:comment>
        <rdfs:label>Title</rdfs:label>
    </owl:DatatypeProperty>
    


    <!-- http://cce.mitre.org/cce#version -->

    <owl:DatatypeProperty rdf:about="http://cce.mitre.org/cce#version">
        <rdfs:domain rdf:resource="http://cce.mitre.org/cce#CceResource"/>
        <rdfs:range rdf:resource="http://www.w3.org/2001/XMLSchema#string"/>
        <rdfs:comment>Specifies the version of the resource</rdfs:comment>
        <rdfs:label>Version</rdfs:label>
    </owl:DatatypeProperty>
    


    <!-- 
    ///////////////////////////////////////////////////////////////////////////////////////
    //
    // Classes
    //
    ///////////////////////////////////////////////////////////////////////////////////////
     -->

    


    <!-- http://cce.mitre.org/cce#CCE -->

    <owl:Class rdf:about="http://cce.mitre.org/cce#CCE">
        <rdfs:subClassOf>
            <owl:Restriction>
                <owl:onProperty rdf:resource="http://cce.mitre.org/cce#platform"/>
                <owl:cardinality rdf:datatype="http://www.w3.org/2001/XMLSchema#nonNegativeInteger">1</owl:cardinality>
            </owl:Restriction>
        </rdfs:subClassOf>
        <rdfs:subClassOf>
            <owl:Restriction>
                <owl:onProperty rdf:resource="http://cce.mitre.org/cce#cceId"/>
                <owl:cardinality rdf:datatype="http://www.w3.org/2001/XMLSchema#nonNegativeInteger">1</owl:cardinality>
            </owl:Restriction>
        </rdfs:subClassOf>
        <rdfs:subClassOf>
            <owl:Restriction>
                <owl:onProperty rdf:resource="http://cce.mitre.org/cce#description"/>
                <owl:cardinality rdf:datatype="http://www.w3.org/2001/XMLSchema#nonNegativeInteger">1</owl:cardinality>
            </owl:Restriction>
        </rdfs:subClassOf>
        <rdfs:subClassOf>
            <owl:Restriction>
                <owl:onProperty rdf:resource="http://cce.mitre.org/cce#lastModifiedDate"/>
                <owl:cardinality rdf:datatype="http://www.w3.org/2001/XMLSchema#nonNegativeInteger">1</owl:cardinality>
            </owl:Restriction>
        </rdfs:subClassOf>
        <rdfs:subClassOf>
            <owl:Restriction>
                <owl:onProperty rdf:resource="http://cce.mitre.org/cce#deprecated"/>
                <owl:maxCardinality rdf:datatype="http://www.w3.org/2001/XMLSchema#nonNegativeInteger">1</owl:maxCardinality>
            </owl:Restriction>
        </rdfs:subClassOf>
        <rdfs:comment>Represents a Common Configuration Enumeration (CCE) Entry</rdfs:comment>
        <rdfs:isDefinedBy rdf:resource="http://cce.mitre.org/cce"/>
        <rdfs:label>CCE</rdfs:label>
    </owl:Class>
    


    <!-- http://cce.mitre.org/cce#CceReference -->

    <owl:Class rdf:about="http://cce.mitre.org/cce#CceReference">
        <rdfs:subClassOf>
            <owl:Restriction>
                <owl:onProperty rdf:resource="http://cce.mitre.org/cce#resource"/>
                <owl:cardinality rdf:datatype="http://www.w3.org/2001/XMLSchema#nonNegativeInteger">1</owl:cardinality>
            </owl:Restriction>
        </rdfs:subClassOf>
        <rdfs:subClassOf>
            <owl:Restriction>
                <owl:onProperty rdf:resource="http://cce.mitre.org/cce#resourceId"/>
                <owl:cardinality rdf:datatype="http://www.w3.org/2001/XMLSchema#nonNegativeInteger">1</owl:cardinality>
            </owl:Restriction>
        </rdfs:subClassOf>
        <rdfs:subClassOf>
            <owl:Restriction>
                <owl:onProperty rdf:resource="http://cce.mitre.org/cce#section"/>
                <owl:cardinality rdf:datatype="http://www.w3.org/2001/XMLSchema#nonNegativeInteger">1</owl:cardinality>
            </owl:Restriction>
        </rdfs:subClassOf>
        <rdfs:subClassOf>
            <owl:Restriction>
                <owl:onProperty rdf:resource="http://cce.mitre.org/cce#lastModifiedDate"/>
                <owl:maxCardinality rdf:datatype="http://www.w3.org/2001/XMLSchema#nonNegativeInteger">1</owl:maxCardinality>
            </owl:Restriction>
        </rdfs:subClassOf>
        <rdfs:comment>Represents a reference for the Configuration Control</rdfs:comment>
        <rdfs:isDefinedBy rdf:resource="http://cce.mitre.org/cce"/>
        <rdfs:label>CCE Reference</rdfs:label>
    </owl:Class>
    


    <!-- http://cce.mitre.org/cce#CceResource -->

    <owl:Class rdf:about="http://cce.mitre.org/cce#CceResource">
        <rdfs:subClassOf>
            <owl:Restriction>
                <owl:onProperty rdf:resource="http://cce.mitre.org/cce#publisher"/>
                <owl:maxCardinality rdf:datatype="http://www.w3.org/2001/XMLSchema#nonNegativeInteger">1</owl:maxCardinality>
            </owl:Restriction>
        </rdfs:subClassOf>
        <rdfs:subClassOf>
            <owl:Restriction>
                <owl:onProperty rdf:resource="http://cce.mitre.org/cce#cceResourceId"/>
                <owl:cardinality rdf:datatype="http://www.w3.org/2001/XMLSchema#nonNegativeInteger">1</owl:cardinality>
            </owl:Restriction>
        </rdfs:subClassOf>
        <rdfs:subClassOf>
            <owl:Restriction>
                <owl:onProperty rdf:resource="http://cce.mitre.org/cce#lastModifiedDate"/>
                <owl:cardinality rdf:datatype="http://www.w3.org/2001/XMLSchema#nonNegativeInteger">1</owl:cardinality>
            </owl:Restriction>
        </rdfs:subClassOf>
        <rdfs:subClassOf>
            <owl:Restriction>
                <owl:onProperty rdf:resource="http://cce.mitre.org/cce#title"/>
                <owl:cardinality rdf:datatype="http://www.w3.org/2001/XMLSchema#nonNegativeInteger">1</owl:cardinality>
            </owl:Restriction>
        </rdfs:subClassOf>
        <rdfs:subClassOf>
            <owl:Restriction>
                <owl:onProperty rdf:resource="http://cce.mitre.org/cce#format"/>
                <owl:maxCardinality rdf:datatype="http://www.w3.org/2001/XMLSchema#nonNegativeInteger">1</owl:maxCardinality>
            </owl:Restriction>
        </rdfs:subClassOf>
        <rdfs:subClassOf>
            <owl:Restriction>
                <owl:onProperty rdf:resource="http://cce.mitre.org/cce#issuedDate"/>
                <owl:maxCardinality rdf:datatype="http://www.w3.org/2001/XMLSchema#nonNegativeInteger">1</owl:maxCardinality>
            </owl:Restriction>
        </rdfs:subClassOf>
        <rdfs:subClassOf>
            <owl:Restriction>
                <owl:onProperty rdf:resource="http://cce.mitre.org/cce#notes"/>
                <owl:maxCardinality rdf:datatype="http://www.w3.org/2001/XMLSchema#nonNegativeInteger">1</owl:maxCardinality>
            </owl:Restriction>
        </rdfs:subClassOf>
        <rdfs:subClassOf>
            <owl:Restriction>
                <owl:onProperty rdf:resource="http://cce.mitre.org/cce#publisherName"/>
                <owl:maxCardinality rdf:datatype="http://www.w3.org/2001/XMLSchema#nonNegativeInteger">1</owl:maxCardinality>
            </owl:Restriction>
        </rdfs:subClassOf>
        <rdfs:subClassOf>
            <owl:Restriction>
                <owl:onProperty rdf:resource="http://cce.mitre.org/cce#version"/>
                <owl:maxCardinality rdf:datatype="http://www.w3.org/2001/XMLSchema#nonNegativeInteger">1</owl:maxCardinality>
            </owl:Restriction>
        </rdfs:subClassOf>
        <rdfs:comment>Represents a published authoritative resource providing configuration guidance.  Such documents include the NSA Security Guides, the Center for Internet Security Benchmarks, and the DISA STIGs.  Authoritative vendor documentation such as Microsoftâ€™s Security Compliance Manager represents acceptable reference material as well.</rdfs:comment>
        <rdfs:isDefinedBy rdf:resource="http://cce.mitre.org/cce"/>
        <rdfs:label>Resource</rdfs:label>
    </owl:Class>
    


    <!-- http://cce.mitre.org/cce#ConfigurationIssueCatalog -->

    <owl:Class rdf:about="http://cce.mitre.org/cce#ConfigurationIssueCatalog">
        <rdfs:subClassOf rdf:resource="http://scap.nist.gov/scap_core#Catalog"/>
        <rdfs:comment>Characterizes a catalog of Configuration Issues</rdfs:comment>
        <rdfs:isDefinedBy rdf:resource="http://cce.mitre.org/cce"/>
        <rdfs:label>Configuration Issue Catalog</rdfs:label>
    </owl:Class>
    


   
</rdf:RDF>



<!-- Generated by the OWL API (version 4.2.6.20160910-2108) https://github.com/owlcs/owlapi -->

