<?xml version="1.0"?>
<rdf:RDF xmlns="http://maec.mitre.org/maec_bundle#"
     xml:base="http://maec.mitre.org/maec_bundle"
     xmlns:maecBundle="http://maec.mitre.org/maec_bundle#"
     xmlns:owl="http://www.w3.org/2002/07/owl#"
     xmlns:xsd="http://www.w3.org/2001/XMLSchema#"
     xmlns:rdfs="http://www.w3.org/2000/01/rdf-schema#"
     xmlns:cyboxCommon="http://cybox.mitre.org/cyboxCommon#"
     xmlns:maec_common="http://maec.mitre.org/maec_common#"
     xmlns:maecPackage="http://maec.mitre.org/maec_package#"
     xmlns:rdf="http://www.w3.org/1999/02/22-rdf-syntax-ns#"
     xmlns:xml="http://www.w3.org/XML/1998/namespace"
     xmlns:mmdef="http://xml/metadatasharing#"
     xmlns:wgs84_pos="http://www.w3.org/2003/01/geo/wgs84_pos#"
     xmlns:cybox_core="http://cybox.mitre.org/cybox_core#"
     xmlns:foaf="http://xmlns.com/foaf/0.1/"
     xmlns:dc="http://purl.org/dc/elements/1.1/">
    <owl:Ontology rdf:about="http://maec.mitre.org/maec_bundle">
        <owl:imports rdf:resource="http://cybox.mitre.org/objects/Code"/>
        <owl:imports rdf:resource="http://cybox.mitre.org/objects/Process"/>
        <owl:imports rdf:resource="http://cybox.mitre.org/objects/API"/>
        <owl:imports rdf:resource="http://cybox.mitre.org/objects/NetworkProtocol"/>
        <owl:imports rdf:resource="http://cybox.mitre.org/objects/DNS"/>
        <owl:imports rdf:resource="http://maec.mitre.org/maec_common"/>
        <owl:imports rdf:resource="http://nvd.nist.gov/cve"/>
        <owl:imports rdf:resource="http://cybox.mitre.org/objects/Socket_Address"/>
        <rdfs:comment>This ontology provides a vocabulary and representation for the  Malware Attribute Enumeration and Characterization (MAEC)  Bundle  types.  

MAEC provides a common mechansim (structure and content) for encoding and communicating high-fidelity information about malware based upon attributes such as behaviors, artifacts, and attack patterns.  The Bundle ontology provides the ability to capture and share data obtained from the analysis of a simple malware instance.  Its underlying structure is formed by Actions, Behaviors, and Capabilities.

The ontology is based on the MAEC Bundle schema maintained by The MITRE Corporation copyright 2012-2014.  The version number of the ontology is kept in sync with the schema in order to more easily relate between the ontology and the corresponding schema version.

Copyright (c) 2014, DaedaFusion, LLC.  All rights reserved.</rdfs:comment>
        <owl:versionInfo rdf:datatype="http://www.w3.org/2001/XMLSchema#string">2.1.0-000</owl:versionInfo>
        <rdfs:label>Malware Attribute Enumeration and Characterization (MAEC)  Bundle Ontology</rdfs:label>
    </owl:Ontology>
    


    <!-- 
    ///////////////////////////////////////////////////////////////////////////////////////
    //
    // Annotation properties
    //
    ///////////////////////////////////////////////////////////////////////////////////////
     -->

    


    <!-- http://cybox.mitre.org/cybox_core#discoveryMethod -->

    <owl:AnnotationProperty rdf:about="http://cybox.mitre.org/cybox_core#discoveryMethod"/>
    


    <!-- http://maec.mitre.org/maec_common#author -->

    <owl:AnnotationProperty rdf:about="http://maec.mitre.org/maec_common#author"/>
    


    <!-- http://maec.mitre.org/maec_common#authorName -->

    <owl:AnnotationProperty rdf:about="http://maec.mitre.org/maec_common#authorName"/>
    


    <!-- http://maec.mitre.org/maec_common#creationDateTime -->

    <owl:AnnotationProperty rdf:about="http://maec.mitre.org/maec_common#creationDateTime"/>
    


    <!-- http://maec.mitre.org/maec_common#importance -->

    <owl:AnnotationProperty rdf:about="http://maec.mitre.org/maec_common#importance"/>
    


    <!-- http://maec.mitre.org/maec_common#lastUpdate -->

    <owl:AnnotationProperty rdf:about="http://maec.mitre.org/maec_common#lastUpdate"/>
    


    <!-- http://maec.mitre.org/maec_common#malwareInstanceObject -->

    <owl:AnnotationProperty rdf:about="http://maec.mitre.org/maec_common#malwareInstanceObject"/>
    


    <!-- http://maec.mitre.org/maec_common#version -->

    <owl:AnnotationProperty rdf:about="http://maec.mitre.org/maec_common#version"/>
    


    <!-- http://www.w3.org/2002/07/owl#cardinality -->

    <owl:AnnotationProperty rdf:about="http://www.w3.org/2002/07/owl#cardinality"/>
    


    <!-- http://www.w3.org/2002/07/owl#maxCardinality -->

    <owl:AnnotationProperty rdf:about="http://www.w3.org/2002/07/owl#maxCardinality"/>
    


    <!-- 
    ///////////////////////////////////////////////////////////////////////////////////////
    //
    // Datatypes
    //
    ///////////////////////////////////////////////////////////////////////////////////////
     -->

    


    <!-- http://www.w3.org/2001/XMLSchema#duration -->

    <rdfs:Datatype rdf:about="http://www.w3.org/2001/XMLSchema#duration"/>
    


    <!-- 
    ///////////////////////////////////////////////////////////////////////////////////////
    //
    // Object Properties
    //
    ///////////////////////////////////////////////////////////////////////////////////////
     -->

    


    <!-- http://maec.mitre.org/maec_bundle#actionComposition -->

    <owl:ObjectProperty rdf:about="http://maec.mitre.org/maec_bundle#actionComposition">
        <rdfs:range>
            <owl:Class>
                <owl:unionOf rdf:parseType="Collection">
                    <rdf:Description rdf:about="http://maec.mitre.org/maec_bundle#ActionCollection"/>
                    <rdf:Description rdf:about="http://maec.mitre.org/maec_bundle#BehavioralAction"/>
                    <rdf:Description rdf:about="http://maec.mitre.org/maec_bundle#BehavioralActionEquivalence"/>
                </owl:unionOf>
            </owl:Class>
        </rdfs:range>
        <rdfs:comment>Specifies the Actions that compose the Behavior.</rdfs:comment>
        <rdfs:isDefinedBy rdf:resource="http://maec.mitre.org/maec_bundle"/>
        <rdfs:label>Action Composition</rdfs:label>
    </owl:ObjectProperty>
    


    <!-- http://maec.mitre.org/maec_bundle#actions -->

    <owl:ObjectProperty rdf:about="http://maec.mitre.org/maec_bundle#actions">
        <rdfs:range rdf:resource="http://maec.mitre.org/maec_common#MalwareAction"/>
        <rdfs:comment>Specifies the list of lower-level actions that were observed for the malware instance.</rdfs:comment>
        <rdfs:isDefinedBy rdf:resource="http://maec.mitre.org/maec_bundle"/>
        <rdfs:label>Actions</rdfs:label>
    </owl:ObjectProperty>
    


    <!-- http://maec.mitre.org/maec_bundle#associatedCode -->

    <owl:ObjectProperty rdf:about="http://maec.mitre.org/maec_bundle#associatedCode">
        <rdfs:range rdf:resource="http://cybox.mitre.org/objects/Code#Code"/>
        <rdfs:comment>Specifies any code snippets that may be associated with the Behavior.</rdfs:comment>
        <rdfs:isDefinedBy rdf:resource="http://maec.mitre.org/maec_bundle"/>
        <rdfs:label>associated code</rdfs:label>
    </owl:ObjectProperty>
    


    <!-- http://maec.mitre.org/maec_bundle#avClassifications -->

    <owl:ObjectProperty rdf:about="http://maec.mitre.org/maec_bundle#avClassifications">
        <rdfs:range rdf:resource="http://maec.mitre.org/maec_bundle#AVClassification"/>
        <rdfs:comment>Sspecifies any Anti-Virus scanner tool classifications of the malware instance object.</rdfs:comment>
        <rdfs:isDefinedBy rdf:resource="http://maec.mitre.org/maec_bundle"/>
        <rdfs:label>AV Classifications</rdfs:label>
    </owl:ObjectProperty>
    


    <!-- http://maec.mitre.org/maec_bundle#behaviorReference -->

    <owl:ObjectProperty rdf:about="http://maec.mitre.org/maec_bundle#behaviorReference">
        <rdfs:range rdf:resource="http://maec.mitre.org/maec_bundle#Behavior"/>
        <rdfs:comment>Specifies a reference to one or more Behavior in the relationship.</rdfs:comment>
        <rdfs:isDefinedBy rdf:resource="http://maec.mitre.org/maec_bundle"/>
        <rdfs:label>Behavior Reference</rdfs:label>
    </owl:ObjectProperty>
    


    <!-- http://maec.mitre.org/maec_bundle#behaviorRelationships -->

    <owl:ObjectProperty rdf:about="http://maec.mitre.org/maec_bundle#behaviorRelationships">
        <rdfs:range rdf:resource="http://maec.mitre.org/maec_bundle#Behavior"/>
        <rdfs:comment>Specifies any relationships between this Behavior and any other Behaviors.</rdfs:comment>
        <rdfs:isDefinedBy rdf:resource="http://maec.mitre.org/maec_bundle"/>
        <rdfs:label>Relationships</rdfs:label>
    </owl:ObjectProperty>
    


    <!-- http://maec.mitre.org/maec_bundle#behaviors -->

    <owl:ObjectProperty rdf:about="http://maec.mitre.org/maec_bundle#behaviors">
        <rdfs:range rdf:resource="http://maec.mitre.org/maec_bundle#Behavior"/>
        <rdfs:comment>Specifies the list of behaviors that were observed for the malware instance.</rdfs:comment>
        <rdfs:isDefinedBy rdf:resource="http://maec.mitre.org/maec_bundle"/>
        <rdfs:label>Behaviors</rdfs:label>
    </owl:ObjectProperty>
    


    <!-- http://maec.mitre.org/maec_bundle#candidateIndicators -->

    <owl:ObjectProperty rdf:about="http://maec.mitre.org/maec_bundle#candidateIndicators">
        <rdfs:range rdf:resource="http://maec.mitre.org/maec_bundle#CandidateIndicator"/>
        <rdfs:comment>Specifies the list of any candidate indicators associated with the malware instance.</rdfs:comment>
        <rdfs:isDefinedBy rdf:resource="http://maec.mitre.org/maec_bundle"/>
        <rdfs:label>Candidate Indicators</rdfs:label>
    </owl:ObjectProperty>
    


    <!-- http://maec.mitre.org/maec_bundle#capabilities -->

    <owl:ObjectProperty rdf:about="http://maec.mitre.org/maec_bundle#capabilities">
        <rdfs:range rdf:resource="http://maec.mitre.org/maec_bundle#Capability"/>
        <rdfs:comment>Specifies the high-level capabilities and objectives of the malware instance.</rdfs:comment>
        <rdfs:isDefinedBy rdf:resource="http://maec.mitre.org/maec_bundle"/>
        <rdfs:label>Capabilities</rdfs:label>
    </owl:ObjectProperty>
    


    <!-- http://maec.mitre.org/maec_bundle#capabilityObjectiveRelationships -->

    <owl:ObjectProperty rdf:about="http://maec.mitre.org/maec_bundle#capabilityObjectiveRelationships">
        <rdfs:range rdf:resource="http://maec.mitre.org/maec_bundle#CapabilityObjective"/>
        <rdfs:comment>Specifies a relationship from the Capability Objective to one or more other Capability Objectives.</rdfs:comment>
        <rdfs:isDefinedBy rdf:resource="http://maec.mitre.org/maec_bundle"/>
        <rdfs:label>Relationships</rdfs:label>
    </owl:ObjectProperty>
    


    <!-- http://maec.mitre.org/maec_bundle#capabilityProperty -->

    <owl:ObjectProperty rdf:about="http://maec.mitre.org/maec_bundle#capabilityProperty">
        <rdfs:range rdf:resource="http://maec.mitre.org/maec_bundle#CapabilityProperty"/>
        <rdfs:comment>Specifies one or more properties of the Capability, as a key/value pair.</rdfs:comment>
        <rdfs:isDefinedBy rdf:resource="http://maec.mitre.org/maec_bundle"/>
        <rdfs:label>Property</rdfs:label>
    </owl:ObjectProperty>
    


    <!-- http://maec.mitre.org/maec_bundle#capabilityReference -->

    <owl:ObjectProperty rdf:about="http://maec.mitre.org/maec_bundle#capabilityReference">
        <rdfs:range rdf:resource="http://maec.mitre.org/maec_bundle#Capability"/>
        <rdfs:comment>Specifies one or more Capabilities that are the target of this relationship</rdfs:comment>
        <rdfs:isDefinedBy rdf:resource="http://maec.mitre.org/maec_bundle"/>
        <rdfs:label>Reference</rdfs:label>
    </owl:ObjectProperty>
    


    <!-- http://maec.mitre.org/maec_bundle#capabilityRelationships -->

    <owl:ObjectProperty rdf:about="http://maec.mitre.org/maec_bundle#capabilityRelationships">
        <rdfs:range rdf:resource="http://maec.mitre.org/maec_bundle#Capability"/>
        <rdfs:comment>Specifies any relationships between this Capability and any other Capabilities.</rdfs:comment>
        <rdfs:isDefinedBy rdf:resource="http://maec.mitre.org/maec_bundle"/>
        <rdfs:label>Relationships</rdfs:label>
    </owl:ObjectProperty>
    


    <!-- http://maec.mitre.org/maec_bundle#collection.actions -->

    <owl:ObjectProperty rdf:about="http://maec.mitre.org/maec_bundle#collection.actions">
        <rdfs:range rdf:resource="http://maec.mitre.org/maec_bundle#ActionCollection"/>
        <rdfs:comment>Specifies any collections of Actions in the Bundle.</rdfs:comment>
        <rdfs:isDefinedBy rdf:resource="http://maec.mitre.org/maec_bundle"/>
        <rdfs:label>Actions Collection</rdfs:label>
    </owl:ObjectProperty>
    


    <!-- http://maec.mitre.org/maec_bundle#collection.behaviors -->

    <owl:ObjectProperty rdf:about="http://maec.mitre.org/maec_bundle#collection.behaviors">
        <rdfs:range rdf:resource="http://maec.mitre.org/maec_bundle#BehaviorCollection"/>
        <rdfs:comment>Specifies any collections of Behaviors in the Bundle.</rdfs:comment>
        <rdfs:isDefinedBy rdf:resource="http://maec.mitre.org/maec_bundle"/>
        <rdfs:label>Behaviors Collection</rdfs:label>
    </owl:ObjectProperty>
    


    <!-- http://maec.mitre.org/maec_bundle#collection.candidateIndicators -->

    <owl:ObjectProperty rdf:about="http://maec.mitre.org/maec_bundle#collection.candidateIndicators">
        <rdfs:range rdf:resource="http://maec.mitre.org/maec_bundle#CandidateIndicatorCollection"/>
        <rdfs:comment>Specifies any collections of Candidate Indicators in the Bundle.</rdfs:comment>
        <rdfs:isDefinedBy rdf:resource="http://maec.mitre.org/maec_bundle"/>
        <rdfs:label>Candidate Indicators Collection</rdfs:label>
    </owl:ObjectProperty>
    


    <!-- http://maec.mitre.org/maec_bundle#collection.objects -->

    <owl:ObjectProperty rdf:about="http://maec.mitre.org/maec_bundle#collection.objects">
        <rdfs:range rdf:resource="http://maec.mitre.org/maec_bundle#ObjectCollection"/>
        <rdfs:comment>Specifies any collections of CybOX Objects in the Bundle.</rdfs:comment>
        <rdfs:isDefinedBy rdf:resource="http://maec.mitre.org/maec_bundle"/>
        <rdfs:label>Objects Collection</rdfs:label>
    </owl:ObjectProperty>
    


    <!-- http://maec.mitre.org/maec_bundle#composition -->

    <owl:ObjectProperty rdf:about="http://maec.mitre.org/maec_bundle#composition">
        <rdfs:range rdf:resource="http://maec.mitre.org/maec_bundle#CandidateIndicatorComposition"/>
        <rdfs:comment>Specifies the actual observables that the Candidate Indicator is composed of, via a reference to a one or more entities contained in the Bundle.</rdfs:comment>
        <rdfs:isDefinedBy rdf:resource="http://maec.mitre.org/maec_bundle"/>
        <rdfs:label>Composition</rdfs:label>
    </owl:ObjectProperty>
    


    <!-- http://maec.mitre.org/maec_bundle#initiatedActions -->

    <owl:ObjectProperty rdf:about="http://maec.mitre.org/maec_bundle#initiatedActions">
        <rdfs:range rdf:resource="http://maec.mitre.org/maec_common#MalwareAction"/>
        <rdfs:comment>Specifies the actions (found inside the top-level Actions element, or an Action Collection inside the top-level Collections element) initiated by the Process.</rdfs:comment>
        <rdfs:isDefinedBy rdf:resource="http://maec.mitre.org/maec_bundle"/>
        <rdfs:label>Initiated Actions</rdfs:label>
    </owl:ObjectProperty>
    


    <!-- http://maec.mitre.org/maec_bundle#injectedProcess -->

    <owl:ObjectProperty rdf:about="http://maec.mitre.org/maec_bundle#injectedProcess">
        <rdfs:range rdf:resource="http://maec.mitre.org/maec_bundle#ProcessTreeNode"/>
        <rdfs:comment>Specifies one or more processes that was injected by this process.</rdfs:comment>
        <rdfs:isDefinedBy rdf:resource="http://maec.mitre.org/maec_bundle"/>
        <rdfs:label>Injected Process</rdfs:label>
    </owl:ObjectProperty>
    


    <!-- http://maec.mitre.org/maec_bundle#malwareEntity -->

    <owl:ObjectProperty rdf:about="http://maec.mitre.org/maec_bundle#malwareEntity">
        <rdfs:range rdf:resource="http://maec.mitre.org/maec_bundle#MalwareEntity"/>
        <rdfs:comment>Specifies a reference to a Malware Entity</rdfs:comment>
        <rdfs:isDefinedBy rdf:resource="http://maec.mitre.org/maec_bundle"/>
        <rdfs:label>Malware Entity</rdfs:label>
    </owl:ObjectProperty>
    


    <!-- http://maec.mitre.org/maec_bundle#objectReference -->

    <owl:ObjectProperty rdf:about="http://maec.mitre.org/maec_bundle#objectReference">
        <rdfs:range rdf:resource="http://cybox.mitre.org/cybox_core#Object"/>
        <rdfs:comment>Specifies a reference to a single Object in the Bundle that is part of the candidate indicator&apos;s composition.</rdfs:comment>
        <rdfs:isDefinedBy rdf:resource="http://maec.mitre.org/maec_bundle"/>
        <rdfs:label>Object Reference</rdfs:label>
    </owl:ObjectProperty>
    


    <!-- http://maec.mitre.org/maec_bundle#objectiveReference -->

    <owl:ObjectProperty rdf:about="http://maec.mitre.org/maec_bundle#objectiveReference">
        <rdfs:range rdf:resource="http://maec.mitre.org/maec_bundle#CapabilityObjective"/>
        <rdfs:comment>Specifies one or more Capability Objective (either Strategic or Objective) in the relationship.</rdfs:comment>
        <rdfs:isDefinedBy rdf:resource="http://maec.mitre.org/maec_bundle"/>
        <rdfs:label>Reference</rdfs:label>
    </owl:ObjectProperty>
    


    <!-- http://maec.mitre.org/maec_bundle#objects -->

    <owl:ObjectProperty rdf:about="http://maec.mitre.org/maec_bundle#objects">
        <rdfs:range rdf:resource="http://cybox.mitre.org/cybox_core#Object"/>
        <rdfs:comment>Specifies the list of objects associated with the malware instance.</rdfs:comment>
        <rdfs:isDefinedBy rdf:resource="http://maec.mitre.org/maec_bundle"/>
        <rdfs:label>Objects</rdfs:label>
    </owl:ObjectProperty>
    


    <!-- http://maec.mitre.org/maec_bundle#parentAction -->

    <owl:ObjectProperty rdf:about="http://maec.mitre.org/maec_bundle#parentAction">
        <rdfs:range rdf:resource="http://cybox.mitre.org/cybox_core#Action"/>
        <rdfs:comment>Specifies the action that created or injected this process.</rdfs:comment>
        <rdfs:isDefinedBy rdf:resource="http://maec.mitre.org/maec_bundle"/>
        <rdfs:label>Parent Action</rdfs:label>
    </owl:ObjectProperty>
    


    <!-- http://maec.mitre.org/maec_bundle#processTree -->

    <owl:ObjectProperty rdf:about="http://maec.mitre.org/maec_bundle#processTree">
        <rdfs:range rdf:resource="http://maec.mitre.org/maec_bundle#ProcessTreeNode"/>
        <rdfs:comment>Specifies the observed process tree of execution for the malware instance, along with references to any corresponding actions that were initiated, if applicable.</rdfs:comment>
        <rdfs:isDefinedBy rdf:resource="http://maec.mitre.org/maec_bundle"/>
        <rdfs:label>Process Tree</rdfs:label>
    </owl:ObjectProperty>
    


    <!-- http://maec.mitre.org/maec_bundle#purpose.exploitTargetedPlatforms -->

    <owl:ObjectProperty rdf:about="http://maec.mitre.org/maec_bundle#purpose.exploitTargetedPlatforms">
        <rdfs:range>
            <owl:Class>
                <owl:unionOf rdf:parseType="Collection">
                    <rdf:Description rdf:about="http://cpe.mitre.org/cpe#CPE"/>
                    <rdf:Description rdf:about="http://cybox.mitre.org/cyboxCommon#PlatformSpecification"/>
                </owl:unionOf>
            </owl:Class>
        </rdfs:range>
        <rdfs:comment>Specifies the platforms(s) targeted by the vulnerability exploit.</rdfs:comment>
        <rdfs:isDefinedBy rdf:resource="http://maec.mitre.org/maec_bundle"/>
        <rdfs:label>Targeted Platforms of Exploit</rdfs:label>
    </owl:ObjectProperty>
    


    <!-- http://maec.mitre.org/maec_bundle#purpose.exploitTargetedVulnerability -->

    <owl:ObjectProperty rdf:about="http://maec.mitre.org/maec_bundle#purpose.exploitTargetedVulnerability">
        <rdfs:range rdf:resource="http://nvd.nist.gov/cve#Vulnerability"/>
        <rdfs:comment>Specifies the vulnerability targeted by the exploit, if available.</rdfs:comment>
        <rdfs:isDefinedBy rdf:resource="http://maec.mitre.org/maec_bundle"/>
        <rdfs:label>Targeted Vulnerability of Exploit</rdfs:label>
    </owl:ObjectProperty>
    


    <!-- http://maec.mitre.org/maec_bundle#purpose.exploitTargetedWeakness -->

    <owl:ObjectProperty rdf:about="http://maec.mitre.org/maec_bundle#purpose.exploitTargetedWeakness">
        <rdfs:range>
            <owl:Class>
                <owl:unionOf rdf:parseType="Collection">
                    <rdf:Description rdf:about="http://cwe.mitre.org/cwe#Category"/>
                    <rdf:Description rdf:about="http://cwe.mitre.org/cwe#CompoundElement"/>
                    <rdf:Description rdf:about="http://cwe.mitre.org/cwe#View"/>
                    <rdf:Description rdf:about="http://cwe.mitre.org/cwe#Weakness"/>
                </owl:unionOf>
            </owl:Class>
        </rdfs:range>
        <rdfs:comment>Specifies the Common Weakness Enumeration (CWE) entry that represents the type of weakness targeted by the exploit.</rdfs:comment>
        <rdfs:isDefinedBy rdf:resource="http://maec.mitre.org/maec_bundle"/>
        <rdfs:label>Targeted Weakness of Exploit</rdfs:label>
    </owl:ObjectProperty>
    


    <!-- http://maec.mitre.org/maec_bundle#spawnedProcess -->

    <owl:ObjectProperty rdf:about="http://maec.mitre.org/maec_bundle#spawnedProcess">
        <rdfs:range rdf:resource="http://maec.mitre.org/maec_bundle#ProcessTreeNode"/>
        <rdfs:comment>Specifies one ore more child processes spawned by this process.</rdfs:comment>
        <rdfs:isDefinedBy rdf:resource="http://maec.mitre.org/maec_bundle"/>
        <rdfs:label>Spawned Process</rdfs:label>
    </owl:ObjectProperty>
    


    <!-- http://maec.mitre.org/maec_bundle#strategicObjective -->

    <owl:ObjectProperty rdf:about="http://maec.mitre.org/maec_bundle#strategicObjective">
        <rdfs:range rdf:resource="http://maec.mitre.org/maec_bundle#CapabilityObjective"/>
        <rdfs:comment>Specifies one or more strategic objectives that the Capability attempts to achieve. It can be considered as a more granular way of capturing the Capabilities present in the malware instance.</rdfs:comment>
        <rdfs:isDefinedBy rdf:resource="http://maec.mitre.org/maec_bundle"/>
        <rdfs:label>Strategic Objective</rdfs:label>
    </owl:ObjectProperty>
    


    <!-- http://maec.mitre.org/maec_bundle#subComposition -->

    <owl:ObjectProperty rdf:about="http://maec.mitre.org/maec_bundle#subComposition">
        <rdfs:range rdf:resource="http://maec.mitre.org/maec_bundle#CandidateIndicatorComposition"/>
        <rdfs:comment></rdfs:comment>
        <rdfs:isDefinedBy rdf:resource="http://maec.mitre.org/maec_bundle"/>
        <rdfs:label>Sub-Composition</rdfs:label>
    </owl:ObjectProperty>
    


    <!-- http://maec.mitre.org/maec_bundle#tacticalObjective -->

    <owl:ObjectProperty rdf:about="http://maec.mitre.org/maec_bundle#tacticalObjective">
        <rdfs:range rdf:resource="http://maec.mitre.org/maec_bundle#CapabilityObjective"/>
        <rdfs:comment>Specifies one or more tactical objectives that the Capability attempts to achieve, typically in the context of a broader Strategic Objective. It can be considered as a way of expounding upon Strategic Objectives to capture the Capabilities of the malware instance in more detail.</rdfs:comment>
        <rdfs:isDefinedBy rdf:resource="http://maec.mitre.org/maec_bundle"/>
        <rdfs:label>Tactical Objective</rdfs:label>
    </owl:ObjectProperty>
    


    <!-- 
    ///////////////////////////////////////////////////////////////////////////////////////
    //
    // Data properties
    //
    ///////////////////////////////////////////////////////////////////////////////////////
     -->

    


    <!-- http://maec.mitre.org/maec_bundle#behaviorDescription -->

    <owl:DatatypeProperty rdf:about="http://maec.mitre.org/maec_bundle#behaviorDescription">
        <rdfs:range rdf:resource="http://www.w3.org/2001/XMLSchema#string"/>
        <rdfs:comment>Specifies a prose textual description of the Behavior.</rdfs:comment>
        <rdfs:isDefinedBy rdf:resource="http://maec.mitre.org/maec_bundle"/>
        <rdfs:label>Description</rdfs:label>
    </owl:DatatypeProperty>
    


    <!-- http://maec.mitre.org/maec_bundle#behaviorDuration -->

    <owl:DatatypeProperty rdf:about="http://maec.mitre.org/maec_bundle#behaviorDuration">
        <rdfs:range rdf:resource="http://www.w3.org/2001/XMLSchema#duration"/>
        <rdfs:comment>Specifies the duration of the Behavior. One way to derive such a value may be to calculate the difference between the timestamps of the first and last actions that compose the behavior.</rdfs:comment>
        <rdfs:isDefinedBy rdf:resource="http://maec.mitre.org/maec_bundle"/>
        <rdfs:label>Duration</rdfs:label>
    </owl:DatatypeProperty>
    


    <!-- http://maec.mitre.org/maec_bundle#behaviorOrdinalPosition -->

    <owl:DatatypeProperty rdf:about="http://maec.mitre.org/maec_bundle#behaviorOrdinalPosition">
        <rdfs:range rdf:resource="http://www.w3.org/2001/XMLSchema#positiveInteger"/>
        <rdfs:comment>Specifies the ordinal position of the Behavior with respect to the execution of the malware.</rdfs:comment>
        <rdfs:isDefinedBy rdf:resource="http://maec.mitre.org/maec_bundle"/>
        <rdfs:label>Ordinal Position</rdfs:label>
    </owl:DatatypeProperty>
    


    <!-- http://maec.mitre.org/maec_bundle#behaviorRelationshipType -->

    <owl:DatatypeProperty rdf:about="http://maec.mitre.org/maec_bundle#behaviorRelationshipType">
        <rdfs:range rdf:resource="http://www.w3.org/2001/XMLSchema#string"/>
        <rdfs:comment>Characterizes a relationship between entities.</rdfs:comment>
        <rdfs:isDefinedBy rdf:resource="http://maec.mitre.org/maec_bundle"/>
        <rdfs:label>Relationship Type</rdfs:label>
    </owl:DatatypeProperty>
    


    <!-- http://maec.mitre.org/maec_bundle#behaviorStatus -->

    <owl:DatatypeProperty rdf:about="http://maec.mitre.org/maec_bundle#behaviorStatus">
        <rdfs:range rdf:resource="http://www.w3.org/2001/XMLSchema#string"/>
        <rdfs:comment>Specifies the execution status of the Behavior being characterized.</rdfs:comment>
        <rdfs:isDefinedBy rdf:resource="http://maec.mitre.org/maec_bundle"/>
        <rdfs:label>Status</rdfs:label>
    </owl:DatatypeProperty>
    


    <!-- http://maec.mitre.org/maec_bundle#behavioralOrdering -->

    <owl:DatatypeProperty rdf:about="http://maec.mitre.org/maec_bundle#behavioralOrdering">
        <rdfs:range rdf:resource="http://www.w3.org/2001/XMLSchema#positiveInteger"/>
        <rdfs:comment>Specifies  the ordering of the Action with respect to the other Actions that make up the behavior. So an action with a behavioral_ordering of &quot;1&quot; would come before an Action with a behavioral_ordering of &quot;2&quot;, etc.</rdfs:comment>
        <rdfs:isDefinedBy rdf:resource="http://maec.mitre.org/maec_bundle"/>
        <rdfs:label>Behavioral Ordering</rdfs:label>
    </owl:DatatypeProperty>
    


    <!-- http://maec.mitre.org/maec_bundle#candidateDescription -->

    <owl:DatatypeProperty rdf:about="http://maec.mitre.org/maec_bundle#candidateDescription">
        <rdfs:range rdf:resource="http://www.w3.org/2001/XMLSchema#string"/>
        <rdfs:comment>Specifies a brief description of the Candidate Indicator.</rdfs:comment>
        <rdfs:isDefinedBy rdf:resource="http://maec.mitre.org/maec_bundle"/>
        <rdfs:label>Description</rdfs:label>
    </owl:DatatypeProperty>
    


    <!-- http://maec.mitre.org/maec_bundle#capabilityDescription -->

    <owl:DatatypeProperty rdf:about="http://maec.mitre.org/maec_bundle#capabilityDescription">
        <rdfs:range rdf:resource="http://www.w3.org/2001/XMLSchema#string"/>
        <rdfs:comment>Speciifies a basic textual description of the Capability.</rdfs:comment>
        <rdfs:isDefinedBy rdf:resource="http://maec.mitre.org/maec_bundle"/>
        <rdfs:label>Description</rdfs:label>
    </owl:DatatypeProperty>
    


    <!-- http://maec.mitre.org/maec_bundle#capabilityName -->

    <owl:DatatypeProperty rdf:about="http://maec.mitre.org/maec_bundle#capabilityName">
        <rdfs:range rdf:resource="http://www.w3.org/2001/XMLSchema#string"/>
        <rdfs:comment>Specifies the name of the Capability</rdfs:comment>
        <rdfs:isDefinedBy rdf:resource="http://maec.mitre.org/maec_bundle"/>
        <rdfs:label>Name</rdfs:label>
    </owl:DatatypeProperty>
    


    <!-- http://maec.mitre.org/maec_bundle#capabilityObjectiveRelationshipType -->

    <owl:DatatypeProperty rdf:about="http://maec.mitre.org/maec_bundle#capabilityObjectiveRelationshipType">
        <rdfs:range rdf:resource="http://www.w3.org/2001/XMLSchema#string"/>
        <rdfs:comment>Characterizes a relationship between entities.</rdfs:comment>
        <rdfs:isDefinedBy rdf:resource="http://maec.mitre.org/maec_bundle"/>
        <rdfs:label>Relationship Type</rdfs:label>
    </owl:DatatypeProperty>
    


    <!-- http://maec.mitre.org/maec_bundle#capabilityPropertyName -->

    <owl:DatatypeProperty rdf:about="http://maec.mitre.org/maec_bundle#capabilityPropertyName">
        <rdfs:range rdf:resource="http://www.w3.org/2001/XMLSchema#string"/>
        <rdfs:comment>Specifies the name of the property being captured.</rdfs:comment>
        <rdfs:isDefinedBy rdf:resource="http://maec.mitre.org/maec_bundle"/>
        <rdfs:label>Name</rdfs:label>
    </owl:DatatypeProperty>
    


    <!-- http://maec.mitre.org/maec_bundle#capabilityPropertyValue -->

    <owl:DatatypeProperty rdf:about="http://maec.mitre.org/maec_bundle#capabilityPropertyValue">
        <rdfs:range rdf:resource="http://www.w3.org/2001/XMLSchema#string"/>
        <rdfs:comment>Specifies the value of the property being captured.</rdfs:comment>
        <rdfs:isDefinedBy rdf:resource="http://maec.mitre.org/maec_bundle"/>
        <rdfs:label>Value</rdfs:label>
    </owl:DatatypeProperty>
    


    <!-- http://maec.mitre.org/maec_bundle#capabilityRelationshipType -->

    <owl:DatatypeProperty rdf:about="http://maec.mitre.org/maec_bundle#capabilityRelationshipType">
        <rdfs:range rdf:resource="http://www.w3.org/2001/XMLSchema#string"/>
        <rdfs:comment>Specifies the type of capability relationship being expressed between.</rdfs:comment>
        <rdfs:isDefinedBy rdf:resource="http://maec.mitre.org/maec_bundle"/>
        <rdfs:label>Relationship Type</rdfs:label>
    </owl:DatatypeProperty>
    


    <!-- http://maec.mitre.org/maec_bundle#classificationName -->

    <owl:DatatypeProperty rdf:about="http://maec.mitre.org/maec_bundle#classificationName">
        <rdfs:range rdf:resource="http://www.w3.org/2001/XMLSchema#string"/>
        <rdfs:comment>Specifies the classification assigned to the malware instance object by the AV scanner tool characterized in the Company Name and Product Name fields.</rdfs:comment>
        <rdfs:isDefinedBy rdf:resource="http://maec.mitre.org/maec_bundle"/>
        <rdfs:label>classification name</rdfs:label>
    </owl:DatatypeProperty>
    


    <!-- http://maec.mitre.org/maec_bundle#contentType -->

    <owl:DatatypeProperty rdf:about="http://maec.mitre.org/maec_bundle#contentType">
        <rdfs:range rdf:resource="http://www.w3.org/2001/XMLSchema#string"/>
        <rdfs:comment></rdfs:comment>
        <rdfs:isDefinedBy rdf:datatype="http://www.w3.org/2001/XMLSchema#string">&lt;http://maec.mitre.org/maec_bundle&gt;</rdfs:isDefinedBy>
        <rdfs:label>content type</rdfs:label>
    </owl:DatatypeProperty>
    


    <!-- http://maec.mitre.org/maec_bundle#definitionVersion -->

    <owl:DatatypeProperty rdf:about="http://maec.mitre.org/maec_bundle#definitionVersion">
        <rdfs:range rdf:resource="http://www.w3.org/2001/XMLSchema#string"/>
        <rdfs:comment>Specifies the version of the AV definitions used by the AV scanner tool that assigned the classification to the malware instance object.</rdfs:comment>
        <rdfs:isDefinedBy rdf:resource="http://maec.mitre.org/maec_bundle"/>
        <rdfs:label>definition version</rdfs:label>
    </owl:DatatypeProperty>
    


    <!-- http://maec.mitre.org/maec_bundle#engineVersion -->

    <owl:DatatypeProperty rdf:about="http://maec.mitre.org/maec_bundle#engineVersion">
        <rdfs:range rdf:resource="http://www.w3.org/2001/XMLSchema#string"/>
        <rdfs:comment>Specifies  the version of the AV engine used by the AV scanner tool that assigned the classification to the malware instance object.</rdfs:comment>
        <rdfs:isDefinedBy rdf:resource="http://maec.mitre.org/maec_bundle"/>
        <rdfs:label>engine version</rdfs:label>
    </owl:DatatypeProperty>
    


    <!-- http://maec.mitre.org/maec_bundle#malwareEntityDescription -->

    <owl:DatatypeProperty rdf:about="http://maec.mitre.org/maec_bundle#malwareEntityDescription">
        <rdfs:range rdf:resource="http://www.w3.org/2001/XMLSchema#string"/>
        <rdfs:comment>Specifies a brief description of the entity that the indicator or signature is written against.</rdfs:comment>
        <rdfs:isDefinedBy rdf:resource="http://maec.mitre.org/maec_bundle"/>
        <rdfs:label>Malware Entity Description</rdfs:label>
    </owl:DatatypeProperty>
    


    <!-- http://maec.mitre.org/maec_bundle#malwareEntityName -->

    <owl:DatatypeProperty rdf:about="http://maec.mitre.org/maec_bundle#malwareEntityName">
        <rdfs:range rdf:resource="http://www.w3.org/2001/XMLSchema#string"/>
        <rdfs:comment>Specifies the name of the malware instance, malware family, or malware class that the indicator or signature is written against.</rdfs:comment>
        <rdfs:isDefinedBy rdf:resource="http://maec.mitre.org/maec_bundle"/>
        <rdfs:label>Malware Entity Name</rdfs:label>
    </owl:DatatypeProperty>
    


    <!-- http://maec.mitre.org/maec_bundle#malwareEntityType -->

    <owl:DatatypeProperty rdf:about="http://maec.mitre.org/maec_bundle#malwareEntityType">
        <rdfs:range rdf:resource="http://www.w3.org/2001/XMLSchema#string"/>
        <rdfs:comment>Specifies the specific type of malware entity that the indicator or signature is written against.</rdfs:comment>
        <rdfs:isDefinedBy rdf:resource="http://maec.mitre.org/maec_bundle"/>
        <rdfs:label>Malware Entity Type</rdfs:label>
    </owl:DatatypeProperty>
    


    <!-- http://maec.mitre.org/maec_bundle#numericImportance -->

    <owl:DatatypeProperty rdf:about="http://maec.mitre.org/maec_bundle#numericImportance">
        <rdfs:range rdf:resource="http://www.w3.org/2001/XMLSchema#positiveInteger"/>
        <rdfs:comment>Specifies the specific numeric importance of the Candidate Indicator.</rdfs:comment>
        <rdfs:isDefinedBy rdf:resource="http://maec.mitre.org/maec_bundle"/>
        <rdfs:label>Numeric Importance</rdfs:label>
    </owl:DatatypeProperty>
    


    <!-- http://maec.mitre.org/maec_bundle#objectiveDescription -->

    <owl:DatatypeProperty rdf:about="http://maec.mitre.org/maec_bundle#objectiveDescription">
        <rdfs:range rdf:resource="http://www.w3.org/2001/XMLSchema#string"/>
        <rdfs:comment></rdfs:comment>
        <rdfs:isDefinedBy rdf:datatype="http://www.w3.org/2001/XMLSchema#string">&lt;http://maec.mitre.org/maec_bundle&gt;</rdfs:isDefinedBy>
        <rdfs:label>objective description</rdfs:label>
    </owl:DatatypeProperty>
    


    <!-- http://maec.mitre.org/maec_bundle#operator -->

    <owl:DatatypeProperty rdf:about="http://maec.mitre.org/maec_bundle#operator">
        <rdfs:range>
            <rdfs:Datatype>
                <owl:oneOf>
                    <rdf:Description>
                        <rdf:type rdf:resource="http://www.w3.org/1999/02/22-rdf-syntax-ns#List"/>
                        <rdf:first rdf:datatype="http://www.w3.org/2001/XMLSchema#string">AND</rdf:first>
                        <rdf:rest>
                            <rdf:Description>
                                <rdf:type rdf:resource="http://www.w3.org/1999/02/22-rdf-syntax-ns#List"/>
                                <rdf:first rdf:datatype="http://www.w3.org/2001/XMLSchema#string">OR</rdf:first>
                                <rdf:rest rdf:resource="http://www.w3.org/1999/02/22-rdf-syntax-ns#nil"/>
                            </rdf:Description>
                        </rdf:rest>
                    </rdf:Description>
                </owl:oneOf>
            </rdfs:Datatype>
        </rdfs:range>
        <rdfs:comment>Specifies the Boolean operator for this level of the Candidate Indicator&apos;s composition.</rdfs:comment>
        <rdfs:isDefinedBy rdf:resource="http://maec.mitre.org/maec_bundle"/>
        <rdfs:label>Operator</rdfs:label>
    </owl:DatatypeProperty>
    


    <!-- http://maec.mitre.org/maec_bundle#processOrdinalPosition -->

    <owl:DatatypeProperty rdf:about="http://maec.mitre.org/maec_bundle#processOrdinalPosition">
        <rdfs:range rdf:resource="http://www.w3.org/2001/XMLSchema#positiveInteger"/>
        <rdfs:comment>Specifies the ordinal position of the process with respect to the other processes spawned or injected by the malware.</rdfs:comment>
        <rdfs:isDefinedBy rdf:resource="http://maec.mitre.org/maec_bundle"/>
        <rdfs:label>Ordinal Position</rdfs:label>
    </owl:DatatypeProperty>
    


    <!-- http://maec.mitre.org/maec_bundle#purpose -->

    <owl:DatatypeProperty rdf:about="http://maec.mitre.org/maec_bundle#purpose">
        <rdfs:range rdf:resource="http://www.w3.org/2001/XMLSchema#string"/>
        <rdfs:comment>Specifies the intended purpose of the collection of Behaviors. 

Since Behaviors are not always successful, and may not be fully observed, this is meant as way of abstracting the nature of the collection of Behaviors away  from its constituent Actions.</rdfs:comment>
        <rdfs:isDefinedBy rdf:resource="http://maec.mitre.org/maec_bundle"/>
        <rdfs:label>Purpose</rdfs:label>
    </owl:DatatypeProperty>
    


    <!-- http://maec.mitre.org/maec_bundle#purpose.description -->

    <owl:DatatypeProperty rdf:about="http://maec.mitre.org/maec_bundle#purpose.description">
        <rdfs:range rdf:resource="http://www.w3.org/2001/XMLSchema#string"/>
        <rdfs:comment>Specifies a prose text description of the purpose of the Behavior, whether it was successful or not.</rdfs:comment>
        <rdfs:isDefinedBy rdf:resource="http://maec.mitre.org/maec_bundle"/>
        <rdfs:label>Purpose Description</rdfs:label>
    </owl:DatatypeProperty>
    


    <!-- http://maec.mitre.org/maec_bundle#purpose.exploitKnownVulnerability -->

    <owl:DatatypeProperty rdf:about="http://maec.mitre.org/maec_bundle#purpose.exploitKnownVulnerability">
        <rdfs:range rdf:resource="http://www.w3.org/2001/XMLSchema#boolean"/>
        <rdfs:comment>Specifies whether the vulnerability that the malware is exploiting has been previously identified. If so, it should be referenced via a CVE ID. If not, the platform(s) targeted by the vulnerability exploitation behavior may be specified.</rdfs:comment>
        <rdfs:isDefinedBy rdf:resource="http://maec.mitre.org/maec_bundle"/>
        <rdfs:label>Exploit of Know Vulnerability</rdfs:label>
    </owl:DatatypeProperty>
    


    <!-- http://maec.mitre.org/maec_bundle#strategicObjectiveName -->

    <owl:DatatypeProperty rdf:about="http://maec.mitre.org/maec_bundle#strategicObjectiveName">
        <rdfs:range rdf:resource="http://www.w3.org/2001/XMLSchema#string"/>
        <rdfs:comment>Specifies the name of the Strategic Capability Objective.</rdfs:comment>
        <rdfs:isDefinedBy rdf:resource="http://maec.mitre.org/maec_bundle"/>
        <rdfs:label>Capabiity Objective Name</rdfs:label>
    </owl:DatatypeProperty>
    


    <!-- http://maec.mitre.org/maec_bundle#tacticalObjectiveName -->

    <owl:DatatypeProperty rdf:about="http://maec.mitre.org/maec_bundle#tacticalObjectiveName">
        <rdfs:range rdf:resource="http://www.w3.org/2001/XMLSchema#string"/>
        <rdfs:comment>Specifies the name of the Tactical Capability Objective.</rdfs:comment>
        <rdfs:isDefinedBy rdf:resource="http://maec.mitre.org/maec_bundle"/>
        <rdfs:label>tactical objective name</rdfs:label>
    </owl:DatatypeProperty>
    


    <!-- http://maec.mitre.org/maec_bundle#timestamp -->

    <owl:DatatypeProperty rdf:about="http://maec.mitre.org/maec_bundle#timestamp">
        <rdfs:range rdf:resource="http://www.w3.org/2001/XMLSchema#dateTime"/>
        <rdfs:comment>Specifies the date and time that the bundle was generated.</rdfs:comment>
        <rdfs:isDefinedBy rdf:resource="http://maec.mitre.org/maec_bundle"/>
        <rdfs:label>timestamp</rdfs:label>
    </owl:DatatypeProperty>
    


    <!-- 
    ///////////////////////////////////////////////////////////////////////////////////////
    //
    // Classes
    //
    ///////////////////////////////////////////////////////////////////////////////////////
     -->

    
    


    <!-- http://maec.mitre.org/maec_bundle#AVClassification -->

    <owl:Class rdf:about="http://maec.mitre.org/maec_bundle#AVClassification">
        <rdfs:subClassOf rdf:resource="http://maec.mitre.org/maec_common#ToolInformation"/>
        <rdfs:subClassOf>
            <owl:Restriction>
                <owl:onProperty rdf:resource="http://maec.mitre.org/maec_bundle#classificationName"/>
                <owl:someValuesFrom rdf:resource="http://www.w3.org/2000/01/rdf-schema#Literal"/>
            </owl:Restriction>
        </rdfs:subClassOf>
        <rdfs:subClassOf>
            <owl:Restriction>
                <owl:onProperty rdf:resource="http://maec.mitre.org/maec_bundle#definitionVersion"/>
                <owl:someValuesFrom rdf:resource="http://www.w3.org/2000/01/rdf-schema#Literal"/>
            </owl:Restriction>
        </rdfs:subClassOf>
        <rdfs:subClassOf>
            <owl:Restriction>
                <owl:onProperty rdf:resource="http://maec.mitre.org/maec_bundle#engineVersion"/>
                <owl:someValuesFrom rdf:resource="http://www.w3.org/2000/01/rdf-schema#Literal"/>
            </owl:Restriction>
        </rdfs:subClassOf>
        <rdfs:comment>Characterizes information on AV scanner classifications for the malware instance object captured in the Bundle or Package.</rdfs:comment>
        <rdfs:isDefinedBy rdf:resource="http://maec.mitre.org/maec_bundle"/>
        <rdfs:label>AVClassification</rdfs:label>
    </owl:Class>
    


    <!-- http://maec.mitre.org/maec_bundle#ActionCollection -->

    <owl:Class rdf:about="http://maec.mitre.org/maec_bundle#ActionCollection">
        <rdfs:subClassOf rdf:resource="http://maec.mitre.org/maec_common#BaseCollection"/>
        <rdfs:comment>Characterizes a collection of actions. This can be useful for organizing actions that may be related and where the exact relationship is unknown, as well as actions whose associated behavior has not yet been established.</rdfs:comment>
        <rdfs:isDefinedBy rdf:resource="http://maec.mitre.org/maec_bundle"/>
        <rdfs:label>Action Collection</rdfs:label>
    </owl:Class>
    


    <!-- http://maec.mitre.org/maec_bundle#AnalysisBundle -->

    <owl:Class rdf:about="http://maec.mitre.org/maec_bundle#AnalysisBundle">
        <rdfs:subClassOf>
            <owl:Restriction>
                <owl:onProperty rdf:resource="http://maec.mitre.org/maec_bundle#contentType"/>
                <owl:someValuesFrom rdf:resource="http://www.w3.org/2000/01/rdf-schema#Literal"/>
            </owl:Restriction>
        </rdfs:subClassOf>
        <rdfs:subClassOf>
            <owl:Restriction>
                <owl:onProperty rdf:resource="http://maec.mitre.org/maec_bundle#timestamp"/>
                <owl:someValuesFrom rdf:resource="http://www.w3.org/2000/01/rdf-schema#Literal"/>
            </owl:Restriction>
        </rdfs:subClassOf>
        <rdfs:comment>Characterizes analysis data (from any arbitrary set of analyses) for a single malware instance in terms of its Behaviors, Actions, Objects, etc.).</rdfs:comment>
        <rdfs:isDefinedBy rdf:resource="http://maec.mitre.org/maec_bundle"/>
        <rdfs:label>Analysis Bundle</rdfs:label>
    </owl:Class>
    


    <!-- http://maec.mitre.org/maec_bundle#Behavior -->

    <owl:Class rdf:about="http://maec.mitre.org/maec_bundle#Behavior">
        <rdfs:subClassOf>
            <owl:Restriction>
                <owl:onProperty rdf:resource="http://maec.mitre.org/maec_bundle#purpose.exploitTargetedVulnerability"/>
                <owl:someValuesFrom rdf:resource="http://www.w3.org/2002/07/owl#Thing"/>
            </owl:Restriction>
        </rdfs:subClassOf>
        <rdfs:subClassOf>
            <owl:Restriction>
                <owl:onProperty rdf:resource="http://maec.mitre.org/maec_bundle#behaviorDescription"/>
                <owl:someValuesFrom rdf:resource="http://www.w3.org/2000/01/rdf-schema#Literal"/>
            </owl:Restriction>
        </rdfs:subClassOf>
        <rdfs:subClassOf>
            <owl:Restriction>
                <owl:onProperty rdf:resource="http://maec.mitre.org/maec_bundle#behaviorDuration"/>
                <owl:someValuesFrom rdf:resource="http://www.w3.org/2000/01/rdf-schema#Literal"/>
            </owl:Restriction>
        </rdfs:subClassOf>
        <rdfs:subClassOf>
            <owl:Restriction>
                <owl:onProperty rdf:resource="http://maec.mitre.org/maec_bundle#behaviorOrdinalPosition"/>
                <owl:someValuesFrom rdf:resource="http://www.w3.org/2000/01/rdf-schema#Literal"/>
            </owl:Restriction>
        </rdfs:subClassOf>
        <rdfs:subClassOf>
            <owl:Restriction>
                <owl:onProperty rdf:resource="http://maec.mitre.org/maec_bundle#behaviorStatus"/>
                <owl:someValuesFrom rdf:resource="http://www.w3.org/2000/01/rdf-schema#Literal"/>
            </owl:Restriction>
        </rdfs:subClassOf>
        <rdfs:subClassOf>
            <owl:Restriction>
                <owl:onProperty rdf:resource="http://maec.mitre.org/maec_bundle#purpose.description"/>
                <owl:someValuesFrom rdf:resource="http://www.w3.org/2000/01/rdf-schema#Literal"/>
            </owl:Restriction>
        </rdfs:subClassOf>
        <rdfs:comment>Characterizes malicious behaviors found or observed in malware. 

Behaviors can be thought of as representing the purpose behind groups of Malware Actions, and are therefore representative of distinct portions of higher-level malware functionality. Thus, while a malware instance may perform some multitude of Actions, it is likely that these Actions represent only a few distinct behaviors. Some examples include vulnerability exploitation, email address harvesting, the disabling of a security service, etc.</rdfs:comment>
        <rdfs:isDefinedBy rdf:resource="http://maec.mitre.org/maec_bundle"/>
        <rdfs:label>Behavior</rdfs:label>
    </owl:Class>
    


    <!-- http://maec.mitre.org/maec_bundle#BehaviorCollection -->

    <owl:Class rdf:about="http://maec.mitre.org/maec_bundle#BehaviorCollection">
        <rdfs:subClassOf rdf:resource="http://maec.mitre.org/maec_common#BaseCollection"/>
        <rdfs:subClassOf>
            <owl:Restriction>
                <owl:onProperty rdf:resource="http://maec.mitre.org/maec_bundle#purpose"/>
                <owl:someValuesFrom rdf:resource="http://www.w3.org/2000/01/rdf-schema#Literal"/>
            </owl:Restriction>
        </rdfs:subClassOf>
        <rdfs:comment>Characterizes a collection of behaviors.</rdfs:comment>
        <rdfs:isDefinedBy rdf:resource="http://maec.mitre.org/maec_bundle"/>
        <rdfs:label>Behavior Collection</rdfs:label>
    </owl:Class>
    


    <!-- http://maec.mitre.org/maec_bundle#BehaviorRelationshipStatement -->

    <owl:Class rdf:about="http://maec.mitre.org/maec_bundle#BehaviorRelationshipStatement">
        <rdfs:subClassOf rdf:resource="http://www.w3.org/1999/02/22-rdf-syntax-ns#Statement"/>
        <rdfs:subClassOf>
            <owl:Restriction>
                <owl:onProperty rdf:resource="http://maec.mitre.org/maec_bundle#behaviorRelationshipType"/>
                <owl:someValuesFrom rdf:resource="http://www.w3.org/2000/01/rdf-schema#Literal"/>
            </owl:Restriction>
        </rdfs:subClassOf>
        <rdfs:comment>Specifies  any relationships between a Behavior and other Behaviors.</rdfs:comment>
        <rdfs:isDefinedBy rdf:resource="http://maec.mitre.org/maec_bundle"/>
        <rdfs:label>Behavior relationship</rdfs:label>
    </owl:Class>
    


    <!-- http://maec.mitre.org/maec_bundle#BehavioralAction -->

    <owl:Class rdf:about="http://maec.mitre.org/maec_bundle#BehavioralAction">
        <rdfs:subClassOf rdf:resource="http://maec.mitre.org/maec_common#MalwareAction"/>
        <rdfs:subClassOf>
            <owl:Restriction>
                <owl:onProperty rdf:resource="http://maec.mitre.org/maec_bundle#behavioralOrdering"/>
                <owl:someValuesFrom rdf:resource="http://www.w3.org/2000/01/rdf-schema#Literal"/>
            </owl:Restriction>
        </rdfs:subClassOf>
        <rdfs:comment>Characterizes an Action field that can be used as part of a Behavior.</rdfs:comment>
        <rdfs:isDefinedBy rdf:resource="http://maec.mitre.org/maec_bundle"/>
        <rdfs:label>Behavioral Action</rdfs:label>
    </owl:Class>
    


    <!-- http://maec.mitre.org/maec_bundle#BehavioralActionEquivalence -->

    <owl:Class rdf:about="http://maec.mitre.org/maec_bundle#BehavioralActionEquivalence">
        <rdfs:subClassOf rdf:resource="http://maec.mitre.org/maec_common#ActionEquivalence"/>
        <rdfs:comment></rdfs:comment>
        <rdfs:isDefinedBy rdf:datatype="http://www.w3.org/2001/XMLSchema#string">&lt;http://maec.mitre.org/maec_bundle&gt;</rdfs:isDefinedBy>
        <rdfs:label>Behavioral action equivalence</rdfs:label>
    </owl:Class>
    


    <!-- http://maec.mitre.org/maec_bundle#CandidateIndicator -->

    <owl:Class rdf:about="http://maec.mitre.org/maec_bundle#CandidateIndicator">
        <rdfs:subClassOf>
            <owl:Restriction>
                <owl:onProperty rdf:resource="http://maec.mitre.org/maec_bundle#composition"/>
                <owl:someValuesFrom rdf:resource="http://www.w3.org/2002/07/owl#Thing"/>
            </owl:Restriction>
        </rdfs:subClassOf>
        <rdfs:subClassOf>
            <owl:Restriction>
                <owl:onProperty rdf:resource="http://maec.mitre.org/maec_bundle#malwareEntity"/>
                <owl:someValuesFrom rdf:resource="http://www.w3.org/2002/07/owl#Thing"/>
            </owl:Restriction>
        </rdfs:subClassOf>
        <rdfs:subClassOf>
            <owl:Restriction>
                <owl:onProperty rdf:resource="http://maec.mitre.org/maec_bundle#candidateDescription"/>
                <owl:someValuesFrom rdf:resource="http://www.w3.org/2000/01/rdf-schema#Literal"/>
            </owl:Restriction>
        </rdfs:subClassOf>
        <rdfs:subClassOf>
            <owl:Restriction>
                <owl:onProperty rdf:resource="http://maec.mitre.org/maec_bundle#numericImportance"/>
                <owl:someValuesFrom rdf:resource="http://www.w3.org/2000/01/rdf-schema#Literal"/>
            </owl:Restriction>
        </rdfs:subClassOf>
        <rdfs:comment>Characterizes the particular components that may signify the presence of the malware instance on a host system or network.</rdfs:comment>
        <rdfs:isDefinedBy rdf:resource="http://maec.mitre.org/maec_bundle"/>
        <rdfs:label>Candidate indicator</rdfs:label>
    </owl:Class>
    


    <!-- http://maec.mitre.org/maec_bundle#CandidateIndicatorCollection -->

    <owl:Class rdf:about="http://maec.mitre.org/maec_bundle#CandidateIndicatorCollection">
        <rdfs:subClassOf rdf:resource="http://maec.mitre.org/maec_common#BaseCollection"/>
        <rdfs:comment>Characterizes a collection of Candidate Indicators.</rdfs:comment>
        <rdfs:isDefinedBy rdf:resource="http://maec.mitre.org/maec_bundle"/>
        <rdfs:label>Candidate Indicator Collection</rdfs:label>
    </owl:Class>
    


    <!-- http://maec.mitre.org/maec_bundle#CandidateIndicatorComposition -->

    <owl:Class rdf:about="http://maec.mitre.org/maec_bundle#CandidateIndicatorComposition">
        <rdfs:subClassOf>
            <owl:Restriction>
                <owl:onProperty rdf:resource="http://maec.mitre.org/maec_bundle#behaviorReference"/>
                <owl:someValuesFrom rdf:resource="http://www.w3.org/2002/07/owl#Thing"/>
            </owl:Restriction>
        </rdfs:subClassOf>
        <rdfs:subClassOf>
            <owl:Restriction>
                <owl:onProperty rdf:resource="http://maec.mitre.org/maec_bundle#objectReference"/>
                <owl:someValuesFrom rdf:resource="http://www.w3.org/2002/07/owl#Thing"/>
            </owl:Restriction>
        </rdfs:subClassOf>
        <rdfs:subClassOf>
            <owl:Restriction>
                <owl:onProperty rdf:resource="http://maec.mitre.org/maec_bundle#operator"/>
                <owl:someValuesFrom rdf:resource="http://www.w3.org/2000/01/rdf-schema#Literal"/>
            </owl:Restriction>
        </rdfs:subClassOf>
        <rdfs:comment>Characterizes the composition of a Candidate Indicator, via references to any corresponding MAEC entities contained in the Bundle.</rdfs:comment>
        <rdfs:isDefinedBy rdf:resource="http://maec.mitre.org/maec_bundle"/>
        <rdfs:label>Candiate Indicator Composition</rdfs:label>
    </owl:Class>
    


    <!-- http://maec.mitre.org/maec_bundle#Capability -->

    <owl:Class rdf:about="http://maec.mitre.org/maec_bundle#Capability">
        <rdfs:subClassOf>
            <owl:Restriction>
                <owl:onProperty rdf:resource="http://maec.mitre.org/maec_bundle#capabilityDescription"/>
                <owl:someValuesFrom rdf:resource="http://www.w3.org/2000/01/rdf-schema#Literal"/>
            </owl:Restriction>
        </rdfs:subClassOf>
        <rdfs:subClassOf>
            <owl:Restriction>
                <owl:onProperty rdf:resource="http://maec.mitre.org/maec_bundle#capabilityName"/>
                <owl:someValuesFrom rdf:resource="http://www.w3.org/2000/01/rdf-schema#Literal"/>
            </owl:Restriction>
        </rdfs:subClassOf>
        <rdfs:comment>Characterizes details of a Capability that may be implemented in the malware instance, along with its child Strategic and Tactical Objectives.</rdfs:comment>
        <rdfs:isDefinedBy rdf:resource="http://maec.mitre.org/maec_bundle"/>
        <rdfs:label>Capability</rdfs:label>
    </owl:Class>
    


    <!-- http://maec.mitre.org/maec_bundle#CapabilityObjective -->

    <owl:Class rdf:about="http://maec.mitre.org/maec_bundle#CapabilityObjective">
        <rdfs:subClassOf>
            <owl:Restriction>
                <owl:onProperty rdf:resource="http://maec.mitre.org/maec_bundle#objectiveDescription"/>
                <owl:someValuesFrom rdf:resource="http://www.w3.org/2000/01/rdf-schema#Literal"/>
            </owl:Restriction>
        </rdfs:subClassOf>
        <rdfs:subClassOf>
            <owl:Restriction>
                <owl:onProperty rdf:resource="http://maec.mitre.org/maec_bundle#strategicObjectiveName"/>
                <owl:someValuesFrom rdf:resource="http://www.w3.org/2000/01/rdf-schema#Literal"/>
            </owl:Restriction>
        </rdfs:subClassOf>
        <rdfs:comment>Characterizes details of a Capability&apos;s Strategic or Tactical Objective.</rdfs:comment>
        <rdfs:isDefinedBy rdf:resource="http://maec.mitre.org/maec_bundle"/>
        <rdfs:label>Capability Objective</rdfs:label>
    </owl:Class>
    


    <!-- http://maec.mitre.org/maec_bundle#CapabilityObjectiveRelationshipStatement -->

    <owl:Class rdf:about="http://maec.mitre.org/maec_bundle#CapabilityObjectiveRelationshipStatement">
        <rdfs:subClassOf rdf:resource="http://www.w3.org/1999/02/22-rdf-syntax-ns#Statement"/>
        <rdfs:subClassOf>
            <owl:Restriction>
                <owl:onProperty rdf:resource="http://maec.mitre.org/maec_bundle#capabilityObjectiveRelationshipType"/>
                <owl:someValuesFrom rdf:resource="http://www.w3.org/2000/01/rdf-schema#Literal"/>
            </owl:Restriction>
        </rdfs:subClassOf>
        <rdfs:comment>Characterizes  a relationship between a Strategic or Tactical Objective and one or more other Strategic or Tactical Objectives.</rdfs:comment>
        <rdfs:isDefinedBy rdf:resource="http://maec.mitre.org/maec_bundle"/>
        <rdfs:label>Capability objective relationship</rdfs:label>
    </owl:Class>
    


    <!-- http://maec.mitre.org/maec_bundle#CapabilityProperty -->

    <owl:Class rdf:about="http://maec.mitre.org/maec_bundle#CapabilityProperty">
        <rdfs:subClassOf>
            <owl:Restriction>
                <owl:onProperty rdf:resource="http://maec.mitre.org/maec_bundle#capabilityPropertyName"/>
                <owl:someValuesFrom rdf:resource="http://www.w3.org/2000/01/rdf-schema#Literal"/>
            </owl:Restriction>
        </rdfs:subClassOf>
        <rdfs:subClassOf>
            <owl:Restriction>
                <owl:onProperty rdf:resource="http://maec.mitre.org/maec_bundle#capabilityPropertyValue"/>
                <owl:someValuesFrom rdf:resource="http://www.w3.org/2000/01/rdf-schema#Literal"/>
            </owl:Restriction>
        </rdfs:subClassOf>
        <rdfs:comment>Characterizes  a single property of a Capability or Capability Objective.</rdfs:comment>
        <rdfs:isDefinedBy rdf:resource="http://maec.mitre.org/maec_bundle"/>
        <rdfs:label>Capability Property</rdfs:label>
    </owl:Class>
    


    <!-- http://maec.mitre.org/maec_bundle#CapabilityRelationshipStatement -->

    <owl:Class rdf:about="http://maec.mitre.org/maec_bundle#CapabilityRelationshipStatement">
        <rdfs:subClassOf rdf:resource="http://maec.mitre.org/maec_bundle#CapabilityObjectiveRelationshipStatement"/>
        <rdfs:subClassOf>
            <owl:Restriction>
                <owl:onProperty rdf:resource="http://maec.mitre.org/maec_bundle#capabilityRelationshipType"/>
                <owl:someValuesFrom rdf:resource="http://www.w3.org/2000/01/rdf-schema#Literal"/>
            </owl:Restriction>
        </rdfs:subClassOf>
        <rdfs:comment>Characterizes a relationship between a Capability and one or more other Capabilities.</rdfs:comment>
        <rdfs:isDefinedBy rdf:resource="http://maec.mitre.org/maec_bundle"/>
        <rdfs:label>Capability Relationship</rdfs:label>
    </owl:Class>
    


    <!-- http://maec.mitre.org/maec_bundle#MalwareEntity -->

    <owl:Class rdf:about="http://maec.mitre.org/maec_bundle#MalwareEntity">
        <rdfs:subClassOf>
            <owl:Restriction>
                <owl:onProperty rdf:resource="http://maec.mitre.org/maec_bundle#malwareEntityDescription"/>
                <owl:someValuesFrom rdf:resource="http://www.w3.org/2000/01/rdf-schema#Literal"/>
            </owl:Restriction>
        </rdfs:subClassOf>
        <rdfs:subClassOf>
            <owl:Restriction>
                <owl:onProperty rdf:resource="http://maec.mitre.org/maec_bundle#malwareEntityName"/>
                <owl:someValuesFrom rdf:resource="http://www.w3.org/2000/01/rdf-schema#Literal"/>
            </owl:Restriction>
        </rdfs:subClassOf>
        <rdfs:subClassOf>
            <owl:Restriction>
                <owl:onProperty rdf:resource="http://maec.mitre.org/maec_bundle#malwareEntityType"/>
                <owl:someValuesFrom rdf:resource="http://www.w3.org/2000/01/rdf-schema#Literal"/>
            </owl:Restriction>
        </rdfs:subClassOf>
        <rdfs:comment>Characterizes a Malware Entity that an indicator or signature is written against, whether it is a particular malware instance, family, etc.</rdfs:comment>
        <rdfs:isDefinedBy rdf:resource="http://maec.mitre.org/maec_bundle"/>
        <rdfs:label>Malware Entity</rdfs:label>
    </owl:Class>
    


    <!-- http://maec.mitre.org/maec_bundle#ObjectCollection -->

    <owl:Class rdf:about="http://maec.mitre.org/maec_bundle#ObjectCollection">
        <rdfs:subClassOf rdf:resource="http://maec.mitre.org/maec_common#BaseCollection"/>
        <rdfs:comment>Ccharacterizes collections of Objects. 

For instance, it can be used to group all of the Objects that are associated with a specific behavior.</rdfs:comment>
        <rdfs:isDefinedBy rdf:resource="http://maec.mitre.org/maec_bundle"/>
        <rdfs:label>Object Collection</rdfs:label>
    </owl:Class>
    


    <!-- http://maec.mitre.org/maec_bundle#ProcessTreeNode -->

    <owl:Class rdf:about="http://maec.mitre.org/maec_bundle#ProcessTreeNode">
        <rdfs:subClassOf rdf:resource="http://cybox.mitre.org/objects/Process#Process"/>
        <rdfs:subClassOf>
            <owl:Restriction>
                <owl:onProperty rdf:resource="http://maec.mitre.org/maec_bundle#parentAction"/>
                <owl:someValuesFrom rdf:resource="http://www.w3.org/2002/07/owl#Thing"/>
            </owl:Restriction>
        </rdfs:subClassOf>
        <rdfs:subClassOf>
            <owl:Restriction>
                <owl:onProperty rdf:resource="http://maec.mitre.org/maec_bundle#processOrdinalPosition"/>
                <owl:someValuesFrom rdf:resource="http://www.w3.org/2000/01/rdf-schema#Literal"/>
            </owl:Restriction>
        </rdfs:subClassOf>
        <rdfs:comment>Characterizes a single process, or node, in the process tree.</rdfs:comment>
        <rdfs:isDefinedBy rdf:resource="http://maec.mitre.org/maec_bundle"/>
        <rdfs:label>Process tree node</rdfs:label>
    </owl:Class>
    


    <!-- http://maec.mitre.org/maec_bundle#StrategicCapabilityObjective -->

    <owl:Class rdf:about="http://maec.mitre.org/maec_bundle#StrategicCapabilityObjective">
        <rdfs:subClassOf rdf:resource="http://maec.mitre.org/maec_bundle#CapabilityObjective"/>
        <rdfs:comment>Characterizes details of a Capability&apos;s Strategic Objective.</rdfs:comment>
        <rdfs:isDefinedBy rdf:resource="http://maec.mitre.org/maec_bundle"/>
        <rdfs:label>Strategic Capability Objective</rdfs:label>
    </owl:Class>
    


    <!-- http://maec.mitre.org/maec_bundle#TacticalCapabilityObjective -->

    <owl:Class rdf:about="http://maec.mitre.org/maec_bundle#TacticalCapabilityObjective">
        <rdfs:subClassOf rdf:resource="http://maec.mitre.org/maec_bundle#CapabilityObjective"/>
        <rdfs:subClassOf>
            <owl:Restriction>
                <owl:onProperty rdf:resource="http://maec.mitre.org/maec_bundle#tacticalObjectiveName"/>
                <owl:someValuesFrom rdf:resource="http://www.w3.org/2000/01/rdf-schema#Literal"/>
            </owl:Restriction>
        </rdfs:subClassOf>
        <rdfs:comment>Characterizes details of a Capability&apos;s Tactical Objective.</rdfs:comment>
        <rdfs:isDefinedBy rdf:resource="http://maec.mitre.org/maec_bundle"/>
        <rdfs:label>Tactical Capability Objective</rdfs:label>
    </owl:Class>
    


    <!-- http://maec.mitre.org/maec_common#ActionEquivalence -->

    <owl:Class rdf:about="http://maec.mitre.org/maec_common#ActionEquivalence"/>
    


    <!-- http://maec.mitre.org/maec_common#BaseCollection -->

    <owl:Class rdf:about="http://maec.mitre.org/maec_common#BaseCollection"/>
    


    <!-- http://maec.mitre.org/maec_common#MalwareAction -->

    <owl:Class rdf:about="http://maec.mitre.org/maec_common#MalwareAction"/>
    


    <!-- http://maec.mitre.org/maec_common#ToolInformation -->

    <owl:Class rdf:about="http://maec.mitre.org/maec_common#ToolInformation"/>
    


    <!-- http://nvd.nist.gov/cve#Vulnerability -->

    <owl:Class rdf:about="http://nvd.nist.gov/cve#Vulnerability"/>
    


    <!-- http://www.w3.org/1999/02/22-rdf-syntax-ns#Statement -->

    <owl:Class rdf:about="http://www.w3.org/1999/02/22-rdf-syntax-ns#Statement"/>
</rdf:RDF>



<!-- Generated by the OWL API (version 4.2.6.20160910-2108) https://github.com/owlcs/owlapi -->

