<?xml version="1.0"?>
<rdf:RDF
    xmlns:rdf="http://www.w3.org/1999/02/22-rdf-syntax-ns#"
    xmlns:owl="http://www.w3.org/2002/07/owl#"
    xmlns:xsd="http://www.w3.org/2001/XMLSchema#"
    
    xmlns:oa="http://www.w3.org/ns/oa#"
    xmlns:rdfs="http://www.w3.org/2000/01/rdf-schema#"
    xmlns:cnt="http://www.w3.org/2011/content#"
  xml:base="http://www.w3.org/ns/oa">
  <owl:Ontology rdf:about="http://www.w3.org/ns/oa">
    
    <owl:imports rdf:resource="http://www.w3.org/2004/02/skos/core"/>
    <owl:versionInfo rdf:datatype="http://www.w3.org/2001/XMLSchema#string"
    >owl:Ontology added by TopBraid</owl:versionInfo>
    <owl:imports rdf:resource="http://www.w3.org/2011/content"/>
  </owl:Ontology>
  <owl:Class rdf:ID="TextPositionSelector">
    
    <rdfs:subClassOf>
      <owl:Restriction>
        <owl:cardinality rdf:datatype="http://www.w3.org/2001/XMLSchema#nonNegativeInteger"
        >1</owl:cardinality>
        <owl:onProperty>
          <owl:DatatypeProperty rdf:ID="end"/>
        </owl:onProperty>
      </owl:Restriction>
    </rdfs:subClassOf>
    <rdfs:subClassOf>
      <owl:Restriction>
        <owl:cardinality rdf:datatype="http://www.w3.org/2001/XMLSchema#nonNegativeInteger"
        >1</owl:cardinality>
        <owl:onProperty>
          <owl:DatatypeProperty rdf:ID="start"/>
        </owl:onProperty>
      </owl:Restriction>
    </rdfs:subClassOf>
    <rdfs:comment >Characterizes a Selector which describes a range of text based on its start and end positions.</rdfs:comment>
    <rdfs:label >Text Position Selector</rdfs:label>
    <rdfs:isDefinedBy rdf:resource=""/>
    <rdfs:subClassOf>
      <owl:Class rdf:ID="Selector"/>
    </rdfs:subClassOf>
  </owl:Class>
  <owl:Class rdf:ID="RdfTripleSelector">
    
    <rdfs:comment rdf:datatype="http://www.w3.org/2001/XMLSchema#string"
    >SELECT ?anno WHERE { ?anno oa:hasTarget ?spt . ?spt a oa:SpecificResource .
            ?spt oa:hasSelector ?data . ?data a oa:RdfTripleSelector . 
            ?spt oa:hasSource &lt;http://www.daedafusion.com/object-12345&gt; .
            ?data oa:hasPredicate &lt;http://stix.mitre.org/title&gt;  }</rdfs:comment>
    <rdfs:subClassOf>
      <owl:Restriction>
        <owl:cardinality rdf:datatype="http://www.w3.org/2001/XMLSchema#nonNegativeInteger"
        >1</owl:cardinality>
        <owl:onProperty>
          <owl:DatatypeProperty rdf:ID="predicate"/>
        </owl:onProperty>
      </owl:Restriction>
    </rdfs:subClassOf>
    <rdfs:label >RDF Triple Selector</rdfs:label>
    <rdfs:isDefinedBy rdf:resource=""/>
    <rdfs:comment >Characterizes a Selector that describes the value of the object of an RDF Triple based on its corresponding predicate. {</rdfs:comment>
    <rdfs:subClassOf>
      <owl:Class rdf:about="#Selector"/>
    </rdfs:subClassOf>
  </owl:Class>
  <owl:Class rdf:ID="Moderation">
    
    <rdfs:comment >Characterizes the body of an annotation that represents an assignment of value or quality to the target resource(s)</rdfs:comment>
    <rdfs:label >Moderation</rdfs:label>
    <rdfs:isDefinedBy rdf:resource=""/>
    <rdfs:subClassOf>
      <owl:Class rdf:ID="Body"/>
    </rdfs:subClassOf>
  </owl:Class>
  <owl:Class rdf:ID="Question">
    
    <rdfs:comment >Characterizes the body of an annotation that represents a question about the target resource(s)</rdfs:comment>
    <rdfs:label >Question</rdfs:label>
    <rdfs:isDefinedBy rdf:resource=""/>
    <rdfs:subClassOf>
      <owl:Class rdf:about="#Body"/>
    </rdfs:subClassOf>
    <rdfs:subClassOf rdf:resource="http://www.w3.org/2011/content#ContentAsText"/>
    <rdfs:subClassOf>
      <owl:Restriction>
        <owl:onProperty rdf:resource="http://www.w3.org/2011/content#chars"/>
        <owl:cardinality rdf:datatype="http://www.w3.org/2001/XMLSchema#nonNegativeInteger"
        >1</owl:cardinality>
      </owl:Restriction>
    </rdfs:subClassOf>
    <rdfs:subClassOf>
      <owl:Restriction>
        <owl:onProperty rdf:resource="http://www.w3.org/2011/content#characterEncoding"/>
        <owl:maxCardinality rdf:datatype="http://www.w3.org/2001/XMLSchema#nonNegativeInteger"
        >1</owl:maxCardinality>
      </owl:Restriction>
    </rdfs:subClassOf>
  </owl:Class>
  <owl:Class rdf:ID="SpecificResource">
    
    <rdfs:subClassOf>
      <owl:Restriction>
        <owl:maxCardinality rdf:datatype="http://www.w3.org/2001/XMLSchema#nonNegativeInteger"
        >1</owl:maxCardinality>
        <owl:onProperty>
          <owl:ObjectProperty rdf:ID="hasState"/>
        </owl:onProperty>
      </owl:Restriction>
    </rdfs:subClassOf>
    <rdfs:comment >Characterizes a Specific Resource that is used to identify the resource, typically a segment, described by the Specifiers.</rdfs:comment>
    <rdfs:subClassOf>
      <owl:Restriction>
        <owl:cardinality rdf:datatype="http://www.w3.org/2001/XMLSchema#nonNegativeInteger"
        >1</owl:cardinality>
        <owl:onProperty>
          <owl:ObjectProperty rdf:ID="hasSource"/>
        </owl:onProperty>
      </owl:Restriction>
    </rdfs:subClassOf>
    <rdfs:label >Specific Resource</rdfs:label>
    <rdfs:isDefinedBy rdf:resource=""/>
    <rdfs:subClassOf>
      <owl:Restriction>
        <owl:maxCardinality rdf:datatype="http://www.w3.org/2001/XMLSchema#nonNegativeInteger"
        >1</owl:maxCardinality>
        <owl:onProperty>
          <owl:ObjectProperty rdf:ID="hasSelector"/>
        </owl:onProperty>
      </owl:Restriction>
    </rdfs:subClassOf>
    <rdfs:subClassOf rdf:resource="http://www.w3.org/2002/07/owl#Thing"/>
  </owl:Class>
  <owl:Class rdf:ID="DataPositionSelector">
    
    <rdfs:subClassOf>
      <owl:Restriction>
        <owl:cardinality rdf:datatype="http://www.w3.org/2001/XMLSchema#nonNegativeInteger"
        >1</owl:cardinality>
        <owl:onProperty>
          <owl:DatatypeProperty rdf:about="#end"/>
        </owl:onProperty>
      </owl:Restriction>
    </rdfs:subClassOf>
    <rdfs:subClassOf>
      <owl:Restriction>
        <owl:cardinality rdf:datatype="http://www.w3.org/2001/XMLSchema#nonNegativeInteger"
        >1</owl:cardinality>
        <owl:onProperty>
          <owl:DatatypeProperty rdf:about="#start"/>
        </owl:onProperty>
      </owl:Restriction>
    </rdfs:subClassOf>
    <rdfs:isDefinedBy rdf:resource=""/>
    <rdfs:label >Data position selector</rdfs:label>
    <rdfs:comment >Characterizes a Selector which describes a range of data based on its start and end positions within the byte stream.</rdfs:comment>
    <rdfs:subClassOf>
      <owl:Class rdf:about="#Selector"/>
    </rdfs:subClassOf>
  </owl:Class>
  <owl:Class rdf:ID="TimeState">
    
    <rdfs:subClassOf>
      <owl:Restriction>
        <owl:minCardinality rdf:datatype="http://www.w3.org/2001/XMLSchema#nonNegativeInteger"
        >1</owl:minCardinality>
        <owl:onProperty>
          <owl:DatatypeProperty rdf:ID="when"/>
        </owl:onProperty>
      </owl:Restriction>
    </rdfs:subClassOf>
    <rdfs:subClassOf>
      <owl:Restriction>
        <owl:cardinality rdf:datatype="http://www.w3.org/2001/XMLSchema#nonNegativeInteger"
        >1</owl:cardinality>
        <owl:onProperty>
          <owl:DatatypeProperty rdf:about="#when"/>
        </owl:onProperty>
      </owl:Restriction>
    </rdfs:subClassOf>
    <rdfs:isDefinedBy rdf:resource=""/>
    <rdfs:label >Time state</rdfs:label>
    <rdfs:comment >Characterizes resource which describes how to retrieve a representation of the Source resource that is temporally appropriate for the Annotation.</rdfs:comment>
    <rdfs:subClassOf>
      <owl:Class rdf:ID="State"/>
    </rdfs:subClassOf>
  </owl:Class>
  <owl:Class rdf:ID="HttpRequestState">
    
    <rdfs:subClassOf>
      <owl:Restriction>
        <owl:cardinality rdf:datatype="http://www.w3.org/2001/XMLSchema#nonNegativeInteger"
        >1</owl:cardinality>
        <owl:onProperty>
          <owl:DatatypeProperty rdf:ID="value"/>
        </owl:onProperty>
      </owl:Restriction>
    </rdfs:subClassOf>
    <rdfs:comment >Specifies a resource which describes how to retrieve an appropriate representation of the Source resource for the Annotation, based on the HTTP Request headers to send to the server.</rdfs:comment>
    <rdfs:isDefinedBy rdf:resource=""/>
    <rdfs:label >Http request state</rdfs:label>
    <rdfs:subClassOf>
      <owl:Class rdf:about="#State"/>
    </rdfs:subClassOf>
  </owl:Class>
  <owl:Class rdf:ID="Comment">
    <rdfs:subClassOf>
      <owl:Restriction>
        <owl:onProperty rdf:resource="http://www.w3.org/2011/content#chars"/>
        <owl:cardinality rdf:datatype="http://www.w3.org/2001/XMLSchema#nonNegativeInteger"
        >1</owl:cardinality>
      </owl:Restriction>
    </rdfs:subClassOf>
    <rdfs:comment >Characterizes the body of an annotation that represents a commentary about or review of the target resource(s).</rdfs:comment>
    <rdfs:label >Comment</rdfs:label>
    
    <rdfs:subClassOf>
      <owl:Class rdf:about="#Body"/>
    </rdfs:subClassOf>
    <rdfs:subClassOf>
      <owl:Restriction>
        <owl:onProperty rdf:resource="http://www.w3.org/2011/content#characterEncoding"/>
        <owl:maxCardinality rdf:datatype="http://www.w3.org/2001/XMLSchema#nonNegativeInteger"
        >1</owl:maxCardinality>
      </owl:Restriction>
    </rdfs:subClassOf>
    <rdfs:subClassOf rdf:resource="http://www.w3.org/2011/content#ContentAsText"/>
    <rdfs:isDefinedBy rdf:resource=""/>
    <rdfs:subClassOf>
      <owl:Restriction>
        <owl:onProperty rdf:resource="http://www.w3.org/2011/content#characterEncoding"/>
        <owl:maxCardinality rdf:datatype="http://www.w3.org/2001/XMLSchema#nonNegativeInteger"
        >1</owl:maxCardinality>
      </owl:Restriction>
    </rdfs:subClassOf>
  </owl:Class>
  <owl:Class rdf:about="#Body">
    
    <rdfs:comment >Characterizes the body of an annotation</rdfs:comment>
    <rdfs:isDefinedBy rdf:resource=""/>
    <rdfs:label >Body</rdfs:label>
    <rdfs:subClassOf rdf:resource="http://www.w3.org/2002/07/owl#Thing"/>
  </owl:Class>
  <owl:Class rdf:ID="Change">
    
    <rdfs:comment >Characterizes the body of an annotation that represents a request for a modification or edit to the target resource.

An instance of Change is MUST be used with the editing motivation.</rdfs:comment>
    <rdfs:isDefinedBy rdf:resource=""/>
    <rdfs:label >Change</rdfs:label>
    <rdfs:subClassOf rdf:resource="#Body"/>
    <rdfs:subClassOf>
      <owl:Restriction>
        <owl:onProperty>
          <owl:DatatypeProperty rdf:ID="changeType"/>
        </owl:onProperty>
        <owl:cardinality rdf:datatype="http://www.w3.org/2001/XMLSchema#nonNegativeInteger"
        >1</owl:cardinality>
      </owl:Restriction>
    </rdfs:subClassOf>
    <rdfs:subClassOf>
      <owl:Restriction>
        <owl:onProperty>
          <owl:ObjectProperty rdf:ID="reference"/>
        </owl:onProperty>
        <owl:maxCardinality rdf:datatype="http://www.w3.org/2001/XMLSchema#nonNegativeInteger"
        >1</owl:maxCardinality>
      </owl:Restriction>
    </rdfs:subClassOf>
    <rdfs:subClassOf>
      <owl:Restriction>
        <owl:onProperty>
          <owl:DatatypeProperty rdf:about="#value"/>
        </owl:onProperty>
        <owl:maxCardinality rdf:datatype="http://www.w3.org/2001/XMLSchema#nonNegativeInteger"
        >1</owl:maxCardinality>
      </owl:Restriction>
    </rdfs:subClassOf>
  </owl:Class>
  <owl:Class rdf:ID="Link">
    
    <rdfs:comment >Characterizes the body of an annotation that represents a link (of unspecified semantics) between the body and target resources</rdfs:comment>
    <rdfs:label >Link</rdfs:label>
    <rdfs:isDefinedBy rdf:resource=""/>
    <rdfs:subClassOf rdf:resource="#Body"/>
    <rdfs:subClassOf>
      <owl:Restriction>
        <owl:onProperty>
          <owl:DatatypeProperty rdf:ID="link"/>
        </owl:onProperty>
        <owl:cardinality rdf:datatype="http://www.w3.org/2001/XMLSchema#nonNegativeInteger"
        >1</owl:cardinality>
      </owl:Restriction>
    </rdfs:subClassOf>
  </owl:Class>
  <owl:Class rdf:ID="CssStyle">
    
    <rdfs:label >CSS style</rdfs:label>
    <rdfs:isDefinedBy rdf:resource=""/>
    <rdfs:comment >Characterizes a resource which describes styles for resources participating in the Annotation using CSS.</rdfs:comment>
    <rdfs:subClassOf>
      <owl:Class rdf:ID="Style"/>
    </rdfs:subClassOf>
  </owl:Class>
  <owl:Class rdf:about="#Style">
    
    <rdfs:comment >Characerizes a resource which describes the style in which the selection or resource should be rendered.</rdfs:comment>
    <rdfs:label >Style</rdfs:label>
    <rdfs:isDefinedBy rdf:resource=""/>
    <rdfs:subClassOf rdf:resource="http://www.w3.org/2002/07/owl#Thing"/>
  </owl:Class>
  <owl:Class rdf:ID="Annotation">
    
    <rdfs:subClassOf>
      <owl:Restriction>
        <owl:onProperty>
          <owl:ObjectProperty rdf:ID="motivatedBy"/>
        </owl:onProperty>
        <owl:minCardinality rdf:datatype="http://www.w3.org/2001/XMLSchema#nonNegativeInteger"
        >1</owl:minCardinality>
      </owl:Restriction>
    </rdfs:subClassOf>
    <rdfs:subClassOf>
      <owl:Restriction>
        <owl:minCardinality rdf:datatype="http://www.w3.org/2001/XMLSchema#nonNegativeInteger"
        >1</owl:minCardinality>
        <owl:onProperty>
          <owl:ObjectProperty rdf:ID="hasTarget"/>
        </owl:onProperty>
      </owl:Restriction>
    </rdfs:subClassOf>
    <rdfs:isDefinedBy rdf:resource=""/>
    <rdfs:subClassOf rdf:resource="http://www.w3.org/2002/07/owl#Thing"/>
    <rdfs:label >Annotation</rdfs:label>
    <rdfs:subClassOf>
      <owl:Restriction>
        <owl:cardinality rdf:datatype="http://www.w3.org/2001/XMLSchema#nonNegativeInteger"
        >1</owl:cardinality>
        <owl:onProperty>
          <owl:DatatypeProperty rdf:ID="annotatedAt"/>
        </owl:onProperty>
      </owl:Restriction>
    </rdfs:subClassOf>
    <rdfs:comment >Characterizes an annotation.

An annotation is considered to be a set of connected resources, typically including a body and target, and conveys that the body is related to the target. The exact nature of this relationship changes according to the intention of the annotation, but most frequently conveys that the body is somehow "about" the target. Other possible relationships include that the body is an identifier for the target, provides a representation of the target, or classifies the target in some way.</rdfs:comment>
    <rdfs:subClassOf>
      <owl:Restriction>
        <owl:maxCardinality rdf:datatype="http://www.w3.org/2001/XMLSchema#nonNegativeInteger"
        >1</owl:maxCardinality>
        <owl:onProperty>
          <owl:ObjectProperty rdf:ID="styledBy"/>
        </owl:onProperty>
      </owl:Restriction>
    </rdfs:subClassOf>
  </owl:Class>
  <owl:Class rdf:ID="Note">
    
    <rdfs:comment >Characterizes the body of an annotation that represents a description of the target resource(s), as opposed to a Comment about them.</rdfs:comment>
    <rdfs:label >Note</rdfs:label>
    <rdfs:isDefinedBy rdf:resource=""/>
    <rdfs:subClassOf rdf:resource="#Body"/>
    <rdfs:subClassOf rdf:resource="http://www.w3.org/2011/content#ContentAsText"/>
    <rdfs:subClassOf>
      <owl:Restriction>
        <owl:onProperty rdf:resource="http://www.w3.org/2011/content#chars"/>
        <owl:cardinality rdf:datatype="http://www.w3.org/2001/XMLSchema#nonNegativeInteger"
        >1</owl:cardinality>
      </owl:Restriction>
    </rdfs:subClassOf>
    <rdfs:subClassOf>
      <owl:Restriction>
        <owl:onProperty rdf:resource="http://www.w3.org/2011/content#characterEncoding"/>
        <owl:maxCardinality rdf:datatype="http://www.w3.org/2001/XMLSchema#nonNegativeInteger"
        >1</owl:maxCardinality>
      </owl:Restriction>
    </rdfs:subClassOf>
  </owl:Class>
  <owl:Class rdf:ID="Motivation">
    <rdfs:comment >Characterizes a reason for the annotation creation, and might include things like Replying to another annotation, Commenting on a resource, or Linking to a related resource.</rdfs:comment>
    <rdfs:subClassOf rdf:resource="http://www.w3.org/2004/02/skos/core#Concept"/>
    <rdfs:isDefinedBy rdf:resource=""/>
    <rdfs:label >Motivation</rdfs:label>
  </owl:Class>
  <owl:Class rdf:ID="Tag">
    
    <rdfs:subClassOf rdf:resource="http://www.w3.org/2011/content#ContentAsText"/>
    <rdfs:comment >Characterizes the body of an annotation that contains a tag on the target resource(s).</rdfs:comment>
    <rdfs:label >Tag</rdfs:label>
    <rdfs:isDefinedBy rdf:resource=""/>
    <rdfs:subClassOf rdf:resource="#Body"/>
    <rdfs:subClassOf>
      <owl:Restriction>
        <owl:onProperty rdf:resource="http://www.w3.org/2011/content#characterEncoding"/>
        <owl:maxCardinality rdf:datatype="http://www.w3.org/2001/XMLSchema#nonNegativeInteger"
        >1</owl:maxCardinality>
      </owl:Restriction>
    </rdfs:subClassOf>
  </owl:Class>
  <owl:Class rdf:about="#Selector">
    
    <rdfs:comment >Characterizes a Selector which is a Specifier that describes how to determine the segment of interest from within the retrieved representation of the Source resource. The nature of the Selector will be dependent on the type of the representation for which the segment is conveyed. 

For example the methods used to describe a section of an image will be very different to the methods used to discover the correct paragraph of text, or the correct slice of a dataset.</rdfs:comment>
    <rdfs:label >Selector</rdfs:label>
    <rdfs:isDefinedBy rdf:resource=""/>
    <rdfs:subClassOf rdf:resource="http://www.w3.org/2002/07/owl#Thing"/>
  </owl:Class>
  <owl:Class rdf:ID="TextQuoteSelector">
    
    <rdfs:subClassOf>
      <owl:Restriction>
        <owl:maxCardinality rdf:datatype="http://www.w3.org/2001/XMLSchema#nonNegativeInteger"
        >1</owl:maxCardinality>
        <owl:onProperty>
          <owl:DatatypeProperty rdf:ID="suffix"/>
        </owl:onProperty>
      </owl:Restriction>
    </rdfs:subClassOf>
    <rdfs:subClassOf>
      <owl:Restriction>
        <owl:maxCardinality rdf:datatype="http://www.w3.org/2001/XMLSchema#nonNegativeInteger"
        >1</owl:maxCardinality>
        <owl:onProperty>
          <owl:DatatypeProperty rdf:ID="prefix"/>
        </owl:onProperty>
      </owl:Restriction>
    </rdfs:subClassOf>
    <rdfs:subClassOf>
      <owl:Restriction>
        <owl:cardinality rdf:datatype="http://www.w3.org/2001/XMLSchema#nonNegativeInteger"
        >1</owl:cardinality>
        <owl:onProperty>
          <owl:DatatypeProperty rdf:ID="extract"/>
        </owl:onProperty>
      </owl:Restriction>
    </rdfs:subClassOf>
    <rdfs:isDefinedBy rdf:resource=""/>
    <rdfs:label >Text quote selector</rdfs:label>
    <rdfs:comment >Characterizes a Selector that describes a textual segment by means of quoting it, plus passages before or after it.</rdfs:comment>
    <rdfs:subClassOf rdf:resource="#Selector"/>
  </owl:Class>
  <owl:Class rdf:ID="Reply">
    
    <rdfs:comment >Characterizes the body of an annotation that represents a reply to a previous statement, either an Annotation or another resource.</rdfs:comment>
    <rdfs:subClassOf rdf:resource="http://www.w3.org/2011/content#ContentAsText"/>
    <rdfs:isDefinedBy rdf:resource=""/>
    <rdfs:label >Reply</rdfs:label>
    <rdfs:subClassOf rdf:resource="#Body"/>
    <rdfs:subClassOf>
      <owl:Restriction>
        <owl:onProperty rdf:resource="http://www.w3.org/2011/content#characterEncoding"/>
        <owl:maxCardinality rdf:datatype="http://www.w3.org/2001/XMLSchema#nonNegativeInteger"
        >1</owl:maxCardinality>
      </owl:Restriction>
    </rdfs:subClassOf>
    <rdfs:subClassOf>
      <owl:Restriction>
        <owl:onProperty rdf:resource="http://www.w3.org/2011/content#chars"/>
        <owl:cardinality rdf:datatype="http://www.w3.org/2001/XMLSchema#nonNegativeInteger"
        >1</owl:cardinality>
      </owl:Restriction>
    </rdfs:subClassOf>
  </owl:Class>
  <owl:Class rdf:ID="FragmentSelector">
    
    <rdfs:subClassOf>
      <owl:Restriction>
        <owl:cardinality rdf:datatype="http://www.w3.org/2001/XMLSchema#nonNegativeInteger"
        >1</owl:cardinality>
        <owl:onProperty>
          <owl:DatatypeProperty rdf:about="#value"/>
        </owl:onProperty>
      </owl:Restriction>
    </rdfs:subClassOf>
    <rdfs:comment >Characterizes a Fragment Selectors that describes the segment of interest in a representation, through the use of the fragment identifier component of a URI.</rdfs:comment>
    <rdfs:isDefinedBy rdf:resource=""/>
    <rdfs:label >Fragment selector</rdfs:label>
    <rdfs:subClassOf rdf:resource="#Selector"/>
  </owl:Class>
  <owl:Class rdf:ID="SvgSelector">
    
    <rdfs:isDefinedBy rdf:resource=""/>
    <rdfs:label >Svg selector</rdfs:label>
    <rdfs:comment >Characterizes a Selector which defines a shape using the SVG standard.</rdfs:comment>
    <rdfs:subClassOf rdf:resource="#Selector"/>
  </owl:Class>
  <owl:Class rdf:ID="Classification">
    
    <rdfs:comment >Characterizes the body of an annotation that represents the assignment of a classification type, typically from a controlled vocabulary, to the target resource(s).</rdfs:comment>
    <rdfs:isDefinedBy rdf:resource=""/>
    <rdfs:label >Classification</rdfs:label>
    <rdfs:subClassOf rdf:resource="#Body"/>
  </owl:Class>
  <owl:Class rdf:ID="SemanticTag">
    
    <rdfs:comment >Characterizes the body of an annotation when it is a semantic tagging resource; a URI that identifies a concept, rather than an embedded string, frequently a term from a controlled vocabulary</rdfs:comment>
    <rdfs:isDefinedBy rdf:resource=""/>
    <rdfs:label >Semantic Tag</rdfs:label>
    <rdfs:subClassOf rdf:resource="#Tag"/>
    <rdfs:subClassOf>
      <owl:Restriction>
        <owl:onProperty>
          <owl:DatatypeProperty rdf:ID="semanticLink"/>
        </owl:onProperty>
        <owl:cardinality rdf:datatype="http://www.w3.org/2001/XMLSchema#nonNegativeInteger"
        >1</owl:cardinality>
      </owl:Restriction>
    </rdfs:subClassOf>
  </owl:Class>
  <owl:Class rdf:about="#State">
    
    <rdfs:comment >Characterizes a resource which describes how to retrieve a representation of the Source resource that is appropriate for the Annotation.</rdfs:comment>
    <rdfs:label >State</rdfs:label>
    <rdfs:isDefinedBy rdf:resource=""/>
    <rdfs:subClassOf rdf:resource="http://www.w3.org/2002/07/owl#Thing"/>
  </owl:Class>
  <owl:ObjectProperty rdf:about="#hasTarget">
    <rdfs:comment >Specifies the relationship between an Annotation and the Target of the Annotation</rdfs:comment>
    <rdfs:isDefinedBy rdf:resource=""/>
    <rdfs:label >Has Target</rdfs:label>
    <rdfs:domain rdf:resource="#Annotation"/>
    <rdfs:range rdf:resource="http://www.w3.org/2002/07/owl#Thing"/>
  </owl:ObjectProperty>
  <owl:ObjectProperty rdf:about="#hasState">
    <rdfs:comment >Specifies the relationship between a Specific Resource and it's State resource.</rdfs:comment>
    <rdfs:label >Has State</rdfs:label>
    <rdfs:isDefinedBy rdf:resource=""/>
    <rdfs:range rdf:resource="#State"/>
    <rdfs:domain rdf:resource="#SpecificResource"/>
  </owl:ObjectProperty>
  <owl:ObjectProperty rdf:ID="cachedSource">
    <rdfs:comment >Specifies a link to a copy of the Source resource's representation, appropriate for the Annotation.</rdfs:comment>
    <rdfs:isDefinedBy rdf:resource=""/>
    <rdfs:label >Cached Source</rdfs:label>
    <rdfs:domain rdf:resource="#TimeState"/>
  </owl:ObjectProperty>
  <owl:ObjectProperty rdf:about="#motivatedBy">
    <rdfs:domain rdf:resource="#Annotation"/>
    <rdfs:isDefinedBy rdf:resource=""/>
    <rdfs:range rdf:resource="#Motivation"/>
    <rdfs:label >Motivated By</rdfs:label>
    <rdfs:comment >Specifies the motivation behind which the annotation was made.</rdfs:comment>
  </owl:ObjectProperty>
  <owl:ObjectProperty rdf:ID="hasScope">
    <rdfs:label >Has Scope</rdfs:label>
    <rdfs:isDefinedBy rdf:resource=""/>
    <rdfs:domain rdf:resource="#SpecificResource"/>
    <rdfs:comment >Specifies the relationship between a Specific Resource and the resource that provides the scope or context for it in this Annotation.</rdfs:comment>
  </owl:ObjectProperty>
  <owl:ObjectProperty rdf:about="#hasSource">
    <rdfs:domain rdf:resource="#SpecificResource"/>
    <rdfs:label >has source</rdfs:label>
    <rdfs:comment ></rdfs:comment>
    <rdfs:isDefinedBy rdf:datatype="http://www.w3.org/2001/XMLSchema#string"
    >&lt;http://www.w3.org/ns/oa&gt;</rdfs:isDefinedBy>
  </owl:ObjectProperty>
  <owl:ObjectProperty rdf:ID="hasBody">
    <rdfs:label >Has Body</rdfs:label>
    <rdfs:domain rdf:resource="#Annotation"/>
    <rdfs:isDefinedBy rdf:resource=""/>
    <rdfs:range rdf:resource="#Body"/>
    <rdfs:comment >Specifies the relationship between an Annotation and the Body of the Annotation</rdfs:comment>
  </owl:ObjectProperty>
  <owl:ObjectProperty rdf:about="#hasSelector">
    <rdfs:domain rdf:resource="#SpecificResource"/>
    <rdfs:comment >Specifies a relationship between a Specific Resource and a Selector.</rdfs:comment>
    <rdfs:label >Has Selector</rdfs:label>
    <rdfs:range rdf:resource="#Selector"/>
    <rdfs:isDefinedBy rdf:resource=""/>
  </owl:ObjectProperty>
  <owl:ObjectProperty rdf:about="#reference">
    <rdfs:domain rdf:resource="#Change"/>
    <rdfs:label >Reference</rdfs:label>
    <rdfs:isDefinedBy rdf:resource=""/>
    <rdfs:comment >Specifies a reference to new target</rdfs:comment>
    <rdfs:range rdf:resource="http://www.w3.org/2002/07/owl#Thing"/>
  </owl:ObjectProperty>
  <owl:ObjectProperty rdf:about="#styledBy">
    <rdfs:range rdf:resource="#Style"/>
    <rdfs:comment >Specifies the elationship between an Annotation and the Style.</rdfs:comment>
    <rdfs:isDefinedBy rdf:resource=""/>
    <rdfs:label >Styled By</rdfs:label>
    <rdfs:domain rdf:resource="#Annotation"/>
  </owl:ObjectProperty>
  <owl:DatatypeProperty rdf:about="#changeType">
    <rdfs:domain rdf:resource="#Change"/>
    <rdfs:label >Change Type</rdfs:label>
    <rdfs:isDefinedBy rdf:resource=""/>
    <rdfs:comment >Specifies the type of the editing change</rdfs:comment>
    <rdfs:range>
      <rdfs:Datatype>
        <owl:oneOf rdf:parseType="Resource">
          <rdf:first rdf:datatype="http://www.w3.org/2001/XMLSchema#string"
          >Add_Value</rdf:first>
          <rdf:rest rdf:parseType="Resource">
            <rdf:first rdf:datatype="http://www.w3.org/2001/XMLSchema#string"
            >Add_Reference</rdf:first>
            <rdf:rest rdf:parseType="Resource">
              <rdf:first rdf:datatype="http://www.w3.org/2001/XMLSchema#string"
              >Replace_Value</rdf:first>
              <rdf:rest rdf:parseType="Resource">
                <rdf:first rdf:datatype="http://www.w3.org/2001/XMLSchema#string"
                >Replace_Reference</rdf:first>
                <rdf:rest rdf:parseType="Resource">
                  <rdf:first rdf:datatype="http://www.w3.org/2001/XMLSchema#string"
                  >Remove_Value</rdf:first>
                  <rdf:rest rdf:parseType="Resource">
                    <rdf:first rdf:datatype="http://www.w3.org/2001/XMLSchema#string"
                    >Remove_Reference</rdf:first>
                    <rdf:rest rdf:resource="http://www.w3.org/1999/02/22-rdf-syntax-ns#nil"/>
                  </rdf:rest>
                </rdf:rest>
              </rdf:rest>
            </rdf:rest>
          </rdf:rest>
        </owl:oneOf>
      </rdfs:Datatype>
    </rdfs:range>
  </owl:DatatypeProperty>
  <owl:DatatypeProperty rdf:about="#prefix">
    <rdfs:isDefinedBy rdf:resource=""/>
    <rdfs:range rdf:resource="http://www.w3.org/2001/XMLSchema#string"/>
    <rdfs:label >prefix</rdfs:label>
    <rdfs:domain rdf:resource="#TextQuoteSelector"/>
    <rdfs:comment >Specifies a snippet of text that occurs immediately before the text which is being selected.</rdfs:comment>
  </owl:DatatypeProperty>
  <owl:DatatypeProperty rdf:about="#extract">
    <rdfs:comment >Specifies a copy of the text which is being selected, after normalization. 

Normalization involves the removal of any markup (e.g., HTML/XML tags), character entities should be replaced with the character that they encode, unnecessary whitespace should be normalized, and so forth.</rdfs:comment>
    <rdfs:range rdf:resource="http://www.w3.org/2001/XMLSchema#string"/>
    <rdfs:isDefinedBy rdf:resource=""/>
    <rdfs:label >Extract</rdfs:label>
    <rdfs:domain rdf:resource="#TextQuoteSelector"/>
  </owl:DatatypeProperty>
  <owl:DatatypeProperty rdf:about="#semanticLink">
    <rdfs:domain rdf:resource="#SemanticTag"/>
    <rdfs:range rdf:resource="http://www.w3.org/2001/XMLSchema#anyURI"/>
    <rdfs:isDefinedBy rdf:resource=""/>
    <rdfs:label >Semantic Link</rdfs:label>
    <rdfs:comment >Specifies a URI that identifies a concept, rather than an embedded string.</rdfs:comment>
  </owl:DatatypeProperty>
  <owl:DatatypeProperty rdf:about="#link">
    <rdfs:comment >Specifies a URL that links the body of the annotation to the target</rdfs:comment>
    <rdfs:domain rdf:resource="#Link"/>
    <rdfs:isDefinedBy rdf:resource=""/>
    <rdfs:label >Link</rdfs:label>
    <rdfs:range rdf:resource="http://www.w3.org/2001/XMLSchema#anyURI"/>
  </owl:DatatypeProperty>
  <owl:DatatypeProperty rdf:about="#end">
    <rdfs:domain rdf:resource="#DataPositionSelector"/>
    <rdfs:comment >Specifies the end position of the segment of text. The last character is not included within the segment.</rdfs:comment>
    <rdfs:domain rdf:resource="#TextPositionSelector"/>
    <rdfs:range rdf:resource="http://www.w3.org/2001/XMLSchema#integer"/>
    <rdfs:isDefinedBy rdf:resource=""/>
    <rdfs:label >End</rdfs:label>
  </owl:DatatypeProperty>
  <owl:DatatypeProperty rdf:about="#value">
    <rdfs:domain rdf:resource="#HttpRequestState"/>
    <rdfs:label >Value</rdfs:label>
    <rdfs:isDefinedBy rdf:resource=""/>
    <rdfs:comment >Specifies the contents of the fragment identifier component of a URI that describes the segment of interest in the resource.</rdfs:comment>
    <rdfs:range rdf:resource="http://www.w3.org/2001/XMLSchema#string"/>
    <rdfs:domain rdf:resource="#FragmentSelector"/>
    <rdfs:domain rdf:resource="#Change"/>
  </owl:DatatypeProperty>
  <owl:DatatypeProperty rdf:about="#start">
    <rdfs:domain rdf:resource="#DataPositionSelector"/>
    <rdfs:range rdf:resource="http://www.w3.org/2001/XMLSchema#integer"/>
    <rdfs:label >Start</rdfs:label>
    <rdfs:isDefinedBy rdf:resource=""/>
    <rdfs:domain rdf:resource="#TextPositionSelector"/>
    <rdfs:comment >Specifies the starting position of the segment of text. The first character in the full text is character position 0, and the character is included within the segment.</rdfs:comment>
  </owl:DatatypeProperty>
  <owl:DatatypeProperty rdf:ID="styleClass">
    <rdfs:label >Style Class</rdfs:label>
    <rdfs:range rdf:resource="http://www.w3.org/2001/XMLSchema#string"/>
    <rdfs:isDefinedBy rdf:resource=""/>
    <rdfs:domain rdf:resource="#CssStyle"/>
    <rdfs:comment >Specifies the string name of the class used in the CSS description that should be applied to the Specific Resource.</rdfs:comment>
  </owl:DatatypeProperty>
  <owl:DatatypeProperty rdf:about="#when">
    <rdfs:isDefinedBy rdf:resource=""/>
    <rdfs:range rdf:resource="http://www.w3.org/2001/XMLSchema#dateTime"/>
    <rdfs:label >when</rdfs:label>
    <rdfs:domain rdf:resource="#TimeState"/>
    <rdfs:comment >Specifies a timestamp at which the Source resource should be interpreted for the Annotation.</rdfs:comment>
  </owl:DatatypeProperty>
  <owl:DatatypeProperty rdf:about="#predicate">
    <rdfs:domain rdf:resource="#RdfTripleSelector"/>
    <rdfs:range rdf:resource="http://www.w3.org/2001/XMLSchema#string"/>
    <rdfs:label >predicate</rdfs:label>
    <rdfs:comment ></rdfs:comment>
    <rdfs:isDefinedBy rdf:datatype="http://www.w3.org/2001/XMLSchema#string"
    >&lt;http://www.w3.org/ns/oa&gt;</rdfs:isDefinedBy>
  </owl:DatatypeProperty>
  <owl:DatatypeProperty rdf:about="#suffix">
    <rdfs:comment >Specifies a snippet of text that occurs immediately after the text which is being selected.</rdfs:comment>
    <rdfs:range rdf:resource="http://www.w3.org/2001/XMLSchema#string"/>
    <rdfs:label >suffix</rdfs:label>
    <rdfs:isDefinedBy rdf:resource=""/>
    <rdfs:domain rdf:resource="#TextQuoteSelector"/>
  </owl:DatatypeProperty>
  <owl:DatatypeProperty rdf:about="#annotatedAt">
    <rdfs:comment >Specifies time at which the Annotation was created.</rdfs:comment>
    <rdfs:range rdf:resource="http://www.w3.org/2001/XMLSchema#dateTime"/>
    <rdfs:isDefinedBy rdf:resource=""/>
    <rdfs:label >Annotated At</rdfs:label>
    <rdfs:domain rdf:resource="#Annotation"/>
  </owl:DatatypeProperty>
  <oa:Motivation rdf:ID="questioning">
    <rdfs:comment >Represents asking a question about the target resource(s). For example to ask for assistance with a particular section of text, or question its veracity. 

An annotation with the questioning motivation MUST be associated with an instance of a Question body that contains the text of the question.</rdfs:comment>
    <rdfs:isDefinedBy rdf:resource=""/>
    <rdfs:label >Questioning</rdfs:label>
  </oa:Motivation>
  <oa:Motivation rdf:ID="moderating">
    <rdfs:comment >Represents an assignment of value or quality to the target resource(s). For example annotating an Annotation to moderate it up in a trust network or threaded discussion. 

An annotation with the moderating motivation MUST be associated with an instance of a Moderation body that describes the actual assignment of value or quality.</rdfs:comment>
    <rdfs:isDefinedBy rdf:resource=""/>
    <rdfs:label >Moderating</rdfs:label>
  </oa:Motivation>
  <oa:Motivation rdf:ID="identifying">
    <rdfs:label >Identifying</rdfs:label>
    <rdfs:isDefinedBy rdf:resource=""/>
    <rdfs:comment >Represents the assignment of an identity to the target resource(s). For example, annotating the name of a city in a string of text with the URI that identifies it.</rdfs:comment>
  </oa:Motivation>
  <oa:Motivation rdf:ID="editing">
    <rdfs:comment >Represents a request for a modification or edit to the target resource. For example, an Annotation that requests a typo to be corrected. 

An annotation with the editing motivation MUST be associated with an instance of a Change body that describes the actual change.</rdfs:comment>
    <rdfs:isDefinedBy rdf:resource=""/>
    <rdfs:label >Editing</rdfs:label>
  </oa:Motivation>
  <oa:Motivation rdf:ID="classifying">
    <rdfs:comment >Represents the assignment of a classification type, typically from a controlled vocabulary, to the target resource(s). For example to classify an Image resource as a Portrait.

An annotation with the classifying motivation MUST be associated with an instance of a Classification body that describes the classification.</rdfs:comment>
    <rdfs:isDefinedBy rdf:resource=""/>
    <rdfs:label >Classifying</rdfs:label>
  </oa:Motivation>
  <oa:Motivation rdf:ID="highlighting">
    <rdfs:comment >Represents a highlighted section of the target resource or segment. For example to draw attention to the selected text that the annotator disagrees with. 

A Highlight may or may not have a Body resource</rdfs:comment>
    <rdfs:isDefinedBy rdf:resource=""/>
    <rdfs:label >Highlighting</rdfs:label>
  </oa:Motivation>
  <oa:Motivation rdf:ID="describing">
    <rdfs:comment >Represents a description of the target resource(s), as opposed to a comment about them. For example describing the above PDF's contents, rather than commenting on their accuracy. 

An annotation with the describing motivation MUST be associated with an instance of a Note body that describes the actual description.</rdfs:comment>
    <rdfs:label >Describing</rdfs:label>
    <rdfs:isDefinedBy rdf:resource=""/>
  </oa:Motivation>
  <oa:Motivation rdf:ID="linking">
    <rdfs:comment >Represents an untyped link to a resource related to the target.

An annotation with the linking motivation MUST be associated with an instance of a Link body that describes the linkage.</rdfs:comment>
    <rdfs:isDefinedBy rdf:resource=""/>
    <rdfs:label >Linking</rdfs:label>
  </oa:Motivation>
  <oa:Motivation rdf:ID="bookmarking">
    <rdfs:comment >Represents the creation of a bookmark to the target resources or recorded point or points within one or more resources. For example, an Annotation that bookmarks the point in a text where the reader finished reading. 

Bookmark Annotations may or may not have a Body resource.</rdfs:comment>
    <rdfs:isDefinedBy rdf:resource=""/>
    <rdfs:label >Bookmarking</rdfs:label>
  </oa:Motivation>
  <oa:Motivation rdf:ID="tagging">
    <rdfs:comment >Represents adding a Tag on the target resource(s).

An annotation with the tagging motivation MUST be associated with an instance of a Tag or SemanticTag body that contains the tag or linkage to a descripion, respectitively.</rdfs:comment>
    <rdfs:isDefinedBy rdf:resource=""/>
    <rdfs:label >Tagging</rdfs:label>
  </oa:Motivation>
  <oa:Motivation rdf:ID="replying">
    <rdfs:comment >Represents a reply to a previous statement, either an Annotation or another resource. For example providing the assistance requested in the above. 

An annotation with the replying motivation MUST be associated with an instance of a Reply body that contains the text of the reply.</rdfs:comment>
    <rdfs:isDefinedBy rdf:resource=""/>
    <rdfs:label >Replying</rdfs:label>
  </oa:Motivation>
  <oa:Motivation rdf:ID="commenting">
    <rdfs:comment >Represents a commentary about or review of the target resource(s). For example to provide a commentary about a particular PDF.

An annotation with the commenting motivation MUST be associated with an instance of a Comment body that contains the actual commentary.</rdfs:comment>
    <rdfs:isDefinedBy rdf:resource=""/>
    <rdfs:label >Commenting</rdfs:label>
  </oa:Motivation>
</rdf:RDF>

<!-- Created with TopBraid -->
